Publisher: The Norwegian EPD Foundation
ENVIRONMENTAL PRODUCT DECLARATION Registration number: NEPD-42-43-MRA
In accordance with ISO 14025 and EN 15804 for:
[GTBUILD - Titanium zinc plate]
From
[Taicang Gronsedt Technology Co., Ltd.]
Declared product:
Programme operator: EPD China
Registration number: EPD-CN-00013
Issued date: 2024-10-21
Valid until: 2029-10-20
Programme operator EPD China
Registration number EPD -CN - 00013
Programme Information
EPD Owner Taicang Gronsedt Technology Co., Ltd.
No.198 Shalu Road, Shaxi Town, Taicang City
www.gronsedt.com
Info@gronsedt.com
Product Name GTBUILD - Titanium zinc plate
Production Site No.198 Shalu Road, Shaxi Town, Taicang City
Identification of product Manufacture of metal structures
Field of Application Construction material
Programme Operator EPD China
Address of Headquarter: Tianping Road, Xuhui District, Shanghai
Website: www.epdchina.cn
Email: info@epdchina.cn | secretary@epdchina.cn
LCA Practitioner Taicang Gronsedt Technology Co., Ltd.
Responsibility The EPD owner has the sole ownership, liability, and responsibility for the EPD
Comparability EPDs within same category of product in different programme operator are not suggested
to be compared. Full conformance with a PCR allows EPD comparability only when all
stages of a life cycle have been considered. However, variations and deviations are
possible even applying the same PCR.
Liability The EPD owner has the sole ownership, liability, and responsibility for the EPD.
Validity The EPD is published on 2024-10-21 and valid to 2029-10-20
LCA Software (version) SimaPro 9.6.0.1
LCI Dataset (version) Ecoinvent 3.10
Year(s) of Primary Data 01/06/2023-31/05/2024
PCR EPDCN-PCR-202204 PCR FOR CONSTRUCTION PRODUCTS AND
CONSTRUCTION SERVICES TO EN 15804 V2.0
Other Reference Document 15804:2012+A2:2019 Sustainability of construction works-Environment product
declarations-Core rules for the product category of construction products
Verification statement according EN15804
Independent verification of the declaration and data according to EN ISO 14025:2010
⧠ internal R external
Third-party institution verification: <Lihua Wen, Ti Certification (Shanghai) Co., Ltd.> is an approved certification
body accountable for third-party verification
Approved by: EPD China
Procedure for follow-up of data during EPD validity involves a third-party certification body:
R Yes £ No
EPD 中国项目 值得信赖
— 2 —
The first EPD Programme Operator registered in China, contributing to the EPD system building in China
www.epdchina.cn
Programme operator EPD China
Registration number EPD -CN - 00013
General Information
1.1 Company information
Gronsedt Technology is a private, family-owned Danish company group established in 2007. We specialize in the
design, production, and sale of stainless steel and aluminum products. Our offerings include both mass-produced
products for the construction industry through our GTBUILD division, as well as smaller series and customized
products for a variety of industries through our GTINDUSTRY division. With a presence in Europe, Asia, and the
Middle East—including our own factories, central warehouse, and distribution center in China—we supply
products to customers worldwide, either directly or via our distribution center in Denmark for European clients.
Figure 1: Picture of the company
1.2 Scope and type of EPD
The system boundary in the EPD report is from cradle to grave, including modules A1–A3, A4, A5, C1-C4 and
module D.
Table1: Process stages and and EPD modules.
CONSTRUC BENEFITSAND
PRODUCT TION LOADSBEYOND
STAGE PROCESS USE STAGE END OF LIFE STAGE THESYSTEM
STAGE BOUNDARIES
Note: X=Declared Module, ND=Module not Declared.
EPD 中国项目 值得信赖
— 3 —
The first EPD Programme Operator registered in China, contributing to the EPD system building in China
www.epdchina.cn
lairetam
waR
ylppus
tropsnarT noitcudorP morf
tropsnarT
eht
ot etag
eht
ylbmessA
esU
ecnanetniaM riapeR tnemecalpeR tnemhsibrufeR lanoitarepO esu
ygrene
lanoitarepO esu
retaw
/noitcurtsnoceD noitilomed tropsnarT etsaW gnissecorp lasopsiD -yrevocer
-esuer
-gnilcycer laitnetop
A1 A2 A3 A4 A5 B1 B2 B3 B4 B5 B6 B7 C1 C2 C3 C4 D
x x x x x ND ND ND ND ND ND ND x x x x x
Programme operator EPD China
Registration number EPD -CN - 00013
Figure 2: System boundary
2 Detailed Product Description
GTBUILD has developed modern, attractive, and easy-to-install, module-based fascia and bargeboard trim parts, as well as
complete systems. These can be used individually or in combination. The products are made of titanium zinc plate, with or
without coating, and are available in various thicknesses and dimensions.
These products ensure a maintenance-free construction for many years, making them suitable for both new builds and
renovations. The design concept involves mounting a long-lasting metal profile on top of wooden fascias, bargeboards, façade
sections, and other house constructions where water ingress or exposure is undesirable.
Additionally, these products provide protection against the ingress of mice, rats, birds, and other small animals into small spaces
within house constructions. They also serve a decorative function, enhancing the aesthetics of modern housing designs.
The following table lists the models and specifications of the GTBUILD - Titanium zinc plate product.
Table 1 Product model and specification
Model and specification
Name Thickness
Model No. Length (mm) Width (mm)
(mm)
TPZ 0.65 500-1000 70-850
GTBUILD - Titanium zinc plate TPX 0.65 500-1000 90-550
TMS 0.65 500-1000 70-850
The declared unit is: 1 kilogram of product
EPD 中国项目 值得信赖
— 4 —
The first EPD Programme Operator registered in China, contributing to the EPD system building in China
www.epdchina.cn
Programme operator EPD China
Registration number EPD -CN - 00013
Figure 3: Picture of the declared product.
Figure 4: The production process in selected stages.
Table 3: Main product components and packaging materials per unit.
Product components Weight, kg Weight-%
Titanium zinc plate 1.03 103%
TOTAL 1.03 103%
Packaging materials Weight, kg Weight-% (versus the product)
Plastic wrap 0.00205 0.205%
PET packing belt 0.000370 0.037%
Steel strap packing band 0.00123 0.123%
Pallet 0.0373 3.73%
Box 0.0410 4.10%
TOTAL 0.08195 8.195%
Dangerous substances
The products do not contain any of the substances of very high concern (SVHC) for authorisation regulated by the
Regulation (EC) No 1907/2006 (REACH) or the Regulation (EC) No 1272/2008 of European parliament.
3 LCA results according to EN 15804
3.1 Environmental Impacts
The LCA results of GTBUILD - Titanium zinc plate metal per declared unit is listed as the table.
EPD 中国项目 值得信赖
— 5 —
The first EPD Programme Operator registered in China, contributing to the EPD system building in China
www.epdchina.cn
Programme operator EPD China
Registration number EPD -CN - 00013
Table3: Environmental impacts according to EN 15804.
RESULTS OF THE LCA - ENVIRONMENTAL IMPACT per functional or declared unit
Core indicator Unit A1-A3 A4 A5 C1 C2 C3 C4 D
Global Warming Potential total (GWP-total) [kg CO2 eq.] 5.75E+00 2.26E-01 8.75E-03 0.00E+00 1.56E-02 2.13E-01 0.00E+00 -5.14E-01
Global Warming Potential fossil fuels (GWP-fossil) [kg CO2 eq.] 5.59E+00 2.26E-01 7.24E-03 0.00E+00 1.56E-02 2.06E-01 0.00E+00 -5.11E-01
Global Warming Potential biogenic (GWP-biogenic) [kg CO2 eq.] 2.69E-01 -6.48E-05 -1.23E-01 0.00E+00 9.19E-07 6.99E-03 0.00E+00 -1.23E-03
Global Warming Potential land use and land use
[kg CO2 eq.] 1.28E-02 1.16E-04 6.39E-06 0.00E+00 6.37E-06 1.71E-04 0.00E+00 -1.13E-03
change (GWP-luluc)
Depletion potential of the stratospheric ozone layer [kg CFC 11
7.32E-08 3.24E-09 6.58E-11 0.00E+00 2.27E-10 1.61E-09 0.00E+00 -9.14E-09
(ODP) eq.]
Acidification potential, Accumulated Exceedance [mol H+
5.83E-02 6.19E-03 3.02E-05 0.00E+00 7.09E-05 7.69E-04 0.00E+00 -5.78E-03
(AP) eq.]
Eutrophication potential, fraction of nutrients
reaching freshwater end compartment 5.24E-03 8.01E-06 7.49E-07 0.00E+00 1.25E-06 6.74E-05 0.00E+00 -1.37E-03
[kg P eq.]
(EP-freshwater)
Eutrophication potential, fraction of nutrients
[kg N eq.] 1.09E-02 1.55E-03 1.20E-05 0.00E+00 2.66E-05 2.42E-04 0.00E+00 -1.25E-03
reaching marine end compartment (EP-marine)
Eutrophication potential, Accumulated Exceedance
[mol N eq.] 1.17E-01 1.72E-02 1.15E-04 0.00E+00 2.90E-04 2.66E-03 0.00E+00 -1.40E-02
(EP-terrestrial)
[kg
Formation potential of tropospheric ozone (POCP) NMVOC 3.30E-02 4.69E-03 4.02E-05 0.00E+00 1.00E-04 8.17E-04 0.00E+00 -3.83E-03
eq.]
Abiotic depletion potential for non-fossil resources
[kg Sb eq.] 1.77E-03 2.56E-07 1.77E-08 0.00E+00 4.88E-08 7.31E-07 0.00E+00 -1.10E-03
(ADP-minerals&metals)
MJ, net
Abiotic depletion potential for fossil resources
calorific 7.69E+01 2.80E+00 6.63E-02 0.00E+00 2.22E-01 1.68E+00 0.00E+00 -6.87E+00
(ADP-fossil)
value
[m3 world
Water (user) deprivation potential,
eq. 3.61E+00 7.08E-03 4.22E-04 0.00E+00 1.06E-03 5.19E-02 0.00E+00 -3.36E-01
deprivation-weighted water consumption (WDP)
Deprived]
3.2 Resource use and waste categories
The LCA results of GTBUILD - Titanium zinc plate metal per declared unit is listed as the table.
Table 4: Resource use and waste categories according to EN 15804.
RESULTS OF THE LCA - Resource use and waste categories per functional or declared unit
Core indicator Unit A1-A3 A4 A5 C1 C2 C3 C4 D
Use of renewable primary energy excluding
MJ -9.32E-01 2.15E-02 2.12E-03 0.00E+00 2.91E-03 5.92E-02 0.00E+00 -8.84E-01
renewable primary energy resources used as
EPD 中国项目 值得信赖
— 6 —
The first EPD Programme Operator registered in China, contributing to the EPD system building in China
www.epdchina.cn
Programme operator EPD China
Registration number EPD -CN - 00013
raw materials (PERE)
Use of renewable primary energy resources
MJ 1.30E+01 0.00E+00 0.00E+00 0.00E+00 0.00E+00 0.00E+00 0.00E+00 0.00E+00
used as raw materials (PERM)
Total use of renewable primary energy
resources (PERT) (primary energy and
MJ 1.20E+01 2.15E-02 2.12E-03 0.00E+00 2.91E-03 5.92E-02 0.00E+00 -8.84E-01
primary energy resources used as raw
materials)
Use of non-renewable primary energy
excluding non- renewable primary energy MJ 7.68E+01 2.80E+00 6.63E-02 0.00E+00 2.22E-01 1.68E+00 0.00E+00 -6.87E+00
resources used as raw materials (PENRE)
Use of non-renewable primary energy
MJ 9.56E-02 0.00E+00 0.00E+00 0.00E+00 0.00E+00 0.00E+00 0.00E+00 0.00E+00
resources used as raw materials (PENRM)
Total use of non-renewable primary energy
resources (PENRT) (primary energy and
MJ 7.69E+01 2.80E+00 6.63E-02 0.00E+00 2.22E-01 1.68E+00 0.00E+00 -6.87E+00
primary energy resources used as raw
materials)
Use of secondary material (SM) kg 0.00E+00 0.00E+00 0.00E+00 0.00E+00 0.00E+00 0.00E+00 0.00E+00 0.00E+00
Use of renewable secondary fuels (RSF) MJ 0.00E+00 0.00E+00 0.00E+00 0.00E+00 0.00E+00 0.00E+00 0.00E+00 0.00E+00
Use of non-renewable secondary fuels
MJ 0.00E+00 0.00E+00 0.00E+00 0.00E+00 0.00E+00 0.00E+00 0.00E+00 0.00E+00
(NRSF)
Net use of fresh water (FW) m3 1.09E-01 2.23E-04 1.31E-05 0.00E+00 3.14E-05 1.52E-03 0.00E+00 -1.07E-02
Hazardous waste disposed (HWD) kg 4.58E-02 4.19E-05 1.52E-05 0.00E+00 5.88E-06 9.37E-01 0.00E+00 -3.17E-04
Non-hazardous waste disposed (NHWD) kg 3.51E-01 2.01E-02 2.03E-03 0.00E+00 1.36E-02 4.83E-01 0.00E+00 -3.14E-02
Radioactive waste disposed (RWD) kg 2.28E-04 3.36E-07 3.28E-08 0.00E+00 4.71E-08 7.32E-07 0.00E+00 -1.19E-05
Components for re-use (CRU) kg 0.00E+00 0.00E+00 0.00E+00 0.00E+00 0.00E+00 0.00E+00 0.00E+00 0.00E+00
Materials for recycling(MR) kg 5.23E-02 0.00E+00 8.20E-02 0.00E+00 0.00E+00 0.00E+00 1.00E+00 0.00E+00
Materials for energy recovery (MER) kg 0.00E+00 0.00E+00 0.00E+00 0.00E+00 0.00E+00 0.00E+00 0.00E+00 0.00E+00
MJ, net
Exported energy (EE) calorific 0.00E+00 0.00E+00 0.00E+00 0.00E+00 0.00E+00 0.00E+00 0.00E+00 0.00E+00
value
MJ, net
Exported thermal energy (ETE) calorific 0.00E+00 0.00E+00 0.00E+00 0.00E+00 0.00E+00 0.00E+00 0.00E+00 0.00E+00
value
3.3 Information on biogenic carbon content
Table 5: Biogenic carbon content
Biogenic carbon content Unit (expressed per functional unit or per declared unit)
Biogenic carbon content in product 0 kg C
Biogenic carbon content in accompanying packaging 0.034 kg C
NOTE：1 kg biogenic carbon is equivalent to 44/12 kg of CO2.
EPD 中国项目 值得信赖
— 7 —
The first EPD Programme Operator registered in China, contributing to the EPD system building in China
www.epdchina.cn
Programme operator EPD China
Registration number EPD -CN - 00013
4 Supplementary information
4.1 Calculation rules
In this section, it is suggested to include but not limited to following information:
l Declared or functional unit: 1 kilogram of product.
l Time representativeness: The data represents the period between 1st June 2023 and 31st May 2024.
l Cut-off rules: On the input side all flows entering the system and comprising more than 1% in total mass or
contributing more than 1% to primary energy consumption are considered.
l Data quality: The evaluation of the quality of the modules used in the database is available in the appendix of
the report.
l Allocation: The plant produces multiple products and the total quantities used on the sites have been allocated
to the products by dividing the amount of the product in question with the total amount of all products
produced at the site.
l In this report, the average value of each product group is used to represent the EPD declared results of the
products in the product group. The product process, equipment and main materials in each product group are
the same, and the differences between different models are mainly due to the differences in length, width and
thickness. The declared unit of 1kg is used, and the difference is small, so the average value is adopted. That
is, the data of the total raw material consumption, raw material transportation, energy consumption, waste,
product transportation and other stages of different models and specifications of each product group are
divided by the total output of the product group.
4.2 Scenarios and additional technical information
In this section, the A1-A3 is divide into 3 parts in the LCA model, including A1 raw material supply, A2 transport,
and A3 manufacture. It is suggested to include but not limited to following information:
l Firstly, the raw material supply part covers the raw material and the packaging material.
l Secondly, the upstream transport of each material is modelled in the A2 part; the transport type, mass and
distance are modelled according to the primary data and the loading rate and empty return rate is respectively
set as 100% and 0%.
l Thirdly, the A3 manufacture process includes the resources input and the manufacture wastes in production.
The production process consumes electricity and diesel according to the primary data. It is assumed that the
distance of end-of-life product transportation (C2), product transportation from downstream customers to the
construction site (A2), and the transportation of waste generated during installation and construction (A5) are
100km, 50km, and 50km respectively, and the transportation means are trucks (no specified model).
EPD 中国项目 值得信赖
— 8 —
The first EPD Programme Operator registered in China, contributing to the EPD system building in China
www.epdchina.cn
Programme operator EPD China
Registration number EPD -CN - 00013
References
l ISO 14040: 2006, Environmental management–Life cycle assessment–Principles and framework
l ISO 14044: 2006, Environmental management–Life cycle assessment–Requirements and guidelines
l ISO 14025: Environmental labels and declarations–Type III environmental declarations–Principles and
procedures (2006)
l EN 15804:2012+A2:2019 Sustainability of construction works-Environment product declarations-Core rules
for the product category of construction products
l EPDCN-PCR-202204 PCR FOR CONSTRUCTION PRODUCTS AND CONSTRUCTION SERVICES TO
EN 15804 V2.0
l EPD CHINA GENERAL PROGRAMME INSTRUCTIONS Version3
l SimaPro Tutorial, Version:6.0
EPD 中国项目 值得信赖
— 9 —
The first EPD Programme Operator registered in China, contributing to the EPD system building in China
www.epdchina.cn
Programme operator EPD China
Registration number EPD -CN - 00013
Revision history
Any revision has been made after the EPD registration shall be clearly updated in this section.
Annex
An Annex may contain all additional information required for specific national use in different countries.
EPD 中国项目 值得信赖
— 10 —
The first EPD Programme Operator registered in China, contributing to the EPD system building in China
www.epdchina.cn
Programme operator EPD China
Registration number EPD -CN - 00013
EPD 中国项目 值得信赖
The first EPD Programme Operator registered in China, contributing to the EPD system building in China
www.epdchina.cn
ENVIRONMENTAL
PRODUCT
DECLARATION
EPD 中国项目 值得信赖
— 11 —
The first EPD Programme Operator registered in China, contributing to the EPD system building in China
www.epdchina.cn
ANNEX 1
ANNEX 1: Self declaration from EPD owner
Specific requirements
1 Applied electricity data set used in the manufacturing phase
The electricity mix for the electricity used in manufacturing (A3) is the electricity grid mix
<0.2367374 kgCO eqv/MJ>
2
2 Transport from the place of manufacture to a central warehouse
Transport distance, and CO -eqv./DU from transport of the product from factory gate to central warehouse
2
in Oslo shall be given. The following table shall be included in the EPD:
Capacit
y
Target Kg
Typ utilisati Distan Fuel/Ener Value
product Type of vehicle Unit CO2-
e on (incl. ce km gy use (l/t)
name eqv./DU
return)
%
Boa 0.0035
t 42.2% container ship 20200 0.0029 59.12
GTBUILD -
Truck 0.0048
Galvanized
Truc 53.3% （EURO5）>32t 20 0.022 l/t·k 0.45
coated
k m
steel sheet
X Truck (unspecified) 100 N/A N/A N/A
metal
Tota 512.4 0.0004
l X X 20320 0.025 4 4
Boa 0.0000
t 42.2% container ship 20310 0.0029 59.44 36
GTBUILD - l/t·k
Truck 0.47
Aluminum m
Truc 53.3% （EURO5）>32t 20 0.022 0.45
k
X Truck (unspecified) 100 N/A N/A N/A
Version 01 januar 2023
Tota 515.2 0.0004
l X X 20430 0.025 1 4
Boa 0.0035
t 42.2% container ship 20308 0.0029 59.44
Truck 0.0048
GTBUILD -
Truc 53.3% （EURO5）>32t 20 0.022 l/t·k 0.45
Titanium
k m
zinc plate
X Truck (unspecified) 100 N/A N/A N/A
Tota 515.1 0.0004
l X X 20428 0.025 6 4
Boa 0.0035
t 42.2% container ship 8909 0.0029 26.07
Truck 0.0056
19.70% （EURO5)3.5~7.5t 2.4 0.111 0.27
GTINDUST
RY - Truc l/t·k
Truck 0.0048
Stainless k m
53.3% （EURO5）>32t 120 0.022 2.67
steel
X Truck (unspecified) 100 N/A N/A N/A
Tota 1241. 0.0001
l X X 9131.4 0.136 90 0
3 Impact on the indoor environment
Version 01 januar 2023
(cid:0) Indoor air emission testing has been performed; specify test method and reference;
M1, _____________________________________________________________
(cid:0) No test has being performed
(cid:0) Not relevant; specify The target products are not used indoors
Version 01 januar 2023
