ENVIRONMENTAL PRODUCT DECLARATION
as per ISO 14025 and EN 15804+A2
Owner of the Declaration Armacell GmbH
Programme holder Institut Bauen und Umwelt e.V. (IBU)
Publisher Institut Bauen und Umwelt e.V. (IBU)
Declaration number EPD-ARM-20200218-IBB1-EN
Issue date 12.03.2021
Valid to 11.03.2026
ArmaFlex Ultima insulation for building equipment and
industrial installations
Armacell GmbH
www.ibu-epd.com | https://epd-online.com
Umwelt Produktdeklaration Name des Herstellers – Name des Produkts
1. General Information
Armacell GmbH ArmaFlex Ultima
Programme holder Owner of the declaration
IBU – Institut Bauen und Umwelt e.V. Armacell GmbH
Panoramastr. 1 Robert-Bosch-Str. 10
10178 Berlin 48153 Münster - Germany
Germany
Declaration number Declared product / declared unit
EPD-ARM-20200218-IBB1-EN 1m³ insulation material ArmaFlex Ultima
This declaration is based on the product Scope:
category rules: Product line ArmaFlex Ultima
Insulating materials made of foam plastics, 06.2017 Insulation material based on flexible elastomeric foam
(PCR checked and approved by the SVR) (FEF) for building equipment and industrial
installations, vulcanized in tubes and sheets.
Issue date This declaration is an Environmental Product
12.03.2021 Declaration according to ISO 14025 describing the
average environmental performance of the product
produced in Germany and Spain.
Valid to
11.03.2026
The average has been calculated based on site
specific annual production volumes.
As the installation of the product is not restricted to
countries where the products have been produced the
validity of this EPD is considered at least EU wide.
The owner of the declaration shall be liable for the
underlying information and evidence; the IBU shall not
be liable with respect to manufacturer information, life
cycle assessment data and evidences.
The EPD was created according to the specifications
of EN 15804+A2. In the following, the standard will be
simplified as EN 15804.
Verification
The standard EN 15804 serves as the core PCR
Independent verification of the declaration and data
according to ISO 14025:2010
Dipl. Ing. Hans Peters internally x externally
(chairman of Institut Bauen und Umwelt e.V.)
Dr. Alexander Röder Mr Carl-Otto Neven
(Managing Director Institut Bauen und Umwelt e.V.)) (Independent verifier)
2. Product
2.1 Information about the enterprise  Engineered Foams develops high-
Armacell International GmbH is a producer of flexible performance foams for the use in a broad
insulation foams for the equipment insulation market
range of end markets including transportation,
and a provider of engineered foams which operates
automotive, wind energy, sports and
two main businesses:
construction.
 Advanced Insulation develops flexible foams
for the insulation of technical equipment
utilised for the transport of energy - such as The product focus is insulation materials enhancing the
energy efficiency of technical equipment, high-
heating, ventilation & air conditioning (HVAC)
performance foams for technical and lightweight
and heating & plumbing (H&P) in residential
applications, 100% recycled PET products and next-
and commercial construction, process lines in
generation aerogel technology.
the heavy- and oil & gas industry, equipment
in transportation, as well as, acoustics.
2 Environmental Product Declaration Armacell GmbH – ArmaFlex Ultima insulation for industrial and building installation
2.2 Product description/Product definition Modulus of elasticity acc. to EN not
N/mm^2
ArmaFlex Ultima is the professional, highly-flexible, 826 relevant
closed-cell elastomeric foam insulation (FEF) for not
Moisture content at 23 °C, 80% M.-%
continuous energy saving and condensation control relevant
purposes with improved fire-retardant properties and Dynamic rigidity acc. to DIN EN not
MN/mm^3
low smoke generation. The combination of very low 29052 relevant
thermal conductivity and extremely high resistance to Creep behaviour or permanent
not
water vapour transmission prevents long-term energy compressive strength acc. to DIN N/mm^2
relevant
losses and water vapour ingress and reduces the risk EN 1606
of corrosion under insulation. Water absorption after diffusion not
acc. to EN 12088 relevant
Vol.-%
For the placing on the market of the product in the Maximum water absorption acc. not
European Union/European Free Trade Association to DIN EN 12091 relevant Vol.-%
(EU/EFTA) (with the exception of Switzerland)
Water absorption by capillarity not
Regulation (EU) No. 305/2011 (CPR) applies. The cm
acc. to DIN EN 15801 relevant
product needs a declaration of performance taking into
consideration EN 14304:2013-04 and the CE-marking.
Insulation materials on the basis of synthetic rubber do
For the application and use the respective national
not absorb moisture from the air. For this reason, the
provisions apply.
normal building moisture does not lead to an increase
in thermal conductivity.
2.3 Application
ArmaFlex Ultima is used to insulate pipes, air ducts
Performance data of the product in accordance with
and vessels including fittings and flanges of industrial
the declaration of performance with respect to its
installations and building equipment.
essential characteristics according to EN 14304:2013-
 Condensation control, energy saving and
04
noise control in refrigeration and air
conditioning equipment and process plants. 2.5 Delivery status
 Energy saving according to local energy- FEF made of cross-linked elastomer with improved
fire-retardant properties and low smoke generations
saving laws, prevention of heat loss and noise
supplied as sheets, tubes and shaped pieces.
reduction of heating and plumbing systems.
Products with self-adhesive backings/closures are
 Condensation control and noise reduction in
available; these variations are not included in the
service-water and waste-water systems. calculations. Insulation thicknesses are available for all
 Condensation control, energy saving and common pipe diameters up to an outer diameter of 89
noise control in refrigeration and air- mm (tubes).
conditioning equipment in the ship-building
2.6 Base materials/Ancillary materials
sector.
ArmaFlex is a highly flexible insulation material based
on synthetic rubber, which consists of around 20 basic
2.4 Technical Data components. The following table displays the
composition split into functional substance groups.
Constructional data Name Value Unit
Name Value Unit Rubber and polymers 15 %
Gross density 57.5 kg/m3 Fillers and pigments 11 %
Water vapour diffusion resistance Blowing agent 11 %
factor acc. to EN 12086, EN 7000 - Vulcanisation system, additives,
23 %
13469 plasticisers
0,040 Flame retardant 40 %
Thermal conductivity W/(mK)
(0°C)
Maximum service temperature Synthetic rubber determines the flexibility;
+110 °C
acc. to EN 14706, EN 14707 Fillers determine the fire properties and firmness;
Minimum service temperature -50 °C Blowing agent causes the expansion process during
Tubes: BL- manufacturing;
Reaction to fire acc. to EN 13501- s1, d0/ Accelerator and sulphur enable the vulcanisation;
-
1 Sheets: B- Plasticizers determine the flexibility;
s2, d0 Flame retardants ensure fire resistance.
Structure-borne sound
not
transmission acc. to EN ISO According to the European Chemicals Regulation
relevant
3822-1 REACH manufacturer, importers and downstream
Weighted sound absorption users must register their chemicals and are
not
coefficient αw acc. to EN ISO responsible for their safe use on their own. For its
relevant
11654 production Armacell uses exclusively verifiably
Compressive strength acc. to EN not registered and approved substances / mixtures.
N/mm^2
826 relevant According to available data and the information
not provided by preliminary suppliers, the product does not
Tensile strength acc. to EN 826 N/mm^2
relevant contain substances (SVHC) that are considered
not substances meeting the criteria for inclusion in annex
Flexural strength relevant N/mm^2 XIV (List of Substances Subject to Authorisation) as
3 Environmental Product Declaration Armacell GmbH – ArmaFlex Ultima insulation for industrial and building installation
laid down in Article 57 and article 59 of REACH (EC)
1907/2006.). Products manufactured and marketed by
Armacell do not have to be registered. The products 2.11 Condition of use
may contain traces of azodicarbonamide (ACDA). When the products are used for the purpose for which
Possible minimal residual amounts are included in the they are intended, there are no changes in the material
polymer matrix. A health impairment can be excluded. composition during use, except in the event of
For the production of insulation material based on extraordinary impacts (see 2.14).
synthetic rubber, there is presently no alternative to
ACDA available. 2.12 Environment and health during use
Ingredients: There are no particular aspects of the
material composition during use.
Eurofins Product Testing A/S has tested a wide range
2.7 Manufacture and varieties of typical FEF (Flexible Elastomeric
ArmaFlex products are manufactured in a Foam) products marketed in the EU from CEFEP
pressureless, continuous and discontinuous production (European Group of FEF manufacturers). Sampling,
process. testing and evaluation were performed according to
In the first step, a homogenous compound is produced CEN TS 16516, AgBB, ISO 16000-3, ISO 16000-6,
with rubber, additives, ancillary materials, blowing and ISO 16000-9, ISO 16000-11 in the latest versions.
vulcanization agents. This is done on the rolling mill or Based on the loading factor 0.05 m²/m³, which was
in the internal mixer followed by the rolling mill. determined after consideration of real life applications
Rubber extruders are used to process the compounds with FEF products (in living rooms) and
to produce raw profiles with defined dimensions. Here recommendation of experts of the test institute, all
exact compliance with the dimensions for the raw results were clearly below the limit values. For
profile is crucial for the dimensional accuracy of the example, the determined total volatile organic
foamed product. compound (TVOC) after 28 days was for all samples
In the case of the discontinuous, pressureless below 100 mg/m3. Certificates are available on
production process, the raw profiles are cut to length request.
and then foamed in a hot-air oven. In the case of the
continuous, pressureless process, the extruded profile
is fed directly onto a vulcanization line whose energy 2.13 Reference service life
source may be hot air, for example. ArmaFlex products are long-lasting products. Findings
In foam production, vulcanization and blowing show that when used and installed properly they can
processes run alongside each other. Both reactions have an estimated service life of more than 50 years. It
are regulated by temperature control. Recipe and is practically only restricted by the service life of the
temperature control determine the properties of the equipment or whole building, which can extent that
foam. time period. The insulation performance is almost
Quality assurance: completely maintained over the entire service life. The
EC Certificate of conformity no. 0543 of the insulation performance is only compromised by
Gütegemeinschaft Hartschaum e.V. Celle. extraordinary impacts and damage during construction.
Quality management system in accordance with EN
ISO 9001.
2.14 Extraordinary effects
2.8 Environment and health during
manufacturing Fire
During all manufacturing steps and at all production According to EN 13501, ArmaFlex is classified as a
sites of Armacell, the production follows the national combustible insulation material. Due to its material
guidelines and regulations. A regenerative thermal structure ArmaFlex does not contribute to an
oxidizer is installed to treat exhaust air. uncontrollable spread of fire under installation
Certification of the environmental management system conditions typical on a building site. ArmaFlex does not
is in accordance with ISO 14001. drip under practical fire conditions, this means that fire
spread is ruled out. The product is self-extinguishing
and therefore only makes a minor contribution to the
2.9 Product processing/Installation actual fire event. There is no possibility of the material
The product is installed by using knives. No special self-igniting. ArmaFlex does not propagate the fire
tools, nor specific protection is necessary. either horizontally or vertically.
When applying adhesives, the information given in the
relevant safety data sheets is to be heeded. Fire protection
The recommendations for installing the product Name Value
depend on the product and system and are described Tubes: BL
in the respective documents (e.g. application manuals) Euro class / Sheets:
or the data sheets. More details under B
www.armacell.com. Tubes/She
Burning droplets
ets: d0
Tubes: s1/
Smoke development
2.10 Packaging Sheets: s2
As a rule, ArmaFlex products are packaged in
cardboard boxes and transported on reusable pallets. Water
Over-sized rolls of sheet material are packaged in Armacell insulation materials have a high resistance to
polyethylene (PE) foil. The cardboard boxes can be water vapour transmission which keeps possible water
recycled through Interseroh’s dual system.
4 Environmental Product Declaration Armacell GmbH – ArmaFlex Ultima insulation for industrial and building installation
vapour transmission processes to a minimum 2.15 Re-use phase
permanently. Therefore, a significant reduction in the If removed properly the product can be re-used.
insulation effect can be ruled out permanently. Correctly sorted material can be ground and used to
If the insulation material is exposed to water over a manufacture new products (e.g. ArmaSound).
long period of time (e.g. flooding) it should be replaced.
2.16 Disposal
Mechanical destruction Dispose of the materials according to local regulations.
ArmaFlex insulation materials are flexible foams and Regulated by the European Waste Catalogue: Waste
thus display limited mechanical stability. Therefore, if code 07 02 13 (waste plastic).
the material will be subject to greater mechanical Note: Please observe Commission Decision
impact it should be protected appropriately, e.g. by a 2001/118/EC.
metal jacket or Arma-Chek covering.
ArmaFlex products (with the exception of 2.17 Further information
HT/ArmaFlex) are not UV resistant. If the material is Further information on ArmaFlex® can be found on the
subject to UV-rays it should be protected accordingly. manufacturer’s website www.armacell.com. Detailed
specification clauses for the products are provided at
www.armaflex.de.
3. LCA: Calculation rules
3.1 Declared Unit and packaging (A5) and the product (C3) are declared
The declaration refers to 1 m³ insulation product. in module D.
For the LCA calculations the average density per
product brand is used.
As additional information and support for installers the 3.3 Estimates and assumptions
thermal conductivity coefficient (lambda-value) and R- Scenario assumptions:
value per 20 cm thickness per product brand are given. Installation (A5):
The additional demand of material for installation
Declared unit depends on the specific frame conditions of the
Name Value Unit building and pipe system to be insulated. Parts of the
Declared unit 1 m3 product can be joined; thus installation off-cut is very
Gross density 57.5 kg/m3 small. A loss of 1% is assumed.
Conversion factor to 1 kg (kg/m³) 57.5 - Transport to customer (A4):
Armacell’s data collectors reported average figures for
Thermal conductivity λ: 0.040 W/(mK (0°C) the distribution of their material. Depending on the
R-value – thickness: 20 cm: 5.0 (m²K)/W country, the transport distance varies from 500 km to
800 km
End-of-life (C2, C3):
The transport from place of usage to a waste
3.2 System boundary incineration plant is assumed as 100 km.
The data collection refers to the yearly production in After the demolition of the product a current realistic
2019. The following life cycle stages are considered. End-of-life scenario is the incineration of the material.
According to the reported net calorific value of the
Type of EPD: Cradle-to-Gate with options: materials and the elementary composition, a partial
stream consideration for the incineration process of
Production A1-A3: PVC-products is applied as an approximation for all
The LCA calculation covers the production of the raw declared products.
materials (supply chain – A1), the mixing of raw Inventory estimations and approximations:
materials according to the respective recipes The reported recipes for the rubber mixes contain
(MasterBatch) exclusively done in Münster, Germany, specific substances of the rubber industry. For these
the transport (A2) of the MasterBatches to the materials only partly life cycle inventories are available.
production facility for foaming and the foaming process Approximations are used with the consideration of
(A3) in Germany and Spain, including the packaging similar supply chain effort or similar elementary
material. composition. Partly an estimation is modelled using
Transport A4: pre-products of the specific material and adding an
Average values for the transport from factory gate to energy effort as well as considering the treatment of
construction site are assumed. production residues for this step in the supply chain.
Installation A5:
The installation considers the production of off-cuts, 3.4 Cut-off criteria
incineration of these off-cuts and the disposal scenario In the assessment, all reported data from the
for the packaging material. Auxiliaries like adhesives or production process are considered, utilised thermal
tapes or energy for installation are not considered. energy, and electric power consumption using best
End-of-life C2, C3: available life cycle inventory (LCI) datasets. Thus
An incineration scenario for the used and demolished material and energy flows contributing less than 1% of
product, including an assumption for the transport to mass or energy are considered.
disposal, is covered. No cut-off criteria are applied in the foreground data in
Benefits for the next product system D: this study.
Credits for electrical and thermal energy resulting from For cut-off criteria in the background system, see
the waste incineration process of the off-cut material information provided in the modelling principles and
5 Environmental Product Declaration Armacell GmbH – ArmaFlex Ultima insulation for industrial and building installation
specific documentations (documentation.gabi- products considered in this study. Data for thermal and
software.com). electrical energy, as well as auxiliary material, refer to
the declared products only. During data collection the
3.5 Background data allocation is done via mass, area, pieces or time spent
The LCA model is created using the GaBi ts Software in the machine, depending on the process step and
system (v9) for life cycle engineering, developed by reasonable split. The data collectors at Armacell
Sphera. The GaBi LCI database provides the life cycle decided on the distribution basis.
inventory data for several of the raw and process Allocation for waste materials:
materials obtained from the background system. The Production waste is sent to a waste incineration plant
most recent update of the database was 2020. and to landfill (Spain). Resulting electrical and thermal
energy from the incineration process is looped inside
3.6 Data quality module A1-A3. The quality of the recovered energy is
The foreground data collected by the manufacturer are assumed to the same as that of the input energy.
based on yearly production amounts and Landfilling of plastic material is assumed not to deliver
extrapolations of measurements on specific machines any landfill gas.
and plants. All applied incineration processes are displayed via a
As the average environmental performance of the partial stream consideration for the combustion
product brand has been calculated by a weighting of process, according to the specific composition of the
the site-specific production volumes the results also incinerated material. For the waste incineration plant
show a representative picture regarding site specific an R1-value of > 0.6 is assumed.
production technologies. The average results therefore Environmental burden of the incineration of installation
can be assessed as robust. residues (off-cuts), packaging and the product in the
Most of the necessary life cycle inventories for the end-of-life scenario are assigned to the system (A5 or
basic materials are available in the GaBi database. C3); resulting credits for thermal and electrical energy
The last update of the database was in 2020 (service are declared in module D.
pack 40). The credits for thermal and electrical energy are
Further LCIs for materials of the supply chain of the calculated via inversion of the life cycle inventory of
basic materials are approximated with LCIs of similar European average data.
materials or estimated by the combination of available Allocation for waste paper:
LCIs. Paper/corrugated board is used as packaging material
For electrical and thermal energy regional specific grid and this usually includes a mix of recycled and virgin
mixes and regional specific supply for natural gas are fibres. When modelling the production of paper, the
considered. scrap paper that is used in this process has been
assumed to be burden free. Similarly, waste paper
3.7 Period under review arising in the product life cycle is assumed to be
The production data refer to an average of the year recycled. Robust data on paper and cardboard
2019. recycling are not promptly available and refer to a very
complex system. Hence, to apply this methodology
3.8 Allocation consistently throughout the model, a cut-off approach
Allocation of upstream data: has been applied, i.e., input of waste paper is
For all refinery products, allocation by mass and net considered without environmental burden, resulting
calorific value is applied. The specific manufacturing waste paper is not credited. The recycling process and
route of every refinery product is modelled and so the the production process of paper are merged in the
impacts associated with the production of these production process. The C-balance referring to fresh
products are calculated individually. fibre is corrected via CO2 emissions (biotic)
Materials and chemicals used in the manufacturing (assumption of final rotting or incineration in the time
process are modelled using the allocation rule most frame of 100 years).
suitable for the respective product. For further
information on a specific product see 3.9 Comparability
documentation.gabi-software.com. Basically, a comparison or an evaluation of EPD data
Allocation in the foreground data: is only possible if all the data sets to be compared
Part of the production residues (ca. 2%) are used for were created according to EN 15804 and the building
the manufacturing of a non-declared product context, respectively the product-specific
(ArmaSound). These materials leave the process characteristics of performance, are taken into account.
without further consideration of any treatment and
without credit (cut-off-approach). The used background dataset DB has been GaBi
No further allocation is applied in the software model. (service pack 40, 2020).
The overall production of the Armacell production
facilities comprises further products beside the
4. LCA: Scenarios and additional technical information
Characteristic product properties less than 5 % of the total mass of the product and
Information on biogenic Carbon accompanying packaging, the declaration of biogenic
carbon content may be omitted. The mass of
The biogenic carbon content quantifies the amount of packaging containing biogenic carbon shall always be
biogenic carbon in a construction product leaving the declared.
factory gate, and it shall be separately declared for the
product and for any accompanying packaging.If the Note: 1 kg biogenic Carbon is equivalent to 44/12 kg of
total mass of biogenic carbon containing materials is CO
2
6 Environmental Product Declaration Armacell GmbH – ArmaFlex Ultima insulation for industrial and building installation
Information on describing the biogenic Carbon
Content at factory gate
Name Value Unit
Biogenic Carbon Content in
0 kg C
product
Biogenic Carbon Content in
18.05 kg C
accompanying packaging
The embodied biogenic carbon leaves the system in
Module A5.
The following technical information serves as basis for
the declared modules. The values refer to the declared
unit of 1 m³.
Transport to the building site (A4)
Name Value Unit
Litres of fuel 0.16 l/100km
Transport distance 800 km
Capacity utilisation (including empty
85 %
runs)
Installation into the building (A5)
Name Value Unit
Material loss 1 %
Estimated service life
Name Value Unit
Life Span according to the
50 a
manufacturer
End of life (C1-C4)
Name Value Unit
Energy recovery in WIP 57,5 kg
Reuse, recovery and/or recycling potentials (D),
relevant scenario information
Module D includes the credits of the incineration
processes from A5 (off-cut of product installation,
packaging waste) and C3 (incineration of the product).
A waste incineration plant with an R1-value > 0.6 is
assumed.
7 Environmental Product Declaration Armacell GmbH – ArmaFlex Ultima insulation for industrial and building installation
5. LCA: Results
The following information on environmental impacts is expressed with the impact category parameters of LCIA
using characterisation factors. The chosen characterisation factors fulfil the requirements of EN 15804.
Disclaimer:
EP-freshwater: This indicator has been calculated as “kg P eq” as required in the characterization model
(EUTREND model, Struijs et al., 2009b, as implemented in ReCiPe;
http://eplca.jrc.ec.europa.eu/LCDN/developerEF.xhtml)
DESCRIPTION OF THE SYSTEM BOUNDARY (X = INCLUDED IN LCA; ND = MODULE OR INDICATOR NOT
DECLARED; MNR = MODULE NOT RELEVANT)
BENEFITS AND
CONSTRUCTI LOADS
PRODUCT STAGE ON PROCESS USE STAGE END OF LIFE STAGE BEYOND THE
STAGE SYSTEM
BOUNDARIES
8 Environmental Product Declaration Armacell GmbH – ArmaFlex Ultima insulation for industrial and building installation
lairetam
waR
ylppus tropsnarT
gnirutcafunaM
eht
morf
tropsnarT
etis
eht
ot
etag
ylbmessA esU
ecnanetniaM
riapeR
tnemecalpeR tnemhsibrufeR
ygrene
lanoitarepO esu
retaw
lanoitarepO esu
noitcurtsnoc-eD
noitilomed tropsnarT
gnissecorp
etsaW
lasopsiD -esueR -yrevoceR -gnilcyceR laitnetop
A1 A2 A3 A4 A5 B1 B2 B3 B4 B5 B6 B7 C1 C2 C3 C4 D
X X X X X ND ND MNR MNR MNR ND ND ND X X ND X
RESULTS OF THE LCA - ENVIRONMENTAL IMPACT according to EN 15804+A2: 1 m³ ArmaFlex Ultima
insulation for industrial and building installation
Core Indicator Unit A1-A3 A4 A5 C2 C3 D
Global warming potential - total [kg CO2-Eq.] 2.31E+2 3.70E+0 4.00E+1 2.68E-1 1.49E+2 -4.11E+1
Global warming potential - fossil fuels [kg CO2-Eq.] 2.64E+2 3.68E+0 5.02E+0 2.66E-1 1.49E+2 -4.09E+1
Global warming potential - biogenic [kg CO2-Eq.] -3.33E+1 -6.36E-3 3.50E+1 -4.61E-4 -6.52E-2 -9.60E-2
GWP from land use and land use change [kg CO2-Eq.] 3.89E-1 3.02E-2 4.69E-3 2.19E-3 3.04E-2 -2.86E-2
Depletion potential of the stratospheric ozone layer [kg CFC11-Eq.] 2.69E-9 4.48E-16 2.72E-11 3.25E-17 2.27E-13 -4.26E-13
Acidification potential, accumulated exceedance [mol H+-Eq.] 4.92E-1 1.14E-2 7.55E-3 8.29E-4 4.43E-2 -5.72E-2
Eutrophication, fraction of nutrients reaching freshwater
end compartment
[kg PO4-Eq.] 3.23E-3 1.13E-5 3.34E-5 8.21E-7 3.82E-5 -5.26E-5
Eutrophication, fraction of nutrients reaching marine end
[kg N-Eq.] 1.65E-1 5.11E-3 2.52E-3 3.70E-4 1.46E-2 -1.48E-2
compartment
Eutrophication, accumulated exceedance [mol N-Eq.] 1.50E+0 5.73E-2 2.70E-2 4.15E-3 1.79E-1 -1.59E-1
Formation potential of tropospheric ozone photochemical
[kg NMVOC-Eq.] 5.93E-1 1.01E-2 8.29E-3 7.31E-4 4.15E-2 -4.26E-2
oxidants
Abiotic depletion potential for non-fossil resources [kg Sb-Eq.] 3.99E+3 4.96E+1 4.67E+1 3.59E+0 2.75E+2 -6.94E+2
Abiotic depletion potential for fossil resources [MJ] 1.39E-3 2.67E-7 1.41E-5 1.94E-8 3.27E-6 -6.70E-6
Water (user) deprivation potential, deprivation-weighted [m³ world-Eq
6.60E+1 3.33E-2 2.25E+0 2.41E-3 1.15E+1 -4.23E+0
water consumption (WDP) deprived]
RESULTS OF THE LCA - INDICATORS TO DESCRIBE RESOURCE USE according to EN 15804+A2: 1 m³
ArmaFlex Ultima insulation for industrial and building installation
Indicator Unit A1-A3 A4 A5 C2 C3 D
Renewable primary energy as energy carrier [MJ] 1.21E+3 2.79E+0 1.11E+2 2.02E-1 5.71E+1 -1.51E+2
Renewable primary energy resources as material utilization [MJ] 9.70E+1 0.00E+0 -9.70E+1 0.00E+0 0.00E+0 0.00E+0
Total use of renewable primary energy resources [MJ] 1.31E+3 2.79E+0 1.44E+1 2.02E-1 5.71E+1 -1.51E+2
Non-renewable primary energy as energy carrier [MJ] 2.13E+3 4.97E+1 5.71E+1 3.60E+0 2.13E+3 -6.95E+2
Non-renewable primary energy as material utilization [MJ] 1.86E+3 0.00E+0 -1.04E+1 0.00E+0 -1.85E+3 0.00E+0
Total use of non-renewable primary energy resources [MJ] 3.99E+3 4.97E+1 4.67E+1 3.60E+0 2.75E+2 -6.95E+2
Use of secondary material [kg] 3.02E+1 0.00E+0 0.00E+0 0.00E+0 0.00E+0 0.00E+0
Use of renewable secondary fuels [MJ] 0.00E+0 0.00E+0 0.00E+0 0.00E+0 0.00E+0 0.00E+0
Use of non-renewable secondary fuels [MJ] 0.00E+0 0.00E+0 0.00E+0 0.00E+0 0.00E+0 0.00E+0
Use of net fresh water [m³] 1.58E+0 3.43E-3 5.42E-2 2.36E-4 3.03E-1 -1.75E-1
RESULTS OF THE LCA – WASTE CATEGORIES AND OUTPUT FLOWS according to EN 15804+A2:
1 m³ ArmaFlex Ultima insulation for industrial and building installation
Indicator Unit A1-A3 A4 A5 C2 C3 D
Hazardous waste disposed [kg] 6.43E-4 2.31E-6 6.53E-6 1.67E-7 1.24E-6 -2.77E-7
Non-hazardous waste disposed [kg] 2.79E+1 7.60E-3 1.35E+0 5.51E-4 9.14E+1 -3.20E-1
Radioactive waste disposed [kg] 1.03E-1 6.15E-5 1.31E-3 4.45E-6 8.73E-3 -5.16E-2
Components for re-use [kg] 0.00E+0 0.00E+0 0.00E+0 0.00E+0 0.00E+0 0.00E+0
Materials for recycling [kg] 0.00E+0 0.00E+0 3.57E+1 0.00E+0 0.00E+0 0.00E+0
Materials for energy recovery [kg] 0.00E+0 0.00E+0 0.00E+0 0.00E+0 0.00E+0 0.00E+0
Exported electrical energy [MJ] 0.00E+0 0.00E+0 2.09E+1 0.00E+0 1.50E+2 0.00E+0
Exported thermal energy [MJ] 0.00E+0 0.00E+0 3.75E+1 0.00E+0 2.74E+2 0.00E+0
RESULTS OF THE LCA – additional impact categories according to EN 15804+A2-optional:
1 m³ ArmaFlex Ultima insulation for industrial and building installation
Indicator Unit A1-A3 A4 A5 C2 C3 D
Potential incidence of disease due to PM emissions [Disease
4.85E-6 5.01E-8 7.11E-8 3.63E-9 1.07E-6 -4.86E-7
Incidence]
Potential Human exposure efficiency relative to U235 [kBq U235-
5.97E+1 8.89E-3 6.39E-1 6.44E-4 8.86E-1 -8.46E+0
Eq.]
Potential comparative toxic unit for ecosystems [CTUe] 3.89E+3 3.51E+1 4.34E+1 2.54E+0 2.28E+2 -1.49E+2
Potential comparative toxic unit for humans - cancerogenic [CTUh] 1.14E-7 7.34E-10 1.34E-9 5.32E-11 9.02E-9 -6.48E-9
Potential comparative toxic unit for humans - not cancerogenic [CTUh] 3.51E-6 4.35E-8 4.94E-8 3.15E-9 9.59E-7 -2.41E-7
Potential soil quality index [-] 9.08E+2 1.74E+1 1.08E+1 1.26E+0 6.24E+1 -1.09E+2
Disclaimer 1 – for the indicator IRP
This impact category deals mainly with the eventual impact of low dose ionizingradiation on human health of the
nuclear fuel cycle. It does not consider effects due to possiblenuclear accidents, occupational exposure nor due to
radioactive waste disposal in undergroundfacilities. Potential ionizing radiation from the soil, from radon and some
construction materials is also not measured by this indicator.
Disclaimer 2 – for the indicators ADPE, ADPF, WDP, ETP-fw, HTP-c, HTP-nc, SQP
The results of this environmental impact indicator shall be used with care as theuncertainties on these results are
high or as there is limited experience with the indicator.
6. LCA: Interpretation
The supply chain, i.e. the production of the purchased the overall greenhouse gas emissions. At the same
materials, causes the highest influence on all impact time a credit (D) of 11% is given to the next system,
categories and the primary energy. due to the use of electrical and thermal energy, gained
in the incineration processes for the product and the
Global Warming Potential off-cut material.
Looking at the GWP for the overall declared life cycle
phases, including production (A1-A3), transport (A4, Further impact categories
C2), installation (losses) (A5) and end-of-life (C3, D), The end-of-life scenarios have less influence on the
the production (A1-A3) contributes to 60%. other considered impact categories than on GWP. The
The production in the supply chain (A1) already main contribution of the considered life cycle phases is
contributes 42% to the total GWP value. Thus, every concentrated on module A1-A3.
increase in the production yield directly improves the The energy consumption in the foaming step
environmental performance of the products. influences all impact categories; variations depend on
The foaming process (A3), which includes the the national grid mixes for electricity.
electrical and thermal energy for the mixing, the
vulcanisation and blowing step as well as the
production of the packaging materials, shows a Primary Energy Demand
significant influence on GWP of the life cycle with 17%. The total primary energy demand is for both categories
Module A5 covers the production and disposal (renewable and non-renewable) significantly (> 100%)
(=incineration) of the off-cut material assumed as 1% influenced by the production of the module A1-A3. The
loss in respect to the required insulation material. other modules play a minor role (C3 with about 7%)
Additionally, the emissions of the incineration of
packaging material (plastic, wood) in a waste The share of primary energy bound as material
incineration plant are considered. The installation step accounts for about 40%, which is partly recovered and
contributes with 10% to the overall GWP. credited for in module D (-17%)
As end-of-life scenario an incineration is considered.
The emissions of the product (C3) contribute to 39% to
7. Requisite evidence
recommendation of the experts of the test institute, all
7.1 VOC emissions results were clearly below the limit values. For
Eurofins Product Testing A/S has tested a wide range example the determined total volatile organic
and varieties of typical FEF (Flexible Elastomeric compound (TVOC) after 28 days was for all samples
Foam) products marketed in the EU from CEFEP below 100 mg/m3. Certificates are available on
(European Group of FEF manufacturers). Sampling, request.
testing and evaluation were performed according to
CEN TS 16516, AgBB, ISO 16000-3, ISO 16000-6, 7.2 Leaching performance
ISO 16000-9, ISO 16000-11 in the latest versions. According to EN 13468 is the content of water-soluble
Based on the loading factor 0.05 m²/m³, which were chloride ions for Armaflex Ultima ≤ 300 ppm.
determined after consideration of real life applications
with FEF products (in living rooms) and
9 Environmental Product Declaration Armacell GmbH – ArmaFlex Ultima insulation for industrial and building installation
8. References
AgBB building equipment and industrial installations -
Umweltbundesamt Germany, Health-related Determination of maximum service temperature
Evaluation of Emissions of Volatile Organic
Compounds (VVOC, VOC and SVOC) from Building EN 14707
Products EN 14707: 2013-01: Thermal insulating products for
building equipment and industrial installations -
CEFEP Determination of maximum service temperature for
The industry association for FEF and PEF insulation preformed pipe insulation
(Celle) in 2012
EN 15801
CEN TS 16516 EN 15801: 2010-04: Conservation of cultural property -
CEN TS 16516:2013-12: Construction products - Test methods - Determination of water absorption by
Assessment of release of dangerous substances - capillarity
Determination of emissions into indoor air
EN 15804
Comission Decision 2001/118/EC EN 15804:2012-04+A1 2013, Sustainability of
Amendment to European Waste Catalogue construction works — Environmental Product
Declarations — Core rules for the product category of
CPR construction products.
Regulation (EC) No 305/2011, Construction Products
Regulation EN 15804
EN 15804:2019+A2 (in press), Sustainability of
EN 826 construction works — Environmental Product
EN 826: 2013-05: Thermal insulating products for Declarations — Core rules for the product category of
building applications - Determination of compression construction products.
behaviour
EN 29052
EN 1606 EN 29052: 1992-08: Acoustics; determination of
EN 1606: 2013-05: Thermal insulating products for dynamic stiffness; part 1: materials used under floating
building applications - Determination of compressive floors in dwellings
creep
EU/EFTA
EN 12091 Regulation (EU) No. 305/2011 (CPR), European
EN 12091: 2013-06: Thermal insulating products for Union/European Free Trade Association (EU/EFTA)
building applications - Determination of freeze-thaw
resistance Eurofins Product Testing A/S
Eurofins Miljo, Smedeskowej 38, 8464 Galten,
EN 12086 Denmark
EN 12086:2013-06: Thermal insulating products for
building applications - Determination of water vapour European Waste Catalogue
transmission properties European Waste Catalogue and Hazardous Waste
List, Commission Decision 2000/532/EC
EN 13468
EN 13468: 2001-12: Thermal insulating products for GaBi
building equipment and industrial installations - GaBi 9 software-system and databases, LBP,
Determination of trace quantities of water soluble University of Stuttgart and Sphera, Leinfelden-
chloride, fluoride, silicate, and sodium ions and pH Echterdingen, 2020 (http://documentation.gabi-
software.com/)
EN 13469
EN 13469:2013-01: Thermal insulating products for IBU
building equipment and industrial installations - Institut Bauen und Umwelt e.V.: General Programme
Determination of water vapour transmission properties Instructions for the Preparation of EPDs at the Institut
of preformed pipe insulation Bauen und Umwelt e.V. Version 1., Berlin: Institut
Bauen und Umwelt e.V., 2016. www.ibu-epd.com
EN 13501-1
EN 13501-1: 2010-01: Fire classification of IBU PCR Part A
construction products and building elements - Part 1: PCR - Part A: Calculation Rules for the Life Cycle
Classification using data from reaction to fire tests Assessment and Requirements on the Project Report,
Institut Bauen und Umwelt e.V., www.ibu-epd.com,
EN 14304 2019.
EN 14304:2013-04: Thermal insulation products for
building equipment and industrial installations – IBU PCR PART B
Factory made flexible elastomeric foam (FEF) products PCR – Part B: Requirements on the EPD for Insulation
– Specification materials made of foam plastics, version 1.7, 01-2019 ,
Institut Bauen und Umwelt e.V., www.ibu-epd.com,
EN 14706 2019
EN 14706: 2013-01: Thermal insulating products for
10 Environmental Product Declaration Armacell GmbH – ArmaFlex Ultima insulation for industrial and building installation
ISO 3822-1 Determination of the emission of volatile organic
ISO 3822-1: 1999-05: Acoustics - Laboratory tests on compounds from building products and furnishing -
noise emission from appliances and equipment used in Sampling, storage of samples and preparation of test
water supply installations - Part 1: Method of specimens
measurement
ISO 16000-3
ISO 9001 ISO 16000-3:2011-10: Determination of formaldehyde
ISO 9001:2014-08: Quality management systems – and other carbonyl compounds in indoor air and test
Requirements chamber air - Active sampling method
ISO 11654 ISO 16000-6
ISO 11654: 1997-04: Acoustics - Sound absorbers for ISO 16000-6:2011-12: Indoor air - Part 6:
use in buildings - Rating of sound absorption Determination of volatile organic compounds in indoor
and test chamber air by active sampling on Tenax TA®
ISO 14001 sorbent, thermal desorption and gas chromatography
ISO 14001:2015, Environmental management systems using MS or MS-FID
— Requirements with guidance for use
ISO 16000-9
ISO 14025 ISO 16000-9:2006-02: Indoor air - Part 9:
ISO 14025:2011-10, Environmental labels and Determination of the emission of volatile organic
declarations — Type III environmental declarations — compounds from building products and furnishing -
Principles and procedures. Emission test chamber method
ISO 14040
ISO 14040:2009-11: Environmental management – REACH
Life cycle assessment – Principles and framework Regulation (EC) No 1907/2006, Regulation concerning
the Registration, Evaluation, Authorisation and
ISO 14044 Restriction of Chemicals (REACH)
ISO 14044:2006-10: Environmental management –
Life cycle assessment – Requirements and guidelines
ISO 15868
ISO 15686:2011-05, Buildings and constructed assets
- Service life planning
ISO 16000-11
ISO 16000-11: 2006-02: Indoor air - Part 11:
11 Environmental Product Declaration Armacell GmbH – ArmaFlex Ultima insulation for industrial and building installation
Publisher
Institut Bauen und Umwelt e.V. Tel +49 (0)30 3087748- 0
Panoramastr. 1 Fax +49 (0)30 3087748- 29
10178 Berlin Mail info@ibu-epd.com
Germany Web www.ibu-epd.com
Programme holder
Institut Bauen und Umwelt e.V. Tel +49 (0)30 - 3087748- 0
Panoramastr 1 Fax +49 (0)30 – 3087748 - 29
10178 Berlin Mail info@ibu-epd.com
Germany Web www.ibu-epd.com
Author of the Life Cycle
Assessment Tel +49 711 341817-0
Sphera Solutions GmbH Fax +49 711 341817-25
Hauptstraße 111- 113 Mail info@sphera.com
70771 Leinfelden-Echterdingen Web http://www.sphera.com
Germany
Owner of the Declaration
Armacell GmbH Tel +49-251-7603-0
Robert-Bosch-Str. 10 Fax +49-251-7603-346
48153 Münster Mail info.de@armacell.com
Germany Web www.armacell.de
