ENVIRONMENTAL PRODUCT DECLARATION
as per ISO 14025 and EN 15804+A2
Owner of the Declaration VELUX Group
Publisher Institut Bauen und Umwelt e.V. (IBU)
Programme holder Institut Bauen und Umwelt e.V. (IBU)
Declaration number EPD-VEL-20220140-IBJ3-EN
Issue date 25.07.2022
Valid to 24.07.2027
VELUX flat roof window CVU - grid-connected
VELUX A/S
www.ibu-epd.com | https://epd-online.com
1. General Information
VELUX A/S VELUX flat roof window CVU - grid-connected
Programme holder Owner of the declaration
IBU – Institut Bauen und Umwelt e.V. VELUX Group
Hegelplatz 1 Ådalsvej 99
10117 Berlin 2970 Hørsholm
Germany Denmark
Declaration number Declared product / declared unit
EPD-VEL-20220140-IBJ3-EN The declaration represents 1 piece of a grid-connected VELUX flat roof
window CVU of the size 1.20 m x 1.20 m = 1.44 m2
This declaration is based on the product category rules: Scope:
Windows and doors , 01.08.2021 The declaration covers 100% of grid-connected VELUX flat roof windows
(PCR checked and approved by the SVR) CVU by Østbirk Bygningsindustri, Denmark.
The owner of the declaration shall be liable for the underlying information
and evidence; the IBU shall not be liable with respect to manufacturer
Issue date information, life cycle assessment data and evidences.
25.07.2022
The EPD was created according to the specifications of EN 15804+A2. In
the following, the standard will be simplified as EN 15804.
Valid to
Verification
24.07.2027
The standard EN 15804 serves as the core PCR
Independent verification of the declaration and data according to ISO
14025:2011
internally X externally
Dipl.-Ing. Hans Peters
(Chairman of Institut Bauen und Umwelt e.V.)
Florian Pronold Dr. Eva Schmincke,
(Managing Director Institut Bauen und Umwelt e.V.) (Independent verifier)
1 Environmental Product Declaration - VELUX A/S - VELUX flat roof window CVU - grid-connected
2. Product
• EAD 220062-00-0401, June 2017, rooflight with bonded
2.1 Product description/Product definition
or mechanically fastened cover glass.
The grid-connected Velux flat roof windows CVU consists of a
motorised base unit made of a PUR/GRP curb with a wooden 2.4 Delivery status
core, with an integrated glazing unit and hinges on one side to
The product is available in pre-defined sizes covering 0,6x0,6m
allow for venting and a single layer flat or curved glass top unit
to 1,5x1,5m.
on top. For the placing of the product on the market in the
European Union/European Free Trade Association /EU/EFTA) 2.5 Base materials/Ancillary materials
(with the exception of Switzerland) the Regulation (EU) No. Composition of the base unit CVU:
305/2011 (CPR) applies. The product needs a declaration of
performance taking into consideration EAD 220062-00-0401, polyurethane 7 %
June 2017, rooflight with bonded or mechanically fastened
cover glass and the CE-marking. For the application and use heat-treated wood 8 %
the respective national provisions apply.
galvanized steel 7 %
2.2 Application
Velux flat roof windows CVU are used in renovation and new
PU with glass fibres 13 %
build.
laminated glass 25 %
2.3 Technical Data
The Declaration of Performance including relevant technical
tempered glass 12 %
specifications and test methods/test standards can be
downloaded from the website www.velux.com/ce.
heat strenghtened glass 15 %
The declared values in the table relate to the reference product
others
incl. an average pane. For other covered product variants,
specific values can be selected at the bottom of the above-
Composition of the top unit (ISU 1093):
mentioned download page
Curved glass 73 % Aluminium 25 % others
Constructional data for CVU 120120 20+ISU 1093
For other variants, see velux.com/ce Composition of the motor (CVP mains):
Name Value Unit
glavanized steel 15 %
Resistance to fire EN
NPD -
13501-2
iron/cast iron 20 %
External fire
performance EN NPD -
steel 15 %
13501-5
Water tightness EN PET/PC/PA 10 %
9A Class
1873
Resistance to wind cables 10 %
C3 Class
load
5 mm toughened/ -- / 4 mm DC motor 10 %
Resistance to snow
toughened / 16 mm / 7.5 mm -
load (33.4) laminated float cables 15 %
Impact resistance 3 Class
others
Bonding of cover
Compliant (ΔX≥0.75) -
glass
1) 'This product/article/at least one partial article contains
Airborne sound substances listed in the candidate list (date: 02.03.2022)
insulation EN ISO 39 (-1;-5) dB exceeding 0.1 percentage by mass:
410-3
• no
Thermal
Urc,ref300: 0,65 W/(m2K) 2) 'This product/article/at least one partial article contains other
transmittance EN -
Arc,ref300: 4,4 m2 CMR substances in categories 1A or 1B which are not on the
1873
candidate list, exceeding 0.1 percentage by mass:
Total solar energy
0,52 - • not investigated with suppliers
transmittance
3) 'Biocide products were added to this construction product or
Light transmittance
0,69 - it has been treated with biocide products (this then concerns a
EN 410
treated product as defined by the (EU) Regulation on Biocidal
Frame factor 0,1 - Products No. 528/2012):
Air permeability EN
4 Class • no
1026
Performance data of the product in accordance with the Recycled content
declaration of performance with respect to its essential
characteristics according to
2 Environmental Product Declaration - VELUX A/S - VELUX flat roof window CVU - grid-connected
The material composition of VELUX flat roof windows does not
change over their service life.
2.11 Environment and health during use
VELUX flat roof windows do not contain any pollutants that
could be released during use.
The values stated in the table relate to the recycled material Environmental protection: According to current knowledge,
streams in VELUX production. hazards to water, air and soil cannot arise when the products
are used as intended.
2.6 Manufacture
Health protection: According to current knowledge, no health
Base unit: hazards or impairments are to be expected.
PU raw material, gaskets and other minor components are 2.12 Reference service life
produced outside Velux. It is not possible to calculate the reference service life
according to ISO 15686. The service life based on a
Cutting and profiling of wood reinforcements are done at manufacturer's declaration is 30 years. The corresponding
production sites in Polen and Denmark. utilization scenario is declared in 4.
The PUR/GRP curb with wooden core, the insulating glass unit 2.13 Extraordinary effects
and the motor and the wall switch are assembled at the Fire
production site in Denmark.
Fire performance according to EN 13501:1
The production and final assembly of the base unit takes place
Name Value
at the production site in Denmark.
Building material class D
The final production processes includes preparation of the Burning droplets s2
PU/wood frame by cutting and profiling of wood, moulding, Smoke gas development d2
cutting, sandblasting and painting, assembly of the GRP sash
by pultrusion, profiling and drilling, cutting and mounting of
Water
gaskets and installation of glazing unit and window opener as
In the event of unforeseen exposure to water (flood), VELUX
well as packaging, stacking and wrapping of the product on
flat roof windows must be replaced as electrical components;
pallets.
no adverse effects on human health or the environment are to
be expected.
Top unit:
Mechanical destruction
All raw materials and components are produced outside Velux.
In the event of unforeseen mechanical destruction, VELUX flat
roof windows must be replaced; apart from potential injuries
The glass top unit is assembled at production site at Slovakia.
from glass cullet, no adverse effects on human health or the
environment are to be expected.
The final production processes include the assembly of the
product as well as packaging, stacking and wrapping of the
2.14 Re-use phase
product on pallets.
VELUX flat roof windows can be dismantled manually without
The factories are ISO 9001 certified.
any problems. The metal parts are usually recycled, and the
2.7 Environment and health during manufacturing plastic parts and wood are sent for thermal recycling for energy
recovery. Flat glass can be recycled whereas laminated glass is
All factories are ISO 14001 and ISO 45001 certified.
usually used as secondary aggregate in road construction or
2.8 Product processing/Installation landfilling.
ThThe product is delivered to the customer in two parts, a top
2.15 Disposal
and bottom part. After the hole in the roof is prepared, the
VELUX flat roof windows are mostly inert and can be disposed
bottom part of the product can be installed with the use of a
of in an appropriate landfill. However, due to the value of the
screwdriver, after which the top unit can be fastened to the
materials or the carbon content of the plastic parts and wood,
bottom unit.
recycling or energy recovery is preferable and common.
2.9 Packaging
The packaging usually consists of: Waste code according to the European Waste List (Regulation
- polyethylene film on the European Waste List):
- polystyrene foam parts
- cardboard 16 02 14 electronic parts
17 02 01 wood
The use of other packaging materials is possible, but 17 02 02 glass
insignificant in terms of quantity. 17 02 03 plastics
17 04 14 mixed metals
The plastic packaging (polyethylene (PE) film, polystyrene foam
2.16 Further information
parts) can be recycled if separated by type; alternatively, they
Further documentation on the products, technical data sheets,
can be incinerated.
BIM files, etc. can be found at:
2.10 Condition of use www.velux.com
3 Environmental Product Declaration - VELUX A/S - VELUX flat roof window CVU - grid-connected
3. LCA: Calculation rules
3.1 Declared Unit Module D includes the benefits and burdens associated with
The declared unit is 1 piece of a grid-connected VELUX flat recycling metals beyond the system boundary, resulting from
roof window CVU with a base unit made of a polyurethane, the treatment of recycled materials from the point of end-of-
heat-treated wood and plywood curb with an integrated glazing waste to the point of substitution (as loads) and substitution of
unit with 1.20 m x 1.20 m = 1.44 m2. primary resources (as benefits).
It also includes the benefits and burdens associated with
Declared unit
energy recovery from plastic waste in a municipal waste
Name Value Unit
incineration plant, as modeled in Module C3.
Declared unit 1 pce. In Module D, only net flows of metals leaving the product
Area 1.44 m2 system are considered.
Weight 133 kg
3.3 Estimates and assumptions
No further assumptions and estimates relevant to the result had
to be made beyond the points made in this chapter 3 and in
3.2 System boundary
chapter 4.
Type of EPD: Cradle to gate with options, with modules C1 –
C4, and module D (A1-A3, C1-C3, D and additional modules 3.4 Cut-off criteria
No data available from the company survey was neglected.
The production of VELUX flat roof windows (modules A1-A3) These include, among other things, material use, energy
includes raw material extraction, energy generation, waste demand (heat, electricity), packaging materials of raw materials
treatment and all transports up to the factory gate. In (insofar as they are generated as waste) and product
accordance with COUNCIL REGULATION (EU) No 333/2011, packaging, consumables in production, waste treatment and
secondary metals are modeled as part of the product system the transport of all inputs and outputs.
from the moment they are available as unmixed scrap. With this approach, mass and energy flows below 1 % were
Waste or secondary fuels are not used for production. also accounted for. No processes were neglected that would
have been known to the project managers and would have
Module A4 is not declared due to large variances in transport contributed significantly to the indicators of the impact
distances between the production site and the construction site, assessment.
where the product is installed.
3.5 Background data
Module A5: The products are delivered to the construction site Ecoinvent 3.8 (2021) is used as the background database.
ready to be installed. Manual installation is assumed, and
electricity consumption related to electric drilling machines, 3.6 Data quality
screw drivers, etc. is considered to be negligible. The The foreground data are based on extensive and detailed data
combustible packaging material (plastics, wood, etc.) is collection at the production site. The foreground data could be
assumed to be thermally treated in a municipal waste fully linked with corresponding data records from the
incineration plant with an efficiency R1 < 0.6 (according to the background database ecoinvent 3.8.
ecoinvent dataset used); the recovered energy is declared as The background data was updated in 2021. Thus, the quality of
exported energy. Metals and cardboard are recycled; it is the foreground and background data can be rated as very
assumed that these fractions reach the end-of-waste state after good.
having been sorted and transported (as a conservative choice)
3.7 Period under review
to a recycler. No packaging waste is landfilled.
The LCA data represents the production conditions for the year
Modules B1 to B7 are not relevant for the product under 2021.
consideration or no significant environmental impacts occur.
3.8 Geographic Representativeness
Land or region, in which the declared product system is
Module C1 includes manual dismantling, with no significant
manufactured, used or handled at the end of the product´s
environmental impact.
lifespan: Europe
Module C2 comprises the transport of the dismantled VELUX
flat roof window to a sorting plant and then to a waste 3.9 Allocation
incineration plant for the thermally treated plastic fraction.
No co-products are generated during the production of the
VELUX products. Sorted production scrap of the different
Modules C3/C4: given the complexity of the inventoried
metals, notably aluminium, is considered a secondary material
products, a mixed end-of-life scenario is modelled, allowing the
with no economic value (so no burdens allocated) and
different materials to follow their most likely path.
considered in the quantification of net flows leaving the product
As a rule of thumb, metals are recycled and plastics are
system. This approach is chosen to ensure a coherent
incinerated (also due to the very limited data availability of
quantification of net flows entering module D.
plastics recycling and its benefits); coated and uncoated flat
Biogenic carbon is allocated based on physical flows
glass is assumed to be recycled whereas laminated glass is
regardless of the allocation procedure chosen for the process.
assumed to be landfilled due to very limited recycling potential.
The biogenic carbon content of wood products entering or
Metals and flat glass recycled; it is assumed that these fractions
leaving the product system is quantified (manually) as part of
reach the end-of-waste state after having been sorted and
the GWP in conformity with DIN EN 16485.
transported to a recycler; laminated glass is landfilled. The
combustible material (plastics, wood, etc.) is assumed to be
No processes were modelled as part of the foreground model
thermally treated in a municipal waste incineration plant.
that would have required an allocation of multi-input processes.
4 Environmental Product Declaration - VELUX A/S - VELUX flat roof window CVU - grid-connected
Background datasets on municipal waste incineration plants
were taken from ecoinvent without any modification. 3.10 Comparability
Basically, a comparison or an evaluation of EPD data is only
Allocation of reuse, recycling and recovery was avoided by the possible if all the data sets to be compared were created
cut-off approach in the foreground model in line with DIN EN according to EN 15804 and the building context, respectively
15804. the product-specific characteristics of performance, are taken
into account.
4. LCA: Scenarios and additional technical information
Name Value Unit
Characteristic product properties of biogenic carbon
Reference service life
according to
30 a
Information on describing the biogenic carbon content at manufacturer's
factury gate declaration
Name ValueUnit The product has passed
Declared product
kg internal quality controls and
Biogenic carbon content in product 4.57 properties (at the gate) -
C complies with EAD 220062-00-
and finishes
0401 for CE marking
Biogenic carbon content in accompanying kg
2.22
packaging C Design application
parameters (if instructed
Note: 1 kg of biogenic carbon is equivalent to 44/12 kg of CO .
2 by the manufacturer), Installation according to
including the references assembly instructions and -
to the appropriate state of the art.
practices and application
codes
An assumed quality of
Module A5
work, when installed in
The products are delivered to the construction site ready to be Carried out in accordance with
accordance with the -
installed. Manual installation is assumed, and electricity the manufacturer's instructions.
manufacturer’s
consumption related to electric drilling machines, screw drivers,
instructions
etc. is considered to be negligible.
Outdoor environment, (for The declared products are
The combustible packaging material (plastics, wood, etc.) is
outdoor applications), e.g. intended for installation outside
assumed to be transported 50 km with a lorry 16-32 metric
weathering, pollutants, UVthe building: They are therefore
tons, EURO6 to an incineration plant with an efficiency R1 < 0.6 -
and wind exposure, designed to withstand outdoor
(according to the ecoinvent dataset used); the recovered
building orientation, conditions throughout their
energy is declared as exported energy; for its quantification an
shading, temperature service life.
efficiency of 25.6 % is assumed for the production of heat and
13.0 % for the production of electricity (always referring to the Indoor environment (for
The declared products are not
lower heating value of the waste). indoor applications), e.g.
intended for installation inside -
Metals and cardboard are recycled; it is assumed that these temperature, moisture,
a building.
fractions reach the end-of-waste state after having been sorted chemical exposure
and transported (as a conservative choice) to a recycler over Usage conditions, e.g. Standard use in any type of
150 km with a lorry 16-32 metric tons, EURO6. frequency of use, building, i.e. opening/closing -
No packaging waste is landfilled. mechanical exposure as often as necessary.
The use of multi-way pallets is not taken into account as The declared products are
packaging material. designed for a reference life of
Maintenance e.g. required
30 years, with the motor
frequency, type and
Reference service life replaced every 15 years. They -
quality and replacement
are maintained by cleaning
of components
water at the discretion of the
building occupants.
Module B1
The products are assumed to have no direct emissions during
the use phase. The indicator values of Module B1 are thus 0.
For biogenic carbon stored in product, see above.
Module B2
The maintenance scenario (B2) covers the replacement of the
motor over the service life of the product. Given that the
detailed composition of the motor and its electronic
components is not known, potential loads and benefits related
to the motor and electronics are disregarded.
Annual cleaning with water (e.g., using 1 l/m2 of tap water per
annual cleaning) is neglected.
Module B6
For motor-operated flat roof windows, electricity is used both in
5 Environmental Product Declaration - VELUX A/S - VELUX flat roof window CVU - grid-connected
stand-by and during operations. Module C4
As stated above, it is assumed that 100 % of the plastic parts
Module C1 and the wooden parts are treated in a waste incineration plant
Manual de-installation is assumed, electricity consumption with an efficiency R1 < 0.6 (according to the ecoinvent dataset
related to electric screw drivers, etc. is considered to be used); 25.57 % of the lower heating value of the plastic parts
negligible. Thus, no environmental impacts are declared in are recovered as heat and 13.0 % as electricity. Recovered
module C1. energy is reported as 'exported energy' and considered in
Module D.
Module C2
Given the complexity of the inventoried products, a mixed end- Some of the material, notably laminated flat glass is assumed
of-life scenario is modelled, allowing the different materials to to be landfilled.
follow their most likely path.
Module D
It should also be noted that the deconstruction and waste Module D contains the benefits and loads beyond the system
treatment scenario can vary a lot, depending on the actual boundary related to the recycling of metals, which result from
situation. Thus, a generic end-of-life scenario is assumed. the treatment of recycled materials from the point of end-of-
waste status to the point of substitution (as loads) and the
As a rule of thumb, metals are recycled, plastics are incinerated substitution of primary resources (as benefits).
(also due to the very limited availability on plastics recycling
and its benefits); coated and uncoated flat glass is assumed to Furthermore, it includes the benefits of raw material substitution
be recycled whereas laminated glass is assumed to be of the recycling of flat glass, with the exception of laminated
landfilled due to very limited recycling potential. glass, which cannot be used for the production of glass again.
Recovered flat glass is assumed to have reached the end-of-
The combustible material (plastics, wood, etc.) is assumed to waste state as sorted glass cullet; glass cullet is assumed to
be transported 50 km with a lorry 16-32 metric tons, EURO6 to replace virgin raw material for glass production – impacts on
an incineration plant. the energy required to remelt recycled glass as compared to
virgin glass production are neglected due to a lack of data.
Metals and flat glass recycled; it is assumed that these fractions
reach the end-of-waste state after having been sorted and It also includes the benefits and loads related to the energy
transported to a recycler over 150 km with a lorry 16-32 metric recovery from plastic wastes in a MWIP as modelled in
tons, EURO6. Modules A3, A5 and C3.
Laminated glass is landfilled, including a transport of 30 km with The benefits of the recycling of the motor and electronic parts
a lorry 16-32 metric tons, EURO6. are not considered due to the absence of data on its
composition and recycled content.
Module C3
A consumption of 0.03 kWh/kg of electricity for shredding and Due to a lack of data for plastics from de-construction activities,
sorting and 0.437 MJ/kg of diesel fuel for internal logistics are the substitution potential of recycled plastics is not taken into
taken into account to disassemble the product. The recovered account.
material leaves the product system as 'materials for recycling'.
The net amounts of the metals leaving the product system are Only net flows leaving the product system are considered in
considered as 'use of secondary material' in Module D. module D.
6 Environmental Product Declaration - VELUX A/S - VELUX flat roof window CVU - grid-connected
5. LCA: Results
Disclaimer:
EP-freshwater: This indicator has been calculated as 'kg P eq' as required in the characterization model (EUTREND model, Struijs et
al., 2009b, as implemented in ReCiPe; http://eplca.jrc.ec.europa.eu/LCDN/developerEF.xhtml)
DESCRIPTION OF THE SYSTEM BOUNDARY (X = INCLUDED IN LCA; MND = MODULE OR INDICATOR NOT DECLARED; MNR
= MODULE NOT RELEVANT)
Benefits and
Construction loads beyond
Product stage Use stage End of life stage
process stage the system
boundaries
la ire ta m w a Ry lp p u s tro p s n a rT g n iru tc a fu n a M e h t m o rf tro p s n a rTe tis e h t o t e ta g y lb m e s s A e s U e c n a n e tn ia M ria p e R tn e m e c a lp e R tn e m h s ib ru fe R y g re n e la n o ita re p Oe s u re ta w la n o ita re p Oe s u n o itc u rts n o c -e Dn o itilo m e d tro p s n a rT g n is s e c o rp e ts a W la s o p s iD -e s u e R-y re v o c e R-g n ilc y c e Rla itn e to p
A1 A2 A3 A4 A5 B1 B2 B3 B4 B5 B6 B7 C1 C2 C3 C4 D
X X X MND X X X MNR MNR MNR X MND X X X X X
RESULTS OF THE LCA - ENVIRONMENTAL IMPACT according to EN 15804+A2: 1 piece VELUX flat roof window CVU - grid-
connected, 1.20 m x 1.20 m = 1.44 m2
Parameter Unit A1-A3 A5 B1 B2 B6 C1 C2 C3 C4 D
GWP-total kg CO 2 eq 4.38E+02 2.14E+01 0 1.39E+01 6.87E+02 0 1.34E+00 2.65E+00 6.46E+01 -1.93E+02
GWP-fossil kg CO 2 eq 4.7E+02 5.33E+00 0 1.39E+01 6.85E+02 0 1.34E+00 2.57E+00 4.78E+01 -1.92E+02
GWP-
biogenic kg CO 2 eq -3.28E+01 1.6E+01 0 0 0 0 0 7.8E-02 1.67E+01 0
GWP-luluc kg CO 2 eq 6.49E-01 1.92E-04 0 1.41E-02 1.71E+00 0 5.44E-04 1.99E-03 3.5E-03 -6.04E-01
ODP kg CFC11 eq 7E-05 1.08E-07 0 3.24E-06 3.47E-05 0 3.13E-07 1.12E-07 1.31E-06 -8.09E-06
AP mol H+ eq 2.39E+00 3.09E-03 0 2.25E-01 3.53E+00 0 7.58E-03 7.01E-03 4.27E-02 -1.07E+00
EP-
kg P eq 1.36E-02 3.72E-06 0 1.13E-03 7.69E-02 0 9.83E-06 2.29E-04 1.06E-04 -8.87E-03
freshwater
EP-marine kg N eq 4.58E-01 1.17E-03 0 1.89E-02 4.52E-01 0 2.72E-03 2.27E-03 1.86E-02 -1.62E-01
EP-terrestrial mol N eq 4.66E+00 1.29E-02 0 2.2E-01 5.23E+00 0 3E-02 2.57E-02 1.92E-01 -1.79E+00
kg NMVOC
POCP 1.39E+00 3.63E-03 0 7.34E-02 1.43E+00 0 8.57E-03 6.83E-03 4.7E-02 -5.33E-01
eq
ADPE kg Sb eq 8.98E+02 1.6E-06 0 4.27E-03 1.66E-03 0 4.48E-06 3.15E-06 2.85E-05 1.22E-03
ADPF MJ 4.53E+03 7.11E+00 0 1.6E+02 1.45E+04 0 2.06E+01 2.46E+01 3.99E+01 -1.95E+03
m3 world eq
WDP 1.37E+02 2.98E-02 0 6.94E+00 1.62E+02 0 6.75E-02 1.08E-01 2.09E+00 -2.21E+01
deprived
GWP = Global warming potential; ODP = Depletion potential of the stratospheric ozone layer; AP = Acidification potential of land and water; EP =
Eutrophication potential; POCP = Formation potential of tropospheric ozone photochemical oxidants; ADPE = Abiotic depletion potential for non-fossil
resources; ADPF = Abiotic depletion potential for fossil resources; WDP = Water (user) deprivation potential)
RESULTS OF THE LCA - INDICATORS TO DESCRIBE RESOURCE USE according to EN 15804+A2: 1 piece VELUX flat roof
window CVU - grid-connected, 1.20 m x 1.20 m = 1.44 m2
Parameter Unit A1-A3 A5 B1 B2 B6 C1 C2 C3 C4 D
PERE MJ 3.44E+02 1.1E-01 0 1.53E+01 2.75E+03 0 2.91E-01 3.09E+00 1.82E+02 -2.3E+02
PERM MJ 3.64E+02 -1.84E+02 0 -2.22E-16 0 0 0 -1.01E+00 -1.79E+02 0
PERT MJ 7.08E+02 -1.84E+02 0 1.72E+01 2.75E+03 0 2.91E-01 2.09E+00 3.18E+00 -2.3E+02
PENRE MJ 5.62E+03 6.95E+01 0 1.59E+02 1.46E+04 0 2.06E+01 2.04E-05 5.24E+02 -1.96E+03
PENRM MJ 5.46E+02 -6.24E+01 0 0 0 0 0 0 -4.84E+02 0
PENRT MJ 6.17E+03 7.11E+00 0 1.59E+02 1.46E+04 0 2.06E+01 2.04E-05 3.99E+01 -1.96E+03
SM kg 2.67E+01 0 0 1.4E+00 0 0 0 0 0 -1.22E+00
RSF MJ 0 0 0 0 0 0 0 0 0 0
NRSF MJ 0 0 0 0 0 0 0 0 0 0
FW m3 3.99E+00 1.56E-03 0 1.57E-01 9.35E+00 0 2.24E-03 6.49E-03 7.01E-02 -1.12E+00
PERE = Use of renewable primary energy excluding renewable primary energy resources used as raw materials; PERM = Use of renewable primary
energy resources used as raw materials; PERT = Total use of renewable primary energy resources; PENRE = Use of non-renewable primary energy
excluding non-renewable primary energy resources used as raw materials; PENRM = Use of non-renewable primary energy resources used as raw
materials; PENRT = Total use of non-renewable primary energy resources; SM = Use of secondary material; RSF = Use of renewable secondary fuels;
NRSF = Use of non-renewable secondary fuels; FW = Use of net fresh water
RESULTS OF THE LCA – WASTE CATEGORIES AND OUTPUT FLOWS according to EN 15804+A2:
1 piece VELUX flat roof window CVU - grid-connected, 1.20 m x 1.20 m = 1.44 m2
Parameter Unit A1-A3 A5 B1 B2 B6 C1 C2 C3 C4 D
HWD kg 5.32E-02 1.93E-05 0 5.41E-03 5.15E-03 0 5.25E-05 2.04E-05 8.07E-05 1.98E-02
NHWD kg 8.73E+01 5.39E-01 0 5.04E+00 5.46E+01 0 1.38E+00 4.92E-01 5.81E+01 -4.03E+01
7 Environmental Product Declaration - VELUX A/S - VELUX flat roof window CVU - grid-connected
RWD kg 4.55E-02 1.01E-04 0 7.09E-04 1.95E-01 0 2.97E-04 2.22E-04 3.27E-04 -6.68E-03
CRU kg 0 0 0 0 0 0 0 0 0 0
MFR kg 5.24E+00 1.09E+01 0 3.07E+00 0 0 0 4.51E+01 0 0
MER kg 0 0 0 0 0 0 0 0 0 0
EEE MJ 1.52E+01 8.11E+00 0 1.82E+00 0 0 0 0 8.62E+01 0
EET MJ 2.96E+01 1.6E+01 0 3.58E+00 0 0 0 0 1.7E+02 0
HWD = Hazardous waste disposed; NHWD = Non-hazardous waste disposed; RWD = Radioactive waste disposed; CRU = Components for re-use;
MFR = Materials for recycling; MER = Materials for energy recovery; EEE = Exported electrical energy; EET = Exported thermal energy
RESULTS OF THE LCA – additional impact categories according to EN 15804+A2-optional:
1 piece VELUX flat roof window CVU - grid-connected, 1.20 m x 1.20 m = 1.44 m2
Parameter Unit A1-A3 A5 B1 B2 B6 C1 C2 C3 C4 D
Disease
PM 2.2E-05 4.44E-08 0 1.04E-06 9.01E-06 0 1.2E-07 1.06E-07 2.75E-07 -1.23E-05
incidence
IR kBq U235 eq 1.02E+01 3.05E-02 0 3.89E-01 1.32E+02 0 8.93E-02 8.56E-02 1.52E-01 -2.57E+00
ETP-fw CTUe 1.19E+04 2.73E+01 0 1.65E+03 7.3E+03 0 1.63E+01 1.92E+01 5.04E+02 -3.44E+03
HTP-c CTUh 1.18E-06 9.25E-10 0 8.56E-08 1.95E-07 0 6.5E-10 4.55E-10 1.58E-08 -1.71E-07
HTP-nc CTUh 1.61E-05 1.24E-08 0 2.76E-06 6.34E-06 0 1.88E-08 2.33E-08 1.82E-07 -2.53E-06
SQP SQP 2.28E+03 5.98E+00 0 9.99E+01 2.23E+03 0 1.75E+01 3.5E+00 2.73E+01 -2.52E+02
PM = Potential incidence of disease due to PM emissions; IR = Potential Human exposure efficiency relative to U235; ETP-fw = Potential comparative
Toxic Unit for ecosystems; HTP-c = Potential comparative Toxic Unit for humans (cancerogenic); HTP-nc = Potential comparative Toxic Unit for humans
(not cancerogenic); SQP = Potential soil quality index
Disclaimer 1 – for the indicator 'Potential Human exposure efficiency relative to U235'.This impact category deals mainly with the
eventual impact of low dose ionizing radiation on human health of the nuclear fuel cycle. It does not consider effects due to possible
nuclear accidents, occupational exposure or radioactive waste disposal in underground facilities. Potential ionizing radiation from the
soil, radon and from some construction materials is also not measured by this indicator.
Disclaimer 2 – for the indicators 'abiotic depletion potential for non-fossil resources', 'abiotic depletion potential for fossil resources',
'water (user) deprivation potential, deprivation-weighted water consumption', 'potential comparative toxic unit for ecosystems', 'potential
comparative toxic unit for humans – cancerogenic', 'Potential comparative toxic unit for humans - not cancerogenic', 'potential soil
quality index'. The results of this environmental impact indicator shall be used with care as the uncertainties on these results are high
as there is limited experience with the indicator.
6. LCA: Interpretation
Figure 1 illustrates the relative contributions of the different
modules along the life cycle of the declared products.
one impact category to another.
Benefits and burdens beyond the system boundary (module D)
Figure 1: Relative environmental impacts of the different are in the order of 0% to 30% of the impacts over the product
life cycle stages for the flat roof window CVU - grid- life cycle (modules A1-C4). [1] The use of renewable primary
connected energy is mainly caused by the share of renewable energy in
the electricity mix, thus the production stage is the main drivers
The largest part of environmental impacts is caused during of this impact category; for the use of non-renewable primary
production (modules A1-A3) ranging from 15% to roughly energy, the operational energy (module B6) is the most
100%, and during the generation of operational energy (module impacting life cycle stage.
B2) The relative contributions of these main drivers differs from Material use of primary energy is negligible and related to
8 Environmental Product Declaration - VELUX A/S - VELUX flat roof window CVU - grid-connected
plastic parts of the product and packaging material. The wastes are mainly caused by the European electricity mix.
material use of primary energy is transferred to its energy use
when the materials containing primary energy are incinerated [1] Benefits resulting from the recycling of plastics as well as
with energy recovery. from the recycling of the electronic parts are disregarded due to
Non-hazardous waste as the quantitatively most relevant waste the lack of data on the recycling processes and related to the
flows is mainly caused during the production of the glass and detailed composition of the electronic parts.
during disposal of the product; hazardous and radio-active
7. Requisite evidence
to AltholzVO
7.1 Formaldehyde Not applicable; not tested based on applicable product
Not tested based on applicable product standard. standard. 7.4. Fire gas toxicity
Not tested based on applicable product standard. 7.5 VOC
7.2 MDI emissions
Not tested based on applicable product standard. 7.3 Not tested based on applicable product standard.
Checking of pre-treatment of substances used according
8. References
Product category rules of IBU methods.
IBU (2021) EAD 220062-00-0401
IBU (2021): General Instructions for the EPD Programme of the EAD 220062-00-0401, June 2017, rooflight with bonded or
Institut Bauen & Umwelt e.V. (General Instructions for the IBU mechanically fastened cover glass
EPD Programme). Version 2.0, Institut Bauen & Umwelt, Berlin
EN 16485
IBU (2017) DIN EN 16485:2014-07, Round and sawn timber -
IBU (2017): PCR Teil A: PCR Part A: Calculation rules for the Environmental Product Declarations - Product category rules
life cycle assessment and requirements for the project report. for wood and wood-based products for use in construction;
Version 1.8., Institut Bauen & Umwelt, Berlin. German version EN 16485:2014.
IBU (2021) ECHA-List
IBU (2021):PCR Part B: Requirements on the EPD for windows The Candidate List of substances of very high concern,
and doors. Version 2021/01, Institut Bauen & Umwelt, Berlin. available via https://echa.europa.eu/nl/-/four-newsubstances-
added-to-the-candidate-list.
Standards and legal documents
Regulation on biocidal products
EN 15804 REGULATION (EU) No 528/2012 OF THE EUROPEAN
DIN EN 15804+A2:2019, Sustainability of construction works - PARLIAMENT AND OF THE COUNCIL of 22 May 2012
Environmental product declarations - Core rules for the product concerning the making available on the market and use of
category construction products. biocidal products.
ISO 14025 Regulation (EU) Nr. 305/2011(CPR)
DIN EN ISO 14025:2006-07, Environmental labels and REGULATION (EU) No 305/2011 OF THE EUROPEAN
declarations - Type III Environmental declarations - Principles PARLIAMENT AND OF THE COUNCIL of 9 March 2011 laying
and procedures. down harmonised conditions for the marketing of construction
products and repealing Council Directive 89/106/EEC.
ISO 14044
DIN EN ISO 14044:2006-07, Environmental management - Life COUNCIL REGULATION (EU) No 333/2011
cycle assessment - Requirements and guidance (ISO COUNCIL REGULATION (EU) No 333/2011 of 31 March 2011
14044:2006); German and English versions EN ISO establishing criteria determining when certain types of scrap
14044:2006. metal cease to be waste under Directive 2008/98/EC of the
European Parliament and of the Council.
ISO 9001
DIN EN ISO 9001:2015, Quality management systems - European Waste List (Waste index)
Requirements. http://www.gesetze-im-internet.de/avv/anlage.htm
ISO 14001 Additional references
DIN EN ISO 14001:2015: Environmental management
systems - Requirements with guidance for use. Weidema et al. (2013)
Weidema, B., C. Bauer, R. Hischier, C. Mutel, T. Nemecek, J.
ISO 45001 Reinhard, C.O. Vadenbo, G. Wernet (2013): Overview and
ISO 45001:2018-03, Occupational health and safety methodology, Data quality guideline for the ecoinvent database
management systems - Requirements with guidance for use. version 3. ecoinvent report no. 1 (v3), St. Gallen, Schweiz.
EN 1873 ecoinvent 3.8
DIN EN 1873:2005, Prefabricated accessories for roofing - ecoinvent 3.8, LCA database, 12/2021. Ecoinvent centre,
Individual rooflights of plastics - Product specification and test Zürich.
9 Environmental Product Declaration - VELUX A/S - VELUX flat roof window CVU - grid-connected
Publisher
Institut Bauen und Umwelt e.V. +49 (0)30 3087748- 0
Hegelplatz 1 info@ibu-epd.com
10117 Berlin www.ibu-epd.com
Germany
Programme holder
Institut Bauen und Umwelt e.V. +49 (0)30 3087748- 0
Hegelplatz 1 info@ibu-epd.com
10117 Berlin www.ibu-epd.com
Germany
Author of the Life Cycle Assessment
Dr. Frank Werner - Umwelt & Entwicklung + 41 (0)44 241 39 06
Kammelenbergstrasse 30 frank@frankwerner.ch
9011 St. Gallen http://www.frankwerner.ch/
Switzerland
Owner of the Declaration
VELUX Group +4545164726
Ådalsvej 99 jakob.roerbech@velux.com
2970 Hørsholm www.velux.com
Denmark
10 Environmental Product Declaration - VELUX A/S - VELUX flat roof window CVU - grid-connected
