ENVIRONMENTAL PRODUCT DECLARATION
as per ISO 14025 and EN 15804+A2
Owner of the Declaration JANSEN AG
Publisher Institut Bauen und Umwelt e.V. (IBU)
Programme holder Institut Bauen und Umwelt e.V. (IBU)
Declaration number EPD-JAN-20240302-CBA1-EN
Issue date 29.11.2024
Valid to 28.11.2029
Janisol HI door width x height: 1230 mm x 2180 mm
Jansen AG
www.ibu-epd.com | https://epd-online.com
General Information
Jansen AG Janisol HI door width x height: 1230 mm x 2180
mm
Programme holder Owner of the declaration
IBU – Institut Bauen und Umwelt e.V. JANSEN AG
Hegelplatz 1 Industriestrasse 34
10117 Berlin 9463 Oberriet
Germany Switzerland
Declaration number Declared product / declared unit
EPD-JAN-20240302-CBA1-EN 1 m2 Jansen Janisol HI with a grammage of 55.67 kg/m². The actual
reference size of the declared single leaf door has dimensions of width x
height: 1230 mm x 2180 mm.
This declaration is based on the product category rules: Scope:
Windows and doors , 01.08.2021 The environmental product declaration refers to a single leaf door type
(PCR checked and approved by the SVR) Jansen Janisol HI in specific dimension width x height. The characteristic
values used for the system components Janisol HI in the LCA are provided
by Jansen AG.
Issue date
The declared product is defined according to the profile series and product
29.11.2024
characteristics.
The location of the production site is Oberriet/ Switzerland.
Valid to
This EPD was created with the help of a semi-automatic LCA-Tool.
28.11.2029 The owner of the declaration shall be liable for the underlying information
and evidence; the IBU shall not be liable with respect to manufacturer
information, life cycle assessment data and evidences.
The EPD was created according to the specifications of EN 15804+A2. In
the following, the standard will be simplified as EN 15804.
Verification
The standard EN 15804 serves as the core PCR
Independent verification of the declaration and data according to ISO
14025:2011
Dipl.-Ing. Hans Peters internally X externally
(Chairman of Institut Bauen und Umwelt e.V.)
Florian Pronold Matthias Schulz,
(Managing Director Institut Bauen und Umwelt e.V.) (Independent verifier)
1 Environmental Product Declaration - Jansen AG - Janisol HI door width x height: 1230 mm x 2180 mm
Product
According to the CE marking, the following structural data for
Product description/Product definition the element must be stated:
Janisol HI doors, with the basic depth of 80 mm, enables the
Constructional data
use of higher glazing thickness up to 57 mm with a sash height
of up to 3000 mm. Combinations with burglar resistance, bullet Name Value Unit
resistance or emergency exits in public buildings are visually Resistance to wind load acc. to EN
4 class
identical and can be excellently integrated into the building 12210
envelope without offsets or visual losses. The insulating bars Water tightness acc. to EN 12208 9A class
have excellent physical properties, which means that the
Sound insulation class according to EN Rw 45 db
system is also suitable for passive house requirements. This -
ISO 10140 (-2;-6)
declaration describes the following element in Janisol HI:
Heat transfer coefficient acc. to DIN EN
Product: Jansen Janisol HI, single leaf door 0.74 W/(m2K)
ISO 10077-2
Face width leaf and frame: 130 mm
Basic depth: 80 mm Air permeability acc. to EN 12207 4 class
Width x height: 1230 mm x 2180 mm Classification of strength requirements
4 class
CE marking according to EN 14351-1 acc. to EN 1192
Mechanical durability acc. to EN 12400 8 class
For the placing on the market in the the European Union/ Operating forces acc. to EN 12217 2 class
European Free Trade Association EU/EFTA the CPR (EU) No.
Burglar protection class acc. to EN 1627 3 class
305/2011/ applies. The products require a declaration of
performance taking into account the harmonized product Product according to the CPR, based on an EN: Performance
standard EN 14351-1 windows and doors and a CE marking. data of the product in accordance with the declaration of
The respective national regulations apply to the use. With this performance with respect to its essential characteristics
declaration the following element is declared: according to EN 14351-1, doors. Other constructional data are
not relevant for this product.
Base materials/Ancillary materials
JANSEN Janisol HI door is made of the following materials:
• Glazing approx. 56%
• Steel approx. 28%
• Plastics and fillers approx. 13%
• Fittings <1%
• Stainless steel approx. 1%
• Aluminium approx. 2%
The percentages relate to the most frequently sold product with
an opening of 2.68 m2. The percentages stated may vary
depending on the product type and dimensions.
Does the product or at least one part product contain materials
from the ECHA candidate list of materials which are especially
problematic for approval: Substances of Very High Concern –
SVHC (date 27.06.2024) above a mass % of 0.1: no.
This product/article/at least one partial article contains other
carcinogenic, mutagenic, reprotoxic (CMR) substances in
categories 1A or 1B which are not on the candidate list,
exceeding 0.1 percentage by mass: no.
Biocide products were added to this construction product or it
has been treated with biocide products (this then concerns a
treated product as defined by the (EU) Ordinance on Biocide
Products No. 528/2012): no.
Application Reference service life
The Jansen Janisol HI door can be integrated for building According to SBR 2011 regarding the specific material
ventilation and light transmission and it meets all the characteristics of steel windows and doors, the reference
requirements of an interior or exterior wall without taking over service life is 75 years (SBR 2011). The practical service life
load-bearing functions. may well be longer. Conditions for a long service life are regular
maintenance, care and upkeep of the product. The specified
Technical Data
service life is independent of the manufacturer's warranty.
LCA: Calculation rules
2 Environmental Product Declaration - Jansen AG - Janisol HI door width x height: 1230 mm x 2180 mm
Module C2 - considers 50 km truck transport to waste
Declared Unit processing. The transport distance can
The declared unit is a 1 m2 of Janisol HI door element. be modified project-specific if required by linear scaling.
The actual reference size of the declared door element has
dimensions of 1230 mm x 2180 mm. Modules C3 and C4 - consider waste processing and/or
disposal with the following scenarios:
Declared unit
Name Value Unit • Scenario 0: 100% thermal treatment of all raw materials
with heating value including plastic system parts and
Declared unit 1 m2
100% recycling of metal system components (C3).
Grammage 55.67 kg/m2 Landfill of all materials without heating value (except
Layer thickness 0.08 m metals) including glazing (C4). For mineral based
components (i.e. gypsum board), construction waste
Other declared units are allowed if the conversion is shown
processing (shredding) and material recycling as filling
transparently.
material (incl. benefits for substitution of gravel in
Module (D) is considered, assuming 3% recycling
For inhomogeneous components made of different materials,
losses are sent to landfill (C4).
the conversion to other dimensions with factors leads to
deviations compared to the exact calculation. The frame • Scenario 1 (module C3/1): 100% recycling of plastic
percentage is 25.495% and the ground reference is 0.098m². system parts (excluding e-waste sent to incineration)
Frame percentage = Frame surface / total area * 100 [%] and 100% recycling of metal system components.
Ground reference = Element depth x element width [m²] Landfill of all materials without heating value (except
metals) including glazing (C4/1). For mineral based
System boundary components (i.e. gypsum board), construction waste
Type of EPD according to EN 15804: "cradle to gate with processing (shredding) and material recycling as filling
options, modules C1–C4, and module D". The following material (incl. benefits for substitution of gravel in
modules are declared: A1–A3, C, D and additional modules: Module D/1) are considered, assuming 3% recycling
A4, A5 losses are sent to landfill (C4/1).
Production (modules A1-A3): Modules C4 & C4/1 are identical.
This module considers the provision of all relevant door Benefits and loads beyond the product system boundary
components (i.e. metal profiles/components, plastic (module D):
parts/profiles and glazing) and raw materials including their
transport to the declared production plant. This considers the Considers credits and loads from the recycling of the metal
manufacturing and assembly of these components, including components and mineral based components (i.e. gypsum
waste processing up to the end-of-waste state. The impact of board) as filling material (incl. benefits for the substitution of
packaging materials is also covered by this module. gravel (duplicated in D and D/1) and the recycling of the plastic
system parts/profiles (D/1). Avoided burdens from the thermal
Transport to the construction site (module A4): treatment of all raw materials with heating value (including
plastic system parts/profiles) (D) and packaging treatment
A distance of 100 km is considered for the transport of the (duplicated in D and D/1) under European conditions are
packed finished product via truck. The transport distance can considered. This affects only the rate of primary materials (no
be modified project-specific if required by linear scaling. secondary materials).
Installation (module A5): Geographic Representativeness
Land or region, in which the declared product system is
Treatment and disposal of packaging material is considered in manufactured, used or handled at the end of the product´s
this module. Credits for potential avoided burdens due to lifespan: Europe
energy substitution of electricity and thermal energy generation
are declared in module D under European conditions and
Comparability
affects only the rate of primary materials (no secondary
materials). Basically, a comparison or an evaluation of EPD data is only
possible if all the data sets to be compared were created
EoL stage (modules C1-C4): according to EN 15804 and the building context, respectively
the product-specific characteristics of performance, are taken
Module C1 - considers manual deconstruction (without into account. The following background database has been
environmental burdens). used for the LCA calculation: Sphera LCA software (GaBi ts)
content update package (CUP) version 2022.2
LCA: Scenarios and additional technical information
Name Value Unit
Characteristic product properties of biogenic carbon
kg
No biogenic carbon is reported in the product. The biogenic Biogenic carbon content in product -
C
carbon content in the accompanying packaging for 1 m2 Janisol
Biogenic carbon content in accompanying kg
HI door is declared below. 0.00858
packaging C
Information on describing the biogenic Carbon Content at
Note: 1 kg of biogenic carbon is equivalent to 44/12 kg of CO .
factory gate 2
3 Environmental Product Declaration - Jansen AG - Janisol HI door width x height: 1230 mm x 2180 mm
losses are sent to landfill (C4).
The following technical information is a basis for the declared Scenario 1 considers 100% recycling of plastic system parts
modules. The values refer to the declared unit of 1 m2 of (excluding e-waste sent to incineration) and 100% recycling of
Jansen Janisol HI door. metal system components (C3/1). Landfill of all materials
without heating value (except metals) including glazing (C4/1).
Transport to the building site (A4)
For mineral based components (i.e. gypsum board),
Name Value Unit construction waste processing (shredding) and material
Litres of fuel 0.103 l/100km recycling as filling material (incl. benefits for substitution of
Transport distance 100 km gravel in Module D/1) are considered, assuming 3% recycling
losses are sent to landfill (C4/1). Modules C4 and C4/1 are
Capacity utilisation (including empty runs) 61 %
identical. The recycling of plastics scenario declared in this
Gross weight of packed products transported 55.70 kg
EPD is currently considered a scenario that is not widely
available in reality due to economic viability limitations
Installation into the building (A5)
associated with higher costs of sorting smaller shares of
Treatment and disposal of packaging material is considered in
plastics such as those present in the declared product.
this module.
The values refer to the declared unit of 1 m2 of Janisol HI door. Name Value Unit
EoL scenario 0 (modules C3 and C4)
Name Value Unit
Recycling (C3) 17.24 kg
Polyethylene (waste packaging to incineration) 0.00185 kg
Energy recovery (C3) 3.54 kg
Cardboard box (waste packaging to incineration) 0.00885 kg
Landfilling (C4) 35.03 kg
Wood (waste packaging to incineration) 0.01167 kg
EoL scenario 1 (modules C3/1 and C4/1)
According to SBR 2011 regarding the specific material
Recycling (C3/1) 20.62 kg
characteristics of steel windows and doors, the reference
service life is 75 years (SBR 2011). The practical service life Energy recovery (C3/1) 0.16 kg
may well be longer. Conditions for a long service life are regular Landfilling (C4/1) 35.03 kg
maintenance, care and upkeep of the product. The specified
Reuse, recovery and/or recycling potentials (D), relevant
service life is independent of the manufacturer's warranty.
scenario information
Reference service life
Name Value Unit Module D includes the credits and loads from the recycling of
the metal components and mineral based components (i.e.
Life Span (according to SBR 2011) 75 a
gypsum board) as filling material (incl. benefits for substitution
End of life (C1-C4) of gravel (duplicated in D and D/1) and the recycling of the
plastic system parts/profiles (D/1). Avoided burdens from the
For the End-of-Life stage two scenarios are considered.
thermal treatment of all raw materials with heating value
Scenario 0 considers 100% thermal treatment of all raw
(including plastic system parts/profiles) (D) and packaging
materials with heating value including plastic system parts and
treatment (duplicated in D and D/1) under European conditions
100% recycling of metal system components (C3). Landfill of all
are considered. This affects only the rate of primary materials
materials without heating value (except metals) including
(no secondary materials). A waste incineration plant with R1-
glazing (C4). For mineral based components (i.e. gypsum
value > 0.6 is assumed.
board), construction waste processing (shredding) and material
For recycling, a collection rate of 100% is considered.
recycling as filling material (incl. benefits for substitution of
gravel in Module D) are considered, assuming 3% recycling
4 Environmental Product Declaration - Jansen AG - Janisol HI door width x height: 1230 mm x 2180 mm
LCA: Results
Results provided in this section are presented in relation to 1 m2 of door type Jansen Janisol HI (reference dimensions 1230 mm x
2180 mm).
For the End-of-Life stage, two scenarios are considered:
C3 - considers 100% recycling of metal system components (duplicated in D and D/1) and 100% thermal treatment of all raw materials
with heating value including plastic system parts. For mineral based components (i.e. gypsum board), construction waste processing
(shredding) and material recycling as filling material is considered.
C3/1 - considers 100% recycling of metal system components (duplicated in D and D/1) and 100% recycling of plastic system parts
(excluding e-waste sent to incineration). For mineral based components (i.e. gypsum board), construction waste processing
(shredding) and material recycling as filling material is considered.
C4 and C4/1 - consider landfill of all materials without heating value (except metals) including glazing and recycling losses from mineral
based components (i.e. gypsum board). Modules C4 and C4/1 are identical.
D - considers credits and loads from the recycling of the metal components and mineral based components (i.e. gypsum board) as
filling material (incl. benefits for the substitution of gravel (duplicated in D and D/1). Avoided burdens from packaging treatment
(duplicated in D and D/1) and thermal treatment of all raw materials with heating value (including plastic system parts/profiles) are
considered.
D/1 - considers credits and loads from the recycling of the metal components and mineral based components (i.e. gypsum board) as
filling material (incl. benefits for the substitution of gravel (duplicated in D and D/1) and the recycling of the plastic system parts/profiles.
Avoided burdens from packaging treatment (duplicated in D and D/1) are considered.
DESCRIPTION OF THE SYSTEM BOUNDARY (X = INCLUDED IN LCA; MND = MODULE OR INDICATOR NOT DECLARED; MNR
= MODULE NOT RELEVANT)
Benefits and
Construction loads beyond
Product stage Use stage End of life stage
process stage the system
boundaries
la ire ta m w a Ry lp p u s tro p s n a rT g n iru tc a fu n a M e h t m o rf tro p s n a rTe tis e h t o t e ta g y lb m e s s A e s U e c n a n e tn ia M ria p e R tn e m e c a lp e R tn e m h s ib ru fe R y g re n e la n o ita re p Oe s u re ta w la n o ita re p Oe s u n o itc u rts n o c -e Dn o itilo m e d tro p s n a rT g n is s e c o rp e ts a W la s o p s iD -e s u e R-y re v o c e R-g n ilc y c e Rla itn e to p
A1 A2 A3 A4 A5 B1 B2 B3 B4 B5 B6 B7 C1 C2 C3 C4 D
X X X X X MND MND MNR MNR MNR X MND X X X X X
RESULTS OF THE LCA - ENVIRONMENTAL IMPACT according to EN 15804+A2: 1 m2 Janisol HI door (55.67 kg/m2)
Parameter Unit A1-A3 A4 A5 B6 C1 C2 C3 C3/1 C4 C4/1 D D/1
GWP-total kg CO 2 eq 1.06E+02 3.36E-01 3.75E-02 0 0 2.61E-01 8.1E+00 1.21E-01 5.25E-01 5.25E-01 -2.29E+01 -2.37E+01
GWP-fossil kg CO 2 eq 1.05E+02 3.33E-01 6.39E-03 0 0 2.59E-01 8.1E+00 1.21E-01 5.23E-01 5.23E-01 -2.29E+01 -2.37E+01
GWP-
biogenic kg CO 2 eq 4.64E-01 1.4E-03 3.11E-02 0 0 1.09E-03 4.71E-04 3.07E-05 1.76E-03 1.76E-03 -2.87E-02 -2.08E-02
GWP-luluc kg CO 2 eq 2.96E-02 1.86E-03 1.02E-07 0 0 1.44E-03 2.58E-05 4.88E-06 9.65E-04 9.65E-04 -1.82E-03 -2.19E-03
kg CFC11
ODP 3.16E-10 2E-14 3.22E-15 0 0 1.55E-14 5.8E-13 4.49E-14 1.23E-12 1.23E-12 -2.29E-11 -1.59E-11
eq
AP mol H+ eq 4.31E-01 3.17E-04 7.02E-06 0 0 2.47E-04 3.06E-03 3.02E-05 3.71E-03 3.71E-03 -6.86E-02 -7.14E-02
EP-
kg P eq 1.3E-04 9.95E-07 8.71E-10 0 0 7.73E-07 2.11E-07 3.35E-08 8.86E-07 8.86E-07 -9.13E-06 -8.26E-06
freshwater
EP-marine kg N eq 1.27E-01 9.88E-05 2.36E-06 0 0 7.68E-05 1.4E-03 1.06E-05 9.48E-04 9.48E-04 -1.02E-02 -1.12E-02
EP-terrestrial mol N eq 1.47E+00 1.19E-03 3.26E-05 0 0 9.23E-04 1.67E-02 1.46E-04 1.04E-02 1.04E-02 -1.01E-01 -1.12E-01
kg NMVOC
POCP 3.51E-01 2.76E-04 6.34E-06 0 0 2.15E-04 3.62E-03 2.86E-05 2.88E-03 2.88E-03 -3.6E-02 -4.25E-02
eq
ADPE kg Sb eq 3.41E-04 2.79E-08 7.88E-11 0 0 2.17E-08 1.53E-08 1.05E-09 5.36E-08 5.36E-08 -2.69E-05 -2.74E-05
ADPF MJ 1.36E+03 4.45E+00 8.85E-03 0 0 3.46E+00 1.8E+00 8.3E-02 6.85E+00 6.85E+00 -2.58E+02 -3.42E+02
m3 world eq
WDP 6.68E+00 2.99E-03 4.28E-03 0 0 2.32E-03 7.67E-01 2.46E-02 5.73E-02 5.73E-02 -3.79E+00 -3.62E+00
deprived
GWP = Global warming potential; ODP = Depletion potential of the stratospheric ozone layer; AP = Acidification potential of land and water; EP =
Eutrophication potential; POCP = Formation potential of tropospheric ozone photochemical oxidants; ADPE = Abiotic depletion potential for non-fossil
resources; ADPF = Abiotic depletion potential for fossil resources; WDP = Water (user) deprivation potential)
RESULTS OF THE LCA - INDICATORS TO DESCRIBE RESOURCE USE according to EN 15804+A2: 1 m2 Janisol HI door (55.67
kg/m2)
Parameter Unit A1-A3 A4 A5 B6 C1 C2 C3 C3/1 C4 C4/1 D D/1
PERE MJ 2.23E+02 2.53E-01 3.11E-01 0 0 1.97E-01 3.59E-01 2.72E-02 1.03E+00 1.03E+00 -5.3E+01 -4.53E+01
PERM MJ 3.09E-01 0 -3.09E-01 0 0 0 0 0 0 0 0 0
PERT MJ 2.23E+02 2.53E-01 2.04E-03 0 0 1.97E-01 3.59E-01 2.72E-02 1.03E+00 1.03E+00 -5.3E+01 -4.53E+01
PENRE MJ 1.25E+03 4.46E+00 9.39E-02 0 0 3.47E+00 1.13E+02 1.11E+02 6.86E+00 6.86E+00 -2.58E+02 -3.43E+02
PENRM MJ 1.11E+02 0 -8.5E-02 0 0 0 -1.11E+02 -1.11E+02 0 0 0 0
PENRT MJ 1.36E+03 4.46E+00 8.86E-03 0 0 3.47E+00 1.8E+00 8.3E-02 6.86E+00 6.86E+00 -2.58E+02 -3.43E+02
5 Environmental Product Declaration - Jansen AG - Janisol HI door width x height: 1230 mm x 2180 mm
SM kg 9.44E+00 0 0 0 0 0 0 0 0 0 8.19E+00 9.93E+00
RSF MJ 0 0 0 0 0 0 0 0 0 0 0 0
NRSF MJ 0 0 0 0 0 0 0 0 0 0 0 0
FW m3 3.78E-01 2.86E-04 1.01E-04 0 0 2.23E-04 1.8E-02 5.55E-04 1.74E-03 1.74E-03 -1.83E-01 -1.92E-01
PERE = Use of renewable primary energy excluding renewable primary energy resources used as raw materials; PERM = Use of renewable primary
energy resources used as raw materials; PERT = Total use of renewable primary energy resources; PENRE = Use of non-renewable primary energy
excluding non-renewable primary energy resources used as raw materials; PENRM = Use of non-renewable primary energy resources used as raw
materials; PENRT = Total use of non-renewable primary energy resources; SM = Use of secondary material; RSF = Use of renewable secondary fuels;
NRSF = Use of non-renewable secondary fuels; FW = Use of net fresh water
RESULTS OF THE LCA – WASTE CATEGORIES AND OUTPUT FLOWS according to EN 15804+A2:
1 m2 Janisol HI door (55.67 kg/m2)
Parameter Unit A1-A3 A4 A5 B6 C1 C2 C3 C3/1 C4 C4/1 D D/1
HWD kg 1.5E-07 2.14E-11 8.66E-13 0 0 1.66E-11 2.16E-10 5.37E-12 3.52E-10 3.52E-10 4.84E-09 -3.09E-10
NHWD kg 6.85E+00 6.4E-04 5.68E-04 0 0 4.97E-04 1.41E-01 1.52E-02 3.51E+01 3.51E+01 -5.12E-01 -4.36E-01
RWD kg 3.53E-02 5.5E-06 5.06E-07 0 0 4.27E-06 8.48E-05 5.82E-06 7.63E-05 7.63E-05 -9.86E-03 -6.32E-03
CRU kg 0 0 0 0 0 0 0 0 0 0 0 0
MFR kg 4.66E-01 0 0 0 0 0 1.72E+01 2.06E+01 0 0 0 0
MER kg 0 0 0 0 0 0 0 0 0 0 0 0
EEE MJ 0 0 4.29E-02 0 0 0 1.33E+01 1.34E-01 0 0 0 0
EET MJ 0 0 7.68E-02 0 0 0 2.39E+01 2.79E-01 0 0 0 0
HWD = Hazardous waste disposed; NHWD = Non-hazardous waste disposed; RWD = Radioactive waste disposed; CRU = Components for re-use;
MFR = Materials for recycling; MER = Materials for energy recovery; EEE = Exported electrical energy; EET = Exported thermal energy
RESULTS OF THE LCA – additional impact categories according to EN 15804+A2-optional:
1 m2 Janisol HI door (55.67 kg/m2)
Parameter Unit A1-A3 A4 A5 B6 C1 C2 C3 C3/1 C4 C4/1 D D/1
Disease
PM 3.32E-06 1.92E-09 3.69E-11 0 0 1.49E-09 1.13E-08 7.47E-10 4.56E-08 4.56E-08 -8.01E-07 -8.14E-07
incidence
kBq U235
IR 5.31E+00 8.06E-04 8.23E-05 0 0 6.26E-04 1.34E-02 6.99E-04 8.48E-03 8.48E-03 -1.64E+00 -9.86E-01
eq
ETP-fw CTUe 2.17E+03 3.09E+00 4.07E-03 0 0 2.4E+00 7.54E-01 6.08E-02 3.84E+00 3.84E+00 -5.16E+01 -1.07E+02
HTP-c CTUh 6.9E-08 6.23E-11 2.67E-13 0 0 4.84E-11 5.29E-11 1.93E-12 5.85E-10 5.85E-10 -9.93E-09 -1.1E-08
HTP-nc CTUh 4.36E-06 3.22E-09 1E-11 0 0 2.51E-09 1.99E-09 7.34E-11 6.48E-08 6.48E-08 -2.82E-07 -3.36E-07
SQP SQP 2.64E+02 1.53E+00 2.57E-03 0 0 1.19E+00 4.37E-01 2.94E-02 1.42E+00 1.42E+00 -1.03E+01 -6.92E+00
PM = Potential incidence of disease due to PM emissions; IR = Potential Human exposure efficiency relative to U235; ETP-fw = Potential comparative
Toxic Unit for ecosystems; HTP-c = Potential comparative Toxic Unit for humans (cancerogenic); HTP-nc = Potential comparative Toxic Unit for humans
(not cancerogenic); SQP = Potential soil quality index
Disclaimer 1 – for the indicator 'Potential Human exposure efficiency relative to U235'.This impact category deals mainly with the
eventual impact of low dose ionizing radiation on human health of the nuclear fuel cycle. It does not consider effects due to possible
nuclear accidents, occupational exposure or radioactive waste disposal in underground facilities. Potential ionizing radiation from the
soil, from radon and from some construction materials is also not measured by this indicator.
Disclaimer 2 – for the indicators 'abiotic depletion potential for non-fossil resources', 'abiotic depletion potential for fossil resources',
'water (user) deprivation potential, deprivation-weighted water consumption', 'potential comparative toxic unit for ecosystems', 'potential
comparative toxic unit for humans – cancerogenic', 'Potential comparative toxic unit for humans - not cancerogenic', 'potential soil
quality index'. The results of this environmental impact indicator shall be used with care as the uncertainties on these results are high
as there is limited experience with the indicator. This EPD was created using a software tool.
References
Standards procedures.
EN 14351-1 EN 12210
EN 14351-1:2016, Windows and doors - Product standard, EN 12210: 2016 Windows and doors - Resistance to wind
performance characteristics - Part 1: windows and external loads - classification
pedestrian doorsets
EN 12208
EN 16034 DIN EN 12208 Windows and doors - Watertightness -
EN 16034:2014, pedestrian doorsets, industrial, commercial, Classification
garage doors and openable windows - Product standard,
performance characteristics - Fire resistance and/or smoke EN ISO 10140
control characteristics EN ISO 10140-1: 2021 Acoustics - Laboratory measurement of
sound insulation of building elements - Part 1: Application
EN 15804 rulesfor specific products
EN 15804:2012+A2:2019+AC:2021, Sustainability of
construction works — Environmental Product Declarations — DIN EN ISO 10077-2
Core rules for the product category of construction products. DIN EN ISO 10077-2: 2017 Thermal performance of windows,
doors and shutters - Calculation of thermal transmittance -
ISO 14025 Part2: Numerical method for frames
EN ISO 14025:2011, Environmental labels and declarations —
Type III environmental declarations — Principles and EN 12207
6 Environmental Product Declaration - Jansen AG - Janisol HI door width x height: 1230 mm x 2180 mm
EN 12207: 2016 Windows and doors - Air permeability - EUROPEANPARLIAMENT AND OF THE COUNCIL, of 22 May
Classification 2012, concerning the making available on the market and use
of biocidal products
EN 1192
EN 1192: 2000 Doors - Classification of strength requirements SBR 2011
SBR life cycle guide [SBR 2011]
EN 1191
EN 1191: 2012 Windows and doors - Resistance to repeated Further References
opening and closing - Test method
Sphera LCA FE Software (GaBi ts)
EN 1603 GaBi ts dataset documentation for the software-system and
DIN EN 1603:2013-05 Thermal insulating products for building databases, LBP, University of Stuttgart and thinkstep,
applications - Determination of dimensional stability under Leinfelden-Echterdingen, 2023 (https://www.gabi-
constant normal laboratory conditions software.com/support/gabi)
EN 13115 Sphera LCA Calculator Software (GaBi Envision)
EN 13115: 2020 Windows - Classification of mechanical GaBi Envision 5.0 Sphera Solution GmbH, the LCA, EPD and
properties - Racking, torsion and operating forces. Ecodesign tool, http://www.gabi-
software.com/international/software/gabi-envision/, 2022
DIN EN 1634-1
DIN EN 1634-1 Fire resistance and smoke control tests for door
and shutter assemblies, openable windows and elements of
building hardware - Part 1: Fire resistance test for door and Jansen LCA tool
shutter assemblies and openable windows LCA tool for façades, windows & door
LCA-Tool No.: IBU-JAN-202301-LT1-EN
Developed by Sphera Solutions GmbH
EN 13501-2
EN 13501-2: 2021 Fire classification of construction products IBU 2021
and building elements - Part 2: Classification using data from Institut Bauen und Umwelt e.V.: General Instructions for the
fire resistance and/or smoke control tests, excluding ventilation EPD programme of Institut Bauen und Umwelt e.V., Version
services 2.0, Berlin: Institut Bauen und Umwelt e.V., 2021
EN 1627 www.ibu-epd.com
DIN EN 1627:2011-09 Pedestrian doorsets, windows, curtain
walling, grilles and shutters - Burglar resistance - Requirements PCR Part A
and classification PCR - Part A: Calculation rules for the Life Cycle Assessment
and Requirements on the Background Report, version 1.3,
ECHA candidate list Institut Bauen und Umwelt e.V., 08-2021.
ECHA candidate list [BSJ1] - Substances of Very High
Concern– SVHC (date 27.06.2024)
Candidate List of substances of very high concern for PCR Part B
Authorisation (published in accordance with Article 59(10) ofthe PCR – Part B: Requirements on the EPD for Windows and
REACH Regulation)REGULATION (EU) No doors, version 1.6, Institut Bauen und Umwelt e.V., 2022
528/2012REGULATION (EU) No 528/2012 OF THE
7 Environmental Product Declaration - Jansen AG - Janisol HI door width x height: 1230 mm x 2180 mm
Publisher
Institut Bauen und Umwelt e.V. +49 (0)30 3087748- 0
Hegelplatz 1 info@ibu-epd.com
10117 Berlin www.ibu-epd.com
Germany
Programme holder
Institut Bauen und Umwelt e.V. +49 (0)30 3087748- 0
Hegelplatz 1 info@ibu-epd.com
10117 Berlin www.ibu-epd.com
Germany
Author of the Life Cycle Assessment
Sphera Solutions GmbH +49 (0)711 341817-0
Hauptstraße 111- 113 info@sphera.com
70771 Leinfelden-Echterdingen www.sphera.com
Germany
Owner of the Declaration
JANSEN AG 0041717639113
Industriestrasse 34 sustainability@jansen.com
9463 Oberriet www.jansen.com
Switzerland
8 Environmental Product Declaration - Jansen AG - Janisol HI door width x height: 1230 mm x 2180 mm
