ENVIRONMENTAL PRODUCT DECLARATION
as per ISO 14025 and EN 15804+A2
Owner of the Declaration European Association for Panels and Profiles e. V. (PPA-Europe)
Publisher Institut Bauen und Umwelt e.V. (IBU)
Programme holder Institut Bauen und Umwelt e.V. (IBU)
Declaration number EPD-PPA-20240127-CBG2-EN
Issue date 19.07.2024
Valid to 18.07.2029
Double skin steel faced sandwich panels with a core made of
mineral wool
PPA-Europe
www.ibu-epd.com | https://epd-online.com
General Information
PPA-Europe Double skin steel faced sandwich panels with a
core made of mineral wool
Programme holder Owner of the declaration
IBU – Institut Bauen und Umwelt e.V. European Association for Panels and Profiles e. V. (PPA-Europe)
Hegelplatz 1 Europark Fichtenhain A 13a
10117 Berlin 47807 Krefeld
Germany Germany
Declaration number Declared product / declared unit
EPD-PPA-20240127-CBG2-EN 1 m² prefabricated double skin steel faced sandwich panels with an
insulating core made of mineral wool
This declaration is based on the product category rules: Scope:
Double skin metal faced sandwich panels, 01.08.2021 This document is an association EPD for 1 m² of MW Core sandwich panel
(PCR checked and approved by the SVR) with 100 mm thickness and it represents an average EPD, based on
vertical averaging of the specific producer datasets under consideration of
the yearly production amounts. Its applicability is limited to continuously
Issue date produced double skin steel faced sandwich panels with an insulating core
made of mineral wool, which are manufactured by member companies of
19.07.2024
the European Association for Panels and Profiles.
The following member companies of the European Association for Panels
Valid to
and Profiles have provided data for the year 2022:
18.07.2029
1. ArcelorMittal Group, Construction Division
• ArcelorMittal Construction Austria
• ArcelorMittal Construction Belgium
• Pflaum & Söhne Bausysteme
2. Assan Panel Sanayi ve Ticaret
3. Brucha
4. Huurre Iberica
5. ISOCAB France (Kingspan Group)
6. Isolpack
7. Joris Ide Belgium (Joris Ide Group)
8. Metecno Bausysteme
Dipl.-Ing. Hans Peters 9. PAGOUNI
(Chairman of Institut Bauen und Umwelt e.V.) 10. Trimo.
These companies are representative for the European production of steel
faced sandwich panels with mineral wool core.
This EPD comprises an annex which includes LCA results for two
additional sandwich panel thicknesses: 50 mm and 200 mm. Additionally,
the EPD annex contains LCA results for 1 kg steel sheet used for the panel
faces and 1 m³ mineral wool (MW) used for the panel core, which allows
the combination and estimation of LCA results for different panel
variations.
The owner of the declaration shall be liable for the underlying information
and evidence; the IBU shall not be liable with respect to manufacturer
information, life cycle assessment data and evidences.
The EPD was created according to the specifications of EN 15804+A2. In
the following, the standard will be simplified as EN 15804.
Verification
The standard EN 15804 serves as the core PCR
Independent verification of the declaration and data according to ISO
14025:2011
internally X externally
Florian Pronold Mr Olivier Muller,
(Managing Director Institut Bauen und Umwelt e.V.) (Independent verifier)
1 Environmental Product Declaration - PPA-Europe - Double skin steel faced sandwich panels with a core made of mineral wool
Product
Product description/Product definition Base materials/Ancillary materials
The EPD applies to prefabricated double-skin steel faced Composition of the sandwich panels:
sandwich panels with a core made of mineral wool, which are
produced by member companies of PPA-Europe.
The profiled internal and external faces are made of a core of
steel, which is protected against corrosion with zinc and organic
coatings. The thermal insulating core material is made of
mineral wool according to EN 13162 with sealing tapes. The
core is bonded with adhesive to the steel sheets on both sides,
to ensure a certain resistance to shear forces of the panel.
The LCA is based on vertical averaging of the specific producer
datasets under
consideration of the respective yearly production amounts. For
the placing of the product on the market in the European
Union/European Free Trade Association (EU/EFTA) (with the Steel sheet according to EN 10346:
exception of Switzerland), CPR applies. The product needs a S280 GD to S350 GD
Declaration of Performance taking into consideration EN 14509
and the CE-marking. The data listed in the Declaration of Metallic coating according to EN 10346:
Performance apply. Zinc Z275, coating 275 g/m²
The zinc layer has a content of at least 99 weight percent zinc
For the application and use, the respective national provisions and typical thickness of 20 μm.
apply.
Organic coating according to EN 10169:
Application
Polyester (SP), coil coating, 25 μm on the application side and
The products are used for self-supporting and structural max. 15 μm on the backside.
applications in roof, wall and ceiling structures.
Thermal insulation core according to EN 13162:
Sandwich panels in wall and roof applications take on tasks of Mineral wool
the building physics, especially sound, heat and moisture The thermal insulating core is bonded with an organic adhesive
safety. They simultaneously perform the function of air tightness between the steel sheets.
of the building envelope.
The panels contain sealing tapes (amount on total weight < 0.1
Technical Data
%).
Technical specifications for sandwich panels with a core made
of mineral wool are:
The product does not contain any SVHCs (Substances of Very
• EN 14509 High Concern) REACH.
• EN 13162
Reference service life
Constructional Data
Double-skin steel faced sandwich panels used in lightweight
Name Value Unit metal constructions must withstand a term of protection of at
100 - least 15 years. The term of protection is the period until first
Density of the insulation kg/m3
130 slight renewals in the surface are required, only if there is no
Thickness of the element , when the outer layers need of frequent inspections and service.
are flat, this is the overall height of the element
100 mm
(D); on heavily profiled elements, this is the The term of protection depends on the location, weather
continuous core thickness without profile (dc) conditions and the quality of the coating.
Thickness of the inner layer 0.5 mm
Double-skin steel faced sandwich panels exhibit an estimated
Weight 21.37 kg/m²
service life of 50 years depending on the use conditions.
Thickness of the outer layer 0.6 mm
Performance data of the product in accordance with the The information in this section does not refer to a reference
declaration of performance with respect to its essential service life according to ISO 15686.
characteristics according to EN 14509
LCA: Calculation rules
Name Value Unit
Declared Unit
Declared unit 1 m2
The declared unit is 1 m² of sandwich panel. The averaging is
done based on the yearly production volume per company. Conversion factor to 1 kg (kg/m²) 0.047 -
Grammage of the panel (total value) 21.37 kg/m2
Declared unit
Layer thickness 0,1 m
2 Environmental Product Declaration - PPA-Europe - Double skin steel faced sandwich panels with a core made of mineral wool
Module D: Potential benefits for substitution processes or
System boundary recycling materials from A5 and C3.
Type of the EPD: cradle to gate - with options, module C1-C4
and module D (A1-A3, C, D and additional modules A4 and A5). For the end of life, it is assumed that the steel proportion is
recycled with benefits for the recycling potential declared in
Production stage (modules A1-A3) includes processes that module D.
provide materials and energy input for the system,
manufacturing and transport processes up to the factory gate, Geographic Representativeness
as well as waste processing. Land or region, in which the declared product system is
Module A4: Delivery to the construction site with a transport manufactured, used or handled at the end of the product´s
distance of 100 km. lifespan: Europe
Module A5: Disposal of transport packaging at the construction
site and energy for installation.
Comparability
Module C1: Dismantling with the use of machinery (diesel Basically, a comparison or an evaluation of EPD data is only
driven). possible if all the data sets to be compared were created
Module C2: Transport to the site of end-of-life treatment- according to EN 15804 and the building context, respectively
transport distance of 50 km . the product-specific characteristics of performance, are taken
Module C3: Metal recycling of the steel sheets. into account. LCA FE (fka GaBi) software and databases
Module C4: Disposal/landfilling of mineral wool. Sphera LCA FE were used as calculation basis.
LCA: Scenarios and additional technical information
polystyrene, polyethylene foil, cardboard and wooden pallets.
Characteristic product properties of biogenic carbon A5 covers the treatment of packaging material at the point of
Information on describing the biogenic Carbon Content at installation.
factory gate
Name ValueUnit Installation into the building (A5)
Biogenic carbon content in accompanying kg Name Value Unit
0.13
packaging C Output substances following waste treatment on
0.42 kg
site
Note: 1 kg of biogenic carbon is equivalent to 44/12 kg of CO
2
Machineries for installation - diesel driven 0.233kg/m²
Note: 1 kg of biogenic carbon is equivalent to 44/12 kg of CO .
2 End of life (C1-C4)
Name Value Unit
The following technical information is a basis for the declared Machineries for dismantling - diesel driven 0.233 kg/m²
modules. Collected separately waste type 20.69 kg
Transport to the building site (A4) Recycling 8.59 kg
Name Value Unit Energy recovery - kg
Transport distance 100 km Landfilling 12.1 kg
Capacity utilisation (including empty runs) 61 % Reuse, recovery or recycling potential (D)
Resulting potential benefits and loads for the metal recycling
Installation (A5)
are declared in module D.
The following packaging material is considered in A1-A3:
3 Environmental Product Declaration - PPA-Europe - Double skin steel faced sandwich panels with a core made of mineral wool
LCA: Results
DESCRIPTION OF THE SYSTEM BOUNDARY (X = INCLUDED IN LCA; MND = MODULE OR INDICATOR NOT DECLARED; MNR
= MODULE NOT RELEVANT)
Benefits and
Construction loads beyond
Product stage Use stage End of life stage
process stage the system
boundaries
la ire ta m w a Ry lp p u s tro p s n a rT g n iru tc a fu n a M e h t m o rf tro p s n a rTe tis e h t o t e ta g y lb m e s s A e s U e c n a n e tn ia M ria p e R tn e m e c a lp e R tn e m h s ib ru fe R y g re n e la n o ita re p Oe s u re ta w la n o ita re p Oe s u n o itc u rts n o c -e Dn o itilo m e d tro p s n a rT g n is s e c o rp e ts a W la s o p s iD -e s u e R-y re v o c e R-g n ilc y c e Rla itn e to p
A1 A2 A3 A4 A5 B1 B2 B3 B4 B5 B6 B7 C1 C2 C3 C4 D
X X X X X MND MND MNR MNR MNR MND MND X X X X X
RESULTS OF THE LCA - ENVIRONMENTAL IMPACT according to EN 15804+A2: 1 m² MW Sandwich panel 100 mm (21.37
kg/m²)
Parameter Unit A1-A3 A4 A5 C1 C2 C3 C4 D
GWP-total kg CO 2 eq 4.1E+01 1.55E-01 1.23E-01 8.26E-01 7.75E-02 0 1.83E-01 -1.54E+01
GWP-fossil kg CO 2 eq 4.03E+01 1.53E-01 7.32E-02 8.15E-01 7.65E-02 0 1.82E-01 -1.55E+01
GWP-biogenic kg CO 2 eq 6.94E-01 4.52E-04 4.97E-02 3.21E-03 2.26E-04 0 0 3.39E-02
GWP-luluc kg CO 2 eq 1.53E-02 1.42E-03 2.94E-05 7.53E-03 7.09E-04 0 5.65E-04 -7.53E-03
ODP kg CFC11 eq 6.24E-11 1.99E-14 1.19E-13 1.06E-13 9.97E-15 0 4.62E-13 5.33E-11
AP mol H+ eq 1.77E-01 1.97E-04 1.37E-04 4.77E-03 9.83E-05 0 1.29E-03 -3.49E-02
EP-freshwater kg P eq 3.84E-05 5.6E-07 4.71E-08 2.97E-06 2.8E-07 0 3.66E-07 -8.53E-07
EP-marine kg N eq 2.54E-02 6.66E-05 4.26E-05 2.33E-03 3.33E-05 0 3.33E-04 -8.8E-03
EP-terrestrial mol N eq 5.08E-01 8.02E-04 5E-04 2.58E-02 4.01E-04 0 3.66E-03 -9.76E-02
kg NMVOC
POCP 8.49E-02 1.69E-04 1.22E-04 6.19E-03 8.47E-05 0 1.01E-03 -2.85E-02
eq
ADPE kg Sb eq 6.25E-04 1.01E-08 1.18E-09 5.36E-08 5.04E-09 0 8.38E-09 7.31E-06
ADPF MJ 4.44E+02 2.09E+00 3.68E-01 1.11E+01 1.04E+00 0 2.42E+00 -1.1E+02
m3 world eq
WDP 1.7E+00 1.85E-03 1.74E-02 9.83E-03 9.26E-04 0 2E-02 2.95E-01
deprived
GWP = Global warming potential; ODP = Depletion potential of the stratospheric ozone layer; AP = Acidification potential of land and water; EP =
Eutrophication potential; POCP = Formation potential of tropospheric ozone photochemical oxidants; ADPE = Abiotic depletion potential for non-fossil
resources; ADPF = Abiotic depletion potential for fossil resources; WDP = Water (user) deprivation potential)
RESULTS OF THE LCA - INDICATORS TO DESCRIBE RESOURCE USE according to EN 15804+A2: 1 m² MW Sandwich panel
100 mm (21.37 kg/m²)
Parameter Unit A1-A3 A4 A5 C1 C2 C3 C4 D
PERE MJ 5E+01 1.52E-01 5.3E+00 8.06E-01 7.59E-02 0 3.94E-01 2.07E+01
PERM MJ 5.24E+00 0 -5.24E+00 0 0 0 0 0
PERT MJ 5.53E+01 1.52E-01 6.61E-02 8.06E-01 7.59E-02 0 3.94E-01 2.07E+01
PENRE MJ 4.29E+02 2.09E+00 4.79E+00 1.11E+01 1.05E+00 0 2.42E+00 -1.12E+02
PENRM MJ 1.66E+01 0 -4.42E+00 0 0 0 0 0
PENRT MJ 4.46E+02 2.09E+00 3.68E-01 1.11E+01 1.05E+00 0 2.42E+00 -1.12E+02
SM kg 1.74E+00 0 0 0 0 0 0 0
RSF MJ 0 0 0 0 0 0 0 0
NRSF MJ 0 0 0 0 0 0 0 0
FW m3 6.98E-02 1.66E-04 4.34E-04 8.83E-04 8.32E-05 0 6.11E-04 6.74E-04
PERE = Use of renewable primary energy excluding renewable primary energy resources used as raw materials; PERM = Use of renewable primary
energy resources used as raw materials; PERT = Total use of renewable primary energy resources; PENRE = Use of non-renewable primary energy
excluding non-renewable primary energy resources used as raw materials; PENRM = Use of non-renewable primary energy resources used as raw
materials; PENRT = Total use of non-renewable primary energy resources; SM = Use of secondary material; RSF = Use of renewable secondary fuels;
NRSF = Use of non-renewable secondary fuels; FW = Use of net fresh water
RESULTS OF THE LCA – WASTE CATEGORIES AND OUTPUT FLOWS according to EN 15804+A2:
1 m² MW Sandwich panel 100 mm (21.37 kg/m²)
Parameter Unit A1-A3 A4 A5 C1 C2 C3 C4 D
HWD kg 8.03E-06 6.49E-12 -7E-03 3.44E-11 3.24E-12 0 5.27E-11 -4.1E-10
NHWD kg 6.83E+00 3.19E-04 5.58E-01 1.7E-03 1.6E-04 0 1.21E+01 -2.11E-01
RWD kg 9.47E-03 3.92E-06 6.22E-06 2.08E-05 1.96E-06 0 2.76E-05 2.22E-03
CRU kg 0 0 0 0 0 0 0 0
MFR kg 3.35E-01 0 0 0 0 9.28E+00 0 0
MER kg 0 0 0 0 0 0 0 0
EEE MJ 0 0 1.2E-01 0 0 0 0 0
EET MJ 0 0 2.83E-01 0 0 0 0 0
4 Environmental Product Declaration - PPA-Europe - Double skin steel faced sandwich panels with a core made of mineral wool
HWD = Hazardous waste disposed; NHWD = Non-hazardous waste disposed; RWD = Radioactive waste disposed; CRU = Components for re-use;
MFR = Materials for recycling; MER = Materials for energy recovery; EEE = Exported electrical energy; EET = Exported thermal energy
RESULTS OF THE LCA – additional impact categories according to EN 15804+A2-optional:
1 m² MW Sandwich panel 100 mm (21.37 kg/m²)
Parameter Unit A1-A3 A4 A5 C1 C2 C3 C4 D
Disease
PM 1.74E-06 1.44E-09 1.43E-09 9.51E-08 7.19E-10 0 1.59E-08 -5.13E-07
incidence
IR kBq U235 eq 1.33E+00 5.85E-04 6.64E-04 3.1E-03 2.92E-04 0 3.19E-03 1.71E-01
ETP-fw CTUe 1.29E+02 1.48E+00 1.51E-01 7.87E+00 7.41E-01 0 1.32E+00 -2.21E+01
HTP-c CTUh 5.38E-08 3.03E-11 2.23E-11 1.61E-10 1.52E-11 0 2.03E-10 -2.7E-08
HTP-nc CTUh 7.28E-07 1.61E-09 1.49E-09 1.06E-08 8.07E-10 0 2.24E-08 -6.86E-08
SQP SQP 1.65E+02 8.72E-01 6.88E-02 4.63E+00 4.36E-01 0 5.88E-01 1.23E+01
PM = Potential incidence of disease due to PM emissions; IR = Potential Human exposure efficiency relative to U235; ETP-fw = Potential comparative
Toxic Unit for ecosystems; HTP-c = Potential comparative Toxic Unit for humans (cancerogenic); HTP-nc = Potential comparative Toxic Unit for humans
(not cancerogenic); SQP = Potential soil quality index
Disclaimer 1 – concerning Potential Human exposure efficiency relative to U235 (IRP) - This impact category deals mainly with the
eventual impact of low-dose ionizing radiation on human health of the nuclear fuel cycle. It does not consider effects due to possible
nuclear accidents, occupational exposure or radioactive waste disposal in underground facilities. Potential ionizing radiation from the
soil, radon and from some construction materials is also not measured by this indicator.
Disclaimer 2 – concerning (ADP-minerals&metals, ADP-fossil, WDP, ETP-fwm HTP-c, HTP-nc, SQP) - The results of this
environmental impact indicator shall be used with care as the uncertainties on these results are high as there is limited experience with
the indicator.
References
EN 10169 Double skin metal faced sandwich panels, Institut Bauen und
Continuously organic coated (coil coated) steel flat products - Umwelt e.V., www.bau-umwelt.com, v8., October 2023
Technical delivery conditions
REACH
EN 10346 Regulation (EC) No 1907/2006 of the European Parliament and
Continuously hot-dip coated steel flat products for cold of the Council of 18 December 2006 concerning the
forming - Technical delivery conditions Registration, Evaluation, Authorisation and Restriction of
Chemicals
EN 13162
Thermal insulation products for buildings - Factory made
mineral wool (MW) products - Specification
EN ISO 14044
Environmental management - Life cycle assessment -
Requirements and guidelines
EN 14509
Self-supporting double skin metal faced insulating panels -
Factory made products - Specifications
EN 15804+A2
EN 15804+A2:2019-04: Sustainability of construction works -
Environmental Product Declarations - Core rules for the product
category of construction products
CPR
REGULATION (EU) No 305/2011 OF THE EUROPEAN
PARLIAMENT AND OF THE COUNCIL of 9 March 2011 laying
down harmonised conditions for the marketing of construction
products and repealing Council Directive 89/106/EEC
LCA FE Software and Database
LCA FE software-system and CUP 2023.1 databases,
University of Stuttgart and Sphera Solutions GmbH, Leinfelden-
Echterdingen, 2023 (https://sphera.com/product-sustainability-
gabi-data-search/)
PCR - Part A
Calculation rules for the Life Cycle Assessment and
Requirements on the Background Report, v1.3, Institut Bauen
und Umwelt e.V., www.bau-umwelt.com, August 2021
PCR - Part B
5 Environmental Product Declaration - PPA-Europe - Double skin steel faced sandwich panels with a core made of mineral wool
6 Environmental Product Declaration - PPA-Europe - Double skin steel faced sandwich panels with a core made of mineral wool
Publisher
Institut Bauen und Umwelt e.V. +49 (0)30 3087748- 0
Hegelplatz 1 info@ibu-epd.com
10117 Berlin www.ibu-epd.com
Germany
Programme holder
Institut Bauen und Umwelt e.V. +49 (0)30 3087748- 0
Hegelplatz 1 info@ibu-epd.com
10117 Berlin www.ibu-epd.com
Germany
Author of the Life Cycle Assessment
Sphera Solutions GmbH +49 (0)711 341817-0
Hauptstraße 111- 113 info@sphera.com
70771 Leinfelden-Echterdingen www.sphera.com
Germany
Owner of the Declaration
European Association for Panels and Profiles e. V. +49 2151 93630-0
(PPA-Europe) info@ppa-europe.eu
Europark Fichtenhain A 13a www.ppa-europe.eu
47807 Krefeld
Germany
7 Environmental Product Declaration - PPA-Europe - Double skin steel faced sandwich panels with a core made of mineral wool
