Environmental Product Declaration (EPD)
According to ISO 14025 and EN 15804
Steel fiber:
waved(undulated),
with hooked ends,
with flattened ends.
Registration number: EPD-Kiwa-EE-169636-EN
Issue date: 23-06-2024
Valid until: 23-06-2029
Declaration owner: PJSC "STALKANAT"
Publisher: Kiwa-Ecobility Experts
Program operator: Kiwa-Ecobility Experts
Status: verified
Steel fiber: waved(undulated), with hooked ends, with flattened ends. | ReTHiNK-69636 1 / 17
Environmental Product Declaration
1 General information
Production location:PJSC " Stalkanat"
1.1 PRODUCT Address production location:Vapnyana St, 52A, 65006 Odesa, UA
Steel fiber: waved(undulated), with hooked ends, with flattened ends.
1.6 VERIFICATION OF THE DECLARATION
1.2 REGISTRATION NUMBER
The independent verification is in accordance with the ISO 14025:2011. The LCA is in
EPD-Kiwa-EE-169636-EN compliance with ISO 14040:2006 and ISO 14044:2006. The EN 15804:2012+A2:2019 serves as
the core PCR.
1.3 VALIDITY Internal External
Issue date:23-06-2024
Valid until:23-06-2029
1.4 PROGRAM OPERATOR
Kiwa-Ecobility Experts
Wattstraße 11-13
13355 Berlin Elisabeth Amat Guasch, Greenize
DE
1.7 STATEMENTS
The owner of this EPD shall be liable for the underlying information and evidence. The
programme operator Kiwa-Ecobility Experts shall not be liable with respect to
manufacturer data, life cycle assessment data and evidence.
Raoul Mancke Dr. Ronny Stadie
1.8 PRODUCT CATEGORY RULES
(Head of programme operations, Kiwa- (Verification body, Kiwa-Ecobility Experts)
Ecobility Experts) PCR A
PCR A – General Program Category Rules for Construction Products from the EPD
programme of Kiwa-Ecobility Experts; Version 2.1 (2022)
1.5 OWNER OF THE DECLARATION
PCR B
Manufacturer:PJSC "STALKANAT" Kiwa-Ecobility Experts, Berlin, 2020: PCR B – Product Category Rules for steel construction
products, Requirements on the Environmental Product Declarations for steel construction
Address:str. Vodoprovidna 16,, 65007 Odesa, UA
products; Version 2020-03-13 (draft)
E-mail:secretary@stalkanat.com.ua
Website:https://stalkanat.com.ua/
Steel fiber: waved(undulated), with hooked ends, with flattened ends. | ReTHiNK-69636 2 / 17
Environmental Product Declaration
1 General information
1.9 COMPARABILITY 1.10 CALCULATION BASIS
In principle, a comparison or assessment of the environmental impacts of different LCA method R<THiNK:Ecobility Experts | EN15804+A2
products is only possible if they have been prepared in accordance with EN 15804+A2. For
the evaluation of the comparability, the following aspects have to be considered in LCA software*:Simapro 9.1
particular: PCR used, functional or declared unit, geographical reference, the definition of Characterization method:EN 15804 +A2 Method v1.0
the system boundary, declared modules, data selection (primary or secondary data,
background database, data quality), scenarios used for use and disposal phases, and the LCA database profiles:EcoInvent version 3.6
life cycle inventory (data collection, calculation methods, allocations, validity period). PCRs Version database:v3.17 (2024-05-22)
and general program instructions of different EPD program operators may differ.
Comparability needs to be evaluated. For further guidance, see EN 15804+A2 (5.3 * Simapro is used for calculating the characterized results of the Environmental profiles
Comparability of EPD for construction products) and ISO 14025 (6.7.2 Requirements for within R<THiNK.
comparability).
1.11 LCA BACKGROUND REPORT
This EPD is generated on the basis of the LCA background report 'Steel fiber:
waved(undulated), with hooked ends, with flattened ends.' with the calculation identifier
ReTHiNK-69636.
Steel fiber: waved(undulated), with hooked ends, with flattened ends. | ReTHiNK-69636 3 / 17
Environmental Product Declaration
2 Product
2.1 PRODUCT DESCRIPTION withstands tensile forces and prevents the opening of microcracks that often form from
exposure to moisture or stress.
This EPD applies to steel fiber manufactured in accordance with EN 14889-1:2006, wavy,
2.3 REFERENCE SERVICE LIFE
with curved ends, with flattened ends with the Nominal Tensile Strength from 1150 to 2150
N/mm2, length 35-60 mm, diameter 0.7-1.20 mm, produced by PJSC "STALKANAT".
RSL PRODUCT
Steel fiber is used for structural reinforcement of concrete throughout the entire volume. It
Since the service life of steel fiber is not considered, there is no need to specify a reference
has the property of increasing the rigidity and strength of a concrete monolith. Steel fiber
service life. The generic life cycle of product can be considered as 100 years for any
is intended for industrial floors of industrial buildings, road and airfield pavements,
calculations basics.
coatings for the mining industry, wall structures, road base reinforcement, underwater
concrete structures, and slope strengthening.
USED RSL (YR) IN THIS LCA CALCULATION:
Steel fiber, compared to conventional reinforcement, eliminates the appearance of cracks 100
during the period when reinforced concrete sets. This is possible due to the fact that steel
fiber concrete is a uniformly distributed reinforcement inside a concrete structure.
2.4 TECHNICAL DATA
As a result, steel fiber concrete has a significantly longer maintenance-free service life.
In particular, the manufacturer declares the following information about the technical
characteristics of the product:
Product type according to REACH No. 1907/2006 – construction product. Fiber is not
classified as a hazardous substance. Conditions for safe storage:
Avoid moisture, acids and other factors that can cause metal corrosion. When storing and
storing, keep the original packaging.
Information on toxicological effects: the product does not have toxicological effects.
Fiber type
Nominal Tensile Nominal Nominal
Strength N/mm² Length mm equivalent
diameter, mm
With hooked ends HE 35/0,75 from 1150 to 2150 35 0,75
With hooked ends HE 50/0,70 from 1150 to 2150 50 0,7
With hooked ends HE 50/0,75 from 1150 to 2150 50 0,75
With hooked ends HE 50/0,80 from 1150 to 2150 50 0,8
2.2 APPLICATION (INTENDED USE OF THE PRODUCT) With hooked ends HE 50/0,90 from 1150 to 2150 50 0,9
With hooked ends HE 50/0,95 from 1150 to 2150 50 0,95
The use of steel fiber in a number of cases has certain advantages over traditionally
reinforced concrete. A certain amount of steel fiber (19-35 kg/m3) is evenly distributed in With hooked ends HE 50/1,0 from 1150 to 2150 50 1
the concrete mixture, resulting in a three-dimensional structure. This steel fiber structure
Steel fiber: waved(undulated), with hooked ends, with flattened ends. | ReTHiNK-69636 4 / 17
Environmental Product Declaration
2 Product
Fiber type
Nominal Tensile Nominal Nominal
Strength N/mm² Length mm equivalent
2.5 DESCRIPTION PRODUCTION PROCESS
diameter, mm
The technological process diagram for manufacturing fiber includes the following
With hooked ends HE 50/1,05 from 1150 to 2150 50 1,05 operations:
With hooked ends HE 50/1,2 from 1150 to 2150 50 1,2
- removal of scale by mechanical means from the surface of steel wire rod: hot-
With hooked ends HE 60/0,70 from 1150 to 2150 60 0,7 rolled steel has a layer of iron oxides on the surface, which must be removed before
drawing. This process is carried out on a surface preparation line installed in front of the
With hooked ends HE 60/0,75 from 1150 to 2150 60 0,75
straight-through drawing machine. The wire rod passes through steel rollers, bends on
With hooked ends HE 60/0,80 from 1150 to 2150 60 0,8 them, and scale falls off the surface of the wire rod. After descaling in the rollers, the
surface of the wire rod is treated with rotating steel brushes to remove any remaining
With hooked ends HE 60/0,85 from 1150 to 2150 60 0,85
scale. Then the wire rod is washed with water (water circulates in a closed cycle), coated in
With hooked ends HE 60/0,90 from 1150 to 2150 60 0,9 a borax solution in order to apply a lubricating layer at the drawing stage, then the wire
rod is dried with hot air using an electric hair dryer;
With hooked ends HE 60/0,95 from 1150 to 2150 60 0,95
With hooked ends HE 60/1,0 from 1150 to 2150 60 1 - first wire drawing on a straight-through drawing machine: the wire rod is
passed through several successive dies installed on the drawing machine, which leads to a
With hooked ends HE 60/1,05 from 1150 to 2150 60 1,05
reduction in the cross-section of the wire and its strengthening. To facilitate passage
With hooked ends HE 60/1,20 from 1150 to 2150 60 1,2 through the dies, powdered lubricants are used to reduce friction of the wire in the dies;
- finishing wire drawing on a drawing machine: when the wire passes through
successive dies, the cross-section is reduced to a given size, the material is strengthened;
With flattened ends FE 50/0,8 from 1150 to 2150 50 0,8
With flattened ends FE 50/1,0 from 1150 to 2150 50 1 - cutting wire into fiber with placing the fiber in cardboard boxes or
polypropylene big bags: fiber is cut from wire on cutting machines and placing it in
With flattened ends FE 50/1,2 from 1150 to 2150 50 1,2
cardboard boxes or polypropylene big bags;
packaging of boxes or polypropylene big bags with fiber on wooden pallets:
Waved (undulated) URW 50/1,0 from 1150 to 2150 50 1
boxes with fiber are placed on a pallet, wrapped with stretch film, pulled together using
Waved (undulated) URW 80/1,0 from 1150 to 2150 55 0,8
polypropylene tape and metal corners / polypropylene big bags are placed on a wooden
Waved (undulated) URW 60/1,0 from 1150 to 2150 60 1 pallet and secured with polypropylene tape to the pallet
Waved (undulated) URW 60/1,2 from 1150 to 2150 60 1,2
Steel fiber: waved(undulated), with hooked ends, with flattened ends. | ReTHiNK-69636 5 / 17
Environmental Product Declaration
3 Calculation rules
3.1 DECLARED UNIT 3.3 SCOPE OF DECLARATION AND SYSTEM BOUNDARIES
Kg This is a Cradle to gate with modules C1-C4 and module D LCA. The life cycle stages
The declared functional unit is 1 kg. included are as shown below:
(X = module included, ND = module not declared)
Reference unit: kilogram (kg)
A1 A2 A3 A4 A5 B1 B2 B3 B4 B5 B6 B7 C1 C2 C3 C4 D
3.2 CONVERSION FACTORS X X X ND ND ND ND ND ND ND ND ND X X X X X
Description Value Unit
The modules of the EN15804 contain the following:
Reference unit 1 kg
Conversion factor to 1 kg 1.000000 kg Module A1 = Raw material supply Module B5 = Refurbishment
Module A2 = Transport Module B6 = Operational energy use
Module A3 = Manufacturing Module B7 = Operational water use
Module A4 = Transport Module C1 = De-construction / Demolition
Module A5 = Construction -
Module C2 = Transport
Installation process
Module B1 = Use Module C3 = Waste Processing
Module B2 = Maintenance Module C4 = Disposal
Module D = Benefits and loads beyond the
Module B3 = Repair
product system boundaries
Module B4 = Replacement
3.4 REPRESENTATIVENESS
This EPD is representative for Steel fiber: waved(undulated), with hooked ends, with
flattened ends., a product of PJSC "STALKANAT". The results of this EPD are representative
for European Union.
3.5 CUT-OFF CRITERIA
Product Stage (A1-A3)
The production stage encompasses the transportation of raw materials, the conversion of
these raw materials(steel Purchased from the steel supplier) into the end product. This
Steel fiber: waved(undulated), with hooked ends, with flattened ends. | ReTHiNK-69636 6 / 17
Environmental Product Declaration
3 Calculation rules
phase accounts for the energy necessary for production, supplementary materials,
packaging materials, and the associated emissions. It's important to note that certain If necessary, distribution was applied to the inputs and outputs of the system based on
processes, such as wire drawing, and emissions generated therein, are excluded from physical properties (mass or volume).
consideration, as their impact is minimal, constituting less than 1% of the overall steel
There was no need to apply economic criteria.
impact. Therefore, the analysis primarily focuses on electricity consumption and input
materials.
3.6 ALLOCATION
End of life stage (C1-C4)
In accordance with the criteria of the reference standard, the system has been extended as
far as possible to avoid attributing environmental impacts to by-products of multi-unit
When the end of the life stage of the building is reached, the de-construction/demolition processes within the manufacturing process.
begins. This EPD includes de-construction/demolition (C1), the necessary transport (C2)
from the demolition site to the sorting location and distance to final disposal. The end of For determining the energy of a product, the plant's total annual energy consumption is
life stage includes the final disposal to landfill (C4), incineration (C3) and needed recycling allocated across the entire production output.
processes up to the end-of-waste point (C3). Loads and benefits of recycling, re-use and
exported energy are part of module D.
3.7 DATA COLLECTION & REFERENCE TIME PERIOD
The prescribed waste scenarios from the NMD Determination method v1.1 have been used
for the various materials in the product. 01.01.2022-01.01.2023
Benefits and Loads beyond the system boundary (Module D) 3.8 ESTIMATES AND ASSUMPTIONS
The Purschase of Steel is 20% from Arcelor Mittal and 80% from Kamet Steel.
This stage contains the potential loads and benefits of recycling and re-use of raw
materials/products. The loads contain the needed recycling processes from end-of-waste- Electricity Mix is used according to the general low voltage electricty mix of Ukraine
point up to the point-of-equivalence of the substituted primary raw material and a load for (location based approach).
secondary material that will be lost at the end-of-life stage.
To ensure the comprehensive assessment of the product's environmental impact across
The loads and benefits of recycling and reuse are included in this module. The benefits are Europe, including Ukraine, the utilization of NMD scenarios from the Netherlands in the
calculated based on the primary content and the primary equivalent. LCA background report and EPD is justified, as these scenarios are applicable and relevant
within the declared geographical scope.
In addition, the benefits of energy recovery are granted at this stage are focused only on
the packaging material. The amount of avoid energy is based on the Lower Heating Values
of the materials and the efficiencies of the incinerators as mentioned in the NMD 3.9 DATA QUALITY
Determination method v1.0 or EcoInvent 3.6 (2019)
In accordance with the criteria outlined in the "UN Environmental Global Guidance on LCA
In accordance with the criteria of the reference standard, the system has been extended as Database Development," as specified in EN 15804+A2, the data quality for all three
far as possible to avoid attributing environmental impacts to by-products of multi-unit representativeness categories—geographical, technical, and temporal—can be described
processes within the manufacturing process. as good.
Steel fiber: waved(undulated), with hooked ends, with flattened ends. | ReTHiNK-69636 7 / 17
Environmental Product Declaration
4 Scenarios and additional technical information
4.1 DE-CONSTRUCTION, DEMOLITION (C1)
No inputs are needed for the product at the de-construction / demolition phase
4.2 TRANSPORT END-OF-LIFE (C2)
The following distances and transport conveyance are assumed for transportation during
end of life for the different types of waste processing.
Waste Scenario Transport conveyance Not removed (stays in work) Landfill Incineration Recycling Re-use
[km] [km] [km] [km] [km]
Steel, reinforcement (NMD ID Lorry (Truck), unspecified (default) | market group for
0 100 150 50 0
74) (GLO)
The transport conveyance(s) used in the scenario(s) for transport during end of life has the
following characteristics.
Value and unit
Vehicle type used for transport Lorry (Truck), unspecified (default) | market group for (GLO)
Fuel type and consumption of vehicle not available
Capacity utilisation (including empty returns) 50 % (loaded up and return empty)
Bulk density of transported products inapplicable
Volume capacity utilisation factor 1
4.3 END OF LIFE (C3, C4)
The scenario(s) assumed for end of life of the product are given in the following tables.
First the assumed percentages per type of waste processing are displayed, followed by the
assumed amounts.
Waste Scenario Region Not removed (stays in work) [%] Landfill [%] Incineration [%] Recycling [%] Re-use [%]
Steel, reinforcement (NMD ID 74) NL 0 5 0 95 0
Steel fiber: waved(undulated), with hooked ends, with flattened ends. | ReTHiNK-69636 8 / 17
Environmental Product Declaration
4 Scenarios and additional technical information
Waste Scenario Not removed (stays in work) [kg] Landfill [kg] Incineration [kg] Recycling [kg] Re-use [kg]
Steel, reinforcement (NMD ID 74) 0.000 0.050 0.000 0.950 0.000
Total 0.000 0.050 0.000 0.950 0.000
4.4 BENEFITS AND LOADS BEYOND THE SYSTEM BOUNDARY (D)
The presented Benefits and loads beyond the system boundary in this EPD are based on
the following calculated Net output flows in kilograms and Energy recovery displayed in
MJ Lower Heating Value.
Waste Scenario Net output flow [kg] Energy recovery [MJ]
Steel, reinforcement (NMD ID 74) 0.714 0.000
Total 0.714 0.000
Steel fiber: waved(undulated), with hooked ends, with flattened ends. | ReTHiNK-69636 9 / 17
Environmental Product Declaration
5 Results
For the impact assessment, the characterization factors of the LCIA method EN 15804 +A2
Method v1.0 are used. Long-term emissions (>100 years) are not considered in the impact
assessment. The results of the impact assessment are only relative statements that do not
make any statements about end-points of the impact categories, exceedance of threshold
values, safety margins or risks. The following tables show the results of the indicators of the
impact assessment, of the use of resources as well as of waste and other output flows.
5.1 ENVIRONMENTAL IMPACT INDICATORS PER KILOGRAM
CORE ENVIRONMENTAL IMPACT INDICATORS EN15804+A2
Abbr. Unit A1 A2 A3 A1- C1 C2 C3 C4 D
A3
AP mol H+ eqv. 8.14E-3 2.31E-4 3.19E-3 1.16E-2 0.00E+0 4.11E-5 0.00E+0 2.50E-6 -3.92E-3
GWP-total kg CO2 eqv. 2.16E+0 2.72E-2 3.55E-1 2.54E+0 0.00E+0 7.09E-3 0.00E+0 2.64E-4 -1.01E+0
GWP-b kg CO2 eqv. -3.02E-3 1.55E-4 -1.54E-1 -1.57E-1 0.00E+0 3.27E-6 0.00E+0 5.20E-7 1.06E-2
GWP-f kg CO2 eqv. 2.16E+0 2.71E-2 5.00E-1 2.69E+0 0.00E+0 7.09E-3 0.00E+0 2.63E-4 -1.02E+0
GWP-luluc kg CO2 eqv. 8.30E-4 3.20E-5 8.99E-3 9.85E-3 0.00E+0 2.60E-6 0.00E+0 7.35E-8 7.49E-4
EP-m kg N eqv. 2.77E-3 8.09E-5 6.39E-4 3.49E-3 0.00E+0 1.45E-5 0.00E+0 8.60E-7 -7.27E-4
EP-fw kg P eqv. 6.98E-1 1.14E-6 1.88E-2 7.17E-1 0.00E+0 7.15E-8 0.00E+0 2.95E-9 -3.59E-5
EP-T mol N eqv. 1.70E-2 8.97E-4 5.82E-3 2.38E-2 0.00E+0 1.60E-4 0.00E+0 9.50E-6 -8.49E-3
ODP kg CFC 11 eqv. 9.42E-8 3.70E-9 3.15E-8 1.29E-7 0.00E+0 1.56E-9 0.00E+0 1.09E-10 -2.48E-8
kg NMVOC
POCP 8.09E-3 2.44E-4 1.62E-3 9.95E-3 0.00E+0 4.56E-5 0.00E+0 2.75E-6 -5.78E-3
eqv.
ADP-f MJ 1.88E+1 3.97E-1 7.05E+0 2.62E+1 0.00E+0 1.07E-1 0.00E+0 7.36E-3 -7.10E+0
ADP-mm kg Sb-eqv. 5.20E+0 2.17E-7 1.39E-1 5.34E+0 0.00E+0 1.80E-7 0.00E+0 2.41E-9 -6.86E-7
WDP m3 world eqv. 5.18E-1 3.51E-3 7.11E-1 1.23E+0 0.00E+0 3.82E-4 0.00E+0 3.30E-4 -1.94E-1
AP=Acidification (AP) | GWP-total=Global warming potential (GWP-total) | GWP-b=Global warming potential - Biogenic (GWP-b) | GWP-f=Global warming potential - Fossil (GWP-f) | GWP-
luluc=Global warming potential - Land use and land use change (GWP-luluc) | EP-m=Eutrophication marine (EP-m) | EP-fw=Eutrophication, freshwater (EP-fw) | EP-T=Eutrophication,
terrestrial (EP-T) | ODP=Ozone depletion (ODP) | POCP=Photochemical ozone formation - human health (POCP) | ADP-f=Resource use, fossils (ADP-f) | ADP-mm=Resource use, minerals and
metals (ADP-mm) | WDP=Water use (WDP)
Steel fiber: waved(undulated), with hooked ends, with flattened ends. | ReTHiNK-69636 10 / 17
Environmental Product Declaration
5 Results
ADDITIONAL ENVIRONMENTAL IMPACT INDICATORS EN15804+A2
Abbr. Unit A1 A2 A3 A1- C1 C2 C3 C4 D
A3
ETP-fw CTUe 5.54E+1 4.25E-1 1.25E+1 6.83E+1 0.00E+0 9.53E-2 0.00E+0 4.77E-3 -3.41E+1
PM disease incidence 1.23E-3 2.02E-9 3.30E-5 1.26E-3 0.00E+0 6.37E-10 0.00E+0 4.86E-11 -5.89E-8
HTP-c CTUh 9.96E-9 2.60E-11 1.41E-9 1.14E-8 0.00E+0 3.09E-12 0.00E+0 1.11E-13 -1.31E-10
HTP-nc CTUh 9.33E-8 4.75E-10 1.65E-8 1.10E-7 0.00E+0 1.04E-10 0.00E+0 3.39E-12 2.00E-7
IR kBq U235 eqv. 4.75E-2 2.22E-3 4.91E-2 9.87E-2 0.00E+0 4.48E-4 0.00E+0 3.02E-5 1.74E-2
SQP Pt 5.36E+0 2.73E-1 8.37E+0 1.40E+1 0.00E+0 9.27E-2 0.00E+0 1.54E-2 -1.57E+0
ETP-fw=Ecotoxicity, freshwater (ETP-fw) | PM=Particulate Matter (PM) | HTP-c=Human toxicity, cancer (HTP-c) | HTP-nc=Human toxicity, non-cancer (HTP-nc) | IR=Ionising radiation, human
health (IR) | SQP=Land use (SQP)
CLASSIFICATION OF DISCLAIMERS TO THE DECLARATION OF CORE AND ADDITIONAL ENVIRONMENTAL IMPACT INDICATORS
ILCD classification Indicator Disclaimer
Global warming potential (GWP) None
ILCD type / level 1 Depletion potential of the stratospheric ozone layer (ODP) None
Potential incidence of disease due to PM emissions (PM) None
AAcidification potential, Accumulated Exceedance (AP) None
Eutrophication potential, Fraction of nutrients reaching freshwater end compartment
None
(EP-freshwater)
Eutrophication potential, Fraction of nutrients reaching marine end compartment
ILCD type / level 2 None
(EP-marine)
Eutrophication potential, Accumulated Exceedance (EP-terrestrial) None
Formation potential of tropospheric ozone (POCP) None
Potential Human exposure efficiency relative to U235 (IRP) 1
Abiotic depletion potential for non-fossil resources (ADP-minerals&metals) 2
ILCD type / level 3
Abiotic depletion potential for fossil resources (ADP-fossil) 2
Water (user) deprivation potential, deprivation-weighted water consumption (WDP) 2
Potential Comparative Toxic Unit for ecosystems (ETP-fw) 2
Steel fiber: waved(undulated), with hooked ends, with flattened ends. | ReTHiNK-69636 11 / 17
Environmental Product Declaration
5 Results
ILCD classification Indicator Disclaimer
Potential Comparative Toxic Unit for humans (HTP-c) 2
Potential Comparative Toxic Unit for humans (HTP-nc) 2
Potential Soil quality index (SQP) 2
Disclaimer 1 – This impact category deals mainly with the eventual impact of low dose ionizing radiation on human health of the nuclear fuel cycle. It does not consider effects due to possible
nuclear accidents, occupational exposure nor due to radioactive waste disposal in underground facilities. Potential ionizing radiation from the soil, from radon and from some construction
materials is also not measured by this indicator.
Disclaimer 2 – The results of this environmental impact indicator shall be used with care as the uncertainties on these results are high or as there is limited experienced with the indicator.
5.2 INDICATORS DESCRIBING RESOURCE USE AND ENVIRONMENTAL INFORMATION BASED ON LIFE CYCLE INVENTORY (LCI)
PARAMETERS DESCRIBING RESOURCE USE
Abbr. Unit A1 A2 A3 A1- C1 C2 C3 C4 D
A3
PERE MJ 1.14E+0 3.42E-2 1.07E-2 1.18E+0 0.00E+0 1.34E-3 0.00E+0 5.95E-5 2.06E-1
PERM MJ 0.00E+0 0.00E+0 1.46E+0 1.46E+0 0.00E+0 0.00E+0 0.00E+0 0.00E+0 0.00E+0
PERT MJ 1.14E+0 3.42E-2 1.47E+0 2.64E+0 0.00E+0 1.34E-3 0.00E+0 5.95E-5 2.06E-1
PENRE MJ 2.40E+1 4.20E-1 7.35E+0 3.18E+1 0.00E+0 1.13E-1 0.00E+0 7.82E-3 -7.37E+0
PENRM MJ 0.00E+0 0.00E+0 1.16E-1 1.16E-1 0.00E+0 0.00E+0 0.00E+0 0.00E+0 0.00E+0
PENRT MJ 2.40E+1 4.20E-1 7.47E+0 3.19E+1 0.00E+0 1.13E-1 0.00E+0 7.82E-3 -7.37E+0
SM Kg 2.70E-1 0.00E+0 8.16E-3 2.78E-1 0.00E+0 0.00E+0 0.00E+0 0.00E+0 0.00E+0
RSF MJ 0.00E+0 0.00E+0 0.00E+0 0.00E+0 0.00E+0 0.00E+0 0.00E+0 0.00E+0 0.00E+0
NRSF MJ 0.00E+0 0.00E+0 0.00E+0 0.00E+0 0.00E+0 0.00E+0 0.00E+0 0.00E+0 0.00E+0
FW M3 3.85E-2 1.86E-4 1.80E-2 5.67E-2 0.00E+0 1.30E-5 0.00E+0 7.85E-6 -3.68E-3
PERE=renewable primary energy ex. raw materials | PERM=renewable primary energy used as raw materials | PERT=renewable primary energy total | PENRE=non-renewable primary energy
ex. raw materials | PENRM=non-renewable primary energy used as raw materials | PENRT=non-renewable primary energy total | SM=use of secondary material | RSF=use of renewable
secondary fuels | NRSF=use of non-renewable secondary fuels | FW=use of net fresh water
Steel fiber: waved(undulated), with hooked ends, with flattened ends. | ReTHiNK-69636 12 / 17
Environmental Product Declaration
5 Results
OTHER ENVIRONMENTAL INFORMATION DESCRIBING WASTE CATEGORIES
Abbr. Unit A1 A2 A3 A1- C1 C2 C3 C4 D
A3
HWD Kg 1.18E-4 7.70E-7 1.10E-5 1.29E-4 0.00E+0 2.71E-7 0.00E+0 1.10E-8 -1.22E-4
NHWD Kg 4.69E-1 5.35E-3 1.39E-1 6.13E-1 0.00E+0 6.78E-3 0.00E+0 5.00E-2 -9.95E-2
RWD Kg 1.69E-4 2.43E-6 4.51E-5 2.17E-4 0.00E+0 7.02E-7 0.00E+0 4.83E-8 5.99E-6
HWD=hazardous waste disposed | NHWD=non hazardous waste disposed | RWD=radioactive waste disposed
ENVIRONMENTAL INFORMATION DESCRIBING OUTPUT FLOWS
Abbr. Unit A1 A2 A3 A1- C1 C2 C3 C4 D
A3
CRU Kg 0.00E+0 0.00E+0 0.00E+0 0.00E+0 0.00E+0 0.00E+0 0.00E+0 0.00E+0 0.00E+0
MFR Kg 9.04E-5 0.00E+0 2.55E-2 2.56E-2 0.00E+0 0.00E+0 9.50E-1 0.00E+0 0.00E+0
MER Kg 0.00E+0 0.00E+0 0.00E+0 0.00E+0 0.00E+0 0.00E+0 0.00E+0 0.00E+0 0.00E+0
EET MJ 0.00E+0 0.00E+0 2.37E-2 2.37E-2 0.00E+0 0.00E+0 0.00E+0 0.00E+0 0.00E+0
EEE MJ 0.00E+0 0.00E+0 1.37E-2 1.37E-2 0.00E+0 0.00E+0 0.00E+0 0.00E+0 0.00E+0
CRU=Components for re-use | MFR=Materials for recycling | MER=Materials for energy recovery | EET=Exported Energy Thermic | EEE=Exported Energy Electric
Steel fiber: waved(undulated), with hooked ends, with flattened ends. | ReTHiNK-69636 13 / 17
Environmental Product Declaration
5 Results
5.3 INFORMATION ON BIOGENIC CARBON CONTENT PER KILOGRAM
BIOGENIC CARBON CONTENT
The following Information describes the biogenic carbon content in (the main parts of) the
product at the factory gate per kilogram:
Biogenic carbon content Amount Unit
Biogenic carbon content in the product 0 kg C
Biogenic carbon content in accompanying packaging 0.04267 kg C
UPTAKE OF BIOGENIC CARBON DIOXIDE
The following amount carbon dioxide uptake is taken into account. Related uptake and
release of carbon dioxide in downstream processes are not taken into account in this
number although they do appear in the presented results.
Uptake Biogenic Carbon dioxide Amount Unit
Packaging 0.1565 kg CO2 (biogenic)
Steel fiber: waved(undulated), with hooked ends, with flattened ends. | ReTHiNK-69636 14 / 17
Environmental Product Declaration
6 Interpretation of results
The graph illustrates the impact of various factors on the x-axis, representing different
indicator factors, while the legends denote the modules on the y-axis. With A1 having the
most impact and D having the most balancing impact. The main impact is from A1 as the
main input is Raw material and there are some small processes happening which has not
so much impact.
Steel fiber: waved(undulated), with hooked ends, with flattened ends. | ReTHiNK-69636 15 / 17
Environmental Product Declaration
7 References
ISO 14040
ISO 14040:2006-10, Environmental management - Life cycle assessment - Principles and
framework; EN ISO 14040:2006
ISO 14044
ISO 14044:2006-10, Environmental management - Life cycle assessment - Requirements
and guidelines; EN ISO 14040:2006
ISO 14025
ISO 14025:2011-10: Environmental labels and declarations — Type III environmental
declarations — Principles and procedures
EN 15804+A2
EN 15804+A2: 2019: Sustainability of construction works — Environmental Product
Declarations — Core rules for the product category of construction products
PCR A
PCR A – General Program Category Rules for Construction Products from the EPD
programme of Kiwa-Ecobility Experts; Version 2.1 (2022)
PCR B
Kiwa-Ecobility Experts, Berlin, 2020: PCR B – Product Category Rules for steel construction
products, Requirements on the Environmental Product Declarations for steel construction
products; Version 2020-03-13 (draft)
Steel fiber: waved(undulated), with hooked ends, with flattened ends. | ReTHiNK-69636 16 / 17
Environmental Product Declaration
8 Contact information
Publisher Operator Owner of declaration
Kiwa-Ecobility Experts Kiwa-Ecobility Experts PJSC "STALKANAT"
Wattstraße 11-13 Wattstraße 11-13 str. Vodoprovidna 16,
13355 Berlin, DE 13355 Berlin, DE 65007 Odesa, UA, UA
E-mail: E-mail: E-mail:
DE.Ecobility.Experts@kiwa.com DE.Ecobility.Experts@kiwa.com secretary@stalkanat.com.ua
Website: Website: Website:
https://www.kiwa.com/de/en/themes/ecobility-experts/ecobility-https://www.kiwa.com/de/en/themes/ecobility-experts/ecobility-https://stalkanat.com.ua/
experts-epd-program/ experts-epd-program/
Kiwa-Ecobility Experts is
established member of the
Steel fiber: waved(undulated), with hooked ends, with flattened ends. | ReTHiNK-69636 17 / 17
