ENVIRONMENTAL PRODUCT DECLARATION
as per ISO 14025 and EN 15804+A2
Owner of the Declaration Grundfos Holding A/S
Publisher Institut Bauen und Umwelt e.V. (IBU)
Programme holder Institut Bauen und Umwelt e.V. (IBU)
Declaration number EPD-GRU-20240019-CBA1-EN
Issue date 21.03.2024
Valid to 20.03.2029
MAGNA3 65-150 (Stainless Steel)
Grundfos Holding A/S
www.ibu-epd.com | https://epd-online.com
General Information
Grundfos Holding A/S MAGNA3 65-150 (Stainless Steel)
Programme holder Owner of the declaration
IBU – Institut Bauen und Umwelt e.V. Grundfos Holding A/S
Hegelplatz 1 Poul Due Jensens Vej 7
10117 Berlin 8850 Bjerringbro
Germany Denmark
Declaration number Declared product / declared unit
EPD-GRU-20240019-CBA1-EN 1 PCS. of MAGNA3 65-150 (Stainless Steel)
This declaration is based on the product category rules: Scope:
Pumps for liquids and liquids with solids, 01.08.2021 The declaration applies to 1 piece of MAGNA3 (Stainless Steel) pump.
(PCR checked and approved by the SVR)
The product is produced in Wahlstedt, Germany, and the life cycle
assessment is based on data collected at the production site.
Issue date
Production has been modeled using annual production data from 2021.
21.03.2024
The declaration covers MAGNA3 65-150 product.
The owner of the declaration shall be liable for the underlying information
Valid to
and evidence; the IBU shall not be liable with respect to manufacturer
20.03.2029 information, life cycle assessment data and evidences.
The EPD was created according to the specifications of EN 15804+A2. In
the following, the standard will be simplified as EN 15804.
Verification
The standard EN 15804 serves as the core PCR
Independent verification of the declaration and data according to ISO
14025:2011
internally X externally
Dipl.-Ing. Hans Peters
(Chairman of Institut Bauen und Umwelt e.V.)
Florian Pronold Mrs Kim Allbury,
(Managing Director Institut Bauen und Umwelt e.V.) (Independent verifier)
1 Environmental Product Declaration - Grundfos Holding A/S - MAGNA3 65-150 (Stainless Steel)
Product
the respective harmonised norms based on the legal provisions
Product description/Product definition above.
The Grundfos MAGNA3 circulator pumps are designed for
circulating liquids in heating systems, air conditioning and MAGNA3 pumps are not harmonised in accordance with the
cooling systems and domestic hot water systems. However, the CPR.
pump range can also be used in ground source heat pump
systems and solar heating systems.
Application
The MAGNA3 pump is a centrifugal pump powered by an For the application and use the respective national provisions
electrical motor. It has a high-performance neodymium magnet apply.
rotor which increases motor efficiency and an insulation shell to
reduce heat loss from the cast iron pump housing with threaded The pump is designed for circulating liquids in the
connections.
following systems:
The declaration covers MAGNA3 65-150 pump. For the placing
on the market in the European Union/European Free Trade · heating systems
Association (EU/EFTA) (with the exception of Switzerland) the
following legal provisions apply: · domestic hot-water systems
Machinery Directive (2006/42/EC) · air-conditioning and cooling systems
Standard used: EN 809:1998 + A1:2009. · ground-source heat-pump systems
· solar-heating systems
Radio Equipment Directive (2014/53/EU) The pump is suitable for thin, clean, non-aggressive and non-
explosive liquids, not containing solid particles or fibres that
Standards used: may attack the pump mechanically or chemically. In heating
EN 60335-1:2012/AC:2014 + A11:2014, EN 60335-2-51:2003 + systems, the water must meet the requirements of accepted
A1:2008 + A2:2012, EN 62233:2008. standards on water quality. The pumps are also suitable for
domestic hot-water systems.
EN 55014-1:2006 + A1:2009 + A2:2011, EN 55014-1:2017, EN
61000-6-2:2005, EN 61000-3-2:2014, EN 61000-3-3:2013, Technical Data
ETSI EN 301 489-1 V2.2.0, ETSI EN 301 489-17 V3.2.0. ETSI The performance data of the product according to the
EN 300 328 V2.1.1 harmonized norms, based on the harmonization provisions
above apply.
The relevant technical specifications according to the PCR Part
Electromagnetic Compatibility (EMC) Directive B are given in the table below.
(2014/30/EU)
Constructional data
Standards used: EN 55014-1:2017, EN 55014-2:2015,
Name Value Unit
Frequency 50 Hz
EN 61000-3-2:2014/2019, EN 61000-6-2:2008/2019,
Voltage 230 V
EN 61000-3-3:2013 A1:2019 Energy Efficiency Index 0,17
Flow range 42,5 m3/h
Head max 15 m
Power input 0,562 kW
RoHS Directive 2011/65/EU and 2015/863//EU
Nominal capacity 1,271 kW
Standard: EN 50581:2012. The performance data of the product according to the
harmonised norms, based on the harmonisation provisions
above apply.
Ecodesign Directive (2009/125/EC) Base materials/Ancillary materials
Commission Regulation (EC) No: 641/2009 and
Commission Regulation (EU) 622/2012
Standards used:
EN 16297-1:2012, EN 16297-2:2012, EN 16297-3:2012.
The CE marking takes into account the proof of conformity with
2 Environmental Product Declaration - Grundfos Holding A/S - MAGNA3 65-150 (Stainless Steel)
Name Value Unit and ISO 9001.
Aluminium 14,07 %
Reference service life
Ceramics 0,25 %
No use stage scenario which refers to the lifetime of the product
Copper 4,37 % is declared. However, to facilitate building calculations, an
Electronics 0,22 % estimated RSL of 10 years can be used.
Magnet Nd 0,92 % This is an EU consensus-based estimation, referenced on page
37 in Appendix 7: Lot 11 – Circulators in Buildings, prepared by
Paper 0,42 %
AEA Energy & Environment for the European Commission in
PCB 3,16 %
the context of the Eco Design Directive:
Plastics 0,31 %
Plastics, foam 1,04 % There is no definitive information on the average circulator life
Plastics GF 4,36 % available, there is consensus within the industry that it is at
least 12 years. However, this is complicated by many factors,
Rubber 0,14 %
including many being scrapped prematurely when e.g. the
Stainless steel 53,45 %
boiler they are connected to is replaced.
Steel 10,48 %
Cardboard 6,76 % From the estimated stock (140Mpa) and annual sales (14Mpa),
Plastic film 0,06 % the average lifetime of the circulator is taken as 10 years for the
purposes of this study.
TOTAL 100 %
REACH The RSL of the declared product is not directly influencing the
results in this study, as no declared use stage scenario is
dependent on the RSL; The use stage sub-module B6 is
declared per year as required by the PCR Part B.
This product/article/at least one partial article contains
substances listed in the ECHA candidate list (date: 10.06.2022)
exceeding 0.1 percentage by mass: no
The Wahlstedt production has been assessed and certified as
meeting the requirements in ISO 14001, ISO 50001, ISO 45001
LCA: Calculation rules
occur according to the polluter pays principle and the modular
Declared Unit approach of EN 15804.
The declared unit is 1 piece (pcs.) of MAGNA3 (Stainless Steel)
pump. The product includes:
Declared unit
· A1 Extraction and processing of raw materials;
Name Value Unit
Declared unit 1 pce.
· A1 Reuse of products or materials from a previous product
Mass reference 27.24 kg/pce system;
Conversion factor [Mass/Declared Unit] 27.24
· A1 Processing of secondary materials;
System boundary
· A1 Generation of electricity, steam and heat from primary
This EPD is Cradle-To-Grave. The system boundaries
energy resources, also including their extraction, refining and
transport;
of the EPD follow the modular approach in EN 15804. By
decision no. 20170712-n of the SVR, the modules B3, B4 and
· A1 Energy recovery and other recovery processes from
B5 are by default declared as "MNR" (module not relevant).
secondary fuels;
The product stage (A1-A3) comprises raw material extraction
· A2 Transportation up to the factory gate and internal transport;
and processing, transport processes as well as the
manufacturing process. The final production and assembly of
· A3 Production of ancillary materials or pre products;
the MAGNA3 pump takes place at a Grundfos manufacturing
site in Germany. However, the full supply-chain leading to the
· A3 Manufacturing of products and coproducts;
finished product at the gate is rather complex and includes a
large amount of raw materials, components and semi-finished
· A3 Manufacturing of packaging;
parts which come from both external suppliers as well as other
Grundfos production facilities.
· A1-A3 processing up to the end-of-waste state or disposal of
final residues.
The product stage is included in the study, and according to EN
15804 the system boundary with nature is set to include those
For secondary material inputs, the system boundary to the
processes that provide the material and energy inputs into the
previous system (providing the secondary material) is set where
system and the following manufacturing, transport up to the
outputs reach the end-of-waste state. The recycling of
factory gate as well as the processing any waste arising from
secondary material into new raw materials is included in the
those processes.
system boundary of this study. Waste
Wastes and losses are included in the modules where they
3 Environmental Product Declaration - Grundfos Holding A/S - MAGNA3 65-150 (Stainless Steel)
materials from production processes that are recycled without
any modification of the material's inherent characteristics are not relevant).
modelled as closed-loop within A1-A3. This is done up to the The modules include the provision and transport of all
input mass flow that was used during production. materials, products and related energy and water use, as well
as waste processing up to the end-of-waste state or disposal of
Waste for incineration arising in the product stage is accounted final residues during the use stage. They also include all
for in the module where the waste is produced. The impacts and
environmental loads from the incineration process are declared
in the module where it occurs and the electricity and heat which aspects related to the losses during the use stage (i.e.
is produced from the incineration are considered as closed-loop production, transport, and waste processing and disposal of the
within A1-A3, as described in PCR Part A, 5.5.1. The input of lost products and materials).
biogenic carbon from the production of packaging material is
inventoried in A3. As required by PCR Part A, the Generally, the geographical coverage of the datasets used
corresponding end-of-life module of the packaging material, A5, matches the actual processes taking place. Meaning, that when
is also declared and the emissions of biogenic carbon are modelling taking place in Grundfos Bjerringbro, the Danish
inventoried. electricity grid mix is used in the model and thermal energy
from natural gas. These are generally of very high quality with
The construction process stage (A4-A5) includes: very good technological, temporal and geographical
representativeness.
A4:
Contributions to operational energy use during the use stage
· Transportation from factory gate to distribution centre: (B6) comes from the electricity consumption of the product. The
annual electricity consumption is calculated by multiplying the
· Consumption of electricity, thermal energy and water at the average power input, which is based on a defined load profile,
distribution centre; with the annual running hours. For use stage (B6) European
Average electricity grid mix has been used. These values are
· Transportation from distribution centre to construction site; declared in the scenarios section.
· Wastage during distribution. The End-of-Life stage (C1-C4) includes all activities from
when the product reaches the end of its service life and no
A5: longer provides any functionality and until all materials and
components are processed for reuse/recycling or disposed of.
· Installation process;
According to EN 15804 and the PCR Part A, the end-of-life
· Transport of packaging waste to treatment site; stage includes:
· Waste treatment of packaging. · C1 deconstruction of the product from the
The packaging material does not reach the end of waste state · building, including initial on-site sorting of the
but is incinerated as waste.
According to European statistics, the average R1 value of · materials;
incineration plants is > 0.6. Therefore, it is assumed
· C2 transportation of the discarded product to a recycling site
that packaging material is treated thermally in an incineration and transportation of waste to final disposal;
plant with R1 > 0.6. The loads from the combustion process of
packaging are declared in module A5 and the resulting energy · C3 waste processing, collection of waste fractions from the
benefits in module deconstruction and waste processing of material flows intended
for reuse, recycling and energy recovery;
D, as required by the PCR Part A, 5.5.2.
· C4 waste disposal including physical pretreatment and
Use stage (B1-B7): management of the disposal site.
The use stage, related to the building fabric includes: At the end of life, the MAGNA3 pump is manually disassembled
from the piping system in which it has been installed. The
· B1, use or application of the installed product; definition of the applied end-of-life scenario in this EPD follows
the requirements in the
· B2, maintenance.
PCR Part A, 6.2 regarding complex products, with a
The use stage related to the operation of the building combination of recycling, thermal waste treatment and
landfilling. 100 % of the material is considered in the end of life
includes: scenario as required by the PCR. An overall collection rate of
90 % has been assumed.
· B6, operational energy use;
Materials from which energy is recovered in an incineration
· B7, operational water use. process with an R1-value above 0.60 are in this study included
with the environmental burdens from the incineration process
In this study, all use stage modules are assessed, though B1, inventoried in C3, the recovered energy is declared as exported
B2 and B7 are assessed to be zero. By decision no. 20170712- energy in C3
n of the SVR, the modules B3, B4 and B5 are by default
declared as "MNR" (module and the energy benefits are declared in D. This procedure is
4 Environmental Product Declaration - Grundfos Holding A/S - MAGNA3 65-150 (Stainless Steel)
according to the PCR Part A, 5.5.6. C3 includes the mechanical specific fractions and net flows are shown in the scenarios
separation of the product followed by a series of sorting steps. section.
Metal fractions are recycled and plastics, cardboard and
electronics are assumed incinerated with energy recovery. The Geographic Representativeness
residual fractions are landfilled and declared in C4. Land or region, in which the declared product system is
manufactured, used or handled at the end of the product´s
The specific amounts are shown in the scenarios section. lifespan: Germany
Beyond system boundary (D): According to EN 15804
Comparability
module D includes the reuse, recovery and/or recycling
Basically, a comparison or an evaluation of EPD data is only
potentials, expressed as net impacts and benefits. Any
possible if all the data sets to be compared were created
declared benefits and loads from net
according to EN 15804 and the building context, respectively
the product-specific characteristics of performance, are taken
flows leaving the product system that have not been allocated
into account. Software and databases used: LCA for Experts
as co-products and that have passed the end-of-waste state
10.7.1.28
are included in module D.
Schema 8007
Sphera and Ecoinvent databases
Contributions to module D comes from waste incineration
processes in A5 and C3 as well as material recycling in C3. The
LCA: Scenarios and additional technical information
Commission in the context of the Eco Design Directive.
Characteristic product properties of biogenic carbon
Reference service life
The biogenic carbon content quantifies the amount of biogenic
carbon in a construction product leaving the factory gate, and it Name Value Unit
will be separately declared for the product and for any Life Span according to the manufacturer 10 a
accompanying packaging, as required from the PCR Part A.
The carbon content of cardboard and paper is assumed to 0.46 Operational energy use (B6)
kg C. It means that 46% of paper and cardboard is assumed to Name Value Unit
be of biogenic carbon. Overall, there is an amount of weight-% Electricity consumption 2810 kWh/a
Carbon in the product leaving the factory gate and has to be
Average power input, 0,562 kW
considered.
Running hours (all groups) 5.000 h/a
Information on describing the biogenic Carbon Content at
factory gate End of life (C1-C4)
Note: 1 kg of biogenic carbon is equivalent to 44/12 kg of CO2. Name Value Unit
Name ValueUnit Collected as mixed construction waste 25,26 kg
Biogenic carbon content in accompanying kg Transportation distance (C2) 500 km
0.9
packaging C Aluminium for recycling 3,38 kg
Steel for recycling 2,51 kg
Copper for recycling 1,05 kg
Transport from the gate to the site (A4) Stainless steel for recycling 12,84 kg
Name Value Unit Plastics for incineration w/energy 1,4 kg
Litres of fuel 0,052 l/100km Electronics for incineration w/energy 0,81 kg
Transport distance 2003 km Landfilling 3,26 kg
Capacity utilisation (including empty runs) 85 %
Reuse, recovery and/or recycling potentials (D), relevant
Gross density of products transported 506 kg/m3
scenario information
Wastage during distribution 0,02 %
Name Value Unit
Installation into the building (A5) A5, incineration w/energy recov. thermal energy 8,91 MJ
A5, incineration w/energy recov. electrical energy 4,92 MJ
Name ValueUnit
C3, steel for recycling (net amounts) -0,601 kg
Packaging waste for incineration (LDPE film) 0,02 kg
C3, stainless steel for recycling (net amounts) 12,5 kg
Packaging waste for incineration
1,96 kg
(Paper/Cardboard) C3, aluminium for recycling (net amounts) -0,528 kg
C3, copper for recycling (net amounts) 0,45 kg
An estimated RSL of 10 years can be used to facilitate building
calculations. This is an EU consensus-based estimation, C3, incineration, w/ ecov. thermal energy 13,5 kg
referenced in Appendix 7: Lot 11 – Circulators in Buildings, C3, incineration, w/ energy recov. electrical energy 7,48 kg
prepared by AEA Energy & Environment for the European
5 Environmental Product Declaration - Grundfos Holding A/S - MAGNA3 65-150 (Stainless Steel)
LCA: Results
Characterization model: EN 15804 - 2012+A2 - 2019, PEF. By Decision no. 20170712-n of the IBU SVR, the modules B3, B4, B5 are
marked as MNR (module not relevant) as default. The LCA results in module B6 are given over a period of one year, according to PCR
Part B. To obtain the results from module B6 over the entire life cycle, the LCA results of module B6 must be multiplied by the
estimated RSL of 10 years.
DESCRIPTION OF THE SYSTEM BOUNDARY (X = INCLUDED IN LCA; MND = MODULE OR INDICATOR NOT DECLARED; MNR
= MODULE NOT RELEVANT)
Benefits and
Construction loads beyond
Product stage Use stage End of life stage
process stage the system
boundaries
la ire ta m w a Ry lp p u s tro p s n a rT g n iru tc a fu n a M e h t m o rf tro p s n a rTe tis e h t o t e ta g y lb m e s s A e s U e c n a n e tn ia M ria p e R tn e m e c a lp e R tn e m h s ib ru fe R y g re n e la n o ita re p Oe s u re ta w la n o ita re p Oe s u n o itc u rts n o c -e Dn o itilo m e d tro p s n a rT g n is s e c o rp e ts a W la s o p s iD -e s u e R-y re v o c e R-g n ilc y c e Rla itn e to p
A1 A2 A3 A4 A5 B1 B2 B3 B4 B5 B6 B7 C1 C2 C3 C4 D
X X X X X X X MNR MNR MNR X X X X X X X
RESULTS OF THE LCA - ENVIRONMENTAL IMPACT according to EN 15804+A2: 1PCS of MAGNA3 65-150
Parameter Unit A1 A2 A3 A4 A5 B1 B2 B6 B7 C1 C2 C3 C4 D
GWP-total kg CO 2 eq 1.55E+02 6.06E+00 7.37E-01 2.09E+00 3.18E+00 0 0 9.14E+02 0 0 8.66E-01 6.52E+00 1.6E-01 -4E+01
GWP-fossil kg CO 2 eq 1.55E+02 6.06E+00 3.95E+00 2.1E+00 4.78E-01 0 0 9.06E+02 0 0 8.71E-01 6.51E+00 1.62E-01 -3.99E+01
GWP- -3.25E
biogenic kg CO 2 eq -5.21E-02 -9.05E-03 +00 -3.07E-02 2.7E+00 0 0 7.88E+00 0 0 -1.29E-02 1.75E-02 -1.99E-03 -9.22E-02
GWP-luluc kg CO 2 eq 1.05E-01 8.79E-03 3.05E-02 1.9E-02 9.57E-05 0 0 9.85E-02 0 0 8.08E-03 2.57E-04 1.46E-04 -7.76E-03
kg CFC11
ODP 4.75E-08 4.73E-13 4.06E-09 1.08E-11 4.19E-13 0 0 1.67E-08 0 0 1.14E-13 3.8E-11 2.7E-13 -2.7E-11
eq
AP mol H+ eq 1.12E+00 1.82E-01 1.97E-02 1.26E-02 8.6E-04 0 0 1.94E+00 0 0 5.24E-03 5.16E-03 4.99E-04 -3.63E-01
EP-
kg P eq 1.56E-03 4.6E-06 6.86E-05 7.84E-06 1.56E-07 0 0 3.38E-03 0 0 3.19E-06 1.08E-05 1.86E-05 -4.07E-05
freshwater
EP-marine kg N eq 1.2E-01 4.33E-02 4.09E-03 6.02E-03 3.15E-04 0 0 4.63E-01 0 0 2.55E-03 1.33E-03 1.19E-04 -4.38E-02
EP-terrestrial mol N eq 1.3E+00 4.75E-01 4.11E-02 6.68E-02 3.95E-03 0 0 4.84E+00 0 0 2.83E-02 1.48E-02 1.31E-03 -4.73E-01
kg
POCP NMVOC 3.81E-01 1.23E-01 1.15E-02 1.15E-02 8.18E-04 0 0 1.24E+00 0 0 4.85E-03 3.55E-03 3.75E-04 -1.41E-01
eq
ADPE kg Sb eq 1.17E-02 1.09E-07 6.2E-05 2.49E-06 4.32E-09 0 0 1.4E-04 0 0 5.78E-08 3.17E-07 4.34E-09 -3.18E-03
ADPF MJ 2.13E+03 7.54E+01 5.86E+01 2.87E+01 1.16E+00 0 0 1.91E+04 0 0 1.19E+01 4.42E+01 2.42E+00 -4.28E+02
m3 world
WDP eq 4.84E+01 1.99E-02 4.97E-02 3.59E-02 3.81E-01 0 0 2.02E+02 0 0 1.05E-02 9.09E-01 -2.25E-03 -2.29E+00
deprived
GWP = Global warming potential; ODP = Depletion potential of the stratospheric ozone layer; AP = Acidification potential of land and water; EP =
Eutrophication potential; POCP = Formation potential of tropospheric ozone photochemical oxidants; ADPE = Abiotic depletion potential for non-fossil
resources; ADPF = Abiotic depletion potential for fossil resources; WDP = Water (user) deprivation potential)
RESULTS OF THE LCA - INDICATORS TO DESCRIBE RESOURCE USE according to EN 15804+A2: 1PCS of MAGNA3 65-150
Parameter Unit A1 A2 A3 A4 A5 B1 B2 B6 B7 C1 C2 C3 C4 D
PERE MJ 5.35E+02 1.21E+00 5.59E+01 2.23E+00 2.62E-01 0 0 1.14E+04 0 0 8.65E-01 2.59E+01 2.18E-01 5.87E+00
PERM MJ 0 0 0 0 0 0 0 0 0 0 0 0 0 0
PERT MJ 5.35E+02 1.21E+00 5.59E+01 2.23E+00 2.62E-01 0 0 1.14E+04 0 0 8.65E-01 2.59E+01 2.18E-01 5.87E+00
-4.27E
PENRE MJ 2.14E+03 7.56E+01 5.86E+01 2.88E+01 1.16E+00 0 0 1.91E+04 0 0 1.19E+01 4.42E+01 2.42E+00
+02
PENRM MJ 0 0 0 0 0 0 0 0 0 0 0 0 0 0
-4.27E
PENRT MJ 2.14E+03 7.56E+01 5.86E+01 2.88E+01 1.16E+00 0 0 1.91E+04 0 0 1.19E+01 4.42E+01 2.42E+00
+02
SM kg 2.17E+01 0 2.4E-01 4.38E-03 0 0 0 0 0 0 0 0 0 0
RSF MJ 1.46E-23 0 0 2.91E-27 0 0 0 0 0 0 0 0 0 0
NRSF MJ 1.71E-22 0 0 3.42E-26 0 0 0 0 0 0 0 0 0 0
FW m3 1.43E+00 1.38E-03 2.35E-02 2.57E-03 8.99E-03 0 0 9.21E+00 0 0 9.47E-04 3.14E-02 2.52E-05 6.63E-04
PERE = Use of renewable primary energy excluding renewable primary energy resources used as raw materials; PERM = Use of renewable primary
energy resources used as raw materials; PERT = Total use of renewable primary energy resources; PENRE = Use of non-renewable primary energy
excluding non-renewable primary energy resources used as raw materials; PENRM = Use of non-renewable primary energy resources used as raw
materials; PENRT = Total use of non-renewable primary energy resources; SM = Use of secondary material; RSF = Use of renewable secondary fuels;
NRSF = Use of non-renewable secondary fuels; FW = Use of net fresh water
RESULTS OF THE LCA – WASTE CATEGORIES AND OUTPUT FLOWS according to EN 15804+A2:
1PCS of MAGNA3 65-150
6 Environmental Product Declaration - Grundfos Holding A/S - MAGNA3 65-150 (Stainless Steel)
Parameter Unit A1 A2 A3 A4 A5 B1 B2 B6 B7 C1 C2 C3 C4 D
HWD kg 7.02E-06 2.37E-10 1.21E-04 2.57E-08 2.93E-11 0 0 2.24E-06 0 0 3.69E-11 5.04E-09 2.02E-10 -7.76E-03
NHWD kg 1.35E+01 7.69E-03 3.8E-01 7.3E-03 1.24E-01 0 0 1.4E+01 0 0 1.82E-03 7.07E-01 2.8E+00 3.88E+00
RWD kg 7.16E-02 9.78E-05 1.8E-03 7.3E-05 5.3E-05 0 0 3.03E+00 0 0 2.23E-05 6.86E-03 2.84E-05 -4.73E-03
CRU kg ND ND ND ND ND ND ND ND ND ND ND ND ND ND
MFR kg 0 0 0 0 0 0 0 0 0 0 0 1.97E+01 0 0
MER kg ND ND ND ND ND ND ND ND ND ND ND ND ND ND
EEE MJ 0 0 0 0 4.92E+00 0 0 0 0 0 0 7.48E+00 0 0
EET MJ 0 0 0 0 8.91E+00 0 0 0 0 0 0 1.35E+01 0 0
HWD = Hazardous waste disposed; NHWD = Non-hazardous waste disposed; RWD = Radioactive waste disposed; CRU = Components for re-use;
MFR = Materials for recycling; MER = Materials for energy recovery; EEE = Exported electrical energy; EET = Exported thermal energy
RESULTS OF THE LCA – additional impact categories according to EN 15804+A2-optional:
1PCS of MAGNA3 65-150
Parameter Unit A1 A2 A3 A4 A5 B1 B2 B6 B7 C1 C2 C3 C4 D
Disease
PM 1.44E-05 3.15E-06 2.92E-07 8.15E-08 5.09E-09 0 0 0 0 0 3.32E-08 4.37E-08 5.07E-09 -8.87E-06
incidence
kBq U235
IR 9.85E+00 1.41E-02 2.89E-01 1.08E-02 8.26E-03 0 0 0 0 0 3.33E-03 1.14E+00 4.2E-03 -3.69E-01
eq
ETP-fw CTUe 1.04E+03 5.34E+01 2.01E+01 2.02E+01 5.61E-01 0 0 0 0 0 8.51E+00 1.27E+01 1.52E+00 -5.87E+01
HTP-c CTUh 3.7E-05 9.92E-10 6.65E-07 7.94E-09 3.06E-11 0 0 0 0 0 1.73E-10 7.03E-10 9.75E-11 -1.71E-06
HTP-nc CTUh 2.33E-06 3.4E-08 4.29E-08 1.86E-08 1.15E-09 0 0 0 0 0 7.69E-09 1.4E-08 8.32E-09 -2.53E-07
SQP SQP 4.81E+02 5.55E+00 1.06E+02 1.18E+01 3.42E-01 0 0 0 0 0 4.97E+00 1.71E+01 2.16E-01 -2.55E+01
PM = Potential incidence of disease due to PM emissions; IR = Potential Human exposure efficiency relative to U235; ETP-fw = Potential comparative
Toxic Unit for ecosystems; HTP-c = Potential comparative Toxic Unit for humans (cancerogenic); HTP-nc = Potential comparative Toxic Unit for humans
(not cancerogenic); SQP = Potential soil quality index
Disclaimer 1 – for the indicator 'Potential Human exposure efficiency relative to U235'.
This impact category deals mainly with the eventual impact of low-dose ionizing radiation on human health of the nuclear fuel cycle. It
does not consider effects due to possible nuclear accidents, occupational exposure or radioactive waste disposal in underground
facilities. Potential ionizing radiation from the soil, radon and from some construction materials is also not measured by this indicator.
Disclaimer 2 – for the indicators 'abiotic depletion potential for non-fossil resources', 'abiotic depletion potential for fossil resources',
'water (user) deprivation potential, deprivation-weighted water consumption', 'potential comparative toxic unit for ecosystems', 'potential
comparative toxic unit for humans – cancerogenic', 'Potential comparative toxic unit for humans - not cancerogenic', 'potential soil
quality index'. The results of this environmental impact indicator shall be used with care as the uncertainties on these results are high
as there is limited experience with the indicator.
Disclaimer 3: JRC Technical Reports, Version 2, 2018 Page 6, for the indicator "EP-freshwater". This indicator has been calculated as
'kg P eq' as required in the characterization model EUTREND model, Struijs et al., 2009b, as implemented in ReCiPe; This EPD was
created using a software tool.
References
Standards IBU 2021
EN 15804 Institut Bauen und Umwelt e.V.: General Instructions for the
EPD programme of Institut Bauen und Umwelt e.V., Version
EN 15804:2012+A1 2013, Sustainability of construction works 2.0, Berlin: Institut Bauen und Umwelt e.V., 2021
— Environmental Product Declarations — Core rules for the www.ibu-epd.com
product category of construction products.
Standards
EN 15804
EN 15804:2012+A2:2019+AC:2021, Sustainability of Machinery Directive
construction works — Environmental Product Declarations —
Core rules for the product category of construction products. DIRECTIVE 2006/42/EC OF THE EUROPEAN PARLIAMENT
AND OF THE COUNCIL of 17 May 2006 on machinery
ISO 14025
EN ISO 14025:2011, Environmental labels and declarations — Radio Equipment Directive
Type III environmental declarations — Principles and
procedures. DIRECTIVE 2014/53/EU OF THE EUROPEAN PARLIAMENT
AND OF THE COUNCIL of 16 April 2014 on the harmonization
Further References of the laws of the Member States relating to the making
available on the market of radio equipment
Title of the software/database
Title of the software/database. Addition to the title, version. Electromagnetic Compatibility (EMC) Directive
Place: Publisher, Date of publication [Access on access date].
DIRECTIVE 2014/30/EU OF THE EUROPEAN PARLIAMENT
7 Environmental Product Declaration - Grundfos Holding A/S - MAGNA3 65-150 (Stainless Steel)
AND OF THE COUNCIL of 26 February 2014 on the
harmonistion of the laws of the Member States relating to
electromagnetic compatibility EN 55014-1
EN 55014-1:2017, Electromagnetic compatibility –
Ecodesign Directive Requirements for household appliances, electric tools and
similar apparatus – Part 1: Emission
DIRECTIVE 2009/125/EC OF THE EUROPEAN PARLIAMENT
AND OF THE COUNCIL of 21 October 2009 establishing a
framework for the setting of eco-design requirements for EN 55014-2
energy-related products
EN 55014-2:2015, Electromagnetic compatibility –
Requirements for household appliances, electric tools and
EC 641/2009 similar apparatus – Part 2: Immunity – Product family standard
(CISPR 14-2:2015)
COMMISSION REGULATION (EC) No 641/2009 of 22 July
2009 implementing Directive 2005/32/EC of the European
Parliament and of the Council with regard to eco-design EN 50581:2012
requirements for glandless standalone circulators and
glandless circulators integrated in products EN 50581:2012, Technical documentation for the assessment
of electrical and electronic products with respect to the
restriction of hazardous substances
EC 622/2012
COMMISSION REGULATION (EU) No 622/2012 of 11 July EN 60335-1
2012 amending Regulation (EC) No 641/2009 with regard to
eco-design requirements for glandless standalone circulators EN 60335-1:2012/A11:2014/A13:2017, Household and similar
and glandless circulators integrated in products electrical appliances – Safety – Part 1: General requirements
DIRECTIVE 2011/65/EU EN 60335-2-51
DIRECTIVE 2011/65/EU OF THE EUROPEAN PARLIAMENT EN 60335-2-51:2003-03 + A1:2008 + A2:2012, Household and
AND OF THE COUNCIL of 8 June 2011 on the restriction of the similar electrical appliances – Safety –Part 2-51: Particular
use of certain hazardous substances in electrical and electronic requirements for stationary circulation pumps for heating and
equipment service water installations
DIRECTIVE 2015/863/EU EN 61000-3-2
DIRECTIVE 2015/863/EU of 31 March 2015 amending Annex II EN 61000-3-2:2014/2019, Electromagnetic compatibility (EMC)
to Directive 2011/65/EU of the European Parliament and of the – Part 3-2: Limits – Limits for harmonic current emissions
Council as regards the list of restricted substances (equipment input current =16 A per phase)
ETSI EN 301 489-1 EN 61000-3-3
ETSI EN 301 489-1 V2.2.0, Electromagnetic Compatibility EN 61000-3-3:2013-08/ A1:2019, Electromagnetic compatibility
(EMC) standard for radio equipment and services; Part 1: (EMC) – Part 3-3:
Common technical requirements
Limits – Limitation of voltage changes, voltage fluctuations and
flicker in public low voltage supply systems, for equipment with
ETSI EN 301 489-17 rated current <= 16 A per phase and not subject to conditional
connection
ETSI EN 301 489-17 V3.2.0, Electromagnetic Compatibility
(EMC) standard for radio equipment and services; Part 17:
Specific conditions for Broadband Data Transmission Systems EN 61000-6-2
EN 61000-6-2:2008/2019, Electromagnetic compatibility (EMC)
ETSI EN 300 328 V2.1.1 – Part 6-2: Generic standards –Immunity for industrial
environments
ETSI EN 300 328 V2.1.1, Wideband transmission systems;
Data transmission equipment operating in the 2,4 GHz ISM
band and using wide band modulation techniques EN 16297-1
EN 16297-1:2012-10, Pumps – Rotodynamic pumps –
EN 809 Glandless circulators – Part 1:
EN 809:1998-10 + A1:2009, Pumps and pump units for liquids - General requirements and procedures for testing and
Common safety requirements calculation of energy efficiency index (EEI)
8 Environmental Product Declaration - Grundfos Holding A/S - MAGNA3 65-150 (Stainless Steel)
CPR
EN 16297-2
REGULATION (EU) No 305/2011 OF THE EUROPEAN
EN 16297-2:2012-10, Pumps – Rotodynamic pumps – PARLIAMENT AND OF THE COUNCIL of 9 March 2011 laying
Glandless circulators – Part 2: Calculation of energy efficiency down harmonized conditions for the marketing of construction
index (EEI) for standalone circulators products and repealing Council Directive 89/106/EEC
EN 16297-3 CML 2001
EN 16297-3:2012, Pumps – Rotodynamic pumps –Glandless Impact assessment characterization factors Institute of
circulators – Part 3: Energy efficiency index (EEI) for circulators Environmental Sciences, Leiden University, Netherlands
integrated in products
ECHA candidate list
ISO 14001 Candidate List of substances of very high concern (SVHCs) for
authorization, European Chemicals Agency (ECHA), Helsinki,
EN ISO 14001:2015-09, Environmental management systems - Finland
Requirements with guidance for use
EUTREND model
ISO 14025
Struijs et al., 2009b
DIN EN /ISO 14025:2011-10, Environmental labels and
declarations — Type III environmental declarations —
Principles and procedures AEA Energy & Environment
Circulators in Buildings
EN 15804
EN 15804:2012-04+A1 2013, Sustainability of construction Ecoinvent
works — Environmental Product Declarations — Core rules for
the product category of construction products Ecoinvent v3.9.1
PCR Part A LCA for Experts
Institut Bauen und Umwelt e.V., Berlin (pub.): Product Category LCA for Experts 10.7.1.28
Rules for Building-Related Products and Services, Product
Category Rules for Construction Products from the range of Schema 8007
Environmental Product Declarations of Institute Bauen und
Umwelt (IBU), Part A: Calculation Rules for the Life Cycle
Assessment and Requirements on the Project Report, Version REACH
1.3.
Regulation (EC) No 1907/2006 of the European Parliament and
of the Council of 18 December 2006 concerning the
PCR Part B Registration, Evaluation, Authorization and Restriction of
Chemicals (REACH) (Status: 27.06.2018)
Institut Bauen und Umwelt e.V., Berlin (pub.): Product Category
Rules for Building-Related Products and Services, Product
Category Rules for Construction Products from the range of SVR
Environmental Product Declarations of Institute Bauen und
Umwelt (IBU), Part B: Requirements on the EPD for Pumps for Advisory Board (formerly SVA)
liquids and liquids with solids, Version 1.0 (2018)
Decision no.
Further references
20170712-n
9 Environmental Product Declaration - Grundfos Holding A/S - MAGNA3 65-150 (Stainless Steel)
Publisher
Institut Bauen und Umwelt e.V. +49 (0)30 3087748- 0
Hegelplatz 1 info@ibu-epd.com
10117 Berlin www.ibu-epd.com
Germany
Programme holder
Institut Bauen und Umwelt e.V. +49 (0)30 3087748- 0
Hegelplatz 1 info@ibu-epd.com
10117 Berlin www.ibu-epd.com
Germany
Author of the Life Cycle Assessment
Grundfos Holding A/S +4587501400
Poul Due Jensens Vej 7 LCA_EPD@grundfos.com
8850 Bjerringbro www.grundfos.com
Denmark
Owner of the Declaration
Grundfos Holding A/S +4587501400
Poul Due Jensens Vej 7 LCA_EPD@grundfos.com
8850 Bjerringbro www.grundfos.com
Denmark
10 Environmental Product Declaration - Grundfos Holding A/S - MAGNA3 65-150 (Stainless Steel)
