Environmental Product
Declaration
as per ISO 14025 and EN 15804
Owner of the declaration: MINIERA SAN ROMEDIO SRL
Publisher: Kiwa-Ecobility Experts
Programme operator: Kiwa-Ecobility Experts
Registration number: EPD-Kiwa-EE-341-EN
Issue date: 24.10.2023
Valid to: 24.10.2028
NHL light plaster:
PAVI ECO LIGHT,
TERMOARENINO,
VOLCALITE
A ready-to-use light and thermal-insulating
plaster, based on NHL and light inert.
1. General information
Miniera San Romedio NHL light plaster
Programme operator Owner of the declaration
Kiwa-Ecobility Experts Miniera San Romedio Srl
Kiwa GmbH, Ecobility Experts Località alla Miniera
Wattstraße 11-13 38012 Predaia (TN)
13355 Berlin Italy
Germany
Registration number Declared product / declared unit
EPD-Kiwa-EE-341-EN 1 ton (1000 kg) of NHL light plaster
This declaration is based on the Product Scope
Category Rules This EPD refers to a product category (NHL
EN 16908:2017+A1:2022 light plaster) produced by Miniera San Rome-
dio Srl in its plants in the province of Trento
Issue date (Italy). The data used to perform the LCA anal-
24.10.2023 ysis were provided by Miniera San Romedio Srl
and referred to the production of one year,
Valid to and the information are relative to the period
24.10.2028 2021-2022. The geographical area assumed
for the application and end-of-life of the prod-
uct is Italy. The study was performed following
the so-called from-cradle-to-gate approach
with modules C1-C4 and D.
This EPD is intended to be used for business-
to-consumer communications. The owner of
the declaration is liable for the underlying in-
formation and evidence.
Kiwa-Ecobility Experts assumes no liability for
manufacturer's information, LCA data and ev-
idence.
Verification
The European standards EN 15804+A2:2019
(10/2021) serve as PCR.
Independent verification of the declaration
and data according to ISO 14025:2006.
☐internal ☒external
Frank Huppertz
(Head of Kiwa-Ecobility Experts)
Prof. Dr. Frank Heimbecher Dr.-Ing. Morteza Nikravan
(Chairman of the independent expert committee – (External verifier of Kiwa GmbH)
Kiwa-Ecobility Experts)
Page | 2 Miniera San Romedio — NHL light plaster
2. Product
2.1 Product description
The premixed Miniera San Romedio’s products are inorganic finely grinded materials, obtained by
means of the combinations at different relative concentrations of natural hydraulic lime and expanded
perlite. In this EPD the NHL light plaster is considered.
2.2 Application
NHL light plaster: a ready-to-use dehumidifying plaster, based on dolomia, NHL and light inert. Prod-
ucts of this category are subjected to CE marking according to EN 998-1 (Dry Soft) and EN 998-2 (Armis
BFluid Connect).
2.3 Technical data
In Table 1 the main physical and applicative properties of the considered product are reported.
Table 1: Physical and applicative properties of the NHL light plaster.
Characteristic Unit Value Standard
Density kg/m3 840-960 UNI EN 1015-10
Mixing water l/kg 0.48-0.65 -
Max granulometry mm 0.5 EN 1015-1
2.4 Placing on the market/ Application rules
The pre-mixed Miniera San Romedio’s products are powder or granulates and therefore they have to
be transported to the building site by using 13 kg paper bags (15 kg for TERMOARENINO), collected
over a pallet. Pallets range from 50 to 60 bags each one, and can be mechanically moved. Once the
product reaches the building site the bags can be used to mix the product with the specified amount
of water and either be manually stirred or mechanically mixed. It can be also transported to the con-
struction site unpackaged and directly pumped into a silo already settled on a nearby position.
2.5 Base materials / Ancillary materials
In order to apply this product, it must be premixed combining at different relative concentrations nat-
ural hydraulic lime, acting as the inorganic binder and the fillers (i.e expanded perlite). Water and small
amounts of additives (less than 5 wt%) are then added to the mix, in order to develop innovative ma-
terials with very peculiar properties and suitable for a wide range of applications in the con-structions
field. The relative composition of the NHL light plaster is summarized in Table 2.
Table 2: Composition of NHL light plaster.
Dolomia Expanded NHL* Cement Polystyrene Additives
Product [wt%] perlite [wt%] [wt%] [wt%] [wt%]
[wt%]
NHL light plaster - 25-40 60-75 - - < 5
* Comprising setting retardant (4 wt% of the total NHL content)
The paper bag used as packaging (2.74 kg for 1 ton of product) contains 1.77 kg of biogenic carbon.
The product does not contain biogenic carbon.
2.6 Manufacturing
2.6.1. Manufacturing process of the binder
The unprocessed marlstone is extracted from the pit in Predaia (TN), through a mixed explosive. The
obtained marlstone is then collected through a Diesel bulldozer and transported with a Diesel lorry
from Predaia (TN) to the Ville d’Anaunia (TN) facility, where the material is subjected to a first crushing.
Page | 3 Miniera San Romedio — NHL light plaster
After the first crushing of the marlstone, part of this material is used as corrective and it is not crushed
anymore, but it is transported into a specific hopper. Through a conveyor belt the crushed marlstone
that is not intended to be used as corrective is then transported to the cooking plant, fed with hard
coal. In the cooking plant, the material is subjected to a slow thermal treatment at 900-1200 °C, that
can last up to 48 hours, and the treated material is then transported through a conveyor belt in the
maturation hopper. After the thermal treatment, the material is then subjected to a first and a second
milling phase, in order to reach the required granulometry. The lime-based end product (i.e. the
binder) is obtained by mixing the milled lime, the setting retardant and the corrective marlstone (i.e.
the marlstone extracted from the pit of Predaia, transported to the cooking plant, milled and not sub-
jected to the thermal treatment).
2.6.2 Manufacturing of the premixed products
The powders (NHL and expanded perlite) are then mixed and packed through a bagging system, by
using a paper bag with capacity of 13 kg paper bags (15 kg for TERMOARENINO), palletized and then
directly distributed. According to the EN 15804:2012+A2:2019 standard, the present LCA study was
performed following the so-called from-cradle-to-gate approach with modules C1-C4 and D consider-
ing thus the following steps:
● Extraction and processing of the raw materials (A1);
● Transport of the acquired raw materials to the manufacturer and internal transport of the ex-
tracted raw materials (A2);
● Production of the materials and mixing operations (A3).
● Deconstruction/demolition (C1)
● Transport of demolition wastes (C2)
● Waste treatment (C3)
● Waste disposal (C4)
● Benefits and impacts beyond the system boundaries (D)
A schematic process flow diagram is shown in Figure 1.
Figure 1: [Graphic schematic process flow diagram for the analysed product.]
* dolomia, NHL, cement and polystyrene are not present in all the compositions, please refer to Table 2.
Page | 4 Miniera San Romedio — NHL light plaster
2.7 Packaging
Paper bags are used to stow 13 kg paper bags (15 kg for TERMOARENINO) of premixed product.
2.8 Reference Service Life (RSL)
Since the use phase is not considered, the reference service life (RSL) as per ISO 15686-1, -2, -7 and -8
has not been declared.
2.9 Other Information
For further information on this product please visit the webpage under the following link:
https://www.tassullo.it/it/
3. LCA: Calculation rules
3.1 Declared unit
In accordance with the EN 15804+A2:2019 and EN 16908:2017+A1 1 ton of product is chosen as the
declared unit (see Table 3).
Table 3: Declared unit used for the calculations.
Product Unit Value
Declared Unit ton 1
Conversion factor to 1 kg kg 1000
3.2 System boundary
In accordance with the EN 15804+A2:2019 this study was performed following the so-called from-cra-
dle-to-gate approach with modules C1-C4 and D. In Table 4 the system boundaries of the considered
product are listed.
Table 4: system boundaries of the NHL light plaster.
Modul within the Outside the system
Module
declared system boundary boundary
A1 Raw Material Yes X
A2 Transport Yes X
A3 Manufacturing Yes X
A4 Transport No X
A5 Installation No X
B1 Use Phase No X
B2 Maintance No X
B3 Repair No X
C1 De-Construction Yes X
C2 Transport Yes X
C3 Waste treatment Yes X
C4 Landfill Yes X
D Considered loads and Yes X
benefits outside of the sys-
tem boundary in Module D
Page | 5 Miniera San Romedio — NHL light plaster
3.3 Estimates and assumptions
The electrical energy consumed in Miniera San Romedio Srl plants is a fully renewable certified energy.
The electrical energy is derived from renewable energy source (hydropower) that have obtained cer-
tification with the renewable energy certification. The electrical energy is converted from high voltage
to low voltage using an electrical transformer located close to the plants. The certification of the re-
newability of the energy covers to whole period analysed in this study (2021-2022). For as concerns
the energy source to feed the furnace for the NHL production, hard coal, with a total heat evolution of
787 Mcal to cook 1 ton of NHL, was considered. For the internal transportations, gasoline with a calo-
rific power of 45 MJ/kg was considered.
For as concerns the end-of-life stage, the demolition, transport, treatment, and disposal of wastes
were modelled using processes present in the Ecoinvent database and modified to the specific case.
In particular,
• for the C1 stage (demolition/deconstruction) the use of a diesel operating machine with a
productivity of 16.6 min/ton of demolished material and a diesel consumption of 0.9 lt/m3 was
considered. A water consumption of 0.018 m3/m3 was considered. Both references were taken
from Ivanica et al.
• for the C2 stage a distance of 15 km was assumed according to data provided by Italia del
Riciclo referred to the year 2021.
• for the C3 and C4 stages, despite the NHL light plaster can be fully recycled and due to the lack
of specific information regarding the end-of-life of this product, it was assumed that, after a
sorting and crushing process, 78.1 wt% of inert wastes is recycled (reaching the end-of-waste
state) while the remaining part is landfilled (data provided by Italia del Riciclo referred to the
year 2021). For the sorting and crushing process an existing Ecoinvent process was adapted to
the specific case.
• for the stage D it was considered that the secondary materials were used as alternative to
gravel for the production of concrete and for road construction (the background process used
refers to the period 2013-2021). Benefits and impacts associated to these operations were
therefore evaluated.
According to EN 16908:2017+A1 the carbonation of cement and natural hydraulic lime can be very
relevant after demolition with consistent carbon dioxide uptake. The evaluation of carbon dioxide up-
take was carried out according to the procedure described in EN 16757. In particular it was considered
that:
• for the C1-C3 stages no carbonation occurs due to the limited time of exposure to air or to the
lack of information regarding the duration of air exposure.
• for the C4 stage it was considered a carbon dioxide uptake equal to 75 % of the maximum
theoretical carbon dioxide uptake for landfilled wastes. No uptake was considered for recycled
wastes.
• for the D stage it was considered a carbon dioxide uptake equal to 100 % of the maximum
theoretical carbon dioxide uptake.
The following values (evaluated according to stoichiometry) were used as maximum uptake values:
• Natural hydraulic lime: 440 kg CO /ton;
2
• Cement: 490 kg CO /ton.
2
Page | 6 Miniera San Romedio — NHL light plaster
It should be highlighted that since Miniera San Romedio produces ready mixed products and has no
control and no information regarding their applications it was impossible, due to lack of data, to cal-
culate the contribution of carbonation in the use stage (module B).
Regarding the end-of-life of the packaging paper (100 % recyclable), it was not considered since beyond
the boundaries of the system.
3.4 Cut-off Criteria
As reported in the EN 15804:2012+A2:2019 standard, all inputs and outputs for which data are availa-
ble were taken into account in the calculation. Eventual data gaps have been filled with conservative
assumptions of average data or generic data available in the Ecoinvent v3.8 database of the SimaPro
software. All flows contributing to more than 1 % of the total mass, energy or environmental impact
of the system have been included in the life cycle assessment. Eventual neglected processes do not
contribute in total more than 5% to the impact categories considered. Moreover, the manufacture of
machinery, plants and other infrastructure required for production of the products under review was
not taken into consideration in the present analysis.
3.5 Period under review and Geographical reference area
The specific data were obtained directly by the commissioning company, and are related to the pro-
duction of one year. The data are referred to the period June 2021-June 2022. They were obtained by
means of specific measures related to the energy consumption and mass flows in the plants of Ville
d’Anaunia (Trento), where NHL is extracted, and of Mollaro (Trento), where NHL is mixed with ex-
panded perlite and packed. Manufacturer-specific data are referred to the period 2021-2022, while
generic data are less than 10 years old. Moreover, process-specific data are based on the average of
an operating year.
3.6 Data quality
For this study, the data quality requirements defined in ISO 14044 regulation have been considered.
In order to ensure coherence, data with the same level of detail have been used, as well as under the
same methodological considerations. Data and methods used for this study have been described with
the purpose of being reproducible by a third independent party. Whenever possible, generic data used
for the study are representative of the location where the process belongs (for example, the produc-
tion of electrical energy). The data has been collected from the plants of Ville d’Anaunia and Mollaro
(both in province of Trento). Data were associated to a specific input selected from the database Ecoin-
vent v3.8 (2021). The inventory analysis has been thus modelled by using the SimaPro software.
3.7 Allocation
Allocations were avoided.
3.8 Comparability
In order to assure the comparability of the obtained results, all datasets to be compared have been
created in accordance with EN 15804, and the product-specific performance characteristics have been
taken into account. In principle, a comparison or assessment of the environmental impacts of different
products is only possible if they have been prepared in accordance with EN 15804.
4. LCA: Scenarios and additional technical information
No scenario or additional technical information to be declared.
Page | 7 Miniera San Romedio — NHL light plaster
5. LCA: Results
Table 5 shows the results of the impact assessment indicators, resource use, waste and other output
streams for the declared unit (1 ton of NHL light plaster). The results presented here refer to the de-
clared product. In Table 6 the results of the biogenic carbon content are reported.
Disclaimer on ADP-e, ADP-f, WDP, ETP-fw, HTP-c, HTP-nc, SQP: The results of these environmental
impact indicators must be used with caution, as the uncertainties in these results are high or as there
is limited experience with the indicator.
Disclaimer on IR: This impact category mainly addresses the potential effect of low dose ionizing radi-
ation on human health in the nuclear fuel cycle. It does not consider effects due to possible nuclear
accidents and occupational exposures, nor does it consider radioactive waste disposal in underground
facilities. Potential ionizing radiation from soil, radon, and some building materials is also not measured
by this indicator.
Page | 8 Miniera San Romedio — NHL light plaster
Description of the system boundary
Construction process Benefits and loads beyond
Product stage Use stage End of life stage
stage the system boundaries
la ir e t a m w a Ry lp p u s t r o p s n a r T u n a M-g n ir u t c a f t r o p s n a r Tu n a m m o r-
f
o t r e r u t c a fe s u fo e c a lp n o it c u r ts n o
C
n o it a lla ts n -is s e c o r p e s U n ia M-e c n a n e t r ia p e R tn e m e c a lp e
R
r u fe R-n e m h s ib la n o it a r e p Oe s u y g r e n e la n o it a r e p Oe s u r e t a w e D- n o it c u r ts n o cn o itilo m e d
/
t r o p s n a r T e ts a Wg n is s e c o r p la s o p s iD e s u e R-y r e v o c e R- g n ilc y c e R- a itn e t o pl
A1 A2 A3 A4 A5 B1 B2 B3 B4 B5 B6 B7 C1 C2 C3 C4 D
X X X MND MND MNR MNR MNR MND MND MND MND X X X X X
X=Module declared | MND=Module not declared
LCA results - Indicators describing environmental impacts based on the impact assessment (LCIA): 1 ton of NHL light plaster (EN 15804+A2)
Parameter Unit A1-A3 C1 C2 C3 C4 D
Core environmental impact indicators (EN 15804+A2)
GWP-total kg CO2 eqv. 8.24E+02 7.62E+00 1.37E+00 1.73E+00 -4.76E+01 -2.35E+02
GWP-f kg CO2 eqv. 8.15E+02 7.61E+00 1.37E+00 1.68E+00 -4.76E+01 -2.35E+02
GWP-b kg CO2 eqv. 8.22E+00 5.33E-03 1.39E-03 4.62E-02 1.25E-03 -1.11E-01
GWP-luluc kg CO2 eqv. 2.10E-01 1.13E-03 4.90E-04 3.51E-03 1.09E-03 -2.15E-03
ODP kg CFC 11 eqv. 3.95E-05 3.16E-06 3.31E-07 1.16E-07 4.67E-07 -3.55E-07
AP mol H+ eqv. 4.69E+00 3.65E-02 9.54E-03 1.04E-02 1.08E-02 -2.35E-02
EP-fw kg P eqv. 2.10E-01 3.03E-04 8.50E-05 1.50E-03 1.06E-04 -6.12E-04
EP-m kg N eqv. 6.89E-01 9.56E-03 3.74E-03 2.26E-03 3.77E-03 -6.73E-03
EP-T mol N eqv. 7.33E+00 1.05E-01 4.10E-02 2.18E-02 4.13E-02 -9.02E-02
POCP kg NMVOC eqv. 2.10E+00 3.41E-02 1.15E-02 6.05E-03 1.20E-02 -2.11E-02
ADP-mm kg Sb-eqv. 9.77E-04 4.85E-06 3.13E-06 1.47E-05 2.63E-06 -5.65E-05
ADP-f MJ 6.02E+03 1.99E+02 2.16E+01 3.39E+01 3.22E+01 -4.07E+01
WDP m3 world eqv. 1.60E+02 4.16E+00 7.31E-02 3.75E-01 1.45E+00 -8.13E-01
Additional environmental impact indicators (EN 15804+A2)
CaPM disease incidence ND ND ND ND ND ND
IR kBq U235 eqv. ND ND ND ND ND ND
ETP-fw CTUe ND ND ND ND ND ND
HTP-c CTUh ND ND ND ND ND ND
HTP-nc CTUh ND ND ND ND ND ND
SQP Pt ND ND ND ND ND ND
ADP-mm= Abiotic depletion potential for non-fossil resources | ADP-f=Abiotic depletion for fossil resources potential | AP= Acidification potential, Accumulated Exceedance | EP-fw = Eutrophication potential, fraction of nutrients reaching
freshwater end compartment | EP-m= Eutrophication potential, fraction of nutrients reaching marine end compartment| EP-T= Eutrophication potential, Accumulated Exceedance | GWP-b=Global Warming Potential biogenic | GWP-f=Global
Warming Potential fossil fuels | GWP-luluc=Global Warming Potential land use and land use change |GWP-total=Global Warming Potential total| ODP=Depletion potential of the stratospheric ozone layer |POCP=Formation potential of
tropospheric ozone | WDP=Water (user) deprivation potential, deprivation- weighted water consumption | ETP-fw=Potential Comparative Toxic Unit for ecosystems | HTP-c=Potential Toxic Unit for Humans toxicity, cancer | HTP-nc= Potential
Toxic Unit for humans, non-cancer | IRP=Potential Human exposure efficiency relative to U235, human health | PM=Potential incidence of disease due to Particulate Matter emissions | SQP=Potential soil quality index
Page | 9 Miniera San Romedio — NHL light plaster
Parameter Unit A1-A3 C1 C2 C3 C4 D
PERE MJ 7.78E+02 8.53E-01 2.71E-01 6.27E+00 2.75E-01 -1.30E+01
PERM MJ 0.00E+00 0.00E+00 0.00E+00 0.00E+00 0.00E+00 0.00E+00
PERT MJ 7.78E+02 8.53E-01 2.71E-01 6.27E+00 2.75E-01 -1.30E+01
PENRE MJ 6.38E+03 2.12E+02 2.29E+01 3.56E+01 3.42E+01 -4.27E+01
PENRM MJ 0.00E+00 0.00E+00 0.00E+00 0.00E+00 0.00E+00 0.00E+00
PENRT MJ 6.38E+03 2.12E+02 2.29E+01 3.56E+01 3.42E+01 -4.27E+01
SM Kg 0.00E+00 0.00E+00 0.00E+00 0.00E+00 0.00E+00 0.00E+00
RSF MJ 0.00E+00 0.00E+00 0.00E+00 0.00E+00 0.00E+00 0.00E+00
NRSF MJ 0.00E+00 0.00E+00 0.00E+00 0.00E+00 0.00E+00 0.00E+00
FW M3 1.58E+02 3.99E+00 7.35E-02 3.69E-01 1.45E+00 -7.11E-01
HWD Kg 3.53E-03 5.41E-04 5.23E-05 3.25E-05 4.87E-05 -1.76E-04
NHWD Kg 4.11E+01 1.79E-01 1.99E+00 1.22E-01 2.19E+02 -6.55E-01
RWD Kg 9.59E-03 1.40E-03 1.46E-04 2.45E-04 2.11E-04 -2.96E-04
CRU Kg 0.00E+00 0.00E+00 0.00E+00 0.00E+00 0.00E+00 0.00E+00
MFR Kg 1.00E-01 0.00E+00 0.00E+00 7.81E+02 0.00E+00 0.00E+00
MER Kg 0.00E+00 0.00E+00 0.00E+00 0.00E+00 0.00E+00 0.00E+00
EET MJ 0.00E+00 0.00E+00 0.00E+00 0.00E+00 0.00E+00 0.00E+00
EEE MJ 0.00E+00 0.00E+00 0.00E+00 0.00E+00 0.00E+00 0.00E+00
PERE=Use of renewable primary energy excluding renewable primary energy resources used as raw materials | PERM= Use of renewable primary energy resources used as raw materials | PERT=Total use of renewable primary energy
resources | PENRE= Use of non-renewable primary energy excluding non-renewable primary energy resources used as raw materials | PENRM= Use of non-renewable primary energy resources used as raw materials | PENRT= Total use of
non-renewable primary energy resources | SM=Use of secondary material | RSF=Use of renewable secondary fuels | NRSF=Use of non-renewable secondary fuels | FW=Use of fresh water | HWD=Hazardous waste disposed | NHWD=Non-
hazardous waste disposed | RWD=Radioactive waste disposed | CRU=Components for re-use | MFR=Materials for recycling | MER=Materials for energy recovery | EET=Exported energy, thermical | EE=Exported energy, electrical
In Table 6 the biogenic content of NHL light plaster is reported.
Table 6: results of the biogenic carbon content of NHL light plaster.
LCA results - information on biogenic carbon content at the factory gate: 1 ton of NHL light plaster (EN 15804+A2)
Parameter Unit Value
biogenic carbon content in product kg C 0
biogenic carbon content in accompanying packaging kg C 1.77
NOTE 1 kg biogenic carbon is equivalent to 44/12 kg CO2
Page | 10 Miniera San Romedio — NHL light plaster
6. References
ISO 14040:2006, Environmental management - Life cycle assessment - Principles and framework
ISO 14044:2006, Environmental management - Life cycle assessment - Requirements and guidelines
ISO 14025:2006: Environmental labels and declarations — Type III environmental declarations — Prin-
ciples and procedures EN 13249
EN 15804:2012+A2:2019 Sustainability of construction works — Environmental Product Declarations
— Core rules for the product category of construction products
PCR A: General Program Category Rules for Construction Products from the EPD program Kiwa-Ecobil-
ity Experts, R.0_2021-07-16
EN 16908:2017+A1: Cement and building lime - environmental product declarations - product category
rules complementary to EN 15804.
EN16757: Sustainability of construction works – Environmental product declarations – Product cate-
gory rules for concrete and concrete elements.
Ivanica, R., M. Risse, G. Weber-Blaschke, and K. Richter, Development of a life cycle inventory database
and life cycle impact assessment of the building demolition stage: A case study in Germany. Journal of
Cleaner Production, 2022. 338: p. 130631.
Frischknecht, R. and N. Jungbluth. Overview and Methodology. Ecoinvent report No. 1. 2007.
Fondazione per lo sviluppo sostenibile, F.U., Unione Imprese Economia Circolare,. L'Italia del Riciclo.
2021; Available from: https://www.cial.it/rapporto-italia-del-riciclo-2021/#:~:text=Se-
condo%20i%20dati%20Ispra%20sono,e%20il%2060%25%20al%202030.
Laveglia, A., L. Sambataro, N. Ukrainczyk, N. De Belie, and E. Koenders, Hydrated lime life-cycle assess-
ment: Current and future scenarios in four EU countries. Journal of Cleaner Production, 2022. 369
7. ANNEX 1 Requirements of the Minimum Environmental Criteria (DM June 23th 2022)
In Table 7 the requirements imposed by Minimum Environmental Criteria (DM June 23th 2022) for the
NHL light plaster considered in this project report are summarized. As it can be seen, the product sat-
isfies the legislative requirements imposed by the Italian Legislation on the Minimum Environmental
Criteria for construction services.
Table 7: Requirements of the Minimum Environmental Criteria DM June 23th 2022) for the NHL light
plaster.
The required emission limits can
not be applied to these materi-
Emissions in confined als since their applications are
2.5.1
environment not included in the list provided
in the DM June 23th 2022 at the
point 2.5.1.
The required minimum recycled
Premixed concrete or content is not applicable since
2.5.2 prepared on the building the products considered in this
site EPD can not be considered as
“concrete”. According to EN
Page | 11 Miniera San Romedio — NHL light plaster
998-1 and EN 998-2 they can be
defined as “plasters” or “mor-
tars” depending on the specific
application.
2.5.7 Thermal and acoustic insulating materials (referred only to
TERMOARENINO, VOLCALITE)
2.5.7c Thermal and acoustic in- The products considered in this
sulating materials study has a CE mark and a decla-
ration of performance (DoP) that
specifies its thermal conductivity
(λ ).
D
2.5.7d Thermal and acoustic in- The products do not contain sub-
sulating materials stances classified as persistent,
bioaccumulative and toxic (PBT)
and very persistent and very bio-
accumulative (vPvB) according
to Annex XIII of the regulation EC
1907/2006 (REACH).
2.5.7e Thermal and acoustic in- The products considered in this
sulating materials study are not produced with
blowing agents having a reduc-
tion potential of the ozone layer
higher than zero.
2.5.7f Thermal and acoustic in- The products considered in this
sulating materials study are not produced, formu-
lated or applied by using lead-
based catalysts.
2.5.7i Thermal and acoustic in- The products considered in this
sulating materials study are not produced using
materials that should contain a
minimum amount of recy-
cled/reused material according
to the list provided in the DM
June 23th 2022.
2.6.2 Dismantling and re- All the products considered in
moval of the materials this EPD, after the dismantling
operations, can be fully sent to
reuse, recovery and recycling
operations.
Note: the other requirements imposed by the Minimum Environmental Criteria are not reported since
not applicable for the analyzed products. Note 2: the satisfaction of the requirements for thermal in-
sulating materials was not verified for PAVI ECO LIGHT and it is therefore excluded from what declared
at point 2.5.7 of Table 7)
Page | 12 Miniera San Romedio — NHL light plaster
Publisher Mail DE.Ecobility.Ex-
Kiwa-Ecobility Experts perts@kiwa.com
Kiwa GmbH, Ecobility Experts Web https://www.kiwa.com/de/
Wattstraße 11-13 de/themes/ecobility-ex-
13355 Berlin perts/ecobility-experts/
Germany
Programme operator Mail DE.Ecobility.Ex-
Kiwa-Ecobility Experts perts@kiwa.com
Kiwa GmbH, Ecobility Experts Web https://www.kiwa.com/de/
Wattstraße 11-13 de/themes/ecobility-ex-
13355 Berlin perts/ecobility-experts/
Germany
LCA Practitioner Tel. (+39) 0461/283724
Prof. Andrea Dorigato, Ing. Fax. andrea.dorigato@unitn.it
Francesco Valentini Mail https://webapps.unitn.it/d
University of Trento Web u/it/Per-
Department of Industrial Engi- sona/PER0009668/Curricu-
neering (DII) lum
Via Sommarive 9
38123 Trento
Italy
Owner of the declaration Tel. (+39) 0463/662100
Miniera San Romedio Srl Fax. (+39) 0463/662113
Località alla Miniera Mail minierasanromedio@pec.it
38012 Predaia Web www.minierasanromedio.it
Italy VAT 00602230229
Kiwa-Ecobility Experts -
established member of
Page | 13 Miniera San Romedio — NHL light plaster
