ENVIRONMENTAL PRODUCT DECLARATION
as per ISO 14025 and EN 15804+A2
Owner of the Declaration SOUDAL N.V.
Publisher Institut Bauen und Umwelt e.V. (IBU)
Programme holder Institut Bauen und Umwelt e.V. (IBU)
Declaration number EPD-SDL-20240123-CBA1-EN
Issue date 03.04.2024
Valid to 23.06.2028
SOUDAFIX P300-SF
SOUDAL N.V.
www.ibu-epd.com | https://epd-online.com
General Information
SOUDAL N.V. SOUDAFIX P300-SF
Programme holder Owner of the declaration
IBU – Institut Bauen und Umwelt e.V. SOUDAL N.V.
Hegelplatz 1 Everdongenlaan 18-20
10117 Berlin 2300 Turnhout
Germany Belgium
Declaration number Declared product / declared unit
EPD-SDL-20240123-CBA1-EN The declared product is the two-component reaction resin mortar
"SOUDAFIX P300-SF", manufactured by SOUDAL N.V.. The declared unit
is based on 1 kg reaction resin product in the ratio at which the two
components must be mixed before use. The packaging is also included in
the calculation, since the product is sold by SOUDAL N.V. with its
packaging. The declared unit is indicated in [kg].
This declaration is based on the product category rules: Scope:
Reaction resin products, 01.08.2021 This document covers two-component reaction resin mortar "SOUDAFIX
(PCR checked and approved by the SVR) P300-SF". To prepare the life cycle assessment [LCA], specific data were
collected from the SOUDAL N.V. manufacturing facility in Germany. The
assessment is based on data from 2020 which correspond to the yearly
Issue date average. The procedure by which the data are allocated to the declared
unit is described in the "Allocation" section. The owner of the Declaration is
03.04.2024
liable for the underlying information and documentation, and IBU cannot
be held liable with regard to any manufacturer information, LCA data or
documentation.
Valid to
23.06.2028
The owner of the declaration shall be liable for the underlying information
and evidence; the IBU shall not be liable with respect to manufacturer
information, life cycle assessment data and evidences.
The EPD was created according to the specifications of EN 15804+A2. In
the following, the standard will be simplified as EN 15804.
Verification
The standard EN 15804 serves as the core PCR
Independent verification of the declaration and data according to ISO
14025:2011
Dipl.-Ing. Hans Peters
(Chairman of Institut Bauen und Umwelt e.V.) internally X externally
Florian Pronold Angela Schindler,
(Managing Director Institut Bauen und Umwelt e.V.) (Independent verifier)
1 Environmental Product Declaration - SOUDAL N.V. - SOUDAFIX P300-SF
Product
Product description/Product definition Curing time in dry substrate:
The declared product SOUDAFIX P300-SF is a two-component -5 °C 360 min.
reaction resin mortar based on polyester resin that is delivered 0 °C 180 min.
in a two-component plastic cartridge or foil tube cartridge. The +5 °C 120 min.
SOUDAFIX P300-SF product is applied through a static mixer +10 °C 100 min.
using a manual, battery-operated or pneumatic gun. It was +20 °C 45 min.
developed as a cost-effective alternative for securing threaded +30 °C 25 min.
rods and internally threaded sleeves in approved applications. +35 °C 20 min.
It can also be used safely and easily in perforated brick by
using a perforated sleeve. SOUDAFIX P300-SF offers a good For more information, please refer to the relevant technical data
range of applications at environmental temperatures of up to 80 sheet.
°C.
Product performance values in accordance with the Declaration
of Performance with regard to its principal charateristics
according to ETA-11/0447 and ETA-13/0064, European
Technical Assessment SOUDAL N.V. SOUDAFIX P300-SF.
Marketing of the product in the EU/EFTA (except for Base materials/Ancillary materials
Switzerland) is governed by Regulation (EU) No. 305/2011 The declared product SOUDAFIX P300-SF is delivered as a
(CPR). The product requires a Declaration of Performance two-component plastic cartridge and consists of a resin
subject to ETA-11/0447, ETA-13/0064 and the CE-marking. component and a curing agent component in a 10:1 volume
ratio. The mixing ratio
Application between the resin component and the curing agent component
The declared product SOUDAFIX P300-SF is used to reliably is set automatically as the product is pushed out of the
secure threaded rods and internally threaded sleeves. Use in cartridge. Curing begins immediately after the components are
cracked non-cracked and solid and perforated brick is possible mixed.
with industry standard anchor rods.
1) "This product/article/at least one partial article contains
substances in the ECHA candidate list of substances of very
Sample applications high concern (SVHC) (10 June 2022) above a concentration of
0.1% by mass: no."
Suitable for securing façades, canopies, wooden structures,
metal structures, metal profiles, panels, railings, gratings,
plumbing fixtures, pipes, cable trays etc.
2) "This product/article/at least one partial article contains other
Technical Data
CMR substances in categories 1A or 1B which are not on the
The following construction data are relevant for the declared candidate list, exceeding 0.1 percentage by mass: no"
product SOUDAFIX P300-SF as delivered:
Construction Data 3)"Biocide products were added to this construction product or
it has been treated with biocide products (this then concerns a
Name Value Unit
treated product as defined by the (EU) Regulation on Biocidal
Density acc. to DIN 51757 for mixing the two
1.7 g/ml Products No. 528/2012): no"
components
Compressive strength acc. to DIN EN 196 Part 1 88.1 N/mm²
Flexural strength acc. to DIN EN 196 Part 1 31.5 N/mm² The product considered in this EPD contains individual
components in the following ranges:
Storage:
Resin component:
Store in a cool, dry and dark place; storage temperature: +5°C
to +25°C
Polyester resin: 30 to 40% by weight
Shelf life:
Mineral fillers: 50 to 70% by weight
18 months in standard cartridge systems
Other components: < 5% by weight
12 months in foil tube cartridge systems
Curing agent component:
Gel and working time:
-5 °C 90 min.
Dibenzoyl peroxide: 10 to 15% by weight
0 °C 45 min.
Mineral fillers: 40 to 60% by weight
+5 °C 25 min.
Other components: 10 to 35% by weight
+10 °C 20 min.
+20 °C 6 min.
Reference service life
+30 °C 4 min.
The declared product SOUDAFIX P300-SF may be exposed to
+35 °C 2 min.
a wide range of environmental conditions during the use phase.
2 Environmental Product Declaration - SOUDAL N.V. - SOUDAFIX P300-SF
Its expected reference service life depends on the specific
installation situation and on the product's resulting exposure.
The main factors influencing service life are weather conditions
and mechanical and chemical stresses.
LCA: Calculation rules
impacts of the declared unit, a total of 8 information modules
Declared Unit are considered. The information modules A1 to A3 describe the
The product declared is a two-component reaction resin mortar material provision, the transport to the production site, as well
manufactured by SOUDAL N.V. with the product name as the production processes of the product itself.
SOUDAFIX P300-SF. The declared unit is based on 1 kg
reaction resin The precursor products are sourced from Germany, Belgium,
product in the ratio at which the two components must be mixed Italy and France. Transport is mainly done by truck. The
before use. following process diagrams illustrate the underlying production
process.
The mixing ratio between the resin component and the curing
agent component is 9:1 [m/m] (volume ratio 10:1). The
packaging is also included in the calculation at 0.3013 kg per 1
kg of reaction resin product. The declared unit data are
presented in the table below.
Declared unit data
Name Value Unit
Declared unit 1 kg
System boundary
Type of EPD: Cradle to factory gate with options. The following
information modules are defined as system boundaries in this
study:
Production stage (A1-A3): Figure 1 Information modules A1 to A3 of the product
• A1,
Raw material extraction,
• A2,
Transport to the manufacturer,
• A3,
Manufacturing.
Figure 2 Information modules A1 to A3 of the packaging
End of life (C1-C4): Geographic Representativeness
Land or region, in which the declared product system is
• C1, manufactured, used or handled at the end of the product´s
Deconstruction/demolition lifespan: Germany
• C2,
Transport,
Comparability
• C3, Basically, a comparison or an evaluation of EPD data is only
Waste processing, possible if all the data sets to be compared were created
• C4, according to EN 15804 and the building context, respectively
Disposal. the product-specific characteristics of performance, are taken
into account. The background databases from the LCA for
Reuse, recovery and recycling potential (D) Experts databases, which this study also draws on, are
documented at the following site (Sphera). 2023.1
To precisely determine the indicators and environmental http://www.gabi-software.com/deutsch/index/
LCA: Scenarios and additional technical information
Name Value Unit
Characteristic product properties of biogenic carbon
Packaging PP 0.0318 kg
No renewable raw materials are used in the product or the
Packaging PA6 0.2696 kg
packaging. The biogenic carbon value is therefore reported as
zero.
Packaging per declared unit End of Life (C1-C4)
3 Environmental Product Declaration - SOUDAL N.V. - SOUDAFIX P300-SF
The product is demolished by using an electric chisel. The
Reuse, recovery and recycling potential (D), relevant
electrical energy consumption for this tool is estimated at 0.05
scenario specifications
MJ for the declared unit. The power consumption is calculated
The product has no reuse, recovery or recycling potential.
using a European energy mix. Construcion waste is transported
Information module D is therefore declared and reported as
200 km by truck to a waste treatment facility. At the waste
zero.
treatment facility, the construction waste is shredded and then
disposed in a landfill. Name Value Unit
Reuse, recovery and recycling potential 0 kg
Name Value Unit
Collected as mixed construction waste 1 kg
Shredding 1 kg
Disposal in landfill 1 kg
4 Environmental Product Declaration - SOUDAL N.V. - SOUDAFIX P300-SF
LCA: Results
DESCRIPTION OF THE SYSTEM BOUNDARY (X = INCLUDED IN LCA; MND = MODULE OR INDICATOR NOT DECLARED; MNR
= MODULE NOT RELEVANT)
Benefits and
Construction loads beyond
Product stage Use stage End of life stage
process stage the system
boundaries
la ire ta m w a Ry lp p u s tro p s n a rT g n iru tc a fu n a M e h t m o rf tro p s n a rTe tis e h t o t e ta g y lb m e s s A e s U e c n a n e tn ia M ria p e R tn e m e c a lp e R tn e m h s ib ru fe R y g re n e la n o ita re p Oe s u re ta w la n o ita re p Oe s u n o itc u rts n o c -e Dn o itilo m e d tro p s n a rT g n is s e c o rp e ts a W la s o p s iD -e s u e R-y re v o c e R-g n ilc y c e Rla itn e to p
A1 A2 A3 A4 A5 B1 B2 B3 B4 B5 B6 B7 C1 C2 C3 C4 D
X X X MND MND MND MND MNR MNR MNR MND MND X X X X X
RESULTS OF THE LCA - ENVIRONMENTAL IMPACT according to EN 15804+A2: 1 kg SOUDAFIX P300-SF
Parameter Unit A1-A3 C1 C2 C3 C4 D
Global Warming Potential total (GWP-total) kg CO 2 eq 3.45E+00 4.58E-03 1.75E-02 2.58E-03 1.46E-02 0
Global Warming Potential fossil fuels (GWP-fossil) kg CO 2 eq 3.38E+00 4.53E-03 1.73E-02 2.56E-03 1.46E-02 0
Global Warming Potential biogenic (GWP-biogenic) kg CO 2 eq 7.32E-02 4.91E-05 0 0 0 0
Global Warming Potential luluc (GWP-luluc) kg CO 2 eq 6.39E-04 4.87E-07 1.58E-04 1.92E-05 4.53E-05 0
Depletion potential of the stratospheric ozone layer (ODP) kg CFC11 eq 6.23E-09 8.27E-14 1.49E-15 4.28E-15 3.71E-14 0
Acidification potential of land and water (AP) mol H+ eq 5.38E-03 9.57E-06 6.48E-05 1.34E-05 1.03E-04 0
Eutrophication potential aquatic freshwater (EP-freshwater) kg P eq 1.63E-05 1.67E-08 6.21E-08 8.71E-09 2.93E-08 0
Eutrophication potential aquatic marine (EP-marine) kg N eq 1.73E-03 2.29E-06 3.03E-05 6.13E-06 2.67E-05 0
Eutrophication potential terrestrial (EP-terrestrial) mol N eq 1.5E-02 2.39E-05 3.39E-04 6.77E-05 2.94E-04 0
Formation potential of tropospheric ozone photochemical oxidants kg NMVOC
5.46E-03 6.11E-06 5.84E-05 1.66E-05 8.06E-05 0
(POCP) eq
Abiotic depletion potential for non fossil resources (ADPE) kg Sb eq 4.89E-07 6.95E-10 1.1E-09 2.74E-09 6.72E-10 0
Abiotic depletion potential for fossil resources (ADPF) MJ 7.38E+01 9.43E-02 2.32E-01 5.04E-02 1.94E-01 0
m3 world eq
Water use (WDP) 1.1E-01 9.98E-04 1.96E-04 4.98E-04 1.6E-03 0
deprived
RESULTS OF THE LCA - INDICATORS TO DESCRIBE RESOURCE USE according to EN 15804+A2: 1 kg SOUDAFIX P300-SF
Parameter Unit A1-A3 C1 C2 C3 C4 D
Renewable primary energy as energy carrier (PERE) MJ 4.87E+00 5.64E-02 1.64E-02 4.68E-03 3.16E-02 0
Renewable primary energy resources as material utilization
MJ 0 0 0 0 0 0
(PERM)
Total use of renewable primary energy resources (PERT) MJ 4.87E+00 5.64E-02 1.64E-02 4.68E-03 3.16E-02 0
Non renewable primary energy as energy carrier (PENRE) MJ 5.49E+01 9.43E-02 2.32E-01 5.05E-02 1.94E-01 0
Non renewable primary energy as material utilization (PENRM) MJ 1.89E+01 0 0 0 0 0
Total use of non renewable primary energy resources (PENRT) MJ 7.39E+01 9.43E-02 2.32E-01 5.05E-02 1.94E-01 0
Use of secondary material (SM) kg 0 0 0 0 0 0
Use of renewable secondary fuels (RSF) MJ 0 0 0 0 0 0
Use of non renewable secondary fuels (NRSF) MJ 0 0 0 0 0 0
Use of net fresh water (FW) m3 1.07E-02 4.55E-05 1.81E-05 1.44E-05 4.9E-05 0
RESULTS OF THE LCA – WASTE CATEGORIES AND OUTPUT FLOWS according to EN 15804+A2:
1 kg SOUDAFIX P300-SF
Parameter Unit A1-A3 C1 C2 C3 C4 D
Hazardous waste disposed (HWD) kg 6.55E-09 7.38E-12 8.59E-13 1.31E-13 4.23E-12 0
Non hazardous waste disposed (NHWD) kg 3.26E-02 6.91E-05 3.35E-05 1.33E-05 9.71E-01 0
Radioactive waste disposed (RWD) kg 1.11E-03 1.5E-05 3E-07 6.77E-07 2.21E-06 0
Components for re-use (CRU) kg 0 0 0 0 0 0
Materials for recycling (MFR) kg 0 0 0 0 0 0
Materials for energy recovery (MER) kg 0 0 0 0 0 0
Exported electrical energy (EEE) MJ 0 0 0 0 0 0
Exported thermal energy (EET) MJ 0 0 0 0 0 0
RESULTS OF THE LCA – additional impact categories according to EN 15804+A2-optional:
1 kg SOUDAFIX P300-SF
Parameter Unit A1-A3 C1 C2 C3 C4 D
Disease
Incidence of disease due to PM emissions (PM) ND ND ND ND ND ND
incidence
Human exposure efficiency relative to U235 (IR) kBq U235 eq ND ND ND ND ND ND
Comparative toxic unit for ecosystems (ETP-fw) CTUe ND ND ND ND ND ND
Comparative toxic unit for humans (carcinogenic) (HTP-c) CTUh ND ND ND ND ND ND
5 Environmental Product Declaration - SOUDAL N.V. - SOUDAFIX P300-SF
Comparative toxic unit for humans (noncarcinogenic) (HTP-nc) CTUh ND ND ND ND ND ND
Soil quality index (SQP) SQP ND ND ND ND ND ND
Disclaimer - applies to the following indicators: "Abiotic shortage potential - non-fossil resources", "Abiotic shortage potential - fossil
fuels", "Water deprivation potential (users)", "Potential comparative toxic unit for ecosystems", "Potential comparative toxic unit for
human health - carcinogenic effects", Potential comparative toxic unit for human health - non-carcinogenic effects", "Potential soil
quality index". The results of this environmental impact indicator shall be used with care, as the uncertainties of the results are high and
as there is limited experience with the indicator.
References
Standards ecoinvent 3.9
Background database: ecoinvent 3.9.1
DIN 51757 Zürich: ecoinvent (Ed.)
DIN 51757:2011-01 http://www.ecoinvent.org
Testing of mineral oils and related materials - Determination of (28.04.2023)
density.
ETA-11/0447
EN 196 European Technical Assessment.
DIN EN 196-1:2016-11
Test methods for cement - Part 1: Determination of strength ETA-13/0064
German version EN 196-1:2016 European Technical Assessment.
EN 12504 IBU 2021
DIN EN 12504-4:2021-10 Institut Bauen und Umwelt e.V.: General guidance for the EPD
Testing concrete in structures - Part 4: Determination of programme of the Institut Bauen und Umwelt e.V., Version 2.0,
ultrasonic pulse velocity. Berlin: Institut Bauen und Umwelt e.V., 2021.
www.ibu-epd.com
EN 15804
EN 15804:2019-04+A2 (in print), Sustainability of construction PCR PART A
works - Product Category Rules for Building-Related Products and
Environmental Product Declarations - Core rules for the product Services - Calculation Rules for the Life Cycle Assessment and
category of construction products. requirements on the Project Report V2.1, Institut Bauen und
Umwelt e.V., 11.2021.
EN/TR 15941
CEN/TR 15941:2010-03, Sustainability of construction works - PCR: Reaction resin products
Environmental product declarations - Methodology for selection Guidance-Texts for Building-Related Products and Services.
and use of generic data. Part B: Requirements on the EPD for Reaction resin products,
Version 1.3. Berlin: Institut Bauen und Umwelt e.V.
ISO 14025 (Hrsg.),07.2014.
DIN EN ISO 14025:2011-10, Environmental labels and
declarations - Type III environmental declarations - Principles Sphera
and procedures. LCA for Experts: 2023.1
Leinfelden-Echterdingen; Sphera
ISO 14044 Solution GmbH (Hrsg.)
DIN EN ISO 14044:2006-10, Environmental management - Life http://www.gabi-software.com/deutsch/index/
cycle assessment - Requirements and guidelines. (28.04.2023)
Further references
6 Environmental Product Declaration - SOUDAL N.V. - SOUDAFIX P300-SF
Publisher
Institut Bauen und Umwelt e.V. +49 (0)30 3087748- 0
Hegelplatz 1 info@ibu-epd.com
10117 Berlin www.ibu-epd.com
Germany
Programme holder
Institut Bauen und Umwelt e.V. +49 (0)30 3087748- 0
Hegelplatz 1 info@ibu-epd.com
10117 Berlin www.ibu-epd.com
Germany
Author of the Life Cycle Assessment
FIT-Umwelttechnik GmbH 05362 72 69 474
Westerstr. 13 bertram@fit-umwelttechnik.de
38442 Wolfsburg www.fit-umwelttechnik.com
Germany
Owner of the Declaration
SOUDAL N.V. +32 014 42 42 31
Everdongenlaan 18-20 info@soudal.com
2300 Turnhout www.soudal.com
Belgium
7 Environmental Product Declaration - SOUDAL N.V. - SOUDAFIX P300-SF
