ENVIRONMENTAL PRODUCT DECLARATION
as per ISO 14025 and EN 15804+A2
Owner of the Declaration Armacell GmbH
Programme holder Institut Bauen und Umwelt e.V. (IBU)
Publisher Institut Bauen und Umwelt e.V. (IBU)
Declaration number EPD-ARM-20200219-IBB1-EN
Issue date 12.03.2021
Valid to 11.03.2026
AF/ArmaFlex insulation for building equipment and industrial
installation
Armacell GmbH
www.ibu-epd.com | https://epd-online.com
Umwelt Produktdeklaration Name des Herstellers – Name des Produkts
1. General Information
Armacell GmbH AF/ArmaFlex
Programme holder Owner of the declaration
IBU – Institut Bauen und Umwelt e.V. Armacell GmbH
Panoramastr. 1 Robert-Bosch-Str. 10
10178 Berlin 48153 Münster - Germany
Germany
Declaration number Declared product / declared unit
EPD-ARM-20200219-IBB1-EN 1m³ insulation material AF/ArmaFlex
This declaration is based on the product Scope:
category rules: Product line AF/ArmaFlex
Insulating materials made of foam plastics, 06.2017 Insulation material for industrial and building
(PCR checked and approved by the SVR) installations vulcanized in tubes and sheets.
This declaration is an Environmental Product
Issue date Declaration according to ISO 14025 describing the
12.03.2021 average environmental performance of the product
produced in Germany, Spain and Poland. The average
Valid to has been calculated based on site specific annual
production volumes.
11.03.2026
As the installation of the product is not restricted to
countries where the products have been produced the
validity of this EPD is considered at least EU wide.
The owner of the declaration shall be liable for the
underlying information and evidence; the IBU shall not
be liable with respect to manufacturer information, life
cycle assessment data and evidences.
The EPD was created according to the specifications
of EN 15804+A2. In the following, the standard will be
simplified as EN 15804.
Verification
The standard EN 15804 serves as the core PCR
Independent verification of the declaration and data
according to ISO 14025:2010
Dipl. Ing. Hans Peters internally x externally
(chairman of Institut Bauen und Umwelt e.V.)
Dr. Alexander Röder Mr Carl-Otto Neven
(Managing Director Institut Bauen und Umwelt e.V.)) (Independent verifier)
2. Product
2.1 Information about the enterprise automotive, wind energy, sports and
Armacell International GmbH is a producer of flexible construction.
insulation foams for the equipment insulation market
and a provider of engineered foams which operates
The product focus is insulation materials enhancing the
two main businesses:
energy efficiency of technical equipment, high-
 Advanced Insulation develops flexible foams
performance foams for technical and lightweight
for the insulation of technical equipment
applications, 100% recycled PET products and next-
utilised for the transport of energy - such as
generation aerogel technology.
heating, ventilation & air conditioning (HVAC)
and heating & plumbing (H&P) in residential 2.2 Product description/Product definition
and commercial construction, process lines in AF/ArmaFlex is the professional, highly-flexible,
closed-cell elastomeric foam insulation (FEF) for
the heavy- and oil & gas industry, equipment
continuous energy saving and condensation control
in transportation, as well as, acoustics.
purposes. The combination of very low thermal
 Engineered Foams develops high-
conductivity and extremely high resistance to water
performance foams for the use in a broad vapour transmission prevents long-term energy losses
range of end markets including transportation,
2 Environmental Product Declaration Armacell GmbH – AF/ArmaFlex insulation for industrial and building installation
and water vapour ingress and reduces the risk of adhesive backings/closures are available; these
corrosion under insulation. variations are not included in the calculations.
Insulation thicknesses are available for all common
For the placing on the market of the product in the pipe diameters up to an outer diameter of 168 mm
European Union/European Free Trade Association (tubes).
(EU/EFTA) (with the exception of Switzerland)
Regulation (EU) No. 305/2011 (CPR) applies. The 2.6 Base materials/Ancillary materials
product needs a declaration of performance taking into
consideration EN 14304:2013-04 and the CE-marking. ArmaFlex is a highly flexible insulation material based
For the application and use the respective national on synthetic rubber, which consists of around 20 basic
provisions apply. components. The following table displays the
composition split into functional substance groups.
2.3 Application
AF/ArmaFlex is used to insulate pipes, air ducts and Name Value Unit
vessels including fittings and flanges of industrial Rubber and polymers 24 %
installations and building equipment. Fillers and pigments 3 %
 Condensation control, energy saving and Blowing agent 13 %
noise control in refrigeration and air Vulcanisation system, additives,
37 %
conditioning equipment and process plants. plasticisers
Flame retardant 23 %
 Energy saving according to local energy-
saving laws, prevention of heat loss and noise
Synthetic rubber determines the flexibility;
reduction of heating and plumbing systems.
Fillers determine the fire properties and firmness;
 Condensation control and noise reduction in Blowing agent causes the expansion process during
service-water and waste-water systems. manufacturing;
 Condensation control, energy saving and Accelerator and sulphur enable the vulcanisation;
Plasticizers determine the flexibility;
noise control in refrigeration and air-
Flame retardants ensure fire resistance.
conditioning equipment in the ship-building
sector.
According to the European Chemicals Regulation
REACH manufacturer, importers and downstream
users must register their chemicals and are
2.4 Technical Data responsible for their safe use on their own. For its
production Armacell uses exclusively verifiably
registered and approved substances / mixtures.
Constructional data According to available data and the information
Name Value Unit provided by preliminary suppliers, the product does not
Gross density 52.5 kg/m3 contain substances (SVHC) that are considered
Water vapour diffusion resistance substances meeting the criteria for inclusion in annex
≥ 10000/ ≥
factor acc. to EN 12086, EN - XIV (List of Substances Subject to Authorisation) as
7000
13469/ laid down in Article 57 and article 59 of REACH (EC)
0,033/0,03 1907/2006.). Products manufactured and marketed by
Thermal conductivity 6 (0°C) W/(mK) Armacell do not have to be registered. The products
may contain traces of azodicarbonamide (ACDA).
Maximum service temperature
+110 °C Possible minimal residual amounts are included in the
acc. to EN 14706, EN 14707
polymer matrix. A health impairment can be excluded.
Minimum service temperature -50 °C
For the production of insulation material based on
Tubes: BL-
synthetic rubber, there is presently no alternative to
Reaction to fire acc. to EN 13501- s3, d0/
- ADCA available.
1 Sheets: B-
AF/Armaflex is treated with the antimicrobial biocide
s3, d0
pyrithione zinc.
Structure-borne sound
transmission acc. to EN ISO ≤ 28 dB(A)
3822-1
2.7 Manufacture
Weighted sound absorption
ArmaFlex products are manufactured in a
coefficient αw acc. to EN ISO ≤ 0,45 -
pressureless, continuous and discontinuous production
11654
process.
In the first step, a homogenous compound is produced
Insulation materials on the basis of synthetic rubber do
with rubber, additives, ancillary materials, blowing and
not absorb moisture from the air. For this reason the
vulcanization agents. This is done on the rolling mill or
normal building moisture does not lead to an increase
in the internal mixer followed by the rolling mill.
in thermal conductivity.
Rubber extruders are used to process the compounds
to produce raw profiles with defined dimensions. Here
Performance data of the product in accordance with
exact compliance with the dimensions for the raw
the declaration of performance with respect to its
profile is crucial for the dimensional accuracy of the
essential characteristics according to EN 14304:2013-
foamed product.
04
In the case of the discontinuous, pressureless
production process, the raw profiles are cut to length
2.5 Delivery status
and then foamed in a hot-air oven. In the case of the
FEF made of cross-linked elastomer is supplied as
continuous, pressureless process, the extruded profile
sheets, tubes and shaped pieces. Products with self-
3 Environmental Product Declaration Armacell GmbH – AF/ArmaFlex insulation for industrial and building installation
is fed directly onto a vulcanization line whose energy 2.13 Reference service life
source may be hot air, for example. ArmaFlex products are long-lasting products. Findings
In foam production, vulcanization and blowing show that when used and installed properly they can
processes run alongside each other. Both reactions have an estimated service life of more than 50 years.
are regulated by temperature control. Recipe and It is practically only restricted by the service life of the
temperature control determine the properties of the equipment or whole building, which can extent that
foam. time period. The insulation performance is almost
Quality assurance: completely maintained over the entire service life. The
EC Certificate of conformity no. 0543 of the insulation performance is only compromised by
Gütegemeinschaft Hartschaum e.V. Celle. extraordinary impacts and damage during construction
Quality management system in accordance with EN
ISO 9001.
2.14 Extraordinary effects
2.8 Environment and health during
manufacturing Fire
During all manufacturing steps and at all production According to /EN 13501/, ArmaFlex is classified as a
sites of Armacell, the production follows the national combustible insulation material. Due to its material
guidelines and regulations. A regenerative thermal structure ArmaFlex does not contribute to an
oxidizer is installed to treat exhaust air. uncontrollable spread of fire under installation
Certification of the environmental management system conditions typical on a building site. ArmaFlex does not
is in accordance with ISO 14001. drip under practical fire conditions, this means that fire
spread is ruled out. The product is self-extinguishing
and therefore only makes a minor contribution to the
2.9 Product processing/Installation actual fire event. There is no possibility of the material
The product is installed by using knives. No special self-igniting. ArmaFlex does not propagate the fire
tools, nor specific protection is necessary. either horizontally or vertically.
When applying adhesives the information given in the
relevant safety data sheets is to be heeded. Fire protection
The recommendations for installing the product Name Value
depend on the product and system and are described Tubes: BL
Euro class
in the respective documents (e.g. application manuals) / Sheets B
or the data sheets. More details under Tubes/She
Burning droplets
www.armacell.com. ets: d0
Tubes/She
Smoke development
ets: s3
2.10 Packaging
As a rule, ArmaFlex products are packaged in Water
cardboard boxes and transported on reusable pallets. Armacell insulation materials have a high resistance to
Over-sized rolls of sheet material are packaged in water vapour transmission which keeps possible water
polyethylene (PE) foil. The cardboard boxes can be vapour transmission processes to a minimum
recycled through Interseroh’s dual system. permanently. Therefore, a significant reduction in the
insulation effect can be ruled out permanently.
If the insulation material is exposed to water over a
2.11 Condition of use long period of time (e.g. flooding) it should be replaced.
When the products are used for the purpose for which
they are intended, there are no changes in the material Mechanical destruction
composition during use, except in the event of ArmaFlex insulation materials are flexible foams and
extraordinary impacts (see 2.14). thus display limited mechanical stability. Therefore, if
the material will be subject to greater mechanical
2.12 Environment and health during use impact it should be protected appropriately, e.g. by a
Ingredients: There are no particular aspects of the metal jacket or Arma-Chek covering.
material composition during use. ArmaFlex products (with the exception of
Eurofins Product Testing A/S has tested a wide range HT/ArmaFlex) are not UV resistant. If the material is
and varieties of typical FEF (Flexible Elastomeric subject to UV-rays it should be protected accordingly.
Foam) products marketed in the EU from CEFEP
(European Group of FEF manufacturers). Sampling, 2.15 Re-use phase
testing and evaluation were performed according to If removed properly the product can be re-used.
CEN TS 16516, AgBB, ISO 16000-3, ISO 16000-6, Correctly sorted material can be ground and used to
ISO 16000-9, ISO 16000-11 in the latest versions. manufacture new products (e.g. ArmaSound).
Based on the loading factor 0.05 m²/m³, which was
determined after consideration of real life applications 2.16 Disposal
with FEF products (in living rooms) and Dispose of the materials according to local regulations.
recommendation of experts of the test institute, all Regulated by the European Waste Catalogue: Waste
results were clearly below the limit values. For code 07 02 13 (waste plastic).
example, the determined total volatile organic Note: Please observe Commission Decision
compound (TVOC) after 28 days was for all samples 2001/118/EC.
below 100 mg/m3. Certificates are available on
request.
4 Environmental Product Declaration Armacell GmbH – AF/ArmaFlex insulation for industrial and building installation
2.17 Further information specification clauses for the products are provided at
Further information on ArmaFlex® can be found on the www.armaflex.de.
manufacturer’s website www.armacell.com. Detailed
3. LCA: Calculation rules
3.1 Declared Unit country, the transport distance varies from 500 km to
The declaration refers to 1 m³ insulation product. 800 km
For the LCA calculations the average density per End-of-life (C2, C3):
product brand is used. The transport from place of usage to a waste
As additional information and support for installers the incineration plant is assumed as 100 km.
thermal conductivity coefficient (lambda-value) and R- After the demolition of the product a current realistic
value per 20 cm thickness per product brand are given. End-of-life scenario is the incineration of the material.
According to the reported net calorific value of the
Declared unit materials and the elementary composition, a partial
Name Value Unit stream consideration for the incineration process of
Declared unit 1 m3 PVC-products is applied as an approximation for all
Gross density 52.5 kg/m3 declared products.
Conversion factor to 1 kg 52.5 - Inventory estimations and approximations:
The reported recipes for the rubber mixes contain
Thermal conductivity λ : 0.033 W/(mK (0°C) specific substances of the rubber industry. For these
R-value – thickness: 20 cm: 6.1 (m²K)/W materials only partly life cycle inventories are available.
Approximations are used with the consideration of
similar supply chain effort or similar elementary
composition. Partly an estimation is modelled using
3.2 System boundary pre-products of the specific material and adding an
The data collection refers to the yearly production in energy effort as well as considering the treatment of
2019. The following life cycle stages are considered: production residues for this step in the supply chain.
Type of EPD: Cradle-to-Gate with options. 3.4 Cut-off criteria
In the assessment, all reported data from the
Production A1-A3: production process are considered, utilised thermal
The LCA calculation covers the production of the raw energy, and electric power consumption using best
materials (supply chain – A1), the mixing of raw available life cycle inventory (LCI) datasets. Thus
materials according to the respective recipes material and energy flows contributing less than 1% of
(MasterBatch) exclusively done in Münster, Germany, mass or energy are considered.
the transport (A2) of the MasterBatches to the No cut-off criteria are applied in the foreground data in
production facility for foaming and the foaming process this study.
(A3) in Germany, Spain, Poland or Great Britain, For cut-off criteria in the background system, see
including the packaging material. information provided in the modelling principles and
Transport A4: specific documentations (documentation.gabi-
Average values for the transport from factory gate to software.com).
construction site are assumed.
Installation A5: 3.5 Background data
The installation considers the production of off-cuts, The LCA model is created using the GaBi ts Software
incineration of these off-cuts and the disposal scenario system (v9) for life cycle engineering, developed by
for the packaging material. Auxiliaries like adhesives or Sphera. The GaBi LCI database provides the life cycle
tapes or energy for installation are not considered. inventory data for several of the raw and process
End-of-life C2, C3: materials obtained from the background system. The
An incineration scenario for the used and demolished most recent update of the database was 2020.
product, including an assumption for the transport to
disposal, is covered. 3.6 Data quality
Benefits for the next product system D: The foreground data collected by the manufacturer are
Credits for electrical and thermal energy resulting from based on yearly production amounts and
the waste incineration process of the off-cut material extrapolations of measurements on specific machines
and packaging (A5) and the product (C3) are declared and plants.
in module D. As the average environmental performance of the
product brand has been calculated by a weighting of
the site-specific production volumes the results also
3.3 Estimates and assumptions show a representative picture regarding site specific
Scenario assumptions: production technologies. The average results therefore
Installation (A5): can be assessed as robust.
The additional demand of material for installation Most of the necessary life cycle inventories for the
depends on the specific frame conditions of the basic materials are available in the GaBi database.
building and pipe system to be insulated. Parts of the The last update of the database was in 2020 (Service
product can be joined; thus installation off-cut is very Pack 40)
small. A loss of 1% is assumed. Further LCIs for materials of the supply chain of the
Transport to customer (A4): basic materials are approximated with LCIs of similar
Armacell’s data collectors reported average figures for materials or estimated by the combination of available
the distribution of their material. Depending on the LCIs.
5 Environmental Product Declaration Armacell GmbH – AF/ArmaFlex insulation for industrial and building installation
For electrical and thermal energy regional specific grid All applied incineration processes are displayed via a
mixes and regional specific supply for natural gas are partial stream consideration for the combustion
considered. process, according to the specific composition of the
incinerated material. For the waste incineration plant
3.7 Period under review an R1-value of >0.6 is assumed.
The production data refer to an average of the year Environmental burden of the incineration of installation
2019. residues (off-cuts), packaging and the product in the
end-of-life scenario are assigned to the system (A5 or
3.8 Allocation C3); resulting credits for thermal and electrical energy
Allocation of upstream data: are declared in module D.
For all refinery products, allocation by mass and net The credits for thermal and electrical energy are
calorific value is applied. The specific manufacturing calculated via inversion of the life cycle inventory of
route of every refinery product is modelled and so the European average data.
impacts associated with the production of these Allocation for waste paper:
products are calculated individually. Paper/corrugated board is used as packaging material
Materials and chemicals used in the manufacturing and this usually includes a mix of recycled and virgin
process are modelled using the allocation rule most fibres. When modelling the production of paper, the
suitable for the respective product. For further scrap paper that is used in this process has been
information on a specific product see assumed to be burden free. Similarly, waste paper
documentation.gabi-software.com. arising in the product life cycle is assumed to be
Allocation in the foreground data: recycled. Robust data on paper and cardboard
Part of the production residues (ca. 2%) are used for recycling are not promptly available and refer to a very
the manufacturing of a non-declared product complex system. Hence, to apply this methodology
(ArmaSound). These materials leave the process consistently throughout the model, a cut-off approach
without further consideration of any treatment and has been applied, i.e., input of waste paper is
without credit (cut-off-approach). considered without environmental burden, resulting
No further allocation is applied in the software model. waste paper is not credited. The recycling process and
The overall production of the Armacell production the production process of paper are merged in the
facilities comprises further products beside the production process. The C-balance referring to fresh
products considered in this study. Data for thermal and fibre is corrected via CO2 emissions (biotic)
electrical energy, as well as auxiliary material, refer to (assumption of final rotting or incineration in the time
the declared products only. During data collection the frame of 100 years).
allocation is done via mass, area, pieces or time spent
in the machine, depending on the process step and 3.9 Comparability
reasonable split. The data collectors at Armacell Basically, a comparison or an evaluation of EPD data
decided on the distribution basis. is only possible if all the data sets to be compared
Allocation for waste materials: were created according to EN 15804 and the building
Production waste is sent to a waste incineration plant context, respectively the product-specific
and to landfill (Spain). Resulting electrical and thermal characteristics of performance, are taken into account.
energy from the incineration process is looped inside
module A1-A3. The quality of the recovered energy is The used background dataset DB has been GaBi
assumed to the same as that of the input energy. (service pack 40, 2020).
Landfilling of plastic material is assumed not to deliver
any landfill gas.
4. LCA: Scenarios and additional technical information
Characteristic product properties
Information on biogenic Carbon Information on describing the biogenic Carbon
Content at factory gate
The biogenic carbon content quantifies the amount of Name Value Unit
biogenic carbon in a construction product leaving the Biogenic Carbon Content in
0 kg C
factory gate, and it shall be separately declared for the product
product and for any accompanying packaging.If the Biogenic Carbon Content in
38.39 kg C
total mass of biogenic carbon containing materials is accompanying packaging
less than 5 % of the total mass of the product and The embodied biogenic carbon leaves the system in
accompanying packaging, the declaration of biogenic Module A5.
carbon content may be omitted. The mass of
packaging containing biogenic carbon shall always be The following technical information serves as a basis
declared. for the declared modules. The values refer to the
declared unit of 1 m³.
Note: 1 kg biogenic Carbon is equivalent to 44/12 kg of
CO2 Transport to the building site (A4)
Name Value Unit
0.12 -
Litres of fuel l/100km
0.16
500 -
Transport distance km
800
Capacity utilisation (including empty
85 %
runs)
6 Environmental Product Declaration Armacell GmbH – AF/ArmaFlex insulation for industrial and building installation
Installation into the building (A5)
Name Value Unit
Material loss 1 %
Estimated service life
Name Value Unit
Life Span according to the
50 a
manufacturer
End of life (C1-C4)
Name Value Unit
Energy recovery in WIP 52,5 kg
Reuse, recovery and/or recycling potentials (D),
relevant scenario information
Module D includes the credits of the incineration
processes from A5 (off-cut of product installation,
packaging waste) and C3 (incineration of the product).
A waste incineration plant with an R1-value > 0.6 is
assumed.
7 Environmental Product Declaration Armacell GmbH – AF/ArmaFlex insulation for industrial and building installation
5. LCA: Results
The following information on environmental impacts is expressed with the impact category parameters of LCIA
using characterisation factors. The chosen characterisation factors fulfil the requirements of EN 15804.
Disclaimer:
EP-freshwater: This indicator has been calculated as “kg P eq” as required in the characterization model
(EUTREND model, Struijs et al., 2009b, as implemented in ReCiPe;
http://eplca.jrc.ec.europa.eu/LCDN/developerEF.xhtml)
DESCRIPTION OF THE SYSTEM BOUNDARY (X = INCLUDED IN LCA; ND = MODULE OR INDICATOR NOT
DECLARED; MNR = MODULE NOT RELEVANT)
BENEFITS AND
CONSTRUCTI LOADS
PRODUCT STAGE ON PROCESS USE STAGE END OF LIFE STAGE BEYOND THE
STAGE SYSTEM
BOUNDARIES
8 Environmental Product Declaration Armacell GmbH – AF/ArmaFlex insulation for industrial and building installation
lairetam
waR
ylppus tropsnarT
gnirutcafunaM
eht
morf
tropsnarT
etis
eht
ot
etag
ylbmessA esU
ecnanetniaM
riapeR
tnemecalpeR tnemhsibrufeR
ygrene
lanoitarepO esu
retaw
lanoitarepO esu
noitcurtsnoc-eD
noitilomed tropsnarT
gnissecorp
etsaW
lasopsiD -esueR -yrevoceR -gnilcyceR laitnetop
A1 A2 A3 A4 A5 B1 B2 B3 B4 B5 B6 B7 C1 C2 C3 C4 D
X X X X X ND ND MNR MNR MNR ND ND ND X X ND X
RESULTS OF THE LCA - ENVIRONMENTAL IMPACT according to EN 15804+A2: 1 m³ AF/ArmaFlex
insulation for industrial and building installation
Core Indicator Unit A1-A3 A4 A5 C2 C3 D
Global warming potential - total [kg CO2-Eq.] 1.94E+2 3.82E+0 8.18E+1 2.50E-1 1.36E+2 -3.82E+1
Global warming potential - fossil fuels [kg CO2-Eq.] 2.67E+2 3.79E+0 4.72E+0 2.49E-1 1.36E+2 -3.81E+1
Global warming potential - biogenic [kg CO2-Eq.] -7.43E+1 -6.48E-3 7.71E+1 -4.25E-4 -5.95E-2 -8.93E-2
GWP from land use and land use change [kg CO2-Eq.] 5.43E-1 3.07E-2 6.17E-3 2.02E-3 2.77E-2 -2.66E-2
Depletion potential of the stratospheric ozone layer [kg CFC11-Eq.] 1.44E-9 4.56E-16 1.47E-11 2.99E-17 2.07E-13 -3.96E-13
Acidification potential, accumulated exceedance [mol H+-Eq.] 1.32E+0 1.14E-2 1.62E-2 7.46E-4 4.05E-2 -5.32E-2
Eutrophication, fraction of nutrients reaching freshwater
end compartment
[kg PO4-Eq.] 2.73E-3 1.15E-5 2.81E-5 7.56E-7 3.49E-5 -4.89E-5
Eutrophication, fraction of nutrients reaching marine end
[kg N-Eq.] 1.78E-1 5.06E-3 2.63E-3 3.32E-4 1.34E-2 -1.38E-2
compartment
Eutrophication, accumulated exceedance [mol N-Eq.] 1.72E+0 5.67E-2 2.96E-2 3.72E-3 1.64E-1 -1.48E-1
Formation potential of tropospheric ozone photochemical
[kg NMVOC-Eq.] 7.62E-1 1.00E-2 1.01E-2 6.56E-4 3.79E-2 -3.96E-2
oxidants
Abiotic depletion potential for non-fossil resources [kg Sb-Eq.] 4.41E+3 5.05E+1 5.04E+1 3.31E+0 2.51E+2 -6.46E+2
Abiotic depletion potential for fossil resources [MJ] 1.27E+0 2.72E-7 1.32E-2 1.78E-8 2.98E-6 -6.23E-6
Water (user) deprivation potential, deprivation-weighted [m³ world-Eq
3.09E+1 3.39E-2 1.97E+0 2.22E-3 1.05E+1 -3.93E+0
water consumption (WDP) deprived]
RESULTS OF THE LCA - INDICATORS TO DESCRIBE RESOURCE USE according to EN 15804+A2: 1 m³
AF/ArmaFlex insulation for industrial and building installation
Indicator Unit A1-A3 A4 A5 C2 C3 D
Renewable primary energy as energy carrier [MJ] 1.59E+3 2.84E+0 1.22E+2 1.86E-1 5.21E+1 -1.41E+2
Renewable primary energy resources as material utilization [MJ] 1.04E+2 0.00E+0 -1.04E+2 0.00E+0 0.00E+0 0.00E+0
Total use of renewable primary energy resources [MJ] 1.69E+3 2.84E+0 1.81E+1 1.86E-1 5.21E+1 -1.41E+2
Non-renewable primary energy as energy carrier [MJ] 3.51E+3 5.05E+1 5.79E+1 3.32E+0 1.15E+3 -6.46E+2
Non-renewable primary energy as material utilization [MJ] 9.05E+2 0.00E+0 -7.41E+0 0.00E+0 -8.98E+2 0.00E+0
Total use of non-renewable primary energy resources [MJ] 4.42E+3 5.05E+1 5.05E+1 3.32E+0 2.51E+2 -6.46E+2
Use of secondary material [kg] 4.72E+1 0.00E+0 0.00E+0 0.00E+0 0.00E+0 0.00E+0
Use of renewable secondary fuels [MJ] 0.00E+0 0.00E+0 0.00E+0 0.00E+0 0.00E+0 0.00E+0
Use of non-renewable secondary fuels [MJ] 0.00E+0 0.00E+0 0.00E+0 0.00E+0 0.00E+0 0.00E+0
Use of net fresh water [m³] 1.71E+0 3.29E-3 5.64E-2 2.16E-4 2.76E-1 -1.63E-1
RESULTS OF THE LCA – WASTE CATEGORIES AND OUTPUT FLOWS according to EN 15804+A2:
1 m³ AF/ArmaFlex insulation for industrial and building installation
Indicator Unit A1-A3 A4 A5 C2 C3 D
Hazardous waste disposed [kg] 2.87E-5 2.35E-6 3.29E-7 1.54E-7 1.14E-6 -2.57E-7
Non-hazardous waste disposed [kg] 2.45E+1 7.73E-3 1.23E+0 5.08E-4 8.35E+1 -2.98E-1
Radioactive waste disposed [kg] 1.05E-1 6.25E-5 1.31E-3 4.11E-6 7.97E-3 -4.80E-2
Components for re-use [kg] 0.00E+0 0.00E+0 0.00E+0 0.00E+0 0.00E+0 0.00E+0
Materials for recycling [kg] 0.00E+0 0.00E+0 4.02E+1 0.00E+0 0.00E+0 0.00E+0
Materials for energy recovery [kg] 0.00E+0 0.00E+0 0.00E+0 0.00E+0 0.00E+0 0.00E+0
Exported electrical energy [MJ] 0.00E+0 0.00E+0 2.19E+1 0.00E+0 1.37E+2 0.00E+0
Exported thermal energy [MJ] 0.00E+0 0.00E+0 3.94E+1 0.00E+0 2.50E+2 0.00E+0
RESULTS OF THE LCA – additional impact categories according to EN 15804+A2-optional:
1 m³ AF/ArmaFlex insulation for industrial and building installation
Indicator Unit A1-A3 A4 A5 C2 C3 D
Potential incidence of disease due to PM emissions [Disease
7.60E-5 6.30E-8 8.07E-7 4.13E-9 9.74E-7 -4.52E-7
Incidence]
Potential Human exposure efficiency relative to U235 [kBq U235-
1.05E+1 9.04E-3 1.42E-1 5.94E-4 8.09E-1 -7.87E+0
Eq.]
Potential comparative toxic unit for ecosystems [CTUe] 4.85E+3 3.57E+1 5.01E+1 2.34E+0 2.08E+2 -1.39E+2
Potential comparative toxic unit for humans - cancerogenic [CTUh] 9.12E-8 7.47E-10 1.11E-9 4.90E-11 8.23E-9 -6.03E-9
Potential comparative toxic unit for humans - not cancerogenic [CTUh] 1.22E-5 4.35E-8 1.37E-7 2.85E-9 8.75E-7 -2.24E-7
Potential soil quality index [-] 4.99E+3 1.77E+1 5.19E+1 1.16E+0 5.70E+1 -1.01E+2
Disclaimer 1 – for the indicator IRP
This impact category deals mainly with the eventual impact of low dose ionizingradiation on human health of the
nuclear fuel cycle. It does not consider effects due to possiblenuclear accidents, occupational exposure nor due to
radioactive waste disposal in undergroundfacilities. Potential ionizing radiation from the soil, from radon and some
construction materials is also not measured by this indicator.
Disclaimer 2 – for the indicators ADPE, ADPF, WDP, ETP-fw, HTP-c, HTP-nc, SQP
The results of this environmental impact indicator shall be used with care as the uncertainties on these results are
high or as there is limited experience with the indicator.
6. LCA: Interpretation
The supply chain, i.e. the production of the purchased the overall green house gas emissions. At the same
materials, causes the highest influence on all impact time a credit (D) of 10% is given to the next system,
categories and the primary energy. due to the use of electrical and thermal energy, gained
in the incineration processes for the product and the
Global Warming Potential off-cut material.
Looking at the GWP for the overall declared life cycle
phases, including production (A1-A3), transport (A4, Further impact categories
C2), installation (losses) (A5) and end-of-life (C3, D), The end-of-life scenarios have less influence on the
the production (A1-A3) contributes to 51%. other considered impact categories than on GWP. The
The production in the supply chain (A1) already main contribution of the considered life cycle phases is
contributes 46% to the total GWP value. Thus, every concentrated on module A1-A3.
increase in the production yield directly improves the The energy consumption in the foaming step
environmental performance of the products. influences all impact categories; variations depend on
The foaming process (A3), which includes the the national grid mixes for electricity.
electrical and thermal energy for the mixing, the
vulcanisation and blowing step as well as the Primary Energy Demand
production of the packaging materials, shows a The total primary energy demand is for both categories
significant influence on GWP of the life cycle with 6%. (renewable and non-renewable) significantly (> 100%)
Module A5 covers the production and disposal influenced by the production of the module A1-A3. The
(=incineration) of the off-cut material assumed as 1% other modules play a minor role (C3 with about 5%)
loss in respect to the required insulation material.
Additionally, the emissions of the incineration of The share of primary energy bound as material
packaging material (plastic, wood) in a waste accounts for about 18%, which is partly recovered and
incineration plant are considered. The installation step credited for in module D (-14%)
contributes with 22% to the overall GWP.
As end-of-life scenario an incineration is considered.
The emissions of the product (C3) contribute to 36% to
7. Requisite evidence
recommendation of the experts of the test institute, all
7.1 VOC emissions results were clearly below the limit values. For
Eurofins Product Testing A/S has tested a wide range example the determined total volatile organic
and varieties of typical FEF (Flexible Elastomeric compound (TVOC) after 28 days was for all samples
Foam) products marketed in the EU from CEFEP below 100 mg/m3. Certificates are available on
(European Group of FEF manufacturers). Sampling, request.
testing and evaluation were performed according to
CEN TS 16516, AgBB, ISO 16000-3, ISO 16000-6, 7.2 Leaching performance
ISO 16000-9, ISO 16000-11 in the latest versions. According to EN 13468 is the content of water-soluble
Based on the loading factor 0.05 m²/m³, which were chloride ions for AF/Armaflex ≤ 300 ppm.
determined after consideration of real life applications
with FEF products (in living rooms) and
9 Environmental Product Declaration Armacell GmbH – AF/ArmaFlex insulation for industrial and building installation
8. References
AgBB building equipment and industrial installations -
Umweltbundesamt Germany, Health-related Determination of maximum service temperature
Evaluation of Emissions of Volatile Organic
Compounds (VVOC, VOC and SVOC) from Building EN 14707
Products EN 14707: 2013-01: Thermal insulating products for
building equipment and industrial installations -
CEFEP Determination of maximum service temperature for
The industry association for FEF and PEF insulation preformed pipe insulation
(Celle) in 2012
EN 15801
CEN TS 16516 EN 15801: 2010-04: Conservation of cultural property -
CEN TS 16516:2013-12: Construction products - Test methods - Determination of water absorption by
Assessment of release of dangerous substances - capillarity
Determination of emissions into indoor air
EN 15804
Comission Decision 2001/118/EC EN 15804:2012-04+A1 2013, Sustainability of
Amendment to European Waste Catalogue construction works — Environmental Product
Declarations — Core rules for the product category of
CPR construction products.
Regulation (EC) No 305/2011, Construction Products
Regulation EN 15804
EN 15804:2019+A2 (in press), Sustainability of
EN 826 construction works — Environmental Product
EN 826: 2013-05: Thermal insulating products for Declarations — Core rules for the product category of
building applications - Determination of compression construction products.
behaviour
EN 29052
EN 1606 EN 29052: 1992-08: Acoustics; determination of
EN 1606: 2013-05: Thermal insulating products for dynamic stiffness; part 1: materials used under floating
building applications - Determination of compressive floors in dwellings
creep
EU/EFTA
EN 12091 Regulation (EU) No. 305/2011 (CPR), European
EN 12091: 2013-06: Thermal insulating products for Union/European Free Trade Association (EU/EFTA)
building applications - Determination of freeze-thaw
resistance Eurofins Product Testing A/S
Eurofins Miljo, Smedeskowej 38, 8464 Galten,
EN 12086 Denmark
EN 12086:2013-06: Thermal insulating products for
building applications - Determination of water vapour European Waste Catalogue
transmission properties European Waste Catalogue and Hazardous Waste
List, Commission Decision 2000/532/EC
EN 13468
EN 13468: 2001-12: Thermal insulating products for GaBi
building equipment and industrial installations - GaBi 9 software-system and databases, LBP,
Determination of trace quantities of water soluble University of Stuttgart and Sphera, Leinfelden-
chloride, fluoride, silicate, and sodium ions and pH Echterdingen, 2020 (http://documentation.gabi-
software.com/)
EN 13469
EN 13469:2013-01: Thermal insulating products for IBU
building equipment and industrial installations - Institut Bauen und Umwelt e.V.: General Programme
Determination of water vapour transmission properties Instructions for the Preparation of EPDs at the Institut
of preformed pipe insulation Bauen und Umwelt e.V. Version 1., Berlin: Institut
Bauen und Umwelt e.V., 2016. www.ibu-epd.com
EN 13501-1
EN 13501-1: 2010-01: Fire classification of IBU PCR Part A
construction products and building elements - Part 1: PCR - Part A: Calculation Rules for the Life Cycle
Classification using data from reaction to fire tests Assessment and Requirements on the Project Report,
Institut Bauen und Umwelt e.V., www.ibu-epd.com,
EN 14304 2019.
EN 14304:2013-04: Thermal insulation products for
building equipment and industrial installations – IBU PCR PART B
Factory made flexible elastomeric foam (FEF) products PCR – Part B: Requirements on the EPD for Insulation
– Specification materials made of foam plastics, version 1.7, 01-2019 ,
Institut Bauen und Umwelt e.V., www.ibu-epd.com,
EN 14706 2019
EN 14706: 2013-01: Thermal insulating products for
10 Environmental Product Declaration Armacell GmbH – AF/ArmaFlex insulation for industrial and building installation
ISO 3822-1 Determination of the emission of volatile organic
ISO 3822-1: 1999-05: Acoustics - Laboratory tests on compounds from building products and furnishing -
noise emission from appliances and equipment used in Sampling, storage of samples and preparation of test
water supply installations - Part 1: Method of specimens
measurement
ISO 16000-3
ISO 9001 ISO 16000-3:2011-10: Determination of formaldehyde
ISO 9001:2014-08: Quality management systems – and other carbonyl compounds in indoor air and test
Requirements chamber air - Active sampling method
ISO 11654 ISO 16000-6
ISO 11654: 1997-04: Acoustics - Sound absorbers for ISO 16000-6:2011-12: Indoor air - Part 6:
use in buildings - Rating of sound absorption Determination of volatile organic compounds in indoor
and test chamber air by active sampling on Tenax TA®
ISO 14001 sorbent, thermal desorption and gas chromatography
ISO 14001:2015, Environmental management systems using MS or MS-FID
— Requirements with guidance for use
ISO 16000-9
ISO 14025 ISO 16000-9:2006-02: Indoor air - Part 9:
ISO 14025:2011-10, Environmental labels and Determination of the emission of volatile organic
declarations — Type III environmental declarations — compounds from building products and furnishing -
Principles and procedures. Emission test chamber method
ISO 14040
ISO 14040:2009-11: Environmental management – REACH
Life cycle assessment – Principles and framework Regulation (EC) No 1907/2006, Regulation concerning
the Registration, Evaluation, Authorisation and
ISO 14044 Restriction of Chemicals (REACH)
ISO 14044:2006-10: Environmental management –
Life cycle assessment – Requirements and guidelines
ISO 15868
ISO 15686:2011-05, Buildings and constructed assets
- Service life planning
ISO 16000-11
ISO 16000-11: 2006-02: Indoor air - Part 11:
11 Environmental Product Declaration Armacell GmbH – AF/ArmaFlex insulation for industrial and building installation
Publisher
Institut Bauen und Umwelt e.V. Tel +49 (0)30 3087748- 0
Panoramastr. 1 Fax +49 (0)30 3087748- 29
10178 Berlin Mail info@ibu-epd.com
Germany Web www.ibu-epd.com
Programme holder
Institut Bauen und Umwelt e.V. Tel +49 (0)30 - 3087748- 0
Panoramastr 1 Fax +49 (0)30 – 3087748 - 29
10178 Berlin Mail info@ibu-epd.com
Germany Web www.ibu-epd.com
Author of the Life Cycle
Assessment Tel +49 711 341817-0
Sphera Solutions GmbH Fax +49 711 341817-25
Hauptstraße 111- 113 Mail info@sphera.com
70771 Leinfelden-Echterdingen Web http://www.sphera.com
Germany
Owner of the Declaration
Armacell GmbH Tel +49-251-7603-0
Robert-Bosch-Str. 10 Fax +49-251-7603-346
48153 Münster Mail info.de@armacell.com
Germany Web www.armacell.de
