ENVIRONMENTAL PRODUCT DECLARATION
In accordance with ISO 14025 and EN 15804+A2
Heidelberg Materials UK – UK average C28/35 CIIIA Ready-mixed concrete
Owner of the declaration Program operator:
Heidelberg Materials UK EPD-Norge
Second Floor, Arena Court Majorstuen P.O. Box 5250
SL6 8QZ Maidenhead N-0303 Oslo
United Kingdom Norway
Product Declaration number
UK average C28/35 CIIIA Ready-mixed NEPD-7893-7537-2
concrete
Registration number
Declared product / Declared unit NEPD-7893-7537-2
1 m³ of UK average C28/35 CIIIA Ready-
Issue date
mixed concrete
21.10.2024
This declaration is based on Product
Valid to
Category Rules
21.10.2029
EN 15804:2012 + A2:2019,
NPCR 020 PART B for concrete and concrete EPD Software
elements (v3.0) Emidat EPD Tool v1.0.0
EPD for the best environmental decision 1
General Information
Product Contact person
UK average C28/35 CIIIA Ready-mixed concrete epd@uk.heidelbergmaterials.com
Program Operator Phone
EPD-Norge 01628 774100
Majorstuen P.O. Box 5250
Email
N-0303 Oslo
epd@uk.heidelbergmaterials.com
Norway
Phone: +47 23 08 80 00
Manufacturer
Email: post@epd-norge.no
Heidelberg Materials UK
Second Floor, Arena Court
Declaration Number
SL6 8QZ Maidenhead, United Kingdom
NEPD-7893-7537-2
Place of production
This declaration is based on Product Category Rules
Maidenhead, United Kingdom
EN 15804:2012 + A2:2019,
NPCR 020 PART B for concrete and concrete elements
Management system
(v3.0)
ISO 9001, ISO 14001, ISO 45003, BES 6001, ISO 50001
Statements
Issue date
The owner of the declaration shall be liable for the
21.10.2024
underlying information and evidence. EPD Norway shall not
be liable with respect to manufacturer, life cycle Valid to
assessment data and evidences. 21.10.2029
Declared unit Year of study
1 m³ of UK average C28/35 CIIIA Ready-mixed concrete 2022
General information on verification of EPD from EPD Comparability
tools EPDs of construction products may not be comparable if
Independent verification of data, other environmental they do not comply with EN 15804 and are not seen in a
information and the declaration according to ISO building context. EPD data may not be comparable if the
14025:2010, § 8.1.3 and § 8.1.4. Verification of each EPD is datasets used are not developed in accordance with EN
made according to EPDNorway's guidelines for verification 15804 and if the background systems are not based on the
and approval requiring that tools are i) integrated into the same database (including primary and secondary data).
company's environmental management system, ii) the
Development and verification of EPD
procedures for use of the EPD tool are approved by EPD-
The declaration was created using the Emidat EPD tool
Norway, and iii) the process is reviewed annually by an
v1.0, developed by Emidat GmbH. The EPD tool has been
independent third party verifier. See Appendix G of EPD-
approved by EPD Norway.
Norway's General Programme Instructions for further
information on EPD tools.
Developer of EPD: Nicola Johnson
Verification of EPD tool Reviewer of company-specific input data and EPD: Dominic
Charlotte Merlin, FORCE Technology Doyle
(no signature required)
Approved
Owner of the declaration
Heidelberg Materials UK
Håkon Hauan, CEO EPD-Norge
EPD for the best environmental decision 2
Product
Product description
Concrete is a building material made up of several components, including cement, water, sand, gravel, and air. Ready-mixed
concrete is manufactured in a batch plant in a controlled environment, using precise mix designs (with the addition of other
cementitious materials or chemical admixtures that improve the properties of the concrete), ensuring consistency in quality,
strength, and composition. This consistency leads to predictable performance in construction projects. Ready-mixed concrete
is then delivered to the construction site in an unhardened state, ready to use, eliminating the need for on-site mixing. This
saves time in labour, equipment setup, and material handling, speeding up the construction process. The product is produced
according to BS 8500 and BS EN 206. Testing was conducted according to BS EN 12350 and BS EN 12390. Performance data
of the product with respect to its characteristics in accordance with the relevant technical provision (no CE-marking).
🪨 Admixtures
🪨 Cement
🪨 GGBS UK average
Mixing and C28/35 CIIIA
🪨 Natural blending Ready-mixed
aggregates concrete
🪨 Sand
🪨 Water
The most common man-made substance in the world is concrete. Regardless of the magnitude of the construction, it is a
necessary component of roads, buildings, bridges, dams, pavements, pipelines, sewers, and other structures. It is made up of
naturally occurring aggregates with varying granulometries (sand, fine gravel, and gravel) joined by hydrated cement paste.
To improve particular qualities of the fresh or hardened concrete, such as workability, durability, or early and final strength,
chemical admixtures can also be used. After manufacture, concrete is workable enough to be transported, poured, pumped,
put in place, and compacted at the project site, where it gradually solidifies and gains strength.
Product specification
Name of ingredient Share of total weight Country of origin
Admixtures 0 - 2 % United Kingdom
Cement 2 - 10 % United Kingdom
GGBS 2 - 10 % United Kingdom
Natural aggregates 50 - 80 % United Kingdom
Sand 10 - 25 % United Kingdom
Water 2 - 10 % United Kingdom
Technical data
Unit Value
Compressive Strength (Cylinder) N / mm² 28.0
Compressive Strength (Cube) N / mm² 35.0
Gross Density kg / m³ 2310.0
Market
United Kingdom
Reference service life
50 years
EPD for the best environmental decision 3
LCA: Calculation rules
Declared unit
1 m³ of UK average C28/35 CIIIA Ready-mixed concrete
Reference service life
50 years
System boundary
Data quality
The Emidat EPD Tool v1.0.0 was used for LCA modeling and calculation. Background data was used from ecoinvent database
v3.10.
EPD for the best environmental decision 4
System boundaries (X=included, MND=module not declared)
Next product
Production Installation Use stage End-of-Life
system
Module A1 A2 A3 A4 A5 B1 B2 B3 B4 B5 B6 B7 C1 C2 C3 C4 D
Modules
x x x x x x MND MND MND MND MND MND x x x x x
declared
Geography GB GB GB GB MND MND MND MND MND MND GB GB GB GB GB
For the geographies modeled in A1 and A2, refer to Product specification.
Type of EPD: cradle to gate with options, modules C1-C4 and module D (A1-A3, C, D, additional modules A4, A5, and B1)
Stage of Material Production and Construction
Module A1: Extraction and processing of raw materials
Module A2: Transportation of raw materials to the plant
Module A3: Concrete production at the plant and waste treatment
Module A4: Transportation to the construction site
Module A5: Includes processes associated with concrete installation (e.g., pumping on the construction site), as well as the production, transportation, and
treatment of unused concrete
Use Stage
Module B1: Carbonation during the utilization phase
Disposal Stage
Module C1: Demolition/Dismantling
Module C2: Transportation of concrete demolition waste for processing
Module C3: Sorting of waste components and recycling of concrete
Module C4: Disposal of concrete
Credits and burdens outside the system boundaries
Module D: Credits and burdens from the use of demolished concrete as a replacement for primary materials
Cut-off criteria
Environmental impacts of the following processes are considered to be negligible: Production and use of formwork and
falsework for the installation of concrete, Materials used for the curing of concrete (e.g. plastics, aluminum).
Allocation
Elementary flows (energy and fuels, ancillary materials and waste) data was collected on production-process-level. Using the
total output of the production process in 2022, elementary flows are assigned to 1 declared unit based on volume.
EPD for the best environmental decision 5
ylppus
lairetam
waR
tropsnarT
gnirutcafunaM
tropsnarT
ssecorP
noitallatsnI
esU
ecnanetniaM
riapeR
tnemecalpeR
tnemhsibrufeR
esU
ygrenE
lanoitarepO
esU
retaW
lanoitarepO noitilomeD
tropsnarT
gnissecorP
etsaW
lasopsiD
dnoyeb
sdaol
dna
stfieneB
yradnuob
metsys
eht
LCA: Scenarios and additional technical information
The following information describe the scenarios in the different modules of the EPD.
Transport to the building site (A4) Value Unit
Transported mass 2310.00 kg
Fuel consumption 5.16 L / 100km
Average distance from manufacturer to construction site 9.00 km
Transport mode truck
Gross density of products transported 2310.00 kg / m³
Formwork and Falsework each contribute less than 1% of the total product CO2 emissions, and are therefore neglected
under cut-off rules. (Kaethner, Burridge, 2012). Other sources: Concrete waste: Adams & Hobbs (2023). Electricity, Diesel:
Ecoinvent benchmark average.
Installation into the building (A5) Value Unit
Formwork - kg
Falsework - kg
Concrete waste (installation losses, typical wastage rate on site) 1.50 %
Distance to waste landfill facility (for installation losses) 50 km
Amount of electricity to pour 1 m3 of concrete 3 kWh
Amount of diesel to pour 1 m3 of concrete 60 MJ
Water 0.29 m³
Wastewater treatment 0.29 m³
Calculation of carbonization according to EN 16757. k-factor results from the concrete's compressive strength and its
application. The cement absorption factor (maximum theoretical CO2 uptake) depends on the average clinker content in
cement. The correction factor results from cement substitutes in the recipe.
Use of the installed product (B1) Value Unit
Reference use period 50 years
Building, inside, without paint
Application
or wallpaper
Degree of carbonation (Dc) 0.40 -
Cement absorption factor 0.49 kg CO₂ / kg Cement
k-factor 6.60 mm / year^0.5
Correction factor 1.00 -
Surface area of concrete 5 m²
EPD for the best environmental decision 6
Carbonation during waste processing is not considered. Recycling rate for concrete of 93% reflects the modeled country.
Source: Department for Environment Food & Rural Affairs (DEFRA), UK statistics on waste, May 2022
(https://www.gov.uk/government/statistics/uk-waste-data/uk-statistics-on-waste).
End of life (C1-C4) Value Unit
Material for recycling (total) 2139.06 kg
Distance to waste recycling facility 50 km
Material for landfill (total) 170.94 kg
Distance to waste landfill facility 50 km
Concrete to recycling 2139.06 kg
Diesel required to demolish 1 kg of concrete 0.06 MJ / kg
PM 10 emissions during the demolishment of 1 kg of concrete 6.0e-05 kg / kg
PM 2.5 emissions during the demolishment of 1 kg of concrete 1.7e-05 kg / kg
Calculation of benefits and loads per EN 15804+A2.
Reuse, recovery and/or recycling potentials (D) Value Unit
Amount of recycled material that system takes in 0 kg
Avoided gravel production 2139.06 kg
EPD for the best environmental decision 7
LCA: Results
Core environmental impact indicators
Indicator Unit A1-3 A4 A5 B1 C1 C2 C3 C4 D
GWP-total kg CO₂-eq. 162.68 (145.40)* 2.15 9.78 -7.04 14.16 11.97 13.12 1.07 -21.47
GWP-fossil kg CO₂-eq. 162.39 (145.15)* 2.15 9.76 -7.04 14.16 11.96 13.12 1.07 -21.42
GWP-biogenic kg CO₂-eq. 0.24 (0.22)* 1.1e-03 0.01 0 1.4e-03 6.0e-03 1.3e-03 1.1e-04 -0.02
GWP-luluc kg CO₂-eq. 0.04 7.6e-04 2.4e-03 0 1.2e-03 4.2e-03 1.1e-03 5.6e-04 -0.02
ODP kg CFC-11-Eq 3.3e-06 4.5e-08 1.9e-07 0 2.2e-07 2.5e-07 2.0e-07 3.1e-08 -1.7e-07
AP mol H+-Eq 0.45 5.1e-03 0.07 0 0.13 0.03 0.12 7.6e-03 -0.13
EP-freshwater kg P-Eq 0.02 1.5e-04 6.0e-04 0 4.1e-04 8.4e-04 3.8e-04 8.9e-05 -6.5e-03
EP-marine kg N-Eq 0.05 1.3e-03 0.03 0 0.06 7.4e-03 0.05 2.9e-03 -0.03
EP-terrestrial mol N-Eq 1.38 0.01 0.31 0 0.65 0.08 0.60 0.03 -0.38
POCP kg NMVOC-Eq 0.39 8.8e-03 0.09 0 0.19 0.05 0.18 0.01 -0.10
ADPE kg Sb-Eq 1.8e-04 6.2e-06 9.0e-06 0 5.1e-06 3.4e-05 4.7e-06 1.7e-06 -1.1e-04
ADPF MJ, net calorific value 1034.87 32.32 125.75 0 185.17 179.56 171.55 26.21 -257.06
WDP m³ world Eq deprived 17.83 0.16 0.73 0 0.45 0.90 0.42 0.07 -32.05
GWP-total: Global Warming Potential - total GWP-fossil: Global warming potential - fossil GWP-biogenic: Global Warming Potential - biogenic GWP-luluc:
Global Warming Potential - luluc ODP: Depletion potential of the stratospheric ozone layer AP: Acidification potential, Accumulated Exceedance EP-
freshwater: Eutrophication potential - freshwater EP-marine: Eutrophication potential - marine EP-terrestrial: Eutrophication potential - terrestrial POCP:
Photochemical Ozone Creation Potential ADPE: Abiotic depletion potential - non-fossil resources ADPF: Abiotic depletion potential - fossil resources WDP:
Water (user) deprivation potential
* The first value is the gross value - it includes the impact from the incineration of secondary fuels. The value in brackets (net value) does not include the
impact from the incineration of secondary fuels.
Additional indicators
Indicator Unit A1-3 A4 A5 B1 C1 C2 C3 C4 D
PM disease incidence ND 2.1e-07 ND 0 2.1e-05 1.2e-06 1.9e-05 1.7e-07 -2.0e-06
IRP kBq U235-Eq ND 0.04 ND 0 0.08 0.22 0.08 0.02 -1.81
ETP-fw CTUe ND 7.66 ND 0 26.24 42.54 24.31 3.58 -117.20
HTP-c CTUh ND 1.4e-08 ND 0 5.5e-08 7.7e-08 5.1e-08 4.8e-09 -1.9e-07
HTP-nc CTUh ND 2.1e-08 ND 0 2.5e-08 1.2e-07 2.3e-08 4.7e-09 -1.7e-07
SQP dimensionless ND 32.50 ND 0 12.97 180.57 12.02 51.57 -240.62
PM: Potential incidence of disease due to PM emissions IRP: Potential Human exposure efficiency relative to U235 ETP-fw: Potential Comparative Toxic Unit
for ecosystems HTP-c: Potential Comparative Toxic Unit for humans - cancer effects HTP-nc: Potential Comparative Toxic Unit for humans - non-cancer
effects SQP: Potential Soil quality index
IRP: This impact category deals mainly with the eventual impact of low dose ionizing radiation on human health of the nuclear fuel cycle. It does not
consider effects due to possible nuclear accidents, occupational exposure nor due to radioactive waste disposal in underground facilities. Potential ionizing
radiation from the soil, from radon and from some construction materials is also not measured by this indicator.
ETP-fw, HTP-c, HTP-nc and SQP: The results of these environmental impact indicators shall be used with care as the uncertainties on these results are high
or as there is limited experienced with these indicators.
EPD for the best environmental decision 8
Use of resources
Indicator Unit A1-3 A4 A5 B1 C1 C2 C3 C4 D
PERE MJ 49.05 0.51 7.86 0 1.13 2.85 1.05 0.24 -23.30
PERM MJ 0.30 0 4.5e-03 0 0 0 -0.28 0 0
PERT MJ 49.35 0.51 7.86 0 1.13 2.85 0.77 0.24 -23.30
PENRE MJ 1024.76 32.32 125.60 0 185.17 179.56 171.55 26.21 -257.07
PENRM MJ 10.17 0 0.15 0 0 0 -9.42 0 0
PENRT MJ 1034.93 32.32 125.75 0 185.17 179.56 162.13 26.21 -257.07
SM kg 173.00 0 2.59 0 0 0 0 0 2139.06
RSF MJ 0 0 0 0 0 0 0 0 0
NRSF MJ 0 0 0 0 0 0 0 0 0
FW m³ 3.18 4.7e-03 0.06 0 0.01 0.03 0.01 0.03 -0.76
PERE: Primary energy resources - renewable: use as energy carrier PERM: Primary energy resources - renewable: used as raw materials PERT: Primary
energy resources - renewable: total PENRE: Primary energy resources - non-renewable: use as energy carrier PENRM: Primary energy resources - non-
renewable: used as raw materials PENRT: Primary energy resources - non-renewable: total SM: Use of secondary material RSF: Renewable secondary fuels
NRSF: Non-renewable secondary fuels FW: Net use of fresh water
Waste flows
Indicator Unit A1-3 A4 A5 B1 C1 C2 C3 C4 D
HWD kg 2.10 0.05 0.17 0 0.21 0.26 0.19 0.03 -2.01
NHWD kg 66.85 0.94 323.01 0 2.83 5.23 2.62 171.61 -35.84
RWD kg ND 9.7e-06 ND 0 2.0e-05 5.4e-05 1.9e-05 4.1e-06 -4.4e-04
HWD: Hazardous waste disposed NHWD: Non hazardous waste disposed RWD: Radioactive waste disposed
Output flows
Indicator Unit A1-3 A4 A5 B1 C1 C2 C3 C4 D
CRU kg 0 0 0 0 0 0 0 0 0
MFR kg 0 0 0 0 0 0 2139.06 0 0
MER kg 0 0 0 0 0 0 0 0 0
EEE MJ 0 0 0 0 0 0 0 0 0
EET MJ 0 0 0 0 0 0 0 0 0
CRU: Components for re-use MFR: Materials for recycling MER: Materials for energy recovery EEE: Exported electrical energy EET: Exported thermal energy
Name Value Unit
Biogenic carbon content in product 0 kg C
Biogenic carbon content in accompanying packaging 0 kg C
EPD for the best environmental decision 9
Additional requirements
Greenhouse gas emissions from the use of electricity in the manufacturing phase
Electricity consumption in the manufacturing phase is composed from the source below. Electricity is represented by data in
ecoinvent 3.10 regionalised for United Kingdom.
Electricity Unit Value
Electricity from grid kg CO₂-eq. / kWh 0.25
Additional environmental information
Additional environmental impact indicators required in NPCR Part A for construction products
Indicator Unit A1-3 A4 A5 B1 C1 C2 C3 C4 D
GWP-IOBC kg CO₂-eq. ND 2.15 ND -7.04 14.16 11.97 13.12 1.07 -21.46
GWP-IOBC: Global Warming Potential - Instantaneous oxidation of biogenic carbon
EPD for the best environmental decision 10
Bibliography
DIN EN ISO 14025:2011-10 Environmental labels and declarations - Type III environmental declarations - Principles and procedures
DIN EN ISO 14040:2021-02 Environmental management - Life cycle assessment - Principles and framework
DIN EN ISO 14044:2021-02 Environmental management - Life cycle assessment - Requirements and guidelines
EN 15804:2012+A2:2019 Sustainability of construction works - Environmental product declarations - Core rules for the product
category of construction products
DIN CENTR 15941:2010-11 Sustainability of construction works - Environmental product declarations - Methodology for selection and use
of generic data
DIN EN 15942:2022-04 Sustainability of construction works - Environmental product declarations - Communication format business-
to-business
ISO 21930:2017-07 Sustainability in buildings and civil engineering works - Core rules for environmental product declarations of
construction products and services
Ecoinvent v3.10 ecoinvent, Zurich, Switzerland, database version 3.10
PCR NPCR 020 PART B for concrete and concrete elements (v3.0)
EN 16757 Sustainability of construction works - Environmental product declarations - Product Category Rules for
concrete and concrete elements
Kaethner, S. C. & Burridge, J. A. Embodied CO2 of structural frames. The Structural Engineer 8 (2012)
Adams, K. & Hobbs, G. Final Report: Wastage Rates for Blocks and Ready-Mix Concrete. Reusefully Ltd for MPA (2023):
https://www.aircrete.co.uk/Sustainability-Environmental/Wastage-Rates.aspx
Dos Santos Gervasio, H. and Dimova, S. Environmental benchmarks for buildings , EUR 29145 EN, Publications Office of the European Union, 2018,
ISBN 978-92-79-80969-9 (print),978-92-79-80970-5 (pdf), doi:10.2760/073513 (online),10.2760/90028 (print),
JRC110085.
Basic principles and recommendations for describing the dismantling, post use, and disposal stage of
construction products: https://www.umweltbundesamt.de/sites/default/files/medien/1410/publikationen/2020-07-06_texte_130-2
020_guidance-document-construction-industry.pdf
ILCD Handbook: https://eplca.jrc.ec.europa.eu/uploads/ILCD-Handbook-LCIA-Background-analysis-online-12March2010.pdf
Program Operator Phone +47 23 08 80 00
EPD-Norge
Majorstuen P.O. Box 5250, N-0303 Oslo Email post@epd-norge.no
Norway Web www.epd-norge.no
Publisher Phone +47 23 08 80 00
The Norwegian EPD Foundation
Post Box 5250 Majorstuen, 0303 Oslo Email post@epd-norge.no
Norway Web www.epd-norge.no
Owner of the declaration Phone 01628 774100
Heidelberg Materials UK
Second Floor, Arena Court, SL6 8QZ Maidenhead Email epd@uk.heidelbergmaterials.com
United Kingdom Web heidelbergmaterials.co.uk
Author of the life cycle assesment Phone 01628 774100
Heidelberg Materials UK
Second Floor, Arena Court, SL6 8QZ Maidenhead Email epd@uk.heidelbergmaterials.com
United Kingdom Web heidelbergmaterials.co.uk
Web www.eco-platform.org
ECO Platform
ECO Portal
Web ECO Portal
Developer of EPD generator Phone +49 176 56 96 77 91
Emidat GmbH
Sandstraße 33, 80335 München Email epd@emidat.com
Germany Web www.emidat.com
EPD for the best environmental decision 11
