Environmental product declaration
In accordance with ISO 14025 and EN 15804 +A2
PN 1,5 FR G/G
Owner of the declaration: Program operator:
Prysmian Group Norge AS The Norwegian EPD Foundation
Declared unit: Declaration number:
1 m PN 1,5 FR G/G
NEPD-3974-3006-EN
This declaration is based on Product Category Rules:
CEN Standard EN 15804:2012+A2:2019 serves as core PCR Registration number:
NPCR 027 Part B for Electrical cables and wires
NEPD-3974-3006-EN
Issue date: 02.12.2022
Valid to: 02.12.2027
The Norwegian EPD Foundation
EPD Software:
LCA.no EPD generator
System ID:
50441
1 / 12
General information
Product Owner of the declaration:
PN 1,5 FR G/G Prysmian Group Norge AS
Contact person: Anders Nymark
Phone: +47 90066733
e-mail: anders.nymark@prysmiangroup.com
Program operator: Manufacturer:
Post Box 5250 Majorstuen, 0303 Oslo, Norway Prysmian Group Norge AS
The Norwegian EPD Foundation Kjerraten 16 , 3013 Drammen
Phone: +47 23 08 80 00 Norway
web: post@epd-norge.no
Declaration number: Place of production:
NEPD-3974-3006-EN Prysmian Group production site Oulu (Finland
Johdintie 5 , 90630 Oulu
Finland
Management system:
This declaration is based on Product Category Rules: ISO 9001, ISO 14001, ISO 45001
CEN Standard EN 15804:2012+A2:2019 serves as core PCR
NPCR 027 Part B for Electrical cables and wires
Organisation no:
Statement of liability: 814 780 422
The owner of the declaration shall be liable for the underlying information and
evidence. EPD Norway shall not be liable with respect t​o manufacturer
information, life cycle assessment data and evidences.
Issue date: 02.12.2022
Declared unit:
1 m PN 1,5 FR G/G
Valid to: 02.12.2027
Declared unit with option:
A1,A2,A3,A4,A5,C1,C2,C3,C4,D
Year of study:
Functional unit: 2021
Comparability:
General information on verification of EPD from EPD tools: EPD of construction products may not be comparable if they not comply with
Independent verification of data, other environmental information and the EN 15804 and seen in a building context.
declaration according to ISO 14025:2010, § 8.1.3 and § 8.1.4. Individualthird party
verification of each EPD is not required when the EPD tool is i) integrated into the
company's environmental management system, ii) the procedures for use of the
EPD tool are approved by EPDNorway, and iii)the proccess is reviewed annualy.
See Appendix G of EPD-Norway's General Programme Instructions for further
information on EPD tools.
Development and verification of EPD:
Verification of EPD tool: The declaration is created using EPD tool lca.tools ver EPD2022.03, developed by
Independent third party verification of the EPD tool, background data and test- LCA.no. The EPD tool is integrated in the company's management system, and
EPD in accordance with EPDNorway's procedures and guidelines for verification has been approved by EPD Norway. Approval number: NEPDT33
and approval of EPD tools. Approval number: NEPDT32.
Developer of EPD:
Third party verifier:
Siri Andersen
Reviewer of company-specific input data and EPD:​
Vito D’Incognito - Take Care International Anders Nymark
(no signature required)
Approved:
2 / 12
Product
Product description:
Cable for open or hidden pipe installation and as a connecting cable. Yellow / red color is allowed for signal reference earth, tele and data
(SRJ). H07V-R.
Product specification
Conductor material Copper
Core insulation material Polyvinyl chloride (PVC)
Material outer sheath Polyvinyl chloride (PVC)
Cable shape Round
Materials kg %
Metal - Copper 0,01 61,52
Plastic - Polyvinyl chloride (PVC) 0,01 38,48
Total 0,02
Technical data:
PN 1,5 FR G/G
Art.Nr: 20075842
Elnummer: 1060703
Cenelec HD 21
Nominal voltage U0 [V] 450
Nominal voltage U [V] 750
Flame retardant Other
Reaction-to-fire class (acc. EN 13501-6) Eca
Max. conductor temperature [°C] 70
Bending radius (rule) 3xD
EN 50525-2-31
IEC 60227-3 Construction
IEC 60332-1 Flame retardant properties
EN 50575:2014+A1:2016 Reaction to fire
Flame retardant Yes
Halogenfree No
IEC 60228 class 2 Conductors
Market:
Norway
Reference service life, product
The reference service life of the product is highly dependent on the
conditions of use. Expected lifetime at least 30 years, provided proper installation, load and ambient temperature.
Reference service life, building or construction works
60 years, standard service life for buildings, according to NPCR 027.
LCA: Calculation rules
Declared unit:
1 m PN 1,5 FR G/G
Cut-off criteria:
All major raw materials and all the essential energy is included. The production processes for raw materials and energy flows with very small amounts (less than 1%) are
not included. These cut-off criteria do not apply for hazardous materials and substances.
Allocation:
The allocation is made in accordance with the provisions of EN 15804. Incoming energy and water and waste production in-house is allocated equally among all products
through mass allocation. Effects of primary production of recycled materials is allocated to the main product in which the material was used. The recycling process and
transportation of the material is allocated to this analysis.
Data quality:
Specific data for the product composition are provided by the manufacturer. The data represent the production of the declared product and were collected for EPD
development in the year of study. Background data is based on EPDs according to EN 15804 and different LCA databases. The data quality of the raw materials in A1 is
presented in the table below.
Materials Source Data quality Year
Metal - Copper ecoinvent 3.6 Database 2019
Plastic - Polyvinyl chloride (PVC) ecoinvent 3.6 Database 2019
3 / 12
System boundaries (X=included, MND=module not declared, MNR=module not relevant)
Construction Beyond the
Product stage installation Use stage End of life stage system
stage boundaries
A1 A2 A3 A4 A5 B1 B2 B3 B4 B5 B6 B7 C1 C2 C3 C4 D
X X X X X MND MND MND MND MND MND MND X X X X X
System boundary:
The flowchart below illustrates the system boundaries of the analysis:
Additional technical information:
This article represents a group of products of identical cross section, but with different colors.
Expenditure of raw materials and energy consumption during manufacturing is the same for all articles listed below.
El no. 1060702 PN 1,5mm2 BLUE, SAP 20075370
El no. 1060704 PN 1,5mm2 BROWN, SAP 20075369
El.no. 1060701 PN 1,5mm2 GREY, SAP 20075373
El.no. 1060700 PN 1,5mm2 LIGHT GREY, SAP 20075844
All articles are delivered on 100% recycled plastic bobbins, with a standard length of 150m.
waR slairetam tropsnarT gnirutcafunaM tropsnarT ylbmessA e​sU ecnanetniaM riapeR tnemecalpeR tnemhsibrufeR lanoitarepO esu ygrene lanoitarepO esu retaw -eD noitcurtsnoc noitilomed tropsnarT etsaW gnissecorp lasopsiD -yrevoceR-esueR -gnilcyceR laitnetop
4 / 12
LCA: Scenarios and additional technical information
The following information describe the scenarios in the different modules of the EPD.
In A4, a transport distance of 1445 km from the Prysmian Group production site in Oulu to Prysmian Group's warehouse in Loesmoen was included. A distance of 300 km
was also added as additional transport to market.
Installation in trenches (A5) and removal (C1) is assumed to be done with other products such as piping systems and should be assessed at a construction works level.
For B1-B7 the default environmental impact and resource indicators in the EPD are assumed to be zero. In C2, a distance of 300 km has been added as average transport to
the Norwegian waste treatment facilities. In C3, datasets are developed for the recycling of metals and plastics and for the incinerations of plastic fractions (including
energy recovery and fly ash extraction). All other minor raw materials in the product are assumed to be incinerated. Net benefit of material recycling and energy recovery
are given in module D.
Capacity utilisation Value
Transport from production place to user (A4) Distance (km) Fuel/Energy Consumption Unit
(incl. return) % (Liter/tonne)
Truck, 16-32 tonnes, EURO 5 (km) 36,7 % 1745 0,044 l/tkm 76,78
Capacity utilisation Value
Transport to waste processing (C2) Distance (km) Fuel/Energy Consumption Unit
(incl. return) % (Liter/tonne)
Truck, 16-32 tonnes, EURO 5 (km) 36,7 % 300 0,044 l/tkm 13,20
Waste processing (C3) Unit Value
Copper to recycling (kg) kg 0,01
Waste treatment of plastic mixture, incineration
kg 0,00
with energy recovery and fly ash extraction (kg)
Disposal (C4) Unit Value
Landfilling of ashes from incineration of Plastic
kg 0,00
mixture, process per kg ashes and residues (kg)
Landfilling of copper (kg) kg 0,01
Landfilling of plastic mixture (kg) kg 0,00
Benefits and loads beyond the system
Unit Value
boundaries (D)
Substitution of primary copper with net scrap (kg) kg 0,00
Substitution of electricity, in Norway (MJ) MJ 0,01
Substitution of thermal energy, district heating, in
MJ 0,09
Norway (MJ)
5 / 12
LCA: Results
The LCA results are presented below for the declared unit defined on page 2 of the EPD document.
Environmental impact
Parameter Unit A1 A2 A3 A4 A5 C1 C2 C3 C4 D
GWP-total
kg CO2 -
1,27E-01 6,29E-03 4,04E-03 6,05E-03 3,04E-03 0 1,04E-03 9,47E-03 5,31E-04 -3,09E-03
eq
GWP-fossil
kg CO2 -
1,25E-01 6,29E-03 3,77E-03 6,05E-03 2,99E-03 0 1,04E-03 9,47E-03 5,31E-04 -3,05E-03
eq
GWP-biogenic
kg CO2 -
2,00E-03 2,65E-06 2,40E-04 2,47E-06 4,49E-05 0 4,24E-07 2,06E-07 4,09E-08 -1,28E-05
eq
GWP-luluc
kg CO2 -
1,21E-04 2,14E-06 2,96E-05 2,11E-06 3,09E-06 0 3,64E-07 3,84E-08 3,76E-08 -2,12E-05
eq
kg
ODP CFC11 - 1,34E-08 1,42E-09 3,90E-10 1,38E-09 3,27E-10 0 2,37E-10 2,10E-11 3,30E-11 -3,93E-05
eq
mol H+
AP 9,07E-03 2,85E-05 1,27E-05 2,47E-05 1,83E-04 0 4,25E-06 2,08E-06 8,81E-07 -4,27E-04
-eq
EP-FreshWater kg P -eq 7,26E-05 5,13E-08 1,22E-07 4,75E-08 1,46E-06 0 8,17E-09 1,83E-09 1,75E-09 -2,89E-06
EP-Marine kg N -eq 4,48E-04 8,99E-06 2,56E-06 7,33E-06 9,30E-06 0 1,26E-06 9,93E-07 7,91E-07 -1,88E-05
mol N
EP-Terrestial 6,62E-03 9,93E-05 2,69E-05 8,11E-05 1,36E-04 0 1,39E-05 1,02E-05 3,54E-06 -2,85E-04
eq
kg
POCP NMVOC 1,78E-03 3,02E-05 6,92E-06 2,48E-05 3,66E-05 0 4,27E-06 2,45E-06 1,10E-06 -7,74E-05
-eq
ADP- Kg Sb-
2,74E-04 1,40E-07 2,35E-08 1,64E-07 5,49E-06 0 2,82E-08 1,04E-09 8,64E-10 -2,37E-06
minerals&metals1 eq
ADP-fossil1 MJ 1,64E+00 9,52E-02 8,30E-02 9,12E-02 3,77E-02 0 1,57E-02 1,30E-03 2,62E-03 -3,02E-02
WDP1 m3 2,35E+00 8,34E-02 4,54E+00 8,70E-02 1,42E-01 0 1,50E-02 9,39E-03 5,17E-02 4,17E-02
GWP total Global Warming Potential total; GWP fossil Global Warming Potential fossil fuels ; GWP biogenic Global Warming Potential biogenic; GWP luluc Global W
Potential land use change; ODP Ozone Depletion; AP Acidification; EP freshwater Eutrophication aquatic freshwater; EP marine Eutrophication aquatic marine; EP
terrestrial Eutrophication terrestrial ;POCP Photochemical zone formation; ADPE Abiotic Depletion Potential minerals and metals; ADPf Abiotic Depletion Potential fossil
fuels;
"Reading example: 9,0 E-03 = 9,0*10-3 = 0,009"
*INA Indicator Not Assessed
1. The results of this environmental impact indicator shall be used with care as the uncertainties on these results are high or as there is limited experienced with the
indicator
Remarks to environmental impacts
6 / 12
Additional environmental impact indicators
Parameter Unit A1 A2 A3 A4 A5 C1 C2 C3 C4 D
PM Disease incidence 2,15E-08 5,02E-10 6,20E-11 4,36E-10 4,47E-10 0 7,50E-11 9,00E-12 1,60E-11 -1,11E-09
IRP2 kgBq U235 eq. 4,94E-03 4,15E-04 2,01E-03 3,99E-04 1,54E-04 0 6,86E-05 3,27E-06 1,58E-05 -7,71E-05
ETP-fw1 CTUe 8,88E+01 7,11E-02 6,34E-02 6,72E-02 1,84E+00 0 1,16E-02 2,00E-02 3,17E+00 -3,93E+00
HTP-c1 CTUh 1,23E-09 0,00E+00 1,00E-12 0,00E+00 2,50E-11 0 0,00E+00 1,00E-12 0,00E+00 -5,60E-11
HTP-nc1 CTUh 1,02E-07 7,60E-11 4,90E-11 7,30E-11 2,04E-09 0 1,20E-11 2,50E-11 4,00E-12 -4,74E-09
SQP1 Pt 1,29E+00 8,14E-02 5,08E-02 6,29E-02 2,91E-02 0 1,08E-02 2,38E-04 6,43E-03 -1,01E-01
PM Particulate Matter emissions; IRP Ionizing radiation – human health; ETP-fw Eco toxicity – freshwater; HTP-c Human toxicity – cancer effects; HTP-nc Human
toxicity – non cancer effects; SQP Soil Quality (dimensionless)
"Reading example: 9,0 E-03 = 9,0*10-3 = 0,009"
*INA Indicator Not Assessed
1. The results of this environmental impact indicator shall be used with care as the uncertainties on these results are high or as there is limited experienced with the
indicator
2. This impact category deals mainly with the eventual impact of low dose ionizing radiation on human health of the nuclear fuel cycle. It does not consider effects due
to possible nuclear accidents, occupational exposure nor due to radioactive waste disposal in underground facilities. Potential ionizing radiation from the soil, from
radon and from some construction materials is also not measured by this indicator.
7 / 12
Resource use
Parameter Unit A1 A2 A3 A4 A5 C1 C2 C3 C4 D
PERE MJ 2,95E-01 1,36E-03 2,54E-02 1,29E-03 6,45E-03 0 2,21E-04 7,25E-05 2,80E-04 -5,66E-02
PERM MJ 0,00E+00 0,00E+00 0,00E+00 0,00E+00 0,00E+00 0 0,00E+00 0,00E+00 0,00E+00 0,00E+00
PERT MJ 2,95E-01 1,36E-03 2,54E-02 1,29E-03 6,45E-03 0 2,21E-04 7,24E-05 2,80E-04 -5,66E-02
PENRE MJ 1,47E+00 9,52E-02 8,59E-02 9,12E-02 3,44E-02 0 1,57E-02 1,30E-03 2,62E-03 -3,02E-02
PENRM MJ 1,69E-01 0,00E+00 0,00E+00 0,00E+00 3,42E-05 0 0,00E+00 -1,67E-01 0,00E+00 0,00E+00
PENRT MJ 1,64E+00 9,52E-02 8,59E-02 9,12E-02 3,44E-02 0 1,57E-02 -1,66E-01 2,62E-03 -6,35E-02
SM kg 6,85E-03 0,00E+00 3,50E-05 0,00E+00 1,38E-04 0 0,00E+00 0,00E+00 2,71E-05 7,36E-04
RSF MJ 3,42E-03 4,62E-05 2,99E-04 4,61E-05 7,62E-05 0 7,92E-06 1,56E-06 5,80E-06 6,16E-05
NRSF MJ 1,93E-03 1,78E-04 9,54E-04 1,64E-04 6,33E-05 0 2,83E-05 -7,16E-06 -3,57E-07 -2,67E-03
FW m3 1,99E-03 1,07E-05 1,16E-04 9,61E-06 4,27E-05 0 1,65E-06 1,10E-05 3,37E-06 -1,19E-04
PERE Use of renewable primary energy excluding renewable primary energy resources used as raw materials; PERM Use of renewable primary energy resources used as
raw materials; PERT Total use of renewable primary energy resources; PENRE Use of non renewable primary energy excluding non-renewable primary energy resources
used as raw materials; PENRM Use of non renewable primary energy resources used as raw materials; PENRT Total use of non renewable primary energy resources; SM
Use of secondary materials; RSF Use of renewable secondary fuels; NRSF Use of non renewable secondary fuels; FW Use of net fresh water
"Reading example: 9,0 E-03 = 9,0*10-3 = 0,009"
*INA Indicator Not Assessed
8 / 12
End of life - Waste
Parameter Unit A1 A2 A3 A4 A5 C1 C2 C3 C4 D
HWD kg 8,76E-04 5,20E-06 4,44E-04 4,65E-06 3,05E-05 0 8,00E-07 5,18E-07 1,96E-04 -2,89E-05
NHWD kg 3,34E-02 5,75E-03 6,63E-04 4,36E-03 1,02E-03 0 7,50E-04 2,71E-05 9,20E-03 -1,39E-03
RWD kg 4,87E-06 6,46E-07 9,25E-07 6,22E-07 1,38E-07 0 1,07E-07 3,77E-09 1,79E-08 -6,56E-08
HWD = Hazardous waste disposed; NHWD = Non-hazardous waste disposed; RWD = Radioactive waste disposed;
"Reading example: 9,0 E-03 = 9,0*10-3 = 0,009"
*INA Indicator Not Assessed
End of life - Output flow
Parameter Unit A1 A2 A3 A4 A5 C1 C2 C3 C4 D
CRU kg 0,00E+00 0,00E+00 0,00E+00 0,00E+00 0,00E+00 0 0,00E+00 0,00E+00 0,00E+00 0,00E+00
MFR kg 0,00E+00 0,00E+00 3,28E-05 0,00E+00 1,54E-04 0 0,00E+00 7,68E-03 4,07E-07 -2,88E-05
MER kg 0,00E+00 0,00E+00 2,98E-06 0,00E+00 7,30E-08 0 0,00E+00 1,63E-08 6,55E-07 -3,79E-06
EEE MJ 0,00E+00 0,00E+00 1,17E-03 0,00E+00 1,46E-04 0 0,00E+00 6,15E-03 6,31E-06 -9,29E-06
EET MJ 0,00E+00 0,00E+00 1,77E-02 0,00E+00 2,22E-03 0 0,00E+00 9,30E-02 9,54E-05 -1,41E-04
CRU = Components for re-use; MFR = Materials for recycling; MER = Materials for energy recovery; EEE = Exported electrical energy; EET = Exported energy ​ Thermal
"Reading example: 9,0 E-03 = 9,0*10-3 = 0,009"
*INA Indicator Not Assessed
Biogenic Carbon Content
Parameter Unit At the factory gate
Biogenic carbon content in product kg C 0,00E+00
Biogenic carbon content in accompanying packaging kg C 0,00E+00
Note: 1 kg biogenic carbon is equivalent to 44/12 kg CO2
9 / 12
Additional Norwegian requirements
Greenhouse gas emissions from the use of electricity in the manufacturing phase
National production mix from import, low voltage (production of transmission lines, in addition to direct emissions and losses in grid) of applied electricity for the
manufacturing process (A3).
Electricity mix Data source Amount Unit
Electricity, Finland (kWh) ecoinvent 3.6 255,20 g CO2-eq/kWh
Dangerous substances
The product contains no substances given by the REACH Candidate list or the Norwegian priority list.
Indoor environment
No known impact on indoor environment.
Additional Environmental Information
Environmental impact indicators EN 15804+A1 and NPCR Part A v2.0
Parameter Unit A1 A2 A3 A4 A5 C1 C2 C3 C4 D
GWP kg CO2 -eq 1,22E-01 6,22E-03 4,82E-03 5,99E-03 2,95E-03 0 1,03E-03 9,47E-03 4,42E-04 -2,98E-03
ODP kg CFC11 -eq 1,25E-08 1,13E-09 5,71E-10 1,09E-09 3,01E-10 0 1,87E-10 1,90E-11 2,80E-11 -1,61E-10
POCP kg C2H4-eq 3,03E-04 8,60E-07 4,94E-07 8,00E-07 6,09E-06 0 1,38E-07 3,00E-08 8,50E-08 -1,47E-05
AP kg SO2 -eq 7,69E-03 1,45E-05 9,99E-06 1,19E-05 1,54E-04 0 2,04E-06 1,45E-06 3,76E-07 -3,64E-04
EP kg PO43- -eq 3,90E-04 1,86E-06 1,50E-06 1,27E-06 7,89E-06 0 2,18E-07 4,90E-07 2,74E-07 -1,61E-05
ADPM kg Sb -eq 2,74E-04 1,40E-07 2,35E-08 1,64E-07 5,49E-06 0 2,82E-08 1,04E-09 9,13E-10 -2,37E-06
ADPE MJ 1,48E+00 9,32E-02 8,66E-02 8,94E-02 3,45E-02 0 1,54E-02 1,30E-03 2,40E-03 -2,93E-02
GWPIOBC kg CO2 -eq 1,27E-01 6,29E-03 3,60E-03 6,05E-03 3,02E-03 0 1,04E-03 9,47E-03 1,00E-04 -1,74E-03
GWP Global warming potential; ODP Depletion potential of the stratospheric ozone layer; POCP Formation potential of tropospheric photochemical oxidants; AP
Acidification potential of land and water; EP Eutrophication potential; ADPM Abiotic depletion potential for non fossil resources; ADPE Abiotic depletion​ potential for
fossil resources; GWP-IOBC/GHG Global warming potential calculated according to the principle of instantanious oxidation (except emissions and uptake of biogenic
carbon)
10 / 12
Bibliography
ISO 14025:2010. Environmental labels and declarations - Type III environmental declarations - Principles and procedures. International Organization for Standardization.
ISO 14044:2006. Environmental management - Life cycle assessment - Requirements and guidelines. International Organization for Standardization.
EN 15804:2012+A2:2019. Environmental product declaration - Core rules for the product category of construction products. European Committee for Standardization.
ISO 21930:2017. Sustainability in buildings and civil engineering works - Core rules for environmental product declarations of construction products. International
Organization for Standardization.
EN 50693:2019. Product category rules for life cycle assessments of electronic and electrical products and systems. European Committee for Standardization.
Ecoinvent v3, 2019. Allocation, cut-off by classification. Swiss Centre of Life Cycle Inventories.
Iversen et al., (2021). eEPD v2021.09, background information for EPD generator tool system verification, LCA.no. Report number: 07.21. System verification report.
Philis et al., (2022). EPD generator for NPCR 027 part B for electrical wires and cables, background information for EPD generator application and LCA data, LCA.no Report
number: 03.22. PCR verification report.
EPD Norway (2022). NPCR Part A: Construction products and services. The Norwegian EPD foundation. Version 2.0 published 24.03.2021.
EPD Norway (2022). NPCR 027 Part B for electrical cables and wires. The Norwegian EPD foundation. Version 2.0 published 01.03.2022.
Program operator and publisher Phone: +47 23 08 80 00
The Norwegian EPD Foundation e-mail: post@epd-norge.no
Post Box 5250 Majorstuen, 0303 Oslo, Norway web: www.epd-norge.no
Owner of the declaration: Phone: +47 90066733
Prysmian Group Norge AS e-mail: anders.nymark@prysmiangroup.com
Kjerraten 16, 3013 Drammen web: www.prysmiangroup.no
Author of the Life Cycle Assessment Phone: +47 916 50 916
LCA.no AS e-mail: post@lca.no
Dokka 6B, 1671 web: www.lca.no
Developer of EPD generator Phone: +47 916 50 916
LCA.no AS e-mail: post@lca.no
Dokka 6B,1671 Kråkerøy web: www.lca.no
ECO Platform Web: www.eco-platform.org
ECO Portal Web: ECO Portal
11 / 12
EPD for the best
environmental
decision
The Norwegian EPD Foundation
www.epd-norge.no
12 / 12
