Environmental product declaration
In accordance with ISO 14025 and EN 15804 +A2
IFSI-EMC Pure 4x240FV/120mm2
Owner of the declaration: Program operator:
Prysmian Group Norge AS The Norwegian EPD Foundation
Declared unit: Declaration number:
1 m IFSI-EMC Pure 4x240FV/120mm2
NEPD-3960-2998-EN
This declaration is based on Product Category Rules:
CEN Standard EN 15804:2012+A2:2019 serves as core PCR Registration number:
NPCR 027 Part B for Electrical cables and wires
NEPD-3960-2998-EN
Issue date: 29.11.2022
Valid to: 29.11.2027
The Norwegian EPD Foundation
EPD Software:
LCA.no EPD generator
System ID:
55064
1 / 12
General information
Product Owner of the declaration:
IFSI-EMC Pure 4x240FV/120mm2 Prysmian Group Norge AS
Contact person: Anders Nymark
Phone: +47 90066733
e-mail: anders.nymark@prysmiangroup.com
Program operator: Manufacturer:
Post Box 5250 Majorstuen, 0303 Oslo, Norway Prysmian Group Norge AS
The Norwegian EPD Foundation Kjerraten 16 , 3013 Drammen
Phone: +47 23 08 80 00 Norway
web: post@epd-norge.no
Declaration number: Place of production:
NEPD-3960-2998-EN Prysmian Group production site Nässjö (Sweden
Vallgatan 5 , 571 41 Nässjö
Sweden
Management system:
This declaration is based on Product Category Rules: ISO 9001, ISO 14001, ISO 45001
CEN Standard EN 15804:2012+A2:2019 serves as core PCR
NPCR 027 Part B for Electrical cables and wires
Organisation no:
Statement of liability: 814 780 422
The owner of the declaration shall be liable for the underlying information and
evidence. EPD Norway shall not be liable with respect t​o manufacturer
information, life cycle assessment data and evidences.
Issue date: 29.11.2022
Declared unit:
1 m IFSI-EMC Pure 4x240FV/120mm2
Valid to: 29.11.2027
Declared unit with option:
A1,A2,A3,A4,A5,B1,B2,B3,B4,B5,B6,B7,C1,C2,C3,C4,D
Year of study:
Functional unit: 2021
1 m of installed IFSI-EMC Pure 4x240/120mm2, used to transmit a reference
energy throughput of 1A over a period of 40 years.
Comparability:
General information on verification of EPD from EPD tools: EPD of construction products may not be comparable if they not comply with
Independent verification of data, other environmental information and the EN 15804 and seen in a building context.
declaration according to ISO 14025:2010, § 8.1.3 and § 8.1.4. Individualthird party
verification of each EPD is not required when the EPD tool is i) integrated into the
company's environmental management system, ii) the procedures for use of the
EPD tool are approved by EPDNorway, and iii)the proccess is reviewed annualy.
See Appendix G of EPD-Norway's General Programme Instructions for further
information on EPD tools.
Development and verification of EPD:
Verification of EPD tool: The declaration is created using EPD tool lca.tools ver EPD2022.03, developed by
Independent third party verification of the EPD tool, background data and test- LCA.no. The EPD tool is integrated in the company's management system, and
EPD in accordance with EPDNorway's procedures and guidelines for verification has been approved by EPD Norway. Approval number: NEPDT33
and approval of EPD tools. Approval number: NEPDT32.
Developer of EPD:
Third party verifier:
Siri Andersen
Reviewer of company-specific input data and EPD:​
Vito D’Incognito - Take Care International Anders Nymark
(no signature required)
Approved:
2 / 12
Product
Product description:
Power cable with up to 1 kV operating voltage.
Allowed indoors, outdoors and as a ground cable without extra protection. The Cu screen is 100% tight, has low coupling impedance and meets the EMC directive. The 3-
conductor is symmetrically constructed and has a cu screen from 1.5mm² wire. Halogen-free cable is recommended used when it is important to avoid the formation of
dense smoke and corrosive gases in the event of an overheating or fire. This cable is well suited as a sea cable down to 20m if it is protected against mechanical stress. The
insulation material is PEX, with good seawater resistance.
Product specification
Conductor material Copper
Conductor surface Bare
Core insulation material XLPE
Armoring/reinforcement material Copper, bare
Screen construction Metallised foil
Screen Yes
Screen material Copper, bare
Concentric conductor Copper
Material inner sheath Halogen-free polymer
Material outer sheath Halogen-free polymer
Cable shape Round
Materials kg %
HFFR Polyolefin 0,65 6,08
Metal - Copper 9,53 89,33
Plastic - Polyethylene 0,44 4,15
Tape - Polyester 0,05 0,43
Total 10,67
Technical data:
SAP nr. 20193412
El nr. 1003844
STANDARDS APPLIED:
HD 604-5D Construction
IEC 60502-1 Construction
IEC 60228 Class 1 or Class 2 Conductors
EN 50575:2014 + A1:2016 CPR standard - Fire properties
EN 60754-1 and EN 60754-2 Halogen free properties: EN 60754-1 (pH = 4,3, Conductivity = 10µS), EN
60754-2 ( < 0,5% Halogen)
IEC 61034-1, -2 Low smoke properties: IEC 61034-1, -2 (minimum 60% light transmittance)
Market:
Scandinavia
(Calculations for modules B6 and C2 is considering the Norwegian market.)
Reference service life, product
Expected lifetime 40 years, provided proper installation, load and ambient temperature.
Reference service life, building or construction works
40 years.
LCA: Calculation rules
Declared unit:
1 m IFSI-EMC Pure 4x240FV/120mm2
Cut-off criteria:
All major raw materials and all the essential energy is included. The production processes for raw materials and energy flows with very small amounts (less than 1%) are
not included. These cut-off criteria do not apply for hazardous materials and substances.
Allocation:
The allocation is made in accordance with the provisions of EN 15804. Incoming energy and water and waste production in-house is allocated equally among all products
through mass allocation. Effects of primary production of recycled materials is allocated to the main product in which the material was used. The recycling process and
transportation of the material is allocated to this analysis.
Data quality:
Specific data for the product composition are provided by the manufacturer. The data represent the production of the declared product and were collected for EPD
development in the year of study. Background data is based on EPDs according to EN 15804 and different LCA databases. The data quality of the raw materials in A1 is
presented in the table below.
Materials Source Data quality Year
HFFR Polyolefin ecoinvent 3.6 Database 2019
Metal - Copper ecoinvent 3.6 Database 2019
Plastic - Polyethylene ecoinvent 3.6 Database 2019
Tape - Polyester ecoinvent 3.6 Database 2019
3 / 12
System boundaries (X=included, MND=module not declared, MNR=module not relevant)
Construction Beyond the
Product stage installation Use stage End of life stage system
stage boundaries
A1 A2 A3 A4 A5 B1 B2 B3 B4 B5 B6 B7 C1 C2 C3 C4 D
X X X X X X X X X X X X X X X X X
System boundary:
The flowchart below illustrates the system boundaries of the analysis:
Additional technical information:
The article 1017089 IFSI-EMC Pure 1kV 4x240FV/120mm2 represents the product with the highest expenditure of raw materials and energy consumption during
manufacturing of all the following products from the same product family:
1003806 20216062 IFSI-EMC Pure 1kV 3x1.5/1,5mm² ER
1003807 20216067 IFSI-EMC Pure 1kV 3x2.5/2,5mm² ER
1003808 20216058 IFSI-EMC Pure 1kV 3x4/4mm² ER
1003809 20216069 IFSI-EMC Pure 1kV 3x6/6mm² ER
1003811 20216064 IFSI-EMC Pure 1kV 3x10/10mm² FR
1003812 20216065 IFSI-EMC Pure 1kV 3x10/10mm² FR
1003815 20216066 IFSI-EMC Pure 1kV 3x16/16mm² FR
1003816 20193394 IFSI-EMC Pure 1kV 3x25/16mm² FR
1003817 20193395 IFSI-EMC Pure 1kV 3x35/16mm² FR
1003818 20193396 IFSI-EMC Pure 1kV 3x50/25mm² FV
1003819 20193397 IFSI-EMC Pure 1kV 3x70/35mm² FV
1003820 20193398 IFSI-EMC Pure 1kV 3x95/50mm² FV
1003821 20193399 IFSI-EMC Pure 1kV 3x120/70mm² FV
1003822 20193400 IFSI-EMC Pure 1kV 3x150/70mm² FV
1003823 20193401 IFSI-EMC Pure 1kV 3x185/95mm² FV
1003824 20193402 IFSI-EMC Pure 1kV 3x240/120mm² FV
1003825 20216070 IFSI-EMC Pure 1kV 4x1.5/1,5mm² ER
1003826 20216074 IFSI-EMC Pure 1kV 4x2.5/2,5mm² ER
1003827 20216059 IFSI-EMC Pure 1kV 4x4/4mm² ER
1003829 20216075 IFSI-EMC Pure 1kV 4x6/6mm² ER
1003831 20216071 IFSI-EMC Pure 1kV 4x10/10mm² FR
1003832 20216072 IFSI-EMC Pure 1kV 4x10/10mm² FR
1003834 20216073 IFSI-EMC Pure 1kV 4x16/16mm² FR
1003836 20193404 IFSI-EMC Pure 1kV 4x25/16mm² FR
1003837 20193405 IFSI-EMC Pure 1kV 4x35/16mm² FR
1003838 20193406 IFSI-EMC Pure 1kV 4x50/25mm² FV
1003839 20193407 IFSI-EMC Pure 1kV 4x70/35mm² FV
1003840 20193408 IFSI-EMC Pure 1kV 4x95/50mm² FV
1003841 20193409 IFSI-EMC Pure 1kV 4x120/70mm² FV
1003842 20193410 IFSI-EMC Pure 1kV 4x150/70mm² FV
1003843 20193411 IFSI-EMC Pure 1kV 4x185/95mm² FV
waR slairetam tropsnarT gnirutcafunaM tropsnarT ylbmessA e​sU ecnanetniaM riapeR tnemecalpeR tnemhsibrufeR lanoitarepO esu ygrene lanoitarepO esu retaw -eD noitcurtsnoc noitilomed tropsnarT etsaW gnissecorp lasopsiD -yrevoceR-esueR
laitnetop-gnilcyceR
4 / 12
LCA: Scenarios and additional technical information
The following information describe the scenarios in the different modules of the EPD.
Module A4 = An average distance between the factory and the market is considered.
Modules A5 = 2% product losses during installation are estimated by the company. No energy use for installation has been quantified since this operation is assumed to
be done with other products and should be assessed at a construction works level. Cable drums are reused and assumed under the cut-off criterion of 1%.
Modules B1, B2, B3, B4, B5, and B7 = Company data shows that no significant activities have been reported for use, maintenance, repair, replacement, refurbishment, and
water use. This reflects an absence of impacts during the 40 years reference service life of the cable in these modules.
Module B6 = The operational energy use of the cable is calculated based on the methodology described in PEP Ecopassport, Product Specific Rules (PSR) for wires, cables
and accessories, reference PSR-0001-ed3-EN-2015 10 16. The following parameters are used to calculate the electricity loss of the cable:
- Estimate service life = 40 years
- Number of conductors = 4 units
- Use rate = 100 percent (according to appendix 1 of the PSR)
- Linear conductor resistivity = 0,0000754 Ohm per meter
- Current intensity = 1 Ampere
Module C1 = For both buildings and construction works, cables will be taken out as part of a larger demolition. The energy use for cable removal compared to other
heavier materials is assumed to be low. This module can therefore be included with zero impact.
Module C2 = An average distance between the market and the waste treatment facility is considered.
Modules C3 and C4 = Waste treatment of the product follows the default values provided in EN 50693, Product Category Rules for life cycle assessments of electronic and
electrical products and systems, table G.4. This table specified how different types of raw materials used in A1 will likely be treated during the end-of-life of the product.
Waste treatments in C3 include material recycling and incineration with and without energy recovery and fly ash extraction. Disposal in C4 consist of landfilling of
different waste fractions and of ashes.
Module D = The recyclability of metals and plastics allows the producers a credit for the net scrap that is produced at the end of a product’s life. The benefits from
recycling of net scrap are described in formula from EN 15804:2012+A2:2019. Substitution of heat and electricity generated by the incineration with energy recovery of
plastic insulation and other parts is also calculated in module D.
Capacity utilisation Value
Transport from production place to user (A4) Distance (km) Fuel/Energy Consumption Unit
(incl. return) % (Liter/tonne)
Truck, over 32 tonnes, EURO 5 (km) 53,3 % 810 0,023 l/tkm 18,63
Assembly (A5) Unit Value
Material loss during installation A1-A4
Units/DU 0,02
(percentage of cable)
Operational energy (B6) Unit Value
Electricity, Norway (kWh) kWh/DU 0,11
Capacity utilisation Value
Transport to waste processing (C2) Distance (km) Fuel/Energy Consumption Unit
(incl. return) % (Liter/tonne)
Truck, 16-32 tonnes, EURO 5 (km) 36,7 % 300 0,044 l/tkm 13,20
Waste processing (C3) Unit Value
Copper to recycling (kg) kg 5,72
Waste treatment of plastic mixture, incineration
kg 0,35
with energy recovery and fly ash extraction (kg)
Waste treatment of polyethylene (PE),
incineration with energy recovery and fly ash kg 0,22
extraction (kg)
Disposal (C4) Unit Value
Landfilling of ashes from incineration of Plastic
kg 0,01
mixture, process per kg ashes and residues (kg)
Landfilling of ashes from incineration of
Polyethylene (PE), process per kg ashes and kg 0,01
residues (kg)
Landfilling of copper (kg) kg 3,81
Landfilling of plastic mixture (kg) kg 0,57
Benefits and loads beyond the system
Unit Value
boundaries (D)
Substitution of primary copper with net scrap (kg) kg 0,78
Substitution of electricity, in Norway (MJ) MJ 0,96
Substitution of thermal energy, district heating, in
MJ 14,58
Norway (MJ)
5 / 12
LCA: Results
The LCA results are presented below for the declared unit defined on page 2 of the EPD document.
Environmental impact
Parameter Unit A1 A2 A3 A4 A5 B1 B2 B3
GWP-total kg CO2 -eq 7,72E+01 3,69E-01 1,15E+00 7,86E-01 1,59E+00 0 0 0
GWP-fossil kg CO2 -eq 7,56E+01 3,69E-01 9,99E-01 7,85E-01 1,56E+00 0 0 0
GWP-biogenic kg CO2 -eq 1,50E+00 1,51E-04 1,28E-01 3,22E-04 3,26E-02 0 0 0
GWP-luluc kg CO2 -eq 8,24E-02 1,16E-04 2,58E-02 2,29E-04 2,17E-03 0 0 0
ODP kg CFC11 -eq 4,80E-06 8,49E-08 2,06E-07 1,81E-07 1,05E-07 0 0 0
AP mol H+ -eq 6,83E+00 1,54E-03 3,06E-03 3,30E-03 1,37E-01 0 0 0
EP-FreshWater kg P -eq 5,45E-02 2,85E-06 2,92E-05 5,99E-06 1,09E-03 0 0 0
EP-Marine kg N -eq 3,26E-01 4,59E-04 8,14E-04 9,93E-04 6,57E-03 0 0 0
EP-Terrestial mol N eq 4,87E+00 5,08E-03 7,67E-03 1,10E-02 9,78E-02 0 0 0
POCP kg NMVOC -eq 1,30E+00 1,60E-03 1,85E-03 3,53E-03 2,62E-02 0 0 0
ADP-minerals&metals1 Kg Sb-eq 3,89E-02 7,70E-06 1,68E-05 1,34E-05 7,79E-04 0 0 0
ADP-fossil1 MJ 8,71E+02 5,68E+00 4,72E+01 1,22E+01 1,87E+01 0 0 0
WDP1 m3 5,23E+02 4,75E+00 4,71E+03 9,37E+00 1,05E+02 0 0 0
Parameter Unit B4 B5 B6 B7 C1 C2 C3 C4 D
GWP-total kg CO2 -eq 0 0 2,57E-03 0 0 5,34E-01 1,49E+00 1,20E-01 -1,97E+00
GWP-fossil kg CO2 -eq 0 0 2,49E-03 0 0 5,34E-01 1,49E+00 1,20E-01 -1,96E+00
GWP-biogenic kg CO2 -eq 0 0 6,89E-05 0 0 2,18E-04 2,33E-05 6,04E-06 -8,89E-03
GWP-luluc kg CO2 -eq 0 0 1,03E-05 0 0 1,86E-04 4,13E-06 2,26E-05 -4,89E-03
ODP kg CFC11 -eq 0 0 1,71E-10 0 0 1,22E-07 2,30E-09 1,71E-08 -6,16E-03
AP mol H+ -eq 0 0 1,95E-05 0 0 2,18E-03 2,64E-04 4,71E-04 -3,15E-01
EP-FreshWater kg P -eq 0 0 1,79E-07 0 0 4,19E-06 2,10E-07 1,06E-06 -2,13E-03
EP-Marine kg N -eq 0 0 2,14E-06 0 0 6,47E-04 1,26E-04 2,36E-04 -1,32E-02
EP-Terrestial mol N eq 0 0 2,79E-05 0 0 7,15E-03 1,32E-03 1,90E-03 -2,03E-01
POCP kg NMVOC -eq 0 0 7,49E-06 0 0 2,19E-03 3,17E-04 5,50E-04 -5,51E-02
ADP-minerals&metals1 Kg Sb-eq 0 0 1,86E-07 0 0 1,45E-05 1,13E-07 4,62E-07 -1,76E-03
ADP-fossil1 MJ 0 0 3,40E-02 0 0 8,04E+00 1,57E-01 1,40E+00 -1,79E+01
WDP1 m3 0 0 5,93E+00 0 0 7,67E+00 9,15E-01 3,39E+01 8,75E+01
GWP total Global Warming Potential total; GWP fossil Global Warming Potential fossil fuels ; GWP biogenic Global Warming Potential biogenic; GWP luluc Global W
Potential land use change; ODP Ozone Depletion; AP Acidification; EP freshwater Eutrophication aquatic freshwater; EP marine Eutrophication aquatic marine; EP
terrestrial Eutrophication terrestrial ;POCP Photochemical zone formation; ADPE Abiotic Depletion Potential minerals and metals; ADPf Abiotic Depletion Potential fossil
fuels;
"Reading example: 9,0 E-03 = 9,0*10-3 = 0,009"
*INA Indicator Not Assessed
1. The results of this environmental impact indicator shall be used with care as the uncertainties on these results are high or as there is limited experienced with the
indicator
Remarks to environmental impacts
6 / 12
Additional environmental impact indicators
Parameter Unit A1 A2 A3 A4 A5 B1 B2 B3
PM Disease incidence 1,52E-05 3,03E-08 2,39E-08 6,91E-08 3,06E-07 0 0 0
IRP2 kgBq U235 eq. 2,70E+00 2,48E-02 1,59E+00 5,34E-02 8,74E-02 0 0 0
ETP-fw1 CTUe 6,69E+04 4,16E+00 2,82E+01 8,93E+00 1,34E+03 0 0 0
HTP-c1 CTUh 9,31E-07 0,00E+00 9,23E-10 0,00E+00 1,86E-08 0 0 0
HTP-nc1 CTUh 7,77E-05 4,20E-09 2,31E-08 8,64E-09 1,55E-06 0 0 0
SQP1 Pt 9,28E+02 5,55E+00 2,13E+01 1,40E+01 1,94E+01 0 0 0
Parameter Unit B4 B5 B6 B7 C1 C2 C3 C4 D
PM Disease incidence 0 0 1,40E-10 0 0 3,84E-08 1,12E-09 8,26E-09 -6,71E-07
IRP2 kgBq U235 eq. 0 0 6,17E-04 0 0 3,52E-02 3,58E-04 9,12E-03 -2,85E-02
ETP-fw1 CTUe 0 0 1,55E-01 0 0 5,93E+00 1,87E+00 2,36E+03 -2,90E+03
HTP-c1 CTUh 0 0 7,00E-12 0 0 0,00E+00 6,10E-11 1,10E-10 -4,10E-08
HTP-nc1 CTUh 0 0 1,74E-10 0 0 6,40E-09 2,73E-09 2,01E-09 -3,51E-06
SQP1 Pt 0 0 1,71E-02 0 0 5,55E+00 2,59E-02 2,69E+00 -4,48E+01
PM Particulate Matter emissions; IRP Ionizing radiation – human health; ETP-fw Eco toxicity – freshwater; HTP-c Human toxicity – cancer effects; HTP-nc Human
toxicity – non cancer effects; SQP Soil Quality (dimensionless)
"Reading example: 9,0 E-03 = 9,0*10-3 = 0,009"
*INA Indicator Not Assessed
1. The results of this environmental impact indicator shall be used with care as the uncertainties on these results are high or as there is limited experienced with the
indicator
2. This impact category deals mainly with the eventual impact of low dose ionizing radiation on human health of the nuclear fuel cycle. It does not consider effects due
to possible nuclear accidents, occupational exposure nor due to radioactive waste disposal in underground facilities. Potential ionizing radiation from the soil, from
radon and from some construction materials is also not measured by this indicator.
7 / 12
Resource use
Parameter Unit A1 A2 A3 A4 A5 B1 B2 B3
PERE MJ 2,10E+02 7,47E-02 2,23E+01 1,54E-01 4,66E+00 0 0 0
PERM MJ 0,00E+00 0,00E+00 0,00E+00 0,00E+00 0,00E+00 0 0 0
PERT MJ 2,10E+02 7,47E-02 2,23E+01 1,54E-01 4,66E+00 0 0 0
PENRE MJ 8,43E+02 5,68E+00 4,73E+01 1,22E+01 1,82E+01 0 0 0
PENRM MJ 2,99E+01 0,00E+00 0,00E+00 0,00E+00 5,97E-01 0 0 0
PENRT MJ 8,73E+02 5,68E+00 4,73E+01 1,22E+01 1,88E+01 0 0 0
SM kg 5,15E+00 0,00E+00 1,20E-02 0,00E+00 1,03E-01 0 0 0
RSF MJ 1,55E+00 2,64E-03 8,77E-02 5,38E-03 3,29E-02 0 0 0
NRSF MJ 1,61E+00 9,07E-03 2,81E-01 1,80E-02 3,84E-02 0 0 0
FW m3 1,52E+00 6,28E-04 5,63E-02 1,39E-03 3,15E-02 0 0 0
Parameter Unit B4 B5 B6 B7 C1 C2 C3 C4 D
PERE MJ 0 0 4,41E-01 0 0 1,14E-01 7,58E-03 1,83E-01 -1,42E+01
PERM MJ 0 0 0,00E+00 0 0 0,00E+00 0,00E+00 0,00E+00 0,00E+00
PERT MJ 0 0 4,41E-01 0 0 1,14E-01 7,58E-03 1,83E-01 -1,42E+01
PENRE MJ 0 0 3,41E-02 0 0 8,05E+00 1,57E-01 1,40E+00 -1,79E+01
PENRM MJ 0 0 0,00E+00 0 0 0,00E+00 -2,90E+01 0,00E+00 0,00E+00
PENRT MJ 0 0 3,41E-02 0 0 8,05E+00 -2,89E+01 1,40E+00 -2,32E+01
SM kg 0 0 0,00E+00 0 0 0,00E+00 0,00E+00 1,92E-02 5,48E-01
RSF MJ 0 0 3,46E-04 0 0 4,06E-03 1,71E-04 3,79E-03 5,08E-02
NRSF MJ 0 0 8,62E-04 0 0 1,45E-02 -1,02E-03 -6,65E-04 -3,30E-01
FW m3 0 0 3,29E-03 0 0 8,47E-04 1,08E-03 1,82E-03 -5,48E-02
PERE Use of renewable primary energy excluding renewable primary energy resources used as raw materials; PERM Use of renewable primary energy resources used as
raw materials; PERT Total use of renewable primary energy resources; PENRE Use of non renewable primary energy excluding non-renewable primary energy resources
used as raw materials; PENRM Use of non renewable primary energy resources used as raw materials; PENRT Total use of non renewable primary energy resources; SM
Use of secondary materials; RSF Use of renewable secondary fuels; NRSF Use of non renewable secondary fuels; FW Use of net fresh water
"Reading example: 9,0 E-03 = 9,0*10-3 = 0,009"
*INA Indicator Not Assessed
8 / 12
End of life - Waste
Parameter Unit A1 A2 A3 A4 A5 B1 B2 B3
HWD kg 6,50E-01 3,03E-04 2,60E-01 6,69E-04 1,82E-02 0 0 0
NHWD kg 2,43E+01 4,11E-01 3,88E-01 1,06E+00 5,24E-01 0 0 0
RWD kg 2,51E-03 3,87E-05 7,03E-04 8,34E-05 6,66E-05 0 0 0
Parameter Unit B4 B5 B6 B7 C1 C2 C3 C4 D
HWD kg 0 0 2,18E-05 0 0 4,10E-04 6,64E-05 1,50E-01 -2,13E-02
NHWD kg 0 0 2,62E-03 0 0 3,85E-01 3,06E-03 4,44E+00 -9,32E-01
RWD kg 0 0 3,05E-07 0 0 5,49E-05 4,18E-07 9,71E-06 -2,51E-05
HWD = Hazardous waste disposed; NHWD = Non-hazardous waste disposed; RWD = Radioactive waste disposed;
"Reading example: 9,0 E-03 = 9,0*10-3 = 0,009"
*INA Indicator Not Assessed
End of life - Output flow
Parameter Unit A1 A2 A3 A4 A5 B1 B2 B3
CRU kg 0,00E+00 0,00E+00 0,00E+00 0,00E+00 0,00E+00 0 0 0
MFR kg 5,62E-04 0,00E+00 2,28E-02 0,00E+00 4,68E-04 0 0 0
MER kg 1,32E-03 0,00E+00 1,10E-05 0,00E+00 2,66E-05 0 0 0
EEE MJ 2,45E-03 0,00E+00 6,21E-01 0,00E+00 1,25E-02 0 0 0
EET MJ 3,70E-02 0,00E+00 9,39E+00 0,00E+00 1,89E-01 0 0 0
Parameter Unit B4 B5 B6 B7 C1 C2 C3 C4 D
CRU kg 0 0 0,00E+00 0 0 0,00E+00 0,00E+00 0,00E+00 0,00E+00
MFR kg 0 0 0,00E+00 0 0 0,00E+00 5,72E+00 8,75E-05 -2,15E-02
MER kg 0 0 0,00E+00 0 0 0,00E+00 1,80E-06 4,83E-04 -2,83E-03
EEE MJ 0 0 0,00E+00 0 0 0,00E+00 9,64E-01 4,36E-03 -6,92E-03
EET MJ 0 0 0,00E+00 0 0 0,00E+00 1,46E+01 6,59E-02 -1,05E-01
CRU = Components for re-use; MFR = Materials for recycling; MER = Materials for energy recovery; EEE = Exported electrical energy; EET = Exported energy ​ Thermal
"Reading example: 9,0 E-03 = 9,0*10-3 = 0,009"
*INA Indicator Not Assessed
Biogenic Carbon Content
Parameter Unit At the factory gate
Biogenic carbon content in product kg C 0,00E+00
Biogenic carbon content in accompanying packaging kg C 0,00E+00
Note: 1 kg biogenic carbon is equivalent to 44/12 kg CO2
9 / 12
Additional Norwegian requirements
Greenhouse gas emissions from the use of electricity in the manufacturing phase
National production mix from import, low voltage (production of transmission lines, in addition to direct emissions and losses in grid) of applied electricity for the
manufacturing process (A3).
Electricity mix Data source Amount Unit
Electricity, Sweden (kWh) ecoinvent 3.6 54,94 g CO2-eq/kWh
Dangerous substances
The product contains no substances given by the REACH Candidate list or the Norwegian priority list.
Indoor environment
Not relevant.
Additional Environmental Information
Environmental impact indicators EN 15804+A1 and NPCR Part A v2.0
Parameter Unit A1 A2 A3 A4 A5 B1 B2 B3
GWP kg CO2 -eq 7,43E+01 3,65E-01 1,10E+00 7,77E-01 1,53E+00 0 0 0
ODP kg CFC11 -eq 4,33E-06 6,81E-08 3,55E-07 1,47E-07 9,81E-08 0 0 0
POCP kg C2H4-eq 2,28E-01 4,81E-05 1,36E-04 1,01E-04 4,56E-03 0 0 0
AP kg SO2 -eq 5,79E+00 7,32E-04 2,28E-03 1,57E-03 1,16E-01 0 0 0
EP kg PO43- -eq 2,89E-01 7,93E-05 4,78E-04 1,71E-04 5,79E-03 0 0 0
ADPM kg Sb -eq 3,89E-02 7,70E-06 1,68E-05 1,34E-05 7,79E-04 0 0 0
ADPE MJ 7,88E+02 5,57E+00 3,99E+00 1,20E+01 1,62E+01 0 0 0
GWPIOBC kg CO2 -eq 7,71E+01 3,69E-01 4,30E-01 7,86E-01 1,57E+00 0 0 0
Parameter Unit B4 B5 B6 B7 C1 C2 C3 C4 D
GWP kg CO2 -eq 0 0 2,46E-03 0 0 5,28E-01 1,49E+00 1,16E-01 -1,90E+00
ODP kg CFC11 -eq 0 0 2,17E-10 0 0 9,60E-08 2,11E-09 1,46E-08 -8,67E-08
POCP kg C2H4-eq 0 0 7,32E-07 0 0 7,05E-05 3,46E-06 2,25E-05 -1,06E-02
AP kg SO2 -eq 0 0 1,54E-05 0 0 1,05E-03 1,84E-04 2,05E-04 -2,69E-01
EP kg PO43- -eq 0 0 1,44E-06 0 0 1,12E-04 6,06E-05 6,27E-05 -1,14E-02
ADPM kg Sb -eq 0 0 1,86E-07 0 0 1,45E-05 1,13E-07 4,66E-07 -1,76E-03
ADPE MJ 0 0 1,68E-02 0 0 7,88E+00 1,57E-01 1,21E+00 -1,81E+01
GWPIOBC kg CO2 -eq 0 0 2,57E-03 0 0 5,34E-01 1,49E+00 6,72E-02 -9,75E-01
GWP Global warming potential; ODP Depletion potential of the stratospheric ozone layer; POCP Formation potential of tropospheric photochemical oxidants; AP
Acidification potential of land and water; EP Eutrophication potential; ADPM Abiotic depletion potential for non fossil resources; ADPE Abiotic depletion​ potential for
fossil resources; GWP-IOBC/GHG Global warming potential calculated according to the principle of instantanious oxidation (except emissions and uptake of biogenic
carbon)
10 / 12
Bibliography
ISO 14025:2010. Environmental labels and declarations - Type III environmental declarations - Principles and procedures. International Organization for Standardization.
ISO 14044:2006. Environmental management - Life cycle assessment - Requirements and guidelines. International Organization for Standardization.
EN 15804:2012+A2:2019. Environmental product declaration - Core rules for the product category of construction products. European Committee for Standardization.
ISO 21930:2017. Sustainability in buildings and civil engineering works - Core rules for environmental product declarations of construction products. International
Organization for Standardization.
EN 50693:2019. Product category rules for life cycle assessments of electronic and electrical products and systems. European Committee for Standardization.
Ecoinvent v3, 2019. Allocation, cut-off by classification. Swiss Centre of Life Cycle Inventories.
Iversen et al., (2021). eEPD v2021.09, background information for EPD generator tool system verification, LCA.no. Report number: 07.21. System verification report.
Philis et al., (2022). EPD generator for NPCR 027 part B for electrical wires and cables, background information for EPD generator application and LCA data, LCA.no Report
number: 03.22. PCR verification report.
EPD Norway (2022). NPCR Part A: Construction products and services. The Norwegian EPD foundation. Version 2.0 published 24.03.2021.
EPD Norway (2022). NPCR 027 Part B for electrical cables and wires. The Norwegian EPD foundation. Version 2.0 published 01.03.2022.
The operational energy use in module B6 is calculated based on the methodology described in PEP Ecopassport, Product Specific Rules (PSR) for wires, cables and
accessories, reference PSR-0001-ed3-EN-2015 10 16.
Program operator and publisher Phone: +47 23 08 80 00
The Norwegian EPD Foundation e-mail: post@epd-norge.no
Post Box 5250 Majorstuen, 0303 Oslo, Norway web: www.epd-norge.no
Owner of the declaration: Phone: +47 90066733
Prysmian Group Norge AS e-mail: anders.nymark@prysmiangroup.com
Kjerraten 16, 3013 Drammen web: www.prysmiangroup.no
Author of the Life Cycle Assessment Phone: +47 916 50 916
LCA.no AS e-mail: post@lca.no
Dokka 6B, 1671 web: www.lca.no
Developer of EPD generator Phone: +47 916 50 916
LCA.no AS e-mail: post@lca.no
Dokka 6B,1671 Kråkerøy web: www.lca.no
ECO Platform Web: www.eco-platform.org
ECO Portal Web: ECO Portal
11 / 12
EPD for the best
environmental
decision
The Norwegian EPD Foundation
www.epd-norge.no
12 / 12
