Environmental product declaration
In accordance with ISO 14025 and EN 15804 +A2
NorDan NTech Villa Topswing reversible - BG 105/80 (With Aluminium Cladding)
Owner of the declaration: Program operator:
NorDan AS The Norwegian EPD Foundation
Declared unit: Declaration number:
1 pcs NorDan NTech Villa Topswing reversible - BG 105/80
(With Aluminium Cladding) NEPD-4000-3040-EN
This declaration is based on Product Category Rules: Registration number:
CEN Standard EN 15804:2012+A2:2019 serves as core PCR
NCPR 014:2019 Part B for Windows and doors NEPD-4000-3040-EN
Issue date: 05.12.2022
Valid to: 05.12.2027
The Norwegian EPD Foundation
EPD Software:
LCA.no EPD generator
System ID:
50906
1 / 14
General information
Product Owner of the declaration:
NorDan NTech Villa Topswing reversible - BG 105/80 (With Aluminium Cladding) NorDan AS
Contact person: Fredrik Jonsson
Phone: +46 (0) 10-130 01 78
e-mail: fredrik.jonsson@nordan.se
Program operator: Manufacturer:
Post Box 5250 Majorstuen, 0303 Oslo, Norway NorDan AS
The Norwegian EPD Foundation Stasjonsveien 46 , 4460 Moi
Phone: +47 23 08 80 00 Norway
web: post@epd-norge.no
Declaration number: Place of production:
NEPD-4000-3040-EN Otta Nordan AS
Skansen 30 , 2670 Otta
Norway
Management system:
This declaration is based on Product Category Rules: NS-ISO 9001:2015, NS-EN ISO 14001:2015
CEN Standard EN 15804:2012+A2:2019 serves as core PCR
NCPR 014:2019 Part B for Windows and doors
Organisation no:
Statement of liability: 979 776 233
The owner of the declaration shall be liable for the underlying information and
evidence. EPD Norway shall not be liable with respect to manufacturer
information, life cycle assessment data and evidences.
Issue date: 05.12.2022
Declared unit:
1 pcs NorDan NTech Villa Topswing reversible - BG 105/80 (With Aluminium
​
Valid to: 05.12.2027
Declared unit with option:
A1-A3,A4,A5,B1,B2,B3,B4,B5,C1,C2,C3,C4,D
Cladding) Year of study:
Functional unit: 2020
1 window with aluminium cladding measuring 1.23 m x 1.48 m (reference window
based on EN 14351-1) with an expected service life of 60 yrs.
Comparability:
General information on verification of EPD from EPD tools: EPD of construction products may not be comparable if they not comply with
Independent verification of data, other environmental information and the EN 15804 and seen in a building context.
declaration according to ISO 14025:2010, § 8.1.3 and § 8.1.4. Individualthird party
verification of each EPD is not required when the EPD tool is i) integrated into the
company's environmental management system, ii) the procedures for use of the
EPD tool are approved by EPDNorway, and iii)the proccess is reviewed annualy.
See Appendix G of EPD-Norway's General Programme Instructions for further
information on EPD tools.
Development and verification of EPD:
Verification of EPD tool: The declaration is created using EPD tool lca.tools ver EPD2022.03, developed by
Independent third party verification of the EPD tool, background data and test- LCA.no. The EPD tool is integrated in the company's management system, and
EPD in accordance with EPDNorway's procedures and guidelines for verification has been approved by EPD Norway.
and approval of EPD tools.
Developer of EPD:
Third party verifier:
Linda Jonsson
Reviewer of company-specific input data and EPD:​
Gaylord K. Booto, NILU
Fredrik Jonsson
(no signature required)
Approved:
Håkon Hauan, CEO EPD-Norge
2 / 14
Product
Product description:
Window with outward opening fully reversible opening sash for use in exterior walls of domestic and commercial buildings.
Product specification
25% of aluminium and 18% of glass is produced from recycled material.
Product NorDan Ntech Villa Topswing reversible - BG in size 1230x1480 mm is covered in this EPD.
Materials kg %
Absorbent - IGU 0,02 0,03
Adhesive and sealant 0,05 0,07
Aluminium 3,54 5,13
Argon gas - IGU 0,07 0,10
Coating materials 0,88 1,28
Gasket 0,34 0,49
Glass 40,86 59,29
Insulation 0,10 0,14
Metal 4,03 5,85
Plastic 1,12 1,62
Sealant - IGU 1,10 1,59
Wood 16,81 24,39
Total 68,91
Packaging kg %
Packaging - Plastic 0,13 3,47
Packaging - Steel 0,05 1,33
Packaging - Wood 3,59 95,20
Total incl. packaging 72,69
Technical data:
Outward opening window. Triple glazed, 105mm frame with 8mm aluminium clad, 80mm sash. Uwin 0,83W/m2K. Certified: BBA - Bristish Board of Agrément, Secured by
Design, NDVK.
The total weight of the product is 68,91 kg. The packaging has a average weight of 3,77 kg.
Conversion factor is 72,69 [Kg/DU].
Market:
Europe, but scenarios beyond cradle-to-gate are based on the situation in the Norwegian market.
Reference service life, product
The reference service life is 60 years for aluminium cladding timber frame.
Reference service life, building or construction works
60 years.
LCA: Calculation rules
Declared unit:
1 pcs NorDan NTech Villa Topswing reversible - BG 105/80 (With Aluminium Cladding)
Cut-off criteria:
All major raw materials and all the essential energy is included. The production processes for raw materials and energy flows with very small amounts (less than 1%) are
not included. These cut-off criteria do not​ apply for hazardous materials and substances.
Allocation:
The allocation is made in accordance with the provisions of EN 15804. Effects of primary production of recycled materials is allocated to the main product in which the
material was used. The recycling process and transportation of the material is allocated to this analysis. The PCR specific background data follow the allocation rules in
the Ecoinvent v3.7.1 Cut-off database version. The allocation of water, energy and waste flows within the production facilities for windows and doors follows unit-based
allocation adjusted with a point system to different product groups or products. This score system is regulated by a factor which increases with the resource intensity of
each product. The unit-based allocation is adjusted by the weight of the product, excluding the weight of glass.
Data quality:
Specific data for the product composition are provided by the manufacturer. The data represent the production of the declared product and were collected for EPD
development in the year of study. Background data is based on EPDs according to EN 15804 and different LCA databases. The data quality of the raw materials in A1 is
presented in the table below.
The production data was collected in 2021 and is an average for 2020.
3 / 14
Materials Source Data quality Year
Packaging - Plastic ecoinvent 3.6 Database 2019
Packaging - Steel ecoinvent 3.6 Database 2019
Packaging - Wood ecoinvent 3.6 Database 2019
Argon gas - IGU ecoinvent 3.7.1 Database 2020
Glass ecoinvent 3.7.1 Database 2020
Insulation ecoinvent 3.7.1 Database 2020
Absorbent - IGU ecoinvent 3.7.1 Specific 2020
Adhesive and sealant ecoinvent 3.7.1 Specific 2020
Aluminium ecoinvent 3.7.1 Specific 2020
Coating materials ecoinvent 3.7.1 Specific 2020
Gasket ecoinvent 3.7.1 Specific 2020
Metal ecoinvent 3.7.1 Specific 2020
Plastic ecoinvent 3.7.1 Specific 2020
Sealant - IGU ecoinvent 3.7.1 Specific 2020
Wood ecoinvent 3.7.1 Specific 2020
4 / 14
System boundaries (X=included, MND=module not declared, MNR=module not relevant)
Construction Beyond the
Product stage installation Use stage End of life stage system
stage boundaries
A1 A2 A3 A4 A5 B1 B2 B3 B4 B5 B6 B7 C1 C2 C3 C4 D
X X X X X X X X X X MNR MNR X X X X X
System boundary:
Additional technical information:
For the products with different sizes from the declared unit, the environmental impacts must be converted by using a conversion factor. The Norwegian EPD Foundation
has published instructions on how to interpret EPDs for windows on its website (www.epdnorge.no) where different calculation methods have been stated. (Document:
Bruksanvisninger i hvordan tolke EPD'er - Vinduer).
waR slairetam tropsnarT gnirutcafunaM tropsnarT ylbmessA e​sU ecnanetniaM riapeR tnemecalpeR tnemhsibrufeR lanoitarepO esu ygrene lanoitarepO esu retaw -eD noitcurtsnoc noitilomed tropsnarT etsaW gnissecorp lasopsiD -yrevoceR-esueR
laitnetop-gnilcyceR
5 / 14
LCA: Scenarios and additional technical information
The following information describe the scenarios in the different modules of the EPD.
A4
The transportation from production to construction site is based on a scenario where the product is transported on a large lorry from Otta to warehouse in Oslo, Norway
(291 km) . Transport from warehouse to a construction site is assumed to be 50 km on a medium truck.
A5
According to the report from EPD-Norge Harmonising the documentation of scenarios beyond cradle to gate, EN 15804 there is no loss on site during construction
activities. The window products in this EPD are painted and surface treated in the production and not at the building site. Therefore, there is only 2 items left in this
module. 1) Waste treatment of packaging which is considered in the EPD calculations. 1) Energy use during installation. This can be varied depending on the floor, type of
building and several other unknown parameters, and therefore ignored in the calculation.
B2/B3
The maintenance scenario included cleaning, painting and change of IGU. Cleaning is performed three times per year. It is calculated with 1,5 dl of detergent and 3 litres
of water each year. Windows with aluminium cladding are assumed to be painted 3 times during its lifetime from inside. It is assumed that 5 gr of lubricating oil is used
every year for fittings and moving parts. The glazing unit is changed once during the lifetime for the windows with aluminium cladding. No repair is assumed during the
product lifetime.
B4/B5
* Number or RSL (Reference Service Life). The window has RSL of 60 years. Therefore, it is assumed to replace the insulated glass unit after 30 years (See Module B2). The
RSL is determined by using SINTEF design guide 700.320. There is no need for refurbishment during the product lifetime.
C1
As there are no data for de-construction, it is assumed no activites in C1 in this study. The windows are assumed to be treated as mixed waste and sent to incineration.
The combustible materials are then energy recovered, while glass is assumed to end up in the bottom ash and then landfilled. The metals are usually sorted out of the
bottom ash and then recycled, but there is no data of the share which are recycled and therefore standard values from Ecoinvent is utilized.
C2
The transport of window as waste is calculated based on a scenario with 50 km distance.
C3
Windows are assumed to be sorted as mixed construction waste and treated with incineration with energy recovery. However, the manufacturer has documented the
recycling potentials for its product in the Construction Product Declaration eBVD NorDan BG Vridf?nster Tr?/Alu 105, ID: C-SE556294452901-67
URL:https://www.ebvd.org/BMI/Document/Export/2952/0/Pdf In the documentation, Chapter 10, the specific material recovery, and energy recovery potential is reported
for the product.
D
The benefits beyond life cycle has been modelled based on the output flows from module C3. This includes energy from incineration and scrap metal recovered from the
ashes. The amount recovered metal is assumed to avoid production of primary metals in accordance to 6.4.3.3 in EN 15804. The exported energy is substituting
Norwegian district heating mix and electricity mix. Inventory processes causing substitution of avoided virgin raw materials has be constructed for each material.
Capacity utilisation Value
Transport from production place to user (A4) Distance (km) Fuel/Energy Consumption Unit
(incl. return) % (Liter/tonne)
Truck, over 32 tonnes, EURO 5 (kgkm) - RER 53,3 % 291 0,023 l/tkm 6,69
Truck, 16-32 tonnes, EURO 5 (kgkm) - RER 36,7 % 50 0,044 l/tkm 2,20
Assembly (A5) Unit Value
Waste, metal, average treatment (kg) kg 0,05
Waste, packaging, pallet, EUR wooden pallet,
kg 3,59
reusable, average treatment (kg) A5
Waste, packaging, plastic film (LDPE), to average
kg 0,13
treatment (kg)
Maintenance (B2) Unit Value
Waste treatment per kg Paint, hazardous waste
kg 0,55
incineration (kg)
Waste, glass, incineration (kg) kg 40,86
Waste, plastic, mixture, for incineration (kg) kg 0,34
110 Plastic parts, gasket, Ethylene propylene diene
kg/DU 0,34
monomer (EPDM), Europe (kg)
179 Uncoated flat glass, Europe (kg) kg/DU 13,62
180 Coated flat glass, Europe (kg) kg/DU 27,24
193 Spacer for IGU, Europe (kg) kg/DU 0,74
194 Argon gas for IGU, liquid, global (kg) kg/DU 0,06
208 Sealant for IGU, generic, global (kg) kg/DU 1,10
209 Absorbent for IGU, generic, global (kg) kg/DU 0,02
Detergent, Husvask (kg) kg/DU 9,00
Lubricating oil (kg) - RER kg/DU 0,30
Paint, 50% water, wet mass (kg) kg/DU 0,55
Water, tap water (kg) - Europe without Switzerland kg/DU 180,00
Truck, over 32 tonnes, EURO 5 (kgkm) - RER kgkm/DU 2955,50
Capacity utilisation Value
Transport to waste processing (C2) Distance (km) Fuel/Energy Consumption Unit
(incl. return) % (Liter/tonne)
Truck, unspecified (kgkm) - RER 48,7 % 50 0,051 l/tkm 2,55
6 / 14
Waste processing (C3) Unit Value
Materials to recycling (kg) kg 0,37
Waste treatment per kg Glass, incineration with fly
kg 42,55
ash extraction (kg) - CH - C3
Waste treatment per kg Hazardous waste,
incineration (kg) kg 0,01
Waste treatment per kg Paint, hazardous waste
kg 0,79
incineration (kg)
Waste treatment per kg Paint, hazardous waste
kg 0,01
incineration (kg) - C3
Waste treatment per kg Plastic, Mixture,
kg 0,75
municipal incineration with fly ash extraction (kg)
Waste treatment per kg Polyurethane (PU),
kg 0,55
incineration (kg)
Waste treatment per kg Scrap aluminium,
kg 3,54
incineration with fly ash extraction (kg) - CH - C3
Waste treatment per kg Scrap steel, incineration
kg 4,03
with fly ash extraction (kg) - CH - C3
Waste treatment per kg Wood, from incineration
kg 18,10
(kg)
Disposal (C4) Unit Value
Landfilling of ashes from incineration of Glass,
kg 49,15
process of ashes and residues (kg) - CH - C4
Landfilling of ashes from incineration of Plastics,
Mixture, municipal incineration with fly ash kg 0,03
extraction, process per kg ashes and residues (kg)
Landfilling of ashes from incineration of
Polyurethane (PU), process per kg ashes and kg 0,02
residues - C4 (kg)
Landfilling of ashes from incineration of Scrap
aluminium, process of ashes and residues (kg) - kg 3,17
CH - C4
Landfilling of ashes from incineration of Scrap
kg 2,66
steel, process of ashes and residues (kg) - CH - C4
Landfilling of ashes from incineration of Wood,
kg 0,21
process per kg ashes and residues - C4 (kg)
Landfilling of ashes from incineration per kg
kg 0,02
Paint, hazardous waste incineration (kg)
Benefits and loads beyond the system
Unit Value
boundaries (D)
Substitution of primary aluminium with net scrap
kg 0,28
(kg)
Substitution of primary steel with net scrap (kg) kg 0,06
Substitution of electricity, in Norway (MJ) MJ 16,38
Substitution of thermal energy, district heating, in
MJ 247,77
Norway (MJ)
7 / 14
LCA: Results
The LCA results are presented below for the declared unit defined on page 2 of the EPD document.
Environmental impact
Parameter Unit A1-A3 A4 A5 B1 B2 B3
GWP-total kg CO2 -eq 1,06E+02 2,53E+00 5,55E+00 0 6,27E+01 0
GWP-fossil kg CO2 -eq 1,37E+02 2,53E+00 1,08E-01 0 6,18E+01 0
GWP-biogenic kg CO2 -eq -3,15E+01 1,04E-03 5,44E+00 0 4,82E-01 0
GWP-luluc kg CO2 -eq 5,05E-01 7,73E-04 2,58E-05 0 4,76E-01 0
ODP kg CFC11 -eq 1,36E-05 5,82E-07 1,62E-08 0 6,93E-06 0
AP mol H+ -eq 1,04E+00 1,06E-02 7,92E-04 0 5,44E-01 0
EP-FreshWater kg P -eq 5,36E-03 1,94E-05 1,18E-06 0 1,75E-03 0
EP-Marine kg N -eq 1,79E-01 3,16E-03 3,46E-04 0 9,02E-02 0
EP-Terrestial mol N eq 2,03E+00 3,50E-02 3,63E-03 0 1,06E+00 0
POCP kg NMVOC -eq 5,89E-01 1,11E-02 9,36E-04 0 2,91E-01 0
ADP-minerals&metals1 Kg Sb-eq 1,54E-03 4,92E-05 1,64E-06 0 8,25E-04 0
ADP-fossil1 MJ 1,78E+03 3,90E+01 1,19E+00 0 8,69E+02 0
WDP1 m3 3,44E+03 3,17E+01 1,91E+00 0 9,97E+01 0
Parameter Unit B4 B5 C1 C2 C3 C4 D
GWP-total kg CO2 -eq 0 0 0 4,79E-01 3,26E+01 6,34E-01 -4,12E+00
GWP-fossil kg CO2 -eq 0 0 0 4,78E-01 6,33E+00 6,33E-01 -4,01E+00
GWP-biogenic kg CO2 -eq 0 0 0 2,05E-04 2,63E+01 4,23E-04 -1,40E-02
GWP-luluc kg CO2 -eq 0 0 0 1,69E-04 3,66E-04 1,57E-04 -9,67E-02
ODP kg CFC11 -eq 0 0 0 1,09E-07 2,09E-07 1,80E-07 -1,05E-01
AP mol H+ -eq 0 0 0 2,73E-03 7,95E-03 4,51E-03 -2,90E-02
EP-FreshWater kg P -eq 0 0 0 3,94E-06 1,56E-05 5,04E-06 -2,28E-04
EP-Marine kg N -eq 0 0 0 9,75E-04 3,06E-03 1,66E-03 -6,07E-03
EP-Terrestial mol N eq 0 0 0 1,07E-02 3,22E-02 1,83E-02 -6,60E-02
POCP kg NMVOC -eq 0 0 0 3,07E-03 8,75E-03 5,22E-03 -1,98E-02
ADP-minerals&metals1 Kg Sb-eq 0 0 0 1,24E-05 5,11E-06 1,03E-05 -1,17E-05
ADP-fossil1 MJ 0 0 0 7,34E+00 1,47E+01 1,40E+01 -5,30E+01
WDP1 m3 0 0 0 6,96E+00 5,88E+01 2,80E+01 -1,74E+03
GWP total Global Warming Potential total; GWP fossil Global Warming Potential fossil fuels ; GWP biogenic Global Warming Potential biogenic; GWP luluc Global W
Potential land use change; ODP Ozone Depletion; AP Acidification; EP freshwater Eutrophication aquatic freshwater; EP marine Eutrophication aquatic marine; EP
terrestrial Eutrophication terrestrial ;POCP Photochemical zone formation; ADPE Abiotic Depletion Potential minerals and metals; ADPf Abiotic Depletion Potential fossil
fuels;
"Reading example: 9,0 E-03 = 9,0*10-3 = 0,009"
*INA Indicator Not Assessed
1. The results of this environmental impact indicator shall be used with care as the uncertainties on these results are high or as there is limited experienced with the
indicator
Remarks to environmental impacts
Global warming potential in A1-A3 includes sequestration of carbon in the wood. This amount is accounted as an emission in module C3. Additionally, it is included
sequestration in the wood packaging. This is accounted as an emission in module A5.
8 / 14
Additional environmental impact indicators
Parameter Unit A1-A3 A4 A5 B1 B2 B3
PM Disease incidence 1,32E-05 2,13E-07 9,78E-09 0 5,48E-06 0
IRP2 kgBq U235 eq. 6,37E+00 1,71E-01 4,36E-03 0 2,21E+00 0
ETP-fw1 CTUe 3,71E+03 2,86E+01 1,34E+00 0 1,50E+03 0
HTP-c1 CTUh 3,04E-07 0,00E+00 1,45E-10 0 9,69E-08 0
HTP-nc1 CTUh 2,82E-06 2,84E-08 6,95E-09 0 8,66E-07 0
SQP1 Pt 7,57E+03 4,06E+01 7,18E-01 0 3,33E+02 0
Parameter Unit B4 B5 C1 C2 C3 C4 D
PM Disease incidence 0 0 0 4,36E-08 1,76E-07 7,99E-08 -8,97E-07
IRP2 kgBq U235 eq. 0 0 0 3,21E-02 5,90E-02 5,57E-02 -2,75E-01
ETP-fw1 CTUe 0 0 0 5,49E+00 4,79E+01 7,14E+00 -1,53E+02
HTP-c1 CTUh 0 0 0 0,00E+00 7,56E-09 2,39E-10 -8,65E-09
HTP-nc1 CTUh 0 0 0 7,27E-09 6,03E-08 9,72E-09 -1,73E-07
SQP1 Pt 0 0 0 6,28E+00 6,08E+00 3,05E+01 -1,38E+02
PM Particulate Matter emissions; IRP Ionizing radiation – human health; ETP-fw Eco toxicity – freshwater; HTP-c Human toxicity – cancer effects; HTP-nc Human
toxicity – non cancer effects; SQP Soil Quality (dimensionless)
"Reading example: 9,0 E-03 = 9,0*10-3 = 0,009"
*INA Indicator Not Assessed
1. The results of this environmental impact indicator shall be used with care as the uncertainties on these results are high or as there is limited experienced with the
indicator
2. This impact category deals mainly with the eventual impact of low dose ionizing radiation on human health of the nuclear fuel cycle. It does not consider effects due
to possible nuclear accidents, occupational exposure nor due to radioactive waste disposal in underground facilities. Potential ionizing radiation from the soil, from
radon and from some construction materials is also not measured by this indicator.
9 / 14
Resource use
Parameter Unit A1-A3 A4 A5 B1 B2 B3
PERE MJ 5,74E+02 5,05E-01 2,46E-02 0 5,08E+01 0
PERM MJ 3,39E+02 0,00E+00 -4,98E+01 0 0,00E+00 0
PERT MJ 9,14E+02 5,05E-01 -4,98E+01 0 5,08E+01 0
PENRE MJ 1,67E+03 3,90E+01 1,19E+00 0 8,67E+02 0
PENRM MJ 1,10E+02 0,00E+00 -5,56E+00 0 2,80E+00 0
PENRT MJ 1,78E+03 3,90E+01 -4,37E+00 0 8,70E+02 0
SM kg 1,08E+00 0,00E+00 4,31E-06 0 1,34E-02 0
RSF MJ 1,15E+00 1,78E-02 7,14E-04 0 5,35E-01 0
NRSF MJ 9,42E-01 6,06E-02 7,84E-03 0 1,10E-01 0
FW m3 3,14E+00 4,37E-03 8,50E-04 0 7,63E-01 0
Parameter Unit B4 B5 C1 C2 C3 C4 D
PERE MJ 0 0 0 1,05E-01 2,45E+00 2,39E-01 -1,43E+02
PERM MJ 0 0 0 0,00E+00 -2,89E+02 0,00E+00 0,00E+00
PERT MJ 0 0 0 1,05E-01 -2,87E+02 2,38E-01 -1,43E+02
PENRE MJ 0 0 0 7,34E+00 1,47E+01 1,40E+01 -5,30E+01
PENRM MJ 0 0 0 0,00E+00 -1,05E+02 0,00E+00 0,00E+00
PENRT MJ 0 0 0 7,34E+00 -9,02E+01 1,40E+01 -1,42E+02
SM kg 0 0 0 0,00E+00 5,00E-05 3,61E-05 3,57E-01
RSF MJ 0 0 0 3,75E-03 5,07E-02 6,29E-03 -2,84E-02
NRSF MJ 0 0 0 1,32E-02 -1,30E-01 2,76E-01 -7,44E+00
FW m3 0 0 0 8,31E-04 1,20E-02 1,46E-02 -2,53E-01
PERE Use of renewable primary energy excluding renewable primary energy resources used as raw materials; PERM Use of renewable primary energy resources used as
raw materials; PERT Total use of renewable primary energy resources; PENRE Use of non renewable primary energy excluding non-renewable primary energy resources
used as raw materials; PENRM Use of non renewable primary energy resources used as raw materials; PENRT Total use of non renewable primary energy resources; SM
Use of secondary materials; RSF Use of renewable secondary fuels; NRSF Use of non renewable secondary fuels; FW Use of net fresh water
"Reading example: 9,0 E-03 = 9,0*10-3 = 0,009"
*INA Indicator Not Assessed
10 / 14
End of life - Waste
Parameter Unit A1-A3 A4 A5 B1 B2 B3
HWD kg 1,49E+00 2,10E-03 3,71E-02 0 4,78E+01 0
NHWD kg 2,99E+01 3,04E+00 1,25E-01 0 8,25E+00 0
RWD kg 6,62E-03 2,66E-04 6,55E-06 0 2,66E-03 0
Parameter Unit B4 B5 C1 C2 C3 C4 D
HWD kg 0 0 0 3,96E-04 3,19E-02 5,52E+01 9,12E-03
NHWD kg 0 0 0 4,55E-01 1,88E-01 4,64E-01 -1,26E+00
RWD kg 0 0 0 4,99E-05 8,53E-05 8,63E-05 -2,39E-04
HWD = Hazardous waste disposed; NHWD = Non-hazardous waste disposed; RWD = Radioactive waste disposed;
"Reading example: 9,0 E-03 = 9,0*10-3 = 0,009"
*INA Indicator Not Assessed
End of life - Output flow
Parameter Unit A1-A3 A4 A5 B1 B2 B3
CRU kg 0,00E+00 0,00E+00 0,00E+00 0 0,00E+00 0
MFR kg 5,02E-01 0,00E+00 1,42E+00 0 2,12E-02 0
MER kg 9,77E-03 0,00E+00 6,75E-06 0 4,91E-03 0
EEE MJ 6,76E-01 0,00E+00 1,56E+00 0 1,07E+00 0
EET MJ 9,58E+00 0,00E+00 2,36E+01 0 1,62E+01 0
Parameter Unit B4 B5 C1 C2 C3 C4 D
CRU kg 0 0 0 0,00E+00 0,00E+00 0,00E+00 0,00E+00
MFR kg 0 0 0 0,00E+00 3,97E-01 3,00E+00 3,26E-01
MER kg 0 0 0 0,00E+00 4,24E-04 6,62E-05 -6,10E-04
EEE MJ 0 0 0 0,00E+00 1,53E+01 1,43E+00 1,79E-02
EET MJ 0 0 0 0,00E+00 2,32E+02 2,16E+01 2,71E-01
CRU = Components for re-use; MFR = Materials for recycling; MER = Materials for energy recovery; EEE = Exported electrical energy; EET = Exported energy ​ Thermal
"Reading example: 9,0 E-03 = 9,0*10-3 = 0,009"
*INA Indicator Not Assessed
Biogenic Carbon Content
Parameter Unit At the factory gate
Biogenic carbon content in product kg C 7,47E+00
Biogenic carbon content in accompanying packaging kg C 1,56E+00
Note: 1 kg biogenic carbon is equivalent to 44/12 kg CO2
11 / 14
Additional Norwegian requirements
Greenhouse gas emissions from the use of electricity in the manufacturing phase
National production mix from import, low voltage (production of transmission lines, in addition to direct emissions and losses in grid) of applied electricity for the
manufacturing process (A3).
Electricity mix Data source Amount Unit
Electricity, Poland (kWh) ecoinvent 3.6 1060,47 g CO2-eq/kWh
Electricity, Norway (kWh) ecoinvent 3.6 24,33 g CO2-eq/kWh
Dangerous substances
The product contains no substances on the REACH Candidate list or the Norwegian priority list at or above 100 ppm, 0,01 % by weight.
Indoor environment
The product has not been tested for emissions to indoor environments.
Additional Environmental Information
Environmental impact indicators EN 15804+A1 and NPCR Part A v2.0
Parameter Unit A1-A3 A4 A5 B1 B2 B3
GWP kg CO2 -eq 1,58E+01 2,50E+00 1,05E-01 0 1,21E+01 0
ODP kg CFC11 -eq 1,45E-06 4,69E-07 1,33E-08 0 7,09E-07 0
POCP kg C2H4-eq 5,14E-03 3,28E-04 2,19E-05 0 5,15E-03 0
AP kg SO2 -eq 7,16E-02 5,03E-03 4,97E-04 0 4,95E-02 0
EP kg PO43- -eq 8,09E-03 5,46E-04 1,49E-04 0 6,16E-03 0
ADPM kg Sb -eq 2,05E-04 4,92E-05 1,64E-06 0 1,65E-04 0
ADPE MJ 1,78E+02 3,83E+01 1,16E+00 0 2,29E+02 0
GWPIOBC kg CO2 -eq 1,37E+02 2,53E+00 0,00E+00 0 6,19E+01 0
Parameter Unit B4 B5 C1 C2 C3 C4 D
GWP kg CO2 -eq 0 0 0 4,73E-01 5,62E+01 1,33E-02 -4,01E+00
ODP kg CFC11 -eq 0 0 0 8,72E-08 2,90E-08 1,14E-09 -3,53E-07
POCP kg C2H4-eq 0 0 0 6,75E-05 8,44E-05 1,53E-06 -2,99E-03
AP kg SO2 -eq 0 0 0 9,62E-04 3,12E-03 2,37E-05 -2,25E-02
EP kg PO43- -eq 0 0 0 1,00E-04 1,16E-03 3,21E-06 -3,56E-03
ADPM kg Sb -eq 0 0 0 1,24E-05 1,43E-06 7,31E-08 -1,17E-05
ADPE MJ 0 0 0 7,19E+00 2,69E+00 1,18E-01 -4,38E+01
GWPIOBC kg CO2 -eq 0 0 0 4,79E-01 3,00E+01 1,33E-02 -4,02E+00
GWP Global warming potential; ODP Depletion potential of the stratospheric ozone layer; POCP Formation potential of tropospheric photochemical oxidants; AP
Acidification potential of land and water; EP Eutrophication potential; ADPM Abiotic depletion potential for non fossil resources; ADPE Abiotic depletion​ potential for
fossil resources; GWP-IOBC/GHG Global warming potential calculated according to the principle of instantanious oxidation (except emissions and uptake of biogenic
carbon)
12 / 14
Bibliography
ISO 14025:2010 Environmental labels and declarations - Type III environmental declarations - Principles and procedures.
ISO 14044:2006 Environmental management - Life cycle assessment - Requirements and guidelines.
EN 15804:2012+A2:2019 Environmental product declaration - Core rules for the product category of construction products.
ISO 21930:2017 Sustainability in buildings and civil engineering works - Core rules for environmental product declarations of construction products.
ecoinvent v3, Allocation, cut-off by classification, Swiss Centre of Life Cycle Inventories.
Iversen et al., (2021) eEPD v2021.09 Background information for EPD generator tool system verification, LCA.no Report number: 07.21
Iversen et al., (2022) EPD generator for EPD generator for NPCR 014
Part B for Windows and doors, Background information for EPD generator application and LCA data, LCA.no report number: xx.xx
NPCR Part A: Construction products and services. Ver. 2.0. April 2021, EPD-Norge.
NPCR 014 Part B for Windows and doors, Ver. 4.0, 20.09.2021, EPD Norway.
EPD Norway Bruksanvisninger i hvordan tolke EPD'er - Vinduer URL: https://www.epd-norge.no [in Norwegian]
Program operator and publisher Phone: +47 23 08 80 00
The Norwegian EPD Foundation e-mail: post@epd-norge.no
Post Box 5250 Majorstuen, 0303 Oslo, Norway web: www.epd-norge.no
Owner of the declaration: Phone: +46 (0) 10-130 01 78
NorDan AS e-mail: fredrik.jonsson@nordan.se
Stasjonsveien 46, 4460 Moi web: www.nordan.no
Author of the Life Cycle Assessment Phone: +47 98 85 33 33
Norsk Treteknisk Institutt e-mail: firmapost@treteknisk.no
Postboks 113 Blindern, 0314 web: www.treteknisk.no
Developer of EPD generator Phone: +47 916 50 916
LCA.no AS e-mail: post@lca.no
Dokka 6B,1671 Kråkerøy web: www.lca.no
ECO Platform Web: www.eco-platform.org
ECO Portal Web: ECO Portal
13 / 14
EPD for the best
environmental
decision
The Norwegian EPD Foundation
www.epd-norge.no
14 / 14
