Environmental product declaration
in accordance with ISO 14025 and EN 15804+A2
Herning Wall Midi
OOwwnneerr ooff tthhee ddeeccllaarraattiioonn:: PPrrooggrraamm ooppeerraattoorr::
SG Armaturen AS The Norwegian EPD Foundation
PPrroodduucctt:: DDeeccllaarraattiioonn nnuummbbeerr::
Herning Wall Midi
NEPD-8333-8002-EN
DDeeccllaarreedd uunniitt::
1 pcs RReeggiissttrraattiioonn nnuummbbeerr::
TThhiiss ddeeccllaarraattiioonn iiss bbaasseedd oonn PPrroodduucctt CCaatteeggoorryy NEPD-8333-8002-EN
RRuulleess::
IIssssuuee ddaattee:: 06.12.2024
CEN Standard EN 15804:2012+A2:2019 serves as core
The Norwegian EPD Foundation PCR VVaalliidd ttoo:: 06.12.2029
IBU PCR - Part B for luminaires, lamps, and components
for luminaires EEPPDD ssooffttwwaarree::
LCAno EPD generator ID: 694837
1 / 14
GGeenneerraall iinnffoorrmmaattiioonn
PPrroodduucctt OOwwnneerr ooff tthhee ddeeccllaarraattiioonn::
Herning Wall Midi SG Armaturen AS
Contact person: Audun Skare
Phone: +47 90021243
e-mail: audun.skare@sg-as.no
PPrrooggrraamm ooppeerraattoorr:: MMaannuuffaaccttuurreerr::
The Norwegian EPD Foundation SG Armaturen AS
Post Box 5250 Majorstuen, 0303 Oslo, Norway Skytterheia 25
Phone: +47 977 22 020 4790 Lillesand, Norway
web: www.epd-norge.no
DDeeccllaarraattiioonn nnuummbbeerr:: PPllaaccee ooff pprroodduuccttiioonn::
SG Armaturen production site Dong Guan (China)
NEPD-8333-8002-EN No. 96 Wen Quan South Road, Shi Long Information Industrial Park
523325 Dong Guan, China
TThhiiss ddeeccllaarraattiioonn iiss bbaasseedd oonn PPrroodduucctt CCaatteeggoorryy RRuulleess:: MMaannaaggeemmeenntt ssyysstteemm::
CEN Standard EN 15804:2012+A2:2019 serves as core PCR
IBU PCR - Part B for luminaires, lamps, and components for
luminaires
SSttaatteemmeenntt ooff lliiaabbiilliittyy:: OOrrggaanniissaattiioonn nnoo::
The owner of the declaration shall be liable for the underlying 958560931
information and evidence. EPD Norway shall not be liable with respect
to manufacturer information, life cycle assessment data and
evidences.​
DDeeccllaarreedd uunniitt:: IIssssuuee ddaattee::
1 pcs Herning Wall Midi 06.12.2024
DDeeccllaarreedd uunniitt wwiitthh ooppttiioonn:: VVaalliidd ttoo::
A1,A2,A3,A4,A5,B6,C1,C2,C3,C4,D 06.12.2029
YYeeaarr ooff ssttuuddyy::
2022
FFuunnccttiioonnaall uunniitt:: CCoommppaarraabbiilliittyy::
1 Herning Wall Midi LED luminaire manufactured and installed, used EPD of construction products may not be comparable if they not
according to a specific lighting regime over 10 years, including waste comply with EN 15804 and seen in a building context.
treatment at end-of-life.
GGeenneerraall iinnffoorrmmaattiioonn oonn vveerriiffiiccaattiioonn ooff EEPPDD ffrroomm EEPPDD ttoooollss:: DDeevveellooppmmeenntt aanndd vveerriiffiiccaattiioonn ooff EEPPDD::
Independent verification of data, other environmental information The declaration is created using EPD tool lca.tools ver EPD2021.09,
and the declaration according to ISO 14025:2010, § 8.1.3 and § 8.1.4. developed by LCA.no. The EPD tool is integrated in the company's
Verification of each EPD is made according to EPD-Norway’s management system, and has been approved by EPD Norway.
guidelines for verification and approval requiring that tools are i) NEPDT63
integrated into the company's environmental management system, ii)
the procedures for use of the EPD tool are approved by EPD-Norway, Developer of EPD: Eva Linn Jenssen
and iii) the process is reviewed annually by an independent third
Reviewer of company-specific input data and EPD:​ Audun Skare
party verifier. See Appendix G of EPD-Norway's General Programme
Instructions for further information on EPD tools
VVeerriiffiiccaattiioonn ooff EEPPDD ttooooll:: AApppprroovveedd::
Independent third party verification of the EPD tool, background data
and test-EPD in accordance with EPDNorway's procedures and
guidelines for verification and approval of EPD tools. Approval
number: NEPDT41.
Third party verifier:
Vito D’Incognito, Take Care International
(no signature required)
2 / 14
PPrroodduucctt
PPrroodduucctt ddeessccrriippttiioonn::
A stylishly designed classic outdoor luminaire that is equally at home in urban and more rural settings. In solid powder-coated aluminium and with
a tempered glass front, it is equally suitable in domestic or public settings. The glass front conceals access to switches for 3000K/4000K and for 2
lumen levels, i.e. 4 combinations in one product. By default, it is set to 3000K and the highest lumen level. Easy installation with wall bracket and
quick connector. Multiple rear surface cable inputs plus punch-out entry points.
System Wattage: null W. Luminous flux: 1060/1140/1770/1920lm. Efficacy: 82/88/71/77lm/W. Colour temperature: 3000/4000K. Colour
rendering: Ra>80. MacAdams factor: SDCM: 3. Lifetime: L80/B20>50,000, . Light distribution: Direct. Control/Dimming: Trailing edge dimming.
Luminiare class: Class II. Housing: Aluminium. Optics: . Height: 222.0mm. Length: 402.0 mm. Width: 240.0 mm. EAN: 7021986239621
The EPD also covers the following products:
EAN: 7021986239638 - HERNING WALL MIDI GRAY 3000/4000K
EAN: 7021986239690 - HERNING WALL MIDI CORTEN
Please note that the above has been calculated with the Norwegian Energy-mix. If you want an EPD with a specific energy-mix, please send us a
request.
PPrroodduucctt ssppeecciiffiiccaattiioonn
MMaatteerriiaallss kkgg %%
Electronic - Connector 0,02 0,70
Electronic - Power supply 0,08 2,96
Electronic - Wire 0,01 0,51
Glass 0,41 14,49
Metal - Aluminium wrought alloy 0,43 15,43
Plastic - Polyamide 0,00 0,03
Plastic - Polyethylene (LDPE) 0,00 0,11
Plastic - Polyvinyl chloride (PVC) 0,00 0,01
Silicon products 0,05 1,64
Metal - Aluminium 1,66 58,87
Metal - Brass 0,00 0,02
Metal - Stainless steel 0,08 2,79
Plastic - Polycarbonate (PC) 0,07 2,45
Total 2,82 100,00
PPaacckkaaggiinngg kkgg %%
Packaging - Cardboard 1,14 99,41
Packaging - Recycled paper 0,01 0,59
Total incl. packaging 3,97 100,00
TTeecchhnniiccaall ddaattaa::
Link to product data on our website:
https://www.sg-as.com/products/herning-wall/623962/pdf/specification_623962.pdf
Link to CE Declaration:
https://www.sg-as.com/assets/product/default/data/130060_Herning/50/130060_Herning%20Wall.pdf
MMaarrkkeett::
Nordic + Northwestern Europe
RReeffeerreennccee sseerrvviiccee lliiffee,, pprroodduucctt
10 years. Estimated based on the characteristics of the product and the intended application.
RReeffeerreennccee sseerrvviiccee lliiffee,, bbuuiillddiinngg oorr ccoonnssttrruuccttiioonn wwoorrkkss
LLCCAA:: CCaallccuullaattiioonn rruulleess
DDeeccllaarreedd uunniitt::
1 pcs Herning Wall Midi
CCuutt--ooffff ccrriitteerriiaa::
All major raw materials and all the essential energy is included. The production processes for raw materials and energy flows with very small
amounts (less than 1%) can be excluded. These cut-off criteria do not apply for hazardous materials and substances.
AAllllooccaattiioonn::
3 / 14
The allocation is made in accordance with the provisions of EN 15804. Incoming energy and water and waste production in-house is allocated
equally among all products through mass allocation. Effects of primary production of recycled materials is allocated to the main product in which
the material was used. The recycling process and transportation of the material is allocated to this analysis.
DDaattaa qquuaalliittyy::
Specific data for the product composition are provided by the manufacturer. The data represent the production of the declared product and were
collected for EPD development in the year of study. Background data is based on EPDs according to EN 15804 and different LCA databases. The
data quality of the raw materials in A1 is presented in the table below.
MMaatteerriiaallss SSoouurrccee DDaattaa qquuaalliittyy YYeeaarr
Supplier data +
Electronic - Connector Material composition + ecoinvent 3.6 2019
database
Supplier data +
Electronic - Power supply Product composition + ecoinvent 3.6 2019
database
Supplier data +
Electronic - Wire Material composition + ecoinvent 3.6 2019
database
Glass ecoinvent 3.6 Database 2019
Metal - Aluminium Modified ecoinvent 3.6 Database 2019
Supplier data +
Metal - Aluminium wrought alloy Modified ecoinvent 3.6 2019
database
Metal - Brass Modified ecoinvent 3.6 Database 2019
Metal - Stainless steel Modified ecoinvent 3.6 Database 2019
Packaging - Cardboard Modified ecoinvent 3.6 Database 2019
Packaging - Recycled paper Modified ecoinvent 3.6 Database 2019
Plastic - Polyamide ecoinvent 3.6 Database 2019
Plastic - Polycarbonate (PC) ecoinvent 3.6 Database 2019
Plastic - Polyethylene (LDPE) ecoinvent 3.6 Database 2019
Supplier data +
Plastic - Polyvinyl chloride (PVC) Product composition + ecoinvent 3.6 2019
database
Silicon products ecoinvent 3.6 Database 2019
4 / 14
SSyysstteemm bboouunnddaarriieess ((XX==iinncclluuddeedd,, MMNNDD==mmoodduullee nnoott ddeeccllaarreedd,, MMNNRR==mmoodduullee nnoott rreelleevvaanntt))
CCoonnssttrruuccttiioonn BBeeyyoonndd tthhee ssyysstteemm
PPrroodduucctt ssttaaggee UUssee ssttaaggee EEnndd ooff lliiffee ssttaaggee
iinnssttaallllaattiioonn ssttaaggee bboouunnddaarriieess
A1 A2 A3 A4 A5 B1 B2 B3 B4 B5 B6 B7 C1 C2 C3 C4 D
X X X X X MND MND MND MND MND X MND X X X X X
SSyysstteemm bboouunnddaarryy::
AAddddiittiioonnaall tteecchhnniiccaall iinnffoorrmmaattiioonn::
Link to Mounting instruction on our website:
https://www.sg-as.com/assets/product/default/data/130060_Herning/20/130060_Herning_User%20Manual.pdf
waR slairetam tropsnarT gnirutcafunaM tropsnarT ylbmessA e​sU ecnanetniaM riapeR tnemecalpeR tnemhsibrufeR lanoitarepO ygrene esu lanoitarepO esu retaw -eD noitcurtsnoc noitilomed tropsnarT etsaW gnissecorp lasopsiD -yrevoceR-esueR laitnetop-gnilcyceR
5 / 14
LLCCAA:: SScceennaarriiooss aanndd aaddddiittiioonnaall tteecchhnniiccaall iinnffoorrmmaattiioonn
The following information describe the scenarios in the different modules of the EPD.
Module A4 = Transportation by truck (40 km) from the production site in Dong Guan, China to the harbor. After this the goods are transported
by ship (19000 km) from Dong Guan, China to Hamburg, Germany. Then with a truck (650 km) from Hamburg, Germany to the warehouse in
Lillesand, Norway or to the warehouse in Mechelen, Belgium + 800 km for Nordic / Northwestern Europe Market.
Module A5 = Installation is performed in the Nordic / Northwestern Europe Market and done by manual labor, with the use of electrical machines,
that fall under the cut-off criteria of 1% and is therefore neglected. Packaging of the final product consist of a corrugated board box.
Scenario: Outdoor - Facade
Module B6 = The operational energy use of the luminaire is calculated based on the methodology provided in IBU PCR Part B for luminaires,
lamps, and components for luminaires. The energy consumption model for luminaire used in the PCR follows the application scenarios developed
in EN 15193:2007. To calculate the electricity use of the luminaire, the following scenario parameters have been applied:
- Active power of the luminaire (Pa) = 25 watt
- Passive power of the luminaire (Pp) = 0 watt
- Daylight time usage (tD) = 0 hours
- Non-daylight time usage (tN) = 1825 hours
- Standard year time (ty) = 8760 hours
- The occupancy depency factor (FO) = 1
- The daylight dependency factor (FD) = 1
- The product specific constant illuminance factor (FCP) = 1
- The non-daylight dimming factor (FN) = 0,9
- The application specific empiric lifetime of the luminaire in years (a) = 10 years (corresponding to the reference service life of the product).
Module C1 = The de-installation of the luminaire is done by manual labor, with the help of electrical machines. The use of portable electrical
devices (e.g., drill) usually have low energy requirements falling under the cut-off-criterion of 1% and is therefore neglected.
Module C2 = Transportation from building site to the waste treatment facility with an average distance of 300km.
Modules C3 and C4 = Waste treatment of the product follows the default values provided in EN 50693, Product Category Rules for life cycle
assessments of electronic and electrical products and systems, table G.4. This table specified how different types of raw materials used in A1 will
likely be treated during the end-of-life of the product. Waste treatments in C3 include material recycling and incineration with and without energy
recovery and fly ash extraction. Disposal in C4 consist of landfilling of different waste fractions and of ashes.
Module D = The recyclability of metals, plastics, and electronic components allows the producers a credit for the net scrap that is produced at the
end of a product’s life. The benefits from recycling of net scrap are described in formula from EN 15804:2012+A2:2019. Substitution of heat and
electricity generated by the incineration with energy recovery of plastic insulation and other parts is also calculated in module D.
TTrraannssppoorrtt ffrroomm pprroodduuccttiioonn ppllaaccee ttoo uusseerr CCaappaacciittyy uuttiilliissaattiioonn VVaalluuee
DDiissttaannccee ((kkmm)) FFuueell//EEnneerrggyy CCoonnssuummppttiioonn UUnniitt
((AA44)) ((iinnccll.. rreettuurrnn)) %% ((LLiitteerr//ttoonnnnee))
Ship, Freight, Transoceanic (km) 65,0 % 19000 0,003 l/tkm 57,00
Truck, 16-32 tonnes, EURO 6 (km) - Europe 36,7 % 1450 0,043 l/tkm 62,35
Truck, 16-32 tonnes, EURO 6 (km) - Rest of World 38,8 % 40 0,044 l/tkm 1,76
AAsssseemmbbllyy ((AA55)) UUnniitt VVaalluuee
Waste, packaging, paper printed, 100% recycled
content, to average treatment (kg) - Global - A5, kg 0,01
incl. 85 km transp
Waste, packaging, corrugated board box, with
recycled content, to average treatment (kg) - A5 kg 1,14
including transport
OOppeerraattiioonnaall eenneerrggyy ((BB66)) UUnniitt VVaalluuee
Electricity, Norway (kWh) kWh 410,63
CCaappaacciittyy uuttiilliissaattiioonn VVaalluuee
TTrraannssppoorrtt ttoo wwaassttee pprroocceessssiinngg ((CC22)) DDiissttaannccee ((kkmm)) FFuueell//EEnneerrggyy CCoonnssuummppttiioonn UUnniitt
((iinnccll.. rreettuurrnn)) %% ((LLiitteerr//ttoonnnnee))
Truck, 16-32 tonnes, EURO 6 (km) - Rest of World 38,8 % 300 0,044 l/tkm 13,20
6 / 14
WWaassttee pprroocceessssiinngg ((CC33)) UUnniitt VVaalluuee
Steel to recycling (kg) kg 0,07
Waste treatment of plastic mixture, incineration
kg 0,08
with energy recovery and fly ash extraction (kg)
Waste treatment of polyethylene (PE),
incineration with energy recovery and fly ash kg 0,00
extraction (kg)
Aluminium to recycling (kg) kg 1,47
Waste treatment per kg used PWB, shredding and
kg 0,05
separation - C3 (kg)
Waste treatment per kg electronics scrap from
PWB, with components, recycling of metals C3 kg 0,03
(kg)
Waste treatment per kg used electronic
kg 0,12
components, manual seperation (kg)
Copper to recycling (kg) kg 0,01
Brass to recycling (kg) kg 0,00
Glass to recycling (kg) kg 0,25
DDiissppoossaall ((CC44)) UUnniitt VVaalluuee
Landfilling of steel (kg) kg 0,02
Landfilling of ashes from incineration of Plastic
kg 0,00
mixture, process per kg ashes and residues (kg)
Landfilling of plastic mixture (kg) kg 0,08
Landfilling of ashes from incineration of
Polyethylene (PE), process per kg ashes and kg 0,00
residues (kg)
Landfilling of aluminium (kg) kg 0,63
Landfilling of hazardous waste (kg) kg 0,03
Landfilling of copper (kg) kg 0,01
Landfilling of brass (kg) kg 0,00
Landfilling of glass (kg) kg 0,16
BBeenneeffiittss aanndd llooaaddss bbeeyyoonndd tthhee ssyysstteemm
UUnniitt VVaalluuee
bboouunnddaarriieess ((DD))
Substitution of primary steel with net scrap (kg) kg 0,07
Substitution of electricity (MJ) MJ 0,19
Substitution of thermal energy, district heating
MJ 2,92
(MJ)
Substitution of primary aluminium with net scrap
kg 0,26
(kg)
Substitution of primary metals with net scrap
kg 0,01
from PWB, with components (kg)
Substitution of primary copper with net scrap (kg) kg 0,01
Substitution of primary Brass with net scrap (kg) kg 0,00
Substitution of primary glass with net scrap (kg) kg 0,25
7 / 14
LLCCAA:: RReessuullttss
The LCA results are presented below for the declared unit defined on page 2 of the EPD document.
EEnnvviirroonnmmeennttaall iimmppaacctt
IInnddiiccaattoorr UUnniitt A1 A2 A3 A4 A5
GWP-total kg CO2 -eq 3,24E+01 1,54E-02 1,53E+00 1,68E+00 1,97E+00
GWP-fossil kg CO2 -eq 3,40E+01 1,54E-02 1,53E+00 1,68E+00 1,86E-02
GWP-biogenic kg CO2 -eq -1,65E+00 5,98E-06 3,82E-04 5,95E-04 1,95E+00
GWP-luluc kg CO2 -eq 9,10E-02 5,62E-06 2,42E-04 8,35E-04 6,16E-06
ODP kg CFC11 -eq 1,28E-05 3,34E-09 2,25E-08 3,70E-07 3,93E-09
AP mol H+ -eq 2,55E-01 4,60E-05 8,01E-03 2,59E-02 8,82E-05
EP-FreshWater kg P -eq 2,35E-03 1,44E-07 3,40E-05 1,07E-05 1,53E-07
EP-Marine kg N -eq 3,82E-02 9,05E-06 1,65E-03 6,22E-03 2,92E-05
EP-Terrestial mol N -eq 4,37E-01 1,01E-04 1,82E-02 6,93E-02 3,16E-04
POCP kg NMVOC -eq 1,28E-01 3,79E-05 4,80E-03 1,87E-02 9,08E-05
ADP-minerals&metals1 kg Sb-eq 1,08E-02 4,12E-07 4,74E-06 3,20E-05 4,53E-07
ADP-fossil1 MJ 3,63E+02 2,27E-01 1,36E+01 2,37E+01 2,60E-01
WDP1 m3 1,91E+03 7,40E-02 2,21E+00 1,57E+01 3,30E-01
IInnddiiccaattoorr UUnniitt B6 C1 C2 C3 C4 D
GWP-total kg CO2 -eq 9,99E+00 0,00E+00 2,03E-01 2,27E-01 2,62E-02 -3,19E+00
GWP-fossil kg CO2 -eq 9,68E+00 0,00E+00 2,03E-01 2,27E-01 2,61E-02 -3,13E+00
GWP-biogenic kg CO2 -eq 2,68E-01 0,00E+00 7,89E-05 6,21E-05 1,69E-05 -1,45E-02
GWP-luluc kg CO2 -eq 3,99E-02 0,00E+00 7,41E-05 6,31E-05 5,59E-05 -4,55E-02
ODP kg CFC11 -eq 6,64E-07 0,00E+00 4,41E-08 2,26E-09 3,69E-09 -1,23E-03
AP mol H+ -eq 7,57E-02 0,00E+00 6,06E-04 1,64E-04 1,20E-04 -5,11E-02
EP-FreshWater kg P -eq 6,96E-04 0,00E+00 1,90E-06 1,03E-06 4,57E-07 -2,81E-04
EP-Marine kg N -eq 8,32E-03 0,00E+00 1,19E-04 4,22E-05 4,84E-05 -4,12E-03
EP-Terrestial mol N -eq 1,08E-01 0,00E+00 1,33E-03 4,55E-04 4,30E-04 -5,04E-02
POCP kg NMVOC -eq 2,91E-02 0,00E+00 5,00E-04 1,20E-04 1,36E-04 -1,54E-02
ADP-minerals&metals1 kg Sb-eq 7,22E-04 0,00E+00 5,43E-06 2,42E-07 1,28E-07 -7,28E-04
ADP-fossil1 MJ 1,32E+02 0,00E+00 2,99E+00 3,30E-01 3,36E-01 -3,91E+01
WDP1 m3 2,30E+04 0,00E+00 9,76E-01 3,00E+00 5,80E+00 -1,34E+03
GWP-total = Global Warming Potential total; GWP-fossil = Global Warming Potential fossil fuels; GWP-biogenic = Global Warming Potential biogenic; GWP-luluc =
Global Warming Potential land use and land use change; ODP = Depletion potential of the stratospheric ozone layer; AP = Acidification potential, Accumulated
Exceedance; EP-freshwater = Eutrophication potential, fraction of nutrients reaching freshwater end compartment: EP-marine = Eutrophication potential, fraction of
nutrients reaching marine end compartment; EP-terrestrial = Eutrophication potential, Accumulated Exceedance; POCP = Formation potential of tropospheric ozone;
ADP-minerals&metals = Abiotic depletion potential for non-fossil resources; ADP-fossil = Abiotic depletion for fossil resources potential; WDP = Water (user)
deprivation potential, deprivation-weighted water consumption
"Reading example: 9,0 E-03 = 9,0*10-3 = 0,009"
*INA Indicator Not Assessed
1. The results of this environmental impact indicator shall be used with care as the uncertainties on these results are high or as there is limited experienced with the
indicator
RReemmaarrkkss ttoo eennvviirroonnmmeennttaall iimmppaaccttss
8 / 14
The product is compliant with the European RoHS Directive 2011/65/EU on Restriction of the use of certain Hazardous Substances in Electrical and
Electronic equipment and with the European REACH regulation (EC) no 1907/2006 on Registration, Evaluation, Authorization and Restriction of
Chemicals.
9 / 14
AAddddiittiioonnaall eennvviirroonnmmeennttaall iimmppaacctt iinnddiiccaattoorrss
IInnddiiccaattoorr UUnniitt A1 A2 A3 A4 A5
PM Disease incidence 2,30E-06 9,88E-10 1,08E-07 5,93E-08 1,30E-09
IRP2 kgBq U235 -eq 8,93E-01 9,44E-04 1,17E-02 1,03E-01 1,11E-03
ETP-fw1 CTUe 1,98E+03 1,84E-01 3,98E+01 1,61E+01 3,47E-01
HTP-c1 CTUh 5,19E-08 0,00E+00 4,30E-10 0,00E+00 1,10E-11
HTP-nc1 CTUh 1,20E-06 1,79E-10 1,88E-08 1,18E-08 4,37E-10
SQP1 dimensionless 1,20E+02 1,56E-01 2,88E+00 1,14E+01 1,75E-01
IInnddiiccaattoorr UUnniitt B6 C1 C2 C3 C4 D
PM Disease incidence 5,42E-07 0,00E+00 1,31E-08 1,02E-09 2,15E-09 -2,66E-07
IRP2 kgBq U235 -eq 2,40E+00 0,00E+00 1,24E-02 1,60E-03 1,78E-03 -1,58E-01
ETP-fw1 CTUe 6,02E+02 0,00E+00 2,43E+00 9,42E-01 4,03E+02 -2,81E+02
HTP-c1 CTUh 2,87E-08 0,00E+00 0,00E+00 4,71E-10 4,50E-11 -7,68E-09
HTP-nc1 CTUh 6,77E-07 0,00E+00 2,38E-09 2,78E-08 5,37E-10 -1,67E-07
SQP1 dimensionless 6,66E+01 0,00E+00 2,05E+00 7,80E-02 7,04E-01 -7,91E+00
PM = Particulate Matter emissions; IRP = Ionizing radiation – human health; ETP-fw = Eco toxicity – freshwater; HTP-c = Human toxicity – cancer effects; HTP-nc =
Human toxicity – non cancer effects; SQP = Potential Soil Quality Index (dimensionless)
"Reading example: 9,0 E-03 = 9,0*10-3 = 0,009"
*INA Indicator Not Assessed
1. The results of this environmental impact indicator shall be used with care as the uncertainties on these results are high or as there is limited experienced with the
indicator
2. This impact category deals mainly with the eventual impact of low dose ionizing radiation on human health of the nuclear fuel cycle. It does not consider effects due
to possible nuclear accidents, occupational exposure nor due to radioactive waste disposal in underground facilities. Potential ionizing radiation from the soil, from
radon and from some construction materials is also not measured by this indicator.
10 / 14
RReessoouurrccee uussee
IInnddiiccaattoorr UUnniitt A1 A2 A3 A4 A5
PERE MJ 6,05E+01 2,57E-03 1,37E+00 2,69E-01 4,29E-03
PERM MJ 6,79E+00 0,00E+00 0,00E+00 0,00E+00 -6,79E+00
PERT MJ 6,73E+01 2,57E-03 1,37E+00 2,69E-01 -6,79E+00
PENRE MJ 3,60E+02 2,27E-01 1,36E+01 2,37E+01 2,61E-01
PENRM MJ 3,75E+00 0,00E+00 0,00E+00 0,00E+00 0,00E+00
PENRT MJ 3,63E+02 2,27E-01 1,36E+01 2,37E+01 2,61E-01
SM kg 2,36E+00 0,00E+00 0,00E+00 0,00E+00 0,00E+00
RSF MJ 2,03E-01 5,03E-05 1,20E-03 8,87E-03 1,42E-04
NRSF MJ 1,04E-01 4,27E-04 1,13E-02 4,75E-02 5,86E-04
FW m3 2,84E-01 2,54E-05 3,70E-02 2,04E-03 1,23E-04
IInnddiiccaattoorr UUnniitt B6 C1 C2 C3 C4 D
PERE MJ 1,71E+03 0,00E+00 3,39E-02 4,21E-02 5,40E-02 -1,30E+01
PERM MJ 0,00E+00 0,00E+00 0,00E+00 0,00E+00 0,00E+00 0,00E+00
PERT MJ 1,71E+03 0,00E+00 3,39E-02 4,21E-02 5,40E-02 -1,30E+01
PENRE MJ 1,32E+02 0,00E+00 2,99E+00 3,30E-01 3,36E-01 -3,91E+01
PENRM MJ 0,00E+00 0,00E+00 0,00E+00 -4,40E+00 0,00E+00 0,00E+00
PENRT MJ 1,32E+02 0,00E+00 2,99E+00 -4,07E+00 3,36E-01 -3,91E+01
SM kg 0,00E+00 0,00E+00 0,00E+00 0,00E+00 5,91E-04 5,87E-03
RSF MJ 1,34E+00 0,00E+00 6,63E-04 7,40E-04 6,99E-04 -1,48E-03
NRSF MJ 3,35E+00 0,00E+00 5,63E-03 -2,77E-05 5,22E-03 3,82E-03
FW m3 1,28E+01 0,00E+00 3,35E-04 4,24E-04 3,81E-04 -6,64E-02
PERE = Use of renewable primary energy excluding renewable primary energy resources used as raw materials; PERM = Use of renewable primary energy resources used
as raw materials; PERT = Total use of renewable primary energy resources; PENRE = Use of non renewable primary energy excluding non-renewable primary energy
resources used as raw materials; PENRM = Use of non renewable primary energy resources used as raw materials; PENRT = Total use of non renewable primary energy
resources; SM = Use of secondary materials; RSF = Use of renewable secondary fuels; NRSF = Use of non-renewable secondary fuels; FW = Net use of fresh water
"Reading example: 9,0 E-03 = 9,0*10-3 = 0,009"
*INA Indicator Not Assessed
11 / 14
EEnndd ooff lliiffee -- WWaassttee
IInnddiiccaattoorr UUnniitt A1 A2 A3 A4 A5
HWD kg 2,56E-01 2,05E-05 1,87E-03 1,16E-03 0,00E+00
NHWD kg 5,47E+00 1,09E-02 1,27E-01 7,31E-01 1,15E+00
RWD kg 8,04E-04 1,49E-06 1,04E-05 1,63E-04 0,00E+00
IInnddiiccaattoorr UUnniitt B6 C1 C2 C3 C4 D
HWD kg 8,49E-02 0,00E+00 2,70E-04 1,37E-05 5,19E-02 6,64E-03
NHWD kg 1,02E+01 0,00E+00 1,44E-01 1,84E-02 9,06E-01 -8,11E-01
RWD kg 1,18E-03 0,00E+00 1,96E-05 6,79E-07 1,63E-06 -1,50E-04
HWD = Hazardous waste disposed; NHWD = Non-hazardous waste disposed; RWD = Radioactive waste disposed
"Reading example: 9,0 E-03 = 9,0*10-3 = 0,009"
*INA Indicator Not Assessed
EEnndd ooff lliiffee -- OOuuttppuutt ffllooww
IInnddiiccaattoorr UUnniitt A1 A2 A3 A4 A5
CRU kg 0,00E+00 0,00E+00 0,00E+00 0,00E+00 0,00E+00
MFR kg 0,00E+00 0,00E+00 4,04E-02 0,00E+00 1,07E+00
MER kg 0,00E+00 0,00E+00 8,72E-03 0,00E+00 4,77E-04
EEE MJ 0,00E+00 0,00E+00 1,31E-02 0,00E+00 6,58E-02
EET MJ 0,00E+00 0,00E+00 1,99E-01 0,00E+00 9,96E-01
IInnddiiccaattoorr UUnniitt B6 C1 C2 C3 C4 D
CRU kg 0,00E+00 0,00E+00 0,00E+00 0,00E+00 0,00E+00 0,00E+00
MFR kg 0,00E+00 0,00E+00 0,00E+00 1,78E+00 7,38E-06 -2,36E-04
MER kg 0,00E+00 0,00E+00 0,00E+00 8,23E-02 1,81E-07 -3,11E-05
EEE MJ 0,00E+00 0,00E+00 0,00E+00 1,27E-01 1,17E-05 -7,86E-05
EET MJ 0,00E+00 0,00E+00 0,00E+00 1,92E+00 1,77E-04 -1,19E-03
CRU = Components for re-use; MFR = Materials for recycling; MER = Materials for energy recovery; EEE = Exported energy electrical; EET = Exported energy thermal
"Reading example: 9,0 E-03 = 9,0*10-3 = 0,009"
*INA Indicator Not Assessed
BBiiooggeenniicc CCaarrbboonn CCoonntteenntt
IInnddiiccaattoorr UUnniitt AAtt tthhee ffaaccttoorryy ggaattee
Biogenic carbon content in product kg C 0,00E+00
Biogenic carbon content in accompanying packaging kg C 5,33E-01
Note: 1 kg biogenic carbon is equivalent to 44/12 kg CO2
12 / 14
AAddddiittiioonnaall rreeqquuiirreemmeennttss
GGrreeeennhhoouussee ggaass eemmiissssiioonnss ffrroomm tthhee uussee ooff eelleeccttrriicciittyy iinn tthhee mmaannuuffaaccttuurriinngg pphhaassee
National production mix from import, low voltage (production of transmission lines, in addition to direct emissions and losses in grid) of applied
electricity for the manufacturing process (A3).
EElleeccttrriicciittyy mmiixx SSoouurrccee AAmmoouunntt UUnniitt
Electricity, China (kWh) ecoinvent 3.6 1102,91 g CO2-eq/kWh
DDaannggeerroouuss ssuubbssttaanncceess
The product contains no substances given by the REACH Candidate list.
IInnddoooorr eennvviirroonnmmeenntt
No effect on indoor environment
AAddddiittiioonnaall EEnnvviirroonnmmeennttaall IInnffoorrmmaattiioonn
AAddddiittiioonnaall eennvviirroonnmmeennttaall iimmppaacctt iinnddiiccaattoorrss rreeqquuiirreedd iinn NNPPCCRR PPaarrtt AA ffoorr ccoonnssttrruuccttiioonn pprroodduuccttss
IInnddiiccaattoorr UUnniitt A1 A2 A3 A4 A5
GWPIOBC kg CO2 -eq 3,43E+01 1,54E-02 1,45E+00 1,68E+00 1,86E-02
IInnddiiccaattoorr UUnniitt B6 C1 C2 C3 C4 D
GWPIOBC kg CO2 -eq 9,97E+00 0,00E+00 2,03E-01 2,27E-01 2,83E-02 -3,11E+00
GWP-IOBC: Global warming potential calculated according to the principle of instantaneous oxidation. In order to increase the transparency of biogenic carbon​
contribution to climate impact, the indicator GWP-IOBC is required as it declares climate impacts calculated according to the principle of instantaneous oxidation.​
GWP-IOBC is also referred to as GWP-GHG in context to Swedish public procurement legislation.
13 / 14
BBiibblliiooggrraapphhyy
ISO 14025:2010. Environmental labels and declarations - Type III environmental declarations - Principles and procedures. International
Organization for Standardization.
ISO 14044:2006. Environmental management - Life cycle assessment - Requirements and guidelines. International Organization for
Standardization.
EN 15804:2012+A2:2019. Environmental product declaration - Core rules for the product category of construction products. European
Committee for Standardization.
ISO 21930:2017. Sustainability in buildings and civil engineering works - Core rules for environmental product declarations of construction
products. International Organization for Standardization.
EN 50693:2019. Product category rules for life cycle assessments of electronic and electrical products and systems. European Committee for
Standardization.
Ecoinvent v3, 2019. Allocation, cut-off by classification. Swiss Centre of Life Cycle Inventories.
Iversen et al., (2021). eEPD v2021.09, background information for EPD generator tool system verification, LCA.no. Report number: 07.21. System
verification report.
Philis et al., (2022). EPD generator for IBU PCR part B for luminaires, lamps, and components for luminaires, background information for EPD
generator application and LCA data, LCA.no. Report number: 04.22. PCR verification report.
EPD Norway (2022). NPCR Part A: Construction products and services. The Norwegian EPD foundation. Version 2.0 published 24.03.2021.
IBU (2017). PCR part B for luminaires, lampes and components for luminaires. Institut Bauen und Umwelt e.V. Version 1.7, published 30.11.2017.
PPrrooggrraamm ooppeerraattoorr aanndd ppuubblliisshheerr Phone: +47 977 22 020
The Norwegian EPD Foundation e-mail: post@epd-norge.no
Post Box 5250 Majorstuen, 0303 Oslo, Norway web: www.epd-norge.no
OOwwnneerr ooff tthhee ddeeccllaarraattiioonn:: Phone: +47 90021243
SG Armaturen AS e-mail: audun.skare@sg-as.no
Skytterheia 25, 4790 Lillesand, Norway web: www.sg-as.com
AAuutthhoorr ooff tthhee LLiiffee CCyyccllee AAsssseessssmmeenntt Phone: +47 916 50 916
LCA.no AS e-mail: post@lca.no
Dokka 6A, 1671 Kråkerøy, Norway web: www.lca.no
DDeevveellooppeerr ooff EEPPDD ggeenneerraattoorr Phone: +47 916 50 916
LCA.no AS e-mail: post@lca.no
Dokka 6A, 1671 Kråkerøy, Norway web: www.lca.no
ECO Platform web: www.eco-platform.org
ECO Portal web: ECO Portal
14 / 14
