Environmental product declaration
in accordance with ISO 14025 and EN 15804+A2
HÅG Tribute
Owner of the declaration: Program operator:
Flokk AS The Norwegian EPD Foundation
Product: Declaration number:
HÅG Tribute
Registration number:
Declared unit:
1 pcs Issue date:
This declaration is based on Product Category Rules: Valid to:
CEN Standard EN 15804:2012+A2:2019 serves as core
EPD Software:
PCR
The Norwegian EPD Foundation LCA.no EPD generator ID: 166544
NPCR 026:2022 Part B for Furniture
1 / 13
General information
Product Owner of the declaration:
HÅG Tribute Flokk AS
Contact person: Atle Thiis-Messel
Phone: 0047 98 25 68 30
e-mail: atle.messel@flokk.com
Program operator: Manufacturer:
Post Box 5250 Majorstuen, 0303 Oslo, Norway Flokk AS
The Norwegian EPD Foundation Drammensveien 145,
Phone: +47 23 08 80 00 0277 Oslo, Norway
web: post@epd-norge.no
Declaration number: Place of production:
Flokk - Røros
Sundveien
N-7374 Røros, Norway
This declaration is based on Product Category Rules: Management system:
CEN Standard EN 15804:2012+A2:2019 serves as core PCR ISO 14001, ISO 9001, ISO 50001(Norway, Sweden)
NPCR 026:2022 Part B for Furniture
Statement of liability: Organisation no:
The owner of the declaration shall be liable for the underlying No 928 902 749
information and evidence. EPD Norway shall not be liable with respect
to manufacturer information, life cycle assessment data and
evidences.​
Declared unit: Issue date:
1 pcs HÅG Tribute
Declared unit (cradle to gate) with option: Valid to:
A1-A3,A4,A5,B2,B3,B4,C1,C2,C3,C4,D
Year of study:
2023
Functional unit: Comparability:
1 pcs HÅG Tribute 9031 w/ headrest, including packaging, excluding EPD of construction products may not be comparable if they not
armrests. comply with EN 15804 and seen in a building context.
General information on verification of EPD from EPD tools: Development and verification of EPD:
Independent verification of data, other environmental information The declaration is created using EPD tool lca.tools ver EPD2022.03,
and the declaration according to ISO 14025:2010, § 8.1.3 and § 8.1.4. developed by LCA.no. The EPD tool is integrated in the company's
Verification of each EPD is made according to EPD-Norway’s management system, and has been approved by EPD Norway.
guidelines for verification and approval requiring that tools are i)
integrated into the company's environmental management system, ii) Developer of EPD: Kenneth Dam Lindegaard Knudsen
the procedures for use of the EPD tool are approved by EPD-Norway,
Reviewer of company-specific input data and EPD: Atle Thiis-Messel
and iii) the process is reviewed annually by an independent third
party verifier. See Appendix G of EPD-Norway's General Programme
Instructions for further information on EPD tools
Verification of EPD tool: Approved:
Independent third party verification of the EPD tool, background data
and test-EPD in accordance with EPDNorway's procedures and
guidelines for verification and approval of EPD tools. Håkon Hauan, CEO EPD-Norge
Third party verifier:
Elisabet Amat, GREENIZE projects
(no signature required)
2 / 13
Product
Product description:
The HÅG Tribute family of chairs seamlessly blends unbeatable comfort with exclusive design. Crafted with precision in Røros, Norway, each chair
reflects HÅG's commitment to lasting quality and sustainable craftsmanship. Designed in collaboration with Svein Asbjørnsen, the chairs feature a
unique S-curved back, reducing tension in the upper body.
Boasting HÅG inBalance® technology, the chair provides a smooth tilt function that responds to your every move. The active upper back and
headrest offer ideal support during recline, while the HÅG TiltDown™ armrests, available with black leather tops, enhance freedom of movement.
Whether utilized as a luxury task or meeting chair, the HÅG Tribute combines style and functionality. Crafted by skilled technicians, it is the
epitome of an uncompromisingly comfortable executive chair. The fully integrated lumbar support, easily personalized with a sophisticated wheel,
adds to the tailored sitting experience.
With its timeless design, environmental consciousness, and HÅG inBalance® technology, the HÅG Tribute family commands attention in any
setting, going beyond mere furniture to enhance overall well-being.
Product specification
The model studied in this declaration is the HÅG Tribute 9031, including packaging & headrest. The model declared does not include armrests of
either type.
The key environmental indicators for the other models of the family, and applicable options of the product collection are presented in a table on
page 12 of this declaration.
Recycled share in Recycled share in
Materials kg %
material (kg) material (%)
Metal - Aluminium 5,62 24,10 5,62 100,00
Metal - Steel 6,83 29,33 0,70 10,30
Metal - Steel low alloy 0,01 0,03 0,01 100,00
Metal - Zinc 0,50 2,15 0,00 0,00
Others 0,01 0,03 0,00 1,24
Plastic - Nylon (PA) 0,66 2,85 0,08 12,16
Plastic - Polyamide 0,07 0,32 0,00 0,00
Plastic - Polyethylene (HDPE) 0,06 0,27 0,00 0,00
Plastic - Polyoxymethylene (POM) 0,38 1,62 0,00 0,00
Plastic - Polypropylene (PP) 5,13 22,03 2,96 57,62
Plastic - Polystyrene expandable (EPS) 0,43 1,85 0,00 0,00
Plastic - Polyurethane (PUR) 2,03 8,71 0,00 0,00
Powder coating 0,33 1,40 0,00 0,00
Reinforcement 0,63 2,69 0,00 0,00
Rubber, synthetic 0,11 0,49 0,00 0,00
Textile - Felt 0,00 0,01 0,00 44,44
Textile - Polyester (PE) 0,50 2,12 0,49 97,98
Total 23,30 9,85
Recycled share in Recycled share in
Packaging kg %
material (kg) material (%)
Packaging - Cardboard 1,44 31,13 0,00 0,00
Packaging - Paper 0,03 0,55 0,01 34,31
Packaging - Plastic 0,26 5,71 0,00 0,00
Recycled cardboard 2,90 62,61 2,90 100,00
Total incl. packaging 27,93 12,76
Technical data:
Total weight: 22,87 kg (packaging excluded)
Total weight: 27,93 kg (packaging included)
Market:
Worldwide.
A4 stage based on shipping scenario from factory in Røros, Norway, to Copenhagen, Denmark.
See table on page 6 for further detail.
Reference service life, product
15 years
Reference service life, building
LCA: Calculation rules
Declared unit:
1 pcs HÅG Tribute
3 / 13
Cut-off criteria:
All major raw materials and all the essential energy is included. The production processes for raw materials and energy flows with very small
amounts (less than 1%) are not included. These cut-off criteria do not apply for hazardous materials and substances.
Allocation:
The allocation is made in accordance with the provisions of EN 15804. Incoming energy and water and waste production in-house is allocated
equally among all products through mass allocation. Effects of primary production of recycled materials is allocated to the main product in which
the material was used. The recycling process and transportation of the material is allocated to this analysis.
Data quality:
Specific data for the product composition are provided by the manufacturer. They represent the production of the declared product and were
collected for EPD development in the year of study. Background data is based on registered EPDs according to EN 15804, Ostfold Research
databases, ecoinvent and other LCA databases. The data quality of the raw materials in A1 is presented in the table below.​
Materials Source Data quality Year
Metal - Aluminium ecoinvent 3.6 database 2019
Metal - Steel ecoinvent 3.6 Database 2019
Metal - Steel low alloy ecoinvent 3.6 Database 2019
Metal - Zinc ecoinvent 3.6 Database 2019
Others ecoinvent 3.6 Database 2019
Packaging - Paper ecoinvent 3.6 Database 2019
Packaging - Plastic ecoinvent 3.6 Database 2019
Plastic - Nylon (PA) ecoinvent 3.6 Database 2019
Plastic - Polyethylene (HDPE) ecoinvent 3.6 Database 2019
Plastic - Polyoxymethylene (POM) ecoinvent 3.6 Database 2019
Plastic - Polypropylene (PP) ecoinvent 3.6 Database 2019
Plastic - Polystyrene expandable (EPS) ecoinvent 3.6 Database 2019
Plastic - Polyurethane (PUR) ecoinvent 3.6 Database 2019
Powder coating Ecoinvent 3.6 Database 2019
Reinforcement ecoinvent 3.6 Database 2019
Rubber, synthetic ecoinvent 3.6 Database 2019
Textile - Felt ecoinvent 3.6 Database 2019
Textile - Polyester (PE) ecoinvent 3.6 Database 2019
Packaging - Cardboard Modified ecoinvent 3.6 Database 2019
Plastic - Nylon (PA) Modified ecoinvent 3.6 Database 2019
Plastic - Polyamide Modified ecoinvent 3.6 Database 2019
Plastic - Polypropylene (PP) Modified ecoinvent 3.6 Database 2019
Recycled cardboard Modified ecoinvent 3.6 Database 2019
Textile - Felt Modified ecoinvent 3.6 Database 2019
Textile - Polyester (PE) Modified ecoinvent 3.6 Database 2019
EPD
(EN15804A1) +
Metal - Steel SSAB company 2020
dataset
(EN15804A2)
4 / 13
System boundaries (X=included, MND=module not declared, MNR=module not relevant)
Construction Beyond the system
Product stage Use stage End of life stage
installation stage boundaries
A1 A2 A3 A4 A5 B1 B2 B3 B4 B5 B6 B7 C1 C2 C3 C4 D
X X X X X MND X X X MND MND MND X X X X X
System boundary:
Additional technical information:
waR slairetam tropsnarT gnirutcafunaM tropsnarT ylbmessA e​sU ecnanetniaM riapeR tnemecalpeR tnemhsibrufeR lanoitarepO ygrene esu lanoitarepO esu retaw -eD noitcurtsnoc noitilomed tropsnarT etsaW gnissecorp lasopsiD -yrevoceR-esueR laitnetop-gnilcyceR
5 / 13
LCA: Scenarios and additional technical information
The following information describe the scenarios in the different modules of the EPD.
Capacity utilisation Value
Transport from production place to user (A4) Distance (km) Fuel/Energy Consumption Unit
(incl. return) % (Liter/tonne)
Truck, over 32 tonnes, EURO 6 (km) 53,3 % 1000 0,023 l/tkm 23,00
Assembly (A5) Unit Value
Waste, packaging, cardboard, 100 % recycled, to
kg 2,90
average treatment (kg)
Waste, packaging, corrugated board box, 0 %
kg 1,44
recycled, to average treatment (kg)
Waste, packaging, paper printed, to average
kg 0,03
treatment (kg)
Waste, packaging, plastic film (LDPE), to average
kg 0,26
treatment - A5 (kg)
Maintenance (B2) Unit Value
Electricity, Nordic (kWh) kWh/DU 0,81
Water, tap water (m3) m3/DU 11,70
Repair (B3) Unit Value
Electricity, Nordic (kWh) kWh/DU 0,55
Capacity utilisation Value
Transport to waste processing (C2) Distance (km) Fuel/Energy Consumption Unit
(incl. return) % (Liter/tonne)
Truck, 16-32 tonnes, EURO 6 (km) 36,7 % 100 0,043 l/tkm 4,30
Waste processing (C3) Unit Value
Waste treatment per kg Expanded Polystyrene
kg 0,43
(EPS), incineration - C3 (kg)
Waste treatment per kg Non-hazardous waste,
kg 1,54
incineration with fly ash extraction - C3 (kg)
Waste treatment per kg Plastics, Mixture,
kg 0,58
municipal incineration with fly ash extraction (kg)
Waste treatment per kg Polyethylene, PE,
kg 0,06
incineration with fly ash extraction - C3 (kg)
Waste treatment per kg Polyoxymethylene (POM),
kg 0,38
incineration with fly ash extraction (kg) - CH - C3
Waste treatment per kg Polypropylene (PP),
kg 5,13
incineration with fly ash extraction - C3 (kg)
Waste treatment per kg Polyurethane (PU),
kg 2,03
incineration (kg)
Waste treatment per kg Rubber, municipal
kg 0,11
incineration with fly ash extraction (kg)
Waste treatment per kg Scrap aluminium,
kg 5,62
incineration with fly ash extraction (kg)
Waste treatment per kg Scrap steel, incineration
kg 6,84
with fly ash extraction (kg)
Waste treatment per kg Textile, incineration with
kg 0,57
fly ash extraction (kg)
Waste, materials to recycling (kg) kg 2,90
6 / 13
Disposal (C4) Unit Value
Landfilling of ashes and residues from
kg 5,03
incineration of Scrap aluminium (kg)
Landfilling of ashes and residues from
kg 4,52
incineration of Scrap steel (kg)
Landfilling of ashes from incineration of
expanded polystyrene (EPS), process per kg ashes kg 0,02
and residues - C4 (kg)
Landfilling of ashes from incineration of Non-
hazardous waste, process per kg ashes and kg 0,36
residues - C4 (kg)
Landfilling of ashes from incineration of Plastics,
Mixture, municipal incineration with fly ash
kg 0,02
extraction, process per kg ashes and residues - C4
(kg)
Landfilling of ashes from incineration of
Polyethylene, PE, process per kg ashes and kg 0,00
residues - C4 (kg)
Landfilling of ashes from incineration of
Polyoxymethylene (POM), process per kg ashes kg 0,01
and residues (kg) - CH - C4
Landfilling of ashes from incineration of
Polypropylene, PP, process per kg ashes and kg 0,15
residues - C4 (kg)
Landfilling of ashes from incineration of
Polyurethane (PU), process per kg ashes and kg 0,08
residues - C4 (kg)
Landfilling of ashes from incineration of Rubber,
kg 0,01
process per kg ashes and residues - C4 (kg)
Landfilling of ashes from incineration of Textile,
kg 0,03
soiled, process per kg ashes and residues (kg)
Benefits and loads beyond the system
Unit Value
boundaries (D)
Substitution of electricity, in Norway (MJ) MJ 14,86
Substitution of primary aluminium with net scrap
kg 0,00
(kg)
Substitution of primary steel with net scrap (kg) kg 1,99
Substitution of thermal energy, district heating, in
MJ 224,83
Norway (MJ)
7 / 13
LCA: Results
The LCA results are presented below for the declared unit defined on page 2 of the EPD document.
Environmental impact
Indicator Unit A1-A3 A4 A5 B2 B3
GWP-total kg CO2 -eq 6,57E+01 2,43E+00 7,50E+00 4,16E+00 8,01E-02
GWP-fossil kg CO2 -eq 7,25E+01 2,43E+00 9,15E-02 4,12E+00 7,47E-02
GWP-biogenic kg CO2 -eq -6,85E+00 1,04E-03 7,41E+00 2,72E-02 1,36E-03
GWP-luluc kg CO2 -eq 7,10E-02 7,41E-04 2,50E-05 1,26E-02 4,09E-03
ODP kg CFC11 -eq 4,13E-06 5,87E-07 1,62E-08 3,67E-07 8,08E-09
AP mol H+ -eq 3,46E-01 7,83E-03 3,60E-04 2,39E-02 3,44E-04
EP-FreshWater kg P -eq 3,21E-03 1,94E-05 6,23E-07 3,28E-04 4,94E-06
EP-Marine kg N -eq 7,06E-02 1,72E-03 1,34E-04 3,79E-03 5,44E-05
EP-Terrestial mol N -eq 7,23E-01 1,91E-02 1,29E-03 4,43E-02 7,31E-04
POCP kg NMVOC -eq 2,40E-01 7,51E-03 3,75E-04 1,38E-02 1,71E-04
ADP-minerals&metals1 kg Sb -eq 6,27E-02 4,33E-05 1,83E-06 1,14E-04 1,16E-06
ADP-fossil1 MJ 1,16E+03 3,95E+01 1,07E+00 7,15E+01 2,02E+00
WDP1 m3 5,51E+03 3,03E+01 1,56E+00 1,46E+03 1,56E+02
Indicator Unit B4 C1 C2 C3 C4 D
GWP-total kg CO2 -eq 0 0 4,57E-01 2,71E+01 1,21E-01 -3,54E+00
GWP-fossil kg CO2 -eq 0 0 4,56E-01 2,63E+01 1,21E-01 -3,49E+00
GWP-biogenic kg CO2 -eq 0 0 1,89E-04 8,37E-01 9,03E-05 -3,90E-03
GWP-luluc kg CO2 -eq 0 0 1,62E-04 1,36E-04 3,45E-05 -4,59E-02
ODP kg CFC11 -eq 0 0 1,03E-07 7,41E-08 3,47E-08 -9,50E-02
AP mol H+ -eq 0 0 1,31E-03 8,43E-03 8,07E-04 -2,16E-02
EP-FreshWater kg P -eq 0 0 3,64E-06 7,53E-06 1,25E-06 -2,51E-04
EP-Marine kg N -eq 0 0 2,59E-04 4,34E-03 2,86E-04 -5,76E-03
EP-Terrestial mol N -eq 0 0 2,90E-03 4,33E-02 3,16E-03 -6,10E-02
POCP kg NMVOC -eq 0 0 1,11E-03 1,04E-02 9,09E-04 -2,14E-02
ADP-minerals&metals1 kg Sb -eq 0 0 1,26E-05 3,10E-06 1,93E-06 -5,07E-05
ADP-fossil1 MJ 0 0 6,90E+00 4,86E+00 2,58E+00 -3,71E+01
WDP1 m3 0 0 6,67E+00 2,34E+00 6,11E+00 -1,19E+02
GWP-total = Global Warming Potential total; GWP-fossil = Global Warming Potential fossil fuels; GWP-biogenic = Global Warming Potential biogenic; GWP-luluc =
Global Warming Potential land use and land use change; ODP = Depletion potential of the stratospheric ozone layer; AP = Acidification potential, Accumulated
Exceedance; EP-freshwater = Eutrophication potential, fraction of nutrients reaching freshwater end compartment: EP-marine = Eutrophication potential, fraction of
nutrients reaching marine end compartment; EP-terrestrial = Eutrophication potential, Accumulated Exceedance; POCP = Formation potential of tropospheric ozone;
ADP-minerals&metals = Abiotic depletion potential for non-fossil resources; ADP-fossil = Abiotic depletion for fossil resources potential; WDP = Water (user)
deprivation potential, deprivation-weighted water consumption
"Reading example: 9,0 E-03 = 9,0*10-3 = 0,009"
*INA Indicator Not Assessed
1. The results of this environmental impact indicator shall be used with care as the uncertainties on these results are high or as there is limited experienced with the
indicator
Remarks to environmental impacts
8 / 13
Additional environmental impact indicators
Indicator Unit A1-A3 A4 A5 B2 B3
PM Disease incidence 4,05E-06 2,23E-07 5,40E-09 1,99E-07 1,83E-09
IRP2 kgBq U235 -eq 3,08E+00 1,73E-01 4,62E-03 5,42E-01 4,60E-02
ETP-fw1 CTUe 1,96E+03 2,89E+01 1,40E+00 7,79E+01 2,53E+00
HTP-c1 CTUh 1,13E-07 0,00E+00 4,00E-11 1,12E-08 5,90E-11
HTP-nc1 CTUh 1,44E-06 2,79E-08 1,73E-09 2,49E-07 1,55E-09
SQP1 dimensionless 7,18E+02 4,53E+01 8,13E-01 2,14E+01 1,52E+00
Indicator Unit B4 C1 C2 C3 C4 D
PM Disease incidence 0 0 2,79E-08 5,01E-08 1,45E-08 -8,32E-07
IRP2 kgBq U235 -eq 0 0 3,01E-02 9,98E-03 1,04E-02 -1,11E-01
ETP-fw1 CTUe 0 0 5,11E+00 6,10E+01 1,69E+00 -2,23E+02
HTP-c1 CTUh 0 0 0,00E+00 1,54E-09 5,70E-11 -1,24E-08
HTP-nc1 CTUh 0 0 5,59E-09 4,44E-08 1,82E-09 1,32E-07
SQP1 dimensionless 0 0 4,82E+00 6,93E-01 5,66E+00 -1,26E+02
PM = Particulate Matter emissions; IRP = Ionizing radiation – human health; ETP-fw = Eco toxicity – freshwater; HTP-c = Human toxicity – cancer effects; HTP-nc =
Human toxicity – non cancer effects; SQP = Soil Quality (dimensionless)
"Reading example: 9,0 E-03 = 9,0*10-3 = 0,009"
*INA Indicator Not Assessed
1. The results of this environmental impact indicator shall be used with care as the uncertainties on these results are high or as there is limited experienced with the
indicator
2. This impact category deals mainly with the eventual impact of low dose ionizing radiation on human health of the nuclear fuel cycle. It does not consider effects due
to possible nuclear accidents, occupational exposure nor due to radioactive waste disposal in underground facilities. Potential ionizing radiation from the soil, from
radon and from some construction materials is also not measured by this indicator.
9 / 13
Resource use
Indicator Unit A1-A3 A4 A5 B2 B3
PERE MJ 2,02E+02 4,97E-01 1,84E-02 1,22E+01 1,98E+00
PERM MJ 4,71E+01 0,00E+00 -4,03E+01 0,00E+00 0,00E+00
PERT MJ 2,50E+02 4,97E-01 -4,02E+01 1,22E+01 1,98E+00
PENRE MJ 9,33E+02 3,95E+01 1,07E+00 7,16E+01 2,05E+00
PENRM MJ 3,11E+02 0,00E+00 -1,12E+01 0,00E+00 0,00E+00
PENRT MJ 1,24E+03 3,95E+01 -1,01E+01 7,16E+01 2,05E+00
SM kg 1,28E+01 0,00E+00 0,00E+00 0,00E+00 0,00E+00
RSF MJ 2,15E+00 1,74E-02 5,97E-04 7,76E-01 2,00E-02
NRSF MJ 1,74E+00 5,83E-02 2,37E-03 7,36E-01 0,00E+00
FW m3 1,64E+00 4,50E-03 5,12E-04 1,18E+01 9,03E-03
Indicator Unit B4 C1 C2 C3 C4 D
PERE MJ 0 0 9,87E-02 1,96E-01 5,27E-02 -1,17E+02
PERM MJ 0 0 0,00E+00 0,00E+00 0,00E+00 0,00E+00
PERT MJ 0 0 9,87E-02 1,95E-01 5,27E-02 -1,17E+02
PENRE MJ 0 0 6,90E+00 5,03E+00 2,58E+00 -3,71E+01
PENRM MJ 0 0 0,00E+00 -3,00E+02 0,00E+00 0,00E+00
PENRT MJ 0 0 6,90E+00 -2,95E+02 2,58E+00 -3,71E+01
SM kg 0 0 0,00E+00 0,00E+00 0,00E+00 0,00E+00
RSF MJ 0 0 3,53E-03 4,73E-03 1,38E-03 5,89E-02
NRSF MJ 0 0 1,26E-02 0,00E+00 7,74E-02 -4,52E+00
FW m3 0 0 7,38E-04 1,49E-02 2,33E-03 -1,43E-01
PERE = Use of renewable primary energy excluding renewable primary energy resources used as raw materials; PERM = Use of renewable primary energy resources used
as raw materials; PERT = Total use of renewable primary energy resources; PENRE = Use of non renewable primary energy excluding non-renewable primary energy
resources used as raw materials; PENRM = Use of non renewable primary energy resources used as raw materials; PENRT = Total use of non renewable primary energy
resources; SM = Use of secondary materials; RSF = Use of renewable secondary fuels; NRSF = Use of non-renewable secondary fuels; FW = Net use of fresh water
"Reading example: 9,0 E-03 = 9,0*10-3 = 0,009"
*INA Indicator Not Assessed
10 / 13
End of life - Waste
Indicator Unit A1-A3 A4 A5 B2 B3
HWD kg 9,83E-01 2,16E-03 0,00E+00 1,32E-02 1,89E-04
NHWD kg 1,44E+01 3,43E+00 4,63E+00 8,51E-01 1,25E-02
RWD kg 4,11E-03 2,70E-04 0,00E+00 4,33E-04 2,11E-05
Indicator Unit B4 C1 C2 C3 C4 D
HWD kg 0 0 3,56E-04 0,00E+00 1,01E+01 -1,23E-02
NHWD kg 0 0 3,35E-01 1,54E+00 2,55E-01 -1,34E+00
RWD kg 0 0 4,70E-05 0,00E+00 1,63E-05 -9,16E-05
HWD = Hazardous waste disposed; NHWD = Non-hazardous waste disposed; RWD = Radioactive waste disposed
"Reading example: 9,0 E-03 = 9,0*10-3 = 0,009"
*INA Indicator Not Assessed
End of life - Output flow
Indicator Unit A1-A3 A4 A5 B2 B3
CRU kg 0,00E+00 0,00E+00 0,00E+00 0,00E+00 0,00E+00
MFR kg 3,00E+00 0,00E+00 4,20E+00 0,00E+00 0,00E+00
MER kg 2,75E-01 0,00E+00 1,80E-03 0,00E+00 0,00E+00
EEE MJ 1,79E-01 0,00E+00 2,50E-01 0,00E+00 0,00E+00
EET MJ 2,71E+00 0,00E+00 3,78E+00 0,00E+00 0,00E+00
Indicator Unit B4 C1 C2 C3 C4 D
CRU kg 0 0 0,00E+00 0,00E+00 0,00E+00 0,00E+00
MFR kg 0 0 0,00E+00 2,90E+00 0,00E+00 0,00E+00
MER kg 0 0 0,00E+00 2,33E+01 0,00E+00 0,00E+00
EEE MJ 0 0 0,00E+00 1,42E+01 0,00E+00 0,00E+00
EET MJ 0 0 0,00E+00 2,15E+02 0,00E+00 0,00E+00
CRU = Components for re-use; MFR = Materials for recycling; MER = Materials for energy recovery; EEE = Exported energy electrical; EET = Exported energy thermal
"Reading example: 9,0 E-03 = 9,0*10-3 = 0,009"
*INA Indicator Not Assessed
Biogenic Carbon Content
Indicator Unit At the factory gate
Biogenic carbon content in product kg C 0,00E+00
Biogenic carbon content in accompanying packaging kg C 2,02E+00
Note: 1 kg biogenic carbon is equivalent to 44/12 kg CO2
11 / 13
Additional requirements
Greenhouse gas emissions from the use of electricity in the manufacturing phase
National production mix from import, low voltage (production of transmission lines, in addition to direct emissions and losses in grid) of applied
electricity for the manufacturing process (A3).
Electricity mix Data source Amount Unit
Electricity, Norway, high voltage, hydro power (kWh) ecoinvent 3.6 6,29 g CO2-eq/kWh
Dangerous substances
The product contains no substances given by the REACH Candidate list.
Indoor environment
GREENGUARD Gold certified.
Additional Environmental Information
Key Environmental Indicators
Key environmental indicators Unit A1-A3 A4 A1-C4 A1-D
GWPtotal kg CO2 -eq 65,71 2,43 107,58 104,04
Total energy consumption MJ 1138,99 40,09 1284,54 1126,39
Amount of recycled materials % 45,67
Additional environmental impact indicators required in NPCR Part A for construction products
Indicator Unit A1-A3 A4 A5 B2 B3
GWPIOBC kg CO2 -eq 7,30E+01 2,43E+00 9,16E-02 4,20E+00 1,09E-01
Indicator Unit B4 C1 C2 C3 C4 D
GWPIOBC kg CO2 -eq 0 0 4,57E-01 2,55E+01 1,28E-01 -4,61E+00
GWP-IOBC: Global warming potential calculated according to the principle of instantaneous oxidation. In order to increase the transparency of biogenic carbon
contribution to climate impact, the indicator GWP-IOBC is required as it declares climate impacts calculated according to the principle of instantaneous oxidation.
GWP-IOBC is also referred to as GWP-GHG in context to Swedish public procurement legislation.
Variants and Options
Key environmental indicators (A1-A3) for variants of this EPD
Weight GWPtotal (kg Total energy Amount of recycled
Variants
(kg) CO2 -eq) consumption (MJ) materials (%)
HÅG Tribute 9021 - Upholstered seat & back (Cura/Gabriel) w/o armrests - No
21,76 61,53 934,46 42,88
packaging
HÅG Tribute 9031 - Upholstered seat & back (Cura/Gabriel) including headrest, w/o
22,87 65,81 986,94 43,08
armrests - No packaging
HÅG Tribute 9073 Meeting - Upholstered seat & back (Cura/Gabriel) w/o options -
20,65 59,45 902,83 41,66
No packaging
Key environmental indicators (A1-A3) for options for this EPD
Options
Weight GWPtotal (kg CO2 - Total energy consumption Amount of recycled materials
(kg) eq) (MJ) (%)
HÅG Executive Basic/Meeting armrests (height & width
3,57 20,15 202,23 56,81
adjustment)
HÅG TiltDown armrests (tilt, height & width adjustment) 5,32 18,60 271,32 58,00
Packaging 1 (Small box, fully assembled - used in declared unit) 5,06 -0,10 152,04 57,46
12 / 13
Bibliography
ISO 14025:2010 Environmental labels and declarations - Type III environmental declarations - Principles and procedures.
ISO 14044:2006 Environmental management - Life cycle assessment - Requirements and guidelines.
EN 15804:2012+A2:2019 Environmental product declaration - Core rules for the product category of construction products.
ISO 21930:2017 Sustainability in buildings and civil engineering works - Core rules for environmental product declarations of construction
products.
ecoinvent v3, Allocation, cut-off by classification, Swiss Centre of Life Cycle Inventories.
Iversen et al., (2021) eEPD v2021.09 Background information for EPD generator tool system verification, LCA.no Report number: 07.21
Ruud et al., (2023) EPD generator for NPCR026 Part B for Furniture - Background information for EPD generator application and LCA data,
LCA.no report number 01.23
NPCR Part A: Construction products and services. Ver. 2.0. March 2021, EPD-Norge.
NPCR 026 Part B for Furniture. Ver. 2.0 March 2022, EPD-Norge.
Program operator and publisher Phone: +47 23 08 80 00
The Norwegian EPD Foundation e-mail: post@epd-norge.no
Post Box 5250 Majorstuen, 0303 Oslo, Norway web: www.epd-norge.no
Owner of the declaration: Phone: 0047 98 25 68 30
Flokk AS e-mail: atle.messel@flokk.com
Drammensveien 145,, 0277 Oslo web: https://www.flokk.com
Author of the Life Cycle Assessment Phone: +47 916 50 916
LCA.no AS e-mail: post@lca.no
Dokka 6B, 1671 web: www.lca.no
Developer of EPD generator Phone: +47 916 50 916
LCA.no AS e-mail: post@lca.no
Dokka 6B,1671 Kråkerøy web: www.lca.no
ECO Platform web: www.eco-platform.org
ECO Portal web: ECO Portal
13 / 13
