Environmental product declaration
in accordance with ISO 14025 and EN 15804+A2
Profim Ana
Owner of the declaration: Program operator:
Flokk AS The Norwegian EPD Foundation
Product: Declaration number:
Profim Ana NEPD-7375-6766-EN
Declared unit: Registration number:
1 pcs NEPD-7375-6766-EN
This declaration is based on Product Category Rules: Issue date: 02.09.2024
CEN Standard EN 15804:2012+A2:2019 serves as core
PCR Valid to: 02.09.2029
The Norwegian EPD Foundation NPCR 026:2022 Part B for Furniture EPD software:
LCAno EPD generator ID: 495463
1 / 12
General information
Product Owner of the declaration:
Profim Ana Flokk AS
Contact person: Atle Thiis-Messel
Phone: 0047 98 25 68 30
e-mail: atle.messel@flokk.com
Program operator: Manufacturer:
The Norwegian EPD Foundation Flokk AS
Post Box 5250 Majorstuen, 0303 Oslo, Norway Drammensveien 145,
Phone: +47 977 22 020 0277 Oslo, Norway
web: www.epd-norge.no
Declaration number: Place of production:
NEPD-7375-6766-EN Flokk - Nässjö
Vallgatan 1
571 23 Nässjö, Sweden
This declaration is based on Product Category Rules: Management system:
CEN Standard EN 15804:2012+A2:2019 serves as core PCR ISO 14001, ISO 9001, ISO 50001(Norway, Sweden)
NPCR 026:2022 Part B for Furniture
Statement of liability: Organisation no:
The owner of the declaration shall be liable for the underlying No 928 902 749
information and evidence. EPD Norway shall not be liable with respect
to manufacturer information, life cycle assessment data and
evidences.​
Declared unit: Issue date:
1 pcs Profim Ana 02.09.2024
Declared unit (cradle to gate) with option: Valid to:
A1-A3,A4,A5,B2,B3,B4,C1,C2,C3,C4,D 02.09.2029
Year of study:
2024
Functional unit: Comparability:
1 pcs Profim Ana (4340 with black/graphite recycled plastic shell, EPD of construction products may not be comparable if they not
including packaging. comply with EN 15804 and seen in a building context.
General information on verification of EPD from EPD tools: Development and verification of EPD:
Independent verification of data, other environmental information The declaration is created using EPD tool lca.tools ver EPD2022.03,
and the declaration according to ISO 14025:2010, § 8.1.3 and § 8.1.4. developed by LCA.no. The EPD tool is integrated in the company's
Verification of each EPD is made according to EPD-Norway’s management system, and has been approved by EPD Norway.
guidelines for verification and approval requiring that tools are i
integrated into the company's environmental management system, ii Developer of EPD: Kenneth Dam Lindegaard Knudsen
the procedures for use of the EPD tool are approved by EPD-Norway,
Reviewer of company-specific input data and EPD: Edward Buzura
and iii the process is reviewed annually by an independent third
party verifier. See Appendix G of EPD-Norway's General Programme
Instructions for further information on EPD tools
Verification of EPD tool: Approved:
Independent third party verification of the EPD tool, background data
and test-EPD in accordance with EPDNorway's procedures and
guidelines for verification and approval of EPD tools.
Third party verifier:
Elisabet Amat, GREENIZE projects
(no signature required
2 / 12
Product
Product description:
The Profim Ana family of chairs, designed by the renowned industrial designer Tias Eckhoff, offers a blend of simplicity, ergonomic comfort, and
versatility, making it a popular choice across various environments such as assembly halls, canteens, meeting rooms, and cafeterias. Known for its
seamless integration into any setting, the Ana chair stands out for its functionality and aesthetic appeal.
The Ana series features a polypropylene (PP) shell available in a broad spectrum of colors, including a recycled graphite option, catering to different
design preferences. The frames, made from durable tubular steel, also come in various colors, allowing for further customization. The chairs are
designed to be easily positioned in rows and stacked, enhancing their practicality in spaces where flexibility is key.
Different models within the Ana family cater to varying needs. The standard Ana model can be stacked up to 12 chairs high when unupholstered,
making it an efficient choice for large spaces. The Ana 4340S, with an upholstered seat pad, offers additional comfort and can be stacked up to 10
chairs high. For those requiring even more comfort, the Ana 4340SR includes both seat and backrest upholstery and can be stacked up to 7 chairs
high.
With its simple yet effective design, the Ana chair family combines style with practicality. Its wide range of options, from colors to upholstery,
ensures it meets the diverse needs of any environment. The success of the Ana series across Europe is a testament to its well-thought-out design
and adaptability.
Product specification
The model studied in this declaration is the Profim Ana 4340 Black/Graphite recycled plastic shell variant, including packaging. The model declared
does not include any options.
The key environmental indicators for the other models of the family, and applicable options of the product collection are presented in a table on
page 12 of this declaration.
Recycled
Recycled share in share in
Materials kg %
material (kg) material
(%)
Metal - Steel 1,60 43,94 0,00 0,00
Metal - Steel low alloy 0,40 10,92 0,40 100,00
Plastic - Polyethylene
0,01 0,37 0,00 0,00
(LDPE)
Plastic -
1,63 44,77 1,63 100,00
Polypropylene (PP)
Total 3,65 100,00 2,03
Recycled
Recycled share in share in
Packaging kg %
material (kg) material
(%)
Packaging -
0,49 62,03 0,00 0,00
Cardboard
Recycled cardboard 0,30 37,97 0,30 100,00
Total incl. packaging 4,44 100,00 2,33
Technical data:
Market:
Worldwide.
A4 stage transportation from factory to market, is assumed to be 1.000 km.
See table on page 6 for further detail.
Reference service life, product
15 years
Reference service life, building
LCA: Calculation rules
Declared unit:
1 pcs Profim Ana
Cut-off criteria:
All major raw materials and all the essential energy is included. The production processes for raw materials and energy flows with very small
amounts (less than 1%) are not included. These cut-off criteria do not apply for hazardous materials and substances.
Allocation:
3 / 12
The allocation is made in accordance with the provisions of EN 15804. Incoming energy and water and waste production in-house is allocated
equally among all products through mass allocation. Effects of primary production of recycled materials is allocated to the main product in which
the material was used. The recycling process and transportation of the material is allocated to this analysis.
Data quality:
Specific data for the product composition are provided by the manufacturer. They represent the production of the declared product and were
collected for EPD development in the year of study. Background data is based on registered EPDs according to EN 15804, Ostfold Research
databases, ecoinvent and other LCA databases. The data quality of the raw materials in A1 is presented in the table below.​
Materials Source Data quality Year
Metal - Steel ecoinvent 3.6 Database 2019
Metal - Steel low alloy ecoinvent 3.6 Database 2019
Packaging - Cardboard Modified ecoinvent 3.6 Database 2019
Plastic - Polyethylene (LDPE) ecoinvent 3.6 Database 2019
Plastic - Polypropylene (PP) Modified ecoinvent 3.6 Database 2019
Recycled cardboard Modified ecoinvent 3.6 Database 2019
4 / 12
System boundaries (X=included, MND=module not declared, MNR=module not relevant)
Construction Beyond the system
Product stage Use stage End of life stage
installation stage boundaries
A1 A2 A3 A4 A5 B1 B2 B3 B4 B5 B6 B7 C1 C2 C3 C4 D
X X X X X MND X X X MND MND MND X X X X X
System boundary:
Additional technical information:
waR slairetam tropsnarT gnirutcafunaM tropsnarT ylbmessA e​sU ecnanetniaM riapeR tnemecalpeR tnemhsibrufeR lanoitarepO ygrene esu lanoitarepO esu retaw -eD noitcurtsnoc noitilomed tropsnarT etsaW gnissecorp lasopsiD -yrevoceR-esueR laitnetop-gnilcyceR
5 / 12
LCA: Scenarios and additional technical information
The following information describe the scenarios in the different modules of the EPD.
Capacity utilisation Value
Transport from production place to user (A4) Distance (km) Fuel/Energy Consumption Unit
(incl. return) % (Liter/tonne)
Truck, over 32 tonnes, EURO 6 (km) 53,3 % 1000 0,023 l/tkm 23,00
Assembly (A5) Unit Value
Waste, packaging, cardboard, 100 % recycled, to
kg 0,30
average treatment (kg)
Waste, packaging, corrugated board box, 0 %
kg 0,49
recycled, to average treatment (kg)
Maintenance (B2) Unit Value
Electricity, Nordic (kWh) kWh/DU 0,81
Water, tap water (m3) m3/DU 11,70
Repair (B3) Unit Value
Electricity, Nordic (kWh) kWh/DU 0,55
Capacity utilisation Value
Transport to waste processing (C2) Distance (km) Fuel/Energy Consumption Unit
(incl. return) % (Liter/tonne)
Truck, 16-32 tonnes, EURO 6 (km) 36,7 % 100 0,043 l/tkm 4,30
Waste processing (C3) Unit Value
Waste treatment per kg Polyethylene, PE,
kg 0,01
incineration with fly ash extraction - C3 (kg)
Waste treatment per kg Polypropylene (PP),
kg 1,63
incineration with fly ash extraction - C3 (kg)
Waste treatment per kg Scrap steel, incineration
kg 2,00
with fly ash extraction (kg)
Waste, materials to recycling (kg) kg 0,68
Disposal (C4) Unit Value
Landfilling of ashes and residues from
kg 1,32
incineration of Scrap steel (kg)
Landfilling of ashes from incineration of
Polyethylene, PE, process per kg ashes and kg 0,00
residues - C4 (kg)
Landfilling of ashes from incineration of
Polypropylene, PP, process per kg ashes and kg 0,05
residues - C4 (kg)
Benefits and loads beyond the system
Unit Value
boundaries (D)
Substitution of electricity, in Norway (MJ) MJ 2,69
Substitution of primary steel with net scrap (kg) kg 0,54
Substitution of thermal energy, district heating, in
MJ 40,66
Norway (MJ)
6 / 12
LCA: Results
The LCA results are presented below for the declared unit defined on page 2 of the EPD document.
Environmental impact
Indicator Unit A1-A3 A4 A5 B2 B3
GWP-total kg CO2 -eq 7,70E+00 3,87E-01 1,36E+00 4,16E+00 8,01E-02
GWP-fossil kg CO2 -eq 8,88E+00 3,87E-01 1,28E-02 4,12E+00 7,47E-02
GWP-biogenic kg CO2 -eq -1,19E+00 1,66E-04 1,35E+00 2,72E-02 1,36E-03
GWP-luluc kg CO2 -eq 1,06E-02 1,18E-04 4,24E-06 1,26E-02 4,09E-03
ODP kg CFC11 -eq 7,25E-07 9,32E-08 2,71E-09 3,67E-07 8,08E-09
AP mol H+ -eq 4,38E-02 1,25E-03 6,07E-05 2,39E-02 3,44E-04
EP-FreshWater kg P -eq 5,24E-04 3,08E-06 1,05E-07 3,28E-04 4,94E-06
EP-Marine kg N -eq 9,16E-03 2,73E-04 2,01E-05 3,79E-03 5,44E-05
EP-Terrestial mol N -eq 1,01E-01 3,04E-03 2,17E-04 4,43E-02 7,31E-04
POCP kg NMVOC -eq 3,56E-02 1,19E-03 6,25E-05 1,38E-02 1,71E-04
ADP-minerals&metals1 kg Sb-eq 1,35E-04 6,89E-06 3,12E-07 1,14E-04 1,16E-06
ADP-fossil1 MJ 1,17E+02 6,28E+00 1,79E-01 7,15E+01 2,02E+00
WDP1 m3 6,46E+03 4,82E+00 2,27E-01 1,46E+03 1,56E+02
Indicator Unit B4 C1 C2 C3 C4 D
GWP-total kg CO2 -eq 0 0 7,26E-02 4,22E+00 1,69E-02 -8,44E-01
GWP-fossil kg CO2 -eq 0 0 7,25E-02 4,22E+00 1,69E-02 -8,35E-01
GWP-biogenic kg CO2 -eq 0 0 3,00E-05 2,32E-04 1,22E-05 -8,17E-04
GWP-luluc kg CO2 -eq 0 0 2,58E-05 8,03E-06 4,80E-06 -8,39E-03
ODP kg CFC11 -eq 0 0 1,64E-08 4,20E-09 4,82E-09 -1,72E-02
AP mol H+ -eq 0 0 2,08E-04 5,99E-04 1,12E-04 -4,92E-03
EP-FreshWater kg P -eq 0 0 5,79E-07 6,67E-07 1,76E-07 -5,78E-05
EP-Marine kg N -eq 0 0 4,12E-05 2,79E-04 3,97E-05 -1,25E-03
EP-Terrestial mol N -eq 0 0 4,61E-04 3,02E-03 4,40E-04 -1,32E-02
POCP kg NMVOC -eq 0 0 1,77E-04 7,46E-04 1,26E-04 -4,89E-03
ADP-minerals&metals1 kg Sb-eq 0 0 2,00E-06 2,18E-07 2,68E-07 -1,27E-05
ADP-fossil1 MJ 0 0 1,10E+00 3,81E-01 3,59E-01 -8,41E+00
WDP1 m3 0 0 1,06E+00 1,00E+00 8,66E-01 -1,09E+01
GWP-total = Global Warming Potential total; GWP-fossil = Global Warming Potential fossil fuels; GWP-biogenic = Global Warming Potential biogenic; GWP-luluc =
Global Warming Potential land use and land use change; ODP = Depletion potential of the stratospheric ozone layer; AP = Acidification potential, Accumulated
Exceedance; EP-freshwater = Eutrophication potential, fraction of nutrients reaching freshwater end compartment: EP-marine = Eutrophication potential, fraction of
nutrients reaching marine end compartment; EP-terrestrial = Eutrophication potential, Accumulated Exceedance; POCP = Formation potential of tropospheric ozone;
ADP-minerals&metals = Abiotic depletion potential for non-fossil resources; ADP-fossil = Abiotic depletion for fossil resources potential; WDP = Water (user)
deprivation potential, deprivation-weighted water consumption
"Reading example: 9,0 E-03 = 9,0*10-3 = 0,009"
*INA Indicator Not Assessed
1. The results of this environmental impact indicator shall be used with care as the uncertainties on these results are high or as there is limited experienced with the
indicator
Remarks to environmental impacts
7 / 12
Additional environmental impact indicators
Indicator Unit A1-A3 A4 A5 B2 B3
PM Disease incidence 7,78E-07 3,55E-08 8,96E-10 1,99E-07 1,83E-09
IRP2 kgBq U235 -eq 5,75E-01 2,75E-02 7,68E-04 5,42E-01 4,60E-02
ETP-fw1 CTUe 3,83E+02 4,59E+00 2,39E-01 7,79E+01 2,53E+00
HTP-c1 CTUh 4,00E-08 0,00E+00 8,00E-12 1,12E-08 5,90E-11
HTP-nc1 CTUh 3,38E-07 4,44E-09 3,00E-10 2,49E-07 1,55E-09
SQP1 dimensionless 2,01E+02 7,20E+00 1,20E-01 2,14E+01 1,52E+00
Indicator Unit B4 C1 C2 C3 C4 D
PM Disease incidence 0 0 4,44E-09 5,94E-09 2,01E-09 -1,67E-07
IRP2 kgBq U235 -eq 0 0 4,79E-03 7,76E-04 1,45E-03 -1,94E-02
ETP-fw1 CTUe 0 0 8,13E-01 1,61E+00 2,35E-01 -5,17E+01
HTP-c1 CTUh 0 0 0,00E+00 1,91E-10 8,00E-12 -3,22E-09
HTP-nc1 CTUh 0 0 8,88E-10 4,05E-09 2,54E-10 4,51E-08
SQP1 dimensionless 0 0 7,67E-01 6,00E-02 7,90E-01 -2,29E+01
PM = Particulate Matter emissions; IRP = Ionizing radiation – human health; ETP-fw = Eco toxicity – freshwater; HTP-c = Human toxicity – cancer effects; HTP-nc =
Human toxicity – non cancer effects; SQP = Soil Quality (dimensionless)
"Reading example: 9,0 E-03 = 9,0*10-3 = 0,009"
*INA Indicator Not Assessed
1. The results of this environmental impact indicator shall be used with care as the uncertainties on these results are high or as there is limited experienced with the
indicator
2. This impact category deals mainly with the eventual impact of low dose ionizing radiation on human health of the nuclear fuel cycle. It does not consider effects due
to possible nuclear accidents, occupational exposure nor due to radioactive waste disposal in underground facilities. Potential ionizing radiation from the soil, from
radon and from some construction materials is also not measured by this indicator.
8 / 12
Resource use
Indicator Unit A1-A3 A4 A5 B2 B3
PERE MJ 6,31E+01 7,90E-02 2,95E-03 1,22E+01 1,98E+00
PERM MJ 9,59E+00 0,00E+00 -9,59E+00 0,00E+00 0,00E+00
PERT MJ 7,27E+01 7,90E-02 -9,59E+00 1,22E+01 1,98E+00
PENRE MJ 1,01E+02 6,28E+00 1,79E-01 7,16E+01 2,05E+00
PENRM MJ 5,42E+01 0,00E+00 0,00E+00 0,00E+00 0,00E+00
PENRT MJ 1,55E+02 6,28E+00 1,79E-01 7,16E+01 2,05E+00
SM kg 2,33E+00 0,00E+00 0,00E+00 0,00E+00 0,00E+00
RSF MJ 4,45E-01 2,76E-03 9,80E-05 7,76E-01 2,00E-02
NRSF MJ 1,24E-01 9,26E-03 4,04E-04 7,36E-01 0,00E+00
FW m3 9,76E-02 7,15E-04 8,47E-05 1,18E+01 9,03E-03
Indicator Unit B4 C1 C2 C3 C4 D
PERE MJ 0 0 1,57E-02 1,34E-02 7,41E-03 -2,12E+01
PERM MJ 0 0 0,00E+00 0,00E+00 0,00E+00 0,00E+00
PERT MJ 0 0 1,57E-02 1,34E-02 7,41E-03 -2,12E+01
PENRE MJ 0 0 1,10E+00 3,81E-01 3,59E-01 -8,41E+00
PENRM MJ 0 0 0,00E+00 -5,42E+01 0,00E+00 0,00E+00
PENRT MJ 0 0 1,10E+00 -5,38E+01 3,59E-01 -8,41E+00
SM kg 0 0 0,00E+00 0,00E+00 0,00E+00 0,00E+00
RSF MJ 0 0 5,62E-04 3,30E-04 1,94E-04 1,80E-02
NRSF MJ 0 0 2,01E-03 0,00E+00 1,34E-02 -6,05E-01
FW m3 0 0 1,17E-04 8,86E-04 3,23E-04 -2,63E-02
PERE = Use of renewable primary energy excluding renewable primary energy resources used as raw materials; PERM = Use of renewable primary energy resources used
as raw materials; PERT = Total use of renewable primary energy resources; PENRE = Use of non renewable primary energy excluding non-renewable primary energy
resources used as raw materials; PENRM = Use of non renewable primary energy resources used as raw materials; PENRT = Total use of non renewable primary energy
resources; SM = Use of secondary materials; RSF = Use of renewable secondary fuels; NRSF = Use of non-renewable secondary fuels; FW = Net use of fresh water
"Reading example: 9,0 E-03 = 9,0*10-3 = 0,009"
*INA Indicator Not Assessed
9 / 12
End of life - Waste
Indicator Unit A1-A3 A4 A5 B2 B3
HWD kg 1,31E-01 3,44E-04 0,00E+00 1,32E-02 1,89E-04
NHWD kg 2,59E+00 5,46E-01 7,93E-01 8,51E-01 1,25E-02
RWD kg 5,01E-04 4,29E-05 0,00E+00 4,33E-04 2,11E-05
Indicator Unit B4 C1 C2 C3 C4 D
HWD kg 0 0 5,66E-05 0,00E+00 1,36E+00 -3,27E-03
NHWD kg 0 0 5,33E-02 0,00E+00 3,02E-02 -3,24E-01
RWD kg 0 0 7,47E-06 0,00E+00 2,20E-06 -1,60E-05
HWD = Hazardous waste disposed; NHWD = Non-hazardous waste disposed; RWD = Radioactive waste disposed
"Reading example: 9,0 E-03 = 9,0*10-3 = 0,009"
*INA Indicator Not Assessed
End of life - Output flow
Indicator Unit A1-A3 A4 A5 B2 B3
CRU kg 0,00E+00 0,00E+00 0,00E+00 0,00E+00 0,00E+00
MFR kg 5,32E-01 0,00E+00 7,37E-01 0,00E+00 0,00E+00
MER kg 4,25E-01 0,00E+00 1,08E-06 0,00E+00 0,00E+00
EEE MJ 2,82E-01 0,00E+00 4,53E-02 0,00E+00 0,00E+00
EET MJ 4,26E+00 0,00E+00 6,86E-01 0,00E+00 0,00E+00
Indicator Unit B4 C1 C2 C3 C4 D
CRU kg 0 0 0,00E+00 0,00E+00 0,00E+00 0,00E+00
MFR kg 0 0 0,00E+00 6,80E-01 0,00E+00 0,00E+00
MER kg 0 0 0,00E+00 3,65E+00 0,00E+00 0,00E+00
EEE MJ 0 0 0,00E+00 2,74E+00 0,00E+00 0,00E+00
EET MJ 0 0 0,00E+00 4,15E+01 0,00E+00 0,00E+00
CRU = Components for re-use; MFR = Materials for recycling; MER = Materials for energy recovery; EEE = Exported energy electrical; EET = Exported energy thermal
"Reading example: 9,0 E-03 = 9,0*10-3 = 0,009"
*INA Indicator Not Assessed
Biogenic Carbon Content
Indicator Unit At the factory gate
Biogenic carbon content in product kg C 0,00E+00
Biogenic carbon content in accompanying packaging kg C 3,67E-01
Note: 1 kg biogenic carbon is equivalent to 44/12 kg CO2
10 / 12
Additional requirements
Greenhouse gas emissions from the use of electricity in the manufacturing phase
National production mix from import, low voltage (production of transmission lines, in addition to direct emissions and losses in grid) of applied
electricity for the manufacturing process (A3).
Electricity mix Source Amount Unit
Electricity, high voltage, hydro (kWh) - SE ecoinvent 3.6 4,02 g CO2-eq/kWh
Dangerous substances
The product contains no substances given by the REACH Candidate list.
Indoor environment
Additional Environmental Information
Key Environmental Indicators
Key environmental indicators Unit A1-A3 A4 A1-C4 A1-D
GWPtotal kg CO2 -eq 7,70 0,39 17,99 17,15
Total energy consumption MJ 164,97 6,37 262,83 232,60
Amount of recycled materials % 52,53
Additional environmental impact indicators required in NPCR Part A for construction products
Indicator Unit A1-A3 A4 A5 B2 B3
GWPIOBC kg CO2 -eq 1,10E+01 3,87E-01 1,28E-02 4,20E+00 1,09E-01
Indicator Unit B4 C1 C2 C3 C4 D
GWPIOBC kg CO2 -eq 0 0 7,26E-02 4,22E+00 1,70E-02 -1,14E+00
GWP-IOBC: Global warming potential calculated according to the principle of instantaneous oxidation. In order to increase the transparency of biogenic carbon
contribution to climate impact, the indicator GWP-IOBC is required as it declares climate impacts calculated according to the principle of instantaneous oxidation.
GWP-IOBC is also referred to as GWP-GHG in context to Swedish public procurement legislation.
Variants and Options
Key environmental indicators (A1-A3) for variants of this EPD
Variants
Weight GWPtotal (kg CO2 Total energy Amount of recycled
(kg) -eq) consumption (MJ) materials (%)
Ana (4340) - Un-upholstered virgin plastic shell - No packaging 3,67 10,57 206,99 10,86
Ana (4340S) - Upholstered seat, virgin plastic shell (Cura/Gabriel) - No
4,32 13,75 247,54 12,69
packaging
Ana (4340SR) - Upholstered seat/back, virgin plastic shell (Cura/Gabriel) - No
4,97 16,91 287,80 13,99
packaging
Ana (4340) - Un-upholstered recycled black plastic seat/back (Cura/Gabriel) -
3,65 8,28 141,29 55,69
No packaging
Ana (4340S) - Upholstered seat, black recycled plastic shell (Cura/Gabriel) - No
4,31 11,46 181,84 50,70
packaging
Ana (4340SR) - Upholstered seat/back, black recycled plastic shell
5,00 14,62 222,10 47,03
(Cura/Gabriel) - No packaging
Key environmental indicators (A1-A3) for options for this EPD
Options
Weight GWPtotal (kg CO2 - Total energy consumption Amount of recycled materials
(kg) eq) (MJ) (%)
Profim Ana Linking device 0,02 0,05 0,61 20,00
Chair Trolley 6,87 25,58 311,52 0,00
Packaging (large box, fully assembled, fits 1-4 chairs - used in
0,79 -0,58 23,68 37,97
declared unit)
11 / 12
Bibliography
ISO 14025:2010 Environmental labels and declarations - Type III environmental declarations - Principles and procedures.
ISO 14044:2006 Environmental management - Life cycle assessment - Requirements and guidelines.
EN 15804:2012+A2:2019 Environmental product declaration - Core rules for the product category of construction products.
ISO 21930:2017 Sustainability in buildings and civil engineering works - Core rules for environmental product declarations of construction
products.
ecoinvent v3, Allocation, cut-off by classification, Swiss Centre of Life Cycle Inventories.
Iversen et al., (2021) eEPD v2021.09 Background information for EPD generator tool system verification, LCA.no Report number: 07.21
Ruud et al., (2023) EPD generator for NPCR026 Part B for Furniture - Background information for EPD generator application and LCA data,
LCA.no report number 01.23
NPCR Part A: Construction products and services. Ver. 2.0. March 2021, EPD-Norge.
NPCR 026 Part B for Furniture. Ver. 2.0 March 2022, EPD-Norge.
Program operator and publisher Phone: +47 977 22 020
The Norwegian EPD Foundation e-mail: post@epd-norge.no
Post Box 5250 Majorstuen, 0303 Oslo, Norway web: www.epd-norge.no
Owner of the declaration: Phone: 0047 98 25 68 30
Flokk AS e-mail: atle.messel@flokk.com
Drammensveien 145,, 0277 Oslo web: https://www.flokk.com
Author of the Life Cycle Assessment Phone: +47 916 50 916
LCA.no AS e-mail: post@lca.no
Dokka 6A, 1671 Kråkerøy web: www.lca.no
Developer of EPD generator Phone: +47 916 50 916
LCA.no AS e-mail: post@lca.no
Dokka 6A, 1671 Kråkerøy web: www.lca.no
ECO Platform web: www.eco-platform.org
ECO Portal web: ECO Portal
12 / 12
