ver1 2015
ENVIRONMENTAL PRODUCT DECLARATION
in accordance with ISO 14025, ISO 21930 and EN 15804
Owner of the declaration: Saint-Gobain Sweden AB, Scanspac
Program operator: The Norwegian EPD Foundation
Publisher: The Norwegian EPD Foundation
Declaration number: NEPD-3387-2007-EN
Registration number: NEPD-3387-2007-EN
ECO Platform reference number: -
Issue date: 07.03.2022
Valid to: 07.03.2027
Dalapro Hydro
Saint-Gobain Sweden AB, Scanspac
www.epd-norge.no
NEPD-3387-2007-EN Dalapro Hydro
1 / 8
General information
Product: Owner of the declaration:
Dalapro Hydro Saint-Gobain Sweden AB, Scanspac
Contact person: Christian Nilsson
Phone: +46 (0)19-46 34 00
e-mail: ehs.scanspac@dalapro.com
Program operator: Manufacturer:
Saint-Gobain Sweden AB, Scanspac
The Norwegian EPD Foundation
Pb. 5250 Majorstuen, 0303 Oslo
Phone: +47 23 08 80 00
e-mail: post@epd-norge.no
Declaration number: Place of production:
Saint-Gobain Sweden AB, Scanspac
NEPD-3387-2007-EN Kemivägen 7 SE-705 97 Glanshammar
Sweden
ECO Platform reference number: Management system:
ISO 9001, ISO 14001
This declaration is based on Product Category Rules: Organisation no:
556241-2592
CEN Standard EN 15804:2012+A1:2013 serves as core PCR.
NPCR 009:2018 Part B for Technical - Chemical products in the building and
construction industry
Statement of liability: Issue date: 07.03.2022
The owner of the declaration shall be liable for the underlying information and
evidence. EPD Norway shall not be liable with respect to manufacturer Valid to: 07.03.2027
information, life cycle assessment data and evidences.
Declared unit: Year of study:
1 kg Dalapro Hydro 2020
Declared unit with option: Comparability:
EPD of construction products may not be comparable if they not comply with EN
A1,A2,A3,A4
15804 and seen in a building context.
Functional unit: Development and verification of EPD:
The declaration has been developed and verified using EPD tool lca.tools
ver EPD2020.11, developed by LCA.no AS. The EPD tool is integrated into
the company's environmental management system, and has been
approved by EPD-Norway
General information on verification of EPD from EPD tools:
Independent verification of data, other environmental information and Developer of EPD:
the declaration according to ISO 14025:2010, § 8.1.3 and § 8.1.4. Individual
third party verification of each EPD is not required when the EPD tool is i) Ellinor Johansson
integrated into the company's environmental management system, ii) the
procedures for use of the EPD tool are approved by EPDNorway, and iii) Reviewer of company-specific input data and EPD:
the proccess is reviewed annualy. See Appendix G of EPD-Norway's
General Programme Instructions for further information on EPD tools. Christian Borgenfalk
Verification of EPD tool: Approved:
Independent third party verification of the EPD tool, background data
Sign
and test-EPD in accordance with EPDNorway's procedures and guidelines
for verification and approval of EPD tools.
Anne Rønning, Norsus AS
(no signature required) Håkon Hauan, CEO EPD-Norge
NEPD-3387-2007-EN Dalapro Hydro
2 / 8
Product
Product description: Technical data:
Dalapro Hydro is a ready-mixed hand filler for use in wet rooms or TECHNICAL DATA
where an extra durable surface is desired. A high binder content in the Binding agent: Latex co-polymer
filler gives the product a hard, water repellent surface, and maximum Solvent: Water
adhesion to the substrate. The product is suitable for joint filling and Grain size: Max. 0.2 mm
thin smoothing. Suitable for most substrates in new construction and pH: Approx. 9
renovation. Colour: Blue
Blue color.
Market:
Nordic Ecolabelled.
Europe
Product specification
Reference service life, product
Packaging:
Filler has a limited shelf life and is date-marked. Unopened packaging can be
Dalapro Hydro: 10 litre bucket, 3 litre bucket and 400 ml tube.
kept in a dark place, free
10 litre and 3 litre bucket is packaged in a bucket manufactured in 100
from frost, for up to 12 months. Containers that have been opened must be
% recyclable plastic and consists of at least 90 % recycled plastic.
sealed well.
All calculations in this EPD is made with the recycled 10 litre bucket. It
represent the majority of the market. Reference service life, building
Materials % Not included in the declaration.
Water 30-50
Filler-dolomite 30-50
Filler-cenospheres 2,5-10
Filler-perlite 2,5-10
Thickener 1-5
Additive 1-3
Packaging
Pallet
Binder 2,5-10
LCA: Calculation rules
Declared unit: Allocation:
The allocation is made in accordance with the provisions of EN 15804.
1 kg Dalapro Hydro
Incoming energy and water and waste production in-house is allocated
Cut-off criteria: equally among all products through mass allocation. Effects of primary
production of recycled materials is allocated to the main product in which
All major raw materials and all the essential energy is included. The
the material was used. The recycling process and transportation of the
production processes for raw materials and energy flows with very small
material is allocated to this analysis.
amounts (less than 1%) are not included. These cut-off criteria do not
apply for hazardous materials and substances.
Data quality:
Specific data for the product composition are provided by the manufacturer. They represent the production of the declared product and were collected for
EPD development in the year of study. Background data is based on registered EPDs according to EN 15804, Ostfold Research databases, ecoinvent and other
LCA databases. The data quality of the raw materials in A1 is presented in the table below.
Materials Source Data quality Year
Chemicals Chemicals below cut-off No data 0
Additives ecoinvent 3.4 Database 2017
Binder ecoinvent 3.4 Database 2017
Filler ecoinvent 3.4 Database 2017
Packaging ecoinvent 3.4 Database 2017
Water ecoinvent 3.4 Database 2017
Packaging Modified ecoinvent 3.4 Database 2017
Filler LCA.no Database 2018
Cellulose Ether ecoinvent 3.4 Database 2019
Packaging Supplier Specific 2020
NEPD-3387-2007-EN Dalapro Hydro
3 / 8
System boundary:
The flowchart shows the system boundaries A1-A4.
All calculations in this EPD is made with the recycled 10 litre bucket. It represent the majority of the market.
Additional technical information:
Suitable for embedding paper tape. Combined with Certain-Teed Marco Joint Tape, the product is suitable for
joint filling on plasterboard. Meets CE-marking requirements in accordance with EN 13963. Manufactured in
accordance with ISO 9001 and ISO 14001. When finishing plasterboard: follow recommendations in accordance with
EN 13963 or National guidlines for finishing plasterboards.
NEPD-3387-2007-EN Dalapro Hydro
4 / 8
LCA: Scenarios and additional technical information
The following information describe the scenarios in the different modules of the EPD.
Transport from production place to user (A4)
Capacity utilisation Fuel/Energy
Type Type of vehicle Distance km Unit Value (l/t)
(incl. return) % consumption
Truck 55,0 % Truck, lorry over 32 tonnes, EURO 6 300 0,022606 l/tkm 6,78
Railway l/tkm
Boat l/tkm
Other Transportation l/tkm
NEPD-3387-2007-EN Dalapro Hydro
5 / 8
LCA: Results
The LCA results are presented below for the declared unit defined on page 2 of the EPD document.
System boundaries (X=included, MND=module not declared, MNR=module not relevant)
Construction Beyond the
Product stage installation User stage End of life stage . system
stage bondaries
A1 A2 A3 A4 A5 B1 B2 B3 B4 B5 B6 B7 C1 C2 C3 C4 . D
X X X X .
Environmental impact
Parameter Unit A1-A3 A4
GWP kg CO 2 -eq 3,13E-01 2,48E-02
ODP kg CFC11 -eq 3,49E-08 5,10E-09
POCP kg C 2H 4-eq 9,54E-05 3,88E-06
AP kg SO 2 -eq 1,20E-03 6,41E-05
EP kg PO 3- -eq 3,47E-04 8,84E-06
4
ADPM kg Sb -eq 7,99E-07 5,91E-08
ADPE MJ 9,81E+00 4,08E-01
GWP Global warming potential; ODP Depletion potential of the stratospheric ozone layer; POCP Formation potential of tropospheric photochemical oxidants;
AP Acidification potential of land and water; EP Eutrophication potential; ADPM Abiotic depletion potential for non fossil resources; ADPE Abiotic depletion
potential for fossil resources
"Reading example: 9,0 E-03 = 9,0*10-3 = 0,009"
*INA Indicator Not Assessed
waR slairetam tropsnarT gnirutcafunaM tropsnarT ylbmessA esU ecnanetniaM riapeR tnemecalpeR tnemhsibrufeR lanoitarepO ygrene esu lanoitarepO esu
retaw
-eD noitcurtsnoc noitilomed tropsnarT etsaW gnissecorp lasopsiD -yrevoceR-esueR -gnilcyceR laitnetop
NEPD-3387-2007-EN Dalapro Hydro
6 / 8
Resource use
Parameter Unit A1-A3 A4
RPEE MJ 1,97E+00 7,41E-03
RPEM MJ 8,97E-01 0,00E+00
TPE MJ 2,87E+00 7,41E-03
NRPE MJ 8,18E+00 4,20E-01
NRPM MJ 2,67E+00 0,00E+00
TRPE MJ 1,09E+01 4,20E-01
SM kg 4,53E-02 0,00E+00
RSF MJ 0,00E+00 0,00E+00
NRSF MJ 0,00E+00 0,00E+00
W m3 7,95E-03 9,95E-05
RPEE Renewable primary energy resources used as energy carrier; RPEM Renewable primary energy resources used as raw materials; TPE Total use of renewable
primary energy resources; NRPE Non renewable primary energy resources used as energy carrier; NRPM Non renewable primary energy resources used as
materials; TRPE Total use of non renewable primary energy resources; SM Use of secondary materials; RSF Use of renewable secondary fuels; NRSF Use of non
renewable secondary fuels; W Use of net fresh water
"Reading example: 9,0 E-03 = 9,0*10-3 = 0,009"
*INA Indicator Not Assessed
End of life - Waste
Parameter Unit A1-A3 A4
HW kg 3,72E-03 2,24E-07
NHW kg 1,36E-01 3,84E-02
RW kg INA* INA*
HW Hazardous waste disposed; NHW Non hazardous waste disposed; RW Radioactive waste disposed
"Reading example: 9,0 E-03 = 9,0*10-3 = 0,009"
*INA Indicator Not Assessed
End of life - Output flow
Parameter Unit A1-A3 A4
CR kg 0,00E+00 0,00E+00
MR kg 8,00E-04 0,00E+00
MER kg 4,73E-03 0,00E+00
EEE MJ INA* INA*
ETE MJ INA* INA*
CR Components for reuse; MR Materials for recycling; MER Materials for energy recovery; EEE Exported electric energy; ETE Exported thermal energy
"Reading example: 9,0 E-03 = 9,0*10-3 = 0,009"
*INA Indicator Not Assessed
NEPD-3387-2007-EN Dalapro Hydro
7 / 8
Additional Norwegian requirements
Greenhouse gas emissions from the use of electricity in the manufacturing phase
National production mix from import, low voltage (production of transmission lines, in addition to direct emissions and losses in grid) of applied electricity for
the manufacturing process (A3).
Electricity mix Data source Amount Unit
Renewable electricity with Guarantee of Origin from LOS (kWh) Modified ecoinvent 3.4 60,20 g CO2-ekv/kWh
Dangerous substances
The product contains no substances given by the REACH Candidate list or the Norwegian priority list.
Indoor environment
Bibliography
ISO 14025:2010 Environmental labels and declarations - Type III environmental declarations - Principles and procedures.
ISO 14044:2006 Environmental management - Life cycle assessment - Requirements and guidelines.
EN 15804:2012+A1:2013 Environmental product declaration - Core rules for the product category of construction products.
ISO 21930:2017 Sustainability in buildings and civil engineering works. Core rules for environmental product declarations of construction products.
ecoinvent v3, Allocation, cut-off by classification, Swiss Centre of Life Cycle Inventories.
Iversen et al., (2018) eEPD v3.0 - Background information for EPD generator system, LCA.no report number 04.18
Iversen et al., (2019) EPD generator for Saint-Gobain Weber and Scanspac - Background information and LCA data, LCA.no report number 05.18
NPCR Part A: Construction products and services. Ver. 1.0. April 2017, EPD-Norge.
NPCR 009 Part B for technical-chemical products. Ver. 1.0 June 2018, EPD-Norge.
Program operator and publisher Phone: +47 23 08 80 00
The Norwegian EPD Foundation e-mail: post@epd-norge.no
Post Box 5250 Majorstuen, 0303 Oslo,Norway web: www.epd-norge.no
Owner of the declaration Phone: +46 (0)19-46 34 00
Saint-Gobain Sweden AB, Scanspac e-mail: ehs.scanspac@dalapro.com
Kemivägen 7 SE-705 97 Glanshammar web: www.dalapro.se
Author of the Life Cycle Assessment Phone: +47 916 50 916
LCA.no AS e-mail: post@lca.no
Dokka 1C 1671 Kråkerøy web: www.lca.no
Developer of EPD generator Phone: +47 916 50 916
LCA.no AS e-mail: post@lca.no
Dokka 1C,1671 Kråkerøy web: www.lca.no
NEPD-3387-2007-EN Dalapro Hydro
8 / 8
