Environmental Product
Declaration
In accordance with ISO 14025 and EN 15804 +A1
Kvillsfors inward opening windows – KS, KN, KU, ES, EN, EU
(with aluminium cladding)
Owner of the declaration:
NorDan AS Product name:
Program holder and publisher: Kvillsfors inward opening
windows – KS, KN, KU, ES, EN,
EU (with aluminium cladding)
The Norwegian EPD foundation
Declaration number:
Manufacturer:
NEPD-3448-2059-EN NorDan AS
Registration Number:
NEPD-3448-2059-EN
Issue date:
Valid to:
02.05.2022
The Norwegian 02.05.2027
EPD Foundation
General information
Product: Owner of the declaration:
Kvillsfors inward opening windows – KS, KN, KU, ES, EN, EU NorDan AS
(with aluminium cladding) Kontaktperson: Fredrik Jonsson
Tlf: +46 (0) 10-130 01 78
e-post: fredrik.jonsson@nordan.se
Program holder: Manufacturer:
The Norwegian EPD Foundation
Post Box 5250 Majorstuen, 0303 Oslo NorDan AB
Tlf: +47 977 22 020 Grebbestadsvägen 8 457 91 Tanumshede
e-mail: post@epd-norge.no
Phone: +46 (0)10 - 130 00 00
Declaration number: Place of production:
NEPD-3448-2059-EN Kvillsfors, Sweden
ECO Platform registration number: Management system:
This declaration is based on Product Category Rules: NorDan AB. Works with EN ISO 9001:2015, ISO 14001:2015
CEN Standard EN 15804 serves as core PCR NPCR014:2019
version 3.0 Part B for Windows and doors Org. no.:
NO 979 776 233 MVA
Declaration of responsibility: Issue date:
The owner of the declaration shall be responsible for the 02.05.2022
underlying information and evidence. EPD Norway shall not be
responsible with regard to manufacturer information, life cycle
data and evidence.
Valid to:
02.05.2027
Declared unit: Year of study:
2021
Declared unit with option: Comparability:
EPD of construction products may not be comparable if they
are not comply with NS-EN 15804 and seen in a building
context.
Functional unit:
1 window measuring 1.23 m x 1.48 m (reference window based on
EN 14351-1) with an expected service life of 60 yrs. with an The EPD has been worked out by:
essential parameter U-value = 1,0 - 1,2 W/m2K. Conversion factor Roja Modaresi
is 70.28 [Kg/FU]. Norsk Treteknisk Institutt
Verification:
Independent verification of the declaration and data,
according to ISO14025:2010
internal external
Approved
Third party verifier:
Gaylord K. Booto PhD., Senior Research Scientist, NORSUS AS
(Independent verifier approved by EPD Norway)
NEPD-3448-2059-EN Kvillsfors inward opening windows – KS, KN, KU, ES, EN, EU (with aluminium cladding)
2/9
Product
Product description: Technical data:
Inward opening windows for use in exterior walls of domestic and Inward opening windows. Triple glazed or double glazed with
commercial buildings. secondary sash, 115mm frame with aluminium clad. Uwin 1,0
-1,2 W/m2K. Manufactured in accordance with ISO
9001:2015 and ISO14001:2015. Certified: Bluesky, SP Sitac
Product specification: “P”,
25% of aluminium and 7% of glass is produced from recycled
material. The total product weight is 70.28 kg. The packaging has an
Product group KS, KN, KU, ES, EN, EU is covered in this EPD. average weight of 4.6 kg.
The highest amount for constituent material has been used.
Materialer kg %
Pine timber 17.79 25.31 Market:
Glue for timber 0.13 0.19
Glass 39.99 56.90 Europe, but scenarios beyond cradle to gate are based
Spacer 0.46 0.65 on the situation in the Norwegian market.
Triple glazed Butyl 0.02 0.03
unit Sealant 0.51 0.73
Absorbent 0.02 0.03
Argon 0.03 0.05
Paint 1.04 1.48 Reference service life:
Aluminium 5.86 8.34 The reference service life is 60 years for aluminium cladding
Plastic 0.04 0.05 timber frame
Gasket 1.09 1.55
Metal 2.91 4.14
Glue 0.04 0.05
Glass list 0.35 0.50
Total weight of the product 70.28 100
Wood packaging 0.35
Steel packaging 0.03
Plastic packaging 0.15
cardboard packaging 0,4
Recycled pallete EU 1200*800 3.70
Total weight with packaging 74.51
LCA: Calculation rules
Functional unit: System boundary:
1 window measuring 1.23 m x 1.48 m (reference window based on EN All modules are included. Below is a technical flowchart for
14351-1) with an expected service life of 60 yrs. with an essential the production line at Nordan. Modul D is calculated with
parameter U-value = 1,0 - 1,2 W/m2K. Conversion factor is 70.28 energy substitution and explained in the scenarios.
[Kg/FU].
NEPD-3448-2059-EN Kvillsfors inward opening windows – KS, KN, KU, ES, EN, EU (with aluminium cladding)
3/9
Data quality Cut-off criteria:
Data is representative of year 2020 and was collected in 2021-2022. All raw materails and energy use is included. Where data was
Data is taken from processes from Ecoinvent 3.1-3.7. Some available for infrastructure from Ecoinvent, it is included.
processes are based on Ecoinvent v3.1 (2014) and v3.2 (2015), but all Example: ‘Metal working factory'. In the production process,
upstream processes are v3.4 (2017)-3.5 (2018). Remaining data is raw materials and energy of low amounts are not included
based on Ecoinvent v3.7 (2020). "Allocation cut-off by classification" (<1%). These cut-off rules do not apply to dangerous
adjusted to improve representativeness. substances.
Allocation: Calculations of biogenic carbon:
Allocation is done in accordance with the provisions of EN 15804. Sequestration and release of biogenic carbon is included
Allocation of energy, water and waste from production is calculated by according to EN 16485:2014. This is based on the modularity
a physical allocation factor based on the manufacturer input. For principle in EN 15804:2012 that specifies that the emissions
waste produced at the manufacturing, the burdens for reuse, recycling shall be accounted in the module that they occur. The
and recovery is allocated by using this allocation factor. amount of carbon dioxide sequestrated is calulated in
accordance to EN 16449:2014. Timber comes from
sustainable forestry and has FSC certified traceability.
LCA: Scenarios and additional technical information
The following information describe the scenarios in the different modules of the EPD
The transportation from production to construction site is based on a scenario where the product is transported on a large lorry from
Kvillsfors, Sweden to Oslo, Norway (500 km) and then to a warehouse which is assumed to be in a 250 km radius from Oslo. Transport
from warehouse to a construction site is assumed to be 50 km on a medium truck.
Transport from production place to assembly/user (A4)
Type Capacity utilisation Type of vehicle Distance km Fuel/Energy Fuel/Energy
(incl. return) % consumption pr tkm consumption pr km
Truck 53 EURO5, >32 tonn 750 0.023 l/tkm 0.31 l/km
Truck 26 EURO5, 16-32 tonn 50 0.045 l/tkm 0.25 l/km
Installation (A5)
Unit Value According to the report from EPD-Norge ‘Harmonising the
Auxiliary kg 0 documentation of scenarios beyond cradle to gate, EN 15804’ there is
Water consumption m3 0 no loss on site during construction activities. The window products in
Electricity consumption MJ 0 this EPD are painted and surface treated in the production and not at
Other energy carriers MJ 0 the building site. Therefore, there is only 2 items left in this module. 1)
Material loss kg 0 Waste treatment of packaging which is considered in the EPD
Output materials from waste treatment kg 0.53 calculations. 1) Energy use during installation. This can be varied
Dust in the air kg 0 depending on the floor, type of building and several other unknown
parameters, and therefore ignored in the calculation.
Maintenance (B2)/Repair (B3)
The maintenance scenario included cleaning, painting and change of
Unit Value (alu cladding) IGU. Cleaning is performed three times per year. It is calculated with
1,5 dl of detergent and 3 litres of water each year. Windows with
Detergents kg 9
aluminium cladding are assumed to be painted 3 times during its
Water consumption l 180
lifetime from inside. It is assumed that 5 gr of lubricating oil is used
Lubricating oil kg 0.30 every year for fittings and moving parts. The glazing unit is changed
Paint kg 0.55 once during the lifetime for the windows with aluminium cladding. No
Transport tkm 2.95 repair is assumed during the product lifetime.
Glazing unit kg 41.04
Synthetic rubber kg 1.09
Transport (IGU) tkm 12.31
NEPD-3448-2059-EN Kvillsfors inward opening windows – KS, KN, KU, ES, EN, EU (with aluminium cladding)
4/9
Replacement (B4)/Refurbishment (B5)
*Number or RSL (Reference Service Life). The window has RSL of 60
Unit Value years. Therefore, it is assumed to replace the insulated glass unit after
Replacement cycle* yr 60 30 years (See Module B4). There is no need for refurbishment during
Electricity consumption kWh 0 the product lifetime.
Replacement of worn parts 0 0
(C1) As there are no data for de-construction, it is assumed no activites in C1 in this study. The windows are assumed to be treated as
mixed waste and sent to incineration. The combustible materials are then energy recovered, while glass is assumed to end up in the bottom
ash and then landfilled. The metals are usually sorted out of the bottom ash and then recycled, but there is no data of the share which are
recycled and therefore standard values from Ecoinvent is utilized.
The transport of window as waste is calculated based on a scenario with 50 km distance.
Transport to waste processing (C2)
Type Capacity utilisation Type of vehicle Distance km Fuel/Energy Fuel/Energy
(incl. return) % consumption pr tkm consumption pr km
Truck 44 Unspecified 50 0.03l/tkm 0.28 l/km
Windows are assumed to be sorted as mixed construction waste and treated with incineration with energy recovery. However, the
manufacturer has documented the recycling potentials for its product in the Construction Product Declaration eBVD
Kvillsfors inåtgående fönster - EN, ID: C-SE556294452901-101 URL: https://www.ebvd.org/BMI/Document/Export/6278/0/Pdf Kvillsfors
inåtgående fönster - ES, ID: C-SE556294452901-118 URL: https://www.ebvd.org/BMI/Document/Export/6593/0/Pdf Kvillsfors
inåtgående fönster - KN, ID: C-SE556294452901-119 URL: https://www.ebvd.org/BMI/Document/Export/6644/0/Pdf Kvillsfors
inåtgående fönster - KS, ID: C-SE556294452901-121 URL: https://www.ebvd.org/BMI/Document/Export/6653/0/Pdf
In the documentation, Chapter 10, the specific material recovery, and energy recovery potential is reported for the product.
End of Life (C1, C3, C4)
Unit Value
Hazardous waste disposed kg 0
Collected as mixed construction waste kg 70.28
Reuse kg 0
Recycling kg 3.40
Energy recovery kg 66.88
To landfill kg 0.00
The benefits beyond life cycle has been modelled based on the output flows from module C3. This includes energy from incineration and
scrap metal recovered from the ashes. The amount recovered metal is assumed to avoid production of primary metals in accordance to
6.4.3.3 in EN 15804. The exported energy is substituting Norwegian district heating mix and electricity mix. Inventory processes causing
substitution of avoided virgin raw materials has be constructed for each material.
Benefits and loads beyond the system boundaries (D)
Value (alu
Unit cladding)
Substitution of electricity MJ 33.5
Substitution of thermal energy MJ 304.9
Substitution of raw materials kg 3.4
NEPD-3448-2059-EN Kvillsfors inward opening windows – KS, KN, KU, ES, EN, EU (with aluminium cladding)
5/9
LCA: Results
Global warming potential in A1-A3 includes sequestration of CO2 as carbon in the wood. This amount is accounted as an emission in
module C3. Additionally, it is included sequestration in the wood packaging. This is accounted as an emission in module A5. The flow of
biogenic carbon for the system is presented in page 9.
System boundaries (X = included)
B4 B7
X X X X X X X X
Environmental impact With alu clad
Parameter Unit A1-A3 A4 A5
GWP kg CO -ekv 1.17E+02 4.59E+00 6.57E+00 0.00E+00 8.76E+01 0.00E+00
2
kg CFC11-ekv 1.27E-05 8.92E-07 0.00E+00 0.00E+00 7.10E-06 1.00E+00 0.00E+00
POCP kg CH -ekv 6.93E-02 5.38E-04 0.00E+00 0.00E+00
2 4
AP kg SO -ekv 1.00E+00 1.17E-02 0.00E+00 0.00E+00 5.92E-01 3.00E+00 0.00E+00 0.00E+00
2
EP kg PO3--ekv 1.00E-01 1.59E-03 0.00E+00 0.00E+00 5.90E-02 4.00E+00 0.00E+00 0.00E+00
4
ADPM kg Sb-ekv 2.33E-03 1.20E-05 0.00E+00 0.00E+00 3.83E-04 5.00E+00 0.00E+00 0.00E+00
ADPE MJ 1.66E+03 7.33E+01 0.00E+00 0.00E+00 1.09E+03 6.00E+00 0.00E+00 0.00E+00
Parameter Unit B6 B7 C1 C2 C3 C4 D
GWP kg CO -ekv 0.00E+00 0.00E+00 0.00E+00 4.42E-01 3.98E+01 5.34E-01 -4.51E+01
2
ODP kg CFC11-ekv 0.00E+00 0.00E+00 0.00E+00 8.09E-08 4.88E-08 1.42E-07 -1.40E-06
POCP kg CH -ekv 0.00E+00 0.00E+00 0.00E+00 5.58E-05 2.78E-04 1.23E-04 -1.65E-02
2 4
AP kg SO -ekv 0.00E+00 0.00E+00 0.00E+00 1.40E-03 4.59E-03 2.99E-03 -2.49E-01
2
EP kg PO3--ekv 0.00E+00 0.00E+00 0.00E+00 2.30E-04 1.40E-03 5.52E-04 -2.33E-02
4
ADPM kg Sb-ekv 0.00E+00 0.00E+00 0.00E+00 1.49E-06 1.17E-06 1.07E-06 -6.52E-05
ADPE MJ 0.00E+00 0.00E+00 0.00E+00 6.67E+00 1.14E+02 1.28E+01 -4.25E+02
GWP Global warming potential; ODP Depletion potential of the stratospheric ozone layer; POCP Formation potential of tropospheric photochemical
oxidants; AP Acidification potential of land and water; EP Eutrophication potential; ADPM Abiotic depletion potential for non fossil resources; ADPE
Abiotic depletion potential for fossil resources.
noitallatsni
noitcurtsnoC
egats esU
tnemhsibrufeR
B5 C2 C3 D
tnemecalpeR
B6
ODP
2.62E-02 2.00E+00 0.00E+00
gnissecorp
etsaW
lasopsiD
Product stage
A1 A3 A4 B1 C4
X X
ecnanetniaM
Beyond the
system
boundaries
X X
B3 B4 B5
0.00E+00 0.00E+00
0.00E+00
0.00E+00
riapeR
End of Life stage
A2 A5 B3 C1
X
B1 B2
gnirutcafunaM
X X
tropsnarT tropsnarT
esu
ygrene
lanoitarepO
Construction
and installation
stage
B2
X X
esu
retaw
lanoitarepO
noitcurtsnoc-eD
noitilomed tropsnarT
-yrevoceR-esueR laitnetop
gnilcyceR
Use stage
slairetam
waR
NEPD-3448-2059-EN Kvillsfors inward opening windows – KS, KN, KU, ES, EN, EU (with aluminium cladding)
6/9
Resource use with alu clad
Parameter Unit A1-A3 A4 A5 B1 B2 B3 B4 B5
RPEE MJ 7.2E+02 9.1E-01 0.0E+00 0.0E+00 7.2E+01 0.0E+00 0.0E+00 0.0E+00
RPEM MJ 3.7E+02 0.0E+00 0.0E+00 0.0E+00 0.0E+00 0.0E+00 0.0E+00 0.0E+00
TPE MJ 1.1E+03 9.1E-01 0.0E+00 0.0E+00 7.2E+01 0.0E+00 0.0E+00 0.0E+00
NRPE MJ 2.0E+03 7.5E+01 0.0E+00 0.0E+00 1.2E+03 0.0E+00 0.0E+00 0.0E+00
NRPM MJ 9.2E+01 0.0E+00 0.0E+00 0.0E+00 -3.4E+01 0.0E+00 0.0E+00 0.0E+00
TRPE MJ 2.1E+03 7.5E+01 0.0E+00 0.0E+00 1.1E+03 0.0E+00 0.0E+00 0.0E+00
SM kg 1.6E+00 0.0E+00 0.0E+00 0.0E+00 0.0E+00 0.0E+00 0.0E+00 0.0E+00
RSF MJ 1.6E-01 0.0E+00 0.0E+00 0.0E+00 9.3E-02 0.0E+00 0.0E+00 0.0E+00
NRSF MJ 1.0E-01 0.0E+00 0.0E+00 0.0E+00 5.9E-02 0.0E+00 0.0E+00 0.0E+00
W m3 2.5E+00 7.9E-03 0.0E+00 0.0E+00 1.1E+00 0.0E+00 0.0E+00 0.0E+00
Resource use with alu clad
Parameter Unit B6 B7 C1 C2 C3 C4 D
RPEE MJ 0.0E+00 0.0E+00 0.0E+00 9.1E-02 3.0E+02 1.9E-01 -2.0E+02
RPEM MJ 0.0E+00 0.0E+00 0.0E+00 0.0E+00 -3.0E+02 0.0E+00 0.0E+00
TPE MJ 0.0E+00 0.0E+00 0.0E+00 9.1E-02 7.1E-01 1.9E-01 -2.0E+02
NRPE MJ 0.0E+00 0.0E+00 0.0E+00 6.8E+00 1.1E+02 1.3E+01 -4.3E+02
NRPM MJ 0.0E+00 0.0E+00 0.0E+00 0.0E+00 -1.1E+02 0.0E+00 0.0E+00
TRPE MJ 0.0E+00 0.0E+00 0.0E+00 6.8E+00 5.0E+00 1.3E+01 -4.3E+02
SM kg 0.0E+00 0.0E+00 0.0E+00 0.0E+00 0.0E+00 0.0E+00 0.0E+00
RSF MJ 0.0E+00 0.0E+00 0.0E+00 0.0E+00 4.8E-01 0.0E+00 -1.3E+02
NRSF MJ 0.0E+00 0.0E+00 0.0E+00 0.0E+00 3.1E-01 0.0E+00 -8.1E+01
W m3 0.0E+00 0.0E+00 0.0E+00 7.3E-04 1.5E-02 1.2E-02 -7.1E-01
RPEE Renewable primary energy resources used as energy carrier; RPEM Renewable primary energy resources used as raw materials; TPE Total
use of renewable primary energy resources; NRPE Non renewable primary energy resources used as energy carrier; NRPM Non renewable primary
energy resources used as materials; TRPE Total use of non renewable primary energy resources; SM Use of secondary materials; RSF Use of
renewable secondary fuels; NRSF Use of non renewable secondary fuels; W Use of net fresh water.
End of life-Waste with alu clad
Parameter Unit A1-A3 A4 A5 B1 B2 B3 B4 B5
HW kg 1.96E+00 3.94E-03 0.00E+00 0.00E+00 4.56E+01 0.00E+00 0.00E+00 0.00E+00
NHW kg 4.41E+01 6.22E+00 0.00E+00 0.00E+00 1.42E+01 0.00E+00 0.00E+00 0.00E+00
RW kg 9.95E-03 5.12E-04 0.00E+00 0.00E+00 3.44E-03 0.00E+00 0.00E+00 0.00E+00
End of life-Waste with alu clad
Parameter Unit B6 B7 C1 C2 C3 C4 D
HW kg 0.00E+00 0.00E+00 0.00E+00 3.55E-04 6.03E-03 5.08E+01 -3.91E-01
NHW kg 0.00E+00 0.00E+00 0.00E+00 4.38E-01 1.53E-01 4.45E-01 -8.23E+00
RW kg 0.00E+00 0.00E+00 0.00E+00 4.66E-05 1.69E-05 8.12E-05 -5.79E-04
HW Hazardous waste disposed; NHW Non hazardous waste disposed; RW Radioactive waste disposed
End of life- Output flow with alu clad
Parameter Unit A1-A3 A4 A5 B1 B2 B3 B4 B5
CR kg 0.00E+00 0.00E+00 0.00E+00 0.00E+00 0.00E+00 0.00E+00 0.00E+00 0.00E+00
MR kg 1.23E+00 0.00E+00 5.80E-01 0.00E+00 2.19E-01 0.00E+00 0.00E+00 0.00E+00
MER kg 0.00E+00 0.00E+00 4.05E+00 0.00E+00 0.00E+00 0.00E+00 0.00E+00 0.00E+00
EEE MJ 1.17E+01 0.00E+00 0.00E+00 0.00E+00 6.37E+00 0.00E+00 0.00E+00 0.00E+00
ETE MJ 1.24E+02 0.00E+00 0.00E+00 0.00E+00 4.40E+01 0.00E+00 0.00E+00 0.00E+00
End of life- Output flow with alu clad
Parameter Unit B6 B7 C1 C2 C3 C4 D
CR kg 0.00E+00 0.00E+00 0.00E+00 0.00E+00 0.00E+00 0.00E+00 0.00E+00
MR kg 0.00E+00 0.00E+00 0.00E+00 0.00E+00 3.40E+00 0.00E+00 -3.44E+00
MER kg 0.00E+00 0.00E+00 0.00E+00 0.00E+00 0.00E+00 0.00E+00 0.00E+00
EEE MJ 0.00E+00 0.00E+00 0.00E+00 0.00E+00 3.38E+01 0.00E+00 -3.35E+01
ETE MJ 0.00E+00 0.00E+00 0.00E+00 0.00E+00 2.35E+02 0.00E+00 -3.05E+02
CR Components for reuse; MR Materials for recycling; MER Materials for energy recovery; EEE Exported electric energy; ETE Exported thermal
energy
Reading example: 9,0 E-03 = 9,0*10-3 = 0,009
NEPD-3448-2059-EN Kvillsfors inward opening windows – KS, KN, KU, ES, EN, EU (with aluminium cladding)
7/9
Norwegian additional requirements
Greenhouse gas emissions from the use of electricity in the production phase
National (Sweden) market with low-voltage, including imports, direct emissions, infrastructure and transmission losses, has been used
for electricity in the production process (A3). The manufacturer is documented the use of electricity from hydropower with guarantees of
origin, which has 6 fold less GWP effect. However, the final result has only be improved by 0.6% in A1-A3 production. Therfore, the
national electricity mix is considerd.
Data source Quantity Unit
Ecoinvent v3.7 (september 2020) 41 gram CO 2-ekv./kWh
Hazardous substances
The product contains no substances from REACH Candidate List or the Norwegian Priority List
The product contains substances below 0.1% by weight on the REACH Candidate List
The product contains substances from REACH Candidate List or the Norwegian Priority List, see table under Specific
Norwegian requirements.
The product does not contain any substances on the REACH Candidate List or the Norwegian Priority List. The product can be
characterized as hazardous waste (according to the Waste Shift, Appendix III), see table under Specific Norwegian
requirements.
Transport
Transport from production site to construction site according to scenario in A4: 750+50 km
Indoor air quality
The product has not been tested for emissions to indoor environments.
Carbon footprint
To increase the transparency of the climate impacts, the GWP indicator has been divided into sub-indicators:
GWP-IOBC Climate impacts calculated according to instant oxidation principle
GWP-BCIP Climate impacts calculated from the net impacts of sequestration and emission of biogenic carbon
Climate impact with alu clad
Parameter Unit A1-A3 A4 A5 B1 B2 B3 B4 B5
GWP-IOBC kg CO -ekv 1.52E+02 4.59E+00 0.00E+00 0.00E+00 8.76E+01 0.00E+00 0.00E+00 0.00E+00
2
GWP-BCIP kg CO -ekv -3.52E+01 0.00E+00 6.57E+00 0.00E+00 0.00E+00 0.00E+00 0.00E+00 0.00E+00
2
GWP kg CO -ekv 1.17E+02 4.59E+00 6.57E+00 0.00E+00 8.76E+01 0.00E+00 0.00E+00 0.00E+00
2
Climate impact with alu clad
Parameter Unit B6 B7 C1 C2 C3 C4 D
GWP-IOBC kg CO -ekv 0.00E+00 0.00E+00 0.00E+00 4.42E-01 1.12E+01 5.34E-01 -4.51E+01
2
GWP-BCIP kg CO -ekv 0.00E+00 0.00E+00 0.00E+00 0.00E+00 2.86E+01 0.00E+00 0.00E+00
2
GWP kg CO -ekv 0.00E+00 0.00E+00 0.00E+00 4.42E-01 3.98E+01 5.34E-01 -4.52E+01
2
Additional information
For the products with different sizes from the declared unit, the environmental impacts must be converted by using a conversion factor.
The Norwegian EPD Foundation has published instructions on how to interpret EPDs for windows on its website (www.epd-norge.no)
where different calculation methods have been stated. (Document: Bruksanvisninger i hvordan tolke EPD'er – Vinduer)
NEPD-3448-2059-EN Kvillsfors inward opening windows – KS, KN, KU, ES, EN, EU (with aluminium cladding)
8/9
Bibliografi
NS-EN ISO 14025:2010 Miljømerker og deklarasjoner - Miljødeklarasjoner type III - Prinsipper og prosedyrer.
NS-EN ISO 14044:2006 Miljøstyring - Livsløpsvurderinger - Krav og retningslinjer
NS-EN 15804:2012+A1:2013 Bærekraftig byggverk - Miljødeklarasjoner - Grunnleggende produktkategoriregler for
byggevarer
ISO 21930:2007 Sustainability in building construction - Environmental declaration of building products
Modaresi, R. 2020 LCA-report for Nordan LCA-report nr. 325039-1 from Norwegian Institute of Wood
Technology, Oslo, Norway.
NPCR014 (04/2019) Product category rules for windows and doors, rev3, April 2019
NS-EN 16485:2014 Tømmer og skurlast - Miljødeklarasjoner - Produktkategoriregler for tre og trebaserte produkter
til bruk i byggverk
NS-EN 16449:2014 Tre og trebaserte produkter - Beregning av biogent karboninnhold i tre og omdanning til
karbondioksid
Ecoinvent v3.0-3.7 Ecoinvent database version 3.0-3.7 Centre for Life Cycle Inventories.
Statistisk sentralbyrå Tabell 04727: Fjernvarmebalansen, 2015
Statistisk sentralbyrå Tabell 09469: Nettoproduksjon av fjernvarme, 2015
NEPD-307-179-NO EPD for skurlast av gran eller furu. Treindustrien
Bruksanvisninger i hvordan tolke EPD'er – Vinduer. https://www.epd-norge.no [in Norwegian]
Publisher Tlf: +47 23 08 80 00
The Norwegian EPD Foundation
Postboks 5250 Majorstuen, 0303 Oslo e-post: post@epd-norge.no
Norway web www.epd-norge.no
Owner of the declaration Tlf: +47 51 40 40 00
NorDan AS
Stasjonsveien 46, N-4460 Moi e-post: firmapost@nordan.no
Norway
web www.nordan.no
Author of the Life Cycle Assessment Tlf: +47 98 85 33 33
Roja Modaresi
Norsk Treteknisk Instiutt e-post: firmapost@treteknisk.no
Postboks 113 Blindern, 0314 Oslo, Norway web www.treteknisk.no
NEPD-3448-2059-EN Kvillsfors inward opening windows – KS, KN, KU, ES, EN, EU (with aluminium cladding)
9/9
EPD for the best
environmental
decision
www.epd-norge.no
The Norwegian EPD foundation
EPD for the best environmental decision
12
