Environmental product declaration
in accordance with ISO 14025 and EN 15804+A2
CC4455 TT004455 GGBB SS44 2200 CC33AA44LL PP22 EECCOO5500
OOwwnneerr ooff tthhee ddeeccllaarraattiioonn:: PPrrooggrraamm ooppeerraattoorr::
Heidelberg Materials Benelux SA - RMC The Norwegian EPD Foundation
PPrroodduucctt:: DDeeccllaarraattiioonn nnuummbbeerr::
C45 T045 GB S4 20 C3A4L P2 ECO50
NEPD-9233-8822
DDeeccllaarreedd uunniitt::
RReeggiissttrraattiioonn nnuummbbeerr::
1 m3
NEPD-9233-8822
TThhiiss ddeeccllaarraattiioonn iiss bbaasseedd oonn PPrroodduucctt CCaatteeggoorryy
RRuulleess:: IIssssuuee ddaattee:: 25.02.2025
CEN Standard EN 15804:2012+A2:2019 serves as core PCR
The Norwegian EPD Foundation EN 16757:2022 for Concrete and concrete elements VVaalliidd ttoo:: 25.02.2030
EEPPDD ssooffttwwaarree::
LCAno EPD generator ID: 822659
1 / 11
GGeenneerraall iinnffoorrmmaattiioonn
PPrroodduucctt OOwwnneerr ooff tthhee ddeeccllaarraattiioonn::
C45 T045 GB S4 20 C3A4L P2 ECO50 Heidelberg Materials Benelux SA - RMC
Contact person: Bart Vandenbussche
e-mail: bart.vandenbussche@heidelbergmaterials.com
PPrrooggrraamm ooppeerraattoorr:: MMaannuuffaaccttuurreerr::
The Norwegian EPD Foundation Heidelberg Materials Benelux SA - RMC
Post Box 5250 Majorstuen, 0303 Oslo, Norway Contact person: Bart Vandenbussche
Phone: +47 977 22 020 e-mail: bart.vandenbussche@heidelbergmaterials.com
web: www.epd-norge.no Phone: +32 2 678 32 11
DDeeccllaarraattiioonn nnuummbbeerr:: PPllaaccee ooff pprroodduuccttiioonn::
Heidelberg Materials Benelux SA - RMC
NEPD-9233-8822
Parc de l'Alliance, Boulevard de France 3-5
1420 Braine-l'Alleud, Belgium
TThhiiss ddeeccllaarraattiioonn iiss bbaasseedd oonn PPrroodduucctt CCaatteeggoorryy RRuulleess:: MMaannaaggeemmeenntt ssyysstteemm::
CEN Standard EN 15804:2012+A2:2019 serves as core PCR
EN 16757:2022 for Concrete and concrete elements
SSttaatteemmeenntt ooff lliiaabbiilliittyy:: OOrrggaanniissaattiioonn nnoo::
The owner of the declaration shall be liable for the underlying BE0400465290
information and evidence. EPD Norway shall not be liable with respect to
manufacturer information, life cycle assessment data and evidences.​
DDeeccllaarreedd uunniitt:: IIssssuuee ddaattee::
1 m3 C45 T045 GB S4 20 C3A4L P2 ECO50 25.02.2025
DDeeccllaarreedd uunniitt wwiitthh ooppttiioonn:: VVaalliidd ttoo::
A1,A2,A3,A4,C1,C2,C3,C4,D 25.02.2030
YYeeaarr ooff ssttuuddyy::
2024
FFuunnccttiioonnaall uunniitt:: CCoommppaarraabbiilliittyy::
EPD of construction products may not be comparable if they not
comply with EN 15804 and seen in a building context.
GGeenneerraall iinnffoorrmmaattiioonn oonn vveerriiffiiccaattiioonn ooff EEPPDD ffrroomm EEPPDD ttoooollss:: DDeevveellooppmmeenntt aanndd vveerriiffiiccaattiioonn ooff EEPPDD::
Independent verification of data, other environmental information and The declaration is created using EPD tool lca.tools ver EPD2022.03,
the declaration according to ISO 14025:2010, § 8.1.3 and § 8.1.4. developed by LCA.no. The EPD tool is integrated in the company's
Verification of each EPD is made according to EPD-Norway’s guidelines management system, and has been approved by EPD Norway. NEPDT17
for verification and approval requiring that tools are i) integrated into
Developer of EPD: Jan De Soete
the company's environmental management system, ii) the procedures
for use of the EPD tool are approved by EPD-Norway, and iii) the process Reviewer of company-specific input data and EPD:​ Zoe Stubbe
is reviewed annually by an independent third party verifier. See
Appendix G of EPD-Norway's General Programme Instructions for
further information on EPD tools
VVeerriiffiiccaattiioonn ooff EEPPDD ttooooll:: AApppprroovveedd::
Independent third party verification of the EPD tool, background data
and test-EPD in accordance with EPDNorway's procedures and
guidelines for verification and approval of EPD tools.
Håkon Hauan, CEO EPD-Norge
Third party verifier:
Ellen Soldal, Norsus AS
(no signature required)
2 / 11
PPrroodduucctt
PPrroodduucctt ddeessccrriippttiioonn::
Concrete is a building material made up of several components, including cement, water, sand, gravel, and air. Ready-mixed
concrete is manufactured in a batch plant in a controlled environment, using precise mix designs (with the addition of other
cementitious materials or chemical admixtures that improve the properties of the concrete), ensuring consistency in quality,
strength, and composition. This consistency leads to predictable performance in construction projects. Ready-mixed concrete
is then delivered to the construction site in an unhardened state, ready to use, eliminating the need for on-site mixing.
PPrroodduucctt ssppeecciiffiiccaattiioonn
The concrete can be delivered in different fluidity's, strength classes, enviromental classes and with different cement types according to NBN B15-001
and EN 206.
MMaatteerriiaallss VVaalluuee UUnniitt
Water 150 - 180 kg
Admixture 1-4 kg
Aggregates fine 650 - 850 kg
Aggregates coarse 950 - 1150 kg
cement min. 340 kg
TTeecchhnniiccaall ddaattaa::
The product is produced according to NBN B15-001 and EN 206. Testing was conducted according to TRA550. Performance data of the product with
respect to its characteristics in accordance with the relevant technical provision (no CE-marking).
MMaarrkkeett::
Belgium
RReeffeerreennccee sseerrvviiccee lliiffee,, pprroodduucctt
100 years
The normal technical lifespan (the period during which the structure fulfills its intended function with "normal maintenance") for a concrete structure is up
to 100 years. The lifespan is influenced by application, maintenance and material choices and can be extended with, for example, thicker concrete
cover, more durable reinforcement or impregnation.
RReeffeerreennccee sseerrvviiccee lliiffee,, bbuuiillddiinngg oorr ccoonnssttrruuccttiioonn wwoorrkkss
50years, RSL building cannot be determined as product application is unknown.
LLCCAA:: CCaallccuullaattiioonn rruulleess
DDeeccllaarreedd uunniitt::
1 m3 C45 T045 GB S4 20 C3A4L P2 ECO50
CCuutt--ooffff ccrriitteerriiaa::
All major raw materials and all the essential energy is included. The production processes for raw materials and energy flows with very small amounts
(less than 1%) are not included. These cut-off criteria do not apply for hazardous materials and substances.
AAllllooccaattiioonn::
The allocation is made in accordance with the provisions of EN 15804. Incoming energy and water and waste production in-house is allocated equally
among all products through mass allocation. Effects of primary production of recycled materials is allocated to the main product in which the material
was used. The recycling process and transportation of the material is allocated to this analysis.
DDaattaa qquuaalliittyy::
Specific data for the product composition are provided by the manufacturer. The data represent the production of the declared product and were
collected for EPD development in the year of study. Background data is based on EPDs according to EN 15804 and different LCA databases. The data
quality of the raw materials in A1 is presented in the table below.
MMaatteerriiaallss SSoouurrccee DDaattaa qquuaalliittyy YYeeaarr
Additives EPD-EFC-20210198-IBG2-EN EPD 2019
Aggregate ecoinvent 3.10 Database 2023
Cement ecoinvent 3.10 Database 2023
Others LCA.no Database 2024
3 / 11
SSyysstteemm bboouunnddaarriieess ((XX==iinncclluuddeedd,, MMNNDD==mmoodduullee nnoott ddeeccllaarreedd,, MMNNRR==mmoodduullee nnoott rreelleevvaanntt))
CCoonnssttrruuccttiioonn
BBeeyyoonndd tthhee ssyysstteemm
PPrroodduucctt ssttaaggee iinnssttaallllaattiioonn UUssee ssttaaggee EEnndd ooff lliiffee ssttaaggee
bboouunnddaarriieess
ssttaaggee
A1 A2 A3 A4 A5 B1 B2 B3 B4 B5 B6 B7 C1 C2 C3 C4 D
X X X X MND MND MND MND MND MND MND MND X X X X X
SSyysstteemm bboouunnddaarryy::
AAddddiittiioonnaall tteecchhnniiccaall iinnffoorrmmaattiioonn::
waR slairetam tropsnarT gnirutcafunaM tropsnarT ylbmessA ​esU ecnanetniaM riapeR tnemecalpeR tnemhsibrufeR lanoitarepO ygrene esu lanoitarepO retaw esu -eD noitcurtsnoc noitilomed tropsnarT etsaW gnissecorp lasopsiD -yrevoceR-esueR laitnetop-gnilcyceR
4 / 11
LLCCAA:: SScceennaarriiooss aanndd aaddddiittiioonnaall tteecchhnniiccaall iinnffoorrmmaattiioonn
The following information describe the scenarios in the different modules of the EPD.
CCaappaacciittyy
TTrraannssppoorrtt ffrroomm pprroodduuccttiioonn ppllaaccee ttoo FFuueell//EEnneerrggyy VVaalluuee
uuttiilliissaattiioonn ((iinnccll.. DDiissttaannccee ((kkmm)) UUnniitt
uusseerr ((AA44)) CCoonnssuummppttiioonn ((LLiitteerr//ttoonnnnee))
rreettuurrnn)) %%
Transport|Truck, 16-32 tonnes, EURO
36,7 % 30 0,044 0 1,32
5|km|GLO|2023
DDee--ccoonnssttrruuccttiioonn ddeemmoolliittiioonn ((CC11)) UUnniitt VVaalluuee
EOL|Demolition of building per kg of cement-
kg 2320,000000000
based product|kg|GLO|2019
CCaappaacciittyy
FFuueell//EEnneerrggyy VVaalluuee
TTrraannssppoorrtt ttoo wwaassttee pprroocceessssiinngg ((CC22)) uuttiilliissaattiioonn ((iinnccll.. DDiissttaannccee ((kkmm)) UUnniitt
CCoonnssuummppttiioonn ((LLiitteerr//ttoonnnnee))
rreettuurrnn)) %%
Transport|Truck, over 32 tonnes, EURO
53,3 % 30 0,023 l/tkm 0,69
5|km|GLO|2023
WWaassttee pprroocceessssiinngg ((CC33)) UUnniitt VVaalluuee
EOL|Waste treatment of cement-based
product after demolition, 100% to kg 2320,000000000
recycling|kg|GLO|2019
BBeenneeffiittss aanndd llooaaddss bbeeyyoonndd tthhee ssyysstteemm
UUnniitt VVaalluuee
bboouunnddaarriieess ((DD))
SUB|Substitution of primary aggregates,
kg 2320,000000000
gravel round|kg|GLO|2019
5 / 11
LLCCAA:: RReessuullttss
The LCA results are presented below for the declared unit defined on page 2 of the EPD document.
EEnnvviirroonnmmeennttaall iimmppaacctt
IInnddiiccaattoorr UUnniitt A1 A2 A3 A4 C1 C2 C3 C4 D
GWP-total kg CO2 -eq 1,92E+02 2,26E+01 1,32E+00 1,35E+01 9,28E+00 7,47E+00 1,67E+00 0 -5,42E+00
GWP-fossil kg CO2 -eq 1,89E+02 2,26E+01 1,32E+00 1,35E+01 9,28E+00 7,46E+00 1,65E+00 0 -5,31E+00
GWP-biogenic kg CO2 -eq 3,10E+00 1,47E-02 7,36E-03 8,77E-03 1,74E-03 3,61E-03 1,42E-02 0 -1,06E-01
GWP-luluc kg CO2 -eq 7,91E-02 7,39E-03 2,90E-04 4,41E-03 7,32E-04 2,56E-03 2,28E-03 0 -3,59E-03
ODP kg CFC11 -eq 9,17E-07 4,66E-07 7,51E-08 2,78E-07 2,00E-06 1,39E-07 3,25E-07 0 -9,67E-07
AP mol H+ -eq 5,76E-01 7,06E-02 3,82E-03 4,21E-02 9,71E-02 2,41E-02 1,33E-02 0 -4,78E-02
EP-FreshWater kg P -eq 2,65E-02 1,51E-03 1,80E-04 8,99E-04 3,38E-05 5,07E-04 1,04E-04 0 -1,41E-04
EP-Marine kg N -eq 1,40E-01 2,38E-02 7,54E-04 1,42E-02 4,29E-02 8,19E-03 3,91E-03 0 -1,66E-02
EP-Terrestial mol N -eq 1,58E+00 2,59E-01 7,54E-03 1,54E-01 4,64E-01 8,90E-02 4,50E-02 0 -1,95E-01
kg NMVOC -
POCP 4,59E-01 1,11E-01 2,72E-03 6,60E-02 1,29E-01 3,93E-02 1,21E-02 0 -5,14E-02
eq
ADP-
kg Sb-eq 6,80E-04 7,38E-05 1,76E-05 4,41E-05 1,42E-05 2,06E-05 2,09E-05 0 -4,72E-04
minerals&metals1
ADP-fossil1 MJ 1,10E+03 3,17E+02 4,29E+01 1,89E+02 1,28E+02 1,08E+02 5,12E+01 0 -8,98E+01
WDP1 m3 3,21E+01 1,53E+00 3,77E+00 9,14E-01 2,71E+01 5,43E-01 5,65E+03 0 -4,21E+03
GWP-total = Global Warming Potential total; GWP-fossil = Global Warming Potential fossil fuels; GWP-biogenic = Global Warming Potential biogenic;
GWP-luluc = Global Warming Potential land use and land use change; ODP = Depletion potential of the stratospheric ozone layer; AP = Acidification
potential, Accumulated Exceedance; EP-freshwater = Eutrophication potential, fraction of nutrients reaching freshwater end compartment: EP-marine =
Eutrophication potential, fraction of nutrients reaching marine end compartment; EP-terrestrial = Eutrophication potential, Accumulated Exceedance;
POCP = Formation potential of tropospheric ozone; ADP-minerals&metals = Abiotic depletion potential for non-fossil resources; ADP-fossil = Abiotic
depletion for fossil resources potential; WDP = Water (user) deprivation potential, deprivation-weighted water consumption
"Reading example: 9,0 E-03 = 9,0*10-3 = 0,009"
*INA Indicator Not Assessed
1. The results of this environmental impact indicator shall be used with care as the uncertainties on these results are high or as there is limited
experienced with the indicator
RReemmaarrkkss ttoo eennvviirroonnmmeennttaall iimmppaaccttss
GWP includes the emissions from the combustion of waste fuel materials in the cement production process.
6 / 11
AAddddiittiioonnaall eennvviirroonnmmeennttaall iimmppaacctt iinnddiiccaattoorrss
IInnddiiccaattoorr UUnniitt A1 A2 A3 A4 C1 C2 C3 C4 D
PM Disease incidence 5,15E-06 1,75E-06 2,48E-08 1,04E-06 1,18E-05 7,66E-07 2,13E-07 0 -1,02E-06
IRP2 kgBq U235 -eq 9,05E+00 4,07E-01 1,43E+00 2,43E-01 5,57E-01 1,31E-01 8,58E-01 0 -8,25E-01
ETP-fw1 CTUe 6,22E+02 8,51E+01 7,60E+00 5,08E+01 6,98E+01 2,56E+01 3,63E+01 0 -9,25E+01
HTP-c1 CTUh 3,02E-07 1,17E-07 2,08E-09 6,96E-08 2,32E-09 6,96E-08 2,32E-09 0 -4,64E-09
HTP-nc1 CTUh 1,34E-06 2,33E-07 1,63E-08 1,39E-07 6,50E-08 6,96E-08 3,25E-08 0 -1,14E-07
SQP1 dimensionless 4,72E+02 1,88E+02 5,54E+00 1,13E+02 1,55E+01 1,09E+02 2,89E+01 0 2,04E+02
PM = Particulate Matter emissions; IRP = Ionizing radiation – human health; ETP-fw = Eco toxicity – freshwater; HTP-c = Human toxicity – cancer effects;
HTP-nc = Human toxicity – non cancer effects; SQP = Potential Soil Quality Index (dimensionless)
"Reading example: 9,0 E-03 = 9,0*10-3 = 0,009"
*INA Indicator Not Assessed
1. The results of this environmental impact indicator shall be used with care as the uncertainties on these results are high or as there is limited
experienced with the indicator
2. This impact category deals mainly with the eventual impact of low dose ionizing radiation on human health of the nuclear fuel cycle. It does not
consider effects due to possible nuclear accidents, occupational exposure nor due to radioactive waste disposal in underground facilities. Potential
ionizing radiation from the soil, from radon and from some construction materials is also not measured by this indicator.
7 / 11
RReessoouurrccee uussee
IInnddiiccaattoorr UUnniitt A1 A2 A3 A4 C1 C2 C3 C4 D
PERE MJ 1,18E+02 5,37E+00 3,01E+00 3,21E+00 6,96E-01 1,72E+00 2,63E+01 0 -2,10E+01
PERM MJ 2,34E-01 0,00E+00 0,00E+00 0,00E+00 0,00E+00 0,00E+00 0,00E+00 0 0,00E+00
PERT MJ 1,18E+02 5,37E+00 3,01E+00 3,21E+00 6,96E-01 1,72E+00 2,63E+01 0 -2,10E+01
PENRE MJ 1,09E+03 3,17E+02 4,29E+01 1,89E+02 1,28E+02 1,08E+02 5,12E+01 0 -9,48E+01
PENRM MJ 1,16E+01 0,00E+00 0,00E+00 0,00E+00 0,00E+00 0,00E+00 0,00E+00 0 0,00E+00
PENRT MJ 1,10E+03 3,17E+02 4,29E+01 1,89E+02 1,28E+02 1,08E+02 5,12E+01 0 -9,48E+01
SM kg 0,00E+00 0,00E+00 0,00E+00 0,00E+00 0,00E+00 0,00E+00 0,00E+00 0 0,00E+00
RSF MJ 5,88E-03 1,83E-03 3,68E-03 1,09E-03 0,00E+00 5,90E-04 0,00E+00 0 -4,30E-01
NRSF MJ 0,00E+00 0,00E+00 0,00E+00 0,00E+00 0,00E+00 0,00E+00 0,00E+00 0 -4,42E-01
FW m3 2,31E+00 4,21E-02 1,04E-02 2,51E-02 6,58E-03 1,57E-02 8,76E-02 0 -3,30E+00
PERE = Use of renewable primary energy excluding renewable primary energy resources used as raw materials; PERM = Use of renewable primary energy
resources used as raw materials; PERT = Total use of renewable primary energy resources; PENRE = Use of non renewable primary energy excluding non-
renewable primary energy resources used as raw materials; PENRM = Use of non renewable primary energy resources used as raw materials; PENRT =
Total use of non renewable primary energy resources; SM = Use of secondary materials; RSF = Use of renewable secondary fuels; NRSF = Use of non-
renewable secondary fuels; FW = Net use of fresh water
"Reading example: 9,0 E-03 = 9,0*10-3 = 0,009"
*INA Indicator Not Assessed
8 / 11
EEnndd ooff lliiffee -- WWaassttee
IInnddiiccaattoorr UUnniitt A1 A2 A3 A4 C1 C2 C3 C4 D
HWD kg 4,90E+00 4,56E-01 4,03E-02 2,72E-01 3,76E-03 1,57E-01 5,11E-03 0 -2,17E-02
NHWD kg 1,59E+02 9,64E+00 1,01E+00 5,75E+00 1,51E-01 3,15E+00 1,61E-01 0 -6,57E-01
RWD kg 3,30E-03 1,01E-04 3,38E-04 6,03E-05 8,87E-04 3,25E-05 5,41E-04 0 -7,13E-04
HWD = Hazardous waste disposed; NHWD = Non-hazardous waste disposed; RWD = Radioactive waste disposed
"Reading example: 9,0 E-03 = 9,0*10-3 = 0,009"
*INA Indicator Not Assessed
EEnndd ooff lliiffee -- OOuuttppuutt ffllooww
IInnddiiccaattoorr UUnniitt A1 A2 A3 A4 C1 C2 C3 C4 D
CRU kg 0,00E+00 0,00E+00 0,00E+00 0,00E+00 0,00E+00 0,00E+00 0,00E+00 0 0,00E+00
MFR kg 0,00E+00 0,00E+00 1,48E+01 0,00E+00 0,00E+00 0,00E+00 2,32E+03 0 0,00E+00
MER kg 0,00E+00 0,00E+00 9,80E-02 0,00E+00 0,00E+00 0,00E+00 0,00E+00 0 0,00E+00
EEE MJ 0,00E+00 0,00E+00 9,70E-05 0,00E+00 0,00E+00 0,00E+00 0,00E+00 0 0,00E+00
EET MJ 0,00E+00 0,00E+00 1,47E-03 0,00E+00 0,00E+00 0,00E+00 0,00E+00 0 0,00E+00
CRU = Components for re-use; MFR = Materials for recycling; MER = Materials for energy recovery; EEE = Exported energy electrical; EET = Exported
energy thermal
"Reading example: 9,0 E-03 = 9,0*10-3 = 0,009"
*INA Indicator Not Assessed
BBiiooggeenniicc CCaarrbboonn CCoonntteenntt
IInnddiiccaattoorr UUnniitt AAtt tthhee ffaaccttoorryy ggaattee
Biogenic carbon content in product kg C 0,00E+00
Biogenic carbon content in accompanying packaging kg C 0,00E+00
Note: 1 kg biogenic carbon is equivalent to 44/12 kg CO2
9 / 11
AAddddiittiioonnaall rreeqquuiirreemmeennttss
GGrreeeennhhoouussee ggaass eemmiissssiioonnss ffrroomm tthhee uussee ooff eelleeccttrriicciittyy iinn tthhee mmaannuuffaaccttuurriinngg pphhaassee
National production mix from import, low voltage (production of transmission lines, in addition to direct emissions and losses in grid) of applied
electricity for the manufacturing process (A3).
EElleeccttrriicciittyy mmiixx SSoouurrccee AAmmoouunntt UUnniitt
EL|residual mix|kWh|BE|2023 ecoinvent 3.10 208,50 g CO2-eq/kWh
DDaannggeerroouuss ssuubbssttaanncceess
The product contains no substances given by the REACH Candidate list.
IInnddoooorr eennvviirroonnmmeenntt
Has no impact on indoor environment.
AAddddiittiioonnaall EEnnvviirroonnmmeennttaall IInnffoorrmmaattiioonn
AAddddiittiioonnaall eennvviirroonnmmeennttaall iimmppaacctt iinnddiiccaattoorrss
IInnddiiccaattoorr UUnniitt A1 A2 A3 A4 C1 C2 C3 C4 D
GWPIOBC kg CO2 -eq 1,89E+02 2,26E+01 1,32E+00 1,35E+01 9,28E+00 7,47E+00 1,65E+00 0 -5,68E+00
GWP-IOBC: Global warming potential calculated according to the principle of instantaneous oxidation. In order to increase the transparency of
biogenic carbon​ contribution to climate impact, the indicator GWP-IOBC is required as it declares climate impacts calculated according to the
principle of instantaneous oxidation.​ GWP-IOBC is also referred to as GWP-GHG in context to Swedish public procurement legislation.
10 / 11
BBiibblliiooggrraapphhyy
ISO 14025:2010 Environmental labels and declarations - Type III environmental declarations - Principles and procedures.
ISO 14044:2006 Environmental management - Life cycle assessment - Requirements and guidelines.
EN 15804:2012+A2:2019 Environmental product declaration - Core rules for the product category of construction products.
ISO 21930:2017 Sustainability in buildings and civil engineering works - Core rules for environmental product declarations of construction products.
ecoinvent v3, Allocation, cut-off by classification, Swiss Centre of Life Cycle Inventories.
Iversen et al., (2021) eEPD v2021.09 Background information for EPD generator tool system verification, LCA.no Report number: 07.21
Graafland et al., (2024) EPD generator for concrete and concrete elements, EN 16757 Background information for EPD generator application and LCA
data, LCA.no report number: 01.24
NS-EN 16757:2022 for concrete and concrete elements, Ver. 1.0,
Vold et al., (2024) EPD generator for Heidelberg, concrete and concrete elements, EN 16757 Additional background information, specific for Heidelberg
Materials, LCA.no report number: 19.24
PPrrooggrraamm ooppeerraattoorr aanndd ppuubblliisshheerr Phone: +47 977 22 020
The Norwegian EPD Foundation e-mail: post@epd-norge.no
Post Box 5250 Majorstuen, 0303 Oslo, Norway web: www.epd-norge.no
OOwwnneerr ooff tthhee ddeeccllaarraattiioonn:: +32 2 678 32 11
Phone:
Heidelberg Materials Benelux SA - RMC bart.vandenbussche@heidelbergmaterials.com
e-mail:
Parc de l'Alliance, Boulevard de France 3-5, 1420 https://www.heidelbergmaterials-
web:
Braine-l'Alleud, Belgium benelux.com/fr
AAuutthhoorr ooff tthhee LLiiffee CCyyccllee AAsssseessssmmeenntt Phone: +47 916 50 916
LCA.no AS e-mail: post@lca.no
Dokka 6A, 1671 Kråkerøy, Norway web: www.lca.no
DDeevveellooppeerr ooff EEPPDD ggeenneerraattoorr Phone: +47 916 50 916
LCA.no AS e-mail: post@lca.no
Dokka 6A, 1671 Kråkerøy, Norway web: www.lca.no
ECO Platform web: www.eco-platform.org
ECO Portal web: ECO Portal
11 / 11
