ver1 2015
ENVIRONMENTAL PRODUCT DECLARATION
in accordance with ISO 14025, ISO 21930 and EN 15804
Owner of the declaration: Saint-Gobain Sweden AB, Weber floor
Program operator: The Norwegian EPD Foundation
Publisher: The Norwegian EPD Foundation
Declaration number: NEPD-3166-1808-EN
Registration number: NEPD-3166-1808-EN
ECO Platform reference number: -
Issue date: 11.10.2021
Valid to: 11.10.2026
weberfloor 4650 Design Colour
Saint-Gobain Sweden AB, Weber floor
www.epd-norge.no
NEPD-3166-1808-EN weberfloor 4650 Design Colour
1 / 8
General information
Product: Owner of the declaration:
weberfloor 4650 Design Colour Saint-Gobain Sweden AB, Weber floor
Contact person: Anders Anderberg
Phone: +46 8 625 6105
e-mail: anders.anderberg@weber.se
Program operator: Manufacturer:
Saint-Gobain Sweden AB, Weber floor
The Norwegian EPD Foundation
Pb. 5250 Majorstuen, 0303 Oslo
Phone: +47 23 08 80 00
e-mail: post@epd-norge.no
Declaration number: Place of production:
Saint-Gobain Sweden AB, Weber floor
NEPD-3166-1808-EN Box 415 SE-19162 Sollentuna
Sweden
ECO Platform reference number: Management system:
ISO 9001, ISO 14001
This declaration is based on Product Category Rules: Organisation no:
SE-556241-2592
CEN Standard EN 15804:2012+A1:2013 serves as core PCR.
NPCR 009:2018 Part B for Technical - Chemical products in the building and
construction industry
Statement of liability: Issue date: 11.10.2021
The owner of the declaration shall be liable for the underlying information and
evidence. EPD Norway shall not be liable with respect to manufacturer Valid to: 11.10.2026
information, life cycle assessment data and evidences.
Declared unit: Year of study:
1 kg weberfloor 4650 Design Colour 2020
Declared unit with option: Comparability:
EPD of construction products may not be comparable if they not comply with EN
A1,A2,A3,A4,A5,C1,C2,C3,C4,D
15804 and seen in a building context.
Functional unit: Development and verification of EPD:
The declaration has been developed and verified using EPD tool lca.tools
ver EPD2020.11, developed by LCA.no AS. The EPD tool is integrated into
the company's environmental management system, and has been
approved by EPD-Norway
General information on verification of EPD from EPD tools:
Independent verification of data, other environmental information and Developer of EPD:
the declaration according to ISO 14025:2010, § 8.1.3 and § 8.1.4. Individual
third party verification of each EPD is not required when the EPD tool is i) Thomas Flycht
integrated into the company's environmental management system, ii) the
procedures for use of the EPD tool are approved by EPDNorway, and iii) Reviewer of company-specific input data and EPD:
the proccess is reviewed annualy. See Appendix G of EPD-Norway's
General Programme Instructions for further information on EPD tools. Helene Wallgren
Verification of EPD tool: Approved:
Independent third party verification of the EPD tool, background data
Sign
and test-EPD in accordance with EPDNorway's procedures and guidelines
for verification and approval of EPD tools.
Anne Rønning, Norsus AS
(no signature required) Håkon Hauan, CEO EPD-Norge
NEPD-3166-1808-EN weberfloor 4650 Design Colour
2 / 8
Product
Product description: Technical data:
weberfloor 4650 Design Colour is a pumpable rapid hardening levelling weberfloor 4650 Design Colour is designed, produced and CE marked
compound for floors internally in buildings. It is designed to form a according to EN 13813
final surface in areas such as offices, commercial areas, show rooms,
etc. where it is an esthetic element in the room. The product is For further information, see www.se.weber/
moisture-resistant and does not contain slag, flyash or casein.
Market:
Product specification
Scandinavian countries
The composition of the product is described in the following table:
Reference service life, product
Materials %
> 50 years
Aggregate 30-60
Filler 20-50 Reference service life, building
Binder 15-35
> 50 years
Additives 1-5
LCA: Calculation rules
Declared unit: Allocation:
The allocation is made in accordance with the provisions of EN 15804.
1 kg weberfloor 4650 Design Colour
Incoming energy and water and waste production in-house is allocated
Cut-off criteria: equally among all products through mass allocation. Effects of primary
production of recycled materials is allocated to the main product in which
All major raw materials and all the essential energy is included. The
the material was used. The recycling process and transportation of the
production processes for raw materials and energy flows with very small
material is allocated to this analysis.
amounts (less than 1%) are not included. These cut-off criteria do not
apply for hazardous materials and substances.
Data quality:
Specific data for the product composition are provided by the manufacturer. They represent the production of the declared product and were collected for
EPD development in the year of study. Background data is based on registered EPDs according to EN 15804, Ostfold Research databases, ecoinvent and other
LCA databases. The data quality of the raw materials in A1 is presented in the table below.
Materials Source Data quality Year
Cement Supplier EPD 2012
Binder EPD-BVG-20140073-IAG1-EN EPD 2014
Additives ecoinvent 3.4 Database 2017
Aggregate ecoinvent 3.4 Database 2017
Filler ecoinvent 3.4 Database 2017
Packaging ecoinvent 3.4 Database 2017
Packaging Modified ecoinvent 3.4 Database 2017
Cement ecoinvent 3.6 Database 2019
NEPD-3166-1808-EN weberfloor 4650 Design Colour
3 / 8
System boundary:
All processes from raw material extraction to product transport to the construction site and assembly are included in the analysis as well as end of life stage
and phases beyond the system boundary (A1 - A5, C1-C4, D). The basic production process comprises of mixing of raw materials together. Ready mixed
product is then packed into small bags for delivery.
Floor screed doesn't require any maintenance during the use stage, so stage B is not considered. When building is demolished at the end-of-life, floor
structure with floor screed integrated into concrete slab are crushed. 90 % of crushed concrete is recycled and used to replace aggregates in concrete,
remaining 10% being disposed into landfill.
System boundaries (cradle-to-gate with options) are illustrated in the picture below
Additional technical information:
The consumption of the product is 1,7 kg / m² / mm.
The remaining powder and cured material may be disposed as construction waste to disposal or recycling.
NEPD-3166-1808-EN weberfloor 4650 Design Colour
4 / 8
LCA: Scenarios and additional technical information
The following information describe the scenarios in the different modules of the EPD.
Transport to market (A4) is calculated based on the default distance of 300 km from NPCR 011
Transport from production place to user (A4)
Capacity utilisation Fuel/Energy
Type Type of vehicle Distance km Unit Value (l/t)
(incl. return) % consumption
Truck 55,0 % Truck, lorry over 32 tonnes, EURO 5 300 0,022823 l/tkm 6,85
Railway l/tkm
Boat l/tkm
Other Transportation l/tkm
Additional A4 information Unit/Range Value
Multiplication factor
Lilleström, Norway (truck/truck to jobsite: 677 km) 1,65
GWP/A4
Multiplication factor
Karlslunde, Denmark (truck/truck to jobsite: 885 km) 2,02
GWP/A4
Multiplication factor
Helsinki, Finland (truck / roro boat / truck to jobsite: 952 km) 2,13
GWP/A4
Assembly (A5) End of Life (C1, C3, C4)
. Unit Value . Unit Value
Auxiliary kg Hazardous waste disposed kg
Water consumption m3 0,0002 Collected as mixed construction waste kg
Electricity consumption kWh 0,0015 Reuse kg
Other energy carriers MJ Recycling kg 0,9000
Material loss kg Energy recovery kg
Output materials from waste treatment kg 0,0305 To landfill kg 0,1000
Dust in the air kg
VOC emissions kg
Transport to waste processing (C2)
Capacity utilisation Fuel/Energy
Type Type of vehicle Distance km Unit Value (l/t)
(incl. return) % consumption
Truck 55,0 % Truck, lorry over 32 tonnes, EURO 5 50 0,022823 l/tkm 1,14
Railway l/tkm
Boat l/tkm
Other Transportation l/tkm
¨
Benefits and loads beyond the system boundaries (D)
. Unit Value
Substitution of primary aggregates with crushed recycled cement-based products (kg) kg/DU 0,90
NEPD-3166-1808-EN weberfloor 4650 Design Colour
5 / 8
LCA: Results
The LCA results are presented below for the declared unit defined on page 2 of the EPD document.
System boundaries (X=included, MND=module not declared, MNR=module not relevant)
Construction Beyond the
Product stage installation User stage End of life stage . system
stage bondaries
A1 A2 A3 A4 A5 B1 B2 B3 B4 B5 B6 B7 C1 C2 C3 C4 . D
X X X X X MNR MNR MNR MNR MNR MNR MNR X X X X . X
Environmental impact
Parameter Unit A1-A3 A4 A5 C1 C2 C3 C4 D
GWP kg CO 2 -eq 2,55E-01 2,62E-02 2,50E-03 3,96E-03 4,36E-03 2,50E-04 5,18E-04 -3,57E-03
ODP kg CFC11 -eq 1,64E-08 5,10E-09 2,05E-10 6,86E-10 8,50E-10 4,90E-11 1,72E-10 -4,62E-10
POCP kg C 2H 4-eq 5,25E-05 4,23E-06 2,75E-07 6,63E-07 7,05E-07 4,58E-08 1,58E-07 -9,30E-07
AP kg SO 2 -eq 6,79E-04 8,51E-05 6,98E-06 2,99E-05 1,42E-05 1,26E-06 3,78E-06 -2,07E-05
EP kg PO 3- -eq 1,66E-04 1,43E-05 1,80E-06 6,53E-06 2,38E-06 2,24E-07 6,67E-07 -3,67E-06
4
ADPM kg Sb -eq 1,94E-06 5,91E-08 3,02E-09 1,70E-11 9,85E-09 1,40E-11 1,00E-11 -1,91E-10
ADPE MJ 4,08E+00 4,11E-01 1,45E-02 5,47E-02 6,84E-02 2,43E-03 1,46E-02 -3,81E-02
GWP Global warming potential; ODP Depletion potential of the stratospheric ozone layer; POCP Formation potential of tropospheric photochemical oxidants;
AP Acidification potential of land and water; EP Eutrophication potential; ADPM Abiotic depletion potential for non fossil resources; ADPE Abiotic depletion
potential for fossil resources
"Reading example: 9,0 E-03 = 9,0*10-3 = 0,009"
*INA Indicator Not Assessed
waR slairetam tropsnarT gnirutcafunaM tropsnarT ylbmessA esU ecnanetniaM riapeR tnemecalpeR tnemhsibrufeR lanoitarepO ygrene esu lanoitarepO esu
retaw
-eD noitcurtsnoc noitilomed tropsnarT etsaW gnissecorp lasopsiD -yrevoceR-esueR -gnilcyceR laitnetop
NEPD-3166-1808-EN weberfloor 4650 Design Colour
6 / 8
Resource use
Parameter Unit A1-A3 A4 A5 C1 C2 C3 C4 D
RPEE MJ 1,01E+00 7,42E-03 3,51E-01 3,00E-04 1,24E-03 3,26E-03 1,19E-04 -1,28E-02
RPEM MJ 5,33E-01 0,00E+00 0,00E+00 0,00E+00 0,00E+00 0,00E+00 0,00E+00 0,00E+00
TPE MJ 1,54E+00 7,42E-03 3,51E-01 3,00E-04 1,24E-03 3,26E-03 1,19E-04 -1,28E-02
NRPE MJ 4,43E+00 4,23E-01 4,19E-02 5,52E-02 7,06E-02 6,36E-03 1,48E-02 -5,25E-02
NRPM MJ 3,19E-02 0,00E+00 0,00E+00 0,00E+00 0,00E+00 0,00E+00 0,00E+00 0,00E+00
TRPE MJ 4,47E+00 4,23E-01 4,19E-02 5,52E-02 7,06E-02 6,37E-03 1,48E-02 -5,25E-02
SM kg 4,52E-02 0,00E+00 0,00E+00 0,00E+00 0,00E+00 0,00E+00 0,00E+00 0,00E+00
RSF MJ 1,76E-02 0,00E+00 4,00E-06 0,00E+00 0,00E+00 0,00E+00 0,00E+00 0,00E+00
NRSF MJ 1,41E-01 0,00E+00 0,00E+00 0,00E+00 0,00E+00 0,00E+00 0,00E+00 0,00E+00
W m3 1,94E-03 9,98E-05 2,51E-04 4,75E-06 1,66E-05 1,60E-06 1,60E-05 -1,04E-03
RPEE Renewable primary energy resources used as energy carrier; RPEM Renewable primary energy resources used as raw materials; TPE Total use of renewable
primary energy resources; NRPE Non renewable primary energy resources used as energy carrier; NRPM Non renewable primary energy resources used as
materials; TRPE Total use of non renewable primary energy resources; SM Use of secondary materials; RSF Use of renewable secondary fuels; NRSF Use of non
renewable secondary fuels; W Use of net fresh water
"Reading example: 9,0 E-03 = 9,0*10-3 = 0,009"
*INA Indicator Not Assessed
End of life - Waste
Parameter Unit A1-A3 A4 A5 C1 C2 C3 C4 D
HW kg 8,64E-05 2,25E-07 2,57E-08 1,50E-07 3,75E-08 5,88E-09 2,20E-08 -2,10E-07
NHW kg 8,49E-02 3,84E-02 1,22E-03 2,50E-04 6,40E-03 7,18E-05 1,00E-01 -1,85E-03
RW kg INA* INA* INA* INA* INA* INA* INA* INA*
HW Hazardous waste disposed; NHW Non hazardous waste disposed; RW Radioactive waste disposed
"Reading example: 9,0 E-03 = 9,0*10-3 = 0,009"
*INA Indicator Not Assessed
End of life - Output flow
Parameter Unit A1-A3 A4 A5 C1 C2 C3 C4 D
CR kg 0,00E+00 0,00E+00 0,00E+00 0,00E+00 0,00E+00 0,00E+00 0,00E+00 0,00E+00
MR kg 6,74E-05 0,00E+00 5,99E-03 0,00E+00 0,00E+00 2,87E-01 0,00E+00 0,00E+00
MER kg 5,52E-03 0,00E+00 2,45E-02 0,00E+00 0,00E+00 0,00E+00 0,00E+00 0,00E+00
EEE MJ INA* INA* INA* INA* INA* INA* INA* INA*
ETE MJ INA* INA* INA* INA* INA* INA* INA* INA*
CR Components for reuse; MR Materials for recycling; MER Materials for energy recovery; EEE Exported electric energy; ETE Exported thermal energy
"Reading example: 9,0 E-03 = 9,0*10-3 = 0,009"
*INA Indicator Not Assessed
NEPD-3166-1808-EN weberfloor 4650 Design Colour
7 / 8
Additional Norwegian requirements
Greenhouse gas emissions from the use of electricity in the manufacturing phase
National production mix from import, low voltage (production of transmission lines, in addition to direct emissions and losses in grid) of applied electricity for
the manufacturing process (A3).
Electricity mix Data source Amount Unit
Renewable electricity with Guarantee of Origin from LOS (kWh) Modified ecoinvent 3.4 60,20 g CO2-ekv/kWh
Dangerous substances
The product contains no substances given by the REACH Candidate list or the Norwegian priority list.
Name CASNo Amount
Portland Cement 65997-15-1 2-5%
Indoor environment
The product meets the requirements for emissions by EMICODE.
Bibliography
ISO 14025:2010 Environmental labels and declarations - Type III environmental declarations - Principles and procedures.
ISO 14044:2006 Environmental management - Life cycle assessment - Requirements and guidelines.
EN 15804:2012+A1:2013 Environmental product declaration - Core rules for the product category of construction products.
ISO 21930:2017 Sustainability in buildings and civil engineering works. Core rules for environmental product declarations of construction products.
ecoinvent v3, Allocation, cut-off by classification, Swiss Centre of Life Cycle Inventories.
Iversen et al., (2018) eEPD v3.0 - Background information for EPD generator system, LCA.no report number 04.18
Iversen et al., (2019) EPD generator for Saint-Gobain Weber and Scanspac - Background information and LCA data, LCA.no report number 05.18
NPCR Part A: Construction products and services. Ver. 1.0. April 2017, EPD-Norge.
NPCR 009 Part B for technical-chemical products. Ver. 1.0 June 2018, EPD-Norge.
Program operator and publisher Phone: +47 23 08 80 00
The Norwegian EPD Foundation e-mail: post@epd-norge.no
Post Box 5250 Majorstuen, 0303 Oslo,Norway web: www.epd-norge.no
Owner of the declaration Phone: +46 8 625 6105
Saint-Gobain Sweden AB, Weber floor e-mail: anders.anderberg@weber.se
Box 415 SE-19162 Sollentuna web: www.weber.se
Author of the Life Cycle Assessment Phone: +47 916 50 916
LCA.no AS e-mail: post@lca.no
Dokka 1C 1671 Kråkerøy web: www.lca.no
Developer of EPD generator Phone: +47 916 50 916
LCA.no AS e-mail: post@lca.no
Dokka 1C,1671 Kråkerøy web: www.lca.no
NEPD-3166-1808-EN weberfloor 4650 Design Colour
8 / 8
