Environmental product declaration
in accordance with ISO 14025 and EN 15804+A2
Red Temperate
Owner of the declaration: Program operator:
Fritzøe Engros AS The Norwegian EPD Foundation
Product: Declaration number:
Red Temperate
NEPD-8647-8310
Declared unit:
1 m3 Registration number:
This declaration is based on Product Category Rules: NEPD-8647-8310
CEN Standard EN 15804:2012+A2:2019 serves as core
Issue date: 08.01.2025
PCR
The Norwegian EPD Foundation NPCR 010:2022 Part B for building boards Valid to: 08.01.2030
ver-040225
EPD software:
LCAno EPD generator ID:
518787
1 / 11
General information
Product Owner of the declaration:
Red Temperate Fritzøe Engros AS
Contact person: Jarle Anholt
Program operator:
The Norwegian EPD Foundation Phone: +47 331 364 00
Post Box 5250 Majorstuen, 0303 Oslo, Norway e-mail: engros@fritzoeengros.no
Phone: +47 977 22 020
Manufacturer:
web: www.epd-norge.no
Fritzøe Engros AS
Declaration number:
NEPD-8647-8310
Place of production:
This declaration is based on Product Category Rules: Fritzøe Engros AS
Øya 40
CEN Standard EN 15804:2012+A2:2019 serves as core PCR
NPCR 010:2022 Part B for building boards 3262 Larvik, Norway
Statement of liability: Management system:
The owner of the declaration shall be liable for the underlying Miljøfyrtårn, FSC og PEFC
information and evidence. EPD Norway shall not be liable with respect
to manufacturer information, life cycle assessment data and
Organisation no:
evidences.​
979 778 341
Declared unit:
1 m3 Red Temperate
Declared unit with option:
Issue date:
A1-A3,A4,A5,C1,C2,C3,C4,D
08.01.2025
Valid to:
08.01.2030
Functional unit:
Year of study:
2023
General information on verification of EPD from EPD tools: Comparability:
EPD of construction products may not be comparable if they not
Independent verification of data, other environmental information
and the declaration according to ISO 14025:2010, § 8.1.3 and § 8.1.4. comply with EN 15804 and seen in a building context.
Verification of each EPD is made according to EPD-Norway’s
Development and verification of EPD:
guidelines for verification and approval requiring that tools are i)
The declaration is created using EPD tool lca.tools ver EPD2022.03,
integrated into the company's environmental management system, ii)
developed by LCA.no. The EPD tool is integrated in the company's
the procedures for use of the EPD tool are approved by EPD-Norway,
management system, and has been approved by EPD Norway.
and iii) the process is reviewed annually by an independent third
party verifier. See Appendix G of EPD-Norway's General Programme
Developer of EPD: Terje Olsen
Instructions for further information on EPD tools
Reviewer of company-specific input data and EPD:​ Jarle Anholt
Verification of EPD tool:
Independent third party verification of the EPD tool, background data
and test-EPD in accordance with EPDNorway's procedures and
guidelines for verification and approval of EPD tools.
Approved:
Third party verifier:
Elisabet Amat, GREENIZE projects
(no signature required)
2 / 11
Product
Product description:
Red Temperate is produced from sustainable materials for permanent use in buildings and infrastructure. The panels are suitable for several
different areas of use within construction and areas of use, such as internal wall panels and external, but then as built into the construction.
Product specification
Materials kg %
Adhesive 116,00 20,10
Wood - Veneer 461,00 79,90
Total 577,00 100,00
Packaging kg %
Packaging - Metal 1,00 3,57
Packaging - Paper 2,00 7,14
Packaging - Wood 25,00 89,29
Total incl. packaging 605,00 100,00
Technical data:
Red Temperate plywood are marked with CE-marking containing unambiguous code of Declaration of Performance, i.e. 2010-CPR-090822
Thickness (mm) Length (mm) Width (mm) Volume (m3)
4 2440 1220 0,0119072
6 2440 1220 0,0178608
9 2440 1220 0,0267912
12 2440 1220 0,0357216
15 2440 1220 0,044652
18 2440 1220 0,0535824
22 2440 1220 0,0654896
Market:
Nordic countries.
Reference service life, product
30 years
Reference service life, building or construction works
Not Declared.
LCA: Calculation rules
Declared unit:
1 m3 Red Temperate
Cut-off criteria:
All major raw materials and all the essential energy is included. The production processes for raw materials and energy flows with very small
amounts (less than 1%) are not included when specific information are missing. These cut-off criteria do not apply for hazardous materials and
substances.
Allocation:
The allocation is made in accordance with the provisions of EN 15804. Incoming energy and water and waste production in-house is allocated
equally among all products through mass allocation. Effects of primary production of recycled materials is allocated to the main product in which
the material was used. The recycling process and transportation of the material is allocated to this analysis.
Data quality:
Specific data for the product composition are provided by the manufacturer. The data represent the production of the declared product and were
collected for EPD development in the year of study. Background data is based on EPDs according to EN 15804 and different LCA databases. The
data quality of the raw materials in A1 is presented in the table below.
Materials Source Data quality Year
Packaging - Paper ecoinvent 3.6 Database 2019
Adhesive ecoinvent 3.9.1 Database 2021
Wood - Veneer Modified ecoinvent 3.6 Database 2019
Packaging - Wood ecoinvent 3.6 Database 2019
Packaging - Metal ecoinvent 3.6 Database 2019
3 / 11
System boundaries (X=included, MND=module not declared, MNR=module not relevant)
Construction Beyond the system
Product stage Use stage End of life stage
installation stage boundaries
A1 A2 A3 A4 A5 B1 B2 B3 B4 B5 B6 B7 C1 C2 C3 C4 D
X X X X X MND MND MND MND MND MND MND X X X X X
System boundary:
Figure 1. System diagram.
Module A1 includes the production of raw materials and energy used in the manufacturing of the plywood products. Popular logs are sourced
from China and Eucalyptus is sourced from Uruguay according to mill locations.
Module A2 comprises of transportation processes up to the plywood mill gates. Most of the materials are shipped to the mills by road and few
materials are also shipped by sea.
Module A3 includes the direct emissions of the manufacturing processes at the plywood mills, production of auxiliary and packaging materials,
treatment of solid wastes and pre-treatment of wastewater. Plywood manufacturing process is depicted in Figure 1.
Additional technical information:
Certification and environmental information:
FSC-STD-40-004 V3-1; FSC-STD-50-001 V2-0
Miljøfyrtårn-10745
waR slairetam tropsnarT gnirutcafunaM tropsnarT ylbmessA e​sU ecnanetniaM riapeR tnemecalpeR tnemhsibrufeR lanoitarepO ygrene esu lanoitarepO esu retaw -eD noitcurtsnoc noitilomed tropsnarT etsaW gnissecorp lasopsiD -yrevoceR-esueR laitnetop-gnilcyceR
4 / 11
LCA: Scenarios and additional technical information
The following information describe the scenarios in the different modules of the EPD.
A5: manual instalment, so no energy inputs have been included.
C2: generic transport for Norwegian market between building site and waste treatment.
Capacity utilisation Value
Transport from production place to user (A4) Distance (km) Fuel/Energy Consumption Unit
(incl. return) % (Liter/tonne)
Truck, 16-32 tonnes, EURO 6 (km) - Europe 36,7 % 300 0,043 l/tkm 12,90
Assembly (A5) Unit Value
Product waste during installation (DU) Units/DU 0,050
Waste, metal, to average treatment (kg) kg 1,000000000000000000
Waste, packaging, pallet, to average treatment
kg 25,000000000000000000
(kg)
Waste, packaging, paper, to average treatment
kg 2,000000000000000000
(kg)
De-construction demolition (C1) Unit Value
Demolition of building per kg of building board
MJ/DU 577,000000000
(kg)
Capacity utilisation Value
Transport to waste processing (C2) Distance (km) Fuel/Energy Consumption Unit
(incl. return) % (Liter/tonne)
Truck, 16-32 tonnes, EURO 6 (km) - Europe 36,7 % 85 0,043 l/tkm 3,66
Waste processing (C3) Unit Value
Waste treatment per kg Hazardous waste,
kg 116,000000000000000000
incineration (kg)
Waste treatment per kg Wood, incineration with
kg 461,000000000000000000
fly ash extraction (kg)
Disposal (C4) Unit Value
Landfilling of ashes from incineration of
kg 21,92
Hazardous waste, from incineration (kg)
Landfilling of ashes from incineration of Wood,
kg 5,30
process per kg ashes and residues (kg)
Benefits and loads beyond the system
Unit Value
boundaries (D)
Substitution of electricity (MJ) MJ 338,099
Substitution of thermal energy, district heating
MJ 5115,11
(MJ)
5 / 11
LCA: Results
The LCA results are presented below for the declared unit defined on page 2 of the EPD document.
Environmental impact
Indicator Unit A1-A3 A4 A5 C1 C2 C3 C4 D
GWP-total kg CO2 -eq -3,94E+01 2,97E+01 8,67E+01 1,90E+00 8,41E+00 1,03E+03 9,81E+00 -3,07E+01
GWP-fossil kg CO2 -eq 7,57E+02 2,96E+01 4,68E+01 1,90E+00 8,40E+00 2,63E+02 9,81E+00 -2,97E+01
GWP-biogenic kg CO2 -eq -7,98E+02 1,23E-02 3,99E+01 3,56E-04 3,48E-03 7,69E+02 3,92E-03 -6,12E-02
GWP-luluc kg CO2 -eq 1,42E+00 1,06E-02 2,00E-02 1,49E-04 2,99E-03 6,58E-02 9,59E-04 -1,02E+00
ODP kg CFC11 -eq 7,16E-05 6,72E-06 -1,08E-01 4,10E-07 1,90E-06 2,99E-05 4,91E-07 -2,16E+00
AP mol H+ -eq 8,09E+00 8,52E-02 2,35E-01 1,98E-02 2,41E-02 4,50E-01 1,98E-02 -2,44E-01
EP-FreshWater kg P -eq 1,04E-01 2,37E-04 5,37E-03 6,91E-06 6,71E-05 6,27E-03 9,58E-05 -2,64E-03
EP-Marine kg N -eq 1,96E+00 1,69E-02 5,61E-02 8,76E-03 4,78E-03 1,13E-01 5,19E-03 -7,99E-02
EP-Terrestial mol N -eq 2,25E+01 1,89E-01 6,62E-01 9,61E-02 5,34E-02 1,25E+00 6,07E-02 -8,64E-01
POCP kg NMVOC -eq 5,81E+00 7,22E-02 1,72E-01 2,64E-02 2,05E-02 3,37E-01 1,69E-02 -2,38E-01
ADP-minerals&metals1 kg Sb-eq 1,30E-02 8,19E-04 7,04E-04 2,91E-06 2,32E-04 9,21E-04 1,77E-05 -2,95E-04
ADP-fossil1 MJ 1,05E+04 4,48E+02 5,23E+02 2,61E+01 1,27E+02 1,12E+03 4,69E+01 -4,24E+02
WDP1 m3 3,70E+03 4,34E+02 1,92E+02 5,55E+00 1,23E+02 4,11E+03 1,17E+03 -5,28E+03
GWP-total = Global Warming Potential total; GWP-fossil = Global Warming Potential fossil fuels; GWP-biogenic = Global Warming Potential biogenic; GWP-luluc =
Global Warming Potential land use and land use change; ODP = Depletion potential of the stratospheric ozone layer; AP = Acidification potential, Accumulated
Exceedance; EP-freshwater = Eutrophication potential, fraction of nutrients reaching freshwater end compartment: EP-marine = Eutrophication potential, fraction of
nutrients reaching marine end compartment; EP-terrestrial = Eutrophication potential, Accumulated Exceedance; POCP = Formation potential of tropospheric ozone;
ADP-minerals&metals = Abiotic depletion potential for non-fossil resources; ADP-fossil = Abiotic depletion for fossil resources potential; WDP = Water (user)
deprivation potential, deprivation-weighted water consumption
"Reading example: 9,0 E-03 = 9,0*10-3 = 0,009"
*INA Indicator Not Assessed
1. The results of this environmental impact indicator shall be used with care as the uncertainties on these results are high or as there is limited experienced with the
indicator
Remarks to environmental impacts
6 / 11
Additional environmental impact indicators
Indicator Unit A1-A3 A4 A5 C1 C2 C3 C4 D
PM Disease incidence 1,88E-04 1,82E-06 9,21E-06 5,25E-07 5,14E-07 6,55E-06 1,39E-07 -1,48E-05
IRP2 kgBq U235 -eq 2,88E+01 1,96E+00 1,40E+00 1,12E-01 5,55E-01 5,00E+00 2,59E-01 -2,71E+00
ETP-fw1 CTUe 2,36E+04 3,32E+02 1,32E+03 1,43E+01 9,41E+01 5,32E+03 1,34E+02 -2,31E+03
HTP-c1 CTUh 1,00E-06 0,00E+00 6,25E-08 5,77E-10 0,00E+00 2,63E-07 7,14E-09 -4,22E-08
HTP-nc1 CTUh 9,34E-06 3,63E-07 5,57E-07 1,33E-08 1,03E-07 2,30E-06 2,62E-07 -2,21E-06
SQP1 dimensionless 1,57E+05 3,14E+02 7,77E+03 3,31E+00 8,88E+01 4,32E+02 1,34E+02 -2,84E+03
PM = Particulate Matter emissions; IRP = Ionizing radiation – human health; ETP-fw = Eco toxicity – freshwater; HTP-c = Human toxicity – cancer effects; HTP-nc =
Human toxicity – non cancer effects; SQP = Potential Soil Quality Index (dimensionless)
"Reading example: 9,0 E-03 = 9,0*10-3 = 0,009"
*INA Indicator Not Assessed
1. The results of this environmental impact indicator shall be used with care as the uncertainties on these results are high or as there is limited experienced with the
indicator
2. This impact category deals mainly with the eventual impact of low dose ionizing radiation on human health of the nuclear fuel cycle. It does not consider effects due
to possible nuclear accidents, occupational exposure nor due to radioactive waste disposal in underground facilities. Potential ionizing radiation from the soil, from
radon and from some construction materials is also not measured by this indicator.
7 / 11
Resource use
Indicator Unit A1-A3 A4 A5 C1 C2 C3 C4 D
PERE MJ 2,08E+04 6,42E+00 9,17E+02 1,41E-01 1,82E+00 1,96E+02 5,61E+00 -2,62E+03
PERM MJ 6,82E+03 0,00E+00 -3,56E+02 0,00E+00 0,00E+00 -6,45E+03 0,00E+00 0,00E+00
PERT MJ 2,76E+04 6,42E+00 5,61E+02 1,41E-01 1,82E+00 -6,25E+03 5,61E+00 -2,62E+03
PENRE MJ 1,05E+04 4,48E+02 5,24E+02 2,61E+01 1,27E+02 1,12E+03 4,69E+01 -4,24E+02
PENRM MJ 0,00E+00 0,00E+00 0,00E+00 0,00E+00 0,00E+00 0,00E+00 0,00E+00 0,00E+00
PENRT MJ 1,05E+04 4,48E+02 5,24E+02 2,61E+01 1,27E+02 1,12E+03 4,69E+01 -4,24E+02
SM kg 6,53E-01 0,00E+00 3,27E-02 0,00E+00 0,00E+00 0,00E+00 0,00E+00 0,00E+00
RSF MJ 3,82E+00 2,30E-01 3,96E-01 3,47E-03 6,50E-02 4,33E+00 1,03E-01 -4,59E-01
NRSF MJ 4,32E+00 8,21E-01 -7,48E+00 5,11E-02 2,33E-01 0,00E+00 2,62E+00 -1,55E+02
FW m3 1,34E+01 4,79E-02 5,64E-01 1,34E-03 1,36E-02 1,09E+00 8,15E-02 -3,15E+00
PERE = Use of renewable primary energy excluding renewable primary energy resources used as raw materials; PERM = Use of renewable primary energy resources used
as raw materials; PERT = Total use of renewable primary energy resources; PENRE = Use of non renewable primary energy excluding non-renewable primary energy
resources used as raw materials; PENRM = Use of non renewable primary energy resources used as raw materials; PENRT = Total use of non renewable primary energy
resources; SM = Use of secondary materials; RSF = Use of renewable secondary fuels; NRSF = Use of non-renewable secondary fuels; FW = Net use of fresh water
"Reading example: 9,0 E-03 = 9,0*10-3 = 0,009"
*INA Indicator Not Assessed
8 / 11
End of life - Waste
Indicator Unit A1-A3 A4 A5 C1 C2 C3 C4 D
HWD kg 6,42E+00 2,31E-02 5,09E-01 7,68E-04 6,55E-03 0,00E+00 3,85E+00 -1,99E-02
NHWD kg 8,99E+01 2,18E+01 4,02E+01 3,09E-02 6,18E+00 1,16E+02 2,34E+01 -1,00E+01
RWD kg 2,81E-02 3,05E-03 9,71E-04 1,81E-04 8,65E-04 0,00E+00 1,11E-05 -2,22E-03
HWD = Hazardous waste disposed; NHWD = Non-hazardous waste disposed; RWD = Radioactive waste disposed
"Reading example: 9,0 E-03 = 9,0*10-3 = 0,009"
*INA Indicator Not Assessed
End of life - Output flow
Indicator Unit A1-A3 A4 A5 C1 C2 C3 C4 D
CRU kg 0,00E+00 0,00E+00 0,00E+00 0,00E+00 0,00E+00 0,00E+00 0,00E+00 0,00E+00
MFR kg 3,47E+00 0,00E+00 3,02E+00 0,00E+00 0,00E+00 0,00E+00 0,00E+00 0,00E+00
MER kg 9,65E+00 0,00E+00 5,42E+01 0,00E+00 0,00E+00 5,77E+02 0,00E+00 0,00E+00
EEE MJ 6,33E+00 0,00E+00 3,37E+01 0,00E+00 0,00E+00 3,21E+02 0,00E+00 0,00E+00
EET MJ 9,57E+01 0,00E+00 5,10E+02 0,00E+00 0,00E+00 4,85E+03 0,00E+00 0,00E+00
CRU = Components for re-use; MFR = Materials for recycling; MER = Materials for energy recovery; EEE = Exported energy electrical; EET = Exported energy thermal
"Reading example: 9,0 E-03 = 9,0*10-3 = 0,009"
*INA Indicator Not Assessed
Biogenic Carbon Content
Indicator Unit At the factory gate
Biogenic carbon content in product kg C 2,10E+02
Biogenic carbon content in accompanying packaging kg C 1,13E+01
Note: 1 kg biogenic carbon is equivalent to 44/12 kg CO2
9 / 11
Additional requirements
Greenhouse gas emissions from the use of electricity in the manufacturing phase
National production mix from import, low voltage (production of transmission lines, in addition to direct emissions and losses in grid) of applied
electricity for the manufacturing process (A3).
Electricity mix Source Amount Unit
Electricity, Norway (kWh) ecoinvent 3.6 24,33 g CO2-eq/kWh
Dangerous substances
The product contains no substances given by the REACH Candidate list.
Indoor environment
The product has no influence on the indoor climate. No tests have been conducted.
Additional Environmental Information
Additional environmental impact indicators required in NPCR Part A for construction products
Indicator Unit A1-A3 A4 A5 C1 C2 C3 C4 D
GWPIOBC kg CO2 -eq 7,68E+02 2,97E+01 4,73E+01 1,88E+00 8,41E+00 2,63E+02 9,82E+00 -3,03E+01
GWP-IOBC: Global warming potential calculated according to the principle of instantaneous oxidation. In order to increase the transparency of biogenic carbon​
contribution to climate impact, the indicator GWP-IOBC is required as it declares climate impacts calculated according to the principle of instantaneous oxidation.​
GWP-IOBC is also referred to as GWP-GHG in context to Swedish public procurement legislation.
10 / 11
Bibliography
ISO 14025:2010 Environmental labels and declarations - Type III environmental declarations - Principles and procedures.
ISO 14044:2006 Environmental management - Life cycle assessment - Requirements and guidelines.
EN 15804:2012+A2:2019 Environmental product declaration - Core rules for the product category of construction products.
ISO 21930:2017 Sustainability in buildings and civil engineering works - Core rules for environmental product declarations of construction
products.
ecoinvent v3, Allocation, cut-off by classification, Swiss Centre of Life Cycle Inventories.
Iversen et al., (2021) eEPD v2021.09 Background information for EPD generator tool system verification, LCA.no Report number: 07.21
Vold, M. et al. (2022) EPD generator for Building boards
Background information for EPD generator application and LCA data, LCA.no report number 05.22
NPCR Part A: Construction products and services. Ver. 2.0. April 2021, EPD-Norge.
NPCR 010 Part B for Building Boards. Ver. 4.0, March 2022, EPD-Norge.
Program operator and publisher Phone: +47 977 22 020
The Norwegian EPD Foundation e-mail: post@epd-norge.no
Post Box 5250 Majorstuen, 0303 Oslo, Norway web: www.epd-norge.no
Owner of the declaration: Phone: +47 331 364 00
Fritzøe Engros AS e-mail: engros@fritzoeengros.no
Øya 40, 3262 Larvik, Norway web: https://www.fritzoeengros.no/
Author of the Life Cycle Assessment Phone: +47 916 50 916
LCA.no AS e-mail: post@lca.no
Dokka 6A, 1671 Kråkerøy, Norway web: www.lca.no
Developer of EPD generator Phone: +47 916 50 916
LCA.no AS e-mail: post@lca.no
Dokka 6A, 1671 Kråkerøy, Norway web: www.lca.no
ECO Platform web: www.eco-platform.org
ECO Portal web: ECO Portal
11 / 11
