Environmental product declaration
In accordance with 14025 and EN15804+A2
ArcelorMittal Promirock N 300 mm
Owner of the declaration: Program operator:
ArcelorMittal Construction Norge AS The Norwegian EPD Foundation
Product: Declaration number:
ArcelorMittal Promirock N 300 mm
NEPD-4327-3561-EN
Declared unit:
Registration number:
1 m2
NEPD-4327-3561-EN
This declaration is based on Product Category Rules:
CEN Standard EN 15804:2012+A2:2019 serves as core Issue date: 03.04.2023
PCR
The Norwegian EPD Foundation Valid to: 03.04.2028
NPCR 013:2021 Part B for Steel and aluminium
construction products
EPD Software:
LCA.no EPD generator ID: 56794
1 / 12
General information
Product Owner of the declaration:
ArcelorMittal Promirock N 300 mm ArcelorMittal Construction Norge AS
Contact person: Stig Tore Sjaastad
Phone: +47 41 723939
e-mail: stig-tore.sjaastad@arcelormittal.com
Program operator: Manufacturer:
Post Box 5250 Majorstuen, 0303 Oslo, Norway ArcelorMittal Construction Norge AS
The Norwegian EPD Foundation Sørumgata 11A
Phone: +47 23 08 80 00 2000 Lillestrøm, Norway
web: post@epd-norge.no
Declaration number: NEPD-4327-3561-EN Place of production:
ArcelorMittal Construction Sverige AB - Kungshamn
Televerksvägen 5
456 33 Kungshamn, Sweden
This declaration is based on Product Category Rules: Management system:
CEN Standard EN 15804:2012+A2:2019 serves as core PCR ISO 9001, ISO 14001, ISO 45001
NPCR 013:2021 Part B for Steel and aluminium construction products
Statement of liability: Organisation no:
The owner of the declaration shall be liable for the underlying 976289862
information and evidence. EPD Norway shall not be liable with respect
to manufacturer information, life cycle assessment data and
evidences.​
Declared unit: Issue date: 03.04.2023
1 m2 ArcelorMittal Promirock N 300 mm
Declared unit with option: Valid to: 03.04.2028
A1-A3,A4,A5,C1,C2,C3,C4,D
Year of study:
2022
Comparability:
Functional unit: EPD of construction products may not be comparable if they not
comply with EN 15804 and seen in a building context.
Development and verification of EPD:
General information on verification of EPD from EPD tools: The declaration is created using EPD tool lca.tools ver EPD2022.03,
developed by LCA.no. The EPD tool is integrated in the company's
Independent verification of data, other environmental information
and the declaration according to ISO 14025:2010, § 8.1.3 and § 8.1.4. management system, and has been approved by EPD Norway.
Individual third party verification of each EPD is not required when
Developer of EPD: Stig Tore Sjaastad
the EPD tool is i) integrated into the company's environmental
management system, ii) the procedures for use of the EPD tool are Reviewer of company-specific input data and EPD: Bendik Hovde
approved by EPDNorway, and iii) the proccess is reviewed annualy.
​
See Appendix G of EPD-Norway's General Programme Instructions
for further information on EPD tools.
Approved:
Verification of EPD tool:
Independent third party verification of the EPD tool, background data
and test-EPD in accordance with EPDNorway's procedures and
guidelines for verification and approval of EPD tools.
Third party verifier:
Alexander Borg, Asplan Viak AS
(no signature required)
2 / 12
Product
Product description:
Promirock N from ArcelorMittal Construction Sverige AB is a double skin, organic coated steel faced sandwich panel solution with a core of mineral
wool. The EPD contains several different panel types: Promirock N85 and Promirock N125. Promirock N sandwich panels can be used for facades,
inner walls / partition walls and ceiling applications in buildings, such as industrial, warehouse, commercial or sports facilities. With a wide choice of
coatings the panels
even can be used for food industry application and buildings with high demand for cleanliness.
Product specification
Promirock N double skin steel faced sandwich panels consists of a profiled internal and external face made of a steel core according to EN 10346,
Steel grade from S280 GD to S350 GD, which is protected against corrosion with Zinc or Zinc-Magnesium and organic coatings (Polyester or
equivalent coating).
The thermal insulating core material is made of mineral wool according to EN 13162 with sealing tapes and is bonded with a non-combustible
adhesive according to EN 13501-1 to both sides of the steel sheets.
Promirock N sandwich panels are manufactured in different thicknesses between 100-300mm in two different mineral wool densities.
Promirock N sandwich panels can be used as normal or fire-resistant facade, inner walls / partition walls and ceiling applications.
The products are wrapped to protect them during handling and
Packaging
A typical bundle with sandwich panels consists of EPS spacer, honeycomb cardboard, a plastic wrapping foil and corner pads made of cardboard if
required. Sandwich panel facings are protected with a plastic
strip foil (PE) to protect the steel facings from mechanical damage during loading, unloading, storage and installation.
Packaging material is recycable or alternatively utilised as waste to energy. Packaging materials are sorted at construction sites according to local
regulations by the customer.
Materials kg %
Binders and Resins 0,38 1,09
Insulation - stone wool 25,50 73,09
Metal - Steel 9,01 25,82
Total 34,89
Packaging kg %
Packaging - Paper 0,46 52,88
Packaging - Plastic 0,28 32,60
Packaging - Polystyrene 0,13 14,52
Total incl. packaging 35,76
Technical data:
Promirock N sandwich panels fulfills the requirement of the harmonized standard EN 14509 and EN 13162.
Market:
The products are used for structural, self-supporting and non-supporting applications in roof, wall and
ceiling structures.
Sandwich panels in wall and roof applications take on tasks of the building physics, especially sound, heat
and moisture safety. They simultaneously perform the function of air tightness of the building envelope.
Reference service life, product
Double skin steel faced sandwich panels used in lightweight metal constructions must withstand a term
of protection of at least 15 years. The term of protection is the period until first slight renewals in the
surface are required, only if there is no need of frequent inspections and service.
The term of protection depends on the location,
weather conditions and the quality of the coating.
Reference service life, building or construction works
Double skin steel faced sandwich panels exhibit an estimated service life of 40 – 45 years depending on
the use conditions, according to the /BBSR table/.
LCA: Calculation rules
Declared unit:
1 m2 ArcelorMittal Promirock N 300 mm
Cut-off criteria:
All major raw materials and all the essential energy is included. The production processes for raw materials and energy flows with very small
amounts (less than 1%) are not included. These cut-off criteria do not​ apply for hazardous materials and substances.
Allocation:
3 / 12
The allocation is made in accordance with the provisions of EN 15804. Incoming energy and water and waste production in-house is allocated
equally among all products through mass allocation. Effects of primary production of recycled materials is allocated to the main product in which
the material was used. The recycling process and transportation of the material is allocated to this analysis.
Data quality:
Specific data for the product composition are provided by the manufacturer. The data represent the production of the declared product and were
collected for EPD development in the year of study. Background data is based on EPDs according to EN 15804 and different LCA databases. The
data quality of the raw materials in A1 is presented in the table below.
Materials Source Data quality Year
Packaging - Paper ecoinvent 3.6 Database 2019
Packaging - Plastic ecoinvent 3.6 Database 2019
Packaging - Polystyrene ecoinvent 3.6 Database 2019
Binders and Resins EPD-FEI-20220107-IBG1-EN EPD 2022
EPD
(EN15804A1) +
Metal - Steel Supplier company 2020
dataset
(EN15804A2)
Insulation - stone wool Supplier Specific 2022
4 / 12
System boundaries (X=included, MND=module not declared, MNR=module not relevant)
Construction Beyond the system
Product stage Use stage End of life stage
installation stage boundaries
A1 A2 A3 A4 A5 B1 B2 B3 B4 B5 B6 B7 C1 C2 C3 C4 D
X X X X X MND MND MND MND MND MND MND X X X X X
System boundary:
Type of EPD: cradle to gate - with options. All relevant life cycle stages are covered.
The product stage A1-A3 include the following:
•Transporting and Receiving the raw material to the fabrication plant
•All relevant production processes in the plant including energy inputs, emissions and the electricity consumptions
•Waste processing until end of waste state or disposal of any waste residues during the production of the sandwich panels. For the mineral wool a
used product take-back system is agreed with the supplier, which enable the recycling of old stone wool slabs, wool dust, boards and cut-offs.
Sandwich panel steel sheet is a fully recyclable material and scrap steel has a strong market position and can be re-used
•Production and recycling of packaging
•Manufacturing of the sandwich panel products
The construction installation stage A4-A5 include the following:
•For the transport to the construction site an assumption of an average truck trailer of 16-32 tonnes payload has been taken into consideration.
Transport distance of the finished product to the customer has been estimated with approximate 300km. All values are based on annual average
delivery data
•For the assembly stage average values been taken. Accessories, such as fasteners, sealing materials and flashings, used in the phase A5 to
complete the installation of the sandwich panels are not included in the life cycle assessment
The end of life stage C1-C4 include the following:
•Stages C1-C4 include average assumptions, provision for all materials and transports, and use of related energy and water
•Assumption is made that the sandwich panels will be disposed 100% to landfill
•The Steel is fully recyclable in form of scrap by separating the steel sheets from the insulation core
•Packaging waste is recycled by the customers through their waste management system and cardboards can be re-used or recycled
The use stage B1-B7 have not been included. In addition, module D (Beyond the system boundaries) is included.
Additional technical information:
waR slairetam tropsnarT gnirutcafunaM tropsnarT ylbmessA e​sU ecnanetniaM riapeR tnemecalpeR tnemhsibrufeR lanoitarepO ygrene esu lanoitarepO esu retaw -eD noitcurtsnoc noitilomed tropsnarT etsaW gnissecorp lasopsiD -yrevoceR-esueR laitnetop-gnilcyceR
5 / 12
LCA: Scenarios and additional technical information
The following information describe the scenarios in the different modules of the EPD.
Capacity utilisation Value
Transport from production place to user (A4) Distance (km) Fuel/Energy Consumption Unit
(incl. return) % (Liter/tonne)
Truck, 16-32 tonnes, HVO, EURO 6 (kgkm) - RER 36,7 % 300 0,043 l/tkm 12,90
Assembly (A5) Unit Value
Waste, municipal solid waste, to average
kg 0,13
treatment - A3, A5, inkl. transp. (kg)
Waste, packaging, paper printed, to average
kg 0,46
treatment - A5, inkl. transp. (kg)
Waste, plastic, mixture, to average treatment - A5,
kg 0,28
inkl. transp. (kg)
De-construction demolition (C1) Unit Value
Demolition of building per kg of steel, C1 (kg) kg/DU 18,61
Capacity utilisation Value
Transport to waste processing (C2) Distance (km) Fuel/Energy Consumption Unit
(incl. return) % (Liter/tonne)
Truck, 16-32 tonnes, EURO 6 (km) 36,7 % 80 0,043 l/tkm 3,44
Waste processing (C3) Unit Value
Materials to recycling (kg) kg 8,11
Disposal (C4) Unit Value
Waste, inert waste, to landfill (kg) kg 25,88
Waste, scrap steel, to landfill (kg) kg 0,90
Benefits and loads beyond the system
Unit Value
boundaries (D)
Substitution of primary steel with net scrap (kg) kg 6,31
6 / 12
LCA: Results
The LCA results are presented below for the declared unit defined on page 2 of the EPD document.
Environmental impact
Indicator Unit A1-A3 A4 A5 C1 C2 C3 C4 D
GWP-total kg CO2 -eq 4,23E+01 4,17E-01 8,96E-01 7,44E-02 4,68E-01 0,00E+00 2,16E-01 -6,95E+00
GWP-fossil kg CO2 -eq 4,47E+01 4,16E-01 8,94E-02 7,44E-02 4,67E-01 0,00E+00 2,16E-01 -6,94E+00
GWP-biogenic kg CO2 -eq -2,41E+00 7,05E-04 8,06E-01 1,40E-05 1,93E-04 0,00E+00 2,51E-04 -3,83E-03
GWP-luluc kg CO2 -eq 4,14E-02 6,49E-04 5,73E-06 5,87E-06 1,66E-04 0,00E+00 5,29E-05 -3,11E-03
ODP kg CFC11 -eq 3,95E-07 8,58E-08 3,83E-09 1,61E-08 1,06E-07 0,00E+00 8,22E-08 -2,20E-07
AP mol H+ -eq 2,18E-01 2,92E-03 1,06E-04 7,79E-04 1,34E-03 0,00E+00 1,93E-03 -3,45E-02
EP-FreshWater kg P -eq 3,89E-04 1,53E-05 2,64E-07 2,71E-07 3,73E-06 0,00E+00 2,44E-06 -4,27E-04
EP-Marine kg N -eq 3,82E-02 7,72E-04 7,45E-05 3,44E-04 2,66E-04 0,00E+00 7,16E-04 -7,14E-03
EP-Terrestial mol N -eq 7,17E-01 8,63E-03 4,05E-04 3,72E-03 2,97E-03 0,00E+00 7,90E-03 -7,30E-02
POCP kg NMVOC -eq 1,04E-01 3,16E-03 1,19E-04 1,04E-03 1,14E-03 0,00E+00 2,26E-03 -3,48E-02
ADP-minerals&metals1 kg Sb -eq 1,73E-03 5,06E-05 3,82E-07 1,14E-07 1,29E-05 0,00E+00 1,95E-06 -1,20E-04
ADP-fossil1 MJ 6,03E+02 8,81E+00 2,63E-01 1,02E+00 7,06E+00 0,00E+00 5,97E+00 -5,84E+01
WDP1 m3 1,32E+03 2,61E+01 6,99E-01 2,18E-01 6,83E+00 0,00E+00 3,63E+01 3,60E+02
GWP total Global Warming Potential total; GWP fossil Global Warming Potential fossil fuels; GWP biogenic Global Warming Potential biogenic; GWP luluc Global W
Potential land use change; ODP Ozone Depletion; AP Acidification; EP freshwater Eutrophication aquatic freshwater; EP marine Eutrophication aquatic marine; EP
terrestrial Eutrophication terrestrial ;POCP Photochemical zone formation; ADPE Abiotic Depletion Potential minerals and metals; ADPf Abiotic Depletion Potential fossil
fuels;
"Reading example: 9,0 E-03 = 9,0*10-3 = 0,009"
*INA Indicator Not Assessed
1. The results of this environmental impact indicator shall be used with care as the uncertainties on these results are high or as there is limited experienced with the
indicator
Remarks to environmental impacts
7 / 12
Additional environmental impact indicators
Indicator Unit A1-A3 A4 A5 C1 C2 C3 C4 D
PM Disease incidence 2,11E-06 9,65E-08 1,45E-09 9,43E-08 2,86E-08 0,00E+00 4,11E-08 -5,76E-07
IRP2 kgBq U235 -eq 1,48E+00 2,88E-02 1,10E-03 4,47E-03 3,09E-02 0,00E+00 2,72E-02 2,49E-02
ETP-fw1 CTUe 1,86E+02 1,29E+01 5,42E-01 5,60E-01 5,24E+00 0,00E+00 3,25E+00 -3,87E+02
HTP-c1 CTUh 2,52E-08 0,00E+00 2,30E-11 1,90E-11 0,00E+00 0,00E+00 1,32E-10 -3,34E-08
HTP-nc1 CTUh 3,37E-07 2,15E-08 8,54E-10 5,21E-10 5,72E-09 0,00E+00 2,34E-09 7,26E-07
SQP1 dimensionless 4,88E+02 1,64E+01 2,85E-01 1,25E-01 4,94E+00 0,00E+00 2,29E+01 -4,37E+00
PM Particulate Matter emissions; IRP Ionizing radiation – human health; ETP-fw Eco toxicity – freshwater; HTP-c Human toxicity – cancer effects; HTP-nc Human
toxicity – non cancer effects; SQP Soil Quality (dimensionless)
"Reading example: 9,0 E-03 = 9,0*10-3 = 0,009"
*INA Indicator Not Assessed
1. The results of this environmental impact indicator shall be used with care as the uncertainties on these results are high or as there is limited experienced with the
indicator
2. This impact category deals mainly with the eventual impact of low dose ionizing radiation on human health of the nuclear fuel cycle. It does not consider effects due
to possible nuclear accidents, occupational exposure nor due to radioactive waste disposal in underground facilities. Potential ionizing radiation from the soil, from
radon and from some construction materials is also not measured by this indicator.
8 / 12
Resource use
Indicator Unit A1-A3 A4 A5 C1 C2 C3 C4 D
PERE MJ 1,99E+02 3,99E-01 6,17E-03 5,58E-03 1,01E-01 0,00E+00 2,11E-01 -4,74E+00
PERM MJ 6,76E+00 0,00E+00 -6,48E+00 0,00E+00 0,00E+00 0,00E+00 0,00E+00 0,00E+00
PERT MJ 2,28E+02 3,99E-01 -6,47E+00 5,58E-03 1,01E-01 0,00E+00 2,11E-01 -4,74E+00
PENRE MJ 2,44E+02 8,81E+00 2,63E-01 1,02E+00 7,07E+00 0,00E+00 5,97E+00 -5,84E+01
PENRM MJ 4,07E+01 0,00E+00 -4,87E+00 0,00E+00 0,00E+00 0,00E+00 0,00E+00 0,00E+00
PENRT MJ 6,03E+02 8,81E+00 -4,61E+00 1,02E+00 7,07E+00 0,00E+00 5,97E+00 -5,84E+01
SM kg 2,08E+00 0,00E+00 1,23E-03 5,03E-04 0,00E+00 0,00E+00 2,57E-03 3,28E+00
RSF MJ 1,37E-01 1,30E-02 1,82E-04 1,36E-04 3,62E-03 0,00E+00 4,38E-03 2,51E-01
NRSF MJ 9,79E-02 4,47E-02 6,51E-04 -2,05E-03 1,29E-02 0,00E+00 9,49E-03 7,30E+00
FW m3 4,00E-01 3,60E-03 2,34E-04 5,27E-05 7,56E-04 0,00E+00 7,34E-03 -1,46E-02
PERE Use of renewable primary energy excluding renewable primary energy resources used as raw materials; PERM Use of renewable primary energy resources used as
raw materials; PERT Total use of renewable primary energy resources; PENRE Use of non renewable primary energy excluding non-renewable primary energy resources
used as raw materials; PENRM Use of non renewable primary energy resources used as raw materials; PENRT Total use of non renewable primary energy resources; SM
Use of secondary materials; RSF Use of renewable secondary fuels; NRSF Use of non renewable secondary fuels; FW Use of net fresh water
"Reading example: 9,0 E-03 = 9,0*10-3 = 0,009"
*INA Indicator Not Assessed
9 / 12
End of life - Waste
Indicator Unit A1-A3 A4 A5 C1 C2 C3 C4 D
HWD kg 8,15E-01 1,24E-03 2,46E-02 3,02E-05 3,64E-04 0,00E+00 4,15E-04 -3,61E-02
NHWD kg 3,15E+00 1,31E+00 1,70E-01 1,21E-03 3,44E-01 0,00E+00 2,68E+01 -2,84E+00
RWD kg 9,64E-03 3,53E-05 1,65E-06 7,12E-06 4,81E-05 0,00E+00 3,89E-05 1,91E-05
HWD = Hazardous waste disposed; NHWD = Non-hazardous waste disposed; RWD = Radioactive waste disposed;
"Reading example: 9,0 E-03 = 9,0*10-3 = 0,009"
*INA Indicator Not Assessed
End of life - Output flow
Indicator Unit A1-A3 A4 A5 C1 C2 C3 C4 D
CRU kg 0,00E+00 0,00E+00 0,00E+00 0,00E+00 0,00E+00 0,00E+00 0,00E+00 0,00E+00
MFR kg 1,01E+00 0,00E+00 5,73E-01 4,94E-04 0,00E+00 8,11E+00 2,34E-03 3,29E+00
MER kg 3,63E-04 0,00E+00 1,95E-06 1,53E-06 0,00E+00 0,00E+00 4,39E-05 2,09E-03
EEE MJ 5,23E-01 0,00E+00 9,30E-02 5,25E-06 0,00E+00 0,00E+00 3,59E-03 -2,39E-03
EET MJ 7,91E+00 0,00E+00 1,41E+00 7,95E-05 0,00E+00 0,00E+00 5,44E-02 -3,61E-02
CRU = Components for re-use; MFR = Materials for recycling; MER = Materials for energy recovery; EEE = Exported electrical energy; EET = Exported energy ​ Thermal
"Reading example: 9,0 E-03 = 9,0*10-3 = 0,009"
*INA Indicator Not Assessed
Biogenic Carbon Content
Indicator Unit At the factory gate
Biogenic carbon content in product kg C 0,00E+00
Biogenic carbon content in accompanying packaging kg C 6,85E-01
Note: 1 kg biogenic carbon is equivalent to 44/12 kg CO2
10 / 12
Additional Norwegian requirements
Greenhouse gas emissions from the use of electricity in the manufacturing phase
National production mix from import, low voltage (production of transmission lines, in addition to direct emissions and losses in grid) of applied
electricity for the manufacturing process (A3).
Electricity mix Data source Amount Unit
Electricity, Sweden (kWh) ecoinvent 3.6 54,94 g CO2-eq/kWh
Dangerous substances
The product contains no substances given by the REACH Candidate list or the Norwegian priority list.
Indoor environment
Additional Environmental Information
Environmental impact indicators EN 15804+A1 and NPCR Part A v2.0
Indicator Unit A1-A3 A4 A5 C1 C2 C3 C4 D
GWP kg CO2 -eq 2,84E+01 4,00E-01 9,37E-02 7,35E-02 4,63E-01 0,00E+00 2,12E-01 -6,50E+00
ODP kg CFC11 -eq 3,15E-07 6,44E-08 3,12E-09 1,28E-08 8,58E-08 0,00E+00 6,62E-08 -2,23E-07
POCP kg C2H4 -eq 6,92E-03 1,46E-04 7,08E-06 1,13E-05 5,65E-05 0,00E+00 4,98E-05 -4,29E-03
AP kg SO2 -eq 6,65E-02 1,62E-03 5,85E-05 1,09E-04 9,23E-04 0,00E+00 5,89E-04 -2,60E-02
EP kg PO43- -eq 7,99E-03 2,40E-04 2,99E-05 1,21E-05 9,82E-05 0,00E+00 6,95E-05 -3,86E-03
ADPM kg Sb -eq 1,73E-03 5,06E-05 3,82E-07 1,14E-07 1,29E-05 0,00E+00 1,95E-06 -1,20E-04
ADPE MJ 3,57E+02 8,07E+00 2,55E-01 1,02E+00 6,92E+00 0,00E+00 5,72E+00 -6,35E+01
GWPIOBC kg CO2 -eq 2,90E+00 4,17E-01 0,00E+00 9,99E+01 4,68E-01 0,00E+00 0,00E+00 -1,04E+01
GWP Global warming potential; ODP Depletion potential of the stratospheric ozone layer; POCP Formation potential of tropospheric photochemical oxidants; AP
Acidification potential of land and water; EP Eutrophication potential; ADPM Abiotic depletion potential for non fossil resources; ADPE Abiotic depletion​ potential for
fossil resources; GWP-IOBC/GHG Global warming potential calculated according to the principle of instantanious oxidation (except emissions and uptake of biogenic
carbon)
11 / 12
Bibliography
ISO 14025:2010 Environmental labels and declarations - Type III environmental declarations - Principles and procedures.
ISO 14044:2006 Environmental management - Life cycle assessment - Requirements and guidelines.
EN 15804:2012+A2:2019 Environmental product declaration - Core rules for the product category of construction products.
ISO 21930:2017 Sustainability in buildings and civil engineering works - Core rules for environmental product declarations of construction
products.
ecoinvent v3, Allocation, cut-off by classification, Swiss Centre of Life Cycle Inventories.
Iversen et al., (2021) eEPD v2021.09 Background information for EPD generator tool system verification, LCA.no Report number: 07.21
Graafland and Iversen, (2022) EPD generator for EPD generator for NPCR 013 Part B for Steel and Aluminum, Background information for EPD
generator application and LCA data, LCA.no report number: 08.22
NPCR Part A: Construction products and services. Ver. 2.0. April 2021, EPD-Norge.
NPCR 013 Part B for Steel and Aluminium Construction Products , Ver. 4.0, 06.10.2021, EPD Norway.
Program operator and publisher Phone: +47 23 08 80 00
The Norwegian EPD Foundation e-mail: post@epd-norge.no
Post Box 5250 Majorstuen, 0303 Oslo, Norway web: www.epd-norge.no
Owner of the declaration: Phone: +47 41 723939
stig-
ArcelorMittal Construction Norge AS e-mail:
tore.sjaastad@arcelormittal.com
Sørumgata 11A, 2000 Lillestrøm web:
Author of the Life Cycle Assessment Phone: +47 916 50 916
LCA.no AS e-mail: post@lca.no
Dokka 6B, 1671 web: www.lca.no
Developer of EPD generator Phone: +47 916 50 916
LCA.no AS e-mail: post@lca.no
Dokka 6B,1671 Kråkerøy web: www.lca.no
ECO Platform web: www.eco-platform.org
ECO Portal web: ECO Portal
12 / 12
