Environmental product declaration
In accordance with 14025 and EN15804+A2
Clint cover
Owner of the declaration: Program operator:
Fora Form AS The Norwegian EPD Foundation
Declaration number:
Clint cover
Registration number:
Declared unit:
1 pcs Issue date:
27.04.2023
This declaration is based on Product Category Rules:
CEN Standard EN 15804:2012+A2:2019 serves as core Valid to:
PCR
The Norwegian EPD Foundation EPD Software:
NPCR 026:2022 Part B for Furniture (Version 2.0)
LCA.no EPD generator ID: 61809
1 / 12
General information
Product Owner of the declaration:
Clint cover Fora Form AS
Contact person: Kåre Sætre
Phone: +47 700 46 000
e-mail: info@foraform.com
Program operator: Manufacturer:
Post Box 5250 Majorstuen, 0303 Oslo, Norway Fora Form AS
The Norwegian EPD Foundation
Phone: +47 23 08 80 00
web: post@epd-norge.no
Declaration number: Place of production:
Fora Form AS
Mosflatevegen
6154 Ørsta, Norway
This declaration is based on Product Category Rules: Management system:
CEN Standard EN 15804:2012+A2:2019 serves as core PCR NS-EN ISO 14001: 2015 No. 800406.NS-EN ISO 9001: 2015 No.
NPCR 026:2022 Part B for Furniture (Version 2.0) 901268.NS-EN ISO 45001: 2018 No 907167.
Statement of liability: Organisation no:
The owner of the declaration shall be liable for the underlying 986 581 421
information and evidence. EPD Norway shall not be liable with respect
to manufacturer information, life cycle assessment data and
evidences.​
Declared unit: Issue date:
1 pcs Clint cover 27.04.2023
Declared unit (cradle to gate) with option: Valid to:
A1-A3,A4,A5,B1,B2,C1,C2,C3,C4,D
Year of study:
2023
Functional unit: Comparability:
Production of one table solution provided and maintained for a EPD of construction products may not be comparable if they not
period of 15 years. comply with EN 15804 and seen in a building context.
General information on verification of EPD from EPD tools: Development and verification of EPD:
Independent verification of data, other environmental information The declaration is created using EPD tool lca.tools ver EPD2022.03,
and the declaration according to ISO 14025:2010, § 8.1.3 and § 8.1.4. developed by LCA.no. The EPD tool is integrated in the company's
Individual​ third party verification of each EPD is not required when management system, and has been approved by EPD Norway.
the EPD tool is i) integrated into the company's environmental
management system, ii) the procedures for use of the EPD tool are Developer of EPD: Kåre Sætre
approved by EPDNorway, and iii)​ the proccess is reviewed annualy.
Reviewer of company-specific input data and EPD: Stig Robert
See Appendix G of EPD-Norway's General Programme Instructions
Sporstøl
for further information on EPD tools.
Verification of EPD tool: Approved:
Independent third party verification of the EPD tool, background data
and test-EPD in accordance with EPDNorway's procedures and
guidelines for verification and approval of EPD tools.
Third party verifier:
Elisabet Amat Håkon Hauan, CEO EPD-Norge
(no signature required)
2 / 12
Product
Product description:
Clint Cover is a product that intends to contribute to an increased lifespan of Clint chairs. Compared to a piece of new furniture, the
environmental factor will significantly save energy and carbon emissions.
Product specification
Clint Cover is produced with laminated textile
Lamination is a finishing process where several layers of material is bonded to the back of fabrics to enhance the fabrics’ technical performance
and improve upholstery properties. Our lamination services include flame lamination and glue lamination, and our innovative techniques and
high-end equipment allow us to work with various thicknesses, textures and materials. Lamination is used for multiple purposes and reasons
primarily to boost the fabric’s technical properties such as for example the comfort, strength and stability of the fabric. Lamination can also
compensates for uneven or sharp components, blocks liquids and improves the fabric’s acoustic properties. The soft foam backing added to the
fabric in the lamination process provides superior flexibility allowing the laminated fabrics to be readily used for curved or complex furniture
designs without compromising the quality, performance or aesthetic value of the fabric.
The key benefits of lamination are:
A luxurious soft feel , improved stability , excellent upholstery properties , stronger and more durable fabrics , an exclusive and lavish look ,
acoustic performance
Materials kg %
Plastic - Polyurethane (PUR) 0,30 50,00
Textile - Polyester (PE) 0,10 16,67
Textile - Wool 0,20 33,33
Total 0,60
Packaging kg %
Packaging - Cardboard 0,50 100,00
Total incl. packaging 1,10
Technical data:
Fabric used in EPD is Gabriel Capture / Tested and approved
Abrasion resistance BS EN ISO 12947-2/14465
Acoustic test air flow resistance EN 29053 & ISO 9053-1
Colour fastness to light BS EN ISO 105 B02 / AATCC 16 Light fastness
Flammability BS EN 1021 1&2 / BS 5852 Part 1 0,1 C /Class Uno UNI 9175 Class 1 I EMME / CA TB 117-2013
Flammability / flameretardant treatment BS 5852 Crib 5
Pilling BS EN ISO 12945-2 / ASTM D3511 Pilling
Seam slippage BS EN ISO 13936-2
Wet and dry crocking AATCC 8 or 116 Wet/dry crocking
Capture is a lightly felted and multi-coloured wool fabric in a casual yet sophisticated tweed look. It fuses light and dark colours to a refined
mélange pattern creating a lively and beautifully rugged surface that never ceases to change under your gaze. Available in a versatile selection of
43 colours, Capture offers an abundance of hues to match any design, material and interior. The warm and intense colour palette covers a distinct
selection of brown and yellowish tones inspired by the world of spices as well as a range of timeless neutrals and contemporary shades. These
include variations of grey and beige, soft and dusty shades of blue, powdery pinks, and multiple shades of lavender and green. The colour scale
provides groups of colours that complement each other and make it easy to create harmonious colour combinations.
Market:
Worldwide
Reference service life, product
15 years
Reference service life, building
LCA: Calculation rules
Declared unit:
1 pcs Clint cover
Cut-off criteria:
All major raw materials and all the essential energy is included. The production processes for raw materials and energy flows with very small
amounts (less than 1%) are not included. These cut-off criteria do not apply for hazardous materials and substances.
Allocation:
3 / 12
The allocation is made in accordance with the provisions of EN 15804. Incoming energy and water and waste production in-house is allocated
equally among all products through mass allocation. Effects of primary production of recycled materials is allocated to the main product in which
the material was used. The recycling process and transportation of the material is allocated to this analysis.
Data quality:
Specific data for the product composition are provided by the manufacturer. They represent the production of the declared product and were
collected for EPD development in the year of study. Background data is based on registered EPDs according to EN 15804, Ostfold Research
databases, ecoinvent and other LCA databases. The data quality of the raw materials in A1 is presented in the table below.​
Materials Source Data quality Year
Packaging - Cardboard ecoinvent 3.6 Database 2019
Plastic - Polyurethane (PUR) ecoinvent 3.6 Database 2019
Textile - Polyester (PE) ecoinvent 3.6 Database 2019
Textile - Wool Modified ecoinvent 3.6 Database 2019
4 / 12
System boundaries (X=included, MND=module not declared, MNR=module not relevant)
Construction Beyond the system
Product stage Use stage End of life stage
installation stage boundaries
A1 A2 A3 A4 A5 B1 B2 B3 B4 B5 B6 B7 C1 C2 C3 C4 D
X X X X X X X MND MND MND MND MND X X X X X
System boundary:
Additional technical information:
We want you to enjoy your furniture for many years to come. If you follow our advice in this Quality and Maintenance Manual you contribute to
prolonged life of your furniture. We only use environmentally friendly materials and processes in our manufacturing unit in Ørsta Norway. Our goal
is to manufacture furniture that can last for generations. All furniture made by Fora Form are made of FSC certified wood, manufactured according
to ISO 14001, and has an EPD on all products. This ensures sustainability and a “cradle to cradle” philosophy. We actively work to reduce waste. All
packing materials and waste are being recycled according to Norsk Gjenvinning.
Norwegian and Swedish Møbelfakta are accredited test facilities where furniture quality, strength, durability, flammability, safety, emissions and
materials are tested and documented. A piece of furniture, which lives up to the three areas of requirements of Møbelfakta, has undergone
extensive testing, is produced according to ethical guidelines and has been approved according to environmental requirements. Møbelfakta is a
guarantee of high quality products. Almost all of Fora Forms collection is Møbelfakta approved.
Fora Form are ISO 9001 quality management,ISO 14001 environmental management and ISO 45001 occupational health and safety management
certified. Sustainability is important for Fora Form.
We continuously work to sort and reduce our waste, and collaborate with Norsk Gjenvinning and Grønt Punkt (Green Dot Norway plc) regarding
recycling of used packing materials. All wood is FSC certified.
Our manufacturing unit in Ørsta use electricity that is 100% originated from renewable sources.
Transportation to an average customer in Oslo is 540 km
waR slairetam tropsnarT gnirutcafunaM tropsnarT ylbmessA e​sU ecnanetniaM riapeR tnemecalpeR tnemhsibrufeR lanoitarepO ygrene esu lanoitarepO esu retaw -eD noitcurtsnoc noitilomed tropsnarT etsaW gnissecorp lasopsiD -yrevoceR-esueR laitnetop-gnilcyceR
5 / 12
LCA: Scenarios and additional technical information
The following information describe the scenarios in the different modules of the EPD.
Capacity utilisation Value
Transport from production place to user (A4) Distance (km) Fuel/Energy Consumption Unit
(incl. return) % (Liter/tonne)
Truck, 16-32 tonnes, HVO, EURO 6 (kgkm) 36,7 % 540 0,043 l/tkm 23,22
Assembly (A5) Unit Value
Waste, packaging, corrugated board box, to
kg 0,50
average treatment (kg)
Capacity utilisation Value
Transport to waste processing (C2) Distance (km) Fuel/Energy Consumption Unit
(incl. return) % (Liter/tonne)
Truck, 3.5-7.5 tonnes, HVO, EURO 6 (kgkm) 19,7 % 85 0,129 l/tkm 10,97
Waste processing (C3) Unit Value
Waste treatment per kg Polyurethane (PU),
kg 0,30
incineration (kg)
Waste treatment per kg Textile, incineration with
kg 0,30
fly ash extraction (kg)
Disposal (C4) Unit Value
Landfilling of ashes from incineration of
Polyurethane (PU), process per kg ashes and kg 0,01
residues - C4 (kg)
Landfilling of ashes from incineration of Textile,
kg 0,02
soiled, process per kg ashes and residues (kg)
Benefits and loads beyond the system
Unit Value
boundaries (D)
Substitution of electricity, in Norway (MJ) MJ 0,69
Substitution of thermal energy, district heating, in
MJ 10,49
Norway (MJ)
6 / 12
LCA: Results
The LCA results are presented below for the declared unit defined on page 2 of the EPD document.
Environmental impact
Indicator Unit A1-A3 A4 A5 B1 B2 C1 C2 C3 C4 D
GWP-total
kg CO2 -
1,24E+01 2,31E-02 8,57E-01 0 0 0 1,28E-02 1,25E+00 1,01E-03 -6,31E-02
eq
GWP-fossil
kg CO2 -
6,35E+00 2,30E-02 8,09E-03 0 0 0 1,27E-02 8,10E-01 1,01E-03 -6,08E-02
eq
GWP-biogenic
kg CO2 -
5,11E+00 3,90E-05 8,49E-01 0 0 0 2,59E-05 4,39E-01 2,35E-06 -1,26E-04
eq
GWP-luluc
kg CO2 -
9,03E-01 3,59E-05 2,68E-06 0 0 0 2,74E-05 4,95E-06 1,40E-07 -2,10E-03
eq
kg
ODP CFC11 - 2,80E-07 4,75E-09 1,71E-09 0 0 0 2,06E-09 4,21E-09 8,80E-11 -4,43E-03
eq
mol H+
AP 2,26E-01 1,62E-04 3,83E-05 0 0 0 8,54E-05 7,35E-04 3,18E-06 -5,01E-04
-eq
EP-FreshWater kg P -eq 2,28E-03 8,46E-07 6,64E-08 0 0 0 5,72E-07 2,78E-07 1,40E-08 -5,41E-06
EP-Marine kg N -eq 3,96E-02 4,27E-05 1,27E-05 0 0 0 1,92E-05 4,10E-04 9,62E-07 -1,64E-04
mol N -
EP-Terrestial 9,52E-01 4,78E-04 1,37E-04 0 0 0 2,17E-04 3,93E-03 1,10E-05 -1,77E-03
eq
kg
POCP NMVOC 2,00E-02 1,75E-04 3,94E-05 0 0 0 7,97E-05 9,33E-04 3,01E-06 -4,89E-04
-eq
ADP- kg Sb -
9,35E-05 2,80E-06 1,97E-07 0 0 0 2,42E-06 1,52E-07 4,46E-09 -6,05E-07
minerals&metals1 eq
ADP-fossil1 MJ 7,26E+01 4,88E-01 1,13E-01 0 0 0 2,50E-01 3,46E-01 7,75E-03 -8,70E-01
WDP1 m3 1,73E+02 1,44E+00 1,43E-01 0 0 0 1,12E+00 8,50E-01 1,00E-01 -1,08E+01
GWP total = Global Warming Potential total; GWP fossil = Global Warming Potential fossil fuels ; GWP biogenic = Global Warming Potential biogenic; GWP luluc =
Global W Potential land use change; ODP = Ozone Depletion; AP = Acidification; EP freshwater = Eutrophication aquatic freshwater; EP = marine Eutrophication aquatic
marine; EP = terrestrial Eutrophication terrestrial ;POCP = Photochemical zone formation; ADPE = Abiotic Depletion Potential minerals and metals; ADPF = Abiotic
Depletion Potential fossil fuels;
"Reading example: 9,0 E-03 = 9,0*10-3 = 0,009"
*INA Indicator Not Assessed
1. The results of this environmental impact indicator shall be used with care as the uncertainties on these results are high or as there is limited experienced with the
indicator
Remarks to environmental impacts
The product contains no substances given by the REACH Candidate list or the Norwegian priority list.
7 / 12
Additional environmental impact indicators
Indicator Unit A1-A3 A4 A5 B1 B2 C1 C2 C3 C4 D
PM Disease incidence 1,71E-06 5,35E-09 5,65E-10 0 0 0 1,96E-09 2,59E-09 3,50E-11 -3,04E-08
IRP2 kgBq U235 -eq 1,75E-01 1,59E-03 4,84E-04 0 0 0 8,42E-04 5,24E-04 3,85E-05 -5,56E-03
ETP-fw1 CTUe 2,35E+02 7,12E-01 1,51E-01 0 0 0 4,28E-01 2,10E+00 1,72E-02 -4,73E+00
HTP-c1 CTUh 3,58E-09 0,00E+00 5,00E-12 0 0 0 0,00E+00 6,00E-11 1,00E-12 -8,70E-11
HTP-nc1 CTUh 1,12E-07 1,19E-09 1,90E-10 0 0 0 5,61E-10 2,68E-09 3,30E-11 -4,54E-09
SQP1 dimensionless -8,10E+03 9,09E-01 7,59E-02 0 0 0 2,97E-01 3,76E-02 2,34E-02 -5,82E+00
PM = Particulate Matter emissions; IRP = Ionizing radiation – human health; ETP-fw = Eco toxicity – freshwater; HTP-c = Human toxicity – cancer effects; HTP-nc =
Human toxicity – non cancer effects; SQP = Soil Quality (dimensionless)
"Reading example: 9,0 E-03 = 9,0*10-3 = 0,009"
*INA Indicator Not Assessed
1. The results of this environmental impact indicator shall be used with care as the uncertainties on these results are high or as there is limited experienced with the
indicator
2. This impact category deals mainly with the eventual impact of low dose ionizing radiation on human health of the nuclear fuel cycle. It does not consider effects due
to possible nuclear accidents, occupational exposure nor due to radioactive waste disposal in underground facilities. Potential ionizing radiation from the soil, from
radon and from some construction materials is also not measured by this indicator.
8 / 12
Resource use
Indicator Unit A1-A3 A4 A5 B1 B2 C1 C2 C3 C4 D
PERE MJ 2,40E+01 2,21E-02 1,86E-03 0 0 0 1,58E-02 9,39E-03 5,46E-04 -5,37E+00
PERM MJ 8,50E+00 0,00E+00 -4,10E+00 0 0 0 0,00E+00 -4,40E+00 0,00E+00 0,00E+00
PERT MJ 3,25E+01 2,21E-02 -4,10E+00 0 0 0 1,58E-02 -4,39E+00 5,46E-04 -5,37E+00
PENRE MJ 6,73E+01 4,88E-01 1,13E-01 0 0 0 2,50E-01 3,51E-01 7,78E-03 -8,70E-01
PENRM MJ 1,16E+01 0,00E+00 0,00E+00 0 0 0 0,00E+00 -1,16E+01 0,00E+00 0,00E+00
PENRT MJ 7,89E+01 4,88E-01 1,13E-01 0 0 0 2,50E-01 -1,13E+01 7,78E-03 -8,70E-01
SM kg 1,84E-01 0,00E+00 0,00E+00 0 0 0 0,00E+00 0,00E+00 0,00E+00 0,00E+00
RSF MJ 6,39E-02 7,18E-04 6,18E-05 0 0 0 5,38E-04 2,27E-04 1,35E-05 -9,41E-04
NRSF MJ 1,12E-02 2,47E-03 2,55E-04 0 0 0 1,95E-03 0,00E+00 1,19E-03 -3,19E-01
FW m3 1,08E-01 1,99E-04 5,34E-05 0 0 0 1,21E-04 1,25E-03 7,15E-06 -6,47E-03
PERE Use of renewable primary energy excluding renewable primary energy resources used as raw materials; PERM Use of renewable primary energy resources used as
raw materials; PERT Total use of renewable primary energy resources; PENRE Use of non renewable primary energy excluding non-renewable primary energy resources
used as raw materials; PENRM Use of non renewable primary energy resources used as raw materials; PENRT Total use of non renewable primary energy resources; SM
Use of secondary materials; RSF Use of renewable secondary fuels; NRSF Use of non renewable secondary fuels; FW Use of net fresh water
"Reading example: 9,0 E-03 = 9,0*10-3 = 0,009"
*INA Indicator Not Assessed
9 / 12
End of life - Waste
Indicator Unit A1-A3 A4 A5 B1 B2 C1 C2 C3 C4 D
HWD kg 1,94E-02 6,84E-05 4,99E-04 0 0 0 4,12E-05 0,00E+00 9,13E-03 -4,09E-05
NHWD kg 8,51E-01 7,25E-02 5,66E-03 0 0 0 2,21E-02 0,00E+00 9,05E-03 -2,06E-02
RWD kg 1,76E-04 1,95E-06 7,48E-07 0 0 0 9,36E-07 0,00E+00 4,64E-08 -4,55E-06
HWD = Hazardous waste disposed; NHWD = Non-hazardous waste disposed; RWD = Radioactive waste disposed;
"Reading example: 9,0 E-03 = 9,0*10-3 = 0,009"
*INA Indicator Not Assessed
End of life - Output flow
Indicator Unit A1-A3 A4 A5 B1 B2 C1 C2 C3 C4 D
CRU kg 0,00E+00 0,00E+00 0,00E+00 0 0 0 0,00E+00 0,00E+00 0,00E+00 0,00E+00
MFR kg 0,00E+00 0,00E+00 4,65E-01 0 0 0 0,00E+00 0,00E+00 0,00E+00 0,00E+00
MER kg 0,00E+00 0,00E+00 6,81E-07 0 0 0 0,00E+00 6,00E-01 0,00E+00 0,00E+00
EEE MJ 0,00E+00 0,00E+00 2,86E-02 0 0 0 0,00E+00 6,30E-01 0,00E+00 0,00E+00
EET MJ 0,00E+00 0,00E+00 4,33E-01 0 0 0 0,00E+00 9,54E+00 0,00E+00 0,00E+00
CRU = Components for re-use; MFR = Materials for recycling; MER = Materials for energy recovery; EEE = Exported energy electrical; EET = Exported energy Thermal;
"Reading example: 9,0 E-03 = 9,0*10-3 = 0,009"
*INA Indicator Not Assessed
Biogenic Carbon Content
Indicator Unit At the factory gate
Biogenic carbon content in product kg C 0,00E+00
Biogenic carbon content in accompanying packaging kg C 2,31E-01
Note: 1 kg biogenic carbon is equivalent to 44/12 kg CO2
10 / 12
Additional Norwegian requirements
Greenhouse gas emissions from the use of electricity in the manufacturing phase
National production mix from import, low voltage (production of transmission lines, in addition to direct emissions and losses in grid) of applied
electricity for the manufacturing process (A3).
Electricity mix Data source Amount Unit
Electricity, European average (kWh) ecoinvent 3.6 428,03 g CO2-eq/kWh
Dangerous substances
No substances given by the REACH Candidate list or the Norwegian priority list are intentionally added to the product.
Indoor environment
Our furniture doesn't contain any substanses that effect indoor clima, and therefore satisfies the requirements for low emissions.
Additional Environmental Information
Environmental impact indicators EN 15804+A1 and NPCR Part A v2.0
Indicator Unit A1-A3 A4 A5 B1 B2 C1 C2 C3 C4 D
GWP kg CO2 -eq 2,66E+00 2,21E-02 8,04E-03 0 0 0 1,22E-02 1,30E+00 1,95E-03 -6,19E-02
ODP kg CFC11 -eq 1,30E-07 3,56E-09 1,38E-09 0 0 0 1,78E-09 7,55E-09 1,44E-10 -6,39E-09
POCP kg C2H4 -eq 5,49E-04 8,08E-06 1,15E-06 0 0 0 4,59E-06 1,17E-05 2,13E-07 -7,30E-05
AP kg SO2 -eq 1,03E-02 8,97E-05 2,06E-05 0 0 0 5,42E-05 1,04E-03 3,36E-06 -3,70E-04
EP kg PO43- -eq 2,05E-03 1,33E-05 3,54E-06 0 0 0 7,38E-06 4,53E-04 4,64E-07 -1,06E-04
ADPM kg Sb -eq 2,23E-05 2,80E-06 1,97E-07 0 0 0 2,42E-06 2,72E-07 8,91E-09 -6,06E-07
ADPE MJ 4,26E+01 4,47E-01 1,11E-01 0 0 0 2,24E-01 6,50E-01 1,52E-02 -7,02E-01
GWPIOBC kg CO2 -eq 1,28E+01 2,31E-02 0,00E+00 0 0 0 1,28E-02 1,30E+00 1,95E-03 -6,21E-02
GWP Global warming potential; ODP Depletion potential of the stratospheric ozone layer; POCP Formation potential of tropospheric photochemical oxidants; AP
Acidification potential of land and water; EP Eutrophication potential; ADPM Abiotic depletion potential for non fossil resources; ADPE Abiotic depletion​ potential for
fossil resources; GWP-IOBC/GHG Global warming potential calculated according to the principle of instantanious oxidation (except emissions and uptake of biogenic
carbon)
Key Environmental Indicators
Indicator Unit A1-A3 A4 A1-C4 A1-D
GWPtotal kg CO2 -eq 12,37 0,02 14,51 14,45
Total energy consumption MJ 91,29 0,51 92,56 86,00
Secondary materials % 39,50
11 / 12
Bibliography
ISO 14025:2010 Environmental labels and declarations - Type III environmental declarations - Principles and procedures.
ISO 14044:2006 Environmental management - Life cycle assessment - Requirements and guidelines.
EN 15804:2012+A2:2019 Environmental product declaration - Core rules for the product category of construction products.
ISO 21930:2017 Sustainability in buildings and civil engineering works - Core rules for environmental product declarations of construction
products.
ecoinvent v3, Allocation, cut-off by classification, Swiss Centre of Life Cycle Inventories.
Iversen et al., (2021) eEPD v2021.09 Background information for EPD generator tool system verification, LCA.no Report number: 07.21
Ruud et al., (2023) EPD generator for NPCR026 Part B for Furniture - Background information for EPD generator application and LCA data,
LCA.no report number 01.23
NPCR Part A: Construction products and services. Ver. 2.0. March 2021, EPD-Norge.
NPCR 026 Part B for Furniture. Ver. 2.0 March 2022, EPD-Norge.
Program operator and publisher Phone: +47 23 08 80 00
The Norwegian EPD Foundation e-mail: post@epd-norge.no
Post Box 5250 Majorstuen, 0303 Oslo, Norway web: www.epd-norge.no
Owner of the declaration: Phone: +47 700 46 000
Fora Form AS e-mail: info@foraform.com
Mosflatevegen, 6154 Ørsta web: www.foraform.no
Author of the Life Cycle Assessment Phone: +47 916 50 916
LCA.no AS e-mail: post@lca.no
Dokka 6B, 1671 web: www.lca.no
Developer of EPD generator Phone: +47 916 50 916
LCA.no AS e-mail: post@lca.no
Dokka 6B,1671 Kråkerøy web: www.lca.no
ECO Platform web: www.eco-platform.org
ECO Portal web: ECO Portal
12 / 12
