Environmental product declaration
in accordance with ISO 14025 and EN 15804+A2
Glued laminated timber (Límtré/Glulam/GLT)
Owner of the declaration: Program operator:
Límtré Vírnet The Norwegian EPD Foundation
Product: Declaration number:
Glued laminated timber (Límtré/Glulam/GLT)
NEPD-8842-8494
Declared unit:
1 m3 Registration number:
This declaration is based on Product Category Rules: NEPD-8842-8494
CEN Standard EN 15804:2012+A2:2019 serves as core
Issue date: 27.01.2025
PCR
The Norwegian EPD Foundation NPCR 015:2021 Part B for wood and wood-based Valid to: 27.01.2030
products for use in construction
ver-300125
EPD software:
LCAno EPD generator ID:
766045
1 / 11
General information
Product Owner of the declaration:
Glued laminated timber (Límtré/Glulam/GLT) Límtré Vírnet
Contact person: Einar Bjarnason
Phone: +3544125300
e-mail: einar@limtrevirnet.is
Program operator:
Manufacturer:
The Norwegian EPD Foundation Límtré Vírnet
Post Box 5250 Majorstuen, 0303 Oslo, Norway
Borgarbraut 74
Phone: +47 977 22 020
310 Borgarnes, Iceland
web: www.epd-norge.no
Declaration number:
Place of production:
Límtré Vírnet
NEPD-8842-8494
846 Flúðum
, Iceland
This declaration is based on Product Category Rules:
Management system:
CEN Standard EN 15804:2012+A2:2019 serves as core PCR
NPCR 015:2021 Part B for wood and wood-based products for use in
construction
Statement of liability:
Organisation no:
The owner of the declaration shall be liable for the underlying
information and evidence. EPD Norway shall not be liable with respect
to manufacturer information, life cycle assessment data and
evidences.​
Declared unit:
Issue date:
1 m3 Glued laminated timber (Límtré/Glulam/GLT)
27.01.2025
Declared unit with option:
Valid to:
A1-A3,A4,A5,C1,C2,C3,C4,D
27.01.2030
Year of study:
2023
Functional unit:
Comparability:
EPD of construction products may not be comparable if they not
comply with EN 15804 and seen in a building context.
General information on verification of EPD from EPD tools:
Development and verification of EPD:
Independent verification of data, other environmental information The declaration is created using EPD tool lca.tools ver EPD2022.03,
and the declaration according to ISO 14025:2010, § 8.1.3 and § 8.1.4.
developed by LCA.no. The EPD tool is integrated in the company's
Verification of each EPD is made according to EPD-Norway’s
management system, and has been approved by EPD Norway.
guidelines for verification and approval requiring that tools are i)
integrated into the company's environmental management system, ii) Developer of EPD: Vincent Merida - Verkvist
the procedures for use of the EPD tool are approved by EPD-Norway,
​
and iii) the process is reviewed annually by an independent third Reviewer of company-specific input data and EPD: Børge Heggen
party verifier. See Appendix G of EPD-Norway's General Programme Johansen, Energiråd AS
Instructions for further information on EPD tools
Verification of EPD tool:
Approved:
Independent third party verification of the EPD tool, background data
and test-EPD in accordance with EPDNorway's procedures and
guidelines for verification and approval of EPD tools.
Third party verifier:
Alexander Borg, Asplan Viak AS
(no signature required)
2 / 11
Product
Product description:
Glued laminated timber (GLT) is used for structural purposes like load bearing beams and pillars. The declared product is made of spruce and has
an average moisture content of 11%. The product can be ordered with or without a galvanized steel nail plate.
Product specification
The product is constructed to match individual customer specifications and consists of planed spruce, a melamine urea resin adhesive, and can be
joined with a galvanized steel nail plate.
Materials kg %
Glue for wood 7,50 1,50
Metal - Steel 1,27 0,25
Wood 492,50 98,25
Total 501,27 100,00
Packaging kg %
Packaging - Plastic 0,83 49,11
Packaging - Plastic straps 0,86 50,89
Total incl. packaging 502,96 100,00
Technical data:
This product is produced according to EN 14080:2013 and is delivered according to individual customer specifications.
Market:
Iceland
Reference service life, product
As building
Reference service life, building or construction works
60 years
LCA: Calculation rules
Declared unit:
1 m3 Glued laminated timber (Límtré/Glulam/GLT)
Cut-off criteria:
All major raw materials and all the essential energy is included. The production processes for raw materials and energy flows with very small
amounts (less than 1%) are not included. These cut-off criteria do not​ apply for hazardous materials and substances.
Allocation:
The allocation is made in accordance with the provisions of EN 15804. In forestry, economic allocation between sawn timber and solid wood is
used. At sawmills, energy, water, waste, materials and internal transport are divided into sub-processes and then allocated according to income
between the main and secondary products. Environmental impact and resource consumption for the primary production of recycled materials is
allocated to the original product system. Economic allocation was applied to account for the various co-products originating from mill activities.
The economic value of each co-product was used to allocate energy flows between products.
Data quality:
Specific data for the product composition are provided by the manufacturer. The data represent the production of the declared product and were
collected for EPD development in the year of study. Background data is based on EPDs according to EN 15804 and different LCA databases. The
data quality of the raw materials in A1 is presented in the table below.
Materials Source Data quality Year
Glue for wood ecoinvent 3.6 Database 2019
Metal - Steel S-P-01921 EPD 2017
Packaging - Plastic ecoinvent 3.6 Database 2019
Packaging - Plastic straps ecoinvent 3.6 Database 2019
Wood ecoinvent 3.6 Database 2019
3 / 11
System boundaries (X=included, MND=module not declared, MNR=module not relevant)
Construction Beyond the system
Product stage Use stage End of life stage
installation stage boundaries
A1 A2 A3 A4 A5 B1 B2 B3 B4 B5 B6 B7 C1 C2 C3 C4 D
X X X X X MND MND MND MND MND MND MND X X X X X
System boundary:
Cradle-to-gate plus options C1-C4, D
Additional technical information:
At the end of its useful life, the glulam is assumed to be demolished and transported to a waste processing facility. There it is shredded in a
stationary wood chipping unit and is re-used as animal bedding or landscape materials. Biogenic carbon is calculated according to
EN16485:2014/EN15804+A2, where the net biogenic carbon cycle A to C is zero (i.e. carbon dioxide neutral).
waR slairetam tropsnarT gnirutcafunaM tropsnarT ylbmessA e​sU ecnanetniaM riapeR tnemecalpeR tnemhsibrufeR lanoitarepO ygrene esu lanoitarepO esu retaw -eD noitcurtsnoc noitilomed tropsnarT etsaW gnissecorp lasopsiD -yrevoceR-esueR laitnetop-gnilcyceR
4 / 11
LCA: Scenarios and additional technical information
The following information describe the scenarios in the different modules of the EPD.
The product is typically produced without a nail plate, however, it is included in the LCI to demonstrate the worst case scenario. If the nail plate is
excluded, GWPIOBC would be reduced by 1.59% compared to the results of this EPD.
Capacity utilisation Value
Transport from production place to user (A4) Distance (km) Fuel/Energy Consumption Unit
(incl. return) % (Liter/tonne)
Truck, 16-32 tonnes, EURO 6 (kgkm) - RER 36,7 % 265 0,043 l/tkm 11,40
Assembly (A5) Unit Value
Materials to Recycling (kg) kg 1,69
Diesel, burned (kWh) - GLO kWh 0,27
Electricity, Iceland (kWh) kWh 0,028
De-construction demolition (C1) Unit Value
Diesel, burned in Excavator, 30 ton (L) L 0,052
Capacity utilisation Value
Transport to waste processing (C2) Distance (km) Fuel/Energy Consumption Unit
(incl. return) % (Liter/tonne)
Ship, Freight, Transoceanic (kgkm) 65,0 % 2000 0,003 l/tkm 6,00
Truck, unspecified, EURO 6 (kgkm) - RER 46,1 % 100 0,034 l/tkm 3,40
Truck, unspecified, EURO 6 (kgkm) - RER 46,1 % 100 0,034 l/tkm 3,40
Waste processing (C3) Unit Value
Materials to recycling (kg) - C3 kg 2,98
Wood chipping, industrial residual wood,
kg 504,20
stationary electric chipper (kg) - RER
Balancing waste - RPEM (MJ) - (Type 4) MJ 6948,83
Balancing waste - Biogenic carbon in product (kg)
kg 785,087
- (Type 4)
Benefits and loads beyond the system
Unit Value
boundaries (D)
Substitution of polyethylene terephthalate, PET,
kg 0,86
amorphous (kg) - GLO
Substitution of polyethylene, LDPE, granulate (kg)
kg 0,83
- RER
Substitution of primary steel with net scrap (kg) kg 1,29
substitution of wood chips (kg) - RoW kg 504,20
5 / 11
LCA: Results
The LCA results are presented below for the declared unit defined on page 2 of the EPD document.
Environmental impact
Indicator Unit A1-A3 A4 A5 C1 C2 C3 C4 D
GWP-total kg CO2 -eq -5,91E+02 2,18E+01 1,15E-01 1,79E-01 6,66E+00 7,90E+02 0 -3,13E+01
GWP-fossil kg CO2 -eq 1,90E+02 2,18E+01 1,13E-01 1,79E-01 6,66E+00 4,41E+00 0 -3,10E+01
GWP-biogenic kg CO2 -eq -7,84E+02 9,01E-03 1,92E-04 4,20E-05 2,93E-03 7,85E+02 0 -7,68E-02
GWP-luluc kg CO2 -eq 2,97E+00 7,75E-03 8,72E-04 3,99E-05 2,45E-03 9,90E-03 0 -3,06E-01
ODP kg CFC11 -eq 3,78E-05 4,93E-06 2,47E-08 3,97E-08 1,53E-06 3,69E-07 0 -5,02E-06
AP mol H+ -eq 1,51E+00 6,26E-02 1,03E-03 8,60E-04 2,08E-02 2,44E-02 0 -1,79E-01
EP-FreshWater kg P -eq 2,01E-03 1,74E-04 5,50E-07 9,62E-07 5,63E-05 4,54E-04 0 -2,36E-03
EP-Marine kg N -eq 4,77E-01 1,24E-02 4,40E-04 3,06E-04 4,27E-03 3,26E-03 0 -5,97E-02
EP-Terrestial mol N -eq 5,53E+00 1,38E-01 4,84E-03 3,37E-03 4,77E-02 3,99E-02 0 -6,43E-01
POCP kg NMVOC -eq 1,50E+00 5,30E-02 1,34E-03 1,00E-03 1,82E-02 1,04E-02 0 -2,36E-01
ADP-minerals&metals1 kg Sb-eq 6,57E-03 6,01E-04 8,35E-07 1,29E-06 1,80E-04 1,70E-05 0 -4,46E-04
ADP-fossil1 MJ 2,84E+03 3,29E+02 1,59E+00 2,55E+00 1,03E+02 8,92E+01 0 -4,87E+02
WDP1 m3 2,25E+04 3,18E+02 8,15E+00 8,63E-01 1,00E+02 1,31E+03 0 -2,08E+02
GWP-total = Global Warming Potential total; GWP-fossil = Global Warming Potential fossil fuels; GWP-biogenic = Global Warming Potential biogenic; GWP-luluc =
Global Warming Potential land use and land use change; ODP = Depletion potential of the stratospheric ozone layer; AP = Acidification potential, Accumulated
Exceedance; EP-freshwater = Eutrophication potential, fraction of nutrients reaching freshwater end compartment: EP-marine = Eutrophication potential, fraction of
nutrients reaching marine end compartment; EP-terrestrial = Eutrophication potential, Accumulated Exceedance; POCP = Formation potential of tropospheric ozone;
ADP-minerals&metals = Abiotic depletion potential for non-fossil resources; ADP-fossil = Abiotic depletion for fossil resources potential; WDP = Water (user)
deprivation potential, deprivation-weighted water consumption
"Reading example: 9,0 E-03 = 9,0*10-3 = 0,009"
*INA Indicator Not Assessed
1. The results of this environmental impact indicator shall be used with care as the uncertainties on these results are high or as there is limited experienced with the
indicator
Remarks to environmental impacts
6 / 11
Additional environmental impact indicators
Indicator Unit A1-A3 A4 A5 C1 C2 C3 C4 D
PM Disease incidence 3,73E-05 1,33E-06 2,63E-08 2,81E-09 4,56E-07 7,41E-08 0 -1,76E-06
IRP2 kgBq U235 -eq 1,10E+01 1,44E+00 6,84E-03 1,09E-02 4,51E-01 7,68E-01 0 -1,51E+00
ETP-fw1 CTUe 3,17E+03 2,44E+02 1,08E+00 1,59E+00 7,77E+01 5,60E+01 0 -4,75E+02
HTP-c1 CTUh 2,73E-07 0,00E+00 3,60E-11 7,80E-11 0,00E+00 2,52E-09 0 -2,37E-08
HTP-nc1 CTUh 2,52E-06 2,67E-07 9,73E-10 1,68E-09 1,01E-07 5,60E-08 0 -2,66E-07
SQP1 dimensionless 5,62E+05 2,30E+02 3,93E-01 3,20E-01 8,80E+01 1,75E+01 0 -4,60E+04
PM = Particulate Matter emissions; IRP = Ionizing radiation – human health; ETP-fw = Eco toxicity – freshwater; HTP-c = Human toxicity – cancer effects; HTP-nc =
Human toxicity – non cancer effects; SQP = Potential Soil Quality Index (dimensionless)
"Reading example: 9,0 E-03 = 9,0*10-3 = 0,009"
*INA Indicator Not Assessed
1. The results of this environmental impact indicator shall be used with care as the uncertainties on these results are high or as there is limited experienced with the
indicator
2. This impact category deals mainly with the eventual impact of low dose ionizing radiation on human health of the nuclear fuel cycle. It does not consider effects due
to possible nuclear accidents, occupational exposure nor due to radioactive waste disposal in underground facilities. Potential ionizing radiation from the soil, from
radon and from some construction materials is also not measured by this indicator.
7 / 11
Resource use
Indicator Unit A1-A3 A4 A5 C1 C2 C3 C4 D
PERE MJ 8,61E+03 4,71E+00 1,50E-01 1,78E-02 1,51E+00 1,50E+01 0 -9,84E+03
PERM MJ 6,95E+03 0,00E+00 0,00E+00 0,00E+00 0,00E+00 -6,95E+03 0 0,00E+00
PERT MJ 1,56E+04 4,71E+00 1,50E-01 1,78E-02 1,51E+00 -6,93E+03 0 -9,84E+03
PENRE MJ 2,79E+03 3,29E+02 1,59E+00 2,55E+00 1,03E+02 8,93E+01 0 -4,55E+02
PENRM MJ 1,97E+01 0,00E+00 -1,97E+01 0,00E+00 0,00E+00 0,00E+00 0 -3,53E+01
PENRT MJ 2,81E+03 3,29E+02 -1,81E+01 2,55E+00 1,03E+02 8,93E+01 0 -4,90E+02
SM kg 3,32E-02 0,00E+00 0,00E+00 1,91E-03 0,00E+00 0,00E+00 0 -2,29E-01
RSF MJ 1,15E+00 1,69E-01 3,54E-04 5,78E-04 5,38E-02 1,27E+00 0 -1,55E-01
NRSF MJ 6,85E+00 6,03E-01 3,16E-03 -6,65E-03 1,90E-01 1,80E-01 0 1,47E+00
FW m3 3,95E+00 3,52E-02 7,47E-04 1,45E-04 1,19E-02 7,46E-02 0 -1,36E-01
PERE = Use of renewable primary energy excluding renewable primary energy resources used as raw materials; PERM = Use of renewable primary energy resources used
as raw materials; PERT = Total use of renewable primary energy resources; PENRE = Use of non renewable primary energy excluding non-renewable primary energy
resources used as raw materials; PENRM = Use of non renewable primary energy resources used as raw materials; PENRT = Total use of non renewable primary energy
resources; SM = Use of secondary materials; RSF = Use of renewable secondary fuels; NRSF = Use of non-renewable secondary fuels; FW = Net use of fresh water
"Reading example: 9,0 E-03 = 9,0*10-3 = 0,009"
*INA Indicator Not Assessed
8 / 11
End of life - Waste
Indicator Unit A1-A3 A4 A5 C1 C2 C3 C4 D
HWD kg 3,88E-01 1,70E-02 6,03E-05 9,71E-05 5,63E-03 1,17E-02 0 -8,58E-02
NHWD kg 7,91E+01 1,60E+01 1,93E-02 4,12E-03 6,37E+00 4,86E-01 0 -1,52E+01
RWD kg 1,73E-02 2,24E-03 1,10E-05 1,76E-05 7,01E-04 6,29E-04 0 -2,26E-03
HWD = Hazardous waste disposed; NHWD = Non-hazardous waste disposed; RWD = Radioactive waste disposed
"Reading example: 9,0 E-03 = 9,0*10-3 = 0,009"
*INA Indicator Not Assessed
End of life - Output flow
Indicator Unit A1-A3 A4 A5 C1 C2 C3 C4 D
CRU kg 0,00E+00 0,00E+00 0,00E+00 0,00E+00 0,00E+00 0,00E+00 0 0,00E+00
MFR kg 4,22E+00 0,00E+00 1,69E+00 0,00E+00 0,00E+00 2,98E+00 0 0,00E+00
MER kg 0,00E+00 0,00E+00 0,00E+00 0,00E+00 0,00E+00 0,00E+00 0 0,00E+00
EEE MJ 0,00E+00 0,00E+00 0,00E+00 0,00E+00 0,00E+00 0,00E+00 0 0,00E+00
EET MJ 0,00E+00 0,00E+00 0,00E+00 0,00E+00 0,00E+00 0,00E+00 0 0,00E+00
CRU = Components for re-use; MFR = Materials for recycling; MER = Materials for energy recovery; EEE = Exported energy electrical; EET = Exported energy thermal
"Reading example: 9,0 E-03 = 9,0*10-3 = 0,009"
*INA Indicator Not Assessed
Biogenic Carbon Content
Indicator Unit At the factory gate
Biogenic carbon content in product kg C 2,14E+02
Biogenic carbon content in accompanying packaging kg C 0,00E+00
Note: 1 kg biogenic carbon is equivalent to 44/12 kg CO2
9 / 11
Additional requirements
Greenhouse gas emissions from the use of electricity in the manufacturing phase
National production mix from import, low voltage (production of transmission lines, in addition to direct emissions and losses in grid) of applied
electricity for the manufacturing process (A3).
Electricity mix Source Amount Unit
Electricity, Iceland (kWh) ecoinvent 3.6 55,84 g CO2-eq/kWh
Dangerous substances
The product contains no substances given by the REACH Candidate list.
Indoor environment
Additional Environmental Information
Additional environmental impact indicators required in NPCR Part A for construction products
Indicator Unit A1-A3 A4 A5 C1 C2 C3 C4 D
GWPIOBC kg CO2 -eq 1,94E+02 2,18E+01 1,14E-01 1,79E-01 6,66E+00 4,45E+00 0 -3,20E+01
GWP-IOBC: Global warming potential calculated according to the principle of instantaneous oxidation. In order to increase the transparency of biogenic carbon​
contribution to climate impact, the indicator GWP-IOBC is required as it declares climate impacts calculated according to the principle of instantaneous oxidation.​
GWP-IOBC is also referred to as GWP-GHG in context to Swedish public procurement legislation.
10 / 11
Bibliography
ISO 14025:2010 Environmental labels and declarations - Type III environmental declarations - Principles and procedures.
ISO 14044:2006 Environmental management - Life cycle assessment - Requirements and guidelines.
EN 15804:2012+A2:2019 Environmental product declaration - Core rules for the product category of construction products.
ISO 21930:2017 Sustainability in buildings and civil engineering works - Core rules for environmental product declarations of construction
products.
ecoinvent v3, Allocation, cut-off by classification, Swiss Centre of Life Cycle Inventories.
Iversen et al., (2021) eEPD v2021.09 Background information for EPD generator tool system verification, LCA.no Report number: 07.21
EPD generator for NPCR 015 Part B for Wood-based products, Background information for EPD generator application and LCA data,
NPCR Part A: Construction products and services. Ver. 2.0, 24.03.2021 EPD Norway.
NPCR 015 Part B for wood and wood-based products , Ver. 4.0, 07.10.2021, EPD Norway.
Program operator and publisher Phone: +47 977 22 020
The Norwegian EPD Foundation e-mail: post@epd-norge.no
Post Box 5250 Majorstuen, 0303 Oslo, Norway web: www.epd-norge.no
Owner of the declaration: Phone: +3544125300
Límtré Vírnet e-mail: einar@limtrevirnet.is
Borgarbraut 74 , 310 Borgarnes, Iceland web: limtrevirnet.is
Author of the Life Cycle Assessment: Phone: +354 419 1500
Verkvist e-mail: verkvist@verkvist.is
Hallgerðargata 13, 105 Reykjavik, Iceland web: https://www.verkvist.is/
Developer of EPD generator Phone: +47 916 50 916
LCA.no AS e-mail: post@lca.no
Dokka 6A, 1671 Kråkerøy, Norway web: www.lca.no
ECO Platform web: www.eco-platform.org
ECO Portal web: ECO Portal
11 / 11
