Environmental product declaration
in accordance with ISO 14025 and EN 15804+A2
Nilo Chair
Owner of the declaration: Program operator:
Kinnarps AB The Norwegian EPD Foundation
Product: Declaration number:
Nilo Chair
Registration number:
Declared unit:
1 pcs Issue date:
This declaration is based on Product Category Rules: Valid to:
CEN Standard EN 15804:2012+A2:2019 serves as core
EPD Software:
PCR
The Norwegian EPD Foundation LCA.no EPD generator ID: 120790
NPCR 026:2022 Part B for Furniture
1 / 12
General information
Product Owner of the declaration:
Nilo Chair Kinnarps AB
Contact person: Johanna Ljunggren - Corporate Sustainability
Manager
Phone: +46 515 381 21
e-mail: johanna.ljunggren@kinnarps.se
Program operator: Manufacturer:
Post Box 5250 Majorstuen, 0303 Oslo, Norway Kinnarps AB
The Norwegian EPD Foundation
Phone: +47 23 08 80 00
web: post@epd-norge.no
Declaration number: Place of production:
Kinnarps AB
Industrigatan
521 88 Kinnarp, Sweden
This declaration is based on Product Category Rules: Management system:
CEN Standard EN 15804:2012+A2:2019 serves as core PCR ISO 9001, ISO 14001, ISO 45001
NPCR 026:2022 Part B for Furniture
Statement of liability: Organisation no:
The owner of the declaration shall be liable for the underlying 556256-6736
information and evidence. EPD Norway shall not be liable with respect
to manufacturer information, life cycle assessment data and
evidences.​
Declared unit: Issue date:
1 pcs Nilo Chair
Declared unit (cradle to gate) with option: Valid to:
A1-A3,A4,A5,B2,B3,B4,C1,C2,C3,C4,D
Year of study:
2022
Functional unit: Comparability:
Production of one Nilo chair, provided and maintained for a period of EPD of construction products may not be comparable if they not
15 years. comply with EN 15804 and seen in a building context.
General information on verification of EPD from EPD tools: Development and verification of EPD:
Independent verification of data, other environmental information The declaration is created using EPD tool lca.tools ver EPD2022.03,
and the declaration according to ISO 14025:2010, § 8.1.3 and § 8.1.4. developed by LCA.no. The EPD tool is integrated in the company's
Verification of each EPD is made according to EPD-Norway’s management system, and has been approved by EPD Norway.
guidelines for verification and approval requiring that tools are i)
integrated into the company's environmental management system, ii) Developer of EPD: Isabell Vesterberg
the procedures for use of the EPD tool are approved by EPD-Norway,
Reviewer of company-specific input data and EPD: Johanna Ljunggren
and iii) the process is reviewed annually by an independent third
party verifier. See Appendix G of EPD-Norway's General Programme
Instructions for further information on EPD tools
Verification of EPD tool: Approved:
Independent third party verification of the EPD tool, background data
and test-EPD in accordance with EPDNorway's procedures and
guidelines for verification and approval of EPD tools. Håkon Hauan, CEO EPD-Norge
Third party verifier:
Elisabet Amat, GREENIZE projects
(no signature required)
2 / 12
Product
Product description:
Nilo wooden shell chair with 4-legged steel underframe with castors. Armrests are available as options. Felt pads and connectors are available as
options for Nilo variants with 4-legged underframe and sledge underframe.
Nilo is a practical and sustainable wooden shell chair in several versions that form a complete family of chairs. Thanks to its simple shape, it has the
flexibility to fit into many different spaces, and is ideal for e.g. dining rooms, cafés and meeting rooms.
Read more: https://www.kinnarps.com/products/seating/chairs/nilo/
Product specification
Nilo is made from renewable FSC®-certified wood, which guarantees responsible forestry with respect to both people and the environment. The
chair is made of a few parts, all of which you can either recycle, separate or replace - making it a circular and sustainable choice. Nilo is available
with wooden seat shell, with or without upholstered seat cushion or fully upholstered.
The back has a natural springiness that counteracts static sitting and increases blood circulation. The contoured seat provides a comfortable
seating, as the user’s weight is distributed over a larger area. The seat shell is available in durable laminate, providing durability in especially tough
spaces. Nilo is available with handles at the back, which makes it easy to move and support yourself on. The chair is stackable and available with
castors, offering flexible environments and space efficient solutions. It can also be hung on tables, which frees up floor space and facilitates
cleaning.
This EPD includes the following variants:
Nilo 4-legged with wooden seat shell,
Nilo 4-legged with upholstered seat cushion in two different fabrics; 100 % recycled polyester fabric or wool-blend fabric,
Nilo 4-legged with completely upholstered seat shell, one variant in 100 % recycled polyester, one in polyester fabric and one in wool-blend fabric,
Nilo with sledge underframe.
Included options are:
Armrests,
Felt pads,
Connectors.
Recycled share in Recycled share in
Materials kg %
material (kg) material (%)
Metal - Steel 2,32 45,84 0,46 20,00
Plastic - Nylon (PA) 0,22 4,36 0,00 0,00
Plastic - Polypropylene (PP) 0,22 4,36 0,00 0,00
Powder coating 0,03 0,49 0,00 0,00
Wood - Plywood 2,27 44,96 0,00 0,00
Total 5,05 0,46
Technical data:
Certifications:
Swedish Möbelfakta,
Nilo is FSC®-certified (FSC®C010544) in all executions.
Fulfilled technical standards:
EN 16139:2013 Furniture - Strength, durability and safety - Requirements for non-domestic seating,
EN 1729 Furniture - Chairs and tables for educational institutions.
Fulfilled fire requirements, for upholstered variants:
EN 1021-1 Assessment of the ignitability of upholstered furniture – Part 1: Ignition source smouldering cigarette, with Kinnarps standard fabrics,
EN 1021-2 Assessment of the ignitability of upholstered furniture – Part 2: Ignition source match flame equivalent, with Kinnarps standard fabrics.
Market:
Mainly Europe, but is available world wide.
Reference service life, product
15 years.
Reference service life, building
LCA: Calculation rules
Declared unit:
1 pcs Nilo Chair
3 / 12
Cut-off criteria:
All major raw materials and all the essential energy is included. The production processes for raw materials and energy flows with very small
amounts (less than 1%) are not included. These cut-off criteria do not apply for hazardous materials and substances.
Allocation:
The allocation is made in accordance with the provisions of EN 15804. Incoming energy and water and waste production in-house is allocated
equally among all products through mass allocation. Effects of primary production of recycled materials is allocated to the main product in which
the material was used. The recycling process and transportation of the material is allocated to this analysis.
Data quality:
Specific data for the product composition are provided by the manufacturer. They represent the production of the declared product and were
collected for EPD development in the year of study. Background data is based on registered EPDs according to EN 15804, Ostfold Research
databases, ecoinvent and other LCA databases. The data quality of the raw materials in A1 is presented in the table below.​
Specific data for the manufacturing processes (product stage A3) refers to the year 2020. All other specific data is from year of study.
Materials Source Data quality Year
Metal - Steel ecoinvent 3.6 Database 2019
Plastic - Nylon (PA) ecoinvent 3.6 Database 2019
Plastic - Polypropylene (PP) ecoinvent 3.6 Database 2019
Powder coating Ecoinvent 3.6 Database 2019
Wood - Plywood modified ecoinvent 3.6 Database 2019
4 / 12
System boundaries (X=included, MND=module not declared, MNR=module not relevant)
Construction Beyond the system
Product stage Use stage End of life stage
installation stage boundaries
A1 A2 A3 A4 A5 B1 B2 B3 B4 B5 B6 B7 C1 C2 C3 C4 D
X X X X X MND X X X MND MND MND X X X X X
System boundary:
The wooden seat shell is bought as a premanufactured component. The upholstering is done at Kinnarps' production site in Skillingaryd, where the
fabric is also processed. Certain steel components are manufactured at Kinnarps' production site in Jönköping and some are purchased as
premanufactured components. Final assembly of the product is done at Kinnarps' production site in Kinnarp.
The flow chart below illustrates the system boundaries of the analysis.
Additional technical information:
waR slairetam tropsnarT gnirutcafunaM tropsnarT ylbmessA e​sU ecnanetniaM riapeR tnemecalpeR tnemhsibrufeR lanoitarepO ygrene esu lanoitarepO esu retaw -eD noitcurtsnoc noitilomed tropsnarT etsaW gnissecorp lasopsiD -yrevoceR-esueR laitnetop-gnilcyceR
5 / 12
LCA: Scenarios and additional technical information
The following information describe the scenarios in the different modules of the EPD.
The product is shipped to the consumer in Kinnarps’ trucks with blankets and cardboard sheets as packaging material which is returned to the
factory after delivery and reused. This method saves 270 kg of packaging material per container and enables 50% more products to be
transported in each truck. Kinnarps’ trucks have a load efficiency of over 90% and are run on diesel with renewable content. For more information
about sustainability at Kinnarps, visit https://www.kinnarps.com/about-kinnarps/sustainability/.
The maintenance scenario includes wet-wiping once a week for the whole reference service life. For upholstered variants, the maintenance scenario
includes vaccum cleaning of textiles once a week for the whole reference service life.
In normal use, no repair or replacement is required during the product's referenced service life.
Capacity utilisation Value
Transport from production place to user (A4) Distance (km) Fuel/Energy Consumption Unit
(incl. return) % (Liter/tonne)
Truck, 16-32 tonnes, HVO, EURO 6 (kgkm) 36,7 % 300 0,043 l/tkm 12,90
Maintenance (B2) Unit Value
Water, tap water (m3) m3/DU 0,78
Capacity utilisation Value
Transport to waste processing (C2) Distance (km) Fuel/Energy Consumption Unit
(incl. return) % (Liter/tonne)
Truck, over 32 tonnes, EURO 6 (km) 53,3 % 85 0,023 l/tkm 1,96
Waste processing (C3) Unit Value
Waste treatment per kg Non-hazardous waste,
kg 0,03
incineration with fly ash extraction - C3 (kg)
Waste treatment per kg Plastics, Mixture,
kg 0,22
municipal incineration with fly ash extraction (kg)
Waste treatment per kg Polypropylene (PP),
kg 0,22
incineration with fly ash extraction - C3 (kg)
Waste treatment per kg Scrap steel, incineration
kg 2,32
with fly ash extraction (kg)
Waste treatment per kg Wood, incineration with
kg 2,27
fly ash extraction (kg)
Waste, materials to recycling (kg) kg 0,79
Disposal (C4) Unit Value
Landfilling of ashes and residues from
kg 1,53
incineration of Scrap steel (kg)
Landfilling of ashes from incineration of Non-
hazardous waste, process per kg ashes and kg 0,01
residues - C4 (kg)
Landfilling of ashes from incineration of Plastics,
Mixture, municipal incineration with fly ash
kg 0,01
extraction, process per kg ashes and residues - C4
(kg)
Landfilling of ashes from incineration of
Polypropylene, PP, process per kg ashes and kg 0,01
residues - C4 (kg)
Landfilling of ashes from incineration of Wood,
kg 0,03
process per kg ashes and residues (kg)
Benefits and loads beyond the system
Unit Value
boundaries (D)
Substitution of electricity, in Norway (MJ) MJ 2,29
Substitution of primary steel with net scrap (kg) kg 0,63
Substitution of thermal energy, district heating, in
MJ 34,65
Norway (MJ)
6 / 12
LCA: Results
The LCA results are presented below for the declared unit defined on page 2 of the EPD document.
Environmental impact
Indicator Unit A1-A3 A4 A5 B2 B3
GWP-total kg CO2 -eq 1,12E+01 5,95E-02 0 2,69E-01 0
GWP-fossil kg CO2 -eq 1,47E+01 5,93E-02 0 2,67E-01 0
GWP-biogenic kg CO2 -eq -3,46E+00 1,01E-04 0 1,68E-03 0
GWP-luluc kg CO2 -eq 3,54E-02 9,25E-05 0 4,35E-04 0
ODP kg CFC11 -eq 1,25E-06 1,22E-08 0 2,37E-08 0
AP mol H+ -eq 7,75E-02 4,16E-04 0 1,56E-03 0
EP-FreshWater kg P -eq 7,81E-04 2,18E-06 0 2,14E-05 0
EP-Marine kg N -eq 1,64E-02 1,10E-04 0 2,48E-04 0
EP-Terrestial mol N -eq 1,83E-01 1,23E-03 0 2,88E-03 0
POCP kg NMVOC -eq 6,30E-02 4,51E-04 0 9,05E-04 0
ADP-minerals&metals1 kg Sb -eq 3,00E-04 7,21E-06 0 7,48E-06 0
ADP-fossil1 MJ 2,34E+02 1,26E+00 0 4,57E+00 0
WDP1 m3 4,29E+03 3,72E+00 0 8,18E+01 0
Indicator Unit B4 C1 C2 C3 C4 D
GWP-total kg CO2 -eq 0 0 3,78E-02 4,96E+00 1,79E-02 -9,00E-01
GWP-fossil kg CO2 -eq 0 0 3,78E-02 1,18E+00 1,79E-02 -8,92E-01
GWP-biogenic kg CO2 -eq 0 0 1,62E-05 3,79E+00 1,33E-05 -7,96E-04
GWP-luluc kg CO2 -eq 0 0 1,15E-05 1,12E-05 5,31E-06 -7,23E-03
ODP kg CFC11 -eq 0 0 9,10E-09 5,32E-09 5,42E-09 -1,46E-02
AP mol H+ -eq 0 0 1,22E-04 6,28E-04 1,24E-04 -5,09E-03
EP-FreshWater kg P -eq 0 0 3,00E-07 1,01E-06 1,81E-07 -6,04E-05
EP-Marine kg N -eq 0 0 2,66E-05 2,92E-04 4,43E-05 -1,25E-03
EP-Terrestial mol N -eq 0 0 2,97E-04 3,09E-03 4,91E-04 -1,31E-02
POCP kg NMVOC -eq 0 0 1,17E-04 7,74E-04 1,41E-04 -5,08E-03
ADP-minerals&metals1 kg Sb -eq 0 0 6,73E-07 2,79E-07 3,02E-07 -1,39E-05
ADP-fossil1 MJ 0 0 6,13E-01 4,52E-01 4,01E-01 -8,69E+00
WDP1 m3 0 0 4,70E-01 1,37E+00 8,41E-01 8,57E-02
GWP-total = Global Warming Potential total; GWP-fossil = Global Warming Potential fossil fuels; GWP-biogenic = Global Warming Potential biogenic; GWP-luluc =
Global Warming Potential land use and land use change; ODP = Depletion potential of the stratospheric ozone layer; AP = Acidification potential, Accumulated
Exceedance; EP-freshwater = Eutrophication potential, fraction of nutrients reaching freshwater end compartment: EP-marine = Eutrophication potential, fraction of
nutrients reaching marine end compartment; EP-terrestrial = Eutrophication potential, Accumulated Exceedance; POCP = Formation potential of tropospheric ozone;
ADP-minerals&metals = Abiotic depletion potential for non-fossil resources; ADP-fossil = Abiotic depletion for fossil resources potential; WDP = Water (user)
deprivation potential, deprivation-weighted water consumption
"Reading example: 9,0 E-03 = 9,0*10-3 = 0,009"
*INA Indicator Not Assessed
1. The results of this environmental impact indicator shall be used with care as the uncertainties on these results are high or as there is limited experienced with the
indicator
Remarks to environmental impacts
7 / 12
Additional environmental impact indicators
Indicator Unit A1-A3 A4 A5 B2 B3
PM Disease incidence 1,57E-06 1,38E-08 0 1,31E-08 0
IRP2 kgBq U235 -eq 1,84E+00 4,10E-03 0 3,16E-02 0
ETP-fw1 CTUe 4,70E+02 1,83E+00 0 4,95E+00 0
HTP-c1 CTUh 6,61E-08 0,00E+00 0 7,39E-10 0
HTP-nc1 CTUh 5,38E-07 3,06E-09 0 1,64E-08 0
SQP1 dimensionless 6,35E+02 2,34E+00 0 1,28E+00 0
Indicator Unit B4 C1 C2 C3 C4 D
PM Disease incidence 0 0 3,47E-09 8,59E-09 2,26E-09 -1,58E-07
IRP2 kgBq U235 -eq 0 0 2,68E-03 1,04E-03 1,61E-03 -1,59E-02
ETP-fw1 CTUe 0 0 4,48E-01 2,69E+00 2,44E-01 -5,42E+01
HTP-c1 CTUh 0 0 0,00E+00 2,36E-10 9,00E-12 -3,61E-09
HTP-nc1 CTUh 0 0 4,34E-10 6,41E-09 2,42E-10 5,73E-08
SQP1 dimensionless 0 0 7,03E-01 8,06E-02 8,80E-01 -1,96E+01
PM = Particulate Matter emissions; IRP = Ionizing radiation – human health; ETP-fw = Eco toxicity – freshwater; HTP-c = Human toxicity – cancer effects; HTP-nc =
Human toxicity – non cancer effects; SQP = Soil Quality (dimensionless)
"Reading example: 9,0 E-03 = 9,0*10-3 = 0,009"
*INA Indicator Not Assessed
1. The results of this environmental impact indicator shall be used with care as the uncertainties on these results are high or as there is limited experienced with the
indicator
2. This impact category deals mainly with the eventual impact of low dose ionizing radiation on human health of the nuclear fuel cycle. It does not consider effects due
to possible nuclear accidents, occupational exposure nor due to radioactive waste disposal in underground facilities. Potential ionizing radiation from the soil, from
radon and from some construction materials is also not measured by this indicator.
8 / 12
Resource use
Indicator Unit A1-A3 A4 A5 B2 B3
PERE MJ 1,38E+02 5,69E-02 0 6,21E-01 0
PERM MJ 3,18E+01 0,00E+00 0 0,00E+00 0
PERT MJ 1,70E+02 5,69E-02 0 6,21E-01 0
PENRE MJ 2,20E+02 1,26E+00 0 4,57E+00 0
PENRM MJ 1,58E+01 0,00E+00 0 0,00E+00 0
PENRT MJ 2,35E+02 1,26E+00 0 4,57E+00 0
SM kg 4,81E-01 0,00E+00 0 0,00E+00 0
RSF MJ 2,44E-01 1,85E-03 0 4,98E-02 0
NRSF MJ 3,42E-01 6,37E-03 0 4,91E-02 0
FW m3 1,79E-01 5,14E-04 0 7,85E-01 0
Indicator Unit B4 C1 C2 C3 C4 D
PERE MJ 0 0 7,71E-03 1,90E-02 7,68E-03 -1,82E+01
PERM MJ 0 0 0,00E+00 -3,18E+01 0,00E+00 0,00E+00
PERT MJ 0 0 7,71E-03 -3,18E+01 7,68E-03 -1,82E+01
PENRE MJ 0 0 6,13E-01 4,55E-01 4,01E-01 -8,69E+00
PENRM MJ 0 0 0,00E+00 -1,58E+01 0,00E+00 0,00E+00
PENRT MJ 0 0 6,13E-01 -1,53E+01 4,01E-01 -8,69E+00
SM kg 0 0 0,00E+00 0,00E+00 0,00E+00 0,00E+00
RSF MJ 0 0 2,70E-04 4,19E-04 2,03E-04 2,19E-02
NRSF MJ 0 0 9,04E-04 0,00E+00 1,76E-02 -3,25E-01
FW m3 0 0 6,98E-05 1,30E-03 3,62E-04 -2,28E-02
PERE = Use of renewable primary energy excluding renewable primary energy resources used as raw materials; PERM = Use of renewable primary energy resources used
as raw materials; PERT = Total use of renewable primary energy resources; PENRE = Use of non renewable primary energy excluding non-renewable primary energy
resources used as raw materials; PENRM = Use of non renewable primary energy resources used as raw materials; PENRT = Total use of non renewable primary energy
resources; SM = Use of secondary materials; RSF = Use of renewable secondary fuels; NRSF = Use of non-renewable secondary fuels; FW = Net use of fresh water
"Reading example: 9,0 E-03 = 9,0*10-3 = 0,009"
*INA Indicator Not Assessed
9 / 12
End of life - Waste
Indicator Unit A1-A3 A4 A5 B2 B3
HWD kg 1,37E-01 1,76E-04 0 8,64E-04 0
NHWD kg 4,73E+00 1,87E-01 0 5,55E-02 0
RWD kg 1,18E-03 5,03E-06 0 2,68E-05 0
Indicator Unit B4 C1 C2 C3 C4 D
HWD kg 0 0 3,36E-05 0,00E+00 1,55E+00 -3,73E-03
NHWD kg 0 0 5,33E-02 2,50E-02 1,97E-02 -3,51E-01
RWD kg 0 0 4,19E-06 0,00E+00 2,46E-06 -1,31E-05
HWD = Hazardous waste disposed; NHWD = Non-hazardous waste disposed; RWD = Radioactive waste disposed
"Reading example: 9,0 E-03 = 9,0*10-3 = 0,009"
*INA Indicator Not Assessed
End of life - Output flow
Indicator Unit A1-A3 A4 A5 B2 B3
CRU kg 0,00E+00 0,00E+00 0 0,00E+00 0
MFR kg 1,23E+00 0,00E+00 0 0,00E+00 0
MER kg 5,12E-06 0,00E+00 0 0,00E+00 0
EEE MJ 4,84E-01 0,00E+00 0 0,00E+00 0
EET MJ 7,33E+00 0,00E+00 0 0,00E+00 0
Indicator Unit B4 C1 C2 C3 C4 D
CRU kg 0 0 0,00E+00 0,00E+00 0,00E+00 0,00E+00
MFR kg 0 0 0,00E+00 7,86E-01 0,00E+00 0,00E+00
MER kg 0 0 0,00E+00 5,05E+00 0,00E+00 0,00E+00
EEE MJ 0 0 0,00E+00 2,34E+00 0,00E+00 0,00E+00
EET MJ 0 0 0,00E+00 3,54E+01 0,00E+00 0,00E+00
CRU = Components for re-use; MFR = Materials for recycling; MER = Materials for energy recovery; EEE = Exported energy electrical; EET = Exported energy thermal
"Reading example: 9,0 E-03 = 9,0*10-3 = 0,009"
*INA Indicator Not Assessed
Biogenic Carbon Content
Indicator Unit At the factory gate
Biogenic carbon content in product kg C 1,03E+00
Biogenic carbon content in accompanying packaging kg C 0,00E+00
Note: 1 kg biogenic carbon is equivalent to 44/12 kg CO2
10 / 12
Additional requirements
Greenhouse gas emissions from the use of electricity in the manufacturing phase
National production mix from import, low voltage (production of transmission lines, in addition to direct emissions and losses in grid) of applied
electricity for the manufacturing process (A3).
Electricity mix Data source Amount Unit
Electricity, Sweden (kWh) ecoinvent 3.6 54,94 g CO2-eq/kWh
Dangerous substances
The product contains substances given by the REACH Candidate list that are less than 0,1 % by weight.
Indoor environment
The product is low-emitting and tested according to Swedish Möbelfakta.
Additional Environmental Information
Key Environmental Indicators
Key environmental indicators Unit A1-A3 A4 A1-C4 A1-D
GWPtotal kg CO2 -eq 11,24 0,06 16,59 15,69
Total energy consumption MJ 358,20 1,32 366,34 339,13
Amount of recycled materials % 9,17
Additional environmental impact indicators required in NPCR Part A for construction products
Indicator Unit A1-A3 A4 A5 B2 B3
GWPIOBC kg CO2 -eq 1,63E+01 5,95E-02 0 2,69E-01 0
Indicator Unit B4 C1 C2 C3 C4 D
GWPIOBC kg CO2 -eq 0 0 3,78E-02 1,15E+00 1,87E-02 -1,24E+00
GWP-IOBC: Global warming potential calculated according to the principle of instantaneous oxidation. In order to increase the transparency of biogenic carbon
contribution to climate impact, the indicator GWP-IOBC is required as it declares climate impacts calculated according to the principle of instantaneous oxidation.
GWP-IOBC is also referred to as GWP-GHG in context to Swedish public procurement legislation.
Variants and Options
Key environmental indicators (A1-A3) for variants of this EPD
Variants
Weight GWPtotal (kg CO2 - Total energy consumption Amount of recycled materials
(kg) eq) (MJ) (%)
Nilo - 4-legged - Wooden seat shell 4,40 6,49 289,79 9,48
Nilo - 4-legged - Upholstered seat cushion - 100 % recycled polyester
5,40 7,45 354,70 11,78
fabric
Nilo - 4-legged - Upholstered seat cushion - Wool blend fabric 5,50 25,88 455,30 7,59
Nilo - 4-legged - Upholstered - 100 % recycled polyester fabric 5,20 11,51 358,14 16,16
Nilo - 4-legged - Upholstered - Wool blend fabric 5,30 46,96 551,42 7,77
Nilo - 4-legged - Upholstered - Polyester fabric 5,20 11,78 382,61 8,00
Nilo - Sledge underframe 5,70 16,77 475,01 12,02
Key environmental indicators (A1-A3) for options for this EPD
Options Weight (kg) GWPtotal (kg CO2 -eq) Total energy consumption (MJ) Amount of recycled materials (%)
Nilo - Armrests, pair 0,50 2,17 39,00 18,35
Nilo - Felt pads, 4 pcs 0,01 0,04 0,79 0,00
Nilo - Connector, 1 pcs 0,13 0,54 10,83 0,00
11 / 12
Bibliography
ISO 14025:2010 Environmental labels and declarations - Type III environmental declarations - Principles and procedures.
ISO 14044:2006 Environmental management - Life cycle assessment - Requirements and guidelines.
EN 15804:2012+A2:2019 Environmental product declaration - Core rules for the product category of construction products.
ISO 21930:2017 Sustainability in buildings and civil engineering works - Core rules for environmental product declarations of construction
products.
ecoinvent v3, Allocation, cut-off by classification, Swiss Centre of Life Cycle Inventories.
Iversen et al., (2021) eEPD v2021.09 Background information for EPD generator tool system verification, LCA.no Report number: 07.21
Ruud et al., (2023) EPD generator for NPCR026 Part B for Furniture - Background information for EPD generator application and LCA data,
LCA.no report number 01.23
NPCR Part A: Construction products and services. Ver. 2.0. March 2021, EPD-Norge.
NPCR 026 Part B for Furniture. Ver. 2.0 March 2022, EPD-Norge.
Program operator and publisher Phone: +47 23 08 80 00
The Norwegian EPD Foundation e-mail: post@epd-norge.no
Post Box 5250 Majorstuen, 0303 Oslo, Norway web: www.epd-norge.no
Owner of the declaration: Phone: +46 515 381 21
Kinnarps AB e-mail: johanna.ljunggren@kinnarps.se
Industrigatan, 521 88 Kinnarp web: kinnarps.com
Author of the Life Cycle Assessment Phone: +47 916 50 916
LCA.no AS e-mail: post@lca.no
Dokka 6B, 1671 web: www.lca.no
Developer of EPD generator Phone: +47 916 50 916
LCA.no AS e-mail: post@lca.no
Dokka 6B,1671 Kråkerøy web: www.lca.no
ECO Platform web: www.eco-platform.org
ECO Portal web: ECO Portal
12 / 12
