Environmental Product
Declaration
In accordance with ISO 14025 and EN 15804 +A2
Owner of the declaration: Product name:
Hunton Fiber AS
Hunton Undertak 18 mm
Program holder and publisher: Hunton Undertak 25 mm
The Norwegian EPD foundation
Declaration number:
NEPD-4038-3072-EN Manufacturer
Hunton Fiber AS
Registration Number:
NEPD-4038-3072-EN
Issue date: 16.12.2022
The Norwegian
Valid to: 16.12.2027
EPD Foundation
ver-210324
General information
Product: Owner of the declaration:
Hunton Fiber AS Hunton Fiber AS
Contact person: Thomas Løkken
Program Operator: Phone: +47 906 33 795
The Norwegian EPD Foundation e-mail: thomas.loekken@hunton.no
Post Box 5250 Majorstuen. 0303 Oslo. Norway
Tlf: +47 23 08 80 00 Manufacturer:
e-mail: post@epd-norge.no Hunton Fiber AS
Declaration Number:
NEPD-4038-3072-EN Place of production:
Gjøvik
This declaration is based on Product
Category Rules: Management system:
ISO 9001 and 50001, Eco-lighthouse, PEFC
NPCR Part A. Construction products and services
vers.2; NPCR 010:03.2022 Part B for building Organisation no:
boards (references to EN 15804 +A2). 964014256
Statements: Issue date:
The owner of the declaration shall be liable for the 16.12.2022
underlying information and evidence. EPD
Norway shall not be liable with respect to Valid to:
manufacturers life cycle assessment data and
16.12.2027
evidence.
Year of study:
Declared unit:
2021
1 kg of installed Hunton Undertak boards.
Comparability:
Declared unit with option:
EPDs from other programs than EPD Norge may
N/A
not be comparable.
Functional unit:
The EPD has been worked out by:
1m2 of installed Hunton Undertak boards, cradle
Maciej Biedacha, Ellen Soldal
to grave with 60 years lifetime.
Verification:
Independent verification of the declaration and
data. according to ISO14025:2010
internal external 
Alexander Borg Approved (Manager of EPD Norway
Alexander Borg, Asplan Viak AS
Independent verifier approved by EPD Norway
EPD for the best environmental decision 2
Product
Product description:
Hunton Undertak™ is a simplified wood fibre sarket underlay and windbarrier sheet combined
in one product.
Product specification:
Calculations have been performed for a declared unit of an average 1 kg of Hunton Undertak
board.
Table 1. Material composition Undertak boards
18 mm Undertak 25 mm Undertak
Materials
kg % kg %
Wood fibre, dry matter 3.28 71.20 4.57 71.89
Water 0.18 4.00 0.25 4.00
Bitumen 0.88 19.09 1.22 19.21
Waste paper 0.11 2.41 0.11 1.75
Other 0.15 3.30 0.20 3.15
Total for product 4.61 100 6.35 100
Plastic packaging 0.01 0.01
Wood packaging 0.07 0.09
Total with packaging 4.69 6.45
The results in this EPD are provided for a declared unit and shall be recalculated to a functional
unit. The table 2 below provides scaling factors to 1 m2 of all Hunton Undertak variants. The
environmental impact of the functional unit (1 m2) can be calculated by multiplying results for
the declared unit (given per 1 kg) by appropriate scaling factor.
Table 2. Scaling factor Hunton Undertak.
Functional
Product Scaling factor
unit
Hunton Undertak 18 mm 1 m2 4.61
Hunton Undertak 25 mm 1 m2 6.35
Technical data:
Property Standard EN Value Unit Tolerance
18 ± 1,2 mm
Thickness 324-1 mm
25 ± 1,8 mm
± 2 mm/m
Width 324-1 595 mm
maks. ± 5 mm
± 2 mm/m
Length 324-1 2420 mm
maks. ± 5 mm
Thermal 0.05*
12667 W/mK -
conductivity λd 0.045**
* Hunton Undertak 18 mm.
**Hunton Undertak 25mm.
EPD for the best environmental decision 3
Hunton Undertak average density ranges from 255 to 260 kg/m³. All relevant technical
information is available in the product’s SINTEF Technical Approval nr. 2190.
Market:
Nordic and European market. Boards are being sold in Scandinavia under tradename Hunton
Undertak™, nonetheless on the other markets Hunton Undertag™ or Sarket™ is being used.
Scenarios assessed in this study were developed for Norway.
Reference service life product:
RSL is assumed to be equal with a reference study period of 60 years for a building.
Reference service life building:
60 years.
LCA: Calculation rules
Functional unit:
1 m2 of installed Hunton Undertak boards, from cradle to grave, with lifetime of 60 years.
Declared unit:
The declared unit used for the calculations was 1 kg of installed Hunton Undertak boards.
Data quality:
The Ecoinvent database (version 3.8) was used as the main source of data for modelling the
background system and the whole value chain. All generic data used in the study are not older
than 10 years. Specific system data were collected by the manufacturer and provided to the
developer of the EPD using an appropriate data collection file. Data were discussed between the
two involved parts to ensure representativity of the system and to produce a reliable model.
Results were compared to similar production systems. Employed data were collected for the
year 2021.
Allocation:
Allocation was done based on specifications stated in the newly published standard EN 15804 +
A2:2019. Energy and water use. as well as generated waste were allocated evenly to the product
using mass allocation. Material recycling and transport was also allocated accordingly.
EPD for the best environmental decision 4
System boundary:
Figure 2. System boundaries.
The studied system includes the following modules: A1(raw materials). A2 (transport of raw
materials). A3 (manufacturing). A4 (transport to the construction site). A5 (Assembly). C1
(disassembly). C2 (transport to waste processing). C3 (waste processing). C4 (waste disposal).
and D (benefits beyond the system boundaries). The above phases were conducted in
accordance with specifications in the new EN15804 + A2:2019 and NPCR Part A Construction
products and services version 2. No scenarios were developed for the use phase (modules B1-
B7) as the environmental impacts are negligible. Hunton Undertak requires no maintenance.
replacement nor additional treatment or energy if properly installed according to the existing
guidelines.
Cut-off criteria:
All the important raw materials and energy use are included in the calculations. For some raw
materials. proxy datasets were used in the model as approximations. This does not include
hazardous materials. The calculations include 100% of materials that make up the product and
the packaging.
LCA: Scenarios and additional technical information
The following information describes the scenarios in the different modules of the EPD.
For transport to a recycling facility. incineration and landfill. distances of 300 and 85 km have
been used in this assessment.
EPD for the best environmental decision 5
Transport from production place to assembly/user (A4)
Fuel/Energy
Capacity utilisation Distance Value
Type Type of vehicle consumption
(incl. return) % (km) (l/t)
(l/tkm)
Euro 6 [> 32t.
Truck 72.6% 300 0.01 6.10
diesel]
The distance of 300 km to the building site is taken as an average distance based on default
values given in NPCR 010 2022 Part B (6.3.8.1).
Assembly (A5)
Unit Value
Material loss kg 0.05
Output materials for waste treatment kg 0.066
Material loss and materials being a subject of waste treatment are reported for a declared unit.
Use phase (B1-B7)
The product does not require any treatment. maintenance or replacement if properly installed.
End of Life (C1, C3, C4)
Unit
kg -
Hazardous waste disposed
kg 1
Collected as mixed construction waste
kg -
Reuse
kg -
Recycling
kg 1
Energy recovery
kg 0.016
To landfill
No hazardous materials are disposed. Scenarios developed for treatment of Hunton Undertak
during waste processing are based on NPCR 010 2022.
Transport to waste processing (C2)
Capacity Fuel/Energy
Distance value
Type utilisation (incl. Type of vehicle consumption
(km) (l/t)
return) % (l/tkm)
Euro 6 [> 32t.
Truck 50% 300 0.01 6.10
diesel]
Euro 6 [> 16-
Truck 50% 85 0.015 2.65
32t. diesel]
Transport for distances refers to recycling and incineration.
EPD for the best environmental decision 6
Benefits and loads beyond the system boundaries (D)
Unit Value
Electricity substitution MJ 1.26
Thermal Heat substitution MJ 14.4
Avoided materials kg 0.001
Electricity and thermal heat substitution data are taken from SSB with 2021 as the basis year.
LCA: Results
The results in this EPD are provided for a declared unit and shall be recalculated to a functional
unit. Table 2 with appropriate scaling factors is presented on page number three.
System boundaries (X=included. MND= module not declared. MNR=module not
relevant)
Benefits
& loads
Assembly
Product stage Use stage End of life stage beoyond
stage
system
boundary
n -
s la ir e t a m w a R t r o p s n a r T g n ir u t c a fu n a M t r o p s n a r T y lb m e s s A e s U e c n a n e t n ia M r ia p e R t n e m e c a lp e R t n e m h s ib r u fe R e s u y g r e n e la n o it a r e p O e s u r e t a w la n o it a r e p O o it ilo m e d n o it c u r t s n eo c - t r o p s n a r T g n is s e c o r p e t s a W la s o p s iD g yn r eil v ec soy uc c ee e RR --la it n e t o p
D R
A1 A2 A3 A4 A5 B1 B2 B3 B4 B5 B6 B7 C1 C2 C3 C4 D
X X X X X X X X X X X X X X X X X
EPD for the best environmental decision 7
Core environmental impact indicators
Indicator Unit A1 A2 A3 A1-A3 A4 A5
GWP-total kg CO2 eq. -1.20E+00 1.45E-02 6.26E-02 -1.13E+00 2.18E-02 6.30E-02
GWP-fossil kg CO2 eq. 1.52E-01 1.45E-02 5.28E-02 2.20E-01 2.18E-02 3.80E-02
GWP-
kg CO2 eq. -1.36E+00 1.54E-05 9.52E-03 -1.35E+00 1.26E-05 2.50E-02
biogenic
GWP-LULUC kg CO2 eq. 5.51E-04 5.45E-06 2.94E-04 8.51E-04 4.93E-06 4.38E-05
ODP kg CFC11 eq. 1.61E-07 3.62E-09 1.88E-09 1.66E-07 5.55E-09 9.14E-09
AP mol H⁺ eq. 1.40E-03 4.63E-05 1.99E-04 1.64E-03 6.77E-05 1.13E-04
EP-
kg P eq. 5.67E-06 1.04E-07 3.99E-06 9.77E-06 2.60E-07 5.73E-07
freshwater
EP-marine kg N eq. 2.00E-04 1.02E-05 3.65E-05 2.47E-04 1.39E-05 2.38E-05
EP-terrestial mol N eq. 2.19E-03 1.13E-04 4.42E-04 2.74E-03 1.60E-04 2.67E-04
kg NMVOC
POCP 1.16E-03 4.46E-05 1.19E-04 1.32E-03 6.35E-05 1.02E-04
eq.
ADP-M&M kg Sb eq. 7.45E-07 3.47E-08 1.47E-06 2.26E-06 4.45E-08 1.25E-07
ADP-fossil MJ 1.01E+01 2.36E-01 8.73E-01 1.12E+01 3.65E-01 6.15E-01
WDP m³ 2.19E-01 8.13E-04 5.30E-02 2.73E-01 2.01E-03 5.96E-02
Indicator Unit B1-B7 C1 C2 C3 C4 D
GWP-total kg CO2 eq. 0.00E+00 1.40E-04 1.39E-02 1.79E+00 6.64E-04 -2.74E-01
GWP-fossil kg CO2 eq. 0.00E+00 1.33E-04 1.38E-02 4.93E-01 6.65E-04 -1.39E-01
GWP-
kg CO2 eq. 0.00E+00 5.70E-06 1.26E-05 1.30E+00 -3.21E-07 -1.29E-01
biogenic
GWP-
kg CO2 eq. 0.00E+00 7.20E-07 5.54E-06 1.12E-05 1.69E-08 -6.57E-03
LULUC
kg CFC11
ODP 0.00E+00 5.24E-12 3.21E-09 6.05E-09 2.34E-10 -1.75E-08
eq.
AP mol H⁺ eq. 0.00E+00 9.79E-07 3.93E-05 4.52E-04 5.01E-06 -1.32E-03
EP-
kg P eq. 0.00E+00 7.15E-09 9.87E-08 1.23E-06 8.01E-09 -1.20E-05
freshwater
EP-marine kg N eq. 0.00E+00 1.11E-07 7.81E-06 1.82E-04 1.98E-06 -4.93E-04
EP-
mol N eq. 0.00E+00 1.40E-06 8.71E-05 2.06E-03 2.18E-05 -5.28E-03
terrestrial
kg NMVOC
POCP 0.00E+00 3.85E-07 3.35E-05 5.42E-04 6.62E-06 -1.46E-03
eq.
ADP-M&M kg Sb eq. 0.00E+00 1.55E-08 4.91E-08 1.15E-07 7.26E-10 -8.72E-07
ADP-fossil MJ 0.00E+00 2.20E-03 2.10E-01 3.50E-01 1.77E-02 -2.21E+00
WDP m³ 0.00E+00 1.36E-04 6.39E-04 9.12E-01 3.50E-02 -6.19E-02
GWP-total: Global Warming Potential; GWP-fossil: Global Warming Potential fossil fuels; GWP-biogenic: Global Warming Potential
biogenic; GWP-LULUC: Global Warming Potential land use and land use change; ODP: Depletion potential of the stratospheric ozone
layer; AP: Acidification potential. Accumulated Exceedance; EP-freshwater: Eutrophication potential. fraction of nutrients reaching
freshwater end compartment; See “additional Norwegian requirements” for indicator given as PO4 eq. EP-marine: Eutrophication
potential. fraction of nutrients reaching freshwater end compartment; EP-terrestrial: Eutrophication potential. Accumulated
Exceedance; POCP: Formation potential of tropospheric ozone; ADP-M&M: Abiotic depletion potential for non-fossil resources
(minerals and metals); ADP-fossil: Abiotic depletion potential for fossil resources; WDP: Water deprivation potential. deprivation
weighted water consumption
EPD for the best environmental decision 8
Additional environmental impact indicators
Indicator Unit A1 A2 A3 A1-A3 A4 A5
Disease
PM 8.82E-09 1.68E-09 2.22E-09 1.27E-08 2.44E-09 1.04E-09
incidence
IRP kBq U235 eq. 4.19E-02 1.02E-03 1.92E-02 6.21E-02 1.69E-03 3.34E-03
ETP-fw CTUe 5.60E+00 1.85E-01 1.17E+00 6.95E+00 2.25E-01 4.24E-01
HTP-c CTUh 9.58E-11 5.03E-12 7.83E-11 1.79E-10 6.43E-12 2.75E-11
HTP-nc CTUh 2.37E-09 1.94E-10 1.20E-09 3.76E-09 2.86E-10 3.10E-10
SQP Dimensionless 8.81E+01 2.70E-01 3.04E-01 8.87E+01 4.24E-01 4.47E+00
Indicator Unit B1-B7 C1 C2 C3 C4 D
PM Disease incidence 0.00E+00 8.09E-12 1.11E-09 3.61E-09 9.27E-11 -9.62E-08
IRP kBq U235 eq. 0.00E+00 4.64E-05 9.11E-04 1.54E-03 2.84E-05 -1.39E-02
ETP-fw CTUe 0.00E+00 6.82E-03 1.65E-01 1.02E+00 2.02E-02 -1.36E+01
HTP-c CTUh 0.00E+00 4.26E-13 5.30E-12 3.47E-10 1.47E-12 -2.20E-10
HTP-nc CTUh 0.00E+00 9.52E-12 1.66E-10 1.51E-09 4.94E-11 -1.30E-08
SQP Dimensionless 0.00E+00 9.58E-04 1.46E-01 9.82E-02 3.45E-02 -1.83E+01
PM: Particulate matter emissions; IRP: Ionising radiation. human health; ETP-fw: Ecotoxicity (freshwater);
HTP-c: Human toxicity. cancer effects; HTP-nc: Human toxicity. non-cancer effects; SQP: Land use related
impacts / soil quality
EPD for the best environmental decision 9
Classification of disclaimers to the declaration of core and additional environmental
impact indicators
ILCD
Indicator Disclaimer
classification
Global warming potential (GWP) None
ILCD type / level
Depletion potential of the stratospheric ozone layer (ODP) None
1
Potential incidence of disease due to PM emissions (PM) None
Acidification potential. Accumulated Exceedance (AP) None
Eutrophication potential. Fraction of nutrients reaching freshwater end
None
compartment (EP-freshwater)
Eutrophication potential. Fraction of nutrients reaching marine end
None
ILCD type / level compartment (EP-marine)
2
Eutrophication potential. Accumulated Exceedance (EP-terrestrial) None
Formation potential of tropospheric ozone (POCP) None
Potential Human exposure efficiency relative to U235 (IRP) 1
Abiotic depletion potential for non-fossil resources (ADP-minerals&metals) 2
Abiotic depletion potential for fossil resources (ADP-fossil) 2
Water (user) deprivation potential. deprivation-weighted water consumption
2
(WDP)
ILCD type / level
Potential Comparative Toxic Unit for ecosystems (ETP-fw) 2
3
Potential Comparative Toxic Unit for humans (HTP-c) 2
Potential Comparative Toxic Unit for humans (HTP-nc) 2
Potential Soil quality index (SQP) 2
Disclaimer 1 – This impact category deals mainly with the eventual impact of low dose ionizing radiation on
human health of the nuclear fuel cycle. It does not consider effects due to
possible nuclear accidents. occupational exposure nor due to radioactive waste disposal in underground facilities.
Potential ionizing radiation from the soil. from radon and from some
construction materials are also not measured by this indicator.
Disclaimer 2 – The results of this environmental impact indicator shall be used with care as the uncertainties on
these results are high or as there is limited experienced with the indicator
EPD for the best environmental decision 10
Resource use
Parameter Unit A1 A2 A3 A4 A5
RPEE MJ 1.51E+01 3.02E-03 8.86E+00 2.40E+01 6.45E-03
RPEM MJ 0.00E+00 0.00E+00 0.00E+00 0.00E+00 0.00E+00
TPE MJ 1.51E+01 3.02E-03 8.86E+00 2.40E+01 6.45E-03
NRPE MJ 1.01E+01 2.36E-01 8.73E-01 1.12E+01 3.65E-01
NRPM MJ 0.00E+00 0.00E+00 0.00E+00 0.00E+00 0.00E+00
TRPE MJ 1.01E+01 2.36E-01 8.73E-01 1.12E+01 3.65E-01
SM kg 2.08E-02 0.00E+00 0.00E+00 2.08E-02 0.00E+00
RSF MJ 0.00E+00 0.00E+00 0.00E+00 0.00E+00 0.00E+00
NRSF MJ 0.00E+00 0.00E+00 0.00E+00 0.00E+00 0.00E+00
W m3 5.26E-03 2.81E-05 6.49E-02 7.02E-02 7.77E-05
Parameter Unit B1-B7 C1 C2 C3 C4 D
RPEE MJ 0.00E+00 2.12E-02 3.01E-03 1.46E+01 2.08E-04 -1.41E+01
RPEM MJ 0.00E+00 0.00E+00 0.00E+00 0.00E+00 0.00E+00 0.00E+00
TPE MJ 0.00E+00 2.12E-02 3.01E-03 1.46E+01 2.08E-04 -1.41E+01
NRPE MJ 0.00E+00 2.21E-03 2.10E-01 3.50E-01 1.77E-02 -2.21E+00
NRPM MJ 0.00E+00 0.00E+00 0.00E+00 0.00E+00 0.00E+00 0.00E+00
TRPE MJ 0.00E+00 2.21E-03 2.10E-01 3.50E-01 1.77E-02 -2.21E+00
SM kg 0.00E+00 0.00E+00 0.00E+00 0.00E+00 0.00E+00 0.00E+00
RSF MJ 0.00E+00 0.00E+00 0.00E+00 0.00E+00 0.00E+00 -6.84E-04
NRSF MJ 0.00E+00 0.00E+00 0.00E+00 0.00E+00 0.00E+00 0.00E+00
W m3 0.00E+00 1.56E-04 2.38E-05 2.16E-02 8.16E-04 -4.03E-02
RPEE Renewable primary energy resources used as energy carrier; RPEM Renewable primary energy resources used as raw materials;
TPE Total use of renewable primary energy resources; NRPE Nonrenewable primary energy resources used as energy carrier; NRPM
Nonrenewable primary energy resources used as materials; TRPE Total use of nonrenewable primary energy resources; SM Use of
secondary materials; RSF Use of renewable secondary fuels; NRSF Use of nonrenewable secondary fuels; W Use of net fresh water
EPD for the best environmental decision 11
End of life - Waste
Parameter Unit A1 A2 A3 A1-A3 A4 A5
HW kg 2.06E-04 5.72E-07 7.15E-07 2.08E-04 1.86E-07 1.05E-05
NHW kg 3.91E-02 2.35E-02 8.42E-02 1.47E-01 3.35E-02 1.56E-02
RW kg 6.77E-05 1.60E-06 9.12E-06 7.84E-05 2.56E-06 4.23E-06
Parameter Unit B1-B7 C1 C2 C3 C4 D
HW kg 0.00E+00 2.09E-09 5.48E-07 1.09E-06 7.50E-09 -2.08E-06
NHW kg 0.00E+00 3.69E-04 1.24E-02 1.08E-01 7.52E-02 -7.65E-02
RW kg 0.00E+00 2.22E-08 1.42E-06 1.45E-06 1.70E-08 -1.15E-05
HW Hazardous waste disposed; NHW Non-hazardous waste disposed; RW Radioactive waste disposed
End of life – output flow
Parameter Unit A1 A2 A3 A1-A3 A4 A5
CR kg 0.00E+00 0.00E+00 0.00E+00 0.00E+00 0.00E+00 0.00E+00
MR kg 0.00E+00 0.00E+00 0.00E+00 0.00E+00 0.00E+00 0.00E+00
MER kg 0.00E+00 0.00E+00 0.00E+00 0.00E+00 0.00E+00 0.00E+00
EEE MJ 0.00E+00 0.00E+00 0.00E+00 0.00E+00 0.00E+00 6.78E-02
ETE MJ 0.00E+00 0.00E+00 0.00E+00 0.00E+00 0.00E+00 6.60E-01
Parameter Unit B1-B7 C1 C2 C3 C4 D
CR kg 0.00E+00 0.00E+00 0.00E+00 0.00E+00 0.00E+00 0.00E+00
MR kg 0.00E+00 0.00E+00 0.00E+00 0.00E+00 0.00E+00 0.00E+00
MER kg 0.00E+00 0.00E+00 0.00E+00 0.00E+00 0.00E+00 0.00E+00
EEE MJ 0.00E+00 0.00E+00 0.00E+00 1.36E+00 0.00E+00 -1.26E+00
ETE MJ 0.00E+00 0.00E+00 0.00E+00 1.32E+01 0.00E+00 -1.44E+01
CR Components for reuse; MR Materials for recycling; MER Materials for energy recovery; EEE Exported
electric energy; ETE Exported thermal energy
Reading example: 9.0 E-03 = 9.0*10-3 = 0.009
Information describing the biogenic carbon content at the factory gate
Biogenic carbon content Unit Value
Biogenic carbon content in the product kg C 0.368
Biogenic carbon content in the accompanying packaging kg C 0.006
EPD for the best environmental decision 12
Additional Norwegian requirements
Greenhouse gas emissions from the use of electricity in the manufacturing phase
For the calculation electricity with certificate of origins has been applied (A3).
National electricity grid Unit Value
El-mix low-voltage Norway (ecoinvent 3.8) g CO2 -eq/kWh 26
El-mix medium-voltage Norway (ecoinvent 3.8) g CO2 -eq/kWh 23
Additional environmental impact indicators required in NPCR Part A for construction
products
In order to increase the transparency of biogenic carbon contribution to climate impact. the
indicator for GWP has been sub-divided into the following:
GWP-IOBC Climate impacts calculated according to the principle of instantaneous oxidation
GWP-BC Climate impacts from the net uptake and emission of biogenic carbon from each
module.
In addition. EP-freshwater shall also be declared as PO4 eq.
Indicator Unit A1 A2 A3 A1-A3 A4 A5
EP-
kg PO4 eq. 1,37E-04 5,04E-06 2,90E-04 4,32E-04 7,59E-06 2,64E-05
freshwater*
GWP-IOBC kg CO2 eq. 1,53E-01 1,45E-02 5,47E-02 2,22E-01 2,18E-02 3,81E-02
GWP-BC kg CO2 eq. -1,36E+00 9,67E-06 7,92E-03 -1,35E+00 4,95E-06 2,49E-02
GWP kg CO2 eq. -1,20E+00 1,45E-02 6,26E-02 -1,13E+00 2,18E-02 6,30E-02
Indicator Unit B1-B7 C1 C2 C3 C4 D
EP- kg PO4
0,00E+00 7,74E-08 4,10E-06 7,29E-05 7,36E-07 -3,09E-04
freshwater* eq.
kg CO2
GWP-IOBC 0,00E+00 1,37E-04 1,39E-02 4,93E-01 6,65E-04 -1,49E-01
eq.
kg CO2
GWP-BC 0,00E+00 2,39E-06 7,27E-06 1,30E+00 -5,92E-07 -1,25E-01
eq.
kg CO2
GWP 0,00E+00 1,40E-04 1,39E-02 1,79E+00 6,64E-04 -2,74E-01
eq.
EP-freshwater* Eutrophication potential. fraction of nutrients reaching freshwater end compartment. Declared as PO4 eq. GWP-IOBC
Global warming potential calculated according to the principle of instantaneous oxidation. GWP-BC Global warming potential from net
uptake and emissions of biogenic carbon from the materials in each module. GWP Global warming potential
EPD for the best environmental decision 13
Hazardous substances
The declaration is based upon reference to threshold values and/or test results and/or material
safety data sheets provided to EPD verifiers. Documentation available upon request to EPD
owner.
□ The product contains no substances given by the REACH Candidate list or the
Norwegian priority list.
 The product contains substances given by the REACH Candidate list or the Norwegian
priority list that are less than 0.1 % by weight.
□ The product contains dangerous substances more than 0.1% by weight, given by the
REACH Candidate List or the Norwegian Priority list, see table.
□ The product contains no substances given by the REACH Candidate list or the
Norwegian priority list. The product is classified as hazardous waste (Avfallsforskiften.
Annex III). see table.
According to SINTEF Technical Approval nr 2190 Hunton Undertak does not contain any
substances from the priority list in quantities which might be assessed as hazardous for health
or environment.
Indoor environment
The product meets the M1 requirements specified in the classification of indoor air 2018 as well
as in the general specifications for the classification of buildings.
Carbon footprint
Calculations related to climate change and global warming potential (GWP) include greenhouse
gas emissions from fossil sources and land use change connected to extraction of raw materials.
Biogenic emissions of CO2 are also calculated and included.
EPD for the best environmental decision 14
Bibliography
ISO 14025:2010 Environmental labels and declarations - Type III environmental
declarations - Principles and procedures
ISO 14044:2006 Environmental management - Life cycle assessment -
Requirements and guidelines
ISO 9001:2015 Quality management system
ISO 50001:2018 Energy management system
EN 15804:2012+A2:2019 Sustainability of construction works - Environmental product
declaration - Core rules for the product category of construction
products
Eco-Lighthouse Certification Environmental management certificate
(2021)
ISO 21930:2007 Sustainability in building construction - Environmental
declaration of building products
NPCR PART A: Construction products and services Version: 2.0
NPCR 010:2022 Part B for building boards (references to EN 15804 +A2)
PEFC ST 2002:2013 Chain of custody of forest-based products
Raadal. H. L. et al (2009) Klimaregnskap for avfallshåndtering. Fase I og II.
Oppdragsrapport nr. 18.09 fra Østfoldforskning. Norge.
SSB (2022) Tabell 04727 F Balance of district heating (GWh), by district
heating, contents and year. For year 2021.
SSB (2022) Tabell 04730 Consumption of fuel used for gross production of
district heating (GWh), by type of energy, contents, and year. For
year 2021.
SSB (2022) Tabell 09469 Net production of district heating, by type of heat
central (GWh). For year 2021.
SINTEF Certification (2021) SINTEF Technical Approval nr .2190 Hunton Undetak / Hunton
Sarket
EPD for the best environmental decision 15
Program Operator tlf +47 23 08 80 00
The Norwegian EPD Foundation
Post Box 5250 Majorstuen. 0303 Oslo e-mail: post@epd-norge.no
Norway web www.epd-norge.no
Publisher tlf +47 23 08 80 00
The Norwegian EPD Foundation
Post Box 5250 Majorstuen. 0303 Oslo e-mail: post@epd-norge.no
Norway web www.epd-norge.no
Owner of the declaration tlf +47 61 13 47 00
Hunton Fiber AS Fax +47 61 13 47 10
Postbox 633 e-mail: hunton@hunton.no
2808 Gjøvik. Norway web www.hunton.no
Author of the life cycle assessment tlf +47 69 35 11 00
NORSUS Fax +47 69 34 24 94
Norsk institutt for bærekraftsforskning e-mail: post@norsus.no
Stadion 4. 1671 Kråkerøy. Norway web www.norsus.no
EPD for the best environmental decision 16
EPD for the best
environmental
decision
The Norwegian EPD foundation
www.epd-norge.no
EPD for the best environmental decision 17
