Environmental product declaration
in accordance with ISO 14025 and EN 15804+A2
Nordic CL3 Air Handling Unit
Owner of the declaration: Program operator:
Flexit AS The Norwegian EPD Foundation
Product: Declaration number:
Nordic CL3 Air Handling Unit
Registration number:
Declared unit:
1 pcs Issue date:
This declaration is based on Product Category Rules: Valid to:
CEN Standard EN 15804:2012+A2:2019 serves as core
EPD software:
PCR
The Norwegian EPD Foundation LCAno EPD generator ID: 484906
NPCR 030:2021 Part B for ventilation components
1 / 13
General information
Product Owner of the declaration:
Nordic CL3 Air Handling Unit Flexit AS
Contact person: Anton Olsson
Phone: +46761325238
e-mail: anton.olsson@flexit.no
Program operator: Manufacturer:
The Norwegian EPD Foundation Flexit AB
Post Box 5250 Majorstuen, 0303 Oslo, Norway
Phone: +47 977 22 020
web: www.epd-norge.no
Declaration number: Place of production:
Flexit AB
Källhultsvängen 5B
672 41 Töcksfors, Sweden
This declaration is based on Product Category Rules: Management system:
CEN Standard EN 15804:2012+A2:2019 serves as core PCR ISO 14001 : 2015 iaf
NPCR 030:2021 Part B for ventilation components
Statement of liability: Organisation no:
The owner of the declaration shall be liable for the underlying 502066-4826
information and evidence. EPD Norway shall not be liable with respect
to manufacturer information, life cycle assessment data and
evidences.​
Declared unit: Issue date:
1 pcs Nordic CL3 Air Handling Unit
Declared unit with option: Valid to:
A1-A3,A4,C1,C2,C3,C4,D
Year of study:
2022
Functional unit: Comparability:
EPD of construction products may not be comparable if they not
comply with EN 15804 and seen in a building context.
General information on verification of EPD from EPD tools: Development and verification of EPD:
Independent verification of data, other environmental information The declaration is created using EPD tool lca.tools ver EPD2022.03,
and the declaration according to ISO 14025:2010, § 8.1.3 and § 8.1.4. developed by LCA.no. The EPD tool is integrated in the company's
Verification of each EPD is made according to EPD-Norway’s management system and has been approved by EPD Norway.
guidelines for verification and approval requiring that tools are i) NEPDT46 VKEs EPD-generator
integrated into the company's environmental management system, ii)
the procedures for use of the EPD tool are approved by EPD-Norway, Developer of EPD: Alva Träff
and iii) the process is reviewed annually by an independent third
Reviewer of company-specific input data and EPD:​ Anton Olsson
party verifier. See Appendix G of EPD-Norway's General Programme
Instructions for further information on EPD tools
Verification of EPD tool: Approved:
Independent third party verification of the EPD tool, background data
and test-EPD in accordance with EPDNorway's procedures and
guidelines for verification and approval of EPD tools.
Third party verifier:
Alexander Borg, Asplan Viak AS
(no signature required)
2 / 13
Product
Product description:
Flexit Nordic CL3 ventilation unit is developed to be energy efficient in the Nordic climate. Suitable for apartments, detached houses, villas and
small commercial buildings. Connection option for the cooker hood with bypass solution. Highly efficient rotating heat exchangers, with
temperature efficiency up to 85%, and fans with low energy consumption. The low building height makes the unit excellent for suspended ceiling
mounting or mounting in the attic. With a configurable door, you can choose which way the door should open. Controlled as standard via the
Flexit GO app and can be supplemented with various accessories, wireless or wired, e.g. humidifier, CO2 sensor etc. The automation is prepared for
local demand control. Cooling recovery is a standard function.
Can be installed both in cold attics and in suspended ceilings
- Low weight and height < 30 cm
- Built-in humidity sensor
- Configurable door solution
- Very quiet, below 35 dB(A) 10m2 Sabine
- Control via app and cloud services
Product specification
Materials kg %
Electronic - Unspecified 1,70 3,00
Filter, mineral based 0,67 1,18
Filter, plastic based 1,35 2,38
Insulation, Plastic based 0,15 0,27
Metal - Aluminium 6,00 10,58
Metal - Copper 1,10 1,94
Metal - Stainless steel 0,28 0,49
Metal - Steel 40,90 72,13
Motor 2,03 3,58
Plastic - Acrylonitrile butadiene
0,78 1,38
styrene (ABS)
Plastic - Polyamide 0,17 0,29
Plastic - Polyethylene 0,23 0,41
Plastic - Polypropylene (PP) 0,04 0,06
Plastic - Polystyrene (PS) 0,41 0,72
Plastic - Polyvinyl chloride (PVC) 0,31 0,55
Rubber, synthetic 0,15 0,27
Sealant 0,40 0,71
Textile - Polyester (PE) 0,04 0,07
Total 56,70 100,00
Packaging kg %
Packaging - Cardboard 3,20 34,26
Packaging - Pallet 6,00 64,24
Packaging - Plastic 0,14 1,50
Total incl. packaging 66,04 100,00
Technical data:
Please visit our webpage and find the technical data specification under the product description
www.flexit@.com
Market:
Europe
Reference service life, product
25 years;
The reference service life depends on the area of use
Reference service life, building or construction works
60 years;
The reference service life depends on the area of use
LCA: Calculation rules
Declared unit:
1 pcs Nordic CL3 Air Handling Unit
3 / 13
Cut-off criteria:
All major raw materials and all the essential energy is included. The production processes for raw materials and energy flows with very small
amounts (less than 1%) are not included. These cut-off criteria do not​ apply for hazardous materials and substances.
Allocation:
The allocation is made in accordance with the provisions of EN 15804. Energy, water and waste production in-house is allocated equally among all
products through mass allocation. Effects of primary production of recycled materials is allocated to the main product in which the material was
used. The recycling process and transportation of the material is allocated to this analysis.
Data quality:
Specific data for the product composition are provided by the manufacturer. The data represent the production of the declared product and were
collected for EPD development in the year of study. Background data is based on EPDs according to EN 15804 and different LCA databases. The
data quality of the raw materials in A1 is presented in the table below.
Materials Source Data quality Year
Electronic - Unspecified ecoinvent 3.6 Database 2019
Filter, mineral based ecoinvent 3.6 Database 2019
Filter, plastic based ecoinvent 3.6 Database 2019
Filter, plastic based Modified ecoinvent 3.6 Database 2019
Insulation, Plastic based ecoinvent 3.6 Database 2019
Metal - Aluminium ecoinvent 3.6 Database 2019
Metal - Copper ecoinvent 3.6 Database 2019
Metal - Stainless steel ecoinvent 3.6 Database 2019
Metal - Steel ecoinvent 3.6 Database 2019
Motor Modified ecoinvent 3.6 Database 2019
Packaging - Cardboard ecoinvent 3.6 Database 2019
Packaging - Pallet Modified ecoinvent 3.6 Database 2019
Packaging - Plastic ecoinvent 3.6 Database 2019
Plastic - Acrylonitrile butadiene styrene (ABS) ecoinvent 3.6 Database 2019
Plastic - Polyamide ecoinvent 3.6 Database 2019
Plastic - Polyethylene ecoinvent 3.6 Database 2019
Plastic - Polypropylene (PP) ecoinvent 3.6 Database 2019
Plastic - Polystyrene (PS) ecoinvent 3.6 Database 2019
Plastic - Polyvinyl chloride (PVC) ecoinvent 3.6 Database 2019
Rubber, synthetic ecoinvent 3.6 Database 2019
Sealant ecoinvent 3.6 Database 2019
Textile - Polyester (PE) ecoinvent 3.6 Database 2019
4 / 13
System boundaries (X=included, MND=module not declared, MNR=module not relevant)
Construction Beyond the system
Product stage Use stage End of life stage
installation stage boundaries
A1 A2 A3 A4 A5 B1 B2 B3 B4 B5 B6 B7 C1 C2 C3 C4 D
X X X X MND MND MND MND MND MND MND MND X X X X X
System boundary:
A1 includes the extraction and production of all raw materials used in the product
A2 includes all types of transportation methods used for the raw materials to the production site in Töcksfors, Sweden
A3 includes the manufacturing and packaging process of the air handling unit
A4 includes the transport to the market/user
A5 modules not declared.
B1 - B7 modules not declared
C1 - C4 includes the use of energy and other auxiliary materials required to demolish the building or construction in which the product is included,
as well as transport from the building site to the waste processing facility, distribution of the product to different waste treatment methods and the
disposal
D includes energy and materials that have achieved a new function and are no longer considered waste
Additional technical information:
During the lifetime of the air handling unit, some parts, such as the filters, will need to be replaced minimum once a year.
For a full account of maintenance information, please visit our website:
www.flexit.com
waR slairetam tropsnarT gnirutcafunaM tropsnarT ylbmessA e​sU ecnanetniaM riapeR tnemecalpeR tnemhsibrufeR lanoitarepO ygrene esu lanoitarepO esu retaw -eD noitcurtsnoc noitilomed tropsnarT etsaW gnissecorp lasopsiD -yrevoceR-esueR laitnetop-gnilcyceR
5 / 13
LCA: Scenarios and additional technical information
The following information describe the scenarios in the different modules of the EPD.
A2: The transport methods used then there were no available data from the suppliers, were assumed to be:
Sweden, Finland and Norway - Class EURO 6 trucks
Thailand, Vietnam and Taiwan - Class EURO 4 trucks
Remaining countries - Class EURO 5 trucks
Distances with seagoing vessels - Ship, Freight, Transoceanic (km)
A3: The energy used in manufacturing were calculated by: the total yearly energy consumption (kWh) divided by the total yearly production of air
handling units (kg).
A4: For the Nordic market, the default average travel distance from the manufacturing site to the building site is 300 km provided in NPCR 030
Part B for ventilation components.
C2: The average distance used from the deconstruction site to the waste processing facility is 85 km for the Norwegian market.
Capacity utilisation Value
Transport from production place to user (A4) Distance (km) Fuel/Energy Consumption Unit
(incl. return) % (Liter/tonne)
Truck, 16-32 tonnes, EURO 6 (km) 36,7 % 300 0,043 l/tkm 12,90
De-construction demolition (C1) Unit Value
Demolition of building per kg of ventilation
kg/DU 59,27
product (kg)
Capacity utilisation Value
Transport to waste processing (C2) Distance (km) Fuel/Energy Consumption Unit
(incl. return) % (Liter/tonne)
Truck, 16-32 tonnes, EURO 6 (km) 36,7 % 85 0,043 l/tkm 3,66
Waste processing (C3) Unit Value
Materials to recycling (kg) kg 45,46
Waste treatment per kg Bulk iron waste, excluding
kg 2,03
reinforcement, sorting plant (kg)
Waste treatment per kg Electronics scrap, Control
kg 1,70
units, incineration (kg)
Waste treatment per kg Expanded Polystyrene
kg 0,21
(EPS), incineration with fly ash extraction (kg)
Waste treatment per kg Plastics, to incineration
kg 1,80
(kg)
Waste treatment per kg Polyethylene (PE),
kg 0,12
incineration (kg)
Waste treatment per kg Polypropylene (PP),
kg 0,09
incineration (kg)
Waste treatment per kg Polyvinylchloride (PVC),
kg 0,31
incineration with fly ash extraction (kg)
Waste treatment per kg Rubber, municipal
kg 0,15
incineration with fly ash extraction (kg)
6 / 13
Disposal (C4) Unit Value
Landfilling of ashes from incineration of
Electronics scrap, Control units, process of ashes kg 1,19
and residues (kg)
Landfilling of ashes from incineration of
Expanded polystyrene (EPS), process per kg ashes kg 0,01
and residues (kg)
Landfilling of ashes from incineration of Plastics,
kg 0,04
process per kg ashes and residues (kg)
Landfilling of ashes from incineration of
Polyethylene (PE), process per kg ashes and kg 0,00
residues (kg)
Landfilling of ashes from incineration of
Polypropylene (PP), process per kg ashes and kg 0,00
residues (kg)
Landfilling of ashes from incineration of
Polyvinylchloride (PVC), process per kg ashes and kg 0,05
residues (kg)
Landfilling of ashes from incineration of Rubber,
kg 0,01
municipal incineration with fly ash extraction (kg)
Waste treatment per kg Copper slag, to landfill,
kg 0,14
residual material landfill (kg) - GLO
Waste, aluminium, to landfill (kg) kg 0,43
Waste, Expanded polystyrene, EPS, to landfill (kg) kg 0,21
Waste, mineral wool, to landfil (kg) kg 0,67
Waste, plastic, mixture, to landfill (kg) kg 1,16
Waste, scrap steel, to landfill (kg) kg 4,27
Benefits and loads beyond the system
Unit Value
boundaries (D)
Substitution of electricity, in Norway (MJ) MJ 1,21
Substitution of primary aluminium with net scrap
kg 5,59
(kg)
Substitution of primary copper with net scrap (kg) kg 0,54
Substitution of primary steel with net scrap (kg) kg 35,63
Substitution of thermal energy, district heating, in
MJ 18,24
Norway (MJ)
7 / 13
LCA: Results
The LCA results are presented below for the declared unit defined on page 2 of the EPD document.
Environmental impact
Indicator Unit A1-A3 A4 C1 C2 C3 C4 D
GWP-total kg CO2 -eq 2,72E+02 3,24E+00 7,82E-02 9,18E-01 8,32E+00 3,48E-01 -9,15E+01
GWP-fossil kg CO2 -eq 2,84E+02 3,24E+00 7,82E-02 9,17E-01 8,32E+00 3,48E-01 -9,03E+01
GWP-biogenic kg CO2 -eq -1,30E+01 1,34E-03 1,47E-05 3,80E-04 6,89E-04 2,76E-04 -2,56E-01
GWP-luluc kg CO2 -eq 1,52E+00 1,15E-03 6,16E-06 3,26E-04 1,82E-04 6,67E-05 -9,66E-01
ODP kg CFC11 -eq 2,24E-05 7,33E-07 1,69E-08 2,08E-07 5,88E-08 2,41E-08 -7,71E-03
AP mol H+ -eq 3,08E+00 9,30E-03 8,18E-04 2,64E-03 1,84E-03 6,83E-04 -7,51E-01
EP-FreshWater kg P -eq 3,05E-02 2,59E-05 2,84E-07 7,33E-06 6,87E-06 2,38E-06 -5,82E-03
EP-Marine kg N -eq 3,48E-01 1,84E-03 3,61E-04 5,21E-04 6,87E-04 3,61E-04 -9,20E-02
EP-Terrestial mol N -eq 6,11E+00 2,06E-02 3,96E-03 5,83E-03 7,05E-03 2,40E-03 -1,02E+00
POCP kg NMVOC -eq 1,33E+00 7,89E-03 1,09E-03 2,23E-03 1,77E-03 7,12E-04 -3,93E-01
ADP-minerals&metals1 kg Sb-eq 7,98E-02 8,94E-05 1,20E-07 2,53E-05 3,26E-06 1,03E-06 -1,83E-03
ADP-fossil1 MJ 3,92E+03 4,89E+01 1,08E+00 1,39E+01 2,52E+00 1,91E+00 -9,74E+02
WDP1 m3 6,55E+04 4,73E+01 2,29E-01 1,34E+01 2,53E+01 1,08E+01 -2,64E+04
GWP-total = Global Warming Potential total; GWP-fossil = Global Warming Potential fossil fuels; GWP-biogenic = Global Warming Potential biogenic; GWP-luluc =
Global Warming Potential land use and land use change; ODP = Depletion potential of the stratospheric ozone layer; AP = Acidification potential, Accumulated
Exceedance; EP-freshwater = Eutrophication potential, fraction of nutrients reaching freshwater end compartment: EP-marine = Eutrophication potential, fraction of
nutrients reaching marine end compartment; EP-terrestrial = Eutrophication potential, Accumulated Exceedance; POCP = Formation potential of tropospheric ozone;
ADP-minerals&metals = Abiotic depletion potential for non-fossil resources; ADP-fossil = Abiotic depletion for fossil resources potential; WDP = Water (user)
deprivation potential, deprivation-weighted water consumption
"Reading example: 9,0 E-03 = 9,0*10-3 = 0,009"
*INA Indicator Not Assessed
1. The results of this environmental impact indicator shall be used with care as the uncertainties on these results are high or as there is limited experienced with the
indicator
Remarks to environmental impacts
8 / 13
Additional environmental impact indicators
Indicator Unit A1-A3 A4 C1 C2 C3 C4 D
PM Disease incidence 2,37E-05 1,98E-07 2,16E-08 5,61E-08 1,07E-08 1,07E-08 -7,21E-06
IRP2 kgBq U235 -eq 2,59E+01 2,14E-01 4,61E-03 6,06E-02 1,05E-02 8,80E-03 -2,63E+00
ETP-fw1 CTUe 2,23E+04 3,63E+01 5,88E-01 1,03E+01 5,65E+01 2,74E+02 -4,95E+03
HTP-c1 CTUh 1,28E-06 0,00E+00 0,00E+00 0,00E+00 6,29E-10 3,38E-09 -3,43E-07
HTP-nc1 CTUh 2,05E-05 3,96E-08 5,33E-10 1,12E-08 3,32E-08 2,29E-07 1,95E-07
SQP1 dimensionless 1,53E+03 3,42E+01 1,37E-01 9,70E+00 7,92E-01 4,66E+00 -6,57E+01
PM = Particulate Matter emissions; IRP = Ionizing radiation – human health; ETP-fw = Eco toxicity – freshwater; HTP-c = Human toxicity – cancer effects; HTP-nc =
Human toxicity – non cancer effects; SQP = Potential Soil Quality Index (dimensionless)
"Reading example: 9,0 E-03 = 9,0*10-3 = 0,009"
*INA Indicator Not Assessed
1. The results of this environmental impact indicator shall be used with care as the uncertainties on these results are high or as there is limited experienced with the
indicator
2. This impact category deals mainly with the eventual impact of low dose ionizing radiation on human health of the nuclear fuel cycle. It does not consider effects due
to possible nuclear accidents, occupational exposure nor due to radioactive waste disposal in underground facilities. Potential ionizing radiation from the soil, from
radon and from some construction materials is also not measured by this indicator.
9 / 13
Resource use
Indicator Unit A1-A3 A4 C1 C2 C3 C4 D
PERE MJ 7,74E+02 7,00E-01 5,82E-03 1,98E-01 2,48E-01 1,01E-01 -2,69E+02
PERM MJ 1,10E+02 0,00E+00 0,00E+00 0,00E+00 0,00E+00 0,00E+00 0,00E+00
PERT MJ 8,83E+02 7,00E-01 5,82E-03 1,98E-01 2,48E-01 1,01E-01 -2,69E+02
PENRE MJ 3,83E+03 4,89E+01 1,08E+00 1,39E+01 2,52E+00 1,91E+00 -9,74E+02
PENRM MJ 1,29E+02 0,00E+00 0,00E+00 0,00E+00 0,00E+00 0,00E+00 0,00E+00
PENRT MJ 3,96E+03 4,89E+01 1,08E+00 1,39E+01 2,52E+00 1,91E+00 -9,74E+02
SM kg 4,03E+00 0,00E+00 5,28E-04 0,00E+00 2,24E-05 1,72E-05 3,81E-01
RSF MJ 6,55E+00 2,51E-02 1,43E-04 7,10E-03 5,41E-03 2,30E-03 1,36E+00
NRSF MJ 8,57E+01 8,96E-02 2,11E-03 2,54E-02 -1,04E-03 4,54E-03 4,11E+01
FW m3 4,39E+00 5,23E-03 5,54E-05 1,48E-03 2,55E-02 4,60E-03 -1,37E+00
PERE = Use of renewable primary energy excluding renewable primary energy resources used as raw materials; PERM = Use of renewable primary energy resources used
as raw materials; PERT = Total use of renewable primary energy resources; PENRE = Use of non renewable primary energy excluding non-renewable primary energy
resources used as raw materials; PENRM = Use of non renewable primary energy resources used as raw materials; PENRT = Total use of non renewable primary energy
resources; SM = Use of secondary materials; RSF = Use of renewable secondary fuels; NRSF = Use of non-renewable secondary fuels; FW = Net use of fresh water
"Reading example: 9,0 E-03 = 9,0*10-3 = 0,009"
*INA Indicator Not Assessed
10 / 13
End of life - Waste
Indicator Unit A1-A3 A4 C1 C2 C3 C4 D
HWD kg 1,73E+00 2,52E-03 3,17E-05 7,15E-04 5,65E-03 5,85E-02 -9,32E-03
NHWD kg 7,90E+01 2,38E+00 1,27E-03 6,74E-01 8,03E-01 7,75E+00 -3,11E+01
RWD kg 1,71E-02 3,33E-04 7,47E-06 9,44E-05 3,50E-06 5,80E-06 -2,49E-03
HWD = Hazardous waste disposed; NHWD = Non-hazardous waste disposed; RWD = Radioactive waste disposed
"Reading example: 9,0 E-03 = 9,0*10-3 = 0,009"
*INA Indicator Not Assessed
End of life - Output flow
Indicator Unit A1-A3 A4 C1 C2 C3 C4 D
CRU kg 0,00E+00 0,00E+00 0,00E+00 0,00E+00 0,00E+00 0,00E+00 0,00E+00
MFR kg 2,76E-01 0,00E+00 5,19E-04 0,00E+00 4,55E+01 1,37E-04 -1,49E-02
MER kg 1,49E-02 0,00E+00 1,61E-06 0,00E+00 8,71E-01 2,98E-06 -1,96E-03
EEE MJ 6,19E-02 0,00E+00 5,51E-06 0,00E+00 2,16E+00 1,67E-04 -4,81E-03
EET MJ 9,36E-01 0,00E+00 8,34E-05 0,00E+00 3,27E+01 2,53E-03 -7,27E-02
CRU = Components for re-use; MFR = Materials for recycling; MER = Materials for energy recovery; EEE = Exported energy electrical; EET = Exported energy thermal
"Reading example: 9,0 E-03 = 9,0*10-3 = 0,009"
*INA Indicator Not Assessed
Biogenic Carbon Content
Indicator Unit At the factory gate
Biogenic carbon content in product kg C 0,00E+00
Biogenic carbon content in accompanying packaging kg C 3,96E+00
Note: 1 kg biogenic carbon is equivalent to 44/12 kg CO2
11 / 13
Additional requirements
Greenhouse gas emissions from the use of electricity in the manufacturing phase
National production mix from import, low voltage (production of transmission lines, in addition to direct emissions and losses in grid) of applied
electricity for the manufacturing process (A3).
Electricity mix Source Amount Unit
Electricity, Sweden (kWh) ecoinvent 3.6 54,94 g CO2-eq/kWh
Dangerous substances
The product contains no substances on the REACH Candidate list at or above 100 ppm, 0,01 % by weight.
Indoor environment
Additional Environmental Information
Additional environmental impact indicators required in NPCR Part A for construction products
Indicator Unit A1-A3 A4 C1 C2 C3 C4 D
GWPIOBC kg CO2 -eq 2,87E+02 3,24E+00 7,82E-02 9,18E-01 8,32E+00 3,54E-01 -1,08E+02
GWP-IOBC: Global warming potential calculated according to the principle of instantaneous oxidation. In order to increase the transparency of biogenic carbon​
contribution to climate impact, the indicator GWP-IOBC is required as it declares climate impacts calculated according to the principle of instantaneous oxidation.​
GWP-IOBC is also referred to as GWP-GHG in context to Swedish public procurement legislation.
12 / 13
Bibliography
ISO 14025:2010 Environmental labels and declarations - Type III environmental declarations - Principles and procedures.
ISO 14044:2006 Environmental management - Life cycle assessment - Requirements and guidelines.
EN 15804:2012+A2:2019 Environmental product declaration - Core rules for the product category of construction products.
ISO 21930:2017 Sustainability in buildings and civil engineering works - Core rules for environmental product declarations of construction
products.
ecoinvent v3, Allocation, cut-off by classification, Swiss Centre of Life Cycle Inventories.
Iversen et al., (2021) eEPD v2021.09 Background information for EPD generator tool system verification, LCA.no Report number: 07.21
Graafland and Iversen (2022) EPD generator for NPCR 030 Ventilation components, Background information for EPD generator application and
LCA data, LCA.no report number: 12.22
NPCR Part A: Construction products and services. Ver. 2.0. April 2021, EPD-Norge.
NPCR 030 Part B for Ventilation components, Ver. 1.0, 18.05.2021, EPD Norway.
Program operator and publisher Phone: +47 977 22 020
The Norwegian EPD Foundation e-mail: post@epd-norge.no
Post Box 5250 Majorstuen, 0303 Oslo, Norway web: www.epd-norge.no
Owner of the declaration: Phone: +46761325238
Flexit AS e-mail: anton.olsson@flexit.no
Moseveien 8, 1870 Ørje web: https://www.flexit.no/
Author of the Life Cycle Assessment Phone: +47 916 50 916
LCA.no AS e-mail: post@lca.no
Dokka 6A, 1671 web: www.lca.no
Developer of EPD generator Phone: +47 916 50 916
LCA.no AS e-mail: post@lca.no
Dokka 6B,1671 Kråkerøy web: www.lca.no
ECO Platform web: www.eco-platform.org
ECO Portal web: ECO Portal
13 / 13
