Environmental product declaration
in accordance with ISO 14025 and EN 15804+A2
GREENLINE EPS SWEDEN
Owner of the declaration: Program operator:
BEWI ASA, Insulation and Construction The Norwegian EPD Foundation
Product: Declaration number:
GREENLINE EPS SWEDEN NEPD-9159-8728
Declared unit: Registration number:
1 m2 NEPD-9159-8728
This declaration is based on Product Category Rules: Issue date:
CEN Standard EN 15804:2012+A2:2019 serves as core 13.02.2025
PCR.
Valid to:
The Norwegian EPD Foundation NPCR 012:2022 Part B for Thermal insulation products
13.02.2030
EPD software:
LCAno EPD generator ID: 285421
1 / 13
General information
Product Owner of the declaration:
GREENLINE EPS SWEDEN BEWI ASA, Insulation and Construction
Contact person: Marc Storm Andersen
Phone: +45 72157902
e-mail: marc.andersen@bewi.com
Program operator: Manufacturer:
The Norwegian EPD Foundation BEWI ASA, Insulation and Construction
Post Box 5250 Majorstuen, 0303 Oslo, Norway
Phone: +47 977 22 020
web: www.epd-norge.no
Declaration number: Place of production:
BEWI ASA, Insulation and Construction
NEPD-9159-8728
Hammarvikringen 64
HAMAR 7263, Norway
This declaration is based on Product Category Rules: Management system:
CEN Standard EN 15804:2012+A2:2019 serves as core PCR. ISO 14001 og 9001 for all production sites
NPCR 012:2022 Part B for Thermal insulation products
Statement of liability: Organisation no:
The owner of the declaration shall be liable for the underlying 925437948
information and evidence. EPD Norway shall not be liable with respect
to manufacturer information, life cycle assessment data and
evidences.​
Declared unit: Issue date:
1 m2 GREENLINE EPS SWEDEN 13.02.2025
Declared unit with option: Valid to:
A1,A2,A3,A4,A5,C1,C2,C3,C4,D 13.02.2030
Year of study:
2021
Functional unit: Comparability:
1 m² Greenline 80 EPS insulation board with 38 mm thickness at R=1 EPD of construction products may not be comparable if they not
m²K/W, transportation to site, waste handling and recovery. comply with EN 15804:2012+A2:2019 and seen in a building context.
Use the conversion table on page 5 for other thicknesses and
qualities than the declared unit.
General information on verification of EPD from EPD tools: Development and verification of EPD:
Independent verification of data, other environmental information The declaration is created using EPD tool lca.tools ver EPD2022.03,
and the declaration according to ISO 14025:2010, § 8.1.3 and § 8.1.4. developed by LCA.no. The EPD tool is integrated in the company's
Verification of each EPD is made according to EPD-Norway’s management system, and has been approved by EPD Norway.
guidelines for verification and approval requiring that tools are i) NEPDT97
integrated into the company's environmental management system, ii)
the procedures for use of the EPD tool are approved by EPD-Norway, Developer of EPD: Ahmad Nazal
and iii) the process is reviewed annually by an independent third
Reviewer of company-specific input data and EPD:​ Mikael Danestedt
party verifier. See Appendix G of EPD-Norway's General Programme
Instructions for further information on EPD tools
Verification of EPD tool: Approved:
2 / 13
Independent third party verification of the EPD tool, background data
and test-EPD in accordance with EPDNorway's procedures and
guidelines for verification and approval of EPD tools.
Third party verifier:
Elisabet Amat, GREENIZE projects
(no signature required)
3 / 13
Product
Product description:
Product variation and calculation of averages
The insulation board is provided in several dimensions and thicknesses.
No variation between sites; single production site declared.
Product description
Expanded polystyrene (EPS) is a common material used for thermal insulation of buildings, including floors, walls and ceilings. It is a polymer foam,
consisting of air-filled polystyrene cells. As 98% of the material is air, EPS provides good insulating properties at a low weight. Other characteristics
of the material include low moisture absorption, long service life and high compressive strength.
EPS is manufactured through permeating polystyrene beads with pentane, allowing the beads to expand when exposed to steam. This addition of
a so-called blowing agent adds 4% - 6% w/w. The expanded polystyrene (EPS) beads are then fed into a block molding machine, where steam and
pressure forms large blocks of EPS. The amount of EPS going into the mold determines the densitiy of the block, where pressure class 80 provides
a density at 80 kN/m2, which is approximately 15 kg/m3. After molding, the remaining blowing agent, pentane, is aired out and the blocks are cut
into the desired shape.
Weight per declared unit is 0,57 kg given a density of 15 kg/cubic meter with a thickness of 38 mm.
Product specification
Density:
80: 15,0 kg/m3
100: 17,5 kg/m3
150: 23,5 kg/m3
200: 28,5 kg/m3
300: 39,5 kg/m3
Materials kg %
Plastic - Polystyrene expandable
0,57 100,00
(EPS)
Total 0,57 100,00
Packaging kg %
Packaging - EPS 0,00 33,63
Packaging - Plastic 0,01 66,37
Total incl. packaging 0,58 100,00
Technical data:
Typical size: 600 mm x 1200 mm, 1200 x 2400mm
Typical thickness: 10 mm - 400 mm
Moisture absoprtion: < 5 vol%
Fire Class: F
Market:
Sweden, Norway, Denmark
Reference service life, product
As in the construction where it is used
Reference service life, building or construction works
As in the construction where it is used
LCA: Calculation rules
Declared unit:
1 m2 GREENLINE EPS SWEDEN
Cut-off criteria:
All major raw materials and all the essential energy is included. The production processes for raw materials and energy flows with very small
amounts (less than 1%) are not included. These cut-off criteria do not apply for hazardous materials and substances.
Allocation:
The allocation is made in accordance with the provisions of EN 15804+A2. Incoming energy and water and waste production in-house is allocated
equally among all products through mass allocation. Effects of primary production of recycled materials is allocated to the main product in which
the material was used. The recycling process and transportation of the material is allocated to this analysis.
Data quality:
4 / 13
Specific data for the product composition are provided by the manufacturer. The data represent the production of the declared product and were
collected for EPD development in the year of study. Background data is based on EPDs according to EN 15804 and different LCA databases. The
data quality of the raw materials in A1 is presented in the table below.
Materials Source Data quality Year
European
Packaging - EPS Plastics Europe + ecoinvent 3.6 2019
average.
Packaging - Plastic ecoinvent 3.6 Database 2019
Plastic - Polystyrene expandable (EPS) Supplier Specific Project EPD 2024
5 / 13
System boundaries (X=included, MND=module not declared, MNR=module not relevant)
Construction Beyond the system
Product stage Use stage End of life stage
installation stage boundaries
A1 A2 A3 A4 A5 B1 B2 B3 B4 B5 B6 B7 C1 C2 C3 C4 D
X X X X X MND MND MND MND MND MND MND X X X X X
System boundary:
Additional technical information:
waR slairetam tropsnarT gnirutcafunaM tropsnarT ylbmessA e​sU ecnanetniaM riapeR tnemecalpeR tnemhsibrufeR lanoitarepO ygrene esu lanoitarepO esu retaw -eD noitcurtsnoc noitilomed tropsnarT etsaW gnissecorp lasopsiD -yrevoceR-esueR laitnetop-gnilcyceR
6 / 13
LCA: Scenarios and additional technical information
The following information describe the scenarios in the different modules of the EPD.
Capacity utilisation Value
Transport from production place to user (A4) Distance (km) Fuel/Energy Consumption Unit
(incl. return) % (Liter/tonne)
Truck, 16-32 tonnes, EURO 6 (kgkm) 36,7 % 100 0,043 l/tkm 4,30
Assembly (A5) Unit Value
Waste, packaging, plastic to average treatment -
kg 0,011
A5 (inkl transport) (kg)
De-construction demolition (C1) Unit Value
Manual demolition of EPS in C1 kg 0,57
Capacity utilisation Value
Transport to waste processing (C2) Distance (km) Fuel/Energy Consumption Unit
(incl. return) % (Liter/tonne)
Truck, over 32 tonnes, EURO 6 (kgkm) 53,3 % 20 0,023 l/tkm 0,46
Waste processing (C3) Unit Value
Waste, Polystyrene, incineration kg 0,57
Disposal (C4) Unit Value
Landfilling of ashes from incineration of PS kg 0,0017
Benefits and loads beyond the system
Unit Value
boundaries (D)
substitution of electricity (MJ) MJ 0,33
Substitution of thermal energy (MJ) MJ 18,20
7 / 13
LCA: Results
The LCA results are presented below for the declared unit defined on page 2 of the EPD document.
Environmental impact
Indicator Unit A1 A2 A3 A4 A5 C1 C2 C3 C4 D
GWP-total
kg CO2 -
4,21E-01 4,85E-02 1,07E-01 9,50E-03 8,95E-04 0,00E+00 1,01E-03 1,82E+00 8,86E-05 -1,03E-01
eq
GWP-fossil
kg CO2 -
4,19E-01 4,85E-02 1,02E-01 9,50E-03 8,95E-04 0,00E+00 1,01E-03 1,82E+00 8,85E-05 -9,98E-02
eq
GWP-biogenic
kg CO2 -
1,32E-03 1,80E-05 2,04E-03 3,93E-06 1,24E-07 0,00E+00 4,34E-07 1,25E-05 4,70E-08 -5,99E-05
eq
GWP-luluc
kg CO2 -
1,42E-03 2,00E-05 3,58E-03 3,38E-06 6,86E-08 0,00E+00 3,09E-07 1,99E-06 1,36E-08 -3,61E-03
eq
kg
ODP CFC11 - 5,53E-08 1,10E-08 2,71E-08 2,15E-09 5,40E-11 0,00E+00 2,44E-10 1,30E-09 1,00E-11 -7,69E-03
eq
mol H+
AP 3,12E-03 6,41E-04 3,64E-04 2,73E-05 1,10E-06 0,00E+00 3,26E-06 2,16E-04 3,12E-07 -8,25E-04
-eq
EP-FreshWater kg P -eq 2,06E-05 3,18E-07 3,76E-06 7,59E-08 1,84E-09 0,00E+00 8,06E-09 1,29E-07 1,20E-09 -8,97E-06
EP-Marine kg N -eq 6,59E-04 1,57E-04 6,43E-05 5,40E-06 1,01E-06 0,00E+00 7,14E-07 1,04E-04 9,73E-08 -2,79E-04
mol N -
EP-Terrestial 7,33E-03 1,74E-03 8,22E-04 6,04E-05 3,95E-06 0,00E+00 7,96E-06 1,11E-03 1,11E-06 -3,01E-03
eq
kg
POCP NMVOC 2,23E-03 4,84E-04 6,78E-03 2,31E-05 1,30E-06 0,00E+00 3,13E-06 2,67E-04 3,06E-07 -8,30E-04
-eq
ADP- kg Sb-
6,19E-06 6,82E-07 2,22E-06 2,62E-07 4,76E-09 0,00E+00 1,80E-08 5,61E-08 4,96E-10 -6,23E-07
minerals&metals1 eq
ADP-fossil1 MJ 7,73E+00 7,31E-01 6,47E+00 1,44E-01 3,69E-03 0,00E+00 1,64E-02 1,11E-01 8,05E-04 -1,43E+00
WDP1 m3 -1,54E+01 4,40E-01 6,55E+02 1,39E-01 1,30E-02 0,00E+00 1,26E-02 2,47E-01 8,35E-03 -5,19E+00
GWP-total = Global Warming Potential total; GWP-fossil = Global Warming Potential fossil fuels; GWP-biogenic = Global Warming Potential biogenic; GWP-luluc =
Global Warming Potential land use and land use change; ODP = Depletion potential of the stratospheric ozone layer; AP = Acidification potential, Accumulated
Exceedance; EP-freshwater = Eutrophication potential, fraction of nutrients reaching freshwater end compartment: EP-marine = Eutrophication potential, fraction of
nutrients reaching marine end compartment; EP-terrestrial = Eutrophication potential, Accumulated Exceedance; POCP = Formation potential of tropospheric ozone;
ADP-minerals&metals = Abiotic depletion potential for non-fossil resources; ADP-fossil = Abiotic depletion for fossil resources potential; WDP = Water (user)
deprivation potential, deprivation-weighted water consumption
"Reading example: 9,0 E-03 = 9,0*10-3 = 0,009"
*INA Indicator Not Assessed
1. The results of this environmental impact indicator shall be used with care as the uncertainties on these results are high or as there is limited experienced with the
indicator
Remarks to environmental impacts
8 / 13
Additional environmental impact indicators
Indicator Unit A1 A2 A3 A4 A5 C1 C2 C3 C4 D
PM Disease incidence 2,17E-08 3,39E-09 2,63E-09 5,81E-10 2,00E-11 0,00E+00 9,30E-11 9,10E-10 4,00E-12 -5,24E-08
IRP2 kgBq U235 -eq 1,84E-02 3,18E-03 2,21E-01 6,27E-04 1,67E-05 0,00E+00 7,19E-05 1,86E-04 3,82E-06 -8,22E-03
ETP-fw1 CTUe 7,01E+00 5,00E-01 3,44E+00 1,06E-01 3,52E-03 0,00E+00 1,20E-02 2,69E-01 1,48E-03 -7,85E+00
HTP-c1 CTUh 4,61E-10 0,00E+00 1,00E-10 0,00E+00 0,00E+00 0,00E+00 0,00E+00 7,60E-11 0,00E+00 -1,33E-10
HTP-nc1 CTUh 5,46E-09 5,18E-10 2,43E-09 1,16E-10 3,00E-12 0,00E+00 1,20E-11 3,02E-09 3,00E-12 -7,47E-09
SQP1 dimensionless 5,52E+00 6,24E-01 2,86E+00 1,00E-01 6,44E-03 0,00E+00 1,89E-02 1,33E-02 2,22E-03 -1,01E+01
PM = Particulate Matter emissions; IRP = Ionizing radiation – human health; ETP-fw = Eco toxicity – freshwater; HTP-c = Human toxicity – cancer effects; HTP-nc =
Human toxicity – non cancer effects; SQP = Potential Soil Quality Index (dimensionless)
"Reading example: 9,0 E-03 = 9,0*10-3 = 0,009"
*INA Indicator Not Assessed
1. The results of this environmental impact indicator shall be used with care as the uncertainties on these results are high or as there is limited experienced with the
indicator
2. This impact category deals mainly with the eventual impact of low dose ionizing radiation on human health of the nuclear fuel cycle. It does not consider effects due
to possible nuclear accidents, occupational exposure nor due to radioactive waste disposal in underground facilities. Potential ionizing radiation from the soil, from
radon and from some construction materials is also not measured by this indicator.
9 / 13
Resource use
Indicator Unit A1 A2 A3 A4 A5 C1 C2 C3 C4 D
PERE MJ 8,08E-01 7,88E-03 3,10E+00 2,06E-03 9,32E-05 0,00E+00 2,07E-04 3,20E-03 4,69E-05 -8,31E+00
PERM MJ 9,50E-01 0,00E+00 0,00E+00 0,00E+00 0,00E+00 0,00E+00 0,00E+00 0,00E+00 0,00E+00 0,00E+00
PERT MJ 7,97E-01 7,88E-03 3,10E+00 2,06E-03 9,32E-05 0,00E+00 2,07E-04 3,20E-03 4,69E-05 -8,31E+00
PENRE MJ 8,02E+00 7,31E-01 6,48E+00 1,44E-01 3,69E-03 0,00E+00 1,64E-02 1,11E-01 8,06E-04 -1,43E+00
PENRM MJ 6,84E-01 0,00E+00 0,00E+00 0,00E+00 0,00E+00 0,00E+00 0,00E+00 0,00E+00 0,00E+00 0,00E+00
PENRT MJ 7,63E+00 7,31E-01 6,48E+00 1,44E-01 3,69E-03 0,00E+00 1,64E-02 1,11E-01 8,06E-04 -1,43E+00
SM kg 5,70E-01 0,00E+00 0,00E+00 0,00E+00 0,00E+00 0,00E+00 0,00E+00 0,00E+00 0,00E+00 0,00E+00
RSF MJ 3,96E-03 2,63E-04 1,21E-02 7,35E-05 2,44E-06 0,00E+00 7,24E-06 8,94E-05 1,17E-06 -8,39E-04
NRSF MJ 5,35E-03 7,69E-04 3,81E-02 2,63E-04 6,40E-06 0,00E+00 2,43E-05 0,00E+00 1,86E-04 -5,51E-01
FW m3 2,96E-03 6,94E-05 7,75E-03 1,54E-05 1,95E-06 0,00E+00 1,87E-06 3,15E-04 7,40E-07 -3,68E-03
PERE = Use of renewable primary energy excluding renewable primary energy resources used as raw materials; PERM = Use of renewable primary energy resources used
as raw materials; PERT = Total use of renewable primary energy resources; PENRE = Use of non renewable primary energy excluding non-renewable primary energy
resources used as raw materials; PENRM = Use of non renewable primary energy resources used as raw materials; PENRT = Total use of non renewable primary energy
resources; SM = Use of secondary materials; RSF = Use of renewable secondary fuels; NRSF = Use of non-renewable secondary fuels; FW = Net use of fresh water
"Reading example: 9,0 E-03 = 9,0*10-3 = 0,009"
*INA Indicator Not Assessed
10 / 13
End of life - Waste
Indicator Unit A1 A2 A3 A4 A5 C1 C2 C3 C4 D
HWD kg 3,80E-03 3,70E-05 2,12E-03 7,40E-06 0,00E+00 0,00E+00 9,00E-07 0,00E+00 1,47E-03 -2,08E-05
NHWD kg 3,09E-01 4,57E-02 2,32E-02 6,98E-03 1,13E-02 0,00E+00 1,43E-03 0,00E+00 7,28E-04 -2,96E-02
RWD kg 2,53E-05 5,02E-06 9,74E-05 9,78E-07 0,00E+00 0,00E+00 1,12E-07 0,00E+00 4,86E-09 -7,20E-06
HWD = Hazardous waste disposed; NHWD = Non-hazardous waste disposed; RWD = Radioactive waste disposed
"Reading example: 9,0 E-03 = 9,0*10-3 = 0,009"
*INA Indicator Not Assessed
End of life - Output flow
Indicator Unit A1 A2 A3 A4 A5 C1 C2 C3 C4 D
CRU kg 0,00E+00 0,00E+00 0,00E+00 0,00E+00 0,00E+00 0,00E+00 0,00E+00 0,00E+00 0,00E+00 0,00E+00
MFR kg 0,00E+00 0,00E+00 2,81E-03 0,00E+00 5,77E-03 0,00E+00 0,00E+00 0,00E+00 0,00E+00 0,00E+00
MER kg 0,00E+00 0,00E+00 8,63E-03 0,00E+00 5,65E-07 0,00E+00 0,00E+00 5,70E-01 0,00E+00 0,00E+00
EEE MJ 0,00E+00 0,00E+00 5,72E-03 0,00E+00 8,68E-07 0,00E+00 0,00E+00 1,00E+00 0,00E+00 0,00E+00
EET MJ 0,00E+00 0,00E+00 8,65E-02 0,00E+00 1,31E-05 0,00E+00 0,00E+00 1,52E+01 0,00E+00 0,00E+00
CRU = Components for re-use; MFR = Materials for recycling; MER = Materials for energy recovery; EEE = Exported energy electrical; EET = Exported energy thermal
"Reading example: 9,0 E-03 = 9,0*10-3 = 0,009"
*INA Indicator Not Assessed
Biogenic Carbon Content
Indicator Unit At the factory gate
Biogenic carbon content in product kg C 0,00E+00
Biogenic carbon content in accompanying packaging kg C 0,00E+00
Note: 1 kg biogenic carbon is equivalent to 44/12 kg CO2
11 / 13
Additional requirements
Greenhouse gas emissions from the use of electricity in the manufacturing phase
National production mix from import, low voltage (production of transmission lines, in addition to direct emissions and losses in grid) of applied
electricity for the manufacturing process (A3).
Electricity mix Source Amount Unit
Electricity, Sweden (kWh) ecoinvent 3.6 54,94 g CO2-eq/kWh
Dangerous substances
The product contains no substances given by the REACH Candidate list.
Indoor environment
Additional Environmental Information
Additional environmental impact indicators required in NPCR Part A for construction products
Indicator Unit A1 A2 A3 A4 A5 C1 C2 C3 C4 D
GWPIOBC kg CO2 -eq 4,13E-01 4,85E-02 1,07E-01 9,50E-03 8,95E-04 0,00E+00 1,01E-03 1,82E+00 9,19E-05 -1,02E-01
GWP-IOBC: Global warming potential calculated according to the principle of instantaneous oxidation. In order to increase the transparency of biogenic carbon​
contribution to climate impact, the indicator GWP-IOBC is required as it declares climate impacts calculated according to the principle of instantaneous oxidation.​
GWP-IOBC is also referred to as GWP-GHG in context to Swedish public procurement legislation.
12 / 13
Bibliography
ISO 14025:2010 Environmental labels and declarations - Type III environmental declarations - Principles and procedures.
ISO 14044:2006 Environmental management - Life cycle assessment - Requirements and guidelines.
EN 15804:2012+A2:2019 Environmental product declaration - Core rules for the product category of construction products.
ISO 21930:2017 Sustainability in buildings and civil engineering works - Core rules for environmental product declarations of construction
products.
ecoinvent v3, Allocation, cut-off by classification, Swiss Centre of Life Cycle Inventories.
Iversen et al., (2021) eEPD v2021.09 Background information for EPD generator tool system verification, LCA.no Report number: 07.21
Vold et. al., (2022) EPD generator for NPCR 012 Thermal insulation, Background information for EPD generator application and LCA data, LCA.no
report number: 07.22.
NPCR Part A: Construction products and services. Ver. 2.0. April 2021, EPD-Norge.
NPCR 012 Part B for Part B for Thermal insulation products, Ver. 2.0, 31.03.2022, EPD Norway.
Program operator and publisher Phone: +47 977 22 020
The Norwegian EPD Foundation e-mail: post@epd-norge.no
Post Box 5250 Majorstuen, 0303 Oslo, Norway web: www.epd-norge.no
Owner of the declaration: Phone: +45 72157902
BEWI ASA, Insulation and Construction e-mail: marc.andersen@bewi.com
Hammarvikringen 64, HAMAR 7263, Norway web: https://bewi.com
Author of the Life Cycle Assessment Phone: +47 916 50 916
LCA.no AS e-mail: post@lca.no
Dokka 6A, 1671 Kråkerøy, Norway web: www.lca.no
Developer of EPD generator Phone: +47 916 50 916
LCA.no AS e-mail: post@lca.no
Dokka 6A, 1671 Kråkerøy, Norway web: www.lca.no
ECO Platform web: www.eco-platform.org
ECO Portal web: ECO Portal
13 / 13
