Environmental Product
Declaration
In accordance with ISO 14025 and EN 15804 +A2
Owner of the declaration: PE100/PE100 RC
Norsk Wavin AS
Program holder and publisher:
PE100/PE100 RC are Wavin's
The Norwegian EPD foundation
pressure pipe systems made with
black color with blue stripes.
Declaration number: Wavin pressure pipe systems
NEPD-3586-2251-EN
made of PE100 and PE100 RC
have proven themselves around
Registration Number: the world to be effective and
NEPD-3586-2251-EN economical systems for supplying
potable water and gas, as well as
Issue date: 16.08.2022 for waste water pressure
Valid to: 16.08.2027 discharge.
The Norwegian
EPD Foundation
Ver2-101122 Manufacturer
AB Svenska Wavin
General information
Product: Owner of the declaration:
PE100 / PE100 RC Pipe; PN 6,3, 10, 16, 20; SDR 9, Norsk Wavin AS
11, 17, 26 black (BK) with blue (BL) or brown Contact person: Matteo Tagliaferri
(BR) stripes Phone: +31 623193684
e-mail: matteo.tagliaferri@wavin.com
Program Operator:
The Norwegian EPD Foundation Manufacturer:
Post Box 5250 Majorstuen, 0303 Oslo, Norway AB Svenska Wavin
Tlf: +47 23 08 80 00 Kjulamon 6, 635 06, Eskilstuna, Sweden
e-mail: post@epd-norge.no Phone: +46 (0) 16 541 00 00
e-mail: kundservice.se@wavin.com
Declaration Number:
NEPD-3586-2251-EN Place of production:
Kjulamon 6, 635 06, Eskilstuna, Sweden
This declaration is based on Product
Category Rules: Management system:
CEN standard EN 15804:2012+A2:2019 serves as EN ISO 9001:2015 and EN ISO 14001:2015
core PCR, supplied with NPCR Part A and NPCR
Part B, Version 2.0. Organization no:
823355092
Statements:
The owner of the declaration shall be liable for the Issue date:
underlying information and evidence. EPD 16.08.2022
Norway shall not be liable with respect to
manufacturer, life cycle assessment data and
Valid to:
evidences.
16.08.2027
Declared unit:
Year of study:
1 kg PE100/PE100RC Pipe BK/BL
2020
Declared unit with option:
Comparability:
A1,A2,A3,A4,A5,C1,C2,C3,C4,D
EPDs from other programmes than the Norwegian
EPD foundation may not be comparable.
Functional unit:
Not applicable.
The EPD has been worked out by:
Verification: Lisa Overmars and Emma Thunnissen,
Ecochain Technologies
Independent verification of the declaration and
data, according to ISO14025:2010
internal external
Approved (Manager of EPD Norway)
Harry van Ewijk, SGS Search
Independent verifier approved by EPD Norway
EPD for the best environmental decision 2
Product
Product description:
PE100 and PE100 RC are Wavin's pressure pipe systems for transport of potable water and gas,
as well as for waste water pressure discharge. The PE material ensures flexibility, and the pipes
are thus easy to handle, even in large dimensions. At the same time, the flexibility means that
the pipes follow the movements of the earth, prolonging its life. The color is black with blue
stripes. PE100 is distinguished by:
- Great wear and tear resistance
- High corrosion resistance
- Slight friction due to the smooth inside
The abbreviation “RC” in the designation PE100 RC stands for “Resistance to Crack” and
describes the pipe materials resistance to the formation of slow-growing cracks.
Product specification:
A typical composition of the pipes covered by this EPD is as follows:
Materials %
PE 99,6%
Packaging 0,4%
The physical properties of the pipes covered in this EPD are:
• Pipe material: Polyethylene (PE)
• Density ~ 950 kg/m³
• E-Modul ~ 1.100 Mpa
• Elongation at break ~ > 600%
• Permitted elongation ~ 2,5-5%
• Linear expansion coefficient ~ 0,17 mm/mx°C
• Thermal Conductivity: 0,43 W / mK
The color of the pipe is black (BK) with blue (BL) or brown (BR) stripes.
Technical data:
The declared unit of this EPD is 1 kg PE100 Pipe. The results per kg are based on the product
‘PE100 Pipe BK/BL 160 PN10 SDR17 L=12’ (‘base product’). The number 160 in the product
name refers to the diameter, which is equal to 160 mm. It follows that the pipe diameters can
be derived from the product names by taking the number after the colour abbreviations.
The table below provides the products covered with this EPD. The selected base product is
representative for all products described in this table; deviations of the LCA results of the other
products compared to the base product are not more than 10%.
The list below provides the mass per 1 meter pipe (including packaging). These masses should
be used to calculate the LCA results per 1 meter pipe, by multiplying the results of all modules,
except ‘A5 – installation only’ presented on page 10-13, with the weight specified below. The
EPD for the best environmental decision 3
LCA results of ‘A5 – installation’ should be calculated from the LCA results presented on pages
8-9 under ‘additional technical information’.
Mass Mass
Product Product
(kg/meter) (kg/meter)
PE100 RC Pipe BK/BL 20 SDR11 L= 25 0,12 PE100 Pipe BK/BL 180 PN16 SDR11 L=12 8,52
PE100 RC Pipe BK/BL 20 SDR11 L=100 0,12 PE100 RC Pipe BK/BL 180 PN16 SDR11 L=12 8,52
PE100 RC Pipe BK/BL 20 SDR11 L= 10 0,12 PE100 Pipe BK/BL 180 PN16 SDR11 L=6 8,52
PE100 RC Pipe BK/BL 20 SDR11 L= 50 0,12 PE100 RC Pipe BK/BL 180 PN16 SDR11 L=6 8,52
PE100 RC Pipe BK/BL 20 SDR11 L=300 0,12 PE100 Pipe BK/BR 200 PN10 SDR17 L=12 7,06
PE100 RC Pipe BK/BL 25 SDR11 L= 10 0,17 PE100 Pipe BK/BL 200 PN10 SDR17 L=12 7,12
PE100 RC Pipe BK/BL 25 SDR11 L= 25 0,17 PE100 Pipe BK/BL 200 PN10 SDR17 L=6 7,12
PE100 RC Pipe BK/BL 25 SDR11 L=300 0,17 PE100 Pipe BK/BL 200 PN16 SDR11 L=12 10,50
PE100 RC Pipe BK/BL 25 SDR11 L=100 0,17 PE100 Pipe BK/BR 200 PN16 SDR11 L=12 10,50
PE100 RC Pipe BK/BL 25 SDR11 L= 50 0,17 PE100 Pipe BK/BL 200 PN16 SDR11 L=6 10,51
PE100 RC Pipe BK/BL 32 SDR11 L=300 0,28 PE100 Pipe BK/BL 225 PN6,3 SDR26 L=6 5,95
PE100 RC Pipe BK/BL 32 SDR11 L=25 0,28 PE100 Pipe BK/BR 225 PN10 SDR17 L=12 9,02
PE100 RC Pipe BK/BL 32 SDR11 L=100 0,28 PE100 Pipe BK/BL 225 PN10 SDR17 L=12 9,03
PE100 RC Pipe BK/BL 32 SDR11 L=50 0,28 PE100 Pipe BK/BL 225 PN10 SDR17 L=6 9,03
PE100 RC Pipe BK/BL 32 SDR11 L=10 0,28 PE100 Pipe BK/BL 225 PN16 SDR11 L=12 13,29
PE100 RC Pipe BK/BL 40 SDR11 L=25 0,43 PE100 RC Pipe BK/BL 225 PN16 SDR11 L=12 13,29
PE100 RC Pipe BK/BR 40 SDR11 L=150 0,43 PE100 Pipe BK/BL 225 PN16 SDR11 L=6 13,30
PE100 RC Pipe BK/BL 40 SDR11 L=150 0,43 PE100 Pipe BK/BR 250 PN6,3 SDR26 L=12 7,36
PE100 RC Pipe BK/BL 40 SDR11 L=50 0,43 PE100 Pipe BK/BL 250 PN10 SDR17 L=12 11,06
PE100 RC Pipe BK/BL 50 SDR11 L=150 0,67 PE100 Pipe BK/BR 250 PN10 SDR17 L=12 11,06
PE100 RC Pipe BK/BR 50 SDR11 L=150 0,67 PE100 Pipe BK/BL 250 PN10 SDR17 L=6 11,07
PE100 RC Pipe BK/BL 50 SDR11 L= 50 0,67 PE100 Pipe BK/BL 250 PN16 SDR11 L=12 16,35
PE100 RC Pipe BK/BL 63 SDR11 L=150 1,05 PE100 Pipe BK/BR 250 PN16 SDR11 L=12 16,35
PE100 RC Pipe BK/BR 63 SDR11 L=150 1,05 PE100 RC Pipe BK/BL 250 PN16 SDR11 L=12 16,35
PE100 RC Pipe BK/BL 63 SDR11 L= 50 1,05 PE100 Pipe BK/BL 250 PN16 SDR11 L=6 16,36
PE100 RC Pipe BK/BL 75 SDR11 L=75 1,47 PE100 Pipe BK/BL 250 PN20 SDR9 L=12 19,59
PE100 Pipe BK/BL 90 PN16 SDR11 L=6 2,14 PE100 Pipe BK/BL 280 PN10 SDR17 L=12 13,90
PE100 Pipe BK 110 PN10 SDR17 L=6 2,17 PE100 Pipe BK/BR 280 PN10 SDR17 L=12 13,90
PE100 Pipe BK/BL 110 PN10 SDR17 L=12 2,18 PE100 Pipe BK 280 PN10 SDR17 L=12 13,90
PE100 Pipe BK/BR 110 PN10 SDR17 L=12 2,18 PE100 Pipe BK/BL 280 PN16 SDR11 L=12 20,50
PE100 Pipe BK/BL 110 PN16 SDR11 L=12 3,17 PE100 Pipe BK/BL 315 PN10 SDR17 L=18 17,59
PE100 RC Pipe BK/BL 110 PN16 SDR11 L=12 3,17 PE100 Pipe BK/BL 315 PN10 SDR17 L=12 17,60
PE100 Pipe BK/BL 110 PN16 SDR11 L=6 3,18 PE100 Pipe BK/BR 315 PN10 L=12 17,60
PE100 Pipe BK/BR 110 PN16 SDR11 L=12 3,18 PE100 Pipe BK/BR 315 PN10 SDR17 L=6 17,61
PE100 Pipe BK/BR 125 PN6,3 SDR26 L=12 1,85 PE100 Pipe BK/BL 315 PN16 SDR11 L=12 25,94
PE100 Pipe BK/BR 125 PN10 SDR17 L=12 2,77 PE100 Pipe BK 315 PN16 SDR11 L=12 25,94
PE100 Pipe BK/BL 125 PN10 SDR17 L=12 2,78 PE100 Pipe BK/BL 315 PN16 SDR11 L=6 25,97
PE100 Pipe BK/BL 125 PN16 SDR11 L=12 4,14 PE100 Pipe BK/BL 355 PN10 SDR17 L=12 22,40
PE100 Pipe BK/BL 125 SDR11 L=6 4,15 PE100 Pipe BK/BR 355 PN10 SDR17 L=12 22,40
PE100 Pipe BK/BR 140 PN10 SDR17 L=12 3,49 PE100 Pipe BK/BL 355 PN10 SDR17 L=6 22,42
PE100 Pipe BK/BL 140 PN10 SDR17 L=12 3,51 PE100 Pipe BK/BR 355 PN10 SDR17 L=6 22,42
PE100 Pipe BK/BL 140 PN16 SDR11 L=6 5,14 PE100 Pipe BK/BL 355 PN16 SDR11 L=12 32,93
PE100 Pipe BK 160 PN6,3 SDR26 L=12 3,06 PE100 Pipe BK/BR 400 PN6,3 SDR26 L=12 18,75
PE100 Pipe BK 160 PN10 SDR17 L=12 4,55 PE100 Pipe BK/BL 400 PN10 SDR17 L=12 28,31
EPD for the best environmental decision 4
PE100 Pipe BK/BL 160 PN10 SDR17 L=12 4,56 PE100 Pipe BK/BR 400 PN10 SDR17 L=12 28,31
PE100 Pipe BK/BR 160 PN10 SDR17 L=12 4,56 PE100 Pipe BK/BL 400 PN10 SDR17 L=6 28,33
PE100 Pipe BK/BL 160 PN10 SDR17 L=6 4,56 PE100 RC Pipe BK/BL 400 PN16 SDR11 L=12 41,81
PE100 Pipe BK 160x9,5 PN10 SDR17 L=6 4,56 PE100 Pipe BK/BL 450 PN10 SDR17 L=12 35,86
PE100 Pipe BK/BR 160 PN16 SDR11 L=12 6,74 PE100 Pipe BK/BL 450 PN16 SDR11 L=12 52,95
PE100 RC Pipe BK/BL 160 PN16 SDR11 L=12 6,74 PE100 Pipe BK/BL 500 PN10 SDR17 L=12 44,31
PE100 Pipe BK/BL 160 PN16 SDR11 L=12 6,74 PE100 Pipe BK/BR 500 PN10 SDR17 L=12 44,31
PE100 Pipe BK/BL 160 PN16 SDR11 L=6 6,76 PE100 Pipe BK/BL 500 PN16 SDR11 L=12 65,33
PE100 Pipe BK/BL 180 PN10 SDR17 L=12 5,77 PE100 Pipe BK/BL 560 PN10 SDR17 L=12 55,51
PE100 Pipe BK/BR 180 PN10 SDR17 L=12 5,77 PE100RC TS Pipe BL 560 SDR17 L=12 55,51
PE100 Pipe BK/BL 180 PN10 SDR17 L=6 5,77 PE100 Pipe BK 560 PN10 SDR17 L=6 55,61
PE100 Pipe BK/BR 180 PN10 SDR17 L=6 5,77 PE100 Pipe BK/BR 630 PN10 SDR17 L=12 70,31
PE100 Pipe BK/BR 180 PN16 SDR11 L=12 8,51 PE100 Pipe BK/BL 710 PN10 SDR17 L=22 89,32
Market:
Europe, but the EPD is specific for Nordic countries.
Reference service life, product:
Lifetime on product calculated more than 100 year.
Reference service life, building:
Equal to building service life.
LCA: Calculation rules
Declared unit:
1 kg PE100/PE100RC Pipe
Data quality:
For module A1, specific data for product compositions as provided by the manufacturer are
used. For module A2, transportation data of the raw materials used to the production site was
collected. For module A3, energy consumption and waste production data was collected for
production year 2020. The used background processes are derived from Ecoinvent 3.6.
Allocation:
Allocation was carried out in accordance with the provisions of the EN15804. All manufacturing
inputs (energy and auxiliary materials) at production site level are allocated to different
production processes, followed by allocation of the production processes to the products that
are produced using these processes through mass allocation. No secondary materials have been
used in the production process.
System boundary:
Modules A1-A5 and C1-D are included. The figure below shows a (simplified) process tree.
EPD for the best environmental decision 5
Cut-off criteria:
All relevant inputs and outputs - like emissions, energy and materials - have been taken into
account in this LCA. In accordance with EN15804, the total neglected input flows per module
does not exceed 5% of energy usage and mass.
EPD for the best environmental decision 6
LCA: Scenarios and additional technical information
The following information describe the scenarios in the different modules of the EPD.
Transport from production place to assembly/user (A4)
The transportation distance from Eskilstuna to Oslo was considered.
Capacity utilisation
Type Type of vehicle Distance KM Fuel/Energy consumption
(incl. return) %
Truck 50% Unspecified 422 0,027 l diesel/tkm
Assembly (A5)
Product losses of 5% are considered. This product is used underground, therefore use of an
excavator, soil transport, and a gravel foundation are necessary. For the foundation, gravel is
used; this gravel is assumed to be transported for 150 km. The excavation of the soil is
performed with a hydraulic digger. It is assumed that most of the soil is backfilled; however, the
soil replaced by the gravel foundation and the pipe is assumed to be transported elsewhere
(150 km). The compaction of the soil is considered negligible. The dimensions of the trench are
dependent on the diameter of the pipe; for this reason, different scenarios were devised.
Unit Value
Material loss kg 0,05
Packaging waste kg 0,0037
Installation 225- Installation 355-
Installation <225
Unit 355 mm diameter 710 mm diameter
mm diameter pipe
pipe pipe
l/tonne
Energy consumption of
excavated 0.07 0.07 0.07
excavated volume
(diesel)
Excavated mass, total kg 853.13 1517.20 4454.19
Excavated mass transported
kg 267.02 454.46 1214.84
to deposite
Transport distance from
km 150.00 150.00 150.00
construction site
Refilling mass (dirt + gravel
kg 754.85 1293.59 3620.05
foundation)
Transport distance for
refilling mass to construction km 150.00 150.00 150.00
site
kWh or
Energy used for compaction l/tonne - - -
compacted
End of Life (C1, C3, C4)
For the end-of life, it is assumed that the pipes are left in the ground after use. Therefore, there
is no data input for the end-of-life (C1, C3, C4).
EPD for the best environmental decision 7
Transport to waste processing (C2)
As it is assumed that the pipes are left in the ground after use, there is no transport to waste
processing (C2).
Benefits and loads beyond the system boundaries (D)
Module D contains the benefits and loads of energy recovery from incineration and recycling of
the packaging materials and product losses. For the product losses, the considered waste
treatment is 70% recycling, 20% incineration and 10% landfill. For the PE, 0,67 kg of saved
virgin PE was considered per kg material recycled. The benefits from exported energy were
calculation from the energy efficiencies for Northern countries reported by CEWEP, which is
equal to an electrical efficiency of 11,0%, and a thermal efficiency of 72,6%. Substition of
Norwegian electricity mix and district heating mix was assumed.
Unit Value
Saving of virgin PE kg 0,023
Substition of electric energy MJ 0,06
Subsitition of thermal energy MJ 0,40
Additional technical information
Although most of this EPD can be scaled with the weight of the pipe, this is not the case for
module A5, which scales with the length and the diameter of the pipe. For each applicable
diameter, a scenario for installation of 1 meter pipe was established. The results of these
scenarios per meter pipe are described in the tables below.
To calculate the results for a specific product, the masses of the pipes per meter as described on
page 4-5 (under technical data) should be used to calculate the LCA results per 1 meter pipe,
combined with the data in the tables below. This should be done by multiplying the LCA results
presented on page 10-13 of all modules, except ‘A5 – installation only’ with the mass per meter.
The LCA results of A5 – installation should be calculated from the LCA results presented in the
tables below.
Impact Installation <225 mm Installation 225-355 mm Installation 355-710 mm
Category/Parameter diameter diameter diameter
GWP-total 6.40E+00 9.53E+00 1.98E+01
GWP-fossil 6.39E+00 9.51E+00 1.98E+01
GWP-biogenic 1.14E-02 1.60E-02 2.86E-02
GWP-LULUC 2.28E-03 3.35E-03 6.72E-03
ODP 1.44E-06 2.15E-06 4.47E-06
AP 3.97E-02 5.96E-02 1.26E-01
EP-freshwater 5.87E-05 8.62E-05 1.73E-04
EP-marine 1.45E-02 2.19E-02 4.71E-02
EP-terrestial 1.61E-01 2.43E-01 5.20E-01
POCP 4.55E-02 6.86E-02 1.47E-01
ADP-M&M 1.78E-04 2.60E-04 5.09E-04
ADP-fossil 9.79E+01 1.46E+02 3.01E+02
WDP 6.35E-01 9.01E-01 1.65E+00
PM 6.96E-07 1.06E-06 2.30E-06
IRP 4.60E-01 6.79E-01 1.39E+00
EPD for the best environmental decision 8
ETP-fw 8.06E+01 1.19E+02 2.44E+02
HTP-c 3.14E-09 4.65E-09 9.52E-09
HTP-nc 9.51E-08 1.41E-07 2.86E-07
SQP 8.49E+01 1.24E+02 2.47E+02
RPEE 3.01E+00 4.26E+00 7.82E+00
RPEM 0.00E+00 0.00E+00 0.00E+00
TPE 3.01E+00 4.26E+00 7.82E+00
NRPE 1.04E+02 1.54E+02 3.20E+02
NRPM 0.00E+00 0.00E+00 0.00E+00
TRPE 1.04E+02 1.54E+02 3.20E+02
SM 0.00E+00 0.00E+00 0.00E+00
RSF 0.00E+00 0.00E+00 0.00E+00
NRSF 0.00E+00 0.00E+00 0.00E+00
W 2.51E-01 3.44E-01 5.74E-01
HW 2.52E-04 3.75E-04 7.78E-04
NHW 5.33E+00 7.86E+00 1.59E+01
RW 6.74E-04 1.00E-03 2.07E-03
CR 0.00E+00 0.00E+00 0.00E+00
MR 0.00E+00 0.00E+00 0.00E+00
MER 0.00E+00 0.00E+00 0.00E+00
EEE 0.00E+00 0.00E+00 0.00E+00
ETE 0.00E+00 0.00E+00 0.00E+00
LCA: Results
The LCA results are presented below for the declared unit defined on page 2 of the EPD
document. Recalculation to results for pipes per meter should be done based on the technical
data specified on pages 4-5, and the additional technical information specified on pages 8-9.
System boundaries (X=included, MND= module not declared, MNR=module not
relevant)
Benefits
& loads
Assembly
Product stage Use stage End of life stage beyond
stage
system
boundary
n -
s la ir e wt a am R t r o p s n a r T g n ir u t c a fu n a M t r o p s n a r T y lb m e s s A e s U e c n a n e t n ia M r ia p e R t n e m e c a lp e R t n e m h s ib r u fe R la n o iy t ag rr eee pns Ou e la n o it ar re ete a ps w Ou n o io t cit ui rlo t sm ne od
c
-
t r o p s n a r T g n is s ee tc so ar Wp la s o p s iD g yn r eil v ec soy uc ce e RR --la it n e t o p
e e
D R
A1 A2 A3 A4 A5 B1 B2 B3 B4 B5 B6 B7 C1 C2 C3 C4 D
X X X X X X X X X X
EPD for the best environmental decision 9
Core environmental impact indicators
A5, insta-
Indicator Unit A1-A3 A4 A5, other C1 C2 C3 C4 D
llation
kg CO2
GWP-total 2,15E+00 5,52E-02 1,40E+00 1,62E-01 0,00E+00 0,00E+00 0,00E+00 0,00E+00 -8,20E-02
eq.
GWP- kg CO2
2,12E+00 5,51E-02 1,40E+00 1,61E-01 0,00E+00 0,00E+00 0,00E+00 0,00E+00 -8,18E-02
fossil eq.
GWP- kg CO2
2,33E-02 3,35E-05 2,49E-03 1,11E-03 0,00E+00 0,00E+00 0,00E+00 0,00E+00 -2,57E-04
biogenic eq.
GWP- kg CO2
6,60E-03 1,95E-05 5,00E-04 3,38E-04 0,00E+00 0,00E+00 0,00E+00 0,00E+00 -1,56E-05
LULUC eq.
kg
ODP CFC11 1,27E-07 1,27E-08 3,16E-07 7,68E-09 0,00E+00 0,00E+00 0,00E+00 0,00E+00 -5,64E-09
eq.
mol H⁺
AP 8,32E-03 3,14E-04 8,71E-03 4,66E-04 0,00E+00 0,00E+00 0,00E+00 0,00E+00 -1,96E-04
eq.
EP-
freshwate kg P eq. 3,53E-05 4,54E-07 1,29E-05 1,99E-06 0,00E+00 0,00E+00 0,00E+00 0,00E+00 -8,44E-07
r
EP-marine kg N eq. 1,50E-03 1,12E-04 3,19E-03 9,04E-05 0,00E+00 0,00E+00 0,00E+00 0,00E+00 -3,70E-05
EP- mol N
1,68E-02 1,24E-03 3,53E-02 1,01E-03 0,00E+00 0,00E+00 0,00E+00 0,00E+00 -4,12E-04
terrestial eq.
kg
POCP NMVOC 7,45E-03 3,54E-04 9,97E-03 4,25E-04 0,00E+00 0,00E+00 0,00E+00 0,00E+00 -1,87E-04
eq.
kg Sb
ADP-M&M 2,80E-05 1,43E-06 3,91E-05 1,60E-06 0,00E+00 0,00E+00 0,00E+00 0,00E+00 -4,30E-07
eq.
ADP-fossil MJ 7,25E+01 8,47E-01 2,15E+01 3,78E+00 0,00E+00 0,00E+00 0,00E+00 0,00E+00 -2,23E+00
WDP m³ 1,87E+00 2,60E-03 1,39E-01 9,59E-02 0,00E+00 0,00E+00 0,00E+00 0,00E+00 -3,90E-02
GWP-total: Global Warming Potential; GWP-fossil: Global Warming Potential fossil fuels; GWP-biogenic:
Global Warming Potential biogenic; GWP-LULUC: Global Warming Potential land use and land use change;
ODP: Depletion potential of the stratospheric ozone layer; AP: Acidification potential, Accumulated
Exceedance; EP-freshwater: Eutrophication potential, fraction of nutrients reaching freshwater end
compartment; See “additional Norwegian requirements” for indicator given as PO4 eq. EP-marine:
Eutrophication potential, fraction of nutrients reaching freshwater end compartment; EP-terrestial:
Eutrophication potential, Accumulated Exceedance; POCP: Formation potential of tropospheric ozone; ADP-
M&M: Abiotic depletion potential for non-fossil resources (minerals and metals); ADP-fossil: Abiotic
depletion potential for fossil resources; WDP: Water deprivation potential, deprivation weighted water
counsumption
Additional environmental impact indicators
Indic A5, insta-
Unit A1-A3 A4 A5, other C1 C2 C3 C4 D
ator llation
Disease
PM 8,42E-08 4,98E-09 1,53E-07 5,02E-09 0,00E+00 0,00E+00 0,00E+00 0,00E+00 -1,49E-09
incidence
kBq U235
IRP 6,65E-02 3,70E-03 1,01E-01 3,82E-03 0,00E+00 0,00E+00 0,00E+00 0,00E+00 -1,32E-03
eq.
ETP-
CTUe 1,54E+01 6,87E-01 1,77E+01 9,37E-01 0,00E+00 0,00E+00 0,00E+00 0,00E+00 -2,93E-01
fw
HTP-
CTUh 6,43E-10 2,45E-11 6,89E-10 5,13E-11 0,00E+00 0,00E+00 0,00E+00 0,00E+00 -1,50E-11
c
HTP-
CTUh 1,53E-08 8,19E-10 2,08E-08 1,01E-09 0,00E+00 0,00E+00 0,00E+00 0,00E+00 -3,19E-10
nc
Dimensio
SQP 4,00E+00 7,24E-01 1,86E+01 3,30E-01 0,00E+00 0,00E+00 0,00E+00 0,00E+00 -6,42E-02
nless
EPD for the best environmental decision 10
PM: Particulate matter emissions; IRP: Ionising radiation, human health; ETP-fw: Ecotoxicity (freshwater);
ETP-c: Human toxicity, cancer effects; HTP-nc: Human toxicity, non-cancer effects; SQP: Land use related
impacts / soil quality
Classification of disclaimers to the declaration of core and additional environmental
impact indicators
ILCD
Indicator Disclaimer
classification
Global warming potential (GWP) None
ILCD type / level
Depletion potential of the stratospheric ozone layer (ODP) None
1
Potential incidence of disease due to PM emissions (PM) None
Acidification potential, Accumulated Exceedance (AP) None
Eutrophication potential, Fraction of nutrients reaching freshwater end
None
compartment (EP-freshwater)
Eutrophication potential, Fraction of nutrients reaching marine end
None
ILCD type / level compartment (EP-marine)
2
Eutrophication potential, Accumulated Exceedance (EP-terrestrial) None
Formation potential of tropospheric ozone (POCP) None
Potential Human exposure efficiency relative to U235 (IRP) 1
Abiotic depletion potential for non-fossil resources (ADP-minerals&metals) 2
Abiotic depletion potential for fossil resources (ADP-fossil) 2
Water (user) deprivation potential, deprivation-weighted water consumption
2
(WDP)
ILCD type / level
Potential Comparative Toxic Unit for ecosystems (ETP-fw) 2
3
Potential Comparative Toxic Unit for humans (HTP-c) 2
Potential Comparative Toxic Unit for humans (HTP-nc) 2
Potential Soil quality index (SQP) 2
Disclaimer 1 – This impact category deals mainly with the eventual impact of low dose ionizing radiation on
human health of the nuclear fuel cycle. It does not consider effects due to
possible nuclear accidents, occupational exposure nor due to radioactive waste disposal in underground facilities.
Potential ionizing radiation from the soil, from radon and from some
construction materials is also not measured by this indicator.
Disclaimer 2 – The results of this environmental impact indicator shall be used with care as the uncertainties on
these results are high or as there is limited experienced with the indicator
Resource use
A5, insta-
Parameter Unit A1-A3 A4 A5, other C1 C2 C3 C4 D
llation
RPEE MJ 4,39E+00 1,21E-02 6,59E-01 2,26E-01 0,00E+00 0,00E+00 0,00E+00 0,00E+00 -2,96E-02
RPEM MJ 0,00E+00 0,00E+00 0,00E+00 0,00E+00 0,00E+00 0,00E+00 0,00E+00 0,00E+00 0,00E+00
TPE MJ 4,39E+00 1,21E-02 6,59E-01 2,26E-01 0,00E+00 0,00E+00 0,00E+00 0,00E+00 -2,96E-02
NRPE MJ 7,78E+01 8,99E-01 2,28E+01 4,05E+00 0,00E+00 0,00E+00 0,00E+00 0,00E+00 -2,41E+00
NRPM MJ 0,00E+00 0,00E+00 0,00E+00 0,00E+00 0,00E+00 0,00E+00 0,00E+00 0,00E+00 0,00E+00
TRPE MJ 7,78E+01 8,99E-01 2,28E+01 4,05E+00 0,00E+00 0,00E+00 0,00E+00 0,00E+00 -2,41E+00
EPD for the best environmental decision 11
SM kg 0,00E+00 0,00E+00 0,00E+00 0,00E+00 0,00E+00 0,00E+00 0,00E+00 0,00E+00 0,00E+00
RSF MJ 0,00E+00 0,00E+00 0,00E+00 0,00E+00 0,00E+00 0,00E+00 0,00E+00 0,00E+00 0,00E+00
NRSF MJ 0,00E+00 0,00E+00 0,00E+00 0,00E+00 0,00E+00 0,00E+00 0,00E+00 0,00E+00 0,00E+00
W m3 3,12E-02 9,58E-05 5,50E-02 1,64E-03 0,00E+00 0,00E+00 0,00E+00 0,00E+00 -5,91E-04
RPEE Renewable primary energy resources used as energy carrier; RPEM Renewable primary energy
resources used as raw materials; TPE Total use of renewable primary energy resources; NRPE Non
renewable primary energy resources used as energy carrier; NRPM Non renewable primary energy
resources used as materials; TRPE Total use of non renewable primary energy resources; SM Use of
secondary materials; RSF Use of renewable secondary fuels; NRSF Use of non renewable secondary fuels; W
Use of net fresh water
End of life - Waste
A5, insta-
Parameter Unit A1-A3 A4 A5, other C1 C2 C3 C4 D
llation
HW KG 1,36E-05 2,16E-06 5,53E-05 9,50E-07 0,00E+00 0,00E+00 0,00E+00 0,00E+00 -9,06E-07
NHW KG 1,27E-01 5,25E-02 1,17E+00 1,94E-02 0,00E+00 0,00E+00 0,00E+00 0,00E+00 -1,70E-03
RW KG 7,45E-05 5,76E-06 1,48E-04 4,37E-06 0,00E+00 0,00E+00 0,00E+00 0,00E+00 -1,29E-06
HW Hazardous waste disposed; NHW Non hazardous waste disposed; RW Radioactive waste dispos ed
End of life – output flow
Paramet A5, insta-
Unit A1-A3 A4 A5, other C1 C2 C3 C4 D
er llation
CR kg 0,00E+00 0,00E+00 0,00E+00 8,44E-10 0,00E+00 0,00E+00 0,00E+00 0,00E+00 0,00E+00
MR kg 0,00E+00 0,00E+00 0,00E+00 3,51E-02 0,00E+00 0,00E+00 0,00E+00 0,00E+00 0,00E+00
MER kg 0,00E+00 0,00E+00 0,00E+00 1,31E-02 0,00E+00 0,00E+00 0,00E+00 0,00E+00 0,00E+00
EEE MJ 0,00E+00 0,00E+00 0,00E+00 0,00E+00 0,00E+00 0,00E+00 0,00E+00 0,00E+00 6,11E-02
ETE MJ 0,00E+00 0,00E+00 0,00E+00 0,00E+00 0,00E+00 0,00E+00 0,00E+00 0,00E+00 4,03E-01
CR Components for reuse; MR Materials for recycling; MER Materials for energy recovery; EEE Exported
electric energy; ETE Exported thermal energy
Information describing the biogenic carbon content at the factory gate
Biogenic carbon content Unit Value
Biogenic carbon content in product kg C 0
Biogenic carbon content in the accompanying packaging kg C 0
Additional Norwegian requirements
Greenhous gas emission from the use of electricity in the manufacturing phase
National production mix from import, low voltage (production of transmission lines, in addition
to direct emissions and losses in grid) of applied electricity for the manufacturing prosess(A3).
National electricity grid Unit Value
Hydroelectricity, average (Ecoinvent 3.6) kg CO2 -eq/kWh 0,0496
EPD for the best environmental decision 12
Additional environmental impact indicators required in NPCR Part A for construction
products
In order to increase the transparency of biogenic carbon contribution to climate impact, the
indicator for GWP has been sub-divided into the following:
GWP-IOBC Climate impacts calculated according to the principle of instantaneous
oxidationGWP-BC Climate impacts from the net uptake and emission of biogenic carbon
from each module.
A5, insta-
Indicator Unit A1-A3 A4 A5, other C1 C2 C3 C4 D
llation
GWP- kg CO2
2,12E+00 5,52E-02 1,40E+00 1,61E-01 0,00E+00 0,00E+00 0,00E+00 0,00E+00 -8,18E-02
IOBC eq.
kg CO2
GWP-BC 2,33E-02 3,35E-05 2,49E-03 1,11E-03 0,00E+00 0,00E+00 0,00E+00 0,00E+00 -2,57E-04
eq.
kg CO2
GWP 2,15E+00 5,52E-02 1,40E+00 1,62E-01 0,00E+00 0,00E+00 0,00E+00 0,00E+00 -8,20E-02
eq.
EP-freshwater* Eutrophication potential, fraction of nutrients reaching freshwater end compartment.
Declared as PO4 eq. GWP-IOBC Global warming potential calculated according to the principle of
instantaneous oxidation. GWP-BC Global warming potential from net uptake and emissions of biogenic
carbon from the materials in each module. GWP Global warming potential
Hazardous substances
The declaration is based upon reference to threshold values and/or test results and/or material
safety data sheets provided to EPD verifiers. Documentation available upon request to EPD
owner.
✓ The product contains no substances given by the REACH Candidate list or the
Norwegian priority list.
□ The product contains substances given by the REACH Candidate list or the Norwegian
priority list that are less than 0,1 % by weight.
□ The product contain dangerous substances, more then 0,1% by weight, given by the
REACH Candidate List or the Norwegian Priority list, see table.
□ The product contains no substances given by the REACH Candidate list or the
Norwegian priority list. The product is classified as hazardous waste (Avfallsforskiften,
Annex III), see table.
Indoor environment
The product meets the requirements for low emissions.
Carbon footprint
Carbon footprint has not been worked out for the product.
EPD for the best environmental decision 13
Bibliography
ISO 14025:2010 Environmental labels and declarations - Type III environmental
declarations - Principles and procedures
ISO 14044:2006 Environmental management - Life cycle assessment -
Requirements and guidelines
EN 15804:2012+A2:2019 Sustainability of construction works - Environmental product
declaration - Core rules for the product category of construction
products
ISO 21930:2007 Sustainability in building construction – Environmental
declaration of building products
NPCR Part A Construction products and services. Ver. 2.0. March 2021, EPD-
Norge
NPCR Part B NPCR - Part B for piping systems for use in sewage and storm
water systems (under gravity), the Norwegian EPD
Foundation/EPD-Norge, version 2.0, dated 18-10-2018
CEWEP Results of Specific Data for Energy, R1 Plant Efficiency Factor and
NCV of 314 European Waste-to-Energy (WtE) Plants, CEWEP
Energy Report III (status 2007-2010), 2012, Reiman, D.O.
Program Operator tlf +47 23 08 80 00
The Norwegian EPD Foundation
Post Box 5250 Majorstuen, 0303 Oslo e-post: post@epd-norge.no
Norway web www.epd-norge.no
Publisher tlf +47 23 08 80 00
The Norwegian EPD Foundation
Post Box 5250 Majorstuen, 0303 Oslo e-post: post@epd-norge.no
Norway web www.epd-norge.no
Owner of the declaration tlf +4745190625
Norsk Wavin AS Fax
Karihaugveien 89, 1086, Oslo e-post: Invoice.no@wavin.com
Norway web www.wavin.com/nn-no
Author of the life cycle assessment tlf +31 (0)20 303 5777
Emma Thunissen Fax
H.J.E. Wenckebachweg 123, 1096 AM
e-post: emma@ecochain.com
Amsterdam
The Netherlands web www.ecochain.com
EPD for the best environmental decision 14
EPD for the best
environmental
decision
The Norwegian EPD foundation
www.epd-norge.no
