ver1 2015
ENVIRONMENTAL PRODUCT DECLARATION
in accordance with ISO 14025, ISO 21930 and EN 15804
Owner of the declaration: Kinnarps AB
Program operator: The Norwegian EPD Foundation
Publisher: The Norwegian EPD Foundation
Declaration number: NEPD-3617-2541-EN
Registration number: NEPD-3617-2541-EN
ECO Platform reference number: -
Issue date: 30.06.2022
Valid to: 30.06.2027
Task Chair 6000/8000
Kinnarps AB
www.epd-norge.no
NEPD-3617-2541-EN Task Chair 6000/8000 (ver2-071022)
1 / 8
General information
Product: Owner of the declaration:
Task Chair 6000/8000
Kinnarps AB
Contact person: Johanna Ljunggren - Corporate Sustainability Manager
Phone: +46 515 381 21
e-mail: johanna.ljunggren@kinnarps.se
Program operator: Manufacturer:
Kinnarps AB
The Norwegian EPD Foundation
Pb. 5250 Majorstuen, 0303 Oslo
Phone: +47 23 08 80 00
e-mail: post@epd-norge.no
Declaration number: Place of production:
Kinnarps AB
NEPD-3617-2541-EN Industrigatan 521 88 Kinnarp
Sweden
ECO Platform reference number: Management system:
ISO 9001, ISO 14001, ISO 45001, FSC® (C010544)
This declaration is based on Product Category Rules: Organisation no:
556256-6736
CEN Standard EN 15804:2012+A1:2013 serves as core PCR
NPCR 026:2018 Part B for furniture
Statement of liability: Issue date:
The owner of the declaration shall be liable for the underlying information and 30.06.2022
evidence. EPD Norway shall not be liable with respect to manufacturer
information, life cycle assessment data and evidences. Valid to:
30.06.2027
Declared unit: Year of study:
1 Pcs Task Chair 6000/8000 2022
Declared unit with option: Comparability:
A1,A2,A3,A4 EPDs from programmes other than the Norwegian EPD Foundation may not be
comparable
Functional unit: Development and verification of EPD:
The declaration has been developed and verified using EPD tool lca.tools
ver EPD2020.11, developed by LCA.no AS. The EPD tool is integrated into
the company's environmental management system, and has been
approved by EPD-Norway
General information on verification of EPD from EPD tools:
Independent verification of data, other environmental information and Developer of EPD:
the declaration according to ISO 14025:2010, § 8.1.3 and § 8.1.4. Individual
third party verification of each EPD is not required when the EPD tool is i) Rickard Thil
integrated into the company's environmental management system, ii) the
procedures for use of the EPD tool are approved by EPDNorway, and iii) Reviewer of company-specific input data and EPD:
the proccess is reviewed annualy. See Appendix G of EPD-Norway's
General Programme Instructions for further information on EPD tools. Isabell Vesterberg
Verification of EPD tool: Approved:
Independent third party verification of the EPD tool, background data
Sign
and test-EPD in accordance with EPDNorway's procedures and guidelines
for verification and approval of EPD tools.
Erik Svanes, Norsus AS
(no signature required) Håkon Hauan, CEO EPD-Norge
Key environmental indicators Unit Cradle to gate A1 - A3
Global warming kg CO2 eqv 79,40
Total energy use MJ 1702,67
Amount of recycled materials % 21,17
NEPD-3617-2541-EN Task Chair 6000/8000 (ver2-071022)
2 / 8
Product
Market: Technical data:
The 6000/8000 task chairs are certified according to the following
Mainly Europe, but is available world wide.
environmental and quality standards:
Product description: Möbelfakta, NF Environnement, NF OEC. Some executions are also certified
according to the Nordic Swan.
6240 task chair with high back, wool fabric and black plastic starbase.
The data applies for castors for soft floors as well as for hard floors.
Fulfilled technical standards:
Armrests and headrest available as options.
EN 1335-1 Dimensions
EN 1335-2 Safety requirements
Together with its sister the 8000, the 6000 is a real favourite in European
EN 1335-3 Safety test methods, tested against 110 kg personnel weight
offices. One reason for this success is the combination of timeless
FIRA BS 5459-2 Suitable for use up to 24 hours a day
design, good ergonomics, numerous adjustment possibilities and great
freedom to adapt to personal taste. There are four different backrests,
Fulfilled fire requirements:
two seats and two kinds of armrest to choose from. Most combinations
EN 1021-1 Assessment of the ignitability of upholstered furniture – part 1:
are also available with headrests.
Ignition source smouldering cigarette, with Kinnarps standard fabrics
EN 1021-2 Assessment of the ignitability of upholstered furniture – part 2:
Link to product description:
Ignition source match flame equivalent, with Kinnarps standard fabrics
https://www.kinnarps.com/products/seating/task-chairs/6000/
https://www.kinnarps.com/products/seating/task-chairs/8000/
Reference service life, product
Product specification
10 years (5 years warranty).
The 6000 features a FreeFloat™ tilting mechanism with ergonomic
freedom of movement. The 8000 has a Synchrone mechanism, where Reference service life, building
the ratio between the seat and the back is well synchronised for a
smooth tilting movement. The 6000/8000 chair family offers many
variants with several different backrests, seats and armrests to choose
from. Possibility to choose from all fabrics in Kinnarps Color Studio
(KCS).
The task chair is available in both high and low back and with several
different options such as headrest and different armrests.
For other options, see variants and options.
Recycled share in Recycled share in
Materials kg %
material (kg) material (%)
Metal - Aluminium 1,89 9,41 1,46 77,25
Metal - Steel 12,37 61,60 2,78 22,48
Textile - Polyester (PE) 0,01 0,04 0,00 0,00
Textile - Wool 0,51 2,55 0,00 0,00
Glass fibre 0,01 0,02 0,00 0,83
Plastic - Polyurethane (PUR) 1,56 7,78 0,00 0,00
Wood - Medium Density Fibreboard (MDF) 0,67 3,36 0,00 0,00
Plastic - Polypropylene (PP) 0,68 3,64 0,00 0,00
Plastic - Polyoxymethylene (POM) 0,09 0,46 0,00 0,00
Wood - Plywood 0,15 0,75 0,00 0,00
Powder coating 0,03 0,15 0,00 0,00
Plastic - Nylon (PA) 0,34 1,71 0,00 0,00
Plastic - Polyamide with glass fibre (PAGF30) 1,71 8,52 0,00 0,00
Total: 20,03 4,24
LCA: Calculation rules
Declared unit: Allocation:
The allocation is made in accordance with the provisions of EN 15804. Effects
1 Pcs Task Chair 6000/8000
of primary production of recycled materials is allocated to the main product
Cut-off criteria: in which the material was used. The recycling process and transportation of
the material is allocated to this analysis.
All major raw materials and all the essential energy is included. The
production processes for raw materials and energy flows with very small
amounts (less than 1%) are not included. These cut-off criteria do not
apply for hazardous materials and substances.
Data quality:
Specific data for the product composition are provided by the manufacturer. They represent the production of the declared product and were collected for
EPD development in the year of study. Background data is based on registered EPDs according to EN 15804, Ostfold Research databases, ecoinvent and other
LCA databases. The data quality of the raw materials in A1 is presented in the table below.
Data for the manufacturing processes (product stage A3) refers to the year 2020. All other specific data is from year of study.
NEPD-3617-2541-EN Task Chair 6000/8000 (ver2-071022)
3 / 8
System boundary:
The upholstering and certain plastic components are manufactured at Kinnarps' production site in Skillingaryd, where the fabric is also processed. Certain steel
components are manufactured at Kinnarps' production site in Jönköping and some are purchased as premanufactured components. Final assembly of the
product is done at Kinnarps' production site in Kinnarp.
The flow chart below illustrates the system boundaries of the analysis.
Additional technical information:
NEPD-3617-2541-EN Task Chair 6000/8000 (ver2-071022)
4 / 8
LCA: Scenarios and additional technical information
The following information describe the scenarios in the different modules of the EPD.
The product is shipped to consumer in Kinnarps’ trucks with blankets and cardboard sheets as packaging material which is returned to the factory after
delivery and reused. This method saves 270 kg of packaging material per container and enables 50% more products to be transported in each truck. Kinnarps’
trucks have a load efficiency of over 90% and are run on diesel with renewable content. For more information about sustainability at Kinnarps, visit
https://www.kinnarps.com/about-kinnarps/sustainability/.
Transport from production place to user (A4)
Capacity utilisation Fuel/Energy
Type Type of vehicle Distance km Unit Value (l/t)
(incl. return) % consumption
Truck, 16-32 tonnes, HVO, EURO 6
Truck 36,7 % 300 0,043113 l/tkm 12,93
(kgkm) - RER
Railway l/tkm
Boat l/tkm
Other Transportation l/tkm
NEPD-3617-2541-EN Task Chair 6000/8000 (ver2-071022)
5 / 8
LCA: Results
The LCA results are presented below for the declared unit defined on page 2 of the EPD document.
System boundaries (X=included, MND=module not declared, MNR=module not relevant)
Construction Beyond the
Product stage installation User stage End of life stage . system
stage bondaries
A1 A2 A3 A4 A5 B1 B2 B3 B4 B5 B6 B7 C1 C2 C3 C4 . D
X X X X MND MND MND MND MND MND MND MND MND MND MND MND . MND
Environmental impact
Parameter Unit A1 A2 A3 A4
GWP kg CO 2 -eq 7,50E+01 1,08E+00 3,30E+00 2,32E-01
ODP kg CFC11 -eq 2,66E-06 1,99E-07 4,04E-06 3,74E-08
POCP kg C 2H 4-eq 2,84E-02 2,48E-04 4,09E-03 8,47E-05
AP kg SO 2 -eq 3,82E-01 5,93E-03 1,63E-02 9,40E-04
EP kg PO 3- -eq 7,09E-02 7,57E-04 3,36E-03 1,39E-04
4
ADPM kg Sb -eq 9,62E-04 7,87E-06 6,58E-05 2,94E-05
ADPE MJ 7,71E+02 1,63E+01 3,05E+01 4,68E+00
GWP Global warming potential; ODP Depletion potential of the stratospheric ozone layer; POCP Formation potential of tropospheric photochemical oxidants;
AP Acidification potential of land and water; EP Eutrophication potential; ADPM Abiotic depletion potential for non fossil resources; ADPE Abiotic depletion
potential for fossil resources
Reading example: 9,0 E-03 = 9,0*10-3 = 0,009
*INA Indicator Not Assessed
waR slairetam tropsnarT gnirutcafunaM tropsnarT ylbmessA esU ecnanetniaM riapeR tnemecalpeR tnemhsibrufeR lanoitarepO ygrene esu lanoitarepO esu
retaw
-eD noitcurtsnoc noitilomed tropsnarT etsaW gnissecorp lasopsiD -yrevoceR-esueR -gnilcyceR laitnetop
NEPD-3617-2541-EN Task Chair 6000/8000 (ver2-071022)
6 / 8
Resource use
Parameter Unit A1 A2 A3 A4
RPEE MJ 1,05E+02 2,86E-01 1,47E+02 2,32E-01
RPEM MJ 2,14E+01 0,00E+00 0,00E+00 0,00E+00
TPE MJ 1,26E+02 2,86E-01 1,47E+02 2,32E-01
NRPE MJ 8,99E+02 1,68E+01 5,34E+02 5,11E+00
NRPM MJ 1,20E+02 0,00E+00 0,00E+00 0,00E+00
TRPE MJ 1,02E+03 1,68E+01 5,34E+02 5,05E+00
SM kg 4,24E+00 6,76E-02 1,13E-02 2,74E-01
RSF MJ 1,22E-03 1,75E-03 3,80E-02 7,52E-03
NRSF MJ -2,47E-04 5,68E-03 3,70E-01 2,59E-02
W m3 6,22E-01 3,33E-03 1,95E-01 2,09E-03
RPEE Renewable primary energy resources used as energy carrier; RPEM Renewable primary energy resources used as raw materials; TPE Total use of renewable
primary energy resources; NRPE Non renewable primary energy resources used as energy carrier; NRPM Non renewable primary energy resources used as
materials; TRPE Total use of non renewable primary energy resources; SM Use of secondary materials; RSF Use of renewable secondary fuels; NRSF Use of non
renewable secondary fuels; W Use of net fresh water
Reading example: 9,0 E-03 = 9,0*10-3 = 0,009
*INA Indicator Not Assessed
End of life - Waste
Parameter Unit A1 A2 A3 A4
HW kg 1,43E-02 2,13E-04 1,86E-01 7,17E-04
NHW kg 5,37E+01 1,07E+00 1,48E+00 7,60E-01
RW kg INA* INA* INA* INA*
HW Hazardous waste disposed; NHW Non hazardous waste disposed; RW Radioactive waste disposed
Reading example: 9,0 E-03 = 9,0*10-3 = 0,009
*INA Indicator Not Assessed
End of life - Output flow
Parameter Unit A1 A2 A3 A4
CR kg 0,00E+00 0,00E+00 0,00E+00 0,00E+00
MR kg 1,76E-05 1,17E-03 3,76E+00 4,91E-03
MER kg 1,20E-05 2,02E-05 2,09E-03 8,72E-05
EEE MJ INA* INA* INA* INA*
ETE MJ INA* INA* INA* INA*
CR Components for reuse; MR Materials for recycling; MER Materials for energy recovery; EEE Exported electric energy; ETE Exported thermal energy
Reading example: 9,0 E-03 = 9,0*10-3 = 0,009
*INA Indicator Not Assessed
NEPD-3617-2541-EN Task Chair 6000/8000 (ver2-071022)
7 / 8
Additional Norwegian requirements
Greenhouse gas emissions from the use of electricity in the manufacturing phase
National production mix from import, low voltage (production of transmission lines, in addition to direct emissions and losses in grid) of applied electricity for the manufacturing
process (A3).
Electricity mix Data source Amount Unit
Energy, district heating, Norwegian average (kWh) Østfoldforskning 19,71 g CO2-ekv/kWh
Energy, electricity, nuclear, Sweden: 1 kWh Modified ecoinvent 3.6 22,11 g CO2-ekv/kWh
Dangerous substances
The product contains substances given by the REACH Candidate list and the Norwegian priority list that are less than 0,1 % by weight.
Indoor environment
The product is low-emitting and tested according to Swedish Möbelfakta.
Additional environmental information
Key environmental indicators for variants for this EPD: Cradle to Gate analyse from A1 to A3
Global warming (kg Share of recycled
Variant number Total energy use (MJ)
CO2) material in product(%)
6000/8000 series - Task chair 6240 with wool fabric and aluminum starbase 75,12 1 644,44 29,99
6000/8000 series - Task chair 6240 with polyester fabric and plastic starbase 77,25 1 693,11 23,56
6000/8000 series - Task chair 6130 with wool fabric and plastic starbase 81,16 1 732,39 20,71
6000/8000 series - Task chair 8240 with wool fabric and plastic starbase 84,16 1 787,54 20,72
Key environmental indicators for options for this EPD: Cradle to Gate analyse from A1 to A3
Global warming (kg Share of recycled
Option number Total energy use (MJ)
CO2) material in product(%)
Headrest N34 4,96 128,72 30,29
Armrest 2, pair 9,92 155,05 0,00
Armrest 4, pair 12,82 212,37 0,80
Bibliography
ISO 14025:2010 Environmental labels and declarations - Type III environmental declarations - Principles and procedures.
ISO 14044:2006 Environmental management - Life cycle assessment - Requirements and guidelines.
EN 15804:2012+A1:2013 Environmental product declaration - Core rules for the product category of construction products.
ISO 21930:2017 Sustainability in buildings and civil engineering works - Core rules for environmental product declarations of construction products.
ecoinvent v3, Allocation, cut-off by classification, Swiss Centre of Life Cycle Inventories.
Iversen et al., (2018) eEPD v3.0 - Background information for EPD generator system. LCA.no report number 04.18
Vold et al., (2019) EPD generator for Norsk Industri, Background information for industry application and LCA data, LCA.no report number 06.19.
NPCR Part A: Construction products and services. Ver. 1.0. April 2017, EPD-Norge.
NPCR 026 Part B for Furniture. Ver. 2.0 October 2018, EPD-Norge.
Program operator and publisher Phone: +47 23 08 80 00
The Norwegian EPD Foundation e-mail: post@epd-norge.no
Post Box 5250 Majorstuen, 0303 Oslo,Norway web: www.epd-norge.no
Owner of the declaration Phone: +46 515 381 21
Kinnarps AB e-mail: johanna.ljunggren@kinnarps.se
Industrigatan 521 88 Kinnarp web: kinnarps.com
Author of the Life Cycle Assessment Phone: +47 916 50 916
LCA.no AS e-mail: post@lca.no
Dokka 6B 1671 Kråkerøy web: www.lca.no
Developer of EPD generator Phone: +47 916 50 916
LCA.no AS e-mail: post@lca.no
Dokka 1C 1671 Kråkerøy web: www.lca.no
NEPD-3617-2541-EN Task Chair 6000/8000 (ver2-071022)
8 / 8
