ENVIRONMENTAL PRODUCT DECLARATION
ISO 14025, ISO 21930 and EN 15804
Owner of the declaration: Paroc Group Oy
Program operator: The Norwegian EPD Foundation
Publisher: The Norwegian EPD Foundation
Declaration number: NEPD-2582-1308-EN
Registration number: NEPD-2582-1308-EN
ECO Platform reference number: -
Issue date: 08.12.2020
Valid to: 08.12.2025
PAROC NATURA Stone Wool Thermal Insulation
PAROC Building Insulation
Paroc Group Oy
Owner of the declaration
1/11
NEPD-2582-1308-EN PAROC NATURA Stone Wool Thermal Insulation
Product
Product: Owner of the declaration:
PAROC NATURA Stone Wool Thermal Insulation Paroc Group Oy
(Lana) Contact person: Emelia Samuelsson
Phone +46 (0) 500 46 90 05
Program operator: E-mail: emelia.samuelsson@owenscorning.com
The Norwegian EPD Foundation
P.O. Box 5250 Majorstuen, N – 0303 Oslo, Norway
Phone: +47 23 08 80 00 Manufacturer:
E-mail: post@epd-norge.no Paroc Group Oy
FI-00181, Helsinki
Declaration number: Finland
NEPD-2582-1308-EN
ECO Platform reference number: Place of production:
<From EPD-Norge> Parainen, Finland
This declaration is based on Product Category Management system:
Rules: ISO 14001 and ISO 9001
CEN Standard EN 15804 serves as core PCR
NPCR 012:2018 version 2. Part B for Thermal Organisation no:
insulation products 887294852
Statement of liability: Issue date:
The owner of the declaration shall be liable for the
08.12.2020
underlying information and evidence.
EPD Norway shall not be liable with respect to Valid to:
manufacturer information, life cycle assessment data
08.12.2025
and evidences.
Year of study:
Declared unit:
2018
1 m² of stone wool with a thermal resistance (R) of 1
Km2/W. 1 m2 PAROC Natura Lana at R=1 is at a
Comparability:
weight of 1 kg.
EPD of construction products may not be comparable
if they not comply with EN 15804 and seen in a
Declared unit with option:
building context.
-
Functional unit:
1 m² of stone wool with thermal resistance (R) of 1
m2K/W with a reference service life of minimum 60
years. Impact exclude any lamination.
The EPD has been worked out by:
Emelia Samuelsson, Paroc AB
Verification:
The CEN Norm EN 15804 serves as the core PCR.
Independent verification of the declaration and data,
according to ISO14025:2010
☐ internal ☒ external Approved
Martin Erlandsson, IVL
(Independent verifier approved by EPD Norway)
2/11
NEPD-2582-1308-EN PAROC NATURA Stone Wool Thermal Insulation
Product
Product description: Product content:
The thermal insulation and air tightness of a building’s
Materials %
envelope is the basis for good indoor air quality, living
comfort and energy efficiency. Reduction of energy
Mineral Wool 96-99%
use in buildings is also the best way to reduce a
building’s CO2 emissions. Thermal insulation’s energy
Binder (phenol-formaldehyde-urea- 0-6%
and CO2 balances become positive after less than half copolymer)
a year’s use. Dustbinding (mineral oil) 0,1-0,5%
PAROC® stone wool insulation in naturally non-
combustible and durable. It is made of natural stone
(~2%) and air (~98%). As stone wools thermal
Technical data:
performance is based on static air, insulation products
keeps their energy saving abilities and dimensions in Name Value Unit
different temperature and moisture conditions during
the life-cycle of a building. Thermal conductivity 0,036 W/(mK)
EN 12939 and
The general insulation slab PAROC Natura Lana is EN 12667
manufactured in Finland using low carbon melting
technology, based on an electric melter with Thickness Class T2
renewable electricity. The insulation slab is used in EN 823
EN 12431
many different building applications where insulation
don’t have mechanical load.
Fire Class A1
EN 13501-1:2007+
A1:2009/
Markets:
Mainly Sweden, Finland, Norway, Denmark, Estonia, Length and width EN 822 L± 2,5 mm
Lithuania, Latvia. W ± 1,5
Compressive Strength NDP
Reference service life:
EN 827
The reference service lifetime of PAROC products is
equal to the reference service life of the building. For
the purpose of this EPD the reference service life is
Dimension Stability at DS(70,-)
considered to be minimum 60 years, which is usually
spec. temperature and
the assumption about the lifetime of the building where humidity
this is installed. EN 1604
Tensile strength NDP
perpendicular to faces
/EN1607/
Water vapour diffusion 1
resistance factor
/EN12086/
Point Load /EN12430/ NDP
3/11
NEPD-2582-1308-EN PAROC NATURA Stone Wool Thermal Insulation
LLCCAA:: CCaallccuullaattiioonn RRuulleess
Functional unit: and transportation of the material is allocated to this
1 m² stone wool with a thermal resistance (R) of 1 analysis.
Km2W-1.
System boundary:
The calculation of the weight per square meter is done Table below identifies the modules included in this
as follows: study.
m2-weight = density [kg/m3] x insulation thickness [m] According to EN 15804 any declared benefits and
(in order to meet a specific thermal resistance) = loads from net flows leaching the product system not
m2-weight insulation = density [kg/m3[ x R [m2K/W] x allocated as co-products and have passed the end-of-
λ [W/m K] = [kg/m2]. waste state shall be included in the module D. Module
D includes reuse, recovery and/or recycling potentials.
The specific product, referred to in the declared unit,
is 1 m2 of PAROC Natura Lana (27,8 kg/m3, 100 mm The production stage (A1-A3) covers the following
in thickness). steps:
Data quality: • Raw materials production (e.g. dolomite,
diabase)
The stone wool production data is line specific from
• Components production (e.g. resin)
PAROC low carbon melting technology production line
• Transports of raw materials and pre-products
in Parainen, Finland. Foreground data refer to the year
to manufacturing plants
2018.
• Production of packaging materials
For life cycle modeling the GaBi 9 Software System for • Waste management, water treatment, end-of-
Life Cycle Assessment, developed by Sphera life of residues
Solutions, Inc. (formerly known as thinkstep AG), is
used (/GaBi 9 2020/). All relevant background With the exception of Modules A1 to A3 (describing
datasets are taken from the GaBi 9 software database. the manufacturing of stone wool) all other modules are
To ensure comparability of results in the LCA, the calculated on the basis of assumptions or scenarios.
basic data of GaBi database were used for energy,
The following scenarios were considered in this study:
transportation and auxiliary materials.
• Modules A4: The average distance to building
The datasets are complete and conform to the system
site is 200 km.
boundaries and the criteria for the exclusion of inputs
• Modules A5: Packaging waste processing,
and outputs.
waste generated at the installation is assumed
Background data refer to the years 2018 until 2021 to be 0 %.
(/GaBi 9 2020/) with a country specific scope as far as • Modules C2-C4: Similar to installation
available, e.g. for raw material extraction and scenario with similar kind of waste. In C2 a
production, transportation, and energy supply. transport to waste treatment distance 50 km is
assumed.
All relevant processes (foreground and background)
• Module D: Credits from waste treatment
have been considered when modelling stone wool
(recycling and incineration with energy
production. Furthermore, the LCA for Parainen
recovery) of product parts after use and from
involves a production connected with a low carbon
installation losses.
melting technology, based on an electric melter with
renewable electricity. The process data and the used Cut-off criteria:
background data are consistent. The data quality can
be qualified as good. All major raw materials and all the essential energy is
included. The production process for raw materials
Allocation: and energy flows that are included with very small
amounts (<1%) are not included. This cut-off rule does
The allocation is made in accordance with the
not apply for hazardous materials and substances.
provisions of EN 15804.
The declared unit is 1 m2 stone wool without any
Incoming energy, water and waste production in-
lamination.
house is allocated equally among all products through
mass allocation. Effects of primary production of
recycled materials allocated to the main product in
which the material was used. The recycling process
4/11
NEPD-2582-1308-EN PAROC NATURA Stone Wool Thermal Insulation
LCA: System Boundaries
5/11
NEPD-2582-1308-EN PAROC NATURA Stone Wool Thermal Insulation
LLCCAA:: SScceennaarriiooss aanndd AAddddiittiioonnaall TTeecchhnniiccaall IInnffoorrmmaattiioonn
The following information describe the scenarios in the different modules of the EPD.
Transports to the customer are calculated on the basis of a sce nario with an average truck trailer with a 27 t payload.
For the final stone wool product, a loading ratio of 30 % of weight capacity has been set. The average transport
distance to the customer is assumed to be 450 km as a basis for this study.
T ransport to the Building Site (A4)
Type Capacity utilisation Type of vehicle Distance km Energy use per km Total energy use
(incl. return)
%
Truck 100% (30% weight Truck fleet 450 0,9 liter 418,5 liter
capacity) (0,46 liter/m3 stone wool)
Installation in the Building (A5)
Parameter Parameter expressed by functional unit
Auxiliary materials for the installation Not applicable
Consumption of other resources Not applicable
Quantitative description of the type of energy and consumption Not applicable
rate during the installation process
Wastes at the construction site generated from the installation Installation waste is assumed to be 0% since all
of the product material can be used within the building
Material outputs as a result from waste management processes Waste management process for packaging
at the installation site. For example, compilation for recycling, materials
for energy recovery and final disposal
Emissions to air, soil and water Not applicable
End of Life (C1, C2, C3, C4)
Parameter Parameter expressed by functional unit
Compilation processes district Not applicable
Recycling systems Not applicable
Final disposal Landfilling
Benefits/loads Beyond the System Boundary (D)
Materials that create a benefit in Module D are packaging materials. Benefits from the packaging waste treatment
are considered in module D. Energy products of incineration (e.g. steam, electricity, metals) are credited using
the European production averages (e.g. European grid mix f or power). Credits are reported in module D.
6/11
NEPD-2582-1308-EN PAROC NATURA Stone Wool Thermal Insulation
LCA: Results
Life Cycle Impact Assessment results represent the environmental impacts for the life cycle of stone wool from
cradle to grave.
The goal is to address all necessary parameters according to EN 15804 for creating EPDs. In a first step the results
are calculated based on 1 kg stone wool representing the PAROC average. After that the data is scaled according
to the provided density and lambda and fixed to the mass required for one square meter product with the respective
R value = 1.
Scaling factors are included in the EPD indicating the factor which to multiply with the indicators in order to get the
environmental burden on product level described. The scaling factors solely refer to the stone wool used in these
products. Due to this fact, the variation is less than 10% by rea son of the density, lambda and binder.
E.g. Lana (thickness 45-50); 1,13 (scaling factor) multiplied wi th 0,593 (GWP value for A1-A3) equals 0,67 kg CO2-
eq per m2.
Environmental Impact: 1m2 PAROC Natura Lana (per 1 kg)
Parameter Unit A1-A3 A4 A5 C2 C4 D
GWP-TOT* [kg CO2-eq.] 0,593* 0,0464 0,114 0,00337 0,0136 -0,0544
ODP [kg CFC11-eq.] 7,22E- 7,54E-018 2E-017 5,49E-019 7,51E-017 -6,9E-016
009
AP [kg SO2-eq.] 0,00348 0,000124 1,1E-005 8,24E-006 8,75E-005 -6,45E-005
EP [kg PO43—eq.] 0,000792 3,08E-005 2,45E-006 2,03E-006 9,85E-006 -8,2E-006
POCP [kg ethene-eq.] 0,000196 -4,6E-005 8,15E-007 -2,95E-006 6,58E-006 -6,1E-006
ADPM [kg Sb-eq.] 1,83E- 3,81E-009 9E-010 2,78E-010 5,26E-009 -9,42E-009
007
ADPE [MJ] 5,99 0,625 0,0181 0,0455 0,194 -0,783
GWP-TOT Global warming potential including emission and uptake of biogenic CO2; ODP Depletion potential of
the stratospheric ozone layer; POCP Formation potential of tropospheric photochemical oxidants; AP Acidification
potential of land and water; EP Eutrophication potential; ADPM Abiotic depletion potential for non-fossil
resources; ADPE Abiotic depletion potential for fossil resources.
*A1-3: including 0,01522 kg CO-eq. uptake of biogenic carbon dioxide included in product (0 kg CO -eq.) and packaging
2 2
(0,01522 kgCO-eq.).
2
7/11
NEPD-2582-1308-EN PAROC NATURA Stone Wool Thermal Insulation
LCA: Results
Resource Use: 1m2 PAROC Natura Lana (per 1 kg)
Parameter Unit A 1-3 A4 A5 C2 C4 D
RPEE [MJ] 6,48 - - - - -
RPEM [MJ] 0,197 - - - - -
TPE [MJ] 6,68 0,0352 0,00377 0,00256 0,0261 -0,184
NRPE [MJ] 3,11 - - - - -
NRPM [MJ] 3,21 - - - - -
TRPE [MJ] 6,32 0,627 0,0199 0,0456 0,199 -0,941
SM [kg] 0 0 0 0 0 0
RSF [MJ] 0 0 0 0 0 0
NRSF [MJ] 0 0 0 0 0 0
W [m3] 0,0173 4,08E-005 0,000264 2,97E-006 5,02E-005 -0,000213
RPEE Renewable primary energy resources used as energy carrier; RPEM Renewable primary energy resources
used as raw materials; TPE Total use of renewable primary energy resources; NRPE Non renewable primary
energy resources used as energy carrier; NRPM Non renew able primary energy resources used as materials;
TRPE Total use of non renewable primary energy resources; SM Use of secondary materials; RSF Use of
renewable secondary fuels; NRSF Use of non renewable secondary fuels; W Use of net fresh water.
End of Life – Waste: 1m2 PAROC Natura Lana (per 1 kg)
Parameter Unit A 1-3 A4 A5 C2 C4 D
HW [kg] 1,02E-008 2,9E-008 1,51E-011 2,12E-009 3,04E-009 -3,47E-010
NHW [kg] 0,296 9,6E-005 0,000549 6,98E-006 1 -0,000411
RW [kg] 8,36E-006 7,76E-007 6,85E-007 5,65E-008 2,27E-006 -6,27E-005
HW Hazardous waste disposed; NHW Nonhazardous waste disposed; RW Radioactive waste disposed.
End of Life – Output Flow: 1m2 PAROC Natura Lana (per 1 kg)
Parameter Unit A 1-3 A4 A5 C2 C4 D
CR [kg] 0 0 0 0 0 0
MR [kg] 0 0 0 0 0 0
MER [kg] 0 0 0,0431 0 0 0
EEE [MJ] 0 0 0,21 0 0 0
ETE [MJ] 0 0 0,468 0 0 0
CR Components for reuse; MR Materials for recycling; MER Materials for energy recovery; EEE Exported electric
energy; ETE Exported thermal energy.
8/11
NEPD-2582-1308-EN PAROC NATURA Stone Wool Thermal Insulation
LCA: Results
Key environmental Unit Cradle to gate Transport
indicators A1-A3 ****
Global Warming kg C0 -eqv 0,59 0,05
2
Energy Use (=TPE+TRPE) MJ 13 -
Dangerous substances * - -
*The product contains no substances from the REACH Candidate list of the Norwegian priority list.
****Average transport from production site to customer.
9/11
NEPD-2582-1308-EN PAROC NATURA Stone Wool Thermal Insulation
Additional Norwegian Requirements
Greenhouse gas emissions from the use of hydroelectricity in the manufacturing phase
The selection of the background data for the hydroelectricity generation is in line with EN 15804 and contribute
to GWP as given below.
Greenhouse gas emissions
Country Amount Unit
Finland 0,0143 kg CO2-eqv/kWh
Dangerous substances
☒ The product contains no substances given by the REACH Candidate list or the
Norwegian priority list. The product is classified as hazardous waste
(Avfallsforskiften, Annex III), see table.
☐ The product contains substances given by the REACH Candidate list or the
Norwegian priority list that are less than 0,1 % by weight.
☐ The product contains dangerou s substances, more then 0,1% by weight, given by
the REACH Candidate List or the Norwegian Priority list, see table.
☐ The product contains no substances given by the REACH Candidate list or the
Norwegian priority list. The product is classified as hazardous waste
(Avfallsforskiften, Annex III), se e table.
Dangerous substances
None of the following substances have been added to the product: Substances on the REACH Candidate list of
substances of very high concern or substances on the Norwegian Priority list as of 03.11.2017 or substances that
lead to the product being classified as hazardous waste. T he chemical content of the product complies with
regulatory levels as given in the Norwegian Product Regulations.
Transport
Average transport distance from production site to customer is: 450 km
Carbon footprint
Carbon footprint has not been worked out for the product.
10/11
NEPD-2582-1308-EN PAROC NATURA Stone Wool Thermal Insulation
Bibliography
ISO 14025:2010 Environmental labels and declarations – Type III environmental
declarations – Principles and procedures.
ISO 14040:2006 Environmental management – Life cycle assessment – Principles and
framework.
ISO 14044:2006 Environmental management – Life cycle assessment – Requirements
and guidelines.
EN 15804:2012+A1:2013 Sustainability of construction works – Environmental product
declaration – Core rules for the product category of construction
products.
ISO 21930:2007 Sustainability in building construction – Environmental declaration of
building products.
Dr. Iris Matzke, Yannick Bernard Background report for EPD of Paroc Stone Wool Insulation.
September 2020.
PCR NPCR 012:2018 version 2. Part B for Thermal insulation products
Program Operator and Publisher Phone +47 23 08 80 00
The Norwegian EPD Foundation
Post Box 5250 Majorstuen, 0303 Oslo e-mail: post@epd-norge.no
Norway web: www.epd-norge.no
Owner of the declaration Phone +358 46 876 8000
Paroc Group Oy
FI-00181, Helsinki e-mail: paroc.communication@owenscorning.com
Finland web: www.paroc.com
Sphera Solutions GmbH Phone: +49 (0) 711 34 18 17-0
Yannick Bernard Fax +49 (0) 711 34 18 17-25
Hauptsraße 111-113 e-mail: info@sphera.com
70771 Leinfelden-Echterdingen web: www.sphera.com
11/11
NEPD-2582-1308-EN PAROC NATURA Stone Wool Thermal Insulation
