Environmental Product Declaration
In accordance with 14025 and EN15804 +A2
Troja Walker
Owner of the declaration: Program holder and publisher:
Topro Industri AS The Norwegian EPD foundation
Product name: Declaration number:
Troja Walker, size S and M
NEPD-5534-4840-EN
Declared unit: Registration number:
1 piece of Troja Walker, modules A1-A3, A4,
C1-C4 and D
NEPD-5534-4840-EN
Issue date:
Product category /PCR:
NPCR 026:2022 Part B for furniture + A2
CEN Standard EN 15804:2012+A2:2019 serves
1V5a.l1id2 .t2o0:2 3
as core PCR
The Norwegian
15.12.2028
EPD Foundation
General information
Product: Owner of the declaration:
Troja Walker Topro Industri AS
Contact person: Ingrid Lonar
Program operator: Phone: +47 980 38 021
e-mail: Ingrid.Lonar@topromobility.com
The Norwegian EPD Foundation
Post Box 5250 Majorstuen, 0303 Oslo, Norway
Tlf: +47 23 08 80 00 Manufacturer:
e-mail: post@epd-norge.no Topro Industri AS
Rambekkvegen 5, 2816 Gjøvik, Norway
Declaration number: Phone: +47 61 13 46 00
e-mail: kundeservice@topromobility.com
NEPD-5534-4840-EN Place of production:
This declaration is based on Product
Rambekkvegen 5, 2816 Gjøvik, Norway
Category Rules:
NPCR 026:2022 Part B for furniture + A2
Management system:
CEN Standard EN 15804:2012+A2:2019 serves as
core PCR ISO 9001:2015
ISO 14001:2015
Statements:
The owner of the declaration shall be liable for the Organisation no:
underlying information and evidence. EPD
914 61 973
Norway shall not be liable with respect to
manufacturer, life cycle assessment data and 5
Issue date:
evidences.
Declared unit:
15.12.2023
Valid to:
1 piece of Troja Walker, modules A1-A3, A4, C1-C4
and D
15.12.2028
Year of study:
Functional unit:
2023
N/A
Verification:
Comparability:
Independent verification of the declaration and
EPDs from other programmes than EPD Norway
data, according to ISO14025:2010
may not be comparable.
internal external
The EPD has been worked out by:
Sander Nørsterud, environmental consultant at
Asplan Viak
Approved
Julie Lyslo Skullestad
Independent verifier approved by EPD Norway
Manager of EPD Norway
EPD for the best environmental decision 2
Product
Product description:
Troja Walker S is a walking aid that helps people with different physical disability stay active
and independent. With two grips and four wheels it provides support while moving around in-
or outdoors. The forearm walker come in different sizes for different surroundings and needs.
The Troja Walker is lightweight and stable forearm walker. The forearm supports have been
designed to provide good upper body support while walking.
The main parts of the forearm walker consist of frame, handles and cross in aluminium and
glass fibre reinforced plastic (GFRP) and wheels in GFRP as well as PP, POM, PU and TPE plastic.
Additional parts include breaks, basket, seats and bolts. The basket is an optional add-on.
Product specification:
This EPD is valid for the two sizes of the Troja Walker model: S and M. The same materials are
used for both sizes, but the amounts differ slightly. The material inventory for both sizes are
shown below. The results shown are for the S size without basket. Results for Troja Walker M
are shown under “Additional results”.
Troja Walker S Troja Walker M
Materials KG % KG %
Aluminium 2,37 28 % 2,66 30 %
GFRP 3,00 36 % 3,00 34 %
Steel 0,84 10 % 0,85 10 %
PP 0,90 11 % 0,90 10 %
PUR 0,80 9 % 0,80 9 %
Other materials 0,52 6 % 0,52 6 %
Weight product 8,44 100 % 8,73 100 %
Packaging
Cardboard 2,12 2,12
PE 0,01 0,01
Paper 0,16 0,16
Total weight incl packaging 10,73 11,02
Technical data:
N/A
Market:
Norway and Scandinavia
Reference service life, product:
Not relevant
Reference service life, building:
N/A
EPD for the best environmental decision 3
LCA: Calculation rules
Declared unit:
1 piece of Troja Walker, modules A1-A3, A4, C1-C4 and D
Data quality:
Data is collected during 2023 and is representative for the year 2022 (yearly average). Data for
raw material inputs, manufacturing of the product and transport to market (A1-A3 and A4) is
based on specific data provided by Topro and technical data sheets from the suppliers. End of
Life (C1-C4) scenarios are uncertain and conservative assumptions have therefore been applied.
Generic data for background processes has been modelled using ecoinvent 3.9.1.
Characterization factors from EN15804: 2012 + A2: 2019.
Allocation:
The allocation is made in accordance with the provisions of EN 15804. Incoming energy and
water and waste production in-house is allocated equally among all products through mass
allocation. Effects of primary production of recycled materials allocated to the main product in
which the material was used.
System boundary:
The system boundary is from cradle to gate with options, A1-A3, A4, C1, C2, C3, C4 and D. The
flow chart for production, transport and end of life is shown in the figure below.
Cut-off criteria:
All major raw materials and all the essential energy is included. The production process for raw
materials and energy flows that are included with very small amounts (<1%) are not included.
This cut-off rule does not apply for hazardous materials and substances.
EPD for the best environmental decision 4
LCA: Scenarios and additional technical information
The following information describe the scenarios in the different modules of the EPD.
Scenarios have been developed for transportation from manufacturing to market (A4) and to
account for downstream for waste treatment in accordance with the requirements of EN 15804
and NPCR PART A.
Transport from production place to assembly/user (A4)
The environmental impacts of transportation to market (A4) are calculated for three different
markets: Norway (main scenario), Scandinavia and Europe.
Capacity utilisation (incl. Type of Fuel/Energy value
Type Distance KM
return) % vehicle consumption (l/t)
Scenario 1: Norway
Truck
Lorry, EURO
(Topro to 50 % 130+300 0,144 l/tkm 12,7
6, 24 ton
NAV)
Scenario 2: Scandinavia
Truck
(Topro to Lorry, EURO
9,1 % 611 0,096 l/tkm 88
distribution 6, 24 ton
center)
Truck
(Distribution Lorry, EURO
50 % 300 0,03 l/tkm 8,86
center to 6, 24 ton
customer)
Scenario 3:
Europe
Truck
(Topro to Lorry, EURO
9,1 % 947 0,144 l/tkm 136,41
distribution 6, 24 ton
center)
Truck
(Distribution
Lorry, EURO
center to 50 % 511 0,03 l/tkm 8,86
6, 24 ton
customer, 1st
leg)
Truck
(Distribution
Van, EURO 6,
center to 50 % 77 0,32 29,33
6 ton
customer,
2nd leg)
Scenario 1: Transportation from Topro to NAV aid centres around the country as part of a larger
distribution network. Therefore, a high capacity utilization is likely. A load factor of 50 % is seen
as a conservative estimation.
Scenario 2: Transportation from Topro to storage centre and final distribution as part of a
larger distribution network. A generic distance of 300 km is assumed as final transport leg.
Scenario 3: Transportation from Topro to distribution centre in Germany. From there it is
transported by larger distribution network in two legs as shown in table above.
The main results will include scenario 1, while the results of A4 for scenario 2 and 3 will be
shown under “Additional results”.
EPD for the best environmental decision 5
End of Life (C1, C3, C4)
Unit Value
g 0
Hazardous waste disposed
g
Collected as mixed construction waste
g
Reuse
g 3234
Recycling
g 5208
Energy recovery
g 1037
To landfill
The end of life scenarios are not well documented. Therefore, conservative scenarios are
assumed. Metal waste (steel, aluminium and brass) are assumed recycled, while plastic
materials are assumed to be incinerated with energy recovery (C3). Solids and ash after
incineration is landfilled (C4). Recovered energy from C3 is assumed to substitute electricity
and district heating (D). The dismantling of the walkers (C1) is assumed to be done manually,
and its environmental impact negligible. C1 is therefore not included in the assessment.
Transport to waste processing (C2)
Waste Capacity utilisation Type of Fuel/Energy value
Type Distance KM
type (incl. return) % vehicle consumption (l/t)
lorry 16-32
GFRP and
Truck 50 % metric ton, 85 0,045 3,79
plastic
EURO5
lorry 16-32
Metal Truck 50 % metric ton, 295 0,045 13,16
EURO5
lorry 16-32
Wood Truck 50 % metric ton, 85 0,045 3,79
EURO5
lorry 16-32
Paper and
Truck 50 % metric ton, 498 0,045 22,21
cardboard
EURO5
Transport distance scenarios to waste processing is based on Raadal et al. (2009).
Benefits and loads beyond the system boundaries (D)
Unit Value
Substitution of delivered electricity 4,0 MJ/pcs
Substitution of delivered district heating 101,7 MJ/pcs
Exported energy replaces the Norwegian district heating mix and electricity mix. All conversion
factors for efficiencies and losses from waste to delivered energy are included.
Additional technical information
Not relevant
EPD for the best environmental decision 6
LCA: Results
The LCA results are presented below for the declared unit “1 piece of Troja Walker, modules A1-
A3, A4, C1-C4 and D”.
The results below are presented for Troja Walker S without basket. For Troja Walker M, results
for certain impact categories are presented further down in the document.
Impact assessment results are presented with core and additional impact indicators presented
in EN15804+A2. Reading example: 9,0 E-03 = 9,0*10-3 = 0,009.
System boundaries (X=included, MND= module not declared, MNR=module not
relevant)
Benefits & loads
Product stage Assembly stage Use stage End of life stage beyond system
boundary
n -
s la ir e t a m w a R t r o p s n a r T g n ir u t c a fu n a M t r o p s n a r T y lb m e s s A e s U e c n a n e t n ia M r ia p e R t n e m e c a lp e R t n e m h s ib r u fe R e s u y g r e n e la n o it a r e p O e s u r e t a w la n o it a r e p O o it ilo m e d n o it c u r t s n eo c - t r o p s n a r T g n is s e c o r p e t s a W la s o p s iD g yn r eil v ec soy uc c ee e RR --la it n e t o p
D R
A1 A2 A3 A4 A5 B1 B2 B3 B4 B5 B6 B7 C1 C2 C3 C4 D
MN MN MN MN MN MN MN MN
X X X X X X X X X
D D D D D D D D
Core environmental impact indicators
Indicator Unit A1 A2 A3 A1-A3 A4
GWP-total kg CO2 eq. 5,7E+01 1,2E+00 3,0E+00 6,1E+01 5,6E-01
GWP-fossil kg CO2 eq. 5,7E+01 1,2E+00 2,4E+00 6,1E+01 5,6E-01
GWP-biogenic kg CO2 eq. -4,7E-01 9,4E-04 6,1E-01 1,3E-01 8,9E-04
GWP-LULUC kg CO2 eq. 6,2E-02 7,4E-04 7,1E-03 7,0E-02 1,6E-04
ODP kg CFC11 eq. 2,6E-06 2,1E-08 4,8E-08 2,7E-06 1,2E-08
AP mol H⁺ eq. 2,9E-01 2,1E-02 1,7E-02 3,3E-01 1,2E-03
EP-freshwater kg P eq. 9,1E-03 6,8E-06 1,3E-04 9,2E-03 2,8E-05
EP-marine kg N eq. 4,6E-02 5,3E-03 2,0E-03 5,3E-02 3,3E-04
EP-terrestial mol N eq. 4,0E-01 5,8E-02 2,4E-02 4,8E-01 3,4E-03
POCP kg NMVOC eq. 1,5E-01 1,7E-02 7,6E-03 1,7E-01 2,0E-03
ADP-M&M kg Sb eq. 4,1E-04 2,0E-06 1,6E-04 5,8E-04 7,5E-07
ADP-fossil MJ 7,2E+02 1,5E+01 3,1E+01 7,6E+02 8,2E+00
WDP m³ 2,1E+01 5,3E-02 1,3E+00 2,2E+01 3,0E-02
EPD for the best environmental decision 7
Indicator Unit C1 C2 C3 C4 D
GWP-total kg CO2 eq. 0,0E+00 2,7E-01 9,7E+00 1,4E-02 -4,4E+00
GWP-fossil kg CO2 eq. 0,0E+00 2,7E-01 9,7E+00 1,4E-02 -4,1E+00
GWP-biogenic kg CO2 eq. 0,0E+00 6,8E-04 8,3E-04 3,2E-04 -3,2E-01
GWP-LULUC kg CO2 eq. 0,0E+00 1,3E-04 3,1E-05 2,6E-06 -6,1E-03
ODP kg CFC11 eq. 0,0E+00 5,6E-09 6,4E-09 2,6E-10 -3,9E-08
AP mol H⁺ eq. 0,0E+00 8,4E-04 3,1E-03 6,0E-05 -2,5E-02
EP-freshwater kg P eq. 0,0E+00 2,1E-06 1,4E-06 1,4E-07 -1,1E-04
EP-marine kg N eq. 0,0E+00 2,9E-04 1,5E-03 2,2E-04 -4,9E-03
EP-terrestial mol N eq. 0,0E+00 3,1E-03 1,7E-02 2,5E-04 -5,4E-02
POCP kg NMVOC eq. 0,0E+00 1,3E-03 4,1E-03 9,7E-05 -1,6E-02
ADP-M&M kg Sb eq. 0,0E+00 8,3E-07 2,8E-07 1,6E-08 -2,1E-05
ADP-fossil MJ 0,0E+00 3,7E+00 1,5E+00 2,3E-01 -4,0E+01
WDP m³ 0,0E+00 1,5E-02 2,7E-02 -1,2E-03 -9,5E+00
GWP-total: Global Warming Potential; GWP-fossil: Global Warming Potential fossil fuels; GWP-biogenic:
Global Warming Potential biogenic; GWP-LULUC: Global Warming Potential land use and land use change;
ODP: Depletion potential of the stratospheric ozone layer; AP: Acidification potential, Accumulated
Exceedance; EP-freshwater: Eutrophication potential, fraction of nutrients reaching freshwater end
compartment; See “additional requirements” for indicator given as PO4 eq. EP-marine: Eutrophication
potential, fraction of nutrients reaching freshwater end compartment; EP-terrestial: Eutrophication
potential, Accumulated Exceedance; POCP: Formation potential of tropospheric ozone; ADP-M&M: Abiotic
depletion potential for non-fossil resources (minerals and metals); ADP-fossil: Abiotic depletion potential
for fossil resources; WDP: Water deprivation potential, deprivation weighted water counsumption
Additional environmental impact indicators
Indicator Unit A1 A2 A3 A1-A3 A4
Disease
PM 2,0E-06 5,9E-08 1,1E-07 2,2E-06 3,6E-08
incidence
IRP kBq U235 eq. 6,1E-01 5,4E-03 4,0E-01 1,0E+00 8,9E-03
ETP-fw CTUe 3,4E+02 8,1E+00 2,0E+01 3,7E+02 4,2E+00
HTP-c CTUh 7,9E-08 5,0E-10 4,0E-09 8,3E-08 1,6E-10
HTP-nc CTUh 9,6E-07 1,1E-08 1,7E-07 1,1E-06 6,3E-09
SQP Dimensionless 1,8E+02 8,5E+00 1,8E+01 2,1E+02 7,1E+00
Indicator Unit C1 C2 C3 C4 D
Disease
PM 0,0E+00 1,7E-08 1,3E-08 1,2E-09 -5,8E-07
incidence
IRP kBq U235 eq. 0,0E+00 1,8E-03 1,0E-03 1,9E-04 1,7E+01
ETP-fw CTUe 0,0E+00 1,9E+00 5,1E-01 6,8E+00 -1,1E+01
HTP-c CTUh 0,0E+00 1,2E-10 1,5E-10 2,0E-10 -3,9E-09
EPD for the best environmental decision 8
HTP-nc CTUh 0,0E+00 3,4E-09 5,7E-09 1,2E-08 -1,1E-07
SQP Dimensionless 0,0E+00 2,2E+00 1,9E-01 4,3E-01 -1,5E+02
PM: Particulate matter emissions; IRP: Ionising radiation, human health; ETP-fw: Ecotoxicity (freshwater);
ETP-c: Human toxicity, cancer effects; HTP-nc: Human toxicity, non-cancer effects; SQP: Land use related
impacts / soil quality
Classification of disclaimers to the declaration of core and additional environmental
impact indicators
ILCD
Indicator Disclaimer
classification
Global warming potential (GWP) None
ILCD type / level
Depletion potential of the stratospheric ozone layer (ODP) None
1
Potential incidence of disease due to PM emissions (PM) None
Acidification potential, Accumulated Exceedance (AP) None
Eutrophication potential, Fraction of nutrients reaching marine end
None
compartment (EP-marine)
ILCD type / level
Eutrophication potential, Accumulated Exceedance (EP-terrestrial) None
2
Formation potential of tropospheric ozone (POCP) None
Potential Human exposure efficiency relative to U235 (IRP) 1
Abiotic depletion potential for non-fossil resources (ADP-minerals&metals) 2
Abiotic depletion potential for fossil resources (ADP-fossil) 2
Water (user) deprivation potential, deprivation-weighted water consumption
2
(WDP)
ILCD type / level
Potential Comparative Toxic Unit for ecosystems (ETP-fw) 2
3
Potential Comparative Toxic Unit for humans (HTP-c) 2
Potential Comparative Toxic Unit for humans (HTP-nc) 2
Potential Soil quality index (SQP) 2
Disclaimer 1 – This impact category deals mainly with the eventual impact of low dose ionizing radiation on
human health of the nuclear fuel cycle. It does not consider effects due to
possible nuclear accidents, occupational exposure nor due to radioactive waste disposal in underground facilities.
Potential ionizing radiation from the soil, from radon and from some
construction materials is also not measured by this indicator.
Disclaimer 2 – The results of this environmental impact indicator shall be used with care as the uncertainties on
these results are high or as there is limited experienced with the indicator
Resource use
Parameter Unit A1 A2 A3 A1-A3 A4
RPEE MJ 1,8E+02 1,7E-01 6,3E+01 2,5E+02 9,4E-02
RPEM MJ 0,0E+00 0,0E+00 4,0E+01 4,0E+01 0,0E+00
TPE MJ 1,8E+02 1,7E-01 1,0E+02 2,9E+02 9,4E-02
NRPE MJ 7,6E+02 1,5E+01 -9,9E+01 6,7E+02 8,2E+00
NRPM MJ 0,0E+00 0,0E+00 1,3E+02 1,3E+02 0,0E+00
EPD for the best environmental decision 9
TRPE MJ 7,6E+02 1,5E+01 3,1E+01 8,0E+02 8,2E+00
SM kg 5,4E-01 0,0E+00 0,0E+00 5,4E-01 0,0E+00
RSF MJ 0,0E+00 0,0E+00 0,0E+00 0,0E+00 0,0E+00
NRSF MJ 0,0E+00 0,0E+00 0,0E+00 0,0E+00 0,0E+00
W m3 4,6E-01 1,7E-03 7,3E-01 1,2E+00 9,8E-04
Parameter Unit C1 C2 C3 C4 D
RPEE MJ 0,0E+00 5,7E-02 4,4E-02 7,9E-03 -5,4E+01
RPEM MJ 0,0E+00 0,0E+00 0,0E+00 0,0E+00 0,0E+00
TPE MJ 0,0E+00 5,7E-02 4,4E-02 7,9E-03 -5,4E+01
NRPE MJ 0,0E+00 3,7E+00 1,5E+00 2,3E-01 -4,0E+01
NRPM MJ 0,0E+00 0,0E+00 0,0E+00 0,0E+00 0,0E+00
TRPE MJ 0,0E+00 3,7E+00 1,5E+00 2,3E-01 -4,0E+01
SM kg 0,0E+00 0,0E+00 0,0E+00 0,0E+00 0,0E+00
RSF MJ 0,0E+00 0,0E+00 0,0E+00 0,0E+00 0,0E+00
NRSF MJ 0,0E+00 0,0E+00 0,0E+00 0,0E+00 0,0E+00
W m3 0,0E+00 4,9E-04 6,2E-03 -1,6E-03 -1,7E-01
RPEE Renewable primary energy resources used as energy carrier; RPEM Renewable primary energy
resources used as raw materials; TPE Total use of renewable primary energy resources; NRPE Non
renewable primary energy resources used as energy carrier; NRPM Non renewable primary energy
resources used as materials; TRPE Total use of non renewable primary energy resources; SM Use of
secondary materials; RSF Use of renewable secondary fuels; NRSF Use of non renewable secondary fuels; W
Use of net fresh water
End of life - Waste
Parameter Unit A1 A2 A3 A1-A3 A4
HW KG 3,5E+00 3,2E-04 6,1E-02 1,7E-04 1,7E-04
NHW KG 1,1E+01 7,0E-01 1,2E+00 6,1E-01 6,1E-01
RW KG 1,2E-03 3,2E-06 2,0E-04 2,2E-06 2,2E-06
Parameter Unit C1 C2 C3 C4 D
HW KG 0,0E+00 9,1E-05 4,4E-04 1,1E+00 -3,5E-03
NHW KG 0,0E+00 1,8E-01 2,2E-02 6,2E-02 -5,8E-01
RW KG 0,0E+00 1,2E-06 6,9E-07 1,1E-07 -3,0E-05
HW Hazardous waste disposed; NHW Non hazardous waste disposed; RW Radioactive waste disposed
EPD for the best environmental decision 10
End of life – output flow
Parameter Unit A1 A2 A3 A1-A3 A4
CR kg 0,0E+00 0,0E+00 0,0E+00 0,0E+00 0,0E+00
MR kg 0,0E+00 0,0E+00 1,3E+00 1,3E+00 0,0E+00
MER kg 0,0E+00 0,0E+00 3,5E-01 3,5E-01 0,0E+00
EEE MJ 0,0E+00 0,0E+00 0,0E+00 0,0E+00 0,0E+00
ETE MJ 0,0E+00 0,0E+00 0,0E+00 0,0E+00 0,0E+00
Parameter Unit C1 C2 C3 C4 D
CR kg 0,0E+00 0,0E+00 0,0E+00 0,0E+00 0,0E+00
MR kg 0,0E+00 0,0E+00 3,2E+00 0,0E+00 0,0E+00
MER kg 0,0E+00 0,0E+00 5,3E+00 0,0E+00 0,0E+00
EEE MJ 0,0E+00 0,0E+00 4,0E+00 0,0E+00 0,0E+00
ETE MJ 0,0E+00 0,0E+00 1,0E+02 0,0E+00 0,0E+00
CR Components for reuse; MR Materials for recycling; MER Materials for energy recovery; EEE Exported
electric energy; ETE Exported thermal energy
Reading example: 9,0 E-03 = 9,0*10-3 = 0,009
Information describing the biogenic carbon content at the factory gate
Biogenic carbon content Unit Value
Biogenic carbon content in product kg C
Biogenic carbon content in the accompanying packaging kg C
EPD for the best environmental decision 11
Additional requirements
Location based electricity mix from the use of electricity in the manufacturing
phase
National production mix from import, low voltage (production of transmission lines, in addition
to direct emissions and losses in grid) of applied electricity for the manufacturing process(A3).
National electricity grid
Foreground/core GWPtotal [kg SUM [kg
[kWh] CO2-eq/kWh] CO2-eq]
Electricity, low voltage {NO}| market for electricity, low
24,87 0,0389 0,97
voltage | Cut-off, U
Topro buys guarantees of origin (GoO) certificates. However, the results are only calculated
with location based electricity mix. Contact EPD-owner to get more information on market-
based electricity mix approach.
Additional environmental impact indicators required in NPCR Part A for construction
products
In order to increase the transparency of biogenic carbon contribution to climate impact, the
indicator GWP-IOBC is required as it declares climate impacts calculated according to the
principle of instantaneous oxidation. GWP-IOBC is also referred to as GWP-GHG in context to
Swedish public procurement legislation.
Indicator Unit A1 A2 A3 A1-A3 A4
GWP-IOBC kg CO2 eq. 5,7E+01 1,2E+00 3,0E+00 6,1E+01 5,6E-01
Indicator Unit C1 C2 C3 C4 D
GWP-IOBC kg CO2 eq. 0,0E+00 2,7E-01 9,7E+00 1,4E-02 1,5E+02
GWP-IOBC Global warming potential calculated according to the principle of instantaneous oxidation.
Hazardous substances
The declaration is based upon reference to threshold values and/or test results and/or material
safety data sheets provided to EPD verifiers. Documentation available upon request to EPD
owner.
■ The product contains no substances given by the REACH Candidate list or the
Norwegian priority list.
□ The product contains substances given by the REACH Candidate list or the Norwegian
priority list that are less than 0,1 % by weight.
□ The product contain dangerous substances, more than 0,1% by weight, given by the
REACH Candidate List or the Norwegian Priority list, see table.
□ The product contains no substances given by the REACH Candidate list or the
Norwegian priority list. The product is classified as hazardous waste (Avfallsforskriften,
Annex III), see table.
Indoor environment
Not relevant
Carbon footprint
Carbon footprint has not been worked out for the product.
EPD for the best environmental decision 12
Additional results
Below the results for the core environmental impact categories for Troja Walker M are
presented, as well as the results of the different scenarios for transport to market (A4) and the
options (inclusion of basket add-on).
Results for Troja Walker M
Indicator Unit A1 A2 A3 A1-A3 A4
GWP-total kg CO2 eq. 6,0E+01 1,2E+00 3,1E+00 6,4E+01 5,8E-01
GWP-fossil kg CO2 eq. 6,0E+01 1,2E+00 2,4E+00 6,4E+01 5,8E-01
GWP-biogenic kg CO2 eq. -4,2E-01 9,5E-04 6,3E-01 2,1E-01 9,2E-04
GWP-LULUC kg CO2 eq. 6,3E-02 7,5E-04 7,3E-03 7,1E-02 1,6E-04
ODP kg CFC11 eq. 2,8E-06 2,1E-08 5,0E-08 2,8E-06 1,3E-08
AP mol H⁺ eq. 3,2E-01 2,1E-02 1,8E-02 3,5E-01 1,2E-03
EP-freshwater kg P eq. 1,0E-02 6,8E-06 1,3E-04 1,0E-02 3,3E-06
EP-marine kg N eq. 4,7E-02 5,3E-03 2,0E-03 5,4E-02 3,3E-04
EP-terrestrial mol N eq. 4,2E-01 5,9E-02 2,5E-02 5,0E-01 3,4E-03
POCP kg NMVOC eq. 1,5E-01 1,7E-02 7,8E-03 1,8E-01 2,1E-03
ADP-M&M kg Sb eq. 4,6E-04 2,1E-06 1,7E-04 6,3E-04 7,7E-07
ADP-fossil MJ 7,5E+02 1,6E+01 3,2E+01 8,0E+02 8,4E+00
WDP m³ 2,1E+01 5,3E-02 1,3E+00 2,3E+01 3,0E-02
Indicator Unit C1 C2 C3 C4 D
GWP-total kg CO2 eq. 0,0E+00 2,8E-01 9,7E+00 1,4E-02 -4,7E+00
GWP-fossil kg CO2 eq. 0,0E+00 2,8E-01 9,7E+00 1,4E-02 -4,4E+00
GWP-biogenic kg CO2 eq. 0,0E+00 7,2E-04 8,3E-04 3,2E-04 -3,2E-01
GWP-LULUC kg CO2 eq. 0,0E+00 1,3E-04 3,1E-05 2,6E-06 -6,6E-03
ODP kg CFC11 eq. 0,0E+00 6,0E-09 6,4E-09 2,6E-10 -4,2E-08
AP mol H⁺ eq. 0,0E+00 9,0E-04 3,1E-03 6,0E-05 -2,7E-02
EP-freshwater kg P eq. 0,0E+00 2,2E-06 1,4E-06 1,4E-07 -1,2E-04
EP-marine kg N eq. 0,0E+00 3,0E-04 1,5E-03 2,2E-04 -5,2E-03
EP-terrestrial mol N eq. 0,0E+00 3,3E-03 1,7E-02 2,5E-04 -5,8E-02
POCP kg NMVOC eq. 0,0E+00 1,3E-03 4,1E-03 9,7E-05 -1,7E-02
ADP-M&M kg Sb eq. 0,0E+00 8,8E-07 2,8E-07 1,6E-08 -2,2E-05
ADP-fossil MJ 0,0E+00 3,9E+00 1,5E+00 2,3E-01 -4,3E+01
WDP m³ 0,0E+00 1,6E-02 2,7E-02 -1,2E-03 -9,6E+00
EPD for the best environmental decision 13
Options
All Topro walkers can be purchased with a basket for transporting goods and possessions.
Found below are the aggregated results for Troja Walker S and M with basket for selected
environmental impacts indicators. The only difference between these results and the results
above are the inclusion of the basket.
Unit Troja Walker S Troja Walker M
Total weight incl. basket kg 8,57 8,86
GWP-total (A1-A3) kg CO2 eq. 61,3 64,8
GWP-total (A1-A4, C1-C4 & D) kg CO2 eq. 69,2 72,4
Total energy consumption MJ 1068 1132
Results for A4 – Transport to market scenarios
To calculate the results for the Scandinavian market (scenario 2) or the European market
(scenario 3), simply substitute the value for A4 in the main results with the results for the
scenarios in the table below.
Troja Walker S
Unit Scenario 1: Norway Scenario 2: Scandinavia Scenario 3: Europe
GWP-total kg CO2 eq. 0,56 3,75 7,59
Troja Walker M
GWP-total kg CO2 eq. 0,58 3,78 7,69
EPD for the best environmental decision 14
Bibliography
ISO 14025:2010 Environmental labels and declarations - Type III environmental
declarations - Principles and procedures
ISO 14044:2006 Environmental management - Life cycle assessment -
Requirements and guidelines
EN 15804:2012+A2:2019 Sustainability of construction works - Environmental product
declaration - Core rules for the product category of construction
products
ISO 21930:2007 Sustainability in building construction - Environmental
declaration of building products
EPD-Norge 2021 NPCR Part A: Construction products and services
EPD-Norge 2022 NPCR 026 Part B for Furniture v. 2
Raadal et al. (2009) Climate account for waste management. Phase I and II: Glass
packaging, Metal Packaging, Paper, Cardboard, Plastic Packaging,
Wet Organic Waste, Tree Waste and Refuse Waste from
Households
Nørsterud (2023) LCA Report for Topro Mobility Aids, Topro Mobility
Program Operator tlf +47 23 08 80 00
The Norwegian EPD Foundation
Post Box 5250 Majorstuen, 0303
e-post: post@epd-norge.no
Oslo
Norway web www.epd-norge.no
Publisher tlf +47 23 08 80 00
The Norwegian EPD Foundation
Post Box 5250 Majorstuen, 0303
e-post: post@epd-norge.no
Oslo
Norway web www.epd-norge.no
Owner of the declaration tlf +47 61 13 46 00
Topro Industri AS Fax
Rambekkvegen 5, 2816 Gjøvik,
e-post: kundeservice@topromobility.com
Norway
Norway web https://www.topromobility.no/
Author of the life cycle assessment tlf +47 41 79 94 17
Sander Nørsterud, Asplan Viak AS Fax
Postboks 24, 1300 Sandvika e-post: asplanviak@asplanviak.no
Norway web www.asplanviak.no
ECO Platform web www.eco-platform.org
ECO Portal web ECO Portal
EPD for the best environmental decision 15
