Environmental product declaration
in accordance with ISO 14025 and EN 15804+A2
Stolit® K/R/MP/Effect
Owner of the declaration: Program operator:
Sto SE & Co. KGaA The Norwegian EPD Foundation
Product: Declaration number:
Stolit® K/R/MP/Effect
NEPD-9260-8849
Declared unit:
1 kg Registration number:
This declaration is based on Product Category Rules: NEPD-9260-8849
CEN Standard EN 15804:2012+A2:2019 serves as core
Issue date: 03.03.2025
PCR
The Norwegian EPD Foundation IBU PCR Part B for coatings with organic binders Valid to: 03.03.2030
EPD software:
LCAno EPD generator ID: 804103
1 / 12
General information
Product Owner of the declaration:
Stolit® K/R/MP/Effect Sto SE & Co. KGaA
Contact person: Linus Kaltenbach
Phone: +49 7744571010
e-mail: l.kaltenbach@sto.com
Program operator: Manufacturer:
The Norwegian EPD Foundation Sto SE & Co. KGaA
Post Box 5250 Majorstuen, 0303 Oslo, Norway Ehrenbachstraße 1
Phone: +47 977 22 020 79780 Stühlingen, Germany
web: www.epd-norge.no
Declaration number: Place of production:
Weizen
NEPD-9260-8849
Ehrenbachstraße 1
79780 Stühlingen, Germany
This declaration is based on Product Category Rules: Management system:
CEN Standard EN 15804:2012+A2:2019 serves as core PCR ISO 14001; ISO 50001; ISO 9001
IBU PCR Part B for coatings with organic binders
Statement of liability: Organisation no:
The owner of the declaration shall be liable for the underlying DE142834082
information and evidence. EPD Norway shall not be liable with respect
to manufacturer information, life cycle assessment data and
evidences.​
Declared unit: Issue date:
1 kg Stolit® K/R/MP/Effect 03.03.2025
Declared unit with option: Valid to:
A1,A2,A3,A4,A5,C1,C2,C3,C4,D 03.03.2030
Year of study:
2023
Functional unit: Comparability:
EPD of construction products may not be comparable if they not
comply with EN 15804 and seen in a building context.
General information on verification of EPD from EPD tools: Development and verification of EPD:
Independent verification of data, other environmental information The declaration is created using EPD tool lca.tools ver EPD2022.03,
and the declaration according to ISO 14025:2010, § 8.1.3 and § 8.1.4. developed by LCA.no. The EPD tool is integrated in the company's
Verification of each EPD is made according to EPD-Norway’s management system, and has been approved by EPD Norway.
guidelines for verification and approval requiring that tools are i) NEPDT143
integrated into the company's environmental management system, ii)
the procedures for use of the EPD tool are approved by EPD-Norway, Developer of EPD: Linus Kaltenbach
and iii) the process is reviewed annually by an independent third
Reviewer of company-specific input data and EPD:​ Angelica Hultin
party verifier. See Appendix G of EPD-Norway's General Programme
Instructions for further information on EPD tools
Verification of EPD tool: Approved:
Independent third party verification of the EPD tool, background data
and test-EPD in accordance with EPDNorway's procedures and
guidelines for verification and approval of EPD tools.
Third party verifier:
Elisabet Amat, GREENIZE projects
(no signature required)
2 / 12
Product
Product description:
Stolit® K/R/MP/Effect is an organic finishing render used on masonry, insulated and rainscreen cladding facades with a base coat and on mineral
and organic substrates. It uses mineral fillers, polymer dispersion ,water and small amounts of additives (thickeners, defoamers, wetting agents,
preservatives, etc.).
Due to the use of different-sized marble granulate, the products texture differs:
Stolit® K is used for a stippled texture.
Stolit® R is used for a rilled texture.
Stolit® MP is used for a fine, free-style texture.
Stolit® Effect is used for a rough, free-style texture.
Stolit® K/R/MP/Effect has the following properties:
-render in accordance with EN 15824
-maximum reliability with regard to application, value retention, color shade, and stability
-A2-s1, d0 in accordance with EN 13501-1
-with encapsulated film protection
-shockproof and highly resistant to cracks and hail when combined with StoTherm Classic®
-highly permeable to water vapour
-highly water-repellent
-weather-resistant
-water-dilutable
-with high-quality marble grains made of natural deposits
For the placing on the market of the product in the European Union/European Free Trade Association (EU/EFTA) (with the exception of
Switzerland) Regulation (EU) No. 305/2011 (CPR) applies. The product needs a declaration of performance taking into consideration EN
15824:2017 title and the CE-marking. For the application and use the respective national provisions apply.
Product specification
The following data is required by the corresponding PCR B. Further information can be found on the Safety Data Sheet on www.sto.de.
1) This product contains substances listed in the candidate list (date: 10.02.2025)
exceeding 0.1 percentage by mass: no.
2) This product contains other
CMR substances in categories 1A or 1B which are not on the
candidate list, exceeding 0.1 percentage by mass: yes
titanium dioxide, pigment, >= 1 - < 10
CAS-nr.: 13463-67-7
3) Biocide products were added to this construction product or
it has been treated with biocide products (this then concerns a
treated product as defined by the (EU) Ordinance on Biocide
Products No. 528/2012): yes
1,2-Benzisothiazol-3(2H)-on; in-can preservative; >= 0,0025 - < 0,025
CAS-nr.: 2634-33-5
2-methyl-2H-isothiazol-3-one in-can preservative; >= 0,0025 - < 0,025
Cas-nr.: 2682-20-4
2-octyl-2H-isothiazol-3-one; dry film preservative; >= 0,0025 - < 0,025
CAS-nr.: 26530-20-1
reaction mass of
5-Chlor-2-methyl-4-isothiazolin-3-on and
2-Methyl-2H​isothiazol-3-on (3:1); in-can preservative; < 0,0002
CAS-nr.: 55965-84-9
The material composition of the declared mixed product is stated below:
Materials Value Unit
Filler 65 - 75 %
Binder 10 - 20 %
Water 10 - 20 %
Additive 1 - 2 %
Pigment 1 - 5 %
3 / 12
Technical data:
The technical data stated here is relevant for the use of the declared product. Further information regarding the technical properties, the
approximate consumption per m2 and the application process can be found on the Technical Data Sheet on www.sto.de.
Criterion Standard/Test specification Class
Density EN ISO 2811 1,7 - 1,9 g/cm³
Water permeability rate w EN 1062-3 W3 low
Reaction to fire EN 13501-1 A2-s1, d0
Market:
The main markets are Germany, Switzerland and Austria.
Reference service life, product
The service life of Stolit® K/R/MP/Effect is 40 years in accordance with the BBSR table "Service lives of components for life cycle assessment
according to BNB" in exterior application.
A reference service life (RSL) in accordance with ISO 15686​-1,-​2,-​7, and ​-8 is not declared. Experience shows that if used as intended and installed
correctly, the working life of finishing render is 50 years and longer.
Reference service life, building or construction works
LCA: Calculation rules
Declared unit:
1 kg Stolit® K/R/MP/Effect
Cut-off criteria:
All major raw materials and all the essential energy is included. The production processes for raw materials and energy flows with very small
amounts (less than 1%) are not included. These cut-off criteria do not​ apply for hazardous materials and substances.
Allocation:
The allocation is made in accordance with the provisions of EN 15804. Incoming energy and water and waste production in-house is allocated
equally among all products through mass allocation. Effects of primary production of recycled materials is allocated to the main product in which
the material was used. The recycling process and transportation of the material is allocated to this analysis.
Data quality:
Specific data for the product composition are provided by the manufacturer. The data represent the production of the declared product and were
collected for EPD development in the year of study. Background data is based on EPDs according to EN 15804 and different LCA databases. The
data quality of the raw materials in A1 is presented in the table below.
Materials Source Data quality Year
Additives CEPE RM Database v3.0 Database 2016
Additives CEPE RM Database v3.0, ecoinvent 3.6 Database 2016
Additives ecoinvent 3.6 Database 2019
Binders CEPE RM Database v3.0, ecoinvent 3.6 Database 2016
Binders and Resins CEPE RM Database v3.0 Database 2016
Chemical ecoinvent 3.6 Database 2019
Fillers ecoinvent 3.6 Database 2019
Packaging - Plastic ecoinvent 3.6 Database 2019
Packaging - Wood Modified ecoinvent 3.6 Database 2019
Pigments and Fillers CEPE RM Database v3.0 Database 2016
Solvent CEPE RM Database v3.0 Database 2016
Water ecoinvent 3.6 Database 2019
4 / 12
System boundaries (X=included, MND=module not declared, MNR=module not relevant)
Construction Beyond the system
Product stage Use stage End of life stage
installation stage boundaries
A1 A2 A3 A4 A5 B1 B2 B3 B4 B5 B6 B7 C1 C2 C3 C4 D
X X X X X MND MND MND MND MND MND MND X X X X X
System boundary:
The scope of this LCA is cradle to gate with options, modules C1-C4 and module D. No actions are to be taken during User stage.
Additional technical information:
Finishing render is categorized under the European Waste Catalogue (EWC), category 17.09 "Other Construction and Demolition Waste" and is
categorized as non-hazardous waste.
waR slairetam tropsnarT gnirutcafunaM tropsnarT ylbmessA e​sU ecnanetniaM riapeR tnemecalpeR tnemhsibrufeR lanoitarepO ygrene esu lanoitarepO esu retaw -eD noitcurtsnoc noitilomed tropsnarT etsaW gnissecorp lasopsiD -yrevoceR-esueR laitnetop-gnilcyceR
5 / 12
LCA: Scenarios and additional technical information
The following information describe the scenarios in the different modules of the EPD.
Modules A1-A3
The raw materials are produced by and transported from suppliers located in Europe. The raw materials are filled in weighting containers and
thereafter mixed together. Quality control checks the consistency of the product and adjusts if necessary. The finished product is filled into pails
and stored. The product is transported on pallets and delivered to the customer.
A4 (Transport to market/building site): Since the distance to the construction site can vary strongly, a distance of 100 km is used to allow simple
scaling for individual projects.
A5 (Installation): The product is applied according to the specifications in the technical data sheet at the construction site. Installation is generally
done manually. Outputs are small amounts of waste from the product itself (assumed to be a maximum of 3 %) and waste from packaging
materials.
C1 (De-construction, demolition): It is assumed that Stolit® K/R/MP/Effect is dismantled using machinery.
C2 (Transport end of life): This stage includes the transportation effects of demolished waste to a waste processing area. The distance between the
demolishing area and a waste processing area is assumed to be quite short (less than 100 km). The distance varies depending on the type of
waste processing.
C3, C4 (Waste processing): Reinforcing compound is not classified as hazardous waste and treated as mixed construction waste. A typical End of
life scenario for construction waste in Germany is a mix of recycling and landfill. Since a 100 % End-of-life scenario has to be declared according to
the PCR, 100 % landfill has been chosen.
D (Environmental costs and benefits of recycling and reuse): Energy credit related to energy recovery from the incineration is included in module
D.
Stages not included:
Once installation is complete, no actions or technical operations are required during the use stage until the end of life stage. Stages B1-B7 are
therefore not declared.
Capacity utilisation Value
Transport from production place to user (A4) Distance (km) Fuel/Energy Consumption Unit
(incl. return) % (Liter/tonne)
Truck, 16-32 tonnes, EURO 6 (kgkm) 36,7 % 104 0,043 l/tkm 4,49
Assembly (A5) Unit Value
Waste, packaging, pallet, EUR wooden pallet,
kg 0,033
reusable, average treatment (kg)
Material loss, including waste treatment (psc) Units 0,030
Waste, packaging, polyethylene, PE plastic parts,
kg 0,017
to average treatment (kg)
De-construction demolition (C1) Unit Value
Electricity, Germany (kWh) kWh 0,013
Capacity utilisation Value
Transport to waste processing (C2) Distance (km) Fuel/Energy Consumption Unit
(incl. return) % (Liter/tonne)
Truck, 16-32 tonnes, EURO 6 (kgkm) 36,7 % 100 0,043 l/tkm 4,30
Disposal (C4) Unit Value
Waste, inert waste, to landfill (kg) kg 1,000000000
Benefits and loads beyond the system
Unit Value
boundaries (D)
Substitution of thermal energy, district heating
MJ 0,017
(MJ)
Substitution of electricity (MJ) MJ 0,0011
Substitution of electricity, in Norway (MJ) MJ 0,00011
Substitution of thermal energy, district heating, in
MJ 0,0016
Norway (MJ)
6 / 12
LCA: Results
The LCA results are presented below for the declared unit defined on page 2 of the EPD document.
Environmental impact
Indicator Unit A1 A2 A3 A4 A5 C1 C2 C3 C4 D
GWP-total
kg CO2 -
3,83E-01 3,94E-02 8,16E-03 1,79E-02 6,39E-02 7,62E-03 1,72E-02 0 8,22E-03 -1,14E-04
eq
GWP-fossil
kg CO2 -
4,32E-01 3,94E-02 6,57E-03 1,79E-02 1,53E-02 7,48E-03 1,72E-02 0 8,20E-03 -1,10E-04
eq
GWP-biogenic
kg CO2 -
-4,95E-02 1,63E-05 7,17E-04 7,42E-06 4,86E-02 1,26E-04 7,10E-06 0 9,58E-06 -2,26E-07
eq
GWP-luluc
kg CO2 -
1,15E-04 1,40E-05 8,76E-04 6,38E-06 2,99E-05 9,07E-06 6,11E-06 0 2,02E-06 -3,78E-06
eq
kg
ODP CFC11 - 8,76E-08 8,92E-09 5,58E-10 4,06E-09 2,92E-09 2,93E-10 3,89E-09 0 3,11E-09 -7,99E-06
eq
mol H+
AP 2,99E-03 1,13E-04 8,12E-06 5,15E-05 9,38E-05 2,17E-05 4,93E-05 0 7,30E-05 -9,04E-07
-eq
EP-FreshWater kg P -eq 6,39E-05 3,14E-07 3,65E-08 1,43E-07 1,90E-06 1,13E-06 1,37E-07 0 9,30E-08 -9,75E-09
EP-Marine kg N -eq 5,32E-04 2,24E-05 2,77E-06 1,02E-05 1,83E-05 3,36E-06 9,76E-06 0 2,71E-05 -2,95E-07
mol N -
EP-Terrestial 4,60E-03 2,50E-04 2,09E-05 1,14E-04 1,51E-04 5,32E-05 1,09E-04 0 2,99E-04 -3,19E-06
eq
kg
POCP NMVOC 1,58E-03 9,59E-05 6,47E-06 4,37E-05 5,15E-05 1,01E-05 4,18E-05 0 8,56E-05 -8,81E-07
-eq
ADP- kg Sb-
9,36E-06 1,09E-06 4,10E-08 4,95E-07 3,33E-07 6,22E-08 4,74E-07 0 7,39E-08 -1,09E-09
minerals&metals1 eq
ADP-fossil1 MJ 8,80E+00 5,95E-01 6,18E-02 2,71E-01 2,76E-01 1,02E-01 2,60E-01 0 2,26E-01 -1,57E-03
WDP1 m3 8,84E+00 5,76E-01 7,59E+00 2,62E-01 4,85E-01 1,03E+00 2,51E-01 0 1,39E+00 -1,95E-02
GWP-total = Global Warming Potential total; GWP-fossil = Global Warming Potential fossil fuels; GWP-biogenic = Global Warming Potential biogenic; GWP-luluc =
Global Warming Potential land use and land use change; ODP = Depletion potential of the stratospheric ozone layer; AP = Acidification potential, Accumulated
Exceedance; EP-freshwater = Eutrophication potential, fraction of nutrients reaching freshwater end compartment: EP-marine = Eutrophication potential, fraction of
nutrients reaching marine end compartment; EP-terrestrial = Eutrophication potential, Accumulated Exceedance; POCP = Formation potential of tropospheric ozone;
ADP-minerals&metals = Abiotic depletion potential for non-fossil resources; ADP-fossil = Abiotic depletion for fossil resources potential; WDP = Water (user)
deprivation potential, deprivation-weighted water consumption
"Reading example: 9,0 E-03 = 9,0*10-3 = 0,009"
*INA Indicator Not Assessed
1. The results of this environmental impact indicator shall be used with care as the uncertainties on these results are high or as there is limited experienced with the
indicator
Remarks to environmental impacts
7 / 12
Additional environmental impact indicators
Indicator Unit A1 A2 A3 A4 A5 C1 C2 C3 C4 D
PM Disease incidence 3,76E-08 2,41E-09 5,40E-11 1,10E-09 1,23E-09 8,40E-11 1,05E-09 0 1,56E-09 -5,40E-11
IRP2 kgBq U235 -eq 2,26E+01 2,60E-03 4,29E-05 1,18E-03 6,77E-01 3,20E-04 1,13E-03 0 1,03E-03 -1,00E-05
ETP-fw1 CTUe 8,81E+00 4,41E-01 4,43E-02 2,01E-01 2,81E-01 8,69E-02 1,92E-01 0 1,23E-01 -8,53E-03
HTP-c1 CTUh 1,29E-09 0,00E+00 2,00E-12 0,00E+00 3,90E-11 2,00E-12 0,00E+00 0 5,00E-12 0,00E+00
HTP-nc1 CTUh 6,96E-08 4,82E-10 6,20E-11 2,19E-10 2,11E-09 8,70E-11 2,10E-10 0 8,90E-11 -9,00E-12
SQP1 dimensionless 2,56E+00 4,16E-01 -1,94E-02 1,89E-01 9,85E-02 2,41E-02 1,82E-01 0 8,69E-01 -1,05E-02
PM = Particulate Matter emissions; IRP = Ionizing radiation – human health; ETP-fw = Eco toxicity – freshwater; HTP-c = Human toxicity – cancer effects; HTP-nc =
Human toxicity – non cancer effects; SQP = Potential Soil Quality Index (dimensionless)
"Reading example: 9,0 E-03 = 9,0*10-3 = 0,009"
*INA Indicator Not Assessed
1. The results of this environmental impact indicator shall be used with care as the uncertainties on these results are high or as there is limited experienced with the
indicator
2. This impact category deals mainly with the eventual impact of low dose ionizing radiation on human health of the nuclear fuel cycle. It does not consider effects due
to possible nuclear accidents, occupational exposure nor due to radioactive waste disposal in underground facilities. Potential ionizing radiation from the soil, from
radon and from some construction materials is also not measured by this indicator.
8 / 12
Resource use
Indicator Unit A1 A2 A3 A4 A5 C1 C2 C3 C4 D
PERE MJ 4,94E-01 8,52E-03 8,56E-02 3,88E-03 1,74E-02 1,85E-02 3,72E-03 0 8,08E-03 -9,69E-03
PERM MJ 4,58E-01 0,00E+00 0,00E+00 0,00E+00 -4,44E-01 0,00E+00 0,00E+00 0 0,00E+00 0,00E+00
PERT MJ 9,52E-01 8,52E-03 8,56E-02 3,88E-03 -4,27E-01 1,85E-02 3,72E-03 0 8,08E-03 -9,69E-03
PENRE MJ 8,79E+00 5,95E-01 6,18E-02 2,71E-01 2,81E-01 1,02E-01 2,60E-01 0 2,26E-01 -1,57E-03
PENRM MJ 7,56E-01 0,00E+00 0,00E+00 0,00E+00 -7,38E-01 0,00E+00 0,00E+00 0 0,00E+00 0,00E+00
PENRT MJ 9,55E+00 5,95E-01 6,18E-02 2,71E-01 -4,57E-01 1,02E-01 2,60E-01 0 2,26E-01 -1,57E-03
SM kg 1,86E-04 0,00E+00 0,00E+00 0,00E+00 4,33E-06 0,00E+00 0,00E+00 0 0,00E+00 0,00E+00
RSF MJ 8,35E-03 3,05E-04 1,80E-05 1,39E-04 2,20E-04 5,78E-03 1,33E-04 0 1,68E-04 -1,70E-06
NRSF MJ 2,58E-03 1,09E-03 2,38E-05 4,96E-04 1,13E-04 1,87E-05 4,75E-04 0 3,62E-04 -5,74E-04
FW m3 8,24E-03 6,36E-05 6,66E-04 2,90E-05 2,67E-04 4,63E-05 2,78E-05 0 2,78E-04 -1,17E-05
PERE = Use of renewable primary energy excluding renewable primary energy resources used as raw materials; PERM = Use of renewable primary energy resources used
as raw materials; PERT = Total use of renewable primary energy resources; PENRE = Use of non renewable primary energy excluding non-renewable primary energy
resources used as raw materials; PENRM = Use of non renewable primary energy resources used as raw materials; PENRT = Total use of non renewable primary energy
resources; SM = Use of secondary materials; RSF = Use of renewable secondary fuels; NRSF = Use of non-renewable secondary fuels; FW = Net use of fresh water
"Reading example: 9,0 E-03 = 9,0*10-3 = 0,009"
*INA Indicator Not Assessed
9 / 12
End of life - Waste
Indicator Unit A1 A2 A3 A4 A5 C1 C2 C3 C4 D
HWD kg 3,21E-03 3,07E-05 1,04E-03 1,40E-05 1,28E-04 1,01E-05 1,34E-05 0 0,00E+00 -7,37E-08
NHWD kg 1,36E-01 2,89E-02 1,55E-03 1,32E-02 2,44E-02 4,28E-04 1,26E-02 0 1,00E+00 -3,71E-05
RWD kg 1,36E-05 4,05E-06 5,93E-08 1,85E-06 4,95E-07 4,11E-07 1,77E-06 0 0,00E+00 -8,21E-09
HWD = Hazardous waste disposed; NHWD = Non-hazardous waste disposed; RWD = Radioactive waste disposed
"Reading example: 9,0 E-03 = 9,0*10-3 = 0,009"
*INA Indicator Not Assessed
End of life - Output flow
Indicator Unit A1 A2 A3 A4 A5 C1 C2 C3 C4 D
CRU kg 0,00E+00 0,00E+00 0,00E+00 0,00E+00 3,14E-02 0,00E+00 0,00E+00 0 0,00E+00 0,00E+00
MFR kg 0,00E+00 0,00E+00 6,19E-04 0,00E+00 9,09E-03 0,00E+00 0,00E+00 0 0,00E+00 0,00E+00
MER kg 0,00E+00 0,00E+00 4,81E-03 0,00E+00 1,78E-03 0,00E+00 0,00E+00 0 0,00E+00 0,00E+00
EEE MJ 0,00E+00 0,00E+00 2,93E-03 0,00E+00 1,33E-03 0,00E+00 0,00E+00 0 0,00E+00 0,00E+00
EET MJ 0,00E+00 0,00E+00 4,43E-02 0,00E+00 2,02E-02 0,00E+00 0,00E+00 0 0,00E+00 0,00E+00
CRU = Components for re-use; MFR = Materials for recycling; MER = Materials for energy recovery; EEE = Exported energy electrical; EET = Exported energy thermal
"Reading example: 9,0 E-03 = 9,0*10-3 = 0,009"
*INA Indicator Not Assessed
Biogenic Carbon Content
Indicator Unit At the factory gate
Biogenic carbon content in product kg C 0,00E+00
Biogenic carbon content in accompanying packaging kg C 1,36E-02
Note: 1 kg biogenic carbon is equivalent to 44/12 kg CO2
10 / 12
Additional requirements
Greenhouse gas emissions from the use of electricity in the manufacturing phase
National production mix from import, low voltage (production of transmission lines, in addition to direct emissions and losses in grid) of applied
electricity for the manufacturing process (A3).
Electricity mix Source Amount Unit
Electricity, low voltage, 100% hydro, certificate, 01.01.2023-31.12.2023, Germany (kWh) Modified ecoinvent 3.6 60,95 g CO2-eq/kWh
Dangerous substances
The product contains no substances given by the REACH Candidate list.
Indoor environment
Additional Environmental Information
Additional environmental impact indicators required in NPCR Part A for construction products
Indicator Unit A1 A2 A3 A4 A5 C1 C2 C3 C4 D
GWPIOBC kg CO2 -eq 4,32E-01 3,94E-02 8,00E-03 1,79E-02 1,53E-02 8,19E-03 1,72E-02 0 8,21E-03 -1,12E-04
GWP-IOBC: Global warming potential calculated according to the principle of instantaneous oxidation. In order to increase the transparency of biogenic carbon​
contribution to climate impact, the indicator GWP-IOBC is required as it declares climate impacts calculated according to the principle of instantaneous oxidation.​
GWP-IOBC is also referred to as GWP-GHG in context to Swedish public procurement legislation.
11 / 12
Bibliography
ISO 14025:2010 Environmental labels and declarations - Type III environmental declarations - Principles and procedures.
ISO 14044:2006 Environmental management - Life cycle assessment - Requirements and guidelines.
EN 15804:2012+A2:2019 Environmental product declaration - Core rules for the product category of construction products.
ISO 21930:2017 Sustainability in buildings and civil engineering works - Core rules for environmental product declarations of construction
products.
ecoinvent v3, Allocation, cut-off by classification, Swiss Centre of Life Cycle Inventories.
Iversen et al., (2021) eEPD v2021.09 Background information for EPD generator tool system verification, LCA.no Report number: 07.21
Ruud and Iversen (2023) EPD generator for PCR IBU Part B: Requirements on the EPD for Coatings with organic binders, LCA.no report number:
13.23
NPCR Part A: Construction products and services. Ver. 2.0. April 2021, EPD-Norge.
IBU PCR Part B: Requirements on the EPD for Coatings with organic binders, version 4, 2023, IBU - Institut Bauen und Umwelt e.V.
Program operator and publisher Phone: +47 977 22 020
The Norwegian EPD Foundation e-mail: post@epd-norge.no
Post Box 5250 Majorstuen, 0303 Oslo, Norway web: www.epd-norge.no
Owner of the declaration: Phone: +49 7744571010
Sto SE & Co. KGaA e-mail: l.kaltenbach@sto.com
Ehrenbachstraße 1, 79780 Stühlingen, Germany web: https://www.sto.com/
Author of the Life Cycle Assessment Phone: +47 916 50 916
LCA.no AS e-mail: post@lca.no
Dokka 6A, 1671 Kråkerøy, Norway web: www.lca.no
Developer of EPD generator Phone: +47 916 50 916
LCA.no AS e-mail: post@lca.no
Dokka 6A, 1671 Kråkerøy, Norway web: www.lca.no
ECO Platform web: www.eco-platform.org
ECO Portal web: ECO Portal
12 / 12
