ver1 2015
ENVIRONMENTAL PRODUCT DECLARATION
in accordance with ISO 14025, ISO 21930 and EN 15804
Owner of the declaration: Hydro Aluminium AS
Program operator: The Norwegian EPD Foundation
Publisher: The Norwegian EPD Foundation
Declaration number: NEPD-2349-1085-EN
Registration number: NEPD-2349-1085-EN
ECO Platform reference number: -
Issue date: 08.09.2020
Valid to: 08.09.2025
Hydro HyForge Aluminium for forging
Hydro Aluminium AS
www.epd-norge.no
NEPD-2349-1085-EN Hydro HyForge Aluminium for forging
General information
Product: Owner of the declaration:
Hydro HyForge Aluminium for forging Hydro Aluminium AS
Contact person: Lars Andre Moen
Phone: +47 977 94 968
e-mail: Lars.Moen@Hydro.com
Program operator: Manufacturer:
The Norwegian EPD Foundation Hydro Aluminium AS
Pb. 5250 Majorstuen, 0303 Oslo Drammensveien 263, N-0240 Oslo
Phone: +47 23 08 80 00 Phone: +47 22538100
e-mail: post@epd-norge.no e-mail: greener.aluminium@hydro.com
Declaration number: Place of production:
NEPD-2349-1085-EN Husnes
ECO Platform reference number: Management system:
ISO 14001, ISO 50001
This declaration is based on Product Category Rules: Organisation no:
CEN Standard EN 15804 serves as core PCR 917 537 534
NPCR 013, "Version 3.0 Part B for steel and aluminium
construction products"
Statement of liability: Issue date:
The owner of the declaration shall be liable for the underlying 08.09.2020
information and evidence. EPD Norway shall not be liable with
respect to manufacturerinformation, life cycle assessment data Valid to:
and evidences. 08.09.2025
Declared unit: Year of study:
1 kg of Hydro HyForge Aluminium for forging produced 2020
according to the certified Hydro Reduxa 4.0 route
Declared unit with option: Comparability:
1 kg of Hydro HyForge Aluminium for forging produced EPD of construction products may not be comparable if they not
according to the certified Hydro Reduxa 4.0 route, including comply with EN 15804 and seen in a building context.
waste handling and possible environmental benefits after
end of life.
Functional unit: The EPD has been worked out by:
The product is an input to several products. No use Irmeline de Sadeleer, Andreas Brekke, Kari-Anne Lyng
scenarios are defined, hence no functional unit.
Verification:
The CEN Norm EN 15804 serves as the core PCR.
Independent verification of the declaration and data,
according to ISO14025:2010
internal external
Approved
Third party verifier:
Jane Anderson, Construction LCA Limited
(Independent verifier approved by EPD Norway)
NEPD-2349-1085-EN Hydro HyForge Aluminium for forging 2/8
Product
Product description: Technical data:
This EPD covers Reduxa HyForge casthouse products made All products are produced with Hycast Low Pressure (LPC)
from Hydro Reduxa certified low carbon footprint aluminium. casting technology. The product has a lean inverse segregation
https://www.hydro.com/en-NO/products-and-services/low- zone (ISZ). As a result, there is no need for further process steps
carbon-aluminium/hydro-reduxa-4.0/ like scalping, extrusion or machining. The HyForge™ material
The primary Aluminum used in the products is produced based can thus be used directly in the forging or impact extrusion
on renewable power production in Norway. This ensures a process. The material is Ultrasonic tested with EN- B594 Class A.
maximum Carbon footprint of 4.09 tons CO e/tAl, of which For more detailed information about shapes, dimensions and
2
infrastructure acounts for 0,09 CO e/t. tolerances:
2
https://www.hydro.com/en-NO/products-and-services/casthouse-
Exampe of applications: products/hyforge/
Automotive: Chassis components, powertrain components. Non
automotive: high pressure tanks, scuba tanks, fire extinguisher
tanks, bicycle parts, motorbike parts.
All products are produced at Husnes Primary casthouses in Typical Material Properties 6082
Norway.
All products are produced according to EN-603, and customer
specifications. The products are variants within the 6000-alloy
groups.
Product specification:
Typical content of the Aluminium Products:
Materials kg %
Primary Liquid Al from own Electrolysis 0.956 96 %
Primary Metal from external sources 0.015 1 %
Alloying Elements 0.029 3 %
Typical values for products following the Reduxa production route
Reference service life, product:
Depends on product application, but the material itself has an
infinite life time.
Market:
Europe and Global
NEPD-2349-1085-EN Hydro HyForge Aluminium for forging 3/8
LCA: Calculation rules
Declared unit: System boundary:
1 kg of Hydro HyForge Aluminium for forging produced Cradle to gate with options. The following stages have been
according to certified Hydro Reduxa 4.0 route. The EPD declared: A1-A4, C2-C4 and D. Further specificed in flow sheet
also covers modules C2-C4 and D. below.
The Hydro HyForge Aluminium for forging is produced in
the Husnes smelter. The results are based on the Module D covers the potential benefits from recycling of Hydro
production volumes of 2017. HyForge Aluminium for forging after end of useful life. Module D
covers all necessary stages from C3 until the aluminium is back
on to the market and compares to the environmental performance
of an average market forge ingot. The module is further specified
under scenarios.
Mass balance over the Hydro HyForge Aluminium for forging value chain:
Data quality: Cut-off criteria:
Specific data were used for all of Hydro's processes, based on All major raw materials and all the essential energy flows are
the production year 2017, and were collected the first months of included. The production processes for raw materials and
2019. As Hydro has ownership in a total value chain from energy flows with very small amounts (<1%) were not included in
mining of bauxite to production of HyForge, all stages from A1 this analysis. This cut-off rule does not apply to
to A4 are covered by specific data. Background data on for hazardous materials and substances, but mostly to
instance transport and electricity production are from ecoinvent alloying elements that are added in less than per
3.4 (April 2018). thousandth.
Allocation:
The allocation is made in accordance with the provisions of
EN 15804. Incoming energy, water and waste production
inhouse are allocated equally among all products through
mass allocation. For almost all processes, detailed data are
provided for each step, and the main allocation is done
between aluminium hydroxide and aluminium oxide in the
production of alumina. Effects of primary production of
recycled materials are allocated to the main product in
which the material was used. The recycling process and
transportation of the material are allocated to this analysis.
NEPD-2349-1085-EN Hydro HyForge Aluminium for forging 4/8
LCA: Scenarios and additional technical information
The following information describe the scenarios in the different modules of the EPD.
The transport from the Husnes production site to market first happens by boat to a location in cental Europe. Therefrom, the average
distance by truck is assumed to be 500km.
Transport from production place to user (A4)
Type Capacity utilisation Type of vehicle Distance km Fuel/Energy
(incl. return) % consumption
Truck 50 Lorry, >32 metric tons, Euro V 500 2.46 E-02 l/tkm
Boat 80 Cargo ship, 5000 tons 954 1.56 E-02 l/tkm
Most of the aluminium used in the automotive industry is collected (approximately 95%) and recycled (approximately 97% of the
collected aluminium), giving a total of 92% recycled. The rest is assumed landfilled.
End of Life (C2, C3, C4)
Unit Value
Hazardous waste disposed kg -
Collected kg 0,95
Reuse kg -
Recycling kg 0,923
Energy recovery kg 0.027*
To landfill kg 0.05**
*27 grams of the original 1 kg of aluminium is going to incineration. No loads or beneifts are attribuded to this flow.
**There will be a small portion of aluminium ending as uncollected. This is included under "To landfill" where no loads or benefits are included.
Transport to waste processing (C2)
Type Capacity utilisation Type of vehicle Distance km Fuel/Energy
Truck 40 Lorry, >32 metric tons, Euro V 50 2.85 E-02 l/tkm
Aluminium from the shredder to waste handling site is assumed to be transported in an older medium-sized lorry with smaller
capacity utilization than in the production system.
Benefits and loads beyond the system boundaries
(D)
Unit Value
Aluminium foundry alloy to recycling g 924
Aluminium collected and recycled is assumed to replace an average extrusion ingot in Europe consisting of 40% recycled and
60% primary aluminium. This is a conservative approach.
NEPD-2349-1085-EN Hydro HyForge Aluminium for forging 5/8
LCA: Results
System boundaries (X=included, MND= module not declared, MNR=module not relevant)
x
Environmental impact
1,74E-05
4,20E-04 6,97E-04 0,00E+00
6,20E-05
8,76E-08
Resource use
0,00E+00
noitilomed
noitcurtsnoc-eD
MND
tnemecalpeR
B5
TRPE MJ 3,39E+01
SM kg
RSF MJ 0,00E+00
MJ
m3 6,40E-02
ecnanetniaM
esu
retaw
lanoitarepO
A1 A5
x
7,77E-03
ODP 3,46E-07
ylbmessA
x
A4 C2
kg PO 3--eqv 4
1,34E+00
MJ
MJ
0,00E+00
gnirutcafunaM
Product stage Assemby stage
x
tropsnarT
0,00E+00
slairetam
waR
esU
A3 A4 B3 D
MND MND
A1-A3 C3
5,90E-02 -4,87E+00
9,62E-09 -2,98E-07
9,54E-04 3,03E-05 0,00E+00 -2,61E-03
-3,10E-02
-7,67E-03
-1,22E-05
0,00E+00 -4,71E+01
D
0,00E+00
0,00E+00
-2,29E+01
-5,72E+01
0,00E+00
-5,72E+01
0,00E+00
0,00E+00
0,00E+00 0,00E+00
0,00E+00 -4,36E-02
lasopsiD
-gnilcyceR-yrevoceR-esueR
laitnetop
C4
x
gnissecorp
etsaW
All results are calculated with the use of SimaPro v.9 (2019) and impact methods according to ISO 15804. Results are based on a weighted
average between three production sites.
Beyond the
system
boundaries
B2 B4 B6 B7 C1 C3
x MND MND MND MND x x
C4 D
GWP 4,09E+00 2,48E-01
kg CFC11-eqv 1,67E-08 1,44E-09 0,00E+00
POCP kg C 2H 4 -eqv 1,29E-06
AP kg SO 2 -eqv 2,08E-02 3,05E-05
EP 6,91E-03 7,15E-06 0,00E+00
ADPM 1,26E-05 2,34E-08 0,00E+00
MJ 3,35E+01 1,42E+00
Unit A1-A3 A4 C3 C4
RPEE MJ 5,71E+01 1,06E-02 1,71E-01 -2,29E+01
RPEM 0,00E+00 0,00E+00 0,00E+00
TPE 1,19E-03 1,71E-01 0,00E+00
NRPE MJ 1,20E-01 1,52E+00 0,00E+00
0,00E+00 0,00E+00 0,00E+00
1,36E+00 1,20E-01 0,00E+00
0,00E+00 0,00E+00 0,00E+00 0,00E+00
0,00E+00 0,00E+00 0,00E+00
NRSF 0,00E+00 0,00E+00
W 0,00E+00 2,25E-05
RPEE Renewable primary energy resources used as energy carrier; RPEM Renewable primary energy resources used as raw materials; TPE Total use
of renewable primary energy resources; NRPE Non renewable primary energy resources used as energy carrier; NRPM Non renewable primary energy
resources used as materials; TRPE Total use of non renewable primary energy resources; SM Use of secondary materials; RSF Use of renewable
secondary fuels; NRSF Use of non renewable secondary fuels; W Use of net fresh water
esu
ygrene
lanoitarepO
Use stage End of life stage
B1
Unit
kg CO -eqv
2
tropsnarT
C2
Parameter
riapeR
tnemhsibrufeR
tropsnarT
A2
MND MND
4,99E-04
kg Sb-eqv 1,64E-06
ADPE 1,25E-01
GWP Global warming potential; ODP Depletion potential of the stratospheric ozone layer; POCP Formation potential of tropospheric photochemical
oxidants; AP Acidification potential of land and water; EP Eutrophication potential; ADPM Abiotic depletion potential for non fossil resources; ADPE
Abiotic depletion potential for fossil resources
Parameter C2
1,19E-03
0,00E+00 0,00E+00
5,71E+01 1,06E-02
3,39E+01 1,36E+00
NRPM MJ 0,00E+00
1,52E+00
0,00E+00
0,00E+00
0,00E+00
7,37E-04
NEPD-2349-1085-EN Hydro HyForge Aluminium for forging 6/8
End of life - Waste
Parameter Unit A1-A3 A4 C2 C3 C4 D
HW kg 4,73E-02 6,28E-07 7,60E-08 6,10E-03 0,00E+00 4,91E-03
NHW kg 3,39E+00 6,68E-02 6,35E-03 1,15E+00 1,00E+00 -2,49E+00
RW kg 1,58E-04 9,42E-06 8,11E-07 4,80E-06 0,00E+00 -2,26E-04
HW Hazardous waste disposed; NHW Non hazardous waste disposed; RW Radioactive waste disposed
End of life - Output flow
Parameter Unit A1-A3 A4 C2 C3 C4 D
CR kg - - - - - -
MR kg - - - 9,24E-01 - -
MER kg - - - 2,57E-02 - -
EEE MJ - - - - - -
ETE MJ - - - - - -
CR Components for reuse; MR Materials for recycling; MER Materials for energy recovery; EEE Exported electric energy; ETE Exported thermal energy
Reading example: 9.0 E-03 = 9.0*10-3 = 0.009
Additional Norwegian requirements
Greenhouse gas emission from the use of electricity in the manufacturing phase
National production mix from import, low voltage (production of transmission lines, in addition to direct emissions and losses in grid)
of applied electricity for the manufacturing prosess (A3).
Data source Amount Unit
econinvent v3.4 (April 2018) 4 g CO -eqv/kWh
2
Dangerous substances
x The product contains no substances given by the REACH Candidate list or the Norwegian priority list
The product contains substances given by the REACH Candidate list or the Norwegian priority list that are less than 0.1 % by
weight.
The product contain dangerous substances, more than 0.1% by weight, given by the REACH Candidate List or the
Norwegian Priority list, see table.
The product contains no substances given by the REACH Candidate list or the Norwegian priority list. The product is classified
as hazardous waste (Avfallsforskiften, Annex III), see table.
Name CAS no. Amount
Indoor environment
Not relevant
Carbon footprint
Calculations connected to climate change and global warming potential (GWP) include greenhouse gas emissions from fossil
sources and land use change connected to extraction of bauxite, but does not include calculations of biogenic emissions of CO .
2
NEPD-2349-1085-EN Hydro HyForge Aluminium for forging 7/8
Bibliography
ISO 14025:2010 Environmental labels and declarations - Type III environmental declarations - Principles and
procedures
ISO 14044:2006 Environmental management - Life cycle assessment - Requirements and guidelines
EN 15804:2012+A1:2013 Sustainability of construction works - Environmental product declaration - Core rules for the
product category of construction products
ISO 21930:2007 Sustainability in building construction - Environmental declaration of building products
NPCR 013 NPCR 013 version 3.0 Part B for steel and aluminium construction products.
Sadeleer, I., Brekke, A. and Background report for the Environmental Product Declarations for Hydro Aluminium Reduxa
Lyng, Kari-Anne (2020) HyForge
Program operator Phone: +47 23 08 80 00
The Norwegian EPD Foundation
Post Box 5250 Majorstuen, 0303 Oslo e-mail: post@epd-norge.no
Norway web www. epd-norge.no
Publisher Phone: +47 23 08 82 92
The Norwegian EPD Foundation
Post Box 5250 Majorstuen, 0303 Oslo e-mail: post@epd-norge.no
Norway web www.epd-norge.no
Owner of the declaration Phone: +47 977 94 968
Hydro Aluminium AS Fax
Drammensveien 263 e-mail: Lars.Moen@Hydro.com
N-0240 Oslo web www.hydro.com
Author of the Life Cycle Assessment Phone: +47 69 35 11 00
NORSUS Norwegian Institute for Sustainability Research Fax +47 69 34 24 94
Stadion 4 e-mail: post@ostfoldforskning.no
1671 Kråkerøy web www.ostfoldforskning.no
NEPD-2349-1085-EN Hydro HyForge Aluminium for forging 8/8
