Environmental Product
Declaration
In accordance with ISO 14025 and EN 15804 +A1
NTech outward opening topswing windows 105/80 – TG &
TY (without aluminium cladding)
Owner of the declaration:
NorDan AS Product name:
Program holder and publisher: NTech outward opening
topswing windows 105/80 –
TG & TY (without aluminium
The Norwegian EPD foundation
Declaration number: cladding)
N ReE gP iD s- t3 ra4 t5 i6 o- n2 0 N5 u7 m-E bN
e r: Manufacturer:
NorDan AS
NEPD-3456-2057-EN
Issue date:
Valid to:
02.05.2022
The Norwegian 02.05.2027
EPD Foundation
General information
Product: Owner of the declaration:
NTech outward opening topswing windows 105/80 – TG & TY NorDan AS
(without aluminium cladding) Kontaktperson: Fredrik Jonsson
Tlf: +46 (0) 10-130 01 78
e-post: fredrik.jonsson@nordan.se
Program holder: Manufacturer:
The Norwegian EPD Foundation NorDan sp. z o.o.
Post Box 5250 Majorstuen, 0303 Oslo Fabryczna 16, PL-64-200 Wolsztyn, Poland
Tlf: +47 977 22 020
e-mail: post@epd-norge.no Phone: +48 68 34 70 500
Fax: 048 68 34 73 541
Declaration number: Place of production:
NEPD-3456-2057-EN Wolsztyn, Poland
ECO Platform registration number: Management system:
NorDan sp. z o.o. Works with EN ISO 9001:2015, ISO
14001:2015
This declaration is based on Product Category Rules:
CEN Standard EN 15804 serves as core PCR
NPCR 014:2019 Part B for windows and doors version 3.0 Org. no.:
NO 979 776 233 MVA
Declaration of responsibility: Issue date:
The owner of the declaration shall be responsible for the 02.05.2022
underlying information and evidence. EPD Norway shall not
be responsible with regard to manufacturer information, life
cycle data and evidence.
Valid to:
02.05.2027
Declared unit: Year of study:
2021
Declared unit with option: Comparability:
EPD of construction products may not be comparable if they
are not comply with NS-EN 15804 and seen in a building
context.
Functional unit:
1 window measuring 1.23 m x 1.48 m (reference window based
on EN 14351-1) with an expected service life of 40 yrs. with an The EPD has been worked out by:
essential parameter U-value = 0,82W/m2K. Conversion factor Roja Modaresi
is 66.21 [Kg/FU]. Norsk Treteknisk Institutt
Verification:
Independent verification of the declaration and data,
according to ISO14025:2010
internal external
Approved
Third party verifier:
Gaylord K. Booto PhD., Senior Research Scientist, NORSUS AS
(Independent verifier approved by EPD Norway)
NEPD-3456-2057-EN NTech outward opening topswing windows 105/80 – TG & TY (without aluminium cladding)
2/9
Product
Product description: Technical data:
Window with outward opening fully reversible opening sash for use Outward opening window. Triple glazed, 105mm frame,
in exterior walls of domestic and commercial buildings. 80mm sash. Uwin 0,82W/m2K. Certified: BBA, Secured by
Design, SP Sitac “P”.
Product specification:
The total weight is 66.2 kg. The packaging has a average
25% of aluminium and 18% of glass is produced from recycled
weight of 3.2 kg.
material.
Product group TG & TY is covered in this EPD. The highest
amount for constituent material has been used.
Materialer kg %
Pine timber 16.57 25.03 Market:
Glass 40.93 61.82 Europe, but scenarios beyond cradle to gate are based
Spacer 0.73 1.11 on the situation in the Norwegian market.
Triple glazed Butyl 0.02 0.04
unit Sealant 1.08 1.63
Argon 0.07 0.11
Absorbent 0.02 0.03
Paint 0.57 0.86 Reference service life:
Aluminium 1.28 1.93 The reference service life is 40 years for windows with a
Plastic 0.11 0.17 painted timber frame.
Gasket 0.49 0.74
Metal- Steel alloys 4.26 6.43
Sealant and Glue 0.08 0.12
Total weight of the product 66.21 100
Wood packaging 3.1
Steel packaging 0.05
Plastic packaging 0.08
Total weight with packaging 69.44
LCA: Calculation rules
Functional unit: System boundary:
1 window measuring 1.23 m x 1.48 m (reference window based on All modules are included. Below is a technical flowchart for
EN 14351-1) with an expected service life of 40 yrs. with an the production line at NorDan. Modul D is calculated with
essential parameter U-value = 0,82W/m2K. Conversion factor is energy substitution and explained in the scenarios.
66.21 [Kg/FU].
NEPD-3456-2057-EN NTech outward opening topswing windows 105/80 – TG & TY (without aluminium cladding)
3/9
Data quality Cut-off criteria:
Data is representative of year 2019 and was collected in 2020- All raw materails and energy use is included. Where data was
2021. Data is taken from processes from Ecoinvent 3.1-3.7. Some available for infrastructure from Ecoinvent, it is included.
processes are based on Ecoinvent v3.1 (2014) and v3.2 (2015), Example: ‘Metal working factory'. In the production process,
but all upstream processes are v3.4 (2017)-3.5 (2018). Remaining raw materials and energy of low amounts are not included
data is based on Ecoinvent v3.7 (2020). "Allocation cut-off by (<1%). These cut-off rules do not apply to dangerous
classification" (2017) adjusted to improve representativeness. substances.
Allocation: Calculations of biogenic carbon:
Allocation is done in accordance with the provisions of EN 15804. Sequestration and release of biogenic carbon is included
Allocation of energy, water and waste from production is calculated according to EN 16485:2014. This is based on the modularity
by a physical allocation factor based on the manufacturer input. principle in EN 15804:2012 that specifies that the emissions
For waste produced at the manufacturing, the burdens for reuse, shall be accounted in the module that they occur. The amount
recycling and recovery is allocated by using this allocation factor. of carbon dioxide sequestrated is calulated in accordance to
EN 16449:2014. Timber comes from sustainable forestry and
has FSC certified traceability.
LCA: Scenarios and additional technical information
The following information describe the scenarios in the different modules of the EPD
The transportation from production to construction site is based on a scenario where the product is transported on a large lorry from
Poland to Oslo, Norway (1250 km) and then to a warehouse which is assumed to be in a 250 km radius from Oslo. Transport from
warehouse to a construction site is assumed to be 50 km on a medium truck.
Transport from production place to assembly/user (A4)
Type Capacity utilisation Type of vehicle Distance km Fuel/Energy Fuel/Energy
(incl. return) % consumption pr tkm consumption pr km
Truck 53 EURO5, >32 tonn 1500 0.023 l/tkm 0.31 l/km
Truck 26 EURO5, 16-32 tonn 50 0.045 l/tkm 0.25 l/km
Installation (A5)
Unit Value According to the report from EPD-Norge ‘Harmonising the
Auxiliary kg 0 documentation of scenarios beyond cradle to gate, EN 15804’ there is
Water consumption m3 0 no loss on site during construction activities. The window products in
Electricity consumption MJ 0 this EPD are painted and surface treated in the production and not at
Other energy carriers MJ 0 the building site. Therefore, there is only 2 items left in this module. 1)
Material loss kg 0 Waste treatment of packaging which is considered in the EPD
Output materials from waste treatment kg 3.23 calculations. 1) Energy use during installation. This can be varied
Dust in the air kg 0 depending on the floor, type of building and several other unknown
parameters, and therefore ignored in the calculation.
Maintenance (B2)/Repair (B3)
The maintenance scenario included cleaning, painting and change of
Unit Value IGU. Cleaning is performed three times per year. It is calculated with
1,5 dl of detergent and 3 litres of water each year. Windows are
Detergents kg 6
painted 2 times from inside and 4 times from outside. It is assumed
Water consumption l 120
that 5 gr of lubricating oil is used every year for fittings and moving
Lubricating oil kg 0.20
parts. No repair is assumed during the product lifetime.
Paint kg 1.31
Transport tkm 2.25
Glazing unit kg 0
Synthetic rubber kg 0
Transport (IGU) tkm 0
NEPD-3456-2057-EN NTech outward opening topswing windows 105/80 – TG & TY (without aluminium cladding)
4/9
Replacement (B4)/Refurbishment (B5)
*Number or RSL (Reference Service Life). The window has RSL of 40
Unit Value years for without aluminium cladding. Windows is assumed to have
Replacement cycle* yr 30 one entire window replacement during the lifetime of the building. It is
Electricity consumption kWh 0 assumed that this change is occured after 30 years when the IGU
Replacement of worn parts 0 0 reaches its end of life. There is no need for refurbishment during the
product lifetime.
(C1) As there are no data for de-construction, it is assumed no activites in C1 in this study. The windows are assumed to be treated as
mixed waste and sent to incineration. The combustible materials are then energy recovered, while glass is assumed to end up in the
bottom ash and then landfilled. The metals are usually sorted out of the bottom ash and then recycled, but there is no data of the share
which are recycled and therefore standard values from Ecoinvent is utilized.
The transport of window as waste is calculated based on a scenario with 50 km distance.
Transport to waste processing (C2)
Type Capacity utilisation Type of vehicle Distance km Fuel/Energy Fuel/Energy
(incl. return) % consumption pr tkm consumption pr km
Truck 44 Unspecified 50 0.03l/tkm 0.28 l/km
Windows are assumed to be sorted as mixed construction waste and treated with incineration with energy recovery. The recycling of
material mentioned in the below table is only from the metals at the EOL with considering efficiency factor, and with the use of
generic processes from Ecoinvent. However, the manufacturer has documented the recycling potentials for its product in the
Construction Product Declaration eBVD
NorDan TG Vridfönster Trä 105, ID: C-SE556294452901-66 URL: https://www.ebvd.org/BMI/Document/Export/2948/0/Pdf NorDan
TY Vridfönster Trä 105, ID: C-SE556294452901-27 URL: https://www.ebvd.org/BMI/Document/Export/1598/0/Pdf
In the documentation, Chapter 10, the specific material recovery, and energy recovery potential is reported for the product.
End of Life (C1, C3, C4)
Unit Value
Hazardous waste disposed kg 0
Collected as mixed construction waste kg 66.21
Reuse kg 0
Recycling kg 2.64
Energy recovery kg 63.57
To landfill kg 0.00
The benefits beyond life cycle has been modelled based on the output flows from module C3. This includes energy from incineration and
scrap metal recovered from the ashes. The amount recovered metal is assumed to avoid production of primary metals in accordance to
6.4.3.3 in EN 15804. The exported energy is substituting Norwegian district heating mix and electricity mix. Inventory processes causing
substitution of avoided virgin raw materials has be constructed for each material.
Benefits and loads beyond the system boundaries (D)
Unit Value
Substitution of electricity MJ 44.8
Substitution of thermal energy MJ 444.8
Substitution of raw materials kg 5.4
NEPD-3456-2057-EN NTech outward opening topswing windows 105/80 – TG & TY (without aluminium cladding)
5/9
LCA: Results
System boundaries (X = included)
Beyond the
system
boundaries
B4
X X
Environmental impact Without alu clad
B1 B3 B4 B5
0.00E+00 9.520831 0.00E+00 1.34E+02 0.00E+00
0.00E+00 6.36E-07 0.00E+00 7.03E-06 0.00E+00
0.00E+00 4.40E-03 0.00E+00 1.66E-01 0.00E+00
0.00E+00
x 0.00E+00
C2
-3.41E+01
-1.31E-06
5.25E-05 2.42E-04 1.18E-04
-1.81E-01
-1.96E-02
-7.20E-05
-3.56E+02
ecnanetniaM
B3 B5 B6 C1
X
B2
1.11E-03
2.40E-02 6.34E-02 0.00E+00 5.73E-01
x
x 0.00E+00 1.24E-03
1.85E+02 0.00E+00
gnissecorp
etsaW
lasopsiD
C4 D
tnemecalpeR
B7 C2
X X X X X X X
riapeR
kg C H -ekv
2 4
kg Sb-ekv 2.26E-05
1.44E+03 1.55E+02
Unit
0.00E+00
kg C H -ekv 0.00E+00 0.00E+00 0.00E+00
2 4
GWP Global warming potential; ODP Depletion potential of the stratospheric ozone layer; POCP Formation potential of tropospheric
photochemical oxidants; AP Acidification potential of land and water; EP Eutrophication potential; ADPM Abiotic depletion potential for non fossil
resources; ADPE Abiotic depletion potential for fossil resources.
tropsnarT tropsnarT
esU
4.55E+00
noitallatsni
noitcurtsnoC
egats
A2
ODP
x
POCP
gnirutcafunaM
Construction
Product stage and installation
stage
A4 A5 B1
X X X X X X X
Parameter Unit A1-A3 A4 A5
GWP kg CO -ekv 8.51E+01 9.09E+00
2
kg CFC11-ekv 5.00E-06 1.77E-06 x
POCP 1.65E-01
ADPE
esu
ygrene
lanoitarepO
esu
retaw
lanoitarepO
noitcurtsnoc-eD
noitilomed tropsnarT
-yrevoceR-esueR laitnetop
gnilcyceR
Global warming potential in A1-A3 includes sequestration of CO2 as carbon in the wood. This amount is accounted as an emission
in module C3. Additionally, it is included sequestration in the wood packaging. This is accounted as an emission in module A5. The
flow of biogenic carbon for the system is presented in page 9.
Use stage
B2 C3
tnemhsibrufeR
A1
slairetam
waR
End of Life stage
A3
AP kg SO -ekv 5.41E-01 x 0.00E+00 0.00E+00
2
EP kg PO 3--ekv 7.23E-02 3.36E-03 0.00E+00 6.54E-03 0.00E+00 7.76E-02 0.00E+00
4
ADPM 1.21E-03 1.10E-04 0.00E+00
MJ 0.00E+00 1.69E+03
Parameter B6 B7 C1 C3 C4 D
GWP kg CO -ekv 0.00E+00 0.00E+00 4.16E-01 3.40E+01 5.17E-01
2
ODP kg CFC11-ekv 0.00E+00 0.00E+00 0.00E+00 7.62E-08 3.99E-08 1.37E-07
-1.50E-02
AP kg SO -ekv 0.00E+00 0.00E+00 0.00E+00 1.32E-03 3.75E-03 2.89E-03
2
EP kg PO 3--ekv 0.00E+00 0.00E+00 0.00E+00 2.17E-04 1.19E-03 5.36E-04
4
ADPM kg Sb-ekv 0.00E+00 0.00E+00 0.00E+00 1.41E-06 1.16E-06 1.09E-06
ADPE MJ 0.00E+00 0.00E+00 0.00E+00 6.69E+00 7.77E+01 1.32E+01
NEPD-3456-2057-EN NTech outward opening topswing windows 105/80 – TG & TY (without aluminium cladding)
6/9
Resource use without alu clad
Parameter Unit A1-A3 A4 A5 B1 B2 B3 B4 B5
RPEE MJ 4.09E+02 1.8E+00 x 0.00E+00 1.86E+01 0.00E+00 6.88E+02 0.00E+00
RPEM MJ 3.30E+02 x x 0.00E+00 x 0.00E+00 5.36E+01 0.00E+00
TPE MJ 7.39E+02 1.8E+00 x 0.00E+00 1.86E+01 0.00E+00 7.42E+02 0.00E+00
NRPE MJ 1.57E+03 1.6E+02 x 0.00E+00 2.01E+02 0.00E+00 1.83E+03 0.00E+00
NRPM MJ 1.02E+02 x x 0.00E+00 7.30E+00 0.00E+00 2.87E+01 0.00E+00
TRPE MJ 1.68E+03 1.6E+02 x 0.00E+00 2.09E+02 0.00E+00 1.86E+03 0.00E+00
SM kg 4.21E-01 x x 0.00E+00 x 0.00E+00 4.21E-01 0.00E+00
RSF MJ 9.22E-02 x x 0.00E+00 6.03E-03 0.00E+00 5.00E-01 0.00E+00
NRSF MJ 1.37E-01 x x 0.00E+00 4.02E-03 0.00E+00 4.02E-01 0.00E+00
W m3 1.68E+00 1.7E-02 x 0.00E+00 2.88E-01 0.00E+00 1.72E+00 0.00E+00
Resource use without alu clad
Parameter Unit B6 B7 C1 C2 C3 C4 D
RPEE MJ 0.0E+00 0.0E+00 0.0E+00 8.6E-02 2.8E+02 1.9E-01 -2.7E+02
RPEM MJ 0.0E+00 0.0E+00 0.0E+00 x -2.8E+02 x x
TPE MJ 0.0E+00 0.0E+00 0.0E+00 8.6E-02 6.3E-01 1.9E-01 -2.7E+02
NRPE MJ 0.0E+00 0.0E+00 0.0E+00 6.8E+00 7.8E+01 1.4E+01 -3.6E+02
NRPM MJ 0.0E+00 0.0E+00 0.0E+00 x -7.3E+01 x x
TRPE MJ 0.0E+00 0.0E+00 0.0E+00 6.8E+00 4.5E+00 1.4E+01 -3.6E+02
SM kg 0.0E+00 0.0E+00 0.0E+00 x x x x
RSF MJ 0.0E+00 0.0E+00 0.0E+00 x 4.1E-01 x -1.8E+02
NRSF MJ 0.0E+00 0.0E+00 0.0E+00 x 2.6E-01 x -1.2E+02
W m3 0.0E+00 0.0E+00 0.0E+00 6.8E-04 1.3E-02 1.2E-02 -8.6E-01
RPEE Renewable primary energy resources used as energy carrier; RPEM Renewable primary energy resources used as raw materials; TPE
Total use of renewable primary energy resources; NRPE Non renewable primary energy resources used as energy carrier; NRPM Non
renewable primary energy resources used as materials; TRPE Total use of non renewable primary energy resources; SM Use of secondary
materials; RSF Use of renewable secondary fuels; NRSF Use of non renewable secondary fuels; W Use of net fresh water
End of life-Waste without alu clad
Parameter Unit A1-A3 A4 A5 B1 B2 B3 B4 B5
HW kg 3.01E+00 8.02E-03 0.00E+00 0.00E+00 3.41E-02 0.00E+00 5.24E+01 0.00E+00
NHW kg 2.68E+01 1.26E+01 0.00E+00 0.00E+00 2.54E+00 0.00E+00 4.03E+01 0.00E+00
RW kg 2.00E-02 1.02E-03 0.00E+00 0.00E+00 3.95E-04 0.00E+00 2.12E-02 0.00E+00
End of life-Waste without alu clad
Parameter Unit B6 B7 C1 C2 C3 C4 D
HW kg 0.00E+00 0.00E+00 0.00E+00 3.35E-04 5.59E-03 4.94E+01 -2.55E-01
NHW kg 0.00E+00 0.00E+00 0.00E+00 4.13E-01 1.50E-01 3.92E-01 -6.11E+00
RW kg 0.00E+00 0.00E+00 0.00E+00 4.39E-05 1.45E-05 7.87E-05 -5.12E-04
HW Hazardous waste disposed; NHW Non hazardous waste disposed; RW Radioactive waste disposed
End of life- Output flow without alu clad
Parameter Unit A1-A3 A4 A5 B1 B2 B3 B4 B5
CR kg x x x 0.00E+00 x 0.00E+00 x 0.00E+00
MR kg 7.00E-01 x 1.30E-01 0.00E+00 x 0.00E+00 3.47E+00 0.00E+00
MER kg 7.10E-02 x 3.10E+00 0.00E+00 x 0.00E+00 3.17E+00 0.00E+00
EEE MJ 7.51E+00 x x 0.00E+00 x 0.00E+00 3.74E+01 0.00E+00
ETE MJ 8.30E+01 x x 0.00E+00 x 0.00E+00 2.90E+02 0.00E+00
End of life- Output flow without alu clad
Parameter Unit B6 B7 C1 C2 C3 C4 D
CR kg 0.00E+00 0.00E+00 0.00E+00 x x x x
MR kg 0.00E+00 0.00E+00 0.00E+00 x 2.64E+00 x -5.36E+00
MER kg 0.00E+00 0.00E+00 0.00E+00 x x x x
EEE MJ 0.00E+00 0.00E+00 0.00E+00 x 2.99E+01 x -4.48E+01
ETE MJ 0.00E+00 0.00E+00 0.00E+00 x 2.07E+02 x -4.45E+02
CR Components for reuse; MR Materials for recycling; MER Materials for energy recovery; EEE Exported electric energy; ETE Exported thermal
energy
Reading example: 9,0 E-03 = 9,0*10-3 = 0,009
NEPD-3456-2057-EN NTech outward opening topswing windows 105/80 – TG & TY (without aluminium cladding)
7/9
Norwegian additional requirements
Greenhouse gas emissions from the use of electricity in the production phase
National (Poland) market with low-voltage, including production of transmission lines and grid losses, has been used for electricity in
the production process (A3).
Data source Quantity Unit
Ecoinvent v3.7 (september 2020) 1030 gram CO -ekv./kWh
2
Hazardous substances
The product contains no substances from REACH Candidate List or the Norwegian Priority List
The product contains substances below 0.1% by weight on the REACH Candidate List
The product contains substances from REACH Candidate List or the Norwegian Priority List, see table under Specific
Norwegian requirements.
The product does not contain any substances on the REACH Candidate List or the Norwegian Priority List. The product can be
characterized as hazardous waste (according to the Waste Shift, Appendix III), see table under Specific Norwegian
requirements.
Transport
Transport from production site to construction site according to scenario in A4: 1500+50 km
Indoor air quality
The product has not been tested for emissions to indoor environments.
Carbon footprint
To increase the transparency of the climate impacts, the GWP indicator has been divided into sub-indicators:
GWP-IOBC Climate impacts calculated according to instant oxidation principle
GWP-BCIP Climate impacts calculated from the net impacts of sequestration and emission of biogenic carbon
Climate impact without alu clad
Parameter Unit A1-A3 A4 A5 B1 B2 B3 B4 B5
GWP-IOBC kg CO -ekv 1.16E+02 9.09E+00 x 0.00E+00 9.52E+00 0.00E+00 1.34E+02 0.00E+00
2
GWP-BCIP kg CO -ekv -3.10E+01 x 4.55E+00 0.00E+00 x 0.00E+00 2.93E-04 0.00E+00
2
GWP kg CO -ekv 8.51E+01 9.09E+00 4.55E+00 0.00E+00 9.52E+00 0.00E+00 1.34E+02 0.00E+00
2
Climate impact without alu clad
Parameter Unit B6 B7 C1 C2 C3 C4 D
GWP-IOBC kg CO -ekv 0.00E+00 0.00E+00 0.00E+00 4.16E-01 7.56E+00 5.17E-01 -3.41E+01
2
GWP-BCIP kg CO -ekv 0.00E+00 0.00E+00 0.00E+00 x 2.64E+01 x x
2
GWP kg CO -ekv 0.00E+00 0.00E+00 0.00E+00 4.16E-01 3.40E+01 5.17E-01 -3.41E+01
2
Additional information
For the products with different sizes from the declared unit, the environmental impacts must be converted by using a conversion
factor. The Norwegian EPD Foundation has published instructions on how to interpret EPDs for windows on its website (www.epd-
norge.no) where different calculation methods have been stated. (Document: Bruksanvisninger i hvordan tolke EPD'er – Vinduer)
NEPD-3456-2057-EN NTech outward opening topswing windows 105/80 – TG & TY (without aluminium cladding)
8/9
Bibliografi
NS-EN ISO 14025:2010 Miljømerker og deklarasjoner - Miljødeklarasjoner type III - Prinsipper og prosedyrer.
NS-EN ISO 14044:2006 Miljøstyring - Livsløpsvurderinger - Krav og retningslinjer
NS-EN 15804:2012+A1:2013 Bærekraftig byggverk - Miljødeklarasjoner - Grunnleggende produktkategoriregler for
byggevarer
ISO 21930:2007 Sustainability in building construction - Environmental declaration of building products
Modaresi, R. 2020 LCA-report for Nordan LCA-report nr. 325039-1 from Norwegian Institute of Wood
Technology, Oslo, Norway.
NPCR014 (04/2019) Product category rules for windows and doors, rev3, April 2019
NS-EN 16485:2014 Tømmer og skurlast - Miljødeklarasjoner - Produktkategoriregler for tre og trebaserte
produkter til bruk i byggverk
NS-EN 16449:2014 Tre og trebaserte produkter - Beregning av biogent karboninnhold i tre og omdanning til
karbondioksid
Ecoinvent v3.0-3.7 Ecoinvent database version 3.0-3.7 Centre for Life Cycle Inventories.
Statistisk sentralbyrå Tabell 04727: Fjernvarmebalansen, 2015
Statistisk sentralbyrå Tabell 09469: Nettoproduksjon av fjernvarme, 2015
NEPD-307-179-NO EPD for skurlast av gran eller furu. Treindustrien
Bruksanvisninger i hvordan tolke EPD'er – Vinduer. https://www.epd-norge.no [in Norwegian]
Program operator and publisher Tlf: +47 23 08 80 00
The Norwegian EPD Foundation
Postboks 5250 Majorstuen, 0303 Oslo e-post: post@epd-norge.no
Norway web www.epd-norge.no
Owner of the declaration Tlf: +47 51 40 40 00
NorDan AS
Stasjonsveien 46, N-4460 Moi e-post: firmapost@nordan.no
Norway
web www.nordan.no
Author of the Life Cycle Assessment Tlf: +47 98 85 33 33
Roja Modaresi
Norsk Treteknisk Instiutt e-post: firmapost@treteknisk.no
Postboks 113 Blindern, 0314 Oslo, Norway web www.treteknisk.no
NEPD-3456-2057-EN NTech outward opening topswing windows 105/80 – TG & TY (without aluminium cladding)
9/9
EPD for the best
environmental
decision
www.epd-norge.no
The Norwegian EPD foundation
EPD for the best environmental decision
12
