Environmental product declaration
in accordance with ISO 14025 and EN 15804+A2
Nordanger LVTgulv Standard
Owner of the declaration: Program operator:
Nordanger Gulv AS The Norwegian EPD Foundation
Product: Declaration number:
Nordanger LVTgulv Standard
NEPD-8635-8303-EN
Declared unit:
1 m2 Registration number:
This declaration is based on Product Category Rules: NEPD-8635-8303-EN
CEN Standard EN 15804:2012+A2:2019 serves as core
Issue date: 03.01.2025
PCR
The Norwegian EPD Foundation IBU PCR Part B: Requirements on the EPD for Floor Valid to: 03.01.2030
coverings
EPD software:
LCAno EPD generator ID: 693711
1 / 12
General information
Product Owner of the declaration:
Nordanger LVTgulv Standard Nordanger Gulv AS
Contact person: Morten Aune
Phone: +47 22731000
e-mail: gulv@nordanger.no
Program operator: Manufacturer:
The Norwegian EPD Foundation Nordanger Gulv AS
Post Box 5250 Majorstuen, 0303 Oslo, Norway Professor Birkelands vei 36
Phone: +47 977 22 020 1082 Oslo, Norway
web: www.epd-norge.no
Declaration number: Place of production:
Nordanger Gulv
NEPD-8635-8303-EN Produksjonsstedet
Jiangsu, China
This declaration is based on Product Category Rules: Management system:
CEN Standard EN 15804:2012+A2:2019 serves as core PCR -
IBU PCR Part B: Requirements on the EPD for Floor coverings
Statement of liability: Organisation no:
The owner of the declaration shall be liable for the underlying 979448759
information and evidence. EPD Norway shall not be liable with respect
to manufacturer information, life cycle assessment data and
evidences.​
Declared unit: Issue date:
1 m2 Nordanger LVTgulv Standard
03.01.2025
Declared unit with option: Valid to:
A1-A3,A4,A5,C1,C2,C3,C4,D 03.01.2030
Year of study:
2023
Functional unit: Comparability:
Not applicable. EPD of construction products may not be comparable if they do not
comply with EN 15804 and seen in a building context.
General information on verification of EPD from EPD tools: Development and verification of EPD:
Independent verification of data, other environmental information The declaration is created using EPD tool lca.tools ver EPD2022.03,
and the declaration according to ISO 14025:2010, § 8.1.3 and § 8.1.4. developed by LCA.no. The EPD tool is integrated in the company's
Verification of each EPD is made according to EPD-Norway’s management system, and has been approved by EPD Norway.
guidelines for verification and approval requiring that tools are i)
integrated into the company's environmental management system, ii) Developer of EPD: Pedro Ferreira
the procedures for use of the EPD tool are approved by EPD-Norway,
Reviewer of company-specific input data and EPD:​ Børge Heggen
and iii) the process is reviewed annually by an independent third
Johansen, Energiråd AS
party verifier. See Appendix G of EPD-Norway's General Programme
Instructions for further information on EPD tools
Verification of EPD tool: Approved:
Independent third party verification of the EPD tool, background data
and test-EPD in accordance with EPDNorway's procedures and
guidelines for verification and approval of EPD tools.
Third party verifier:
Alexander Borg, Asplan Viak AS
(no signature required)
2 / 12
Product
Product description:
Nordanger LVTgulv Standard is available in many beautiful designs. Its wear resistance and durability make it very suitable for commercial use such
as shops, offices, restaurants, hotels, nursing homes, rental apartments, etc.
Nordanger Gulv AS introduced LVT (Luxury Vinyl Tiles) to the Norwegian market in 1978, and has since worked hard to offer products that can
withstand high loads and at the same time have an aesthetically pleasing appearance. Over the years, we have supplied floors to over 10,000
premises in public environments, such as shops, offices, restaurants and hotels. Our floors are developed to withstand high traffic and high wear
while being functional and having a modern design. Nordanger LVT floors are supplied in more than 50 different varieties adapted to the different
areas of use.
• All activity in Nordanger Gulv AS has focus on environmental perspectives. Our work environment shall be clean end safe, and all employees
must consider environmental consequences throughout their workdays.
• Nordanger Gulv AS assures that all production of flooring apply current environmental legislation, both in the short and the long term. The
production must not harm the natural environment, nor threaten people’s health, safety or working environment.
• Nordanger Gulv AS informs our customers about our products’ environmental qualifications, and can present relevant certifications.
• Our products meet the requirements for achieving BREEAM NOR approval.
Product specification:
Materials kg %
Limestone 2,64 61,37
Plastic - Polyvinyl chloride (PVC) 1,18 27,35
Chemicals 0,49 11,28
Total 4,31 100,00
Packaging kg %
Packaging - Recycled cardboard 0,09 100,00
Total incl. packaging 4,40 100,00
Technical data:
Technical information Method Result
Type of flooring EN ISO 16511 Heterogeneous vinyl
Classification of living environment EN ISO 10874 23
Classification public environment EN ISO 10874 33
Size of rods (wood patterns) EN 427 152,4 914,4 mm; 184,15 x 1219,2 mm; 228.6x1219.2 mm
Tile size (stone/concrete patterns) EN 427 304,8 x 457,2 mm; 457,2 x 457,2 mm; 457.2 x 609.6 mm; 609,6 x 609,6 mm
Total thickness EN ISO24337 2.5 mm
Thickness of wear layer EN ISO24340 0.55 mm
Total weight EN ISO23997 4.3057 kg/m2
Surface treatment - PUR/UV
Fire classification EN 13501-1 Bfl-s1
TVOC emissions EN 16516 Approved
Market:
Norway.
Reference service life, product
Not applicable.
Reference service life, building or construction works
Not applicable.
LCA: Calculation rules
Declared unit:
1 m2 Nordanger LVTgulv Standard
Cut-off criteria:
All major raw materials and all the essential energy is included. The production processes for raw materials and energy flows with very small
amounts (less than 1%) are not included. These cut-off criteria do not​ apply for hazardous materials and substances.
Allocation:
The allocation is made in accordance with the provisions of EN 15804. Incoming energy and water and waste production in-house is allocated
equally among all products through mass allocation. Effects of primary production of recycled materials is allocated to the main product in which
the material was used. The recycling process and transportation of the material is allocated to this analysis.
Data quality:
3 / 12
Specific data for the product composition are provided by the manufacturer. The data represent the production of the declared product and were
collected for EPD development in the year of study. Background data is based on EPDs according to EN 15804 and different LCA databases. The
data quality of the raw materials in A1 is presented in the table below.
Materials Source Data quality Year
Chemicals ecoinvent 3.10 Database 2023
Chemicals ecoinvent 3.6 Database 2019
Limestone ecoinvent 3.6 Database 2019
Packaging - Recycled cardboard Modified ecoinvent 3.6 Database 2019
Plastic - Polyvinyl chloride (PVC) ecoinvent 3.6 Database 2019
4 / 12
System boundaries (X=included, MND=module not declared, MNR=module not relevant)
Construction Beyond the system
Product stage Use stage End of life stage
installation stage boundaries
A1 A2 A3 A4 A5 B1 B2 B3 B4 B5 B6 B7 C1 C2 C3 C4 D
X X X X X MND MND MND MND MND MND MND X X X X X
System boundary:
The product phases include the extraction and production of raw materials and packaging materials (module A1), the transport to the production
plant (module A2) and the production of LVT flooring in China (module A3).
Distribution, assembly phase and waste management for the product are included based on the Norwegian market.
Additional technical information:
Not applicable.
waR slairetam tropsnarT gnirutcafunaM tropsnarT ylbmessA e​sU ecnanetniaM riapeR tnemecalpeR tnemhsibrufeR lanoitarepO ygrene esu lanoitarepO esu retaw -eD noitcurtsnoc noitilomed tropsnarT etsaW gnissecorp lasopsiD -yrevoceR-esueR laitnetop-gnilcyceR
5 / 12
LCA: Scenarios and additional technical information
The following information describe the scenarios in the different modules of the EPD.
A4: The LVT flooring is transported from China to Norway by a combination of truck and ship. A standard distance of 150 km is assumed for
national distribution.
Modules C and D include the most likely final treatment scenario for mixed construction waste, based on Statistics Norway 2023. It is assumed
that 88% of the LVT flooring goes to energy recovery, and 12% to landfill.
Capacity utilisation Value
Transport from production place to user (A4) Distance (km) Fuel/Energy Consumption Unit
(incl. return) % (Liter/tonne)
Ship, Freight, Transoceanic (km) 65,0 % 20509 0,003 l/tkm 61,53
Truck, 16-32 tons, EURO 6 (km) 36,7 % 183 0,043 l/tkm 7,87
Assembly (A5) Unit Value
Waste, packaging, corrugated board box, 100 %
kg 0,090
recycled, to average treatment (kg)
Capacity utilisation Value
Transport to waste processing (C2) Distance (km) Fuel/Energy Consumption Unit
(incl. return) % (Liter/tonne)
Truck, 16-32 tons, EURO 6 (km) 36,7 % 85 0,043 l/tkm 3,66
Waste processing (C3) Unit Value
Waste treatment per kg Plastic, Mixture,
kg 3,78
municipal incineration with fly ash extraction (kg)
Disposal (C4) Unit Value
Waste, plastic, mixture, to landfill (kg) kg 0,51
Landfilling of ashes from incineration of Plastics,
kg 0,13
Mixture (kg)
Benefits and loads beyond the system
Unit Value
boundaries (D)
Substitution of thermal energy, district heating, in
MJ 175,82
Norway (MJ)
Substitution of electricity, in Norway (MJ) MJ 11,62
Substitution of thermal energy, district heating, in
MJ 0,078
Norway (MJ)
Substitution of electricity, in Norway (MJ) MJ 0,0052
6 / 12
LCA: Results
The LCA results are presented below for the declared unit defined on page 2 of the EPD document.
Environmental impact
Indicator Unit A1-A3 A4 A5 C1 C2 C3 C4 D
GWP-total kg CO2 -eq 1,01E+01 9,81E-01 1,56E-01 0,00E+00 6,11E-02 8,97E+00 5,94E-02 -1,06E+00
GWP-fossil kg CO2 -eq 1,03E+01 9,81E-01 1,47E-03 0,00E+00 6,10E-02 8,97E+00 5,94E-02 -1,02E+00
GWP-biogenic kg CO2 -eq -1,37E-01 2,88E-04 1,54E-01 0,00E+00 2,53E-05 1,95E-04 5,45E-06 -2,11E-03
GWP-luluc kg CO2 -eq 4,88E-03 6,34E-04 4,87E-07 0,00E+00 2,17E-05 3,64E-05 1,20E-06 -3,51E-02
ODP kg CFC11 -eq 4,82E-06 2,10E-07 3,11E-10 0,00E+00 1,38E-08 1,95E-08 1,65E-09 -7,43E-02
AP mol H+ -eq 4,91E-02 2,80E-02 6,97E-06 0,00E+00 1,75E-04 1,97E-03 4,12E-05 -8,40E-03
EP-FreshWater kg P -eq 7,24E-04 4,57E-06 1,21E-08 0,00E+00 4,88E-07 1,73E-06 5,81E-08 -9,06E-05
EP-Marine kg N -eq 9,82E-03 6,86E-03 2,30E-06 0,00E+00 3,47E-05 9,40E-04 7,61E-05 -2,75E-03
EP-Terrestial mol N -eq 1,07E-01 7,63E-02 2,50E-05 0,00E+00 3,88E-04 9,64E-03 1,63E-04 -2,97E-02
POCP kg NMVOC -eq 3,51E-02 1,99E-02 7,17E-06 0,00E+00 1,49E-04 2,32E-03 5,90E-05 -8,19E-03
ADP-minerals&metals1 kg Sb-eq 9,84E-05 9,95E-06 3,58E-08 0,00E+00 1,69E-06 9,81E-07 4,08E-08 -1,01E-05
ADP-fossil1 MJ 1,54E+02 1,28E+01 2,06E-02 0,00E+00 9,23E-01 1,23E+00 1,22E-01 -1,46E+01
WDP1 m3 6,63E+01 4,09E+00 2,61E-02 0,00E+00 8,93E-01 8,90E+00 1,04E+00 -1,82E+02
GWP-total = Global Warming Potential total; GWP-fossil = Global Warming Potential fossil fuels; GWP-biogenic = Global Warming Potential biogenic; GWP-luluc =
Global Warming Potential land use and land use change; ODP = Depletion potential of the stratospheric ozone layer; AP = Acidification potential, Accumulated
Exceedance; EP-freshwater = Eutrophication potential, fraction of nutrients reaching freshwater end compartment: EP-marine = Eutrophication potential, fraction of
nutrients reaching marine end compartment; EP-terrestrial = Eutrophication potential, Accumulated Exceedance; POCP = Formation potential of tropospheric ozone;
ADP-minerals&metals = Abiotic depletion potential for non-fossil resources; ADP-fossil = Abiotic depletion for fossil resources potential; WDP = Water (user)
deprivation potential, deprivation-weighted water consumption
"Reading example: 9,0 E-03 = 9,0*10-3 = 0,009"
*INA Indicator Not Assessed
1. The results of this environmental impact indicator shall be used with care as the uncertainties on these results are high or as there is limited experienced with the
indicator
Remarks to environmental impacts
Not applicable.
7 / 12
Additional environmental impact indicators
Indicator Unit A1-A3 A4 A5 C1 C2 C3 C4 D
PM Disease incidence 5,63E-07 8,05E-09 1,03E-10 0,00E+00 3,74E-09 8,61E-09 8,22E-10 -5,09E-07
IRP2 kgBq U235 -eq 2,54E-01 5,52E-02 8,81E-05 0,00E+00 4,03E-03 3,10E-03 5,88E-04 -9,32E-02
ETP-fw1 CTUe 2,25E+02 7,79E+00 2,75E-02 0,00E+00 6,84E-01 1,90E+01 1,49E-01 -7,93E+01
HTP-c1 CTUh 7,91E-09 0,00E+00 1,00E-12 0,00E+00 0,00E+00 5,19E-10 3,00E-12 -1,45E-09
HTP-nc1 CTUh 1,17E-07 1,61E-09 3,40E-11 0,00E+00 7,47E-10 2,37E-08 1,03E-10 -7,60E-08
SQP1 dimensionless 2,54E+01 2,84E+00 1,38E-02 0,00E+00 6,46E-01 2,25E-01 4,58E-01 -9,75E+01
PM = Particulate Matter emissions; IRP = Ionizing radiation – human health; ETP-fw = Eco toxicity – freshwater; HTP-c = Human toxicity – cancer effects; HTP-nc =
Human toxicity – non cancer effects; SQP = Potential Soil Quality Index (dimensionless)
"Reading example: 9,0 E-03 = 9,0*10-3 = 0,009"
*INA Indicator Not Assessed
1. The results of this environmental impact indicator shall be used with care as the uncertainties on these results are high or as there is limited experienced with the
indicator
2. This impact category deals mainly with the eventual impact of low dose ionizing radiation on human health of the nuclear fuel cycle. It does not consider effects due
to possible nuclear accidents, occupational exposure nor due to radioactive waste disposal in underground facilities. Potential ionizing radiation from the soil, from
radon and from some construction materials is also not measured by this indicator.
8 / 12
Resource use
Indicator Unit A1-A3 A4 A5 C1 C2 C3 C4 D
PERE MJ 9,61E+00 1,02E-01 3,39E-04 0,00E+00 1,32E-02 6,86E-02 5,69E-03 -9,01E+01
PERM MJ 5,32E-01 0,00E+00 -5,32E-01 0,00E+00 0,00E+00 0,00E+00 0,00E+00 0,00E+00
PERT MJ 1,01E+01 1,02E-01 3,39E-04 0,00E+00 1,32E-02 6,86E-02 5,69E-03 -9,01E+01
PENRE MJ 1,29E+02 1,28E+01 2,06E-02 0,00E+00 9,23E-01 1,23E+00 1,22E-01 -1,46E+01
PENRM MJ 2,53E+01 0,00E+00 0,00E+00 0,00E+00 0,00E+00 -2,52E+01 0,00E+00 0,00E+00
PENRT MJ 1,54E+02 1,28E+01 2,06E-02 0,00E+00 9,23E-01 -2,40E+01 1,22E-01 -1,46E+01
SM kg 1,23E-01 0,00E+00 0,00E+00 0,00E+00 0,00E+00 0,00E+00 0,00E+00 0,00E+00
RSF MJ 6,51E-02 2,81E-03 1,12E-05 0,00E+00 4,73E-04 1,47E-03 1,19E-04 -1,58E-02
NRSF MJ 3,55E-02 2,84E-02 4,63E-05 0,00E+00 1,69E-03 0,00E+00 6,61E-04 -5,34E+00
FW m3 7,35E-02 7,77E-04 9,71E-06 0,00E+00 9,87E-05 1,04E-02 1,51E-04 -1,08E-01
PERE = Use of renewable primary energy excluding renewable primary energy resources used as raw materials; PERM = Use of renewable primary energy resources used
as raw materials; PERT = Total use of renewable primary energy resources; PENRE = Use of non renewable primary energy excluding non-renewable primary energy
resources used as raw materials; PENRM = Use of non renewable primary energy resources used as raw materials; PENRT = Total use of non renewable primary energy
resources; SM = Use of secondary materials; RSF = Use of renewable secondary fuels; NRSF = Use of non-renewable secondary fuels; FW = Net use of fresh water
"Reading example: 9,0 E-03 = 9,0*10-3 = 0,009"
*INA Indicator Not Assessed
9 / 12
End of life - Waste
Indicator Unit A1-A3 A4 A5 C1 C2 C3 C4 D
HWD kg 1,38E-01 5,64E-04 0,00E+00 0,00E+00 4,76E-05 0,00E+00 3,53E-03 -6,85E-04
NHWD kg 3,97E+00 1,22E-01 9,10E-02 0,00E+00 4,49E-02 0,00E+00 5,21E-01 -3,45E-01
RWD kg 3,18E+00 8,90E-05 0,00E+00 0,00E+00 6,29E-06 0,00E+00 8,00E-07 -7,63E-05
HWD = Hazardous waste disposed; NHWD = Non-hazardous waste disposed; RWD = Radioactive waste disposed
"Reading example: 9,0 E-03 = 9,0*10-3 = 0,009"
*INA Indicator Not Assessed
End of life - Output flow
Indicator Unit A1-A3 A4 A5 C1 C2 C3 C4 D
CRU kg 0,00E+00 0,00E+00 0,00E+00 0,00E+00 0,00E+00 0,00E+00 0,00E+00 0,00E+00
MFR kg 3,53E-04 0,00E+00 8,46E-02 0,00E+00 0,00E+00 0,00E+00 4,63E-05 0,00E+00
MER kg 4,08E-04 0,00E+00 6,36E-03 0,00E+00 0,00E+00 3,79E+00 1,13E-06 0,00E+00
EEE MJ 5,00E-07 0,00E+00 5,20E-03 0,00E+00 0,00E+00 5,82E+00 7,35E-05 0,00E+00
EET MJ 7,56E-06 0,00E+00 7,87E-02 0,00E+00 0,00E+00 8,81E+01 1,11E-03 0,00E+00
CRU = Components for re-use; MFR = Materials for recycling; MER = Materials for energy recovery; EEE = Exported energy electrical; EET = Exported energy thermal
"Reading example: 9,0 E-03 = 9,0*10-3 = 0,009"
*INA Indicator Not Assessed
Biogenic Carbon Content
Indicator Unit At the factory gate
Biogenic carbon content in product kg C 0,00E+00
Biogenic carbon content in accompanying packaging kg C 4,21E-02
Note: 1 kg biogenic carbon is equivalent to 44/12 kg CO2
10 / 12
Additional requirements
Greenhouse gas emissions from the use of electricity in the manufacturing phase
National production mix from import, low voltage (production of transmission lines, in addition to direct emissions and losses in grid) of applied
electricity for the manufacturing process (A3).
Electricity mix Source Amount Unit
Electricity, China (kWh) ecoinvent 3.6 1102,91 g CO2-eq/kWh
Dangerous substances
The product contains no substances given by the REACH Candidate list.
Indoor environment
Not applicable.
Additional Environmental Information
Additional environmental impact indicators required in NPCR Part A for construction products
Indicator Unit A1-A3 A4 A5 C1 C2 C3 C4 D
GWPIOBC kg CO2 -eq 1,01E+01 9,81E-01 1,47E-03 0,00E+00 6,11E-02 8,97E+00 7,02E-02 -1,04E+00
GWP-IOBC: Global warming potential calculated according to the principle of instantaneous oxidation. In order to increase the transparency of biogenic carbon​
contribution to climate impact, the indicator GWP-IOBC is required as it declares climate impacts calculated according to the principle of instantaneous oxidation.​
GWP-IOBC is also referred to as GWP-GHG in context to Swedish public procurement legislation.
11 / 12
Bibliography
ISO 14025:2010 Environmental labels and declarations - Type III environmental declarations - Principles and procedures.
ISO 14044:2006 Environmental management - Life cycle assessment - Requirements and guidelines.
EN 15804:2012+A2:2019 Environmental product declaration - Core rules for the product category of construction products.
ecoinvent v3, Allocation, cut-off by classification, Swiss Centre of Life Cycle Inventories.
Iversen et al., (2021) eEPD v2021.09 Background information for EPD generator tool system verification, LCA.no Report number: 07.21
Ferreira and Graafland., (2024) EPD generator for PCR IBU: Part B,
Requirements on the EPD for Floor coverings Background information for EPD generator application and LCA data, LCA.no report number: 16.24.
NPCR Part A: Construction products and services. Ver. 2.0. April 2021, EPD-Norge.
IBU 2023 Part B: Requirements on the EPD for Floor coverings, 2024, IBU – Institut Bauen und Umwelt e.V, version 11
NS-EN 13329:2016+A2:2021 Laminate floor coverings - Elements with a surface layer based on aminoplastic thermosetting resins - Specifications,
requirements and test methods
Program operator and publisher Phone: +47 977 22 020
The Norwegian EPD Foundation e-mail: post@epd-norge.no
Post Box 5250 Majorstuen, 0303 Oslo, Norway web: www.epd-norge.no
Owner of the declaration: Phone:
+47 22731000
Nordanger Gulv AS e-mail:
gulv@nordanger.no
Professor Birkelands vei 36, 1082 Oslo, Norway web:
Author of the Life Cycle Assessment Phone: +47 916 50 916
LCA.no AS e-mail: post@lca.no
Dokka 6A, 1671 Kråkerøy, Norway web: www.lca.no
Developer of EPD generator Phone: +47 916 50 916
LCA.no AS e-mail: post@lca.no
Dokka 6A, 1671 Kråkerøy, Norway web: www.lca.no
ECO Platform web: www.eco-platform.org
ECO Portal web: ECO Portal
12 / 12
