Environmental Product
Declaration
In accordance with ISO 14025 and EN 15804 +A2
Owner of the declaration: Product name
Lindab Ventilation AB
Carat, passive radiant chilled
Stålhögavägen 115, 269 92 Båstad
beam
Sweden
Program holder and publisher: Manufacturer
The Norwegian EPD foundation Lindab Ventilation AB
Declaration number:
NEPD-3535-2124-EN
Registration Number:
NEPD-3535-2124-EN
Issue date:
The Norwegian Valid to:
EPD Foundation 01.06.2022
01.06.2027
General information
Product: Owner of the declaration:
Carat Lindab Ventilation AB
Contact person: Matilda Isaksson
Program Operator: Phone: +46 431 850 12
e-mail: matilda.isaksson@lindab.com
The Norwegian EPD Foundation
Manufacturer:
Post Box 5250 Majorstuen, 0303 Oslo, Norway
Tlf: +47 23 08 80 00 Lindab Ventilation AB
e-mail: post@epd-norge.no Stålhögavägen 115, 269 92 Båstad, Sweden
Phone: +46 431 850 00
e-mail: lindab@lindab.com
Declaration Number:
Place of production:
NEPD-3535-2124-EN Grevie, Sweden
This declaration is based on Product
Category Rules:
Management system:
CEN Standard EN15804:2012+A2:2019 serves as
ISO 9001, ISO 14001
core PCR
PART A: Construction products and services Ver 2
Organisation no:
PART B: PCR NPCR 030 SE556026158701
Statements: Issue date:
The owner of the declaration shall be liable for the
underlying information and evidence. EPD
01.06.2022
Norway shall not be liable with respect to Valid to:
manufacturer, life cycle assessment data and
evidences.
01.06.2027
Year of study:
Declared unit:
2022
1 piece of Carat-31 product with a length of 1.2 m.
Comparability:
The EPD is a specific EPD for this product, and EPDs from other programmes than The
from the EPD results all other Carat products in Norwegian EPD Foundation may not be
several different lengths and sizes can be derived. comparable.
Declared unit with option: The EPD has been worked out by:
Included modules: A1-A4, C1-C4, D Anna Liljenroth and Lisa Hallberg, IVL Swedish
Environmental Research Insitute
Functional unit
Verification:
Independent verification of the declaration and
data, according to ISO14025:2010
internal Approved (Manager of EPD Norway
Charlotte Merlin, Senior project leader,
FORCE Technology
Independent verifier approved by EPD Norway
EPD for the best environmental decision 2
Product
Product description:
Carat is placed above a perforated suspended ceiling and supplies cooling, with a low air
velocity, to the room below.
Carat has a high radiation quotient of approx. 35% (compared to approx. 5% for traditional
finned products). This gives great freedom in placing, when installing Carat, yet keeps air
velocities low.
Product specification:
The material composition of the declared product is given below. This material composition is
based on the specific variant Carat-31 with a length of 1.2 m.
Materials KG %
Aluminium 1.30 55
Copper 0.84 36
Powder coating 0.21 9
Technical data:
Lindabs active chilled beams are Eurovent-certified and tested according to EN-14518.
Market:
Europe, Australia
Reference service life, product:
The reference service life of the product is highly dependent on the conditions of use but an
average lifespan under normal conditions is 20 years. This is an estimated value based on
experience and scientific facts about materials in Carat.
Reference service life, building:
Not declared
EPD for the best environmental decision 4
LCA: Calculation rules
Declared unit:
1 piece of Carat-31 product with a length of 1.2 m.
Calculation of EPD results for other sizes and lenghts:
Carat comes in many different product configurations and sizes, the results presented in this
EPD is representative for Carat-31 with a length of 1.2 m.
It was concluded that the Carat-31 (results per piece for the 1.2 m length) can be used as the
reference (the results in the EPD) and that the results for all other Carat products and lengths
can be obtained by multiplying with a conversion factor and the actual length of the product.
To conclude this, the 10 % rule was checked for all LCIA-indicators to check whether it was
possible to declare all product variants in the same EPD or not. The 10 % rule is used in order to
check that the variation in LCIA indicator results between products is not larger than ± 10 %.
The calculations for the LCIA-indicators showed that the 10 % rule was fulfilled for all
environmental impact categories except ODP, ADP-M&M and WDP. For these indicators the
variation is stated in the Table below. However by using the conversion factors stated below all
these impact categories are overestimated and therefore this is considered as a conservative
approach.
Carat-31 Carat-44 Carat-58 Carat-71 Carat-84
Parameter Unit
(6.0 m) (6.0 m) (6.0 m) (6.0 m) (6.0 m)
ODP kg CFC-11 eq 14 % higher 15 % higher 16 % higher 13 % higher 15 % higher
ADP-M&M kg Sb eq 32 % higher 32 % higher 31 % higher 28 % higher 31 % higher
WDP m3 15 % higher 17 % higher 18 % higher 16 % higher 17 % higher
The result for all variants of Carat can be calculated through this formula.
Results (per 1 piece of Carat) =
EPD results for Carat-31 1.2 m * size specific factor * length of the product
The size specific factors are presented in the Table below:
Product size Size specific factor
Carat-31 0.83
Carat-44 1.25
Carat-58 1.67
Carat-71 2.08
Carat-84 2.5
EPD for the best environmental decision 5
Data quality:
Specific data for the product composition is provided by Lindab Ventilation AB in 2022. Data for
the core process is collected by Lindab in 2020. Background data is based on registered
Gabi/sphera database 2022.1 and Ecoinvent 3.8. Transport data is based on data from Sphera.
Allocation:
The allocation is made in accordance with the provisions of EN 15804. Energy, water and waste
in the core process are allocated equally among all products through mass allocation.
System boundary:
Cradle to Gate with options. Mandatory stages: A1-A3, A4, C1-C4, D
Cut-off criteria:
All raw materials and all the essential energy is included. All hazardous and toxic materials and
substances are considered in the inventory even though they are below the cut off criteria.
EPD for the best environmental decision 6
LCA: Scenarios and additional technical information
The following information describe the scenarios in the different modules of the EPD.
Scenarios have been developed to account for downstream processes such as demolition and
waste treatment in accordance with the requirements of EN 15804 and NPCR 030 Part B. See
more information on next page.
A1 Raw material supply
This module takes into account the extraction and processing of all raw materials and energy
which occur upstream to the studied manufacturing process. The raw material supply covers
production of aluminium, copper, powder coating and packaging materials.
A2 Transport to the manufacturer
The raw materials are transported by truck and boat to the manufacturing site.
A3 Manufacturing
Aluminum strips and copper pipes are purchased from the supplier in coils. The coils from
copper and aluminum are placed in the rolling mill that will produce the raw material for the
product, strips. The aluminum strip and the copper tube are rolled together with high pressure
and heat (metallurgical joining) so that a homogeneous strip of the materials is formed which is
then rolled up on a roll.
The coil of the finished strip is placed in the "Strip machine" where the strip is rolled out, the
copper pipe is inflated and the strip is cut to the correct length according to customer order.
EPD for the best environmental decision 7
The strip is then placed in a press where gills are punched in the material and the edges are
rolled. To join several strips to a predetermined width, the strips are placed in the Carat
machine where they are joined by stucco riveting along the strip. Suspension brackets of square
profile are screwed in place in parallel in the process.
Connecting pipes and manifold are placed on the end of the product and soldered together with
the strip. Cover plugs are placed over the connecting pipes. Finally, the product is powder
coated and then packed on a wooden pallet with packaging of cellular plastic and stretch plastic.
Transport from production place to user (A4)
This module includes transport from the production gate to the user. Transport is calculated on
the basis of a scenario with the parameters described in the table. The scenario is based on an
assumption that 50 % of products are sold to Europe and 50 % to Australia. From this
assumption two generic distances for Europe and Austrailia are combined to an average.
Capacity
Fuel/Energy
utilisation value
Type Type of vehicle Distance (km) consumption
(incl. return) (l/t)
(l/tkm)
%
Truck 85 Long distance truck 224 0.016 3.6
Boat N.R. Container ship 11 228 0.0037 42
End of Life (C1, C3, C4)
The scenarios analysed for these modules are representative for the most likely scenario.
Aluminium and copper are deconstructed and transported to waste processing and 85 % of the
materials were assumed to be recycled and the rest disposed of. The powder coating is assumed
to be combusted in the smelting process.
Unit Value
Hazardous waste disposed kg 0
Collected as mixed construction waste kg 0
Reuse kg 0
Recycling kg 1.58
Energy recovery kg 0
To landfill kg 0.28
Deconstruction, demolition (C1)
This is the amount of energy required for deconstruction/demolition of aluminium and copper.
Process Fuel/energy consumption Type of fuel/energy
Demolition of product 0.004 MJ/kg Diesel
EPD for the best environmental decision 8
Transport to waste processing (C2)
Capacity
Fuel/Energy
utilisation Type of Distance value
Type consumption
(incl. vehicle (km) (l/t)
(l/tkm)
return) %
Long
Truck 85 distance 150 0.016 2.4
truck
Benefits and loads beyond the system boundaries (D)
The Carat product is assumed to be recycled as one unit and used for manufacturing engine
blocks, since this highly alloyed aluminium is good for this purpose. Engine blocks are normally
made from recycled aluminium and therefore the recycled material minus recycled content in
the materials are credited with a dataset for recycled aluminium.
Unit Value
Replacement of recycled aluminium in engine blocks Kg 0.86
Additional technical information
No additional information
EPD for the best environmental decision 9
System boundaries (X=included, MND= module not declared, MNR=module not relevant)
Benefits &
loads
Assembly
Product stage Use stage End of life stage beoyond
stage
system
boundary
EPD for the best environmental decision 10
slairetam
waR
tropsnarT
gnirutcafunaM
tropsnarT ylbmessA
esU
ecnanetniaM
riapeR
tnemecalpeR tnemhsibrufeR
esu
ygrene
lanoitarepO
esu
retaw
lanoitarepO
noitilomed
noitcurtsnoc-eD
tropsnarT
gnissecorp
etsaW
lasopsiD
-yrevoceR-esueR
laitnetop-gnilcyceR
LCA: Results
A1 A2 A3 A4 A5 B1 B2 B3 B4 B5 B6 B7 C1 C2 C3 C4 D
X X X X MND MND MND MND MND MND MND MND X X X X X
Core environmental impact indicators per 1 piece of Carat-31 1.2 m
Indicator Unit A1-A3 A4 C1 C2 C3 C4 D
GWP-total kg CO2 eq. 1.06E+01 4.00E-01 6.85E-04 1.86E-02 2.58E-01 4.04E-03 -2.92E-01
GWP-fossil kg CO2 eq. 1.06E+01 3.99E-01 6.81E-04 1.82E-02 2.64E-01 4.16E-03 -2.92E-01
GWP-
kg CO2 eq. 3.80E-02 7.05E-04 -9.45E-07 1.79E-04 -5.85E-03 -1.23E-04 -2.57E-04
biogenic
GWP-LULUC kg CO2 eq. 3.32E-03 2.79E-04 3.81E-06 1.51E-04 2.51E-05 7.68E-06 -9.31E-05
kg CFC11
ODP 8.74E-08 2.14E-14 4.11E-17 2.35E-18 4.19E-14 9.78E-15 -1.66E-12
eq.
AP mol H⁺ eq. 4.86E-02 1.43E-02 3.97E-06 1.74E-05 5.71E-05 2.95E-05 -7.18E-04
EP-
kg P eq. 1.93E-04 2.72E-07 2.04E-09 5.45E-08 5.16E-08 7.05E-09 -2.02E-07
freshwater
EP-marine kg N eq. 6.59E-03 3.63E-03 1.94E-06 5.36E-06 2.20E-05 7.54E-06 -2.21E-04
EP-terrestial mol N eq. 7.06E-02 3.98E-02 2.15E-05 6.46E-05 2.85E-04 8.29E-05 -2.42E-03
kg NMVOC
POCP 2.10E-02 1.02E-02 3.75E-06 1.50E-05 5.93E-05 2.29E-05 -6.36E-04
eq.
ADP-M&M kg Sb eq. 1.27E-04 1.61E-08 5.73E-11 1.40E-09 5.70E-09 4.27E-10 -3.33E-08
-
ADP-fossil MJ 1.59E+02 4.84E+00 9.14E-03 2.45E-01 1.79E-01 5.45E-02
4.66E+00
WDP m³ 1.83E+00 1.03E-03 6.14E-06 1.60E-04 2.96E-02 4.56E-04 -5.16E-03
GWP-total: Global Warming Potential; GWP-fossil: Global Warming Potential fossil fuels; GWP-biogenic: Global Warming Potential
biogenic; GWP-LULUC: Global Warming Potential land use and land use change; ODP: Depletion potential of the stratospheric ozone
layer; AP: Acidification potential, Accumulated Exceedance; EP-freshwater: Eutrophication potential, fraction of nutrients reaching
freshwater end compartment; See “additional Norwegian requirements” for indicator given as PO4 eq. EP-marine: Eutrophication
potential, fraction of nutrients reaching freshwater end compartment; EP-terrestial: Eutrophication potential, Accumulated
Exceedance; POCP: Formation potential of tropospheric ozone; ADP-M&M: Abiotic depletion potential for non-fossil resources
(minerals and metals); ADP-fossil: Abiotic depletion potential for fossil resources; WDP: Water deprivation potential, deprivation
weighted water consumption
Classification of disclaimers to the declaration of core and additional environmental
impact indicators
ILCD
Indicator Disclaimer
classification
Global warming potential (GWP) None
ILCD type /
Depletion potential of the stratospheric ozone layer (ODP) None
level 1
Potential incidence of disease due to PM emissions (PM) None
Acidification potential, Accumulated Exceedance (AP) None
Eutrophication potential, Fraction of nutrients reaching freshwater end
None
compartment (EP-freshwater)
Eutrophication potential, Fraction of nutrients reaching marine end compartment
None
ILCD type / (EP-marine)
level 2
Eutrophication potential, Accumulated Exceedance (EP-terrestrial) None
Formation potential of tropospheric ozone (POCP) None
Potential Human exposure efficiency relative to U235 (IRP) 1
Abiotic depletion potential for non-fossil resources (ADP-minerals&metals) 2
Abiotic depletion potential for fossil resources (ADP-fossil) 2
Water (user) deprivation potential, deprivation-weighted water consumption
2
(WDP)
ILCD type /
Potential Comparative Toxic Unit for ecosystems (ETP-fw) 2
level 3
Potential Comparative Toxic Unit for humans (HTP-c) 2
Potential Comparative Toxic Unit for humans (HTP-nc) 2
Potential Soil quality index (SQP) 2
Disclaimer 1 – This impact category deals mainly with the eventual impact of low dose ionizing radiation on
human health of the nuclear fuel cycle. It does not consider effects due to
possible nuclear accidents, occupational exposure nor due to radioactive waste disposal in underground facilities.
Potential ionizing radiation from the soil, from radon and from some
construction materials is also not measured by this indicator.
Disclaimer 2 – The results of this environmental impact indicator shall be used with care as the uncertainties on
these results are high or as there is limited experienced with the indicator
EPD for the best environmental decision 11
Resource use per 1 piece of Carat-31 1.2 m
Parameter Unit A1-A3 A4 C1 C2 C3 C4 D
5.20E- 1.37E- 3.72E- 8.18E-
RPEE MJ 7.31E+01 5.24E-02 -4.15E-01
04 02 02 03
0.00E+ 0.00E+ 0.00E+ 0.00E+
RPEM MJ 0.00E+00 0.00E+00 0.00E+00
00 00 00 00
5.20E- 1.37E- 3.72E- 8.18E-
TPE MJ 7.31E+01 5.24E-02 -4.15E-01
04 02 02 03
9.17E- 2.45E- 1.79E- 5.46E-
NRPE MJ 1.59E+02 4.85E+00 -4.66E+00
03 01 01 02
0.00E+ 0.00E+ 0.00E+ 0.00E+
NRPM MJ 0.00E+00 0.00E+00 0.00E+00
00 00 00 00
9.17E- 2.45E- 1.79E- 5.46E-
TRPE MJ 1.59E+02 4.85E+00 -4.66E+00
03 01 01 02
0.00E+ 0.00E+ 0.00E+ 0.00E+
SM kg 6.08E-01 0.00E+00 0.00E+00
00 00 00 00
0.00E+ 0.00E+ 0.00E+ 0.00E+
RSF MJ 0.00E+00 0.00E+00 0.00E+00
00 00 00 00
0.00E+ 0.00E+ 0.00E+ 0.00E+
NRSF MJ 0.00E+00 0.00E+00 0.00E+00
00 00 00 00
5.89E- 1.56E- 6.82E- 1.39E-
W m3 1.46E-01 7.17E-05 -3.87E-04
07 05 04 05
RPEE Renewable primary energy resources used as energy carrier; RPEM Renewable primary energy resources used as raw materials;
TPE Total use of renewable primary energy resources; NRPE Non renewable primary energy resources used as energy carrier; NRPM
Non renewable primary energy resources used as materials; TRPE Total use of non renewable primary energy resources; SM Use of
secondary materials; RSF Use of renewable secondary fuels; NRSF Use of non renewable secondary fuels; W Use of net fresh water
End of life – Waste per 1 piece of Carat-31 1.2 m
Parameter Unit A1-A3 A4 C1 C2 C3 C4 D
3.56E- 4.40E- 1.24E- 6.24E- 2.80E-
HW KG 7.93E-08 -1.19E-09
11 14 11 12 12
5.00E- 1.31E- 3.64E- 1.78E- 2.79E-
NHW KG 2.54E+00 -2.13E-02
04 06 05 02 01
5.64E- 1.13E- 2.97E- 8.74E- 6.07E-
RW KG 1.46E-02 -1.89E-04
06 08 07 06 07
HW Hazardous waste disposed; NHW Non hazardous waste disposed; RW Radioactive waste disposed
End of life – output flow per 1 piece of Carat-31 1.2 m
Parameter Unit A1-A3 A4 C1 C2 C3 C4 D
0.00E+ 0.00E+ 0.00E+ 0.00E+
CR kg 0.00E+00 0.00E+00 0.00E+00
00 00 00 00
0.00E+ 0.00E+ 1.58E+ 0.00E+
MR kg 2.81E-01 0.00E+00 0.00E+00
00 00 00 00
0.00E+ 0.00E+ 0.00E+ 0.00E+
MER kg 0.00E+00 0.00E+00 0.00E+00
00 00 00 00
0.00E+ 0.00E+ 0.00E+ 0.00E+
EEE MJ 0.00E+00 0.00E+00 0.00E+00
00 00 00 00
0.00E+ 0.00E+ 0.00E+ 0.00E+
ETE MJ 0.00E+00 0.00E+00 0.00E+00
00 00 00 00
CR Components for reuse; MR Materials for recycling; MER Materials for energy recovery; EEE Exported electric energy; ETE Exported
thermal energy
Reading example: 9,0 E-03 = 9,0*10-3 = 0,009
EPD for the best environmental decision 12
Information describing the biogenic carbon content at the factory gate per 1
piece of Carat-31 1.2 m
Biogenic carbon content Unit Value
Biogenic carbon content in product kg C N.R.
Biogenic carbon content in the accompanying packaging kg C 0.15
EPD for the best environmental decision 13
Additional Norwegian requirements
Greenhouse gas emission from the use of electricity in the manufacturing phase
National production mix from import, low voltage (production of transmission lines, in addition
to direct emissions and losses in grid) of applied electricity for the manufacturing process(A3).
In Sweden wind power is used in all manufacturing sites, guarantee of origin is available.
National electricity grid Unit Value
Swedish national grid mix kg CO2 -eq/kWh 0.044
The results with using Swedish national grid mix instead, gives the value presented in the table
below per 1 piece of Carat-31 1.2 m.
Indicator Unit A1-A3
GWP-IOBC kg CO2 eq. 1.04E+01
Additional environmental impact indicators required in NPCR Part A for construction
products
In order to increase the transparency of biogenic carbon contribution to climate impact the
indicator GWP-IOBC is presented per 1 piece of Carat-31 1.2 m. This indicator excludes biogenic
carbon dioxide and are sometimes called GWP-GHG.
Indicator Unit A1-A3 A4 C1 C2 C3 C4 D
GWP-IOBC kg CO2 eq. 1.04E+01 3.94E-01 6.73E-04 1.81E-02 2.63E-01 4.10E-03 -2.85E-01
GWP-IOBC Global warming potential calculated according to the principle of instantanious oxidation. In
this indicator is uptake and emission of biogenic carbiondioxide set to zero, i.e. directa balanced out in the
module where it appears. Alternative name of this indicator is GWP-GHG.
EPD for the best environmental decision 14
Hazardous substances
The declaration is based upon reference to threshold values and/or test results and/or material
safety data sheets provided to EPD verifiers. Documentation available upon request to EPD
owner.
□ The product contains no substances given by the REACH Candidate list or the
Norwegian priority list.
□ The product contains substances given by the REACH Candidate list or the Norwegian
priority list that are less than 0,1 % by weight.
□ The product contain dangerous substances, more then 0,1% by weight, given by the
REACH Candidate List or the Norwegian Priority list, see table.
□ The product contains no substances given by the REACH Candidate list or the
Norwegian priority list. The product is classified as hazardous waste (Avfallsforskiften,
Annex III), see table.
Indoor environment
The product meets the requirements for low emissions.
Carbon footprint
Carbon footprint has not been worked out for the product.
EPD for the best environmental decision 15
Bibliography
ISO 14025:2010 Environmental labels and declarations - Type III environmental
declarations - Principles and procedures
ISO 14044:2006 Environmental management - Life cycle assessment -
Requirements and guidelines
EN 15804:2012+A2:2019 Sustainability of construction works - Environmental product
declaration - Core rules for the product category of construction
products
ISO 21930:2007 Sustainability in building construction - Environmental
declaration of building products
PCR PART A Construction products and services Ver 2
NPCR 030:2021 Part B for ventilation components
LCA report LCA methodology report for CARAT
Program Operator and
Phone +47 23 08 80 00
Publisher
The Norwegian EPD Foundation
Post Box 5250 Majorstuen, 0303
e-post: post@epd-norge.no
Oslo
Norway web www.epd-norge.no
Owner of the declaration
Lindab Ventilation AB
Stålhögavägen 115, 269 92 Båstad
Sweden web www.lindab.com
Author of the life cycle
Phone +46 10-788 65 00
assessment
IVL Swedish Environmental
e-mail anna.liljenroth@ivl.se
Research Institute
Valhallavägen 81, 114 28
elisabet.hallberg@ivl.se
Stockholm
Sweden web www.ivl.se
EPD for the best environmental decision 16
EPD for the best
environmental
decision
The Norwegian EPD foundation
www.epd-norge.no
EPD for the best environmental decision 17
