Environmental product declaration
in accordance with ISO 14025 and EN 15804+A2
Tube Wall Shelf
OOwwnneerr ooff tthhee ddeeccllaarraattiioonn:: PPrrooggrraamm ooppeerraattoorr::
SG Armaturen AS The Norwegian EPD Foundation
PPrroodduucctt:: DDeeccllaarraattiioonn nnuummbbeerr::
Tube Wall Shelf
NEPD-8331-8007-EN
DDeeccllaarreedd uunniitt::
1 pcs RReeggiissttrraattiioonn nnuummbbeerr::
TThhiiss ddeeccllaarraattiioonn iiss bbaasseedd oonn PPrroodduucctt CCaatteeggoorryy NEPD-8331-8007-EN
RRuulleess::
IIssssuuee ddaattee:: 06.12.2024
CEN Standard EN 15804:2012+A2:2019 serves as core
The Norwegian EPD Foundation PCR VVaalliidd ttoo:: 06.12.2029
IBU PCR - Part B for luminaires, lamps, and components
for luminaires EEPPDD ssooffttwwaarree::
LCAno EPD generator ID: 676801
1 / 11
GGeenneerraall iinnffoorrmmaattiioonn
PPrroodduucctt OOwwnneerr ooff tthhee ddeeccllaarraattiioonn::
Tube Wall Shelf SG Armaturen AS
Contact person: Audun Skare
Phone: +47 90021243
e-mail: audun.skare@sg-as.no
PPrrooggrraamm ooppeerraattoorr:: MMaannuuffaaccttuurreerr::
The Norwegian EPD Foundation SG Armaturen AS
Post Box 5250 Majorstuen, 0303 Oslo, Norway Skytterheia 25
Phone: +47 977 22 020 4790 Lillesand, Norway
web: www.epd-norge.no
DDeeccllaarraattiioonn nnuummbbeerr:: PPllaaccee ooff pprroodduuccttiioonn::
SG Armaturen production site Dong Guan (China)
NEPD-8331-8007-EN No. 96 Wen Quan South Road, Shi Long Information Industrial Park
523325 Dong Guan, China
TThhiiss ddeeccllaarraattiioonn iiss bbaasseedd oonn PPrroodduucctt CCaatteeggoorryy RRuulleess:: MMaannaaggeemmeenntt ssyysstteemm::
CEN Standard EN 15804:2012+A2:2019 serves as core PCR
IBU PCR - Part B for luminaires, lamps, and components for
luminaires
SSttaatteemmeenntt ooff lliiaabbiilliittyy:: OOrrggaanniissaattiioonn nnoo::
The owner of the declaration shall be liable for the underlying 958560931
information and evidence. EPD Norway shall not be liable with respect
to manufacturer information, life cycle assessment data and
evidences.​
DDeeccllaarreedd uunniitt:: IIssssuuee ddaattee::
1 pcs Tube Wall Shelf
06.12.2024
DDeeccllaarreedd uunniitt wwiitthh ooppttiioonn:: VVaalliidd ttoo::
A1,A2,A3,A4,A5,C1,C2,C3,C4,D 06.12.2029
YYeeaarr ooff ssttuuddyy::
2023
FFuunnccttiioonnaall uunniitt:: CCoommppaarraabbiilliittyy::
1 Tube Wall Shelf LED luminaire manufactured and installed, including EPD of construction products may not be comparable if they not
waste treatment at end-of-life. comply with EN 15804 and seen in a building context.
GGeenneerraall iinnffoorrmmaattiioonn oonn vveerriiffiiccaattiioonn ooff EEPPDD ffrroomm EEPPDD ttoooollss:: DDeevveellooppmmeenntt aanndd vveerriiffiiccaattiioonn ooff EEPPDD::
Independent verification of data, other environmental information The declaration is created using EPD tool lca.tools ver EPD2021.09,
and the declaration according to ISO 14025:2010, § 8.1.3 and § 8.1.4. developed by LCA.no. The EPD tool is integrated in the company's
Verification of each EPD is made according to EPD-Norway’s management system, and has been approved by EPD Norway.
guidelines for verification and approval requiring that tools are i) NEPDT63
integrated into the company's environmental management system, ii)
the procedures for use of the EPD tool are approved by EPD-Norway, Developer of EPD: Eva Linn Jenssen
and iii) the process is reviewed annually by an independent third
Reviewer of company-specific input data and EPD:​ Audun Skare
party verifier. See Appendix G of EPD-Norway's General Programme
Instructions for further information on EPD tools
VVeerriiffiiccaattiioonn ooff EEPPDD ttooooll:: AApppprroovveedd::
Independent third party verification of the EPD tool, background data
and test-EPD in accordance with EPDNorway's procedures and
guidelines for verification and approval of EPD tools. Approval
number: NEPDT41.
Third party verifier:
Vito D’Incognito, Take Care International
(no signature required)
2 / 11
PPrroodduucctt
PPrroodduucctt ddeessccrriippttiioonn::
Accessory to Tube Wall fitting. Shelf to place the mobilphone when charging.
Housing: Aluminium. Optics: . Height: 250.0mm. Width: 85.0 mm. Depth: 90,0 mm. EAN: 7021983208125
The EPD also covers the following product:
EAN: 7021983208132 - TUBE WALL SHELF BLACK
PPrroodduucctt ssppeecciiffiiccaattiioonn
MMaatteerriiaallss kkgg %%
Metal - Aluminium wrought alloy 0,12 100,00
Total 0,12 100,00
PPaacckkaaggiinngg kkgg %%
Packaging - Cardboard 0,09 95,35
Packaging - Recycled paper 0,00 4,65
Total incl. packaging 0,21 100,00
TTeecchhnniiccaall ddaattaa::
Link to product data on our website:
https://www.sg-as.com/products/tube-wall/320812/pdf/specification_320812.pdf
Link to CE Declaration:
https://www.sg-as.com/assets/product/default/data/701199_Tube%20Wall/50/701199_Tube%20Wall.pdf
MMaarrkkeett::
Nordic + Northwestern Europe
RReeffeerreennccee sseerrvviiccee lliiffee,, pprroodduucctt
The reference service life is not relevant for this luminaire shelf.
RReeffeerreennccee sseerrvviiccee lliiffee,, bbuuiillddiinngg oorr ccoonnssttrruuccttiioonn wwoorrkkss
60 years. Standard service life for buildings to the PCR Part A of EPD Norway.
LLCCAA:: CCaallccuullaattiioonn rruulleess
DDeeccllaarreedd uunniitt::
1 pcs Tube Wall Shelf
CCuutt--ooffff ccrriitteerriiaa::
All major raw materials and all the essential energy is included. The production processes for raw materials and energy flows with very small
amounts (less than 1%) can be excluded. These cut-off criteria do not apply for hazardous materials and substances.
AAllllooccaattiioonn::
The allocation is made in accordance with the provisions of EN 15804. Incoming energy and water and waste production in-house is allocated
equally among all products through mass allocation. Effects of primary production of recycled materials is allocated to the main product in which
the material was used. The recycling process and transportation of the material is allocated to this analysis.
DDaattaa qquuaalliittyy::
Specific data for the product composition are provided by the manufacturer. The data represent the production of the declared product and were
collected for EPD development in the year of study. Background data is based on EPDs according to EN 15804 and different LCA databases. The
data quality of the raw materials in A1 is presented in the table below.
MMaatteerriiaallss SSoouurrccee DDaattaa qquuaalliittyy YYeeaarr
Supplier data +
Metal - Aluminium wrought alloy Modified ecoinvent 3.6 2019
database
Packaging - Cardboard Modified ecoinvent 3.6 Database 2019
Packaging - Recycled paper Modified ecoinvent 3.6 Database 2019
3 / 11
SSyysstteemm bboouunnddaarriieess ((XX==iinncclluuddeedd,, MMNNDD==mmoodduullee nnoott ddeeccllaarreedd,, MMNNRR==mmoodduullee nnoott rreelleevvaanntt))
CCoonnssttrruuccttiioonn BBeeyyoonndd tthhee ssyysstteemm
PPrroodduucctt ssttaaggee UUssee ssttaaggee EEnndd ooff lliiffee ssttaaggee
iinnssttaallllaattiioonn ssttaaggee bboouunnddaarriieess
A1 A2 A3 A4 A5 B1 B2 B3 B4 B5 B6 B7 C1 C2 C3 C4 D
X X X X X MND MND MND MND MND MND MND X X X X X
SSyysstteemm bboouunnddaarryy::
AAddddiittiioonnaall tteecchhnniiccaall iinnffoorrmmaattiioonn::
Link to Mounting instruction on our website:
https://www.sg-as.com/assets/product/default/data/701199_Tube%20Wall/20/7021983208125_Tube%20Wall%20Shelf_User%20Manual.pdf
waR slairetam tropsnarT gnirutcafunaM tropsnarT ylbmessA e​sU ecnanetniaM riapeR tnemecalpeR tnemhsibrufeR lanoitarepO ygrene esu lanoitarepO esu retaw -eD noitcurtsnoc noitilomed tropsnarT etsaW gnissecorp lasopsiD -yrevoceR-esueR laitnetop-gnilcyceR
4 / 11
LLCCAA:: SScceennaarriiooss aanndd aaddddiittiioonnaall tteecchhnniiccaall iinnffoorrmmaattiioonn
The following information describe the scenarios in the different modules of the EPD.
Module A4 = Transportation by truck (160 km) from the production site in Guangzhou, China to the harbor in Shenzhen, China. After this the
goods are transported by ship (19000 km) from Shenzhen, China to Bremerhaven, Germany. Then with a truck (650 km) from Bremerhaven,
Germany to the warehouse in Lillesand, Norway or to the warehouse in Mechelen, Belgium + 800 km for Nordic / Northwestern Europe Market.
Module A5 = Installation is performed in the Nordic / Northwestern Europe Market and done by manual labor, with the use of electrical machines,
that fall under the cut-off criteria of 1% and is therefore neglected. Packaging of the final product consist of a corrugated board box.
Module C1 = The de-installation of the luminaire is done by manual labor, with the help of electrical machines. The use of portable electrical
devices (e.g., drill) usually have low energy requirements falling under the cut-off-criterion of 1% and is therefore neglected.
Module C2 = Transportation from building site to the waste treatment facility with an average distance of 300km.
Modules C3 and C4 = Waste treatment of the product follows the default values provided in EN 50693, Product Category Rules for life cycle
assessments of electronic and electrical products and systems, table G.4. This table specified how different types of raw materials used in A1 will
likely be treated during the end-of-life of the product. Waste treatments in C3 include material recycling and incineration with and without energy
recovery and fly ash extraction. Disposal in C4 consist of landfilling of different waste fractions and of ashes.
Module D = The recyclability of metals, plastics, and electronic components allows the producers a credit for the net scrap that is produced at the
end of a product’s life. The benefits from recycling of net scrap are described in formula from EN 15804:2012+A2:2019. Substitution of heat and
electricity generated by the incineration with energy recovery of plastic insulation and other parts is also calculated in module D.
TTrraannssppoorrtt ffrroomm pprroodduuccttiioonn ppllaaccee ttoo uusseerr CCaappaacciittyy uuttiilliissaattiioonn VVaalluuee
DDiissttaannccee ((kkmm)) FFuueell//EEnneerrggyy CCoonnssuummppttiioonn UUnniitt
((AA44)) ((iinnccll.. rreettuurrnn)) %% ((LLiitteerr//ttoonnnnee))
Ship, Freight, Transoceanic (km) 65,0 % 19000 0,003 l/tkm 57,00
Truck, 16-32 tonnes, EURO 6 (km) - Europe 36,7 % 1450 0,043 l/tkm 62,35
Truck, 16-32 tonnes, EURO 6 (km) - Rest of World 38,8 % 40 0,044 l/tkm 1,76
AAsssseemmbbllyy ((AA55)) UUnniitt VVaalluuee
Waste, packaging, corrugated board box, with
recycled content, to average treatment (kg) - A5 kg 0,09
including transport
Waste, packaging, paper printed, 100% recycled
content, to average treatment (kg) - Global - A5, kg 0,00
incl. 85 km transp
CCaappaacciittyy uuttiilliissaattiioonn VVaalluuee
TTrraannssppoorrtt ttoo wwaassttee pprroocceessssiinngg ((CC22)) DDiissttaannccee ((kkmm)) FFuueell//EEnneerrggyy CCoonnssuummppttiioonn UUnniitt
((iinnccll.. rreettuurrnn)) %% ((LLiitteerr//ttoonnnnee))
Truck, 16-32 tonnes, EURO 6 (km) - Rest of World 38,8 % 300 0,044 l/tkm 13,20
WWaassttee pprroocceessssiinngg ((CC33)) UUnniitt VVaalluuee
Aluminium to recycling (kg) kg 0,08
DDiissppoossaall ((CC44)) UUnniitt VVaalluuee
Landfilling of aluminium (kg) kg 0,03
BBeenneeffiittss aanndd llooaaddss bbeeyyoonndd tthhee ssyysstteemm
UUnniitt VVaalluuee
bboouunnddaarriieess ((DD))
Substitution of primary aluminium with net scrap
kg -0,03
(kg)
Substitution of electricity (MJ) MJ 0,01
Substitution of thermal energy, district heating
MJ 0,08
(MJ)
5 / 11
LLCCAA:: RReessuullttss
The LCA results are presented below for the declared unit defined on page 2 of the EPD document.
EEnnvviirroonnmmeennttaall iimmppaacctt
IInnddiiccaattoorr UUnniitt A1 A2 A3 A4 A5 C1 C2 C3 C4 D
GWP-total
kg CO2 -
7,47E-01 8,63E-04 8,23E-02 9,01E-02 1,65E-01 0 1,09E-02 0,00E+00 5,00E-04 3,16E-01
eq
GWP-fossil
kg CO2 -
8,82E-01 8,62E-04 8,23E-02 9,00E-02 1,57E-03 0 1,09E-02 0,00E+00 5,00E-04 3,08E-01
eq
GWP-biogenic
kg CO2 -
-1,37E-01 3,36E-07 2,05E-05 3,19E-05 1,64E-01 0 4,23E-06 0,00E+00 0,00E+00 1,42E-03
eq
GWP-luluc
kg CO2 -
2,63E-03 3,15E-07 1,30E-05 4,48E-05 5,18E-07 0 3,98E-06 0,00E+00 1,94E-07 5,85E-03
eq
kg
ODP CFC11 - 4,89E-08 1,89E-10 1,21E-09 1,98E-08 3,30E-10 0 2,36E-09 0,00E+00 1,40E-10 -3,54E-05
eq
mol H+
AP 5,60E-03 2,58E-06 4,30E-04 1,39E-03 7,42E-06 0 3,25E-05 0,00E+00 3,88E-06 2,09E-03
-eq
EP-FreshWater kg P -eq 4,40E-05 8,09E-09 1,83E-06 5,74E-07 1,29E-08 0 1,02E-07 0,00E+00 9,06E-09 1,19E-05
EP-Marine kg N -eq 9,23E-04 5,08E-07 8,88E-05 3,34E-04 2,45E-06 0 6,40E-06 0,00E+00 1,39E-06 2,63E-04
mol N -
EP-Terrestial 9,86E-03 5,68E-06 9,78E-04 3,72E-03 2,66E-05 0 7,16E-05 0,00E+00 1,57E-05 2,89E-03
eq
kg
POCP NMVOC 3,07E-03 2,13E-06 2,58E-04 1,00E-03 7,63E-06 0 2,68E-05 0,00E+00 4,43E-06 9,76E-04
-eq
ADP- kg Sb-
3,98E-05 2,31E-08 2,54E-07 1,72E-06 3,81E-08 0 2,92E-07 0,00E+00 3,80E-09 -4,80E-07
minerals&metals1 eq
ADP-fossil1 MJ 9,76E+00 1,27E-02 7,28E-01 1,27E+00 2,19E-02 0 1,61E-01 0,00E+00 1,15E-02 3,92E+00
WDP1 m3 3,27E+01 4,15E-03 1,19E-01 8,42E-01 2,78E-02 0 5,24E-02 0,00E+00 2,99E-01 1,77E+02
GWP-total = Global Warming Potential total; GWP-fossil = Global Warming Potential fossil fuels; GWP-biogenic = Global Warming Potential biogenic; GWP-luluc =
Global Warming Potential land use and land use change; ODP = Depletion potential of the stratospheric ozone layer; AP = Acidification potential, Accumulated
Exceedance; EP-freshwater = Eutrophication potential, fraction of nutrients reaching freshwater end compartment: EP-marine = Eutrophication potential, fraction of
nutrients reaching marine end compartment; EP-terrestrial = Eutrophication potential, Accumulated Exceedance; POCP = Formation potential of tropospheric ozone;
ADP-minerals&metals = Abiotic depletion potential for non-fossil resources; ADP-fossil = Abiotic depletion for fossil resources potential; WDP = Water (user)
deprivation potential, deprivation-weighted water consumption
"Reading example: 9,0 E-03 = 9,0*10-3 = 0,009"
*INA Indicator Not Assessed
1. The results of this environmental impact indicator shall be used with care as the uncertainties on these results are high or as there is limited experienced with the
indicator
RReemmaarrkkss ttoo eennvviirroonnmmeennttaall iimmppaaccttss
The product is compliant with the European RoHS Directive 2011/65/EU on Restriction of the use of certain Hazardous Substances in Electrical and
Electronic equipment and with the European REACH regulation (EC) no 1907/2006 on Registration, Evaluation, Authorization and Restriction of
Chemicals.
6 / 11
AAddddiittiioonnaall eennvviirroonnmmeennttaall iimmppaacctt iinnddiiccaattoorrss
IInnddiiccaattoorr UUnniitt A1 A2 A3 A4 A5 C1 C2 C3 C4 D
PM Disease incidence 5,14E-08 5,50E-11 5,81E-09 3,18E-09 1,09E-10 0 7,03E-10 0,00E+00 6,70E-11 2,13E-08
IRP2 kgBq U235 -eq 2,47E-02 5,30E-05 6,30E-04 5,51E-03 9,37E-05 0 6,68E-04 0,00E+00 7,73E-05 1,71E-02
ETP-fw1 CTUe 6,06E+01 1,03E-02 2,14E+00 8,66E-01 2,92E-02 0 1,30E-01 0,00E+00 2,15E+01 4,63E+00
HTP-c1 CTUh 9,04E-10 0,00E+00 2,30E-11 0,00E+00 1,00E-12 0 0,00E+00 0,00E+00 1,00E-12 7,82E-10
HTP-nc1 CTUh 2,52E-08 1,00E-11 1,01E-09 6,35E-10 3,70E-11 0 1,28E-10 0,00E+00 1,70E-11 9,08E-09
SQP1 dimensionless 3,22E+00 8,73E-03 1,54E-01 6,13E-01 1,47E-02 0 1,10E-01 0,00E+00 2,00E-02 -1,29E-02
PM = Particulate Matter emissions; IRP = Ionizing radiation – human health; ETP-fw = Eco toxicity – freshwater; HTP-c = Human toxicity – cancer effects; HTP-nc =
Human toxicity – non cancer effects; SQP = Potential Soil Quality Index (dimensionless)
"Reading example: 9,0 E-03 = 9,0*10-3 = 0,009"
*INA Indicator Not Assessed
1. The results of this environmental impact indicator shall be used with care as the uncertainties on these results are high or as there is limited experienced with the
indicator
2. This impact category deals mainly with the eventual impact of low dose ionizing radiation on human health of the nuclear fuel cycle. It does not consider effects due
to possible nuclear accidents, occupational exposure nor due to radioactive waste disposal in underground facilities. Potential ionizing radiation from the soil, from
radon and from some construction materials is also not measured by this indicator.
7 / 11
RReessoouurrccee uussee
IInnddiiccaattoorr UUnniitt A1 A2 A3 A4 A5 C1 C2 C3 C4 D
PERE MJ 2,27E+00 1,44E-04 7,33E-02 1,44E-02 3,61E-04 0 1,82E-03 0,00E+00 1,61E-03 1,38E+00
PERM MJ 6,04E-01 0,00E+00 0,00E+00 0,00E+00 -6,04E-01 0 0,00E+00 0,00E+00 0,00E+00 0,00E+00
PERT MJ 2,88E+00 1,44E-04 7,33E-02 1,44E-02 -6,03E-01 0 1,82E-03 0,00E+00 1,61E-03 1,38E+00
PENRE MJ 9,76E+00 1,27E-02 7,28E-01 1,27E+00 2,19E-02 0 1,61E-01 0,00E+00 1,15E-02 3,92E+00
PENRM MJ 0,00E+00 0,00E+00 0,00E+00 0,00E+00 0,00E+00 0 0,00E+00 0,00E+00 0,00E+00 0,00E+00
PENRT MJ 9,76E+00 1,27E-02 7,28E-01 1,27E+00 2,19E-02 0 1,61E-01 0,00E+00 1,15E-02 3,92E+00
SM kg 2,13E-01 0,00E+00 0,00E+00 0,00E+00 0,00E+00 0 0,00E+00 0,00E+00 0,00E+00 0,00E+00
RSF MJ 2,13E-02 2,82E-06 6,44E-05 4,76E-04 1,20E-05 0 3,56E-05 0,00E+00 3,34E-05 5,74E-04
NRSF MJ 1,29E-06 2,39E-05 6,07E-04 2,55E-03 4,93E-05 0 3,02E-04 0,00E+00 0,00E+00 -4,64E-03
FW m3 7,55E-03 1,42E-06 1,99E-03 1,09E-04 1,03E-05 0 1,80E-05 0,00E+00 1,51E-05 7,72E-03
PERE = Use of renewable primary energy excluding renewable primary energy resources used as raw materials; PERM = Use of renewable primary energy resources used
as raw materials; PERT = Total use of renewable primary energy resources; PENRE = Use of non renewable primary energy excluding non-renewable primary energy
resources used as raw materials; PENRM = Use of non renewable primary energy resources used as raw materials; PENRT = Total use of non renewable primary energy
resources; SM = Use of secondary materials; RSF = Use of renewable secondary fuels; NRSF = Use of non-renewable secondary fuels; FW = Net use of fresh water
"Reading example: 9,0 E-03 = 9,0*10-3 = 0,009"
*INA Indicator Not Assessed
8 / 11
EEnndd ooff lliiffee -- WWaassttee
IInnddiiccaattoorr UUnniitt A1 A2 A3 A4 A5 C1 C2 C3 C4 D
HWD kg 1,93E-02 1,15E-06 1,01E-04 6,20E-05 0,00E+00 0 1,45E-05 0,00E+00 1,30E-03 -1,30E-03
NHWD kg 1,16E-01 6,12E-04 6,80E-03 3,93E-02 9,68E-02 0 7,71E-03 0,00E+00 3,53E-02 8,96E-02
RWD kg 2,20E-05 8,36E-08 5,57E-07 8,72E-06 0,00E+00 0 1,05E-06 0,00E+00 8,05E-08 1,60E-05
HWD = Hazardous waste disposed; NHWD = Non-hazardous waste disposed; RWD = Radioactive waste disposed
"Reading example: 9,0 E-03 = 9,0*10-3 = 0,009"
*INA Indicator Not Assessed
EEnndd ooff lliiffee -- OOuuttppuutt ffllooww
IInnddiiccaattoorr UUnniitt A1 A2 A3 A4 A5 C1 C2 C3 C4 D
CRU kg 0,00E+00 0,00E+00 0,00E+00 0,00E+00 0,00E+00 0 0,00E+00 0,00E+00 0,00E+00 0,00E+00
MFR kg 0,00E+00 0,00E+00 2,17E-03 0,00E+00 9,01E-02 0 0,00E+00 8,12E-02 0,00E+00 0,00E+00
MER kg 0,00E+00 0,00E+00 4,68E-04 0,00E+00 3,15E-04 0 0,00E+00 0,00E+00 0,00E+00 0,00E+00
EEE MJ 0,00E+00 0,00E+00 7,05E-04 0,00E+00 5,54E-03 0 0,00E+00 0,00E+00 0,00E+00 0,00E+00
EET MJ 0,00E+00 0,00E+00 1,07E-02 0,00E+00 8,38E-02 0 0,00E+00 0,00E+00 0,00E+00 0,00E+00
CRU = Components for re-use; MFR = Materials for recycling; MER = Materials for energy recovery; EEE = Exported energy electrical; EET = Exported energy thermal
"Reading example: 9,0 E-03 = 9,0*10-3 = 0,009"
*INA Indicator Not Assessed
BBiiooggeenniicc CCaarrbboonn CCoonntteenntt
IInnddiiccaattoorr UUnniitt AAtt tthhee ffaaccttoorryy ggaattee
Biogenic carbon content in product kg C 0,00E+00
Biogenic carbon content in accompanying packaging kg C 4,49E-02
Note: 1 kg biogenic carbon is equivalent to 44/12 kg CO2
9 / 11
AAddddiittiioonnaall rreeqquuiirreemmeennttss
GGrreeeennhhoouussee ggaass eemmiissssiioonnss ffrroomm tthhee uussee ooff eelleeccttrriicciittyy iinn tthhee mmaannuuffaaccttuurriinngg pphhaassee
National production mix from import, low voltage (production of transmission lines, in addition to direct emissions and losses in grid) of applied
electricity for the manufacturing process (A3).
EElleeccttrriicciittyy mmiixx SSoouurrccee AAmmoouunntt UUnniitt
Electricity, China (kWh) ecoinvent 3.6 1102,91 g CO2-eq/kWh
DDaannggeerroouuss ssuubbssttaanncceess
The product contains no substances given by the REACH Candidate list.
IInnddoooorr eennvviirroonnmmeenntt
No effect on indoor environment
AAddddiittiioonnaall EEnnvviirroonnmmeennttaall IInnffoorrmmaattiioonn
AAddddiittiioonnaall eennvviirroonnmmeennttaall iimmppaacctt iinnddiiccaattoorrss rreeqquuiirreedd iinn NNPPCCRR PPaarrtt AA ffoorr ccoonnssttrruuccttiioonn pprroodduuccttss
IInnddiiccaattoorr UUnniitt A1 A2 A3 A4 A5 C1 C2 C3 C4 D
GWPIOBC kg CO2 -eq 9,10E-01 8,63E-04 7,78E-02 9,01E-02 1,57E-03 0 1,09E-02 0,00E+00 6,00E-04 3,01E-01
GWP-IOBC: Global warming potential calculated according to the principle of instantaneous oxidation. In order to increase the transparency of biogenic carbon​
contribution to climate impact, the indicator GWP-IOBC is required as it declares climate impacts calculated according to the principle of instantaneous oxidation.​
GWP-IOBC is also referred to as GWP-GHG in context to Swedish public procurement legislation.
10 / 11
BBiibblliiooggrraapphhyy
ISO 14025:2010. Environmental labels and declarations - Type III environmental declarations - Principles and procedures. International
Organization for Standardization.
ISO 14044:2006. Environmental management - Life cycle assessment - Requirements and guidelines. International Organization for
Standardization.
EN 15804:2012+A2:2019. Environmental product declaration - Core rules for the product category of construction products. European
Committee for Standardization.
ISO 21930:2017. Sustainability in buildings and civil engineering works - Core rules for environmental product declarations of construction
products. International Organization for Standardization.
EN 50693:2019. Product category rules for life cycle assessments of electronic and electrical products and systems. European Committee for
Standardization.
Ecoinvent v3, 2019. Allocation, cut-off by classification. Swiss Centre of Life Cycle Inventories.
Iversen et al., (2021). eEPD v2021.09, background information for EPD generator tool system verification, LCA.no. Report number: 07.21. System
verification report.
Philis et al., (2022). EPD generator for IBU PCR part B for luminaires, lamps, and components for luminaires, background information for EPD
generator application and LCA data, LCA.no. Report number: 04.22. PCR verification report.
EPD Norway (2022). NPCR Part A: Construction products and services. The Norwegian EPD foundation. Version 2.0 published 24.03.2021.
IBU (2017). PCR part B for luminaires, lampes and components for luminaires. Institut Bauen und Umwelt e.V. Version 1.7, published 30.11.2017.
PPrrooggrraamm ooppeerraattoorr aanndd ppuubblliisshheerr Phone: +47 977 22 020
The Norwegian EPD Foundation e-mail: post@epd-norge.no
Post Box 5250 Majorstuen, 0303 Oslo, Norway web: www.epd-norge.no
OOwwnneerr ooff tthhee ddeeccllaarraattiioonn:: Phone: +47 90021243
SG Armaturen AS e-mail: audun.skare@sg-as.no
Skytterheia 25, 4790 Lillesand, Norway web: www.sg-as.com
AAuutthhoorr ooff tthhee LLiiffee CCyyccllee AAsssseessssmmeenntt Phone: +47 916 50 916
LCA.no AS e-mail: post@lca.no
Dokka 6A, 1671 Kråkerøy, Norway web: www.lca.no
DDeevveellooppeerr ooff EEPPDD ggeenneerraattoorr Phone: +47 916 50 916
LCA.no AS e-mail: post@lca.no
Dokka 6A, 1671 Kråkerøy, Norway web: www.lca.no
ECO Platform web: www.eco-platform.org
ECO Portal web: ECO Portal
11 / 11
