ver1 2015
ENVIRONMENTAL PRODUCT DECLARATION
in accordance with ISO 14025, ISO 21930 and EN 15804
Owner of the declaration: Amiblu Technology AS
Program operator: The Norwegian EPD Foundation
Publisher: The Norwegian EPD Foundation
Declaration number: NEPD-3383-2004-EN
Registration number: NEPD-3383-2004-EN
ECO Platform reference number: -
Issue date: 03.03.2022
Valid to: 03.03.2027
Hobas Pipe Sewer, Spigot-Coupling
DN800-1400, PN1 SN5000
Amiblu Technology AS
www.epd-norge.no
NEPD-3383-2004-EN Hobas Pipe Sewer, Spigot-Coupling DN800-1400, PN1 SN5000
1 / 8
General information
Product: Owner of the declaration:
Hobas Pipe Sewer, Spigot-Coupling Amiblu Technology AS
DN800-1400, PN1 SN5000 Contact person: Marcin Pazdro
Phone: +47 907 21 877
e-mail: Marcin.Pazdro@amiblu.com
Program operator: Manufacturer:
Amiblu Germany GmbH
The Norwegian EPD Foundation
Pb. 5250 Majorstuen, 0303 Oslo
Phone: +47 23 08 80 00
e-mail: post@epd-norge.no
Declaration number: Place of production:
Amiblu Germany GmbH
NEPD-3383-2004-EN Gewerbepark 1, 17039 Trollenhagen
Germany
ECO Platform reference number: Management system:
ISO 14001
This declaration is based on Product Category Rules: Organisation no:
916 041 195
CEN Standard EN 15804:2012+A1:2013 serves as core PCR
NPCR 019:2018 Part B for Piping systems use in sewage and storm water systems
(under gravity)
Statement of liability: Issue date: 03.03.2022
The owner of the declaration shall be liable for the underlying information and
evidence. EPD Norway shall not be liable with respect to manufacturer Valid to: 03.03.2027
information, life cycle assessment data and evidences.
Declared unit: Year of study:
1 kg Hobas Pipe Sewer, Spigot-Coupling DN800-1400, PN1 SN5000 2020
Declared unit with option: Comparability:
EPD of construction products may not be comparable if they not comply with EN
A1,A2,A3,A4,A5,C1,C2,C3,C4,D
15804 and seen in a construction works context.
Functional unit: Development and verification of EPD:
1kg of installed GRP piping system The declaration has been developed and verified using EPD tool lca.tools
ver EPD2020.11, developed by LCA.no AS. The EPD tool is integrated into
the company's environmental management system, and has been
approved by EPD-Norway
General information on verification of EPD from EPD tools:
Independent verification of data, other environmental information and Developer of EPD:
the declaration according to ISO 14025:2010, § 8.1.3 and § 8.1.4. Individual
third party verification of each EPD is not required when the EPD tool is i) Marcin Pazdro
integrated into the company's environmental management system, ii) the
procedures for use of the EPD tool are approved by EPDNorway, and iii) Reviewer of company-specific input data and EPD:
the proccess is reviewed annualy. See Appendix G of EPD-Norway's
General Programme Instructions for further information on EPD tools. Petter Åsrud
Verification of EPD tool: Approved:
Independent third party verification of the EPD tool, background data
Sign
and test-EPD in accordance with EPDNorway's procedures and guidelines
for verification and approval of EPD tools.
Michael M. Jenssen, Asplan Viak AS
(no signature required) Håkon Hauan, CEO EPD-Norge
NEPD-3383-2004-EN Hobas Pipe Sewer, Spigot-Coupling DN800-1400, PN1 SN5000
2 / 8
Product
Product description: Technical data:
Filled (VO) Pipe, Hobas Diameter Series, Mass calculation includes coupling.
DN800-1400, PN1, SN5000, Liner: Standard,
Length: 6 m, Glass: E, Resin: Ortho, Liner Resin: Ortho, with FWC DN800 PN1 SN5000 - 76.3 kg
Coupling DN860 PN1 SN5000 - 83.9 kg
DN900 PN1 SN5000 - 96.7 kg
Product specification
DN960 PN1 SN5000 - 104.3 kg
Glass: E, Resin: Ortho, Liner Resin: Ortho DN1000 PN1 SN5000 - 119.7 kg
DN1100 PN1 SN5000 - 137.2 kg
Specifications and product details are presented here: DN1200 PN1 SN5000 - 171.6 kg
https://www.amiblu.com/pressure-pipes/ DN1280 PN1 SN5000 - 186 kg
DN1400 PN1 SN5000 - 232.9 kg
A typical composition of the pipes covered by this EPD is as follows:
Materials %
Polyester Resin 25-30
Sand 45-50
Market:
Glass fibers 8-13
Filler 20-25 Europe
Rubber gasket 0-1
Reference service life, product
Peroxide 0-1
Up to 150 years
Reference service life, construcion
LCA: Calculation rules
Declared unit: Allocation:
Allocation was carried out in accordance with EN 15804. There are no-
1 kg Hobas Pipe Sewer, Spigot-Coupling DN800-1400, PN1 SN5000
allocations between co-products in the EPD since there are no co-products
Cut-off criteria: created during the manufacturing. Environmental burdens related to A1 and
A2 stages are allocated to pipes based on the specific pipe composition,
All raw materials which are present in the final product at a
transport modes and distances of raw materials to a plant in which the
concentration greater than 0.1 % are included. Some of the raw
product has been produced. All manufacturing inputs (energy and auxiliary
materials used at lower content are modeled using datasets
materials) are allocated equally to products through mass allocation. Equal
representing the closest match according to the best knowledge of
allocation also applies to waste, although for certain waste flows, a specific
Amiblu. The contribution of capital goods is estimated to be lower than
allocation was performed based on the production process and product
the general cut-off criteria of 1%. Transport of personnel is outside the
formulation. Effects of primary production of recycled materials is allocated
scope of the LCA
to the main product in which the material was used. The recycling process
and transportation of the material is allocated to this analysis.
Data quality:
Specific data for the product compositions are used. In case of some raw materials, data from ecoinvent 3.6 were modified to better reflect the composition of
specific materials used by Amiblu. Transportation modes and distances are collected for all raw materials, specific for each production site. Energy inputs are
also specific for each site. Production site data were collected in the year of study defined on page 2. The data quality of the raw materials in A1 is presented
in the table below.
Materials Source Data quality Year
Chemicals ecoinvent3.6 Database 2019
Glass fibre ecoinvent3.6 Database 2019
Pigments and Fillers ecoinvent3.6 Database 2019
Rubber, synthetic ecoinvent3.6 Database 2019
Sand ecoinvent3.6 Database 2019
Polyester resin Modified ecoinvent3.6 Database 2019
NEPD-3383-2004-EN Hobas Pipe Sewer, Spigot-Coupling DN800-1400, PN1 SN5000
3 / 8
System boundary:
Additional technical information:
https://www.amiblu.com/
NEPD-3383-2004-EN Hobas Pipe Sewer, Spigot-Coupling DN800-1400, PN1 SN5000
4 / 8
LCA: Scenarios and additional technical information
The following information describe the scenarios in the different modules of the EPD.
For A4 stage, a specific transport distance of 700 km from the pipe production plant to the installation site is assumed. For A5 module, a trench geometry is
calculated automatically based on the diameter of the pipe. The trench depth is assume to be DN + 1/4DN + 1m. The diesel consumption of 0,36 liter per 1
cubic meter of excavated soil is used. In addition, the consumption of 1.6 liter of diesel per 1m of the trench length is used to account for material
compaction and trench filling operations. It is assumed that 50% of excavated soil is replaced with gravel. Transport distance for disposal site of unused soil
and gravel from quarry is assumed to be 20 km on average. Use stage has not been included since glass reinforced plastic piping, once installed, does not
require maintenance. It has been assumed that at the end of the functional life of the piping, the installation is either left in ground or re-lined. Potential
relining is considered to be a second life stage, thus, all environmental burdens associated with re-lining are omitted in this declaration. LCA study was
performed for the 6 m Hobas Sewer Pipe DN1000 PN1 SN5000 with the corresponding FWC coupling.
Transport from production place to user (A4)
Capacity utilisation Fuel/Energy
Type Type of vehicle Distance km Unit Value (l/t)
(incl. return) % consumption
Amiblu - Truck, lorry 16-32 tonnes,
Truck 38,8 % 700 0,044606 l/tkm 31,22
EURO 5
Railway l/tkm
Boat l/tkm
Other Transportation l/tkm
Assembly (A5)
. Unit Value
Auxiliary kg 45,9989
Water consumption m3
Electricity consumption kWh
Other energy carriers MJ 1,5754
Material loss kg
Output materials from waste treatment kg
Dust in the air kg
VOC emissions kg
¨
NEPD-3383-2004-EN Hobas Pipe Sewer, Spigot-Coupling DN800-1400, PN1 SN5000
5 / 8
LCA: Results
The LCA results are presented below for the declared unit defined on page 2 of the EPD document.
System boundaries (X=included, MND=module not declared, MNR=module not relevant)
Construction Beyond the
Product stage installation User stage End of life stage . system
stage bondaries
A1 A2 A3 A4 A5 B1 B2 B3 B4 B5 B6 B7 C1 C2 C3 C4 . D
X X X X X X X X X . X
Environmental impact
Parameter Unit A1-A3 A4 A5 C1 C2 C3 C4 D
GWP kg CO 2 -eq 1,34E+00 1,14E-01 2,64E-01 0 0 0 0 0
ODP kg CFC11 -eq 1,70E-07 2,10E-08 4,72E-08 0 0 0 0 0
POCP kg C 2H 4-eq 4,70E-04 1,86E-05 4,52E-05 0 0 0 0 0
AP kg SO 2 -eq 5,60E-03 3,63E-04 7,21E-04 0 0 0 0 0
EP kg PO 3- -eq 7,95E-04 6,02E-05 1,64E-04 0 0 0 0 0
4
ADPM kg Sb -eq 3,40E-05 3,47E-07 9,41E-07 0 0 0 0 0
ADPE MJ 2,85E+01 1,72E+00 3,70E+00 0 0 0 0 0
GWP Global warming potential; ODP Depletion potential of the stratospheric ozone layer; POCP Formation potential of tropospheric photochemical oxidants;
AP Acidification potential of land and water; EP Eutrophication potential; ADPM Abiotic depletion potential for non fossil resources; ADPE Abiotic depletion
potential for fossil resources
"Reading example: 9,0 E-03 = 9,0*10-3 = 0,009"
*INA Indicator Not Assessed
waR slairetam tropsnarT gnirutcafunaM tropsnarT ylbmessA esU ecnanetniaM riapeR tnemecalpeR tnemhsibrufeR lanoitarepO ygrene esu lanoitarepO esu
retaw
-eD noitcurtsnoc noitilomed tropsnarT etsaW gnissecorp lasopsiD -yrevoceR-esueR -gnilcyceR laitnetop
NEPD-3383-2004-EN Hobas Pipe Sewer, Spigot-Coupling DN800-1400, PN1 SN5000
6 / 8
Resource use
Parameter Unit A1-A3 A4 A5 C1 C2 C3 C4 D
RPEE MJ 1,53E+00 2,50E-02 1,79E-01 0 0 0 0 0
RPEM MJ 1,48E-04 0,00E+00 0,00E+00 0 0 0 0 0
TPE MJ 1,53E+00 2,50E-02 1,79E-01 0 0 0 0 0
NRPE MJ 3,23E+01 1,76E+00 4,05E+00 0 0 0 0 0
NRPM MJ 2,44E-03 0,00E+00 0,00E+00 0 0 0 0 0
TRPE MJ 3,23E+01 1,76E+00 4,05E+00 0 0 0 0 0
SM kg 5,63E-03 0,00E+00 2,42E+01 0 0 0 0 0
RSF MJ 9,88E-02 0,00E+00 2,64E-04 0 0 0 0 0
NRSF MJ -3,52E-03 0,00E+00 3,89E-03 0 0 0 0 0
W m3 1,63E-02 3,29E-04 3,09E-02 0 0 0 0 0
RPEE Renewable primary energy resources used as energy carrier; RPEM Renewable primary energy resources used as raw materials; TPE Total use of renewable
primary energy resources; NRPE Non renewable primary energy resources used as energy carrier; NRPM Non renewable primary energy resources used as
materials; TRPE Total use of non renewable primary energy resources; SM Use of secondary materials; RSF Use of renewable secondary fuels; NRSF Use of non
renewable secondary fuels; W Use of net fresh water
"Reading example: 9,0 E-03 = 9,0*10-3 = 0,009"
*INA Indicator Not Assessed
End of life - Waste
Parameter Unit A1-A3 A4 A5 C1 C2 C3 C4 D
HW kg 2,17E-03 1,03E-06 6,02E-05 0 0 0 0 0
NHW kg 2,20E-01 9,24E-02 7,79E-02 0 0 0 0 0
RW kg 6,24E-05 1,21E-05 2,97E-05 0 0 0 0 0
HW Hazardous waste disposed; NHW Non hazardous waste disposed; RW Radioactive waste disposed
"Reading example: 9,0 E-03 = 9,0*10-3 = 0,009"
*INA Indicator Not Assessed
End of life - Output flow
Parameter Unit A1-A3 A4 A5 C1 C2 C3 C4 D
CR kg 0,00E+00 0,00E+00 0,00E+00 0 0 0 0 0
MR kg 1,47E-03 0,00E+00 2,97E-06 0 0 0 0 0
MER kg 4,67E-02 0,00E+00 9,57E-04 0 0 0 0 0
EEE MJ 2,98E-02 0,00E+00 1,02E-05 0 0 0 0 0
ETE MJ 3,33E-01 0,00E+00 1,54E-04 0 0 0 0 0
CR Components for reuse; MR Materials for recycling; MER Materials for energy recovery; EEE Exported electric energy; ETE Exported thermal energy
"Reading example: 9,0 E-03 = 9,0*10-3 = 0,009"
*INA Indicator Not Assessed
NEPD-3383-2004-EN Hobas Pipe Sewer, Spigot-Coupling DN800-1400, PN1 SN5000
7 / 8
Additional requirements
Greenhouse gas emissions from the use of electricity in the manufacturing phase
National production mix from import, low voltage (production of transmission lines, in addition to direct emissions and losses in grid) of applied electricity for
the manufacturing process (A3).
Electricity mix Data source Amount Unit
Amiblu - Electricity, Germany (kWh) ecoinvent 3.6 629,86 g CO2-ekv/kWh
Dangerous substances
The product contains no substances given by the REACH Candidate list or the national priority list.
Indoor environment
Not relevant
Bibliography
ISO 14025:2010 Environmental labels and declarations - Type III environmental declarations - Principles and procedures.
ISO 14044:2006 Environmental management - Life cycle assessment - Requirements and guidelines.
EN 15804:2012+A1:2013 Environmental product declaration - Core rules for the product category of construction products.
ISO 21930:2017 Core rules for environmental product declarations of construction products.
ecoinvent v3, Allocation, cut-off by classification, Swiss Centre of Life Cycle Inventories.
Iversen et al., (2018) eEPD v3.0 - Background information for EPD generator system. LCA.no report 04.18.
Ruttenborg et al., (2021) EPD generator for Amiblu Technology AS Background information for customer application and LCA data, LCA.no report number 01.21
NPCR Part A: Construction products and services. Ver. 1.0. April 2017, EPD-Norge.
NPCR 019 Part B for Piping systems for use in sewage and storm water systems (under gravity), Ver 2.0.
Program operator and publisher Phone: +47 23 08 80 00
The Norwegian EPD Foundation e-mail: post@epd-norge.no
Post Box 5250 Majorstuen, 0303 Oslo,Norway web: www.epd-norge.no
Owner of the declaration Phone: +47 907 21 877
Amiblu Technology AS e-mail: Marcin.Pazdro@amiblu.com
Østre Kullerød 3 3241 Sandefjord web: https://www.amiblu.com/
Author of the Life Cycle Assessment Phone: +47 916 50 916
LCA.no AS e-mail: post@lca.no
Dokka 1C 1671 Kråkerøy web: www.lca.no
Developer of EPD generator Phone: +47 916 50 916
LCA.no AS e-mail: post@lca.no
Dokka 1C,1671 Kråkerøy web: www.lca.no
NEPD-3383-2004-EN Hobas Pipe Sewer, Spigot-Coupling DN800-1400, PN1 SN5000
8 / 8
