1114 NEPD
Ver. 2 2015(17)
ENVIRONMENTAL PRODUCT DECLARATION
in accordance with ISO 14025, ISO 21930 and EN 15804
Owner of the declaration: Flügger Norway AS
Program operator: The Norwegian EPD Foundation
Publisher: The Norwegian EPD Foundation
Declaration number: NEPD-2669-1373-EN
Registration number: NEPD-2669-1373-EN
ECO Platform reference number: -
Issue date: 08.02.2021
Valid to: 08.02.2026
Flügger Dekso 5TM
Flügger Norway AS
www.epd-norge.no
NEPD-2669-1373-EN Flügger Dekso 5TM
General information
Product: Owner of the declaration:
Flügger Dekso 5™ Flügger Norway AS
contact person: Stine Rosendal Tangaa
phone: +45 40 64 75 98
e-mail: regulatoryaffairs@flugger.com
Program operator: Manufacturer:
The Norwegian EPD Foundation Flügger Denmark A/S
Pb. 5250 Majorstuen, 0303 Oslo
Tlf: +47 23 08 82 92
e-post: post@epd-norge.no
Declaration number: Place of production:
NEPD-2669-1373-EN Vejlevej 150
6000 Kolding, Denmark
ECO Platform reference number: Management system:
ISO 14001:2015 (DK011198)
ISO 9001:2015 (DK0012451)
This declaration is based on PCR: Org. no.:
NS-EN 15804:2012+A1:2013 serves as core PCR. 45240118
Product descriptions based on "IBU PCR Part B for coatings
with organic binders". This also applies to products with
inorganic binders.
Issue date:
Statement of liability: 08.02.2021
The owner of the declaration shall be liable for the underlying
informationandevidence.EPDNorwayshallnotbeliablewith
respect to manufacturer information, life cycle assessment
data and evidences. Valid to:
08.02.2026
Declared unit: Year of study:
1 kg Flügger Dekso 5 delivered to market 2019
Declared unit with option: Comparability:
EPD of construction products may not be comparable if they
do not comply with NS-EN 15804 and seen in a building
context.
Functional unit: Author of the Life Cycle Assessment:
Mafalda Silva
NORSUS
Verification:
Independent verification of data, other environmental
information and the declaration according to ISO14025:2010, §
8.1.3 and § 8.1.4
internal external
Approved
Third party verifier:
Erik Svanes, Senior Researcher
(Independent verifier approved by EPD Norway)
NEPD-2669-1373-EN Flügger Dekso 5TM 2/9
Product
Product description: Technical data:
Flügger Dekso 5 is a matt 100% acrylic wall paint for living Density: 1,33 kg/l
rooms, corridors, entrance areas, offices, kitchens, Solids by volume: 42%
washrooms, clinics and retail shops. Recommended for EU VOC limit value for product (Cat. A/a): 30 g/l
premises with high functional and special aesthetic Product VOC max. 10 g/l
requirements, that are exposed to some dirt and wear and tear.
Withstands cleaning, including spot cleaning with soft brush, Nominal spreading rate: 8 m2/l
water and cloth. Wet film thickness: 125 µm
Dry film thickness: 53 µm
All variants are ecolabelled with the EU Ecolabel.
The most representative and worst case formulation is chosen
forthisEPD.Forproductswithaselectionofcolours,thiswill
For information on Green Building Standard credits and be the formulation with the highest content of titanium dioxide.
Ecolabels, see "Additional Information" on page 4.
The product packaging is based on an average sized plastic
packaging and is reported in the A1-phase.
For information on technical data, application and use of the
Product specification:
product,seetheTechnicalDataSheetandFDV(Forvaltning,
Life cycle analysis carried out for the white variant, which is
Drift og Vedlikehold) for the declared product on
estimated to have the greatest environmental impact.
www.flugger.no
The material composition of the declared product:
For safety, health and environmental conditions, see the
Materials %
Safety Data Sheet for the declared product on
Water 10-20
www.flugger.no.
Binder 40-50
Extender 20-25
Titanium dioxide 15-20 Market:
Solvent 1-3 Scandinavia and Europe
Additive 2-3
Biocide < 0.5
Reference service life, product
The reference service life of the product is highly dependent
Packaging kg on the conditions of use.
Wooden packaging - pallet 3,77E-02
Plastic packaging - pallet 1,32E-03 Estimated service life, object
Plastic packaging 2,81E-02 The coated object is not declared.
LCA: Calculation rules
Declared unit: System boundary:
1 kg Flügger Dekso 5 delivered to market The flow chart below illustrates the system boundaries for the
analysisaccordingtothemoduleprincipleinNS-EN15804.The
analysis is carried out from cradle-to-gate (A1-A3), including
module A4 transport to market.
A1 A2 A3 A4 A5 B1-B7 C1-C4 D
Raw materials Transport Production Transport to Application and Usephase Endof life Benefits of
market installation recovery
Preassemblyof
raw materials
Rawmaterial Transport of
extraction and raw materials
production Dispersionof
pigments
Transportof Module not Module not Module not Module not
product to declared declared declared declared
market
Mixing
Packaging Transport of
production packaging
QCcheck and
adjustment
Fillingand
labelling
Systemboundaries«Cradle-to-gate»
System boundary for this EPD
NEPD-2669-1373-EN Flügger Dekso 5TM 3/9
System boundary for this EPD
Data quality:
The CEPE database is used as basis for the rawmaterial composition. Specific datafor theproduct composition and rawmaterial
amounts has been provided bythe manufacturer and represents the production of the declared product. Production site data was
collected in 2020, with 2019 as reference year. Remaining data is based on Ecoinvent v3.6, but adjusted to improve
representativeness. All energy consumption in the database is assumed not to be used as raw material.
Cut-off criteria: Allocation:
All major raw materials and essential energy is included. The Theallocationismadeinaccordancewiththeprovisionsof
production process for raw materials and energy flows with very NS-EN 15804. Incoming energy, water and waste
small amounts (<1%), such as consumables in production and productionin-houseisprimarilyallocatedequallyamongall
administrationandemployeetravel,arenotincluded.Thesecut-off products through volume allocation. The recycling process
criteria do not apply for hazardous materials and substances. and transportation of the material is allocated to this
analysis.
Additional information:
The declared product contributes to Green Building Standard credits by meeting the following specific requirements:
-Emissioncriteriaaccordingto"M1EmissionClassificationofBuildingMaterials:ProtocolforChemicalandSensoryTestingofBuilding
Materials"
-EU Ecolabel (SE/044/002)
-Properties criteria in BASTA (2020:A2)
BREEAM®NOR (2016)
Hea 02: VOC content for Interior matt walls and ceilings (30 g/l) (EU Directive 2004/42/CE) and emission criteria (ISO 16000-series).
Mat01:TheproductcontainsnosubstancesontheNorwegianTechnicalCheckList(A20),whichexceedsthelimitvalueforhealthand
environment.
Additional certificates and approvals may be available on request.
NEPD-2669-1373-EN Flügger Dekso 5TM 4/9
LCA: Scenarios and additional technical information
The following information describe the scenarios in the different modules of the EPD.
The only declared module after the factory gate is A4 transport to market.
Transport from production place to user (A4)
Capacity utilisation Fuel/Energy
Type Type of vehicle Distance km Unit
incl. return [%] consumption
Truck 53 >32t, EURO 6 537 1,92E-02 kg/tkm
Truck 53 >32t, EURO 6 338 1,92E-02 kg/tkm
Truck 26 16-32t, EURO 6 30 4,80E-02 kg/tkm
Other
Construction/Installation (A5) Use (B1)
Unit Value Unit Value
Auxiliary kg Relevant emissions during use kg
Water consumption m3
Electricity consumption kWh
Other energy carriers MJ
Material loss kg
Dust in the air kg
VOC emissions kg
Maintenance (B2)/Repair (B3) Replacement (B4)/Refurbishment (B5)
Unit Value Unit Value
Maintenance cycle* Replacement cycle* stk
Auxiliary kg Electricity consumption kWh
Other resources kg Replacement of worn parts 0
Water consumption m3 * Value or refence shelf-life
Electricity consumption kWh
Other energy carriers MJ
Material loss kg
VOC emissions kg
Operational energy (B6) and water consumption (B7) End of life (C1, C3, C4)
Unit Value Unit Value
Water consumption m3 Hazardous waste disposed kg
Electricity consumption kWh Collected as mixed construction waste kg
Other energy carriers MJ Reuse kg
Power output of equipment kW Recycling kg
Energy recovery kg
Til landfill kg
Transport to waste processing (C2)
Capacity utilisation (incl. Fuel/Energy
Type Type of vehicle Distance km Unit Value (l/t)
return) % consumption
Truck
Railway
Boat
Other
NEPD-2669-1373-EN Flügger Dekso 5TM 5/9
LCA: Results
System boundaries (X=included, MND=module not declared, MNR=module not relevant)
Environmental impact
ecnanetniaM
esu
ygrene
lanoitarepO
2,10E-04
noitilomed
/noitcurtsnoceD
gnissecorp
etsaW
lasopsid
etsaW
Beyond the
system
boundaries
A1 A3 B1 B2 B4
X MND MND MND
ODP kg CFC11-eq.
POCP
AP kg SO -eq. 2
EP 1,30E-03 2,82E-05
6,68E-06 1,49E-06
3,11E+01
tropsnarT
MND
tropsnarT
/noitcurtsnoC egats
noitallatsni esU
riapeR
Construction/
installation stage
slairetam
waR
Product stage
-gnilcycer/yrevocer/esueR
laitnetop
End of life stage
gnirutcafunaM tnemhsibrufeR
A4 A5 B7
X X MND MND
tropsnarT
MND
Parameter
GWP kg CO -eq. 2
esu
retaw
lanoitarepO
User stage
A2 B3 B5
X MND MND MND
Unit
1,58E-08
tnemecalpeR
B6 C1 C2 C3 C4 D
MND MND MND
A1 A2 A3 A4
1,75E+00 3,80E-02 1,19E-01 8,03E-02
1,66E-07 6,96E-09 7,89E-09
kg C 2H 4 -eq. 1,04E-03 5,13E-06 5,36E-05 1,01E-05
1,12E-02 1,31E-04 1,09E-03
kg PO 43--eq. 2,19E-05 1,04E-04
ADPM kg Sb -eq. 9,29E-07 2,71E-05
ADPE MJ 5,69E-01 1,19E+00 1,29E+00
GWP Global warming potential; ODP Depletion potential of the stratospheric ozone layer; POCP Formation potential of tropospheric
photochemical oxidants; AP Acidification potential of land and water; EP Eutrophication potential; ADPM Abiotic depletion potential for non fossil
resources; ADPE Abiotic depletion potential for fossil resources
NEPD-2669-1373-EN Flügger Dekso 5TM 6/9
Resource use
Parameter Unit A1 A2 A3 A4
RPEE MJ 2,11E+00 8,56E-03 6,02E-01 1,67E-02
RPEM MJ 0,00E+00 0,00E+00 2,52E-02 0,00E+00
TPE MJ 2,11E+00 8,56E-03 6,27E-01 1,67E-02
NRPE MJ 1,41E+01 5,82E-01 1,50E+00 1,31E+00
NRPM MJ 1,99E+01 0,00E+00 0,00E+00 0,00E+00
TRPE MJ 3,40E+01 5,82E-01 1,50E+00 1,31E+00
SM kg 0,00E+00 0,00E+00 0,00E+00 0,00E+00
RSF MJ 0,00E+00 0,00E+00 0,00E+00 0,00E+00
NRSF MJ 0,00E+00 0,00E+00 0,00E+00 0,00E+00
W m3 1,73E-01 1,13E-04 1,47E-03 2,70E-04
RPEERenewableprimaryenergyresourcesusedasenergycarrier;RPEMRenewableprimaryenergyresourcesusedasrawmaterials;TPE
Total use of renewable primary energy resources; NRPE Non renewable primary energy resources used as energy carrier; NRPM Non
renewable primary energy resources used as materials; TRPE Total use of non renewable primary energyresources; SM Use of secondary
materials; RSF Use of renewable secondary fuels; NRSF Use of non renewable secondary fuels; W Use of net fresh water
End of life - Waste
Parameter Unit A1 A2 A3 A4
HW kg 2,66E-05 1,48E-06 3,62E-04 3,20E-06
NHW kg 6,12E-01 3,91E-02 1,80E-01 1,18E-01
RW kg 1,24E-04 3,96E-06 5,96E-06 8,96E-06
HW Hazardous waste disposed; NHW Non hazardous waste disposed; RW Radioactive waste disposed
End of life - Output flow
Parameter Unit A1 A2 A3 A4
CR kg 0,00E+00 0,00E+00 0,00E+00 0,00E+00
MR kg 0,00E+00 0,00E+00 7,61E-03 0,00E+00
MER kg 0,00E+00 0,00E+00 3,40E-05 0,00E+00
EEE MJ 0,00E+00 0,00E+00 2,41E-03 0,00E+00
ETE MJ 0,00E+00 0,00E+00 2,58E-02 0,00E+00
CR Components for reuse; MR Materials for recycling; MER Materials for energy recovery; EEE Exported electric energy; ETE Exported thermal
energy
Reading example: 9,0 E-03 = 9,0*10-3 = 0,009
NEPD-2669-1373-EN Flügger Dekso 5TM 7/9
Additional requirements
Greenhouse gas emissions from the use of electricity in the manufacturing phase
Nationalproductionmixfromimport,lowvoltage(productionoftransmissionlines,inadditiontodirectemissionsandlossesingrid)
of applied electricity for the manufacturing process (A3). Background data is presented inthe tablebelow. Characterisationfactors
from NS-EN 15804:2012+A1:2013 is used.
Electricity mix Data source Value Unit
Electricity, Denmark (kWh) ecoinvent 3.6 329 g CO -eq./kWh
2
Dangerous substances
The product contains no substances given by the REACH Candidate list or the Norwegian priority list
The product contains substances given by the REACH Candidate list <0,1 weight%
The product contains substances given by the REACH Candidate list or the Norwegian priority list, see table above
The product contains no substances given by the REACH Candidate list or the Norwegian priority list. The product is
characterised as hazardous waste (acc. to the Waste Directive, Appendix III), se table above.
Indoor environment
The declared product is emission tested according to the ISO-16000 series (2006).
NEPD-2669-1373-EN Flügger Dekso 5TM 8/9
Bibliography
BASTA (2020) Properties criteria - BASTA - in accordance with Regulation (EC) No 1272/2008 (CLP), ed. A2
BREEAM®NOR (2016) BREEAM-NOR for new contractions 2016, SD 5075NOR, version 1.1. The Norwegian Green Building
Council
Building Information Foundation (2017) M1 Emission Classification of Building Materials :Protocol for Chemical and Sensory Testing of
Building Materials”, v. 15.11.2017.
CEPE (2016) Raw materials LCI database for the European coatings and printing ink industries, v3.0
Ecoinvent (2019) Ecoinvent version 3.6, Swiss Centre of Life Cycle Inventories, Dübendorf, Switzerland
EU Directive 2004/42/CE The limitation of emissions of volatile organic compounds due to the use of organic solvents in
certain paints and varnishes and vehicle refinishing products
EU Ecolabel SE/044/002 - Flügger Dekso 5
IBU PCR Part B Requirements on the EPD for Coatings with organic binders. v1.7, January 2019
ISO 16000-series Indoor air standards for VOCs sampling and determination, i.e. 9 (2006)
ISO 14025:2010 Environmental labels and declarations - Type III environmental declarations - Principles and
procedures
ISO 21930:2017 Sustainability in buildings and civil engineering works - Core rules for environmental product
declarations of construction products and services
NS-EN 15804:2012+A1:2013 Environmental product declaration - Core rules for the product category of construction products
REACH Candidate List (2018) Candidate List of substances of very high concern for Authorisation IAW Article 59(10) of the REACH
Regulation
Technical Check List (A20) and Miljøgiftlisten, The Norwegian Environment Agency
Norwegian Priority List (2018)
Program operator and publisher phone: +47 977 22 020
The Norwegian EPD Foundation
Post Box 5250 Majorstuen, 0303 Oslo e-mail: post@epd-norge.no
Norway web www.epd-norge.no
Owner of the declaration phone: +47 23 30 21 90
Flügger Norway AS
Waldemar Thranes gate 84B e-mail: regulatoryaffairs@flugger.com
0175 Oslo, Norway web www.flugger.com
Author of the Life Cycle Assessment phone: +47 69 35 11 00
Mafalda Silva, Lars Tellnes & Gaylord Booto fax: +47 69 34 24 94
NORSUS AS e-mail: post@norsus.no
Stadion 4, 1671 Kråkerøy, Norge web www.norsus.no
NEPD-2669-1373-EN Flügger Dekso 5TM 9/9
