Environmental product declaration
in accordance with ISO 14025 and EN 15804+A2
Joint Mortar 60 / Joint Mortar 60 Winter
Owner of the declaration: Program operator:
Marlon Tørmørtel A/S The Norwegian EPD Foundation
Product: Declaration number:
Joint Mortar 60 / Joint Mortar 60 Winter
Registration number:
Declared unit:
1 kg Issue date:
This declaration is based on Product Category Rules: Valid to:
CEN Standard EN 15804:2012+A2:2019 serves as core
EPD software:
PCR
The Norwegian EPD Foundation LCAno EPD generator ID: 383801
NPCR 009:2021 Part B for Technical - Chemical products
for building and construction industry
1 / 11
General information
Product Owner of the declaration:
Joint Mortar 60 / Joint Mortar 60 Winter Marlon Tørmørtel A/S
Contact person: Bente Vesterager
Phone: +45 7575 4300
e-mail: marlon@marlon.dk
Program operator: Manufacturer:
The Norwegian EPD Foundation Marlon Tørmørtel A/S
Post Box 5250 Majorstuen, 0303 Oslo, Norway
Phone: +47 977 22 020
web: www.epd-norge.no
Declaration number: Place of production:
Marlon Tørmørtel A/S
Virkelyst 20
8740 Brædstrup, Denmark
This declaration is based on Product Category Rules: Management system:
CEN Standard EN 15804:2012+A2:2019 serves as core PCR ISO 9001
NPCR 009:2021 Part B for Technical - Chemical products for building
and construction industry
Statement of liability: Organisation no:
The owner of the declaration shall be liable for the underlying DK13254079
information and evidence. EPD Norway shall not be liable with respect
to manufacturer information, life cycle assessment data and
evidences.​
Declared unit: Issue date:
1 kg Joint Mortar 60 / Joint Mortar 60 Winter
Declared unit with option: Valid to:
A1-A3,A4,A5,C1,C2,C3,C4,D
Year of study:
2023
Functional unit: Comparability:
No functional unit declared EPD of construction products may not be comparable if they not
comply with EN 15804 and seen in a building context.
General information on verification of EPD from EPD tools: Development and verification of EPD:
Independent verification of data, other environmental information The declaration is created using EPD tool lca.tools ver EPD2022.03,
and the declaration according to ISO 14025:2010, § 8.1.3 and § 8.1.4. developed by LCA.no. The EPD tool is integrated in the company's
Verification of each EPD is made according to EPD-Norway’s management system, and has been approved by EPD Norway.
guidelines for verification and approval requiring that tools are i)
integrated into the company's environmental management system, ii) Developer of EPD: Bente Vesterager
the procedures for use of the EPD tool are approved by EPD-Norway,
Reviewer of company-specific input data and EPD: Maria Hosbjerg
and iii) the process is reviewed annually by an independent third
Christensen
party verifier. See Appendix G of EPD-Norway's General Programme
Instructions for further information on EPD tools
Verification of EPD tool: Approved:
Independent third party verification of the EPD tool, background data
and test-EPD in accordance with EPDNorway's procedures and
guidelines for verification and approval of EPD tools. NEPDT73
Third party verifier:
Linda Høibye, Life Cycle Assessment Consulting
(no signature required)
2 / 11
Product
Product description:
Marlon Joint Mortar 60 / Joint Mortar 60 Winter is a pre-mixed expanding dry mortar product that is simply mixed with water at the work site.
With its plastic consistency, Marlon Joint Mortar 60 /Joint Mortar 60 Winter is pumpable and easily mixed in an automatic mixing pump. Marlon
Joint Mortar is used for joining and grouting prefabricated concrete elements with both horizontal and vertical joints. For joining corners, concrete
element floors and similar tasks. See link for more information at: https://marlon.dk/catalog/product/view/id/15/s/elementfuge-60-100025025pp/
Product specification
EPD covers:
Item no 1000250 Joint Mortar 60
Item no 1000255 Joint Mortar 60 Winter
Materials Value Unit
Fillers/Aggregates 50-75 %
Binders 30-50 %
Additives 0-2 %
Packaging 2-3 %
Technical data:
Marlon Joint Mortar 60 / Joint Mortar 60 Winter is produced and declared according to Bulletin no. 5.
Joint Mortar 60: Compressive strength, 28 days > 64 MPa
Joint Mortar 60: Bending tensile strength, 28 days > 8 MPa
Joint Mortar 60 Winter: Compressive strength, 28 days > 50 MPa
Joint Mortar 60 Winter: Bending tensile strength, 28 days > 8 MPa
See all declared properties at: https://marlon.dk/.
Market:
Denmark
Reference service life, product
The reference service life of the product is similar to the service life of the building.
Reference service life, building
> 50 years.
LCA: Calculation rules
Declared unit:
1 kg Joint Mortar 60 / Joint Mortar 60 Winter
Cut-off criteria:
All major raw materials and all the essential energy is included. The production processes for raw materials and energy flows with very small
amounts (less than 1%) are not included. These cut-off criteria do not​ apply for hazardous materials and substances.
Allocation:
The allocation is made in accordance with the provisions of EN 15804. Incoming energy and water and waste production in-house is allocated
equally among all products through mass allocation. Effects of primary production of recycled materials is allocated to the main product in which
the material was used. The recycling process and transportation of the material is allocated to this analysis.
Data quality:
Specific data for the product composition are provided by the manufacturer. The data represent the production of the declared product and were
collected for EPD development in the year of study. Background data is based on EPDs according to EN 15804 and different LCA databases. The
data quality of the raw materials in A1 is presented in the table below.
Materials Source Data quality Year
Cement ecoinvent 3.6 Database 2019
Chemical ecoinvent 3.6 Database 2019
Fillers ecoinvent 3.6 Database 2019
Fillers ecoinvent 3.6 Database 2020
Packaging - Cardboard Modified ecoinvent 3.6 Database 2019
Packaging - Pallet Modified ecoinvent 3.6 Database 2019
Packaging - Plastic ecoinvent 3.6 Database 2019
Quartz sand ecoinvent 3.6 Database 2019
Rheology modifier ecoinvent 3.6 Database 2019
3 / 11
System boundaries (X=included, MND=module not declared, MNR=module not relevant)
Construction Beyond the system
Product stage Use stage End of life stage
installation stage boundaries
A1 A2 A3 A4 A5 B1 B2 B3 B4 B5 B6 B7 C1 C2 C3 C4 D
X X X X X MND MND MND MND MND MND MND X X X X X
System boundary:
All processes from raw material extraction, to production, transport to the construction site and assembly, are included in the analysis as well as
end of life stage and phases beyond the system boundary.
Additional technical information:
The product can be delivered in bulk, Big bag or plastic bags. The calculation includes data for plastic bags, as this is the most frequent used form
of packaging.
waR slairetam tropsnarT gnirutcafunaM tropsnarT ylbmessA e​sU ecnanetniaM riapeR tnemecalpeR tnemhsibrufeR lanoitarepO ygrene esu lanoitarepO esu retaw -eD noitcurtsnoc noitilomed tropsnarT etsaW gnissecorp lasopsiD -yrevoceR-esueR laitnetop-gnilcyceR
4 / 11
LCA: Scenarios and additional technical information
The following information describe the scenarios in the different modules of the EPD.
Capacity utilisation Value
Transport from production place to user (A4) Distance (km) Fuel/Energy Consumption Unit
(incl. return) % (Liter/tonne)
Truck, 16-32 tonnes, EURO 6 (km) - Europe 36,7 % 160 0,043 l/tkm 6,88
Assembly (A5) Unit Value
Electricity, Denmark (kWh) kWh/DU 0,01
Waste, concrete, to landfill (kg) kg/DU 0,02
Waste, packaging, corrugated board box, to
kg/DU 0,00
average treatment (kg) - A5, inkl. 85 km transp.
Waste, packaging, pallet, EUR wooden pallet,
reusable, average treatment (kg) - A5, inkl. 85 km kg 0,02
transp.
Waste, packaging, plastic film/bags (LDPE), to
kg/DU 0,00
average treatment (kg) - A5, inkl. 85 km transp.
Water, tap water (kg) kg/DU 0,17
De-construction demolition (C1) Unit Value
Demolition of building per kg of cement-based
kg/DU 1,00
product, C1 (kg)
Capacity utilisation Value
Transport to waste processing (C2) Distance (km) Fuel/Energy Consumption Unit
(incl. return) % (Liter/tonne)
Truck, 16-32 tonnes, EURO 5 (km) - Europe 36,7 % 50 0,044 l/tkm 2,20
Waste processing (C3) Unit Value
Waste treatment of cement-based product after
kg 0,90
demolition, C3 (kg)
Disposal (C4) Unit Value
Disposal of cement-based product in landfill (kg) kg 0,10
Benefits and loads beyond the system
Unit Value
boundaries (D)
Substitution of primary aggregates with crushed
kg 0,90
recycled cement-based products (kg)
5 / 11
LCA: Results
The LCA results are presented below for the declared unit defined on page 2 of the EPD document.
Environmental impact
Indicator Unit A1-A3 A4 A5 C1 C2 C3 C4 D
GWP-total kg CO2 -eq 3,83E-01 2,68E-02 3,96E-02 4,00E-03 8,54E-03 6,48E-04 8,22E-04 -2,10E-03
GWP-fossil kg CO2 -eq 4,17E-01 2,68E-02 4,96E-03 4,00E-03 8,53E-03 6,39E-04 8,20E-04 -2,06E-03
GWP-biogenic kg CO2 -eq -3,43E-02 1,11E-05 3,47E-02 7,50E-07 3,48E-06 5,52E-06 9,58E-07 -4,11E-05
GWP-luluc kg CO2 -eq 1,19E-04 9,52E-06 6,27E-06 3,15E-07 2,98E-06 8,84E-07 2,02E-07 -1,39E-06
ODP kg CFC11 -eq 1,94E-08 6,06E-09 2,67E-10 8,64E-10 1,95E-09 1,26E-10 3,11E-10 -3,75E-10
AP mol H+ -eq 1,34E-03 7,69E-05 2,02E-05 4,19E-05 3,49E-05 5,17E-06 7,30E-06 -1,85E-05
EP-FreshWater kg P -eq 5,67E-06 2,14E-07 3,76E-07 1,46E-08 6,70E-08 4,04E-08 9,30E-09 -5,48E-08
EP-Marine kg N -eq 4,77E-04 1,52E-05 3,66E-06 1,85E-05 1,03E-05 1,52E-06 2,71E-06 -6,43E-06
EP-Terrestial mol N -eq 4,35E-03 1,70E-04 5,03E-05 2,00E-04 1,14E-04 1,75E-05 2,99E-05 -7,56E-05
POCP kg NMVOC -eq 1,05E-03 6,52E-05 1,14E-05 5,57E-05 3,50E-05 4,68E-06 8,56E-06 -2,00E-05
ADP-minerals&metals1 kg Sb-eq 1,93E-06 7,39E-07 5,08E-08 6,14E-09 2,31E-07 8,11E-09 7,39E-09 -1,83E-07
ADP-fossil1 MJ 2,17E+00 4,04E-01 6,67E-02 5,51E-02 1,29E-01 1,98E-02 2,26E-02 -3,49E-02
WDP1 m3 7,90E+00 3,91E-01 9,81E-01 1,17E-02 1,23E-01 2,19E+00 1,39E-01 -1,63E+00
GWP-total = Global Warming Potential total; GWP-fossil = Global Warming Potential fossil fuels; GWP-biogenic = Global Warming Potential biogenic; GWP-luluc =
Global Warming Potential land use and land use change; ODP = Depletion potential of the stratospheric ozone layer; AP = Acidification potential, Accumulated
Exceedance; EP-freshwater = Eutrophication potential, fraction of nutrients reaching freshwater end compartment: EP-marine = Eutrophication potential, fraction of
nutrients reaching marine end compartment; EP-terrestrial = Eutrophication potential, Accumulated Exceedance; POCP = Formation potential of tropospheric ozone;
ADP-minerals&metals = Abiotic depletion potential for non-fossil resources; ADP-fossil = Abiotic depletion for fossil resources potential; WDP = Water (user)
deprivation potential, deprivation-weighted water consumption
"Reading example: 9,0 E-03 = 9,0*10-3 = 0,009"
*INA Indicator Not Assessed
1. The results of this environmental impact indicator shall be used with care as the uncertainties on these results are high or as there is limited experienced with the
indicator
Remarks to environmental impacts
6 / 11
Additional environmental impact indicators
Indicator Unit A1-A3 A4 A5 C1 C2 C3 C4 D
PM Disease incidence 8,35E-09 1,64E-09 1,28E-10 5,07E-09 6,14E-10 8,30E-11 1,56E-10 -3,95E-10
IRP2 kgBq U235 -eq 9,03E-03 1,77E-03 3,27E-04 2,40E-04 5,62E-04 3,33E-04 1,03E-04 -3,20E-04
ETP-fw1 CTUe 3,65E+00 3,00E-01 1,10E-01 3,01E-02 9,47E-02 1,41E-02 1,23E-02 -3,59E-02
HTP-c1 CTUh 7,00E-11 0,00E+00 2,00E-12 1,00E-12 0,00E+00 1,00E-12 1,00E-12 -2,00E-12
HTP-nc1 CTUh 3,39E-09 3,28E-10 7,60E-11 2,80E-11 1,02E-10 1,30E-11 9,00E-12 -4,40E-11
SQP1 dimensionless 1,67E+00 2,83E-01 1,10E-01 6,69E-03 8,87E-02 1,12E-02 8,69E-02 7,91E-02
PM = Particulate Matter emissions; IRP = Ionizing radiation – human health; ETP-fw = Eco toxicity – freshwater; HTP-c = Human toxicity – cancer effects; HTP-nc =
Human toxicity – non cancer effects; SQP = Potential Soil Quality Index (dimensionless)
"Reading example: 9,0 E-03 = 9,0*10-3 = 0,009"
*INA Indicator Not Assessed
1. The results of this environmental impact indicator shall be used with care as the uncertainties on these results are high or as there is limited experienced with the
indicator
2. This impact category deals mainly with the eventual impact of low dose ionizing radiation on human health of the nuclear fuel cycle. It does not consider effects due
to possible nuclear accidents, occupational exposure nor due to radioactive waste disposal in underground facilities. Potential ionizing radiation from the soil, from
radon and from some construction materials is also not measured by this indicator.
7 / 11
Resource use
Indicator Unit A1-A3 A4 A5 C1 C2 C3 C4 D
PERE MJ 2,73E-01 5,79E-03 5,09E-02 3,00E-04 1,82E-03 1,02E-02 8,08E-04 -8,16E-03
PERM MJ 3,17E-01 0,00E+00 -3,16E-01 0,00E+00 0,00E+00 0,00E+00 0,00E+00 0,00E+00
PERT MJ 5,90E-01 5,79E-03 3,43E-02 3,00E-04 1,82E-03 1,02E-02 8,08E-04 -8,16E-03
PENRE MJ 2,20E+00 4,05E-01 6,67E-02 5,51E-02 1,29E-01 1,99E-02 2,26E-02 -3,68E-02
PENRM MJ 3,41E-02 0,00E+00 0,00E+00 0,00E+00 0,00E+00 0,00E+00 0,00E+00 0,00E+00
PENRT MJ 2,23E+00 4,05E-01 6,67E-02 5,51E-02 1,29E-01 1,99E-02 2,26E-02 -3,68E-02
SM kg 1,26E-02 0,00E+00 0,00E+00 0,00E+00 0,00E+00 0,00E+00 0,00E+00 0,00E+00
RSF MJ 8,37E-03 2,07E-04 1,91E-03 0,00E+00 6,50E-05 0,00E+00 1,68E-05 -1,67E-04
NRSF MJ 2,42E-03 7,41E-04 2,58E-05 0,00E+00 2,32E-04 0,00E+00 3,62E-05 -1,71E-04
FW m3 2,33E-03 4,33E-05 3,57E-04 2,83E-06 1,35E-05 3,40E-05 2,78E-05 -1,28E-03
PERE = Use of renewable primary energy excluding renewable primary energy resources used as raw materials; PERM = Use of renewable primary energy resources used
as raw materials; PERT = Total use of renewable primary energy resources; PENRE = Use of non renewable primary energy excluding non-renewable primary energy
resources used as raw materials; PENRM = Use of non renewable primary energy resources used as raw materials; PENRT = Total use of non renewable primary energy
resources; SM = Use of secondary materials; RSF = Use of renewable secondary fuels; NRSF = Use of non-renewable secondary fuels; FW = Net use of fresh water
"Reading example: 9,0 E-03 = 9,0*10-3 = 0,009"
*INA Indicator Not Assessed
8 / 11
End of life - Waste
Indicator Unit A1-A3 A4 A5 C1 C2 C3 C4 D
HWD kg 4,14E-04 2,09E-05 7,93E-06 1,62E-06 6,56E-06 1,98E-06 0,00E+00 -8,40E-06
NHWD kg 2,03E-02 1,97E-02 2,16E-02 6,52E-05 6,15E-03 6,26E-05 1,00E-01 -2,55E-04
RWD kg 1,07E-05 2,76E-06 1,90E-07 3,82E-07 8,77E-07 2,10E-07 0,00E+00 -2,76E-07
HWD = Hazardous waste disposed; NHWD = Non-hazardous waste disposed; RWD = Radioactive waste disposed
"Reading example: 9,0 E-03 = 9,0*10-3 = 0,009"
*INA Indicator Not Assessed
End of life - Output flow
Indicator Unit A1-A3 A4 A5 C1 C2 C3 C4 D
CRU kg 0,00E+00 0,00E+00 0,00E+00 0,00E+00 0,00E+00 0,00E+00 0,00E+00 0,00E+00
MFR kg 0,00E+00 0,00E+00 5,09E-04 0,00E+00 0,00E+00 9,00E-01 0,00E+00 0,00E+00
MER kg 9,22E-04 0,00E+00 7,31E-06 0,00E+00 0,00E+00 0,00E+00 0,00E+00 0,00E+00
EEE MJ 5,70E-04 0,00E+00 4,98E-04 0,00E+00 0,00E+00 0,00E+00 0,00E+00 0,00E+00
EET MJ 8,62E-03 0,00E+00 7,54E-03 0,00E+00 0,00E+00 0,00E+00 0,00E+00 0,00E+00
CRU = Components for re-use; MFR = Materials for recycling; MER = Materials for energy recovery; EEE = Exported energy electrical; EET = Exported energy thermal
"Reading example: 9,0 E-03 = 9,0*10-3 = 0,009"
*INA Indicator Not Assessed
Biogenic Carbon Content
Indicator Unit At the factory gate
Biogenic carbon content in product kg C 4,84E-05
Biogenic carbon content in accompanying packaging kg C 9,40E-03
Note: 1 kg biogenic carbon is equivalent to 44/12 kg CO2
9 / 11
Additional requirements
Greenhouse gas emissions from the use of electricity in the manufacturing phase
National production mix from import, low voltage (production of transmission lines, in addition to direct emissions and losses in grid) of applied
electricity for the manufacturing process (A3).
Electricity mix Source Amount Unit
Electricity, Denmark (kWh) ecoinvent 3.6 338,20 g CO2-eq/kWh
Dangerous substances
The product contains no substances given by the REACH Candidate list.
Indoor environment
Additional Environmental Information
Additional environmental impact indicators required in NPCR Part A for construction products
Indicator Unit A1-A3 A4 A5 C1 C2 C3 C4 D
GWPIOBC kg CO2 -eq 4,23E-01 2,68E-02 6,37E-03 4,00E-03 8,54E-03 1,19E-03 0,00E+00 -2,20E-03
GWP-IOBC: Global warming potential calculated according to the principle of instantaneous oxidation. In order to increase the transparency of biogenic carbon​
contribution to climate impact, the indicator GWP-IOBC is required as it declares climate impacts calculated according to the principle of instantaneous oxidation.​
GWP-IOBC is also referred to as GWP-GHG in context to Swedish public procurement legislation.
10 / 11
Bibliography
ISO 14025:2010 Environmental labels and declarations - Type III environmental declarations - Principles and procedures.
ISO 14044:2006 Environmental management - Life cycle assessment - Requirements and guidelines.
EN 15804:2012+A2:2019 Environmental product declaration - Core rules for the product category of construction products.
ISO 21930:2017 Sustainability in buildings and civil engineering works - Core rules for environmental product declarations of construction
products.
ecoinvent v3, (2019) Allocation, cut-off by classification, Swiss Centre of Life Cycle Inventories.
Iversen et al., (2021) eEPD v2021.09 Background information for EPD generator tool system verification, LCA.no Report number: 07.21
Ruttenborg, M. and Iversen, O.M.K., (2023) EPD generator for NPCR009:2021, Part B for Technical - Chemical products, Background information
for EPD generator application and LCA data, LCA.no report number: 05.23.
NPCR Part A: Construction products and services. Ver. 2.0, 24.03.2021 EPD Norway.
NPCR 009 Part B for Technical - Chemical products for building and construction industry, Ver. 3.0, 06.10.2021, EPD Norway.
Program operator and publisher Phone: +47 977 22 020
The Norwegian EPD Foundation e-mail: post@epd-norge.no
Post Box 5250 Majorstuen, 0303 Oslo, Norway web: www.epd-norge.no
Owner of the declaration: Phone: +45 7575 4300
Marlon Tørmørtel A/S e-mail: marlon@marlon.dk
Virkelyst 20, 8740 Brædstrup web: https://marlon.dk/
Author of the Life Cycle Assessment Phone: +47 916 50 916
LCA.no AS e-mail: post@lca.no
Dokka 6A, 1671 web: www.lca.no
Developer of EPD generator Phone: +47 916 50 916
LCA.no AS e-mail: post@lca.no
Dokka 6B,1671 Kråkerøy web: www.lca.no
ECO Platform web: www.eco-platform.org
ECO Portal web: ECO Portal
11 / 11
