Environmental product declaration
in accordance with ISO 14025 and EN 15804+A2
Edge Floor, wool fabric
Owner of the declaration: Program operator:
Lintex AB The Norwegian EPD Foundation
Product: Declaration number:
Edge Floor, wool fabric
NEPD-8237-7897-EN
Declared unit:
1 pcs Registration number:
This declaration is based on Product Category Rules: NEPD-8237-7897-EN
CEN Standard EN 15804:2012+A2:2019 serves as core
Issue date: 26.11.2024
PCR
The Norwegian EPD Foundation NPCR 026:2022 Part B for Furniture Valid to: 26.11.2029
EPD software:
LCAno EPD generator ID: 486840
1 / 12
General information
Product Owner of the declaration:
Edge Floor, wool fabric Lintex AB
Contact person: Sara Gripstrand
Phone: +46 (0) 735 06 84 71
e-mail: sara.gripstrand@lintex.se
Program operator: Manufacturer:
The Norwegian EPD Foundation Lintex AB
Post Box 5250 Majorstuen, 0303 Oslo, Norway
Phone: +47 977 22 020
web: www.epd-norge.no
Declaration number: Place of production:
Lintex AB
NEPD-8237-7897-EN
Madesjövägen 17
382 45 Nybro, Sweden
This declaration is based on Product Category Rules: Management system:
CEN Standard EN 15804:2012+A2:2019 serves as core PCR ISO 14001
NPCR 026:2022 Part B for Furniture
Statement of liability: Organisation no:
The owner of the declaration shall be liable for the underlying 556295-1698
information and evidence. EPD Norway shall not be liable with respect
to manufacturer information, life cycle assessment data and
evidences.​
Declared unit: Issue date:
1 pcs Edge Floor, wool fabric
26.11.2024
Declared unit (cradle to gate) with option: Valid to:
A1-A3,A4,A5,B2,B3,B4,C1,C2,C3,C4,D 26.11.2029
Year of study:
2023
Functional unit: Comparability:
Edge Floor is a sound absorber suited for use in environments such EPD of construction products may not be comparable if they not
as schools, offices and conference premises. comply with EN 15804 and seen in a building context.
General information on verification of EPD from EPD tools: Development and verification of EPD:
Independent verification of data, other environmental information The declaration is created using EPD tool lca.tools ver EPD2022.03,
and the declaration according to ISO 14025:2010, § 8.1.3 and § 8.1.4. developed by LCA.no. The EPD tool is integrated in the company's
Verification of each EPD is made according to EPD-Norway’s management system, and has been approved by EPD Norway.
guidelines for verification and approval requiring that tools are i)
integrated into the company's environmental management system, ii) Developer of EPD: Karl Engdahl
the procedures for use of the EPD tool are approved by EPD-Norway,
Reviewer of company-specific input data and EPD: Sara Gripstrand
and iii) the process is reviewed annually by an independent third
party verifier. See Appendix G of EPD-Norway's General Programme
Instructions for further information on EPD tools
Verification of EPD tool: Approved:
Independent third party verification of the EPD tool, background data
and test-EPD in accordance with EPDNorway's procedures and
guidelines for verification and approval of EPD tools.
Third party verifier:
Elisabet Amat, GREENIZE projects
(no signature required)
2 / 12
Product
Product description:
Edge Floor is a sound absorber suited for use in environments such as schools, offices and conference premises. The product is available in twelve
standard sizes and in five standard fabrics. This EPD is based on Edge Floor in the size 1000x1500 mm with wool fabric, more sizes can be found
under "Variants" on page 11.
Find out more on the webpage: https://www.lintex.com/en/products/office-screens/edge-floor-screen
Product specification
Edge Floor consists of a solid wooden frame filled with a sound-absorbent, 50% post-consumer recycled filling and covered by a wool fabric. Inner
fittings and screws are made of steel.
Recycled share in Recycled share in
Materials kg %
material (kg) material (%)
Rubber, synthetic 0,44 3,93 0,00 0,00
Textile - Wool 0,99 8,87 0,11 11,20
Wood - Solid pine 8,25 74,14 0,00 0,00
Metal - Steel 0,08 0,75 0,00 0,00
Polyester filling 1,37 12,31 0,69 50,00
Total 11,13 100,00 0,80
Recycled share in Recycled share in
Packaging kg %
material (kg) material (%)
Packaging -
1,45 49,59 0,87 60,00
Cardboard
Packaging - Pallet 1,46 49,73 0,00 0,00
Packaging - Plastic
0,02 0,68 0,00 0,00
straps
Total incl.
14,06 100,00 1,67
packaging
Technical data:
Size 1000x1500 mm. 40 mm sound absorbent filling. The product is available in twelve different sizes.
Edge Floor is labelled with FSC (R) Mix (FSC-C170086), Möbelfakta (ID 0120141120)
It is tested and approved according to quality standard EN 1023:2000-1,2,3 and sound absorption standards SS-EN ISO 354:2003, SS
25269:2013 and ISO 20189:2018
Market:
Europe
Reference service life, product
15
Reference service life, building
LCA: Calculation rules
Declared unit:
1 pcs Edge Floor, wool fabric
Cut-off criteria:
All major raw materials and all the essential energy is included. The production processes for raw materials and energy flows with very small
amounts (less than 1%) are not included. These cut-off criteria do not apply for hazardous materials and substances.
Allocation:
The allocation is made in accordance with the provisions of EN 15804. Incoming energy and water and waste production in-house is allocated
equally among all products through mass allocation. Effects of primary production of recycled materials is allocated to the main product in which
the material was used. The recycling process and transportation of the material is allocated to this analysis.
Data quality:
Specific data for the product composition are provided by the manufacturer. They represent the production of the declared product and were
collected for EPD development in the year of study. Background data is based on registered EPDs according to EN 15804, Ostfold Research
databases, ecoinvent and other LCA databases. The data quality of the raw materials in A1 is presented in the table below.​
3 / 12
Materials Source Data quality Year
Metal - Steel ecoinvent 3.6 Database 2019
Packaging - Cardboard Modified ecoinvent 3.6 Database 2019
Packaging - Pallet ecoinvent 3.6 Database 2019
Packaging - Plastic straps ecoinvent 3.6 Database 2019
Polyester filling ecoinvent 3.6 Database 2019
Polyester filling Modified ecoinvent 3.6 Database 2019
Rubber, synthetic ecoinvent 3.6 Database 2019
Textile - Wool MD-23110-EN_rev1 EPD 2021
Wood - Solid pine modified ecoinvent 3.6 Database 2019
4 / 12
System boundaries (X=included, MND=module not declared, MNR=module not relevant)
Construction Beyond the system
Product stage Use stage End of life stage
installation stage boundaries
A1 A2 A3 A4 A5 B1 B2 B3 B4 B5 B6 B7 C1 C2 C3 C4 D
X X X X X MND X X X MND MND MND X X X X X
System boundary:
Product stage – Raw materials A1
Lintex has long term relations with its suppliers, with a continuous dialogue about environmental performance of extracting and producing raw
materials and components.
All wood based material is labeled with FSC ® (FSC-C170086) and standards fabrics are EU Ecolabel or Oekotex.
Waste and energy use at the suppliers are included in A1, as well as production of packaging material.
Product stage – Transport A2
Transports are done by truck and/or ship from the supplier to Lintex manufacturing site in Nybro, Sweden.
Product stage – Manufacturing A3
Manufacturing takes place in Nybro, Sweden and includes cutting, assembling and packaging.
Additional technical information:
Edge Floor is labelled with FSC (R) Mix (FSC-C170086) and Möbelfakta (ID 0120141120). With the standard fabrics Blazer lite and Cura Screen
Edge Floor is labeled with EU Ecolabel (SE/049/002).
It is tested and approved according to quality standard EN 1023:2000-1,2,3 and sound absorption standards SS-EN ISO 354:2003, SS 25269:2013
and ISO 20189:2018
Edge Floor is possible to separate down to different materials, that may be material recycled accordingly. Spare parts in the form of wall fittings are
available.
For mounting instructions and information on care and maintenance please visit https://www.lintex.com/en/products/office-screens/edge-floor-
screen/
Lintex AB is certified according to ISO 14001:2015 and FSC Chain of Custody (DNV-COC-002282). The production is loacted in Nybro, Sweden.
Due to 4400 solar panels on the factory roof producing approximately 1 600 MWh per year, Lintex is a net producer of renewable energy (the
yearly production is higher than the consumtion).
Read more about the company's sustainability work at www.lintex.com/sustainability.
waR slairetam tropsnarT gnirutcafunaM tropsnarT ylbmessA e​sU ecnanetniaM riapeR tnemecalpeR tnemhsibrufeR lanoitarepO ygrene esu lanoitarepO esu retaw -eD noitcurtsnoc noitilomed tropsnarT etsaW gnissecorp lasopsiD -yrevoceR-esueR laitnetop-gnilcyceR
5 / 12
LCA: Scenarios and additional technical information
The following information describe the scenarios in the different modules of the EPD.
Installation stage – Transport A4
The main market for Edge Floor is Scandinavia, why a distance of 700 km has been used as an approximation of transport from the factory in
Nybro to the end user.
Installation stage – Assembly A5
When arriving at the end user the products are unpacked. Environmental impact of the packaging material is included in A5. Mounting of the
product is done by hand with simple tools.
User stage - B1-B7:
In the user stage the product doesn’t consume any energy or other resources. If needed, the product may be vacuum cleaned. During normal use
the product doesn’t need to be repaired or refurbished.
End-of-life stage - C1-C4:
The end-of-life stage covers deconstruction, transport to a waste processing site, processing and disposal of waste. The LCA tool calculates this
based on material in the product and generic numbers, including an 85 kilometers transport to the waste management plant.
Beyond the system boundaries, Re-use - Recovery - Recycling -potential - D:
LCA-tool is calculating stage D potential based on material recycling and resource for energy production from materials if product end of lifecycle
would be in Norway. Material amounts are calculated based on the material used to make the product.
Capacity utilisation Value
Transport from production place to user (A4) Distance (km) Fuel/Energy Consumption Unit
(incl. return) % (Liter/tonne)
Truck, 16-32 tonnes, EURO 6 (km) 36,7 % 700 0,043 l/tkm 30,10
Assembly (A5) Unit Value
Waste, packaging, PET straps, to average
kg 0,02
treatment - A5 (kg)
Waste, packaging, cardboard, 100 % recycled, to
kg 0,87
average treatment (kg)
Waste, packaging, corrugated board box, 0 %
kg 0,58
recycled, to average treatment (kg)
Waste, packaging, Pallet, EUR wooden pallet,
kg 1,46
single use, average treatment (kg)
Capacity utilisation Value
Transport to waste processing (C2) Distance (km) Fuel/Energy Consumption Unit
(incl. return) % (Liter/tonne)
Truck, over 32 tonnes, EURO 6 (km) 53,3 % 85 0,023 l/tkm 1,96
Waste processing (C3) Unit Value
Waste, materials to recycling (kg) kg 0,03
Waste treatment per kg Scrap steel, incineration
kg 0,08
with fly ash extraction (kg)
Waste treatment per kg Textile, incineration with
kg 2,36
fly ash extraction (kg)
Waste treatment per kg Rubber, municipal
kg 0,44
incineration with fly ash extraction (kg)
Disposal (C4) Unit Value
Landfilling of ashes and residues from
kg 0,06
incineration of Scrap steel (kg)
Landfilling of ashes from incineration of Textile,
kg 0,12
soiled, process per kg ashes and residues (kg)
Landfilling of ashes from incineration of Rubber,
kg 0,02
process per kg ashes and residues - C4 (kg)
Benefits and loads beyond the system
Unit Value
boundaries (D)
Substitution of primary steel with net scrap (kg) kg 0,01
Substitution of electricity (MJ) MJ 2,73
Substitution of thermal energy, district heating
MJ 41,35
(MJ)
6 / 12
LCA: Results
The LCA results are presented below for the declared unit defined on page 2 of the EPD document.
Environmental impact
Indicator Unit A1-A3 A4 A5 B2 B3
GWP-total kg CO2 -eq 1,60E+01 1,62E+00 4,74E+00 0 0
GWP-fossil kg CO2 -eq 3,33E+01 1,62E+00 6,43E-02 0 0
GWP-biogenic kg CO2 -eq -1,75E+01 6,69E-04 4,67E+00 0 0
GWP-luluc kg CO2 -eq 1,22E-01 5,75E-04 1,79E-05 0 0
ODP kg CFC11 -eq 1,98E-06 3,66E-07 1,13E-08 0 0
AP mol H+ -eq 1,26E-01 4,64E-03 4,28E-04 0 0
EP-FreshWater kg P -eq 1,18E-03 1,29E-05 6,66E-07 0 0
EP-Marine kg N -eq 2,77E-02 9,19E-04 1,74E-04 0 0
EP-Terrestial mol N -eq 3,92E-01 1,03E-02 1,85E-03 0 0
POCP kg NMVOC -eq 9,93E-02 3,94E-03 4,89E-04 0 0
ADP-minerals&metals1 kg Sb-eq 1,51E-03 4,46E-05 1,22E-06 0 0
ADP-fossil1 MJ 5,93E+02 2,44E+01 7,96E-01 0 0
WDP1 m3 9,39E+03 2,36E+01 1,15E+00 0 0
Indicator Unit B4 C1 C2 C3 C4 D
GWP-total kg CO2 -eq 0 0 1,05E-01 2,03E+01 7,42E-03 -7,80E-01
GWP-fossil kg CO2 -eq 0 0 1,05E-01 1,50E+00 7,40E-03 -7,53E-01
GWP-biogenic kg CO2 -eq 0 0 4,48E-05 1,88E+01 1,84E-05 -1,54E-03
GWP-luluc kg CO2 -eq 0 0 3,19E-05 2,54E-05 1,21E-06 -2,56E-02
ODP kg CFC11 -eq 0 0 2,52E-08 1,34E-08 8,97E-10 -5,41E-02
AP mol H+ -eq 0 0 3,37E-04 1,85E-03 2,79E-05 -6,17E-03
EP-FreshWater kg P -eq 0 0 8,32E-07 2,44E-06 9,81E-08 -6,66E-05
EP-Marine kg N -eq 0 0 7,38E-05 8,70E-04 8,86E-06 -2,01E-03
EP-Terrestial mol N -eq 0 0 8,23E-04 9,27E-03 1,00E-04 -2,17E-02
POCP kg NMVOC -eq 0 0 3,23E-04 2,27E-03 2,79E-05 -6,02E-03
ADP-minerals&metals1 kg Sb-eq 0 0 1,86E-06 6,66E-07 4,74E-08 -7,57E-06
ADP-fossil1 MJ 0 0 1,70E+00 1,18E+00 7,44E-02 -1,07E+01
WDP1 m3 0 0 1,30E+00 1,91E+00 6,72E-01 -1,32E+02
GWP-total = Global Warming Potential total; GWP-fossil = Global Warming Potential fossil fuels; GWP-biogenic = Global Warming Potential biogenic; GWP-luluc =
Global Warming Potential land use and land use change; ODP = Depletion potential of the stratospheric ozone layer; AP = Acidification potential, Accumulated
Exceedance; EP-freshwater = Eutrophication potential, fraction of nutrients reaching freshwater end compartment: EP-marine = Eutrophication potential, fraction of
nutrients reaching marine end compartment; EP-terrestrial = Eutrophication potential, Accumulated Exceedance; POCP = Formation potential of tropospheric ozone;
ADP-minerals&metals = Abiotic depletion potential for non-fossil resources; ADP-fossil = Abiotic depletion for fossil resources potential; WDP = Water (user)
deprivation potential, deprivation-weighted water consumption
"Reading example: 9,0 E-03 = 9,0*10-3 = 0,009"
*INA Indicator Not Assessed
1. The results of this environmental impact indicator shall be used with care as the uncertainties on these results are high or as there is limited experienced with the
indicator
Remarks to environmental impacts
7 / 12
Additional environmental impact indicators
Indicator Unit A1-A3 A4 A5 B2 B3
PM Disease incidence 1,58E-06 9,89E-08 5,53E-09 0 0
IRP2 kgBq U235 -eq 4,04E+00 1,07E-01 3,10E-03 0 0
ETP-fw1 CTUe 5,30E+02 1,81E+01 9,69E-01 0 0
HTP-c1 CTUh 2,04E-08 0,00E+00 7,10E-11 0 0
HTP-nc1 CTUh 9,73E-07 1,98E-08 3,35E-09 0 0
SQP1 dimensionless 1,81E+03 1,71E+01 4,90E-01 0 0
Indicator Unit B4 C1 C2 C3 C4 D
PM Disease incidence 0 0 9,61E-09 1,84E-08 3,68E-10 -3,72E-07
IRP2 kgBq U235 -eq 0 0 7,43E-03 2,43E-03 3,44E-04 -6,78E-02
ETP-fw1 CTUe 0 0 1,24E+00 4,51E+00 1,22E-01 -5,84E+01
HTP-c1 CTUh 0 0 0,00E+00 3,86E-10 5,00E-12 -1,11E-09
HTP-nc1 CTUh 0 0 1,20E-09 1,92E-08 2,19E-10 -5,43E-08
SQP1 dimensionless 0 0 1,95E+00 1,83E-01 2,11E-01 -7,10E+01
PM = Particulate Matter emissions; IRP = Ionizing radiation – human health; ETP-fw = Eco toxicity – freshwater; HTP-c = Human toxicity – cancer effects; HTP-nc =
Human toxicity – non cancer effects; SQP = Soil Quality (dimensionless)
"Reading example: 9,0 E-03 = 9,0*10-3 = 0,009"
*INA Indicator Not Assessed
1. The results of this environmental impact indicator shall be used with care as the uncertainties on these results are high or as there is limited experienced with the
indicator
2. This impact category deals mainly with the eventual impact of low dose ionizing radiation on human health of the nuclear fuel cycle. It does not consider effects due
to possible nuclear accidents, occupational exposure nor due to radioactive waste disposal in underground facilities. Potential ionizing radiation from the soil, from
radon and from some construction materials is also not measured by this indicator.
8 / 12
Resource use
Indicator Unit A1-A3 A4 A5 B2 B3
PERE MJ 3,53E+02 3,50E-01 1,50E-02 0 0
PERM MJ 1,69E+02 0,00E+00 -3,46E+01 0 0
PERT MJ 5,22E+02 3,50E-01 -3,45E+01 0 0
PENRE MJ 5,59E+02 2,44E+01 7,96E-01 0 0
PENRM MJ 4,70E+01 0,00E+00 -4,59E-01 0 0
PENRT MJ 6,06E+02 2,44E+01 3,37E-01 0 0
SM kg 1,67E+00 0,00E+00 0,00E+00 0 0
RSF MJ 4,10E-01 1,25E-02 4,60E-04 0 0
NRSF MJ 8,92E-01 4,47E-02 3,89E-03 0 0
FW m3 5,50E-01 2,61E-03 4,94E-04 0 0
Indicator Unit B4 C1 C2 C3 C4 D
PERE MJ 0 0 2,14E-02 4,39E-02 3,87E-03 -6,56E+01
PERM MJ 0 0 0,00E+00 -1,21E+02 0,00E+00 0,00E+00
PERT MJ 0 0 2,14E-02 -1,21E+02 3,87E-03 -6,56E+01
PENRE MJ 0 0 1,70E+00 1,21E+00 7,46E-02 -1,07E+01
PENRM MJ 0 0 0,00E+00 -4,65E+01 0,00E+00 0,00E+00
PENRT MJ 0 0 1,70E+00 -4,53E+01 7,46E-02 -1,07E+01
SM kg 0 0 0,00E+00 0,00E+00 0,00E+00 0,00E+00
RSF MJ 0 0 7,48E-04 1,03E-03 9,65E-05 -1,11E-02
NRSF MJ 0 0 2,51E-03 0,00E+00 3,11E-02 -3,88E+00
FW m3 0 0 1,93E-04 3,54E-03 6,82E-05 -7,91E-02
PERE = Use of renewable primary energy excluding renewable primary energy resources used as raw materials; PERM = Use of renewable primary energy resources used
as raw materials; PERT = Total use of renewable primary energy resources; PENRE = Use of non renewable primary energy excluding non-renewable primary energy
resources used as raw materials; PENRM = Use of non renewable primary energy resources used as raw materials; PENRT = Total use of non renewable primary energy
resources; SM = Use of secondary materials; RSF = Use of renewable secondary fuels; NRSF = Use of non-renewable secondary fuels; FW = Net use of fresh water
"Reading example: 9,0 E-03 = 9,0*10-3 = 0,009"
*INA Indicator Not Assessed
9 / 12
End of life - Waste
Indicator Unit A1-A3 A4 A5 B2 B3
HWD kg 1,04E-01 1,26E-03 0,00E+00 0 0
NHWD kg 4,66E+00 1,19E+00 2,93E+00 0 0
RWD kg 6,54E-03 1,66E-04 0,00E+00 0 0
Indicator Unit B4 C1 C2 C3 C4 D
HWD kg 0 0 9,30E-05 0,00E+00 1,45E-01 -5,52E-04
NHWD kg 0 0 1,48E-01 0,00E+00 5,12E-02 -2,55E-01
RWD kg 0 0 1,16E-05 0,00E+00 4,05E-07 -5,56E-05
HWD = Hazardous waste disposed; NHWD = Non-hazardous waste disposed; RWD = Radioactive waste disposed
"Reading example: 9,0 E-03 = 9,0*10-3 = 0,009"
*INA Indicator Not Assessed
End of life - Output flow
Indicator Unit A1-A3 A4 A5 B2 B3
CRU kg 0,00E+00 0,00E+00 0,00E+00 0 0
MFR kg 2,99E-01 0,00E+00 1,36E+00 0 0
MER kg 5,56E-01 0,00E+00 1,44E+00 0 0
EEE MJ 3,82E-01 0,00E+00 1,09E+00 0 0
EET MJ 5,78E+00 0,00E+00 1,65E+01 0 0
Indicator Unit B4 C1 C2 C3 C4 D
CRU kg 0 0 0,00E+00 0,00E+00 0,00E+00 0,00E+00
MFR kg 0 0 0,00E+00 2,85E-02 0,00E+00 0,00E+00
MER kg 0 0 0,00E+00 1,11E+01 0,00E+00 0,00E+00
EEE MJ 0 0 0,00E+00 7,98E+00 0,00E+00 0,00E+00
EET MJ 0 0 0,00E+00 1,21E+02 0,00E+00 0,00E+00
CRU = Components for re-use; MFR = Materials for recycling; MER = Materials for energy recovery; EEE = Exported energy electrical; EET = Exported energy thermal
"Reading example: 9,0 E-03 = 9,0*10-3 = 0,009"
*INA Indicator Not Assessed
Biogenic Carbon Content
Indicator Unit At the factory gate
Biogenic carbon content in product kg C 4,63E+00
Biogenic carbon content in accompanying packaging kg C 1,27E+00
Note: 1 kg biogenic carbon is equivalent to 44/12 kg CO2
10 / 12
Additional requirements
Greenhouse gas emissions from the use of electricity in the manufacturing phase
National production mix from import, low voltage (production of transmission lines, in addition to direct emissions and losses in grid) of applied
electricity for the manufacturing process (A3).
Electricity mix Source Amount Unit
Electricity, Sweden (kWh) ecoinvent 3.6 54,94 g CO2-eq/kWh
Dangerous substances
The product contains no substances given by the REACH Candidate list.
Indoor environment
Additional Environmental Information
Key Environmental Indicators
Key environmental indicators Unit A1-A3 A4 A1-C4 A1-D
GWPtotal kg CO2 -eq 15,98 1,62 42,77 41,99
Total energy consumption MJ 912,94 24,84 941,68 861,45
Amount of recycled materials % 11,86
Additional environmental impact indicators required in NPCR Part A for construction products
Indicator Unit A1-A3 A4 A5 B2 B3
GWPIOBC kg CO2 -eq 3,37E+01 1,62E+00 6,43E-02 0 0
Indicator Unit B4 C1 C2 C3 C4 D
GWPIOBC kg CO2 -eq 0 0 1,05E-01 5,36E+00 1,47E-02 -7,74E-01
GWP-IOBC: Global warming potential calculated according to the principle of instantaneous oxidation. In order to increase the transparency of biogenic carbon
contribution to climate impact, the indicator GWP-IOBC is required as it declares climate impacts calculated according to the principle of instantaneous oxidation.
GWP-IOBC is also referred to as GWP-GHG in context to Swedish public procurement legislation.
Variants and Options
Key environmental indicators (A1-A3) for variants of this EPD
Variants Weight (kg) GWPtotal (kg CO2 -eq) Total energy consumption (MJ) Amount of recycled materials (%)
Edge Floor, wool fabric, 800x1350 mm 10,64 13,22 712,84 10,71
Edge Floor, wool fabric, 800x1500 mm 12,33 12,12 780,33 10,21
Edge Floor, wool fabric, 800x1650 mm 13,78 16,32 884,49 10,56
Edge Floor, wool fabric, 800x1800 mm 14,62 18,06 945,77 10,85
Edge Floor, wool fabric, 1000x1350 mm 12,08 17,27 830,53 12,57
Edge Floor, wool fabric, 1000x1650 mm 15,49 25,05 1089,74 11,47
Edge Floor, wool fabric, 1000x1800 mm 16,40 27,59 1178,63 12,67
Edge Floor, wool fabric, 1200x1350 mm 14,32 20,22 955,57 11,75
Edge Floor, wool fabric, 1200x1500 mm 16,73 18,71 1051,56 11,10
Edge Floor, wool fabric, 1200x1650 mm 17,94 26,04 1211,97 11,55
Edge Floor, wool fabric, 1200x1800 mm 18,89 29,12 1295,38 12,02
Edge Floor, wool fabric, 1400x1500 mm 18,44 22,42 1187,45 12,60
Key environmental indicators (A1-A3) for options for this EPD
Options Weight (kg) GWPtotal (kg CO2 -eq) Total energy consumption (MJ) Amount of recycled materials (%)
Slim foot 0,31 5,26 65,24 24,55
Blade foot 0,67 12,76 155,70 30,15
Arc foot 0,61 11,51 140,60 30,78
11 / 12
Bibliography
ISO 14025:2010 Environmental labels and declarations - Type III environmental declarations - Principles and procedures.
ISO 14044:2006 Environmental management - Life cycle assessment - Requirements and guidelines.
EN 15804:2012+A2:2019 Environmental product declaration - Core rules for the product category of construction products.
ISO 21930:2017 Sustainability in buildings and civil engineering works - Core rules for environmental product declarations of construction
products.
ecoinvent v3, Allocation, cut-off by classification, Swiss Centre of Life Cycle Inventories.
Iversen et al., (2021) eEPD v2021.09 Background information for EPD generator tool system verification, LCA.no Report number: 07.21
Ruud et al., (2023) EPD generator for NPCR026 Part B for Furniture - Background information for EPD generator application and LCA data,
LCA.no report number 01.23
NPCR Part A: Construction products and services. Ver. 2.0. March 2021, EPD-Norge.
NPCR 026 Part B for Furniture. Ver. 2.0 March 2022, EPD-Norge.
Program operator and publisher Phone: +47 977 22 020
The Norwegian EPD Foundation e-mail: post@epd-norge.no
Post Box 5250 Majorstuen, 0303 Oslo, Norway web: www.epd-norge.no
Owner of the declaration: Phone: +46 (0) 735 06 84 71
Lintex AB e-mail: sara.gripstrand@lintex.se
Madesjövägen 17, 382 45 Nybro, Sweden web:
Author of the Life Cycle Assessment Phone: +47 916 50 916
LCA.no AS e-mail: post@lca.no
Dokka 6A, 1671 Kråkerøy, Norway web: www.lca.no
Developer of EPD generator Phone: +47 916 50 916
LCA.no AS e-mail: post@lca.no
Dokka 6A, 1671 Kråkerøy, Norway web: www.lca.no
ECO Platform web: www.eco-platform.org
ECO Portal web: ECO Portal
12 / 12
