Environmental product declaration
in accordance with ISO 14025 and EN 15804+A2
Senso 3 seat sofa - Pall
Owner of the declaration: Program operator:
Fora Form AS The Norwegian EPD Foundation
Product: Declaration number:
Senso 3 seat sofa - Pall
Registration number:
Declared unit:
1 pcs Issue date:
This declaration is based on Product Category Rules: Valid to:
CEN Standard EN 15804:2012+A2:2019 serves as core
EPD software:
PCR
The Norwegian EPD Foundation LCAno EPD generator ID: 403072
NPCR 026:2022 Part B for Furniture
1 / 12
General information
Product Owner of the declaration:
Senso 3 seat sofa - Pall Fora Form AS
Contact person: Kåre Sætre
Phone: +47 700 46 000
e-mail: info@foraform.com
Program operator: Manufacturer:
The Norwegian EPD Foundation Fora Form AS
Post Box 5250 Majorstuen, 0303 Oslo, Norway Mosflatevegen
Phone: +47 977 22 020 6154 Ørsta, Norway
web: www.epd-norge.no
Declaration number: Place of production:
POD Furniture UAB
Labrencu Dvaro g. 2
LT-92291 Klaipeda, Lithuania
This declaration is based on Product Category Rules: Management system:
CEN Standard EN 15804:2012+A2:2019 serves as core PCR NS-EN ISO 14001: 2015 No. 800406.NS-EN ISO 9001: 2015 No.
NPCR 026:2022 Part B for Furniture 901268.NS-EN ISO 45001: 2018 No 907167.
Statement of liability: Organisation no:
The owner of the declaration shall be liable for the underlying 986 581 421
information and evidence. EPD Norway shall not be liable with respect
to manufacturer information, life cycle assessment data and
evidences.​
Declared unit: Issue date:
1 pcs Senso 3 seat sofa - Pall
Declared unit (cradle to gate) with option: Valid to:
A1-A3,A4,A5,B1,B2,C1,C2,C3,C4,D
Year of study:
2023
Functional unit: Comparability:
Production of one furniture solution provided and maintained for a EPD of construction products may not be comparable if they not
period of 15 years. comply with EN 15804 and seen in a building context.
General information on verification of EPD from EPD tools: Development and verification of EPD:
Independent verification of data, other environmental information The declaration is created using EPD tool lca.tools ver EPD2022.03,
and the declaration according to ISO 14025:2010, § 8.1.3 and § 8.1.4. developed by LCA.no. The EPD tool is integrated in the company's
Verification of each EPD is made according to EPD-Norway’s management system, and has been approved by EPD Norway.
guidelines for verification and approval requiring that tools are i)
integrated into the company's environmental management system, ii) Developer of EPD: Kåre Sætre
the procedures for use of the EPD tool are approved by EPD-Norway,
Reviewer of company-specific input data and EPD: Katrine Østgaard
and iii) the process is reviewed annually by an independent third
party verifier. See Appendix G of EPD-Norway's General Programme
Instructions for further information on EPD tools
Verification of EPD tool: Approved:
Independent third party verification of the EPD tool, background data
and test-EPD in accordance with EPDNorway's procedures and
guidelines for verification and approval of EPD tools.
Third party verifier:
Elisabet Amat, GREENIZE projects
(no signature required)
2 / 12
Product
Product description:
Senso sofa system was designed by the design duo Anderssen & Voll. The idea behind the design is a modular sofa system that is flexible, narrow
and appeals to informal meetings between people. Senso sofa system takes into account the acoustic challenges you encounter in office
environments. Senso is designed to enable and inhibit interaction and letting the space decide how what interaction you desire. From work zones
that require quiet reflextion and working alone to building bigger set ups specifically for great conversations. The module system stands out in
that it is very narrow and offers a large number of modules that provide opportunities for creative solutions. The seat height ensures
requirements for universal design met. Senso is available with a 10 mm cleaning gap between seat and backrest. This is called Senso Café.
Product specification
Furniture approval NS-EN 16139:2013 / Level 1
This EPD includes these variants :
Senso 3 seat pall - Senso 3 seat low back/corner - Senso 3 seat high back/corner
Recycled
Recycled share in share in
Materials kg %
material (kg) material
(%)
Glass fibre 0,15 0,56 0,00 0,00
Metal - Aluminium 2,38 8,86 1,19 50,00
Metal - Steel 13,53 50,37 2,71 20,00
Plastic -
Polyoxymethylene 0,10 0,37 0,00 0,00
(POM)
Plastic - Polyurethane
6,21 23,12 0,00 0,00
(PUR)
Textile - Wool 3,99 14,85 0,00 0,00
Wood - Plywood 0,50 1,86 0,00 0,00
Total 26,86 100,00 3,90
Recycled
Recycled share in share in
Packaging kg %
material (kg) material
(%)
Recycled cardboard 2,00 100,00 2,00 100,00
Total incl. packaging 28,86 100,00 5,90
Technical data:
Lenght 1950mm
Depht 630mm
Seat hight 460mm
Weight Senso 3 seat sofa pall 26,86 kg whithout packaging
Seat hight BAR modell 650mm
Market:
The product is available worldwide
The distanse from production site in Lithauen to customer is stipulated to be an average of 1050km
Reference service life, product
At least 15 years,with a 5-year warranty and a 10-year spare part guarantee
Reference service life, building
If the furniture should become worn after a long life, Fora Form offers to renew the furniture. It's called Reform. The expected lifespan of the
furniture is, using Reform, 50 - 60 years
LCA: Calculation rules
Declared unit:
1 pcs Senso 3 seat sofa - Pall
Cut-off criteria:
All major raw materials and all the essential energy is included. The production processes for raw materials and energy flows with very small
amounts (less than 1%) are not included. These cut-off criteria do not apply for hazardous materials and substances.
Allocation:
3 / 12
The allocation is made in accordance with the provisions of EN 15804. Incoming energy and water and waste production in-house is allocated
equally among all products through mass allocation. Effects of primary production of recycled materials is allocated to the main product in which
the material was used. The recycling process and transportation of the material is allocated to this analysis.
Data quality:
Specific data for the product composition are provided by the manufacturer. They represent the production of the declared product and were
collected for EPD development in the year of study. Background data is based on registered EPDs according to EN 15804, Ostfold Research
databases, ecoinvent and other LCA databases. The data quality of the raw materials in A1 is presented in the table below.​
Materials Source Data quality Year
Glass fibre ecoinvent 3.6 Database 2019
Metal - Aluminium ecoinvent 3.6 Database 2019
Metal - Steel ecoinvent 3.6 Database 2019
Plastic - Polyoxymethylene (POM) ecoinvent 3.6 Database 2019
Plastic - Polyurethane (PUR) ecoinvent 3.6 Database 2019
Recycled cardboard Modified ecoinvent 3.6 Database 2019
Textile - Wool Modified ecoinvent 3.6 Database 2019
Wood - Plywood modified ecoinvent 3.6 Database 2019
4 / 12
System boundaries (X=included, MND=module not declared, MNR=module not relevant)
Construction Beyond the system
Product stage Use stage End of life stage
installation stage boundaries
A1 A2 A3 A4 A5 B1 B2 B3 B4 B5 B6 B7 C1 C2 C3 C4 D
X X X X X X X MND MND MND MND MND X X X X X
System boundary:
Additional technical information:
We want you to enjoy your furniture for many years to come. If you follow our advice in our’s Quality and Maintenance manual you contribute to
prolonged life of your furniture. We use as far as possible environmentally friendly materials and processes in our manufacturing unit in Lithauen.
Our goal is to manufacture furniture that can last for generations. All furniture made by Fora Form are made of FSC certified wood, manufactured
according to ISO 14001, and has an EPD on all products. This ensures sustainability and a “cradle to cradle” philosophy. We actively work to reduce
waste. All pa For a Form collaborate with Norsk Gjenvinning and Grønt Punkt (Green Dot Norway plc) regarding recycling of used packing
materials. All wood is FSC certified.
Norwegian and Swedish Møbelfakta are accredited test facilities where furniture quality, strength, durability, flammability, safety, emissions and
materials are tested and documented. A piece of furniture, which lives up to the three areas of requirements of Møbelfakta, has undergone
extensive testing, is produced according to ethical guidelines and has been approved according to environmental requirements. Møbelfakta is an
guarantee of high quality products.
Almost all of Fora Forms collection is Møbelfakta approved.
Fora Form are ISO 9001 quality management,ISO 14001 environmental management and ISO 45001 occupational health and safety management
certified.
Sustainability is important for Fora Form.
Transportation of Senso products from the production site to the customer is stipulated to be an average of 1050km
waR slairetam tropsnarT gnirutcafunaM tropsnarT ylbmessA e​sU ecnanetniaM riapeR tnemecalpeR tnemhsibrufeR lanoitarepO ygrene esu lanoitarepO esu retaw -eD noitcurtsnoc noitilomed tropsnarT etsaW gnissecorp lasopsiD -yrevoceR-esueR laitnetop-gnilcyceR
5 / 12
LCA: Scenarios and additional technical information
The following information describe the scenarios in the different modules of the EPD.
Capacity utilisation Value
Transport from production place to user (A4) Distance (km) Fuel/Energy Consumption Unit
(incl. return) % (Liter/tonne)
Truck, 16-32 tonnes, EURO 6 (km) 36,7 % 1050 0,043 l/tkm 45,15
Assembly (A5) Unit Value
Waste, packaging, cardboard, 100 % recycled, to
kg 2,00
average treatment (kg)
Maintenance (B2) Unit Value
Water, tap water (kg) kg/DU 1,00
Capacity utilisation Value
Transport to waste processing (C2) Distance (km) Fuel/Energy Consumption Unit
(incl. return) % (Liter/tonne)
Truck, 7.5-16 tonnes, HVO, EURO 6 (kgkm) 35,4 % 85 0,056 l/tkm 4,76
Waste processing (C3) Unit Value
Waste treatment per kg Plastics, Mixture,
kg 0,15
municipal incineration with fly ash extraction (kg)
Waste treatment per kg Polyoxymethylene (POM),
kg 0,10
incineration with fly ash extraction (kg) - CH - C3
Waste treatment per kg Polyurethane (PU),
kg 6,21
incineration (kg)
Waste treatment per kg Scrap aluminium,
kg 2,38
incineration with fly ash extraction (kg)
Waste treatment per kg Scrap steel, incineration
kg 13,53
with fly ash extraction (kg)
Waste treatment per kg Textile, incineration with
kg 3,99
fly ash extraction (kg)
Waste treatment per kg Wood, incineration with
kg 0,50
fly ash extraction (kg)
Waste, materials to recycling (kg) kg 4,84
Disposal (C4) Unit Value
Landfilling of ashes and residues from
kg 2,13
incineration of Scrap aluminium (kg)
Landfilling of ashes and residues from
kg 8,94
incineration of Scrap steel (kg)
Landfilling of ashes from incineration of Plastics,
Mixture, municipal incineration with fly ash
kg 0,01
extraction, process per kg ashes and residues - C4
(kg)
Landfilling of ashes from incineration of
Polyoxymethylene (POM), process per kg ashes kg 0,00
and residues (kg) - CH - C4
Landfilling of ashes from incineration of
Polyurethane (PU), process per kg ashes and kg 0,24
residues - C4 (kg)
Landfilling of ashes from incineration of Textile,
kg 0,20
soiled, process per kg ashes and residues (kg)
Landfilling of ashes from incineration of Wood,
kg 0,01
process per kg ashes and residues (kg)
Benefits and loads beyond the system
Unit Value
boundaries (D)
Substitution of electricity, in Norway (MJ) MJ 13,03
Substitution of primary aluminium with net scrap
kg 0,12
(kg)
Substitution of primary steel with net scrap (kg) kg 3,67
Substitution of thermal energy, district heating, in
MJ 197,10
Norway (MJ)
6 / 12
LCA: Results
The LCA results are presented below for the declared unit defined on page 2 of the EPD document.
Environmental impact
Indicator Unit A1-A3 A4 A5 B1 B2 C1 C2 C3 C4 D
GWP-total
kg CO2 -
3,47E+02 4,61E+00 3,43E+00 0 3,46E-04 0 1,20E-01 2,41E+01 1,40E-01 -6,35E+00
eq
GWP-fossil
kg CO2 -
2,13E+02 4,61E+00 3,24E-02 0 3,43E-04 0 1,20E-01 1,74E+01 1,40E-01 -6,28E+00
eq
GWP-biogenic
kg CO2 -
1,15E+02 1,91E-03 3,40E+00 0 2,16E-06 0 2,21E-04 6,67E+00 1,25E-04 -9,63E-03
eq
GWP-luluc
kg CO2 -
1,81E+01 1,64E-03 1,07E-05 0 5,59E-07 0 2,18E-04 1,23E-04 3,96E-05 -6,20E-02
eq
kg
ODP CFC11 - 1,09E-05 1,04E-06 6,83E-09 0 3,00E-11 0 2,05E-08 9,42E-08 3,97E-08 -8,32E-02
eq
mol H+
AP 5,14E+00 1,32E-02 1,53E-04 0 2,00E-06 0 8,24E-04 1,58E-02 9,26E-04 -3,69E-02
-eq
EP-FreshWater kg P -eq 5,12E-02 3,68E-05 2,66E-07 0 2,74E-08 0 4,83E-06 7,98E-06 1,45E-06 -3,93E-04
EP-Marine kg N -eq 8,76E-01 2,62E-03 5,07E-05 0 3,18E-07 0 2,04E-04 8,71E-03 3,28E-04 -8,17E-03
mol N -
EP-Terrestial 2,00E+01 2,93E-02 5,49E-04 0 3,70E-06 0 2,30E-03 8,38E-02 3,63E-03 -8,61E-02
eq
kg
POCP NMVOC 7,27E-01 1,12E-02 1,58E-04 0 1,16E-06 0 8,36E-04 2,00E-02 1,04E-03 -3,29E-02
-eq
ADP- kg Sb-
9,35E-03 1,27E-04 7,87E-07 0 9,59E-09 0 1,82E-05 3,64E-06 2,21E-06 -7,94E-05
minerals&metals1 eq
ADP-fossil1 MJ 2,36E+03 6,97E+01 4,53E-01 0 5,86E-03 0 2,45E+00 7,89E+00 2,96E+00 -6,43E+01
WDP1 m3 7,80E+03 6,74E+01 5,74E-01 0 1,04E-01 0 8,85E+00 2,20E+01 7,15E+00 -6,23E+02
GWP-total = Global Warming Potential total; GWP-fossil = Global Warming Potential fossil fuels; GWP-biogenic = Global Warming Potential biogenic; GWP-luluc =
Global Warming Potential land use and land use change; ODP = Depletion potential of the stratospheric ozone layer; AP = Acidification potential, Accumulated
Exceedance; EP-freshwater = Eutrophication potential, fraction of nutrients reaching freshwater end compartment: EP-marine = Eutrophication potential, fraction of
nutrients reaching marine end compartment; EP-terrestrial = Eutrophication potential, Accumulated Exceedance; POCP = Formation potential of tropospheric ozone;
ADP-minerals&metals = Abiotic depletion potential for non-fossil resources; ADP-fossil = Abiotic depletion for fossil resources potential; WDP = Water (user)
deprivation potential, deprivation-weighted water consumption
"Reading example: 9,0 E-03 = 9,0*10-3 = 0,009"
*INA Indicator Not Assessed
1. The results of this environmental impact indicator shall be used with care as the uncertainties on these results are high or as there is limited experienced with the
indicator
Remarks to environmental impacts
The product meets the requirements for low emissions.
7 / 12
Additional environmental impact indicators
Indicator Unit A1-A3 A4 A5 B1 B2 C1 C2 C3 C4 D
PM Disease incidence 4,03E-05 2,82E-07 2,26E-09 0 1,70E-11 0 2,28E-08 7,87E-08 1,66E-08 -9,83E-07
IRP2 kgBq U235 -eq 6,33E+00 3,04E-01 1,94E-03 0 4,05E-05 0 8,05E-03 1,30E-02 1,20E-02 -1,51E-01
ETP-fw1 CTUe 9,57E+03 5,16E+01 6,04E-01 0 6,35E-03 0 3,83E+00 6,12E+01 1,94E+00 -3,31E+02
HTP-c1 CTUh 4,74E-07 0,00E+00 1,80E-11 0 1,00E-12 0 0,00E+00 1,89E-09 7,30E-11 -2,38E-08
HTP-nc1 CTUh 7,88E-06 5,64E-08 7,58E-10 0 2,10E-11 0 6,85E-09 5,79E-08 2,10E-09 3,05E-07
SQP1 dimensionless -1,61E+05 4,87E+01 3,04E-01 0 1,64E-03 0 3,77E+00 9,60E-01 6,53E+00 -1,12E+02
PM = Particulate Matter emissions; IRP = Ionizing radiation – human health; ETP-fw = Eco toxicity – freshwater; HTP-c = Human toxicity – cancer effects; HTP-nc =
Human toxicity – non cancer effects; SQP = Soil Quality (dimensionless)
"Reading example: 9,0 E-03 = 9,0*10-3 = 0,009"
*INA Indicator Not Assessed
1. The results of this environmental impact indicator shall be used with care as the uncertainties on these results are high or as there is limited experienced with the
indicator
2. This impact category deals mainly with the eventual impact of low dose ionizing radiation on human health of the nuclear fuel cycle. It does not consider effects due
to possible nuclear accidents, occupational exposure nor due to radioactive waste disposal in underground facilities. Potential ionizing radiation from the soil, from
radon and from some construction materials is also not measured by this indicator.
8 / 12
Resource use
Indicator Unit A1-A3 A4 A5 B1 B2 C1 C2 C3 C4 D
PERE MJ 6,48E+02 9,97E-01 7,45E-03 0 7,95E-04 0 1,30E-01 2,31E-01 6,11E-02 -1,09E+02
PERM MJ 1,06E+02 0,00E+00 -1,17E+01 0 0,00E+00 0 0,00E+00 -9,48E+01 0,00E+00 0,00E+00
PERT MJ 7,55E+02 9,97E-01 -1,17E+01 0 7,95E-04 0 1,30E-01 -9,45E+01 6,11E-02 -1,09E+02
PENRE MJ 2,28E+03 6,97E+01 4,53E-01 0 5,87E-03 0 2,45E+00 7,95E+00 2,96E+00 -6,43E+01
PENRM MJ 1,98E+02 0,00E+00 0,00E+00 0 0,00E+00 0 0,00E+00 -1,98E+02 0,00E+00 0,00E+00
PENRT MJ 2,48E+03 6,97E+01 4,53E-01 0 5,87E-03 0 2,45E+00 -1,90E+02 2,96E+00 -6,43E+01
SM kg 5,90E+00 0,00E+00 0,00E+00 0 0,00E+00 0 0,00E+00 0,00E+00 0,00E+00 0,00E+00
RSF MJ 4,25E-01 3,57E-02 2,47E-04 0 6,39E-05 0 4,32E-03 5,39E-03 1,60E-03 1,26E-01
NRSF MJ 3,15E+00 1,28E-01 1,02E-03 0 6,30E-05 0 1,52E-02 0,00E+00 8,68E-02 -1,73E+00
FW m3 2,80E+00 7,45E-03 2,14E-04 0 1,01E-03 0 1,08E-03 2,67E-02 2,67E-03 -1,58E-01
PERE = Use of renewable primary energy excluding renewable primary energy resources used as raw materials; PERM = Use of renewable primary energy resources used
as raw materials; PERT = Total use of renewable primary energy resources; PENRE = Use of non renewable primary energy excluding non-renewable primary energy
resources used as raw materials; PENRM = Use of non renewable primary energy resources used as raw materials; PENRT = Total use of non renewable primary energy
resources; SM = Use of secondary materials; RSF = Use of renewable secondary fuels; NRSF = Use of non-renewable secondary fuels; FW = Net use of fresh water
"Reading example: 9,0 E-03 = 9,0*10-3 = 0,009"
*INA Indicator Not Assessed
9 / 12
End of life - Waste
Indicator Unit A1-A3 A4 A5 B1 B2 C1 C2 C3 C4 D
HWD kg 1,12E+00 3,59E-03 0,00E+00 0 1,11E-06 0 3,68E-04 0,00E+00 1,12E+01 -1,71E-02
NHWD kg 3,91E+01 3,39E+00 2,00E+00 0 7,12E-05 0 2,94E-01 0,00E+00 2,49E-01 -2,36E+00
RWD kg 6,04E-03 4,74E-04 0,00E+00 0 3,43E-08 0 9,44E-06 0,00E+00 1,82E-05 -1,31E-04
HWD = Hazardous waste disposed; NHWD = Non-hazardous waste disposed; RWD = Radioactive waste disposed
"Reading example: 9,0 E-03 = 9,0*10-3 = 0,009"
*INA Indicator Not Assessed
End of life - Output flow
Indicator Unit A1-A3 A4 A5 B1 B2 C1 C2 C3 C4 D
CRU kg 0,00E+00 0,00E+00 0,00E+00 0 0,00E+00 0 0,00E+00 0,00E+00 0,00E+00 0,00E+00
MFR kg 0,00E+00 0,00E+00 1,86E+00 0 0,00E+00 0 0,00E+00 4,84E+00 0,00E+00 0,00E+00
MER kg 0,00E+00 0,00E+00 2,72E-06 0 0,00E+00 0 0,00E+00 2,69E+01 0,00E+00 0,00E+00
EEE MJ 0,00E+00 0,00E+00 1,14E-01 0 0,00E+00 0 0,00E+00 1,26E+01 0,00E+00 0,00E+00
EET MJ 0,00E+00 0,00E+00 1,73E+00 0 0,00E+00 0 0,00E+00 1,91E+02 0,00E+00 0,00E+00
CRU = Components for re-use; MFR = Materials for recycling; MER = Materials for energy recovery; EEE = Exported energy electrical; EET = Exported energy thermal
"Reading example: 9,0 E-03 = 9,0*10-3 = 0,009"
*INA Indicator Not Assessed
Biogenic Carbon Content
Indicator Unit At the factory gate
Biogenic carbon content in product kg C 2,27E-01
Biogenic carbon content in accompanying packaging kg C 9,26E-01
Note: 1 kg biogenic carbon is equivalent to 44/12 kg CO2
10 / 12
Additional requirements
Greenhouse gas emissions from the use of electricity in the manufacturing phase
National production mix from import, low voltage (production of transmission lines, in addition to direct emissions and losses in grid) of applied
electricity for the manufacturing process (A3).
Electricity mix Source Amount Unit
Electricity, European average (kWh) ecoinvent 3.6 428,03 g CO2-eq/kWh
Dangerous substances
The product contains no substances given by the REACH Candidate list.
Indoor environment
Our furniture doesn't contain any substanses that effect indoor clima
Additional Environmental Information
Key Environmental Indicators
Key environmental indicators Unit A1-A3 A4 A1-C4 A1-D
GWPtotal kg CO2 -eq 346,78 4,61 379,14 372,79
Total energy consumption MJ 2936,83 70,82 3022,02 2847,39
Amount of recycled materials % 20,43
Additional environmental impact indicators required in NPCR Part A for construction products
Indicator Unit A1-A3 A4 A5 B1 B2 C1 C2 C3 C4 D
GWPIOBC kg CO2 -eq 3,43E+02 4,61E+00 3,24E-02 0 3,46E-04 0 1,20E-01 2,39E+01 1,53E-01 -8,29E+00
GWP-IOBC: Global warming potential calculated according to the principle of instantaneous oxidation. In order to increase the transparency of biogenic carbon
contribution to climate impact, the indicator GWP-IOBC is required as it declares climate impacts calculated according to the principle of instantaneous oxidation.
GWP-IOBC is also referred to as GWP-GHG in context to Swedish public procurement legislation.
Variants and Options
Key environmental indicators (A1-A3) for variants of this EPD
Variants Weight (kg) GWPtotal (kg CO2 -eq) Total energy consumption (MJ) Amount of recycled materials (%)
Senso 3 seat sofa - low backrest/corner 52,03 815,82 6209,78 11,73
Senso 3 seat sofa - high backrest/corner 76,16 932,42 8034,71 8,71
11 / 12
Bibliography
ISO 14025:2010 Environmental labels and declarations - Type III environmental declarations - Principles and procedures.
ISO 14044:2006 Environmental management - Life cycle assessment - Requirements and guidelines.
EN 15804:2012+A2:2019 Environmental product declaration - Core rules for the product category of construction products.
ISO 21930:2017 Sustainability in buildings and civil engineering works - Core rules for environmental product declarations of construction
products.
ecoinvent v3, Allocation, cut-off by classification, Swiss Centre of Life Cycle Inventories.
Iversen et al., (2021) eEPD v2021.09 Background information for EPD generator tool system verification, LCA.no Report number: 07.21
Ruud et al., (2023) EPD generator for NPCR026 Part B for Furniture - Background information for EPD generator application and LCA data,
LCA.no report number 01.23
NPCR Part A: Construction products and services. Ver. 2.0. March 2021, EPD-Norge.
NPCR 026 Part B for Furniture. Ver. 2.0 March 2022, EPD-Norge.
Program operator and publisher Phone: +47 977 22 020
The Norwegian EPD Foundation e-mail: post@epd-norge.no
Post Box 5250 Majorstuen, 0303 Oslo, Norway web: www.epd-norge.no
Owner of the declaration: Phone: +47 700 46 000
Fora Form AS e-mail: info@foraform.com
Mosflatevegen, 6154 Ørsta web: www.foraform.no
Author of the Life Cycle Assessment Phone: +47 916 50 916
LCA.no AS e-mail: post@lca.no
Dokka 6A, 1671 web: www.lca.no
Developer of EPD generator Phone: +47 916 50 916
LCA.no AS e-mail: post@lca.no
Dokka 6B,1671 Kråkerøy web: www.lca.no
ECO Platform web: www.eco-platform.org
ECO Portal web: ECO Portal
12 / 12
